@prefix owl: <http://www.w3.org/2002/07/owl#> .
@prefix rdfs: <http://www.w3.org/2000/01/rdf-schema#> .
@prefix dc: <http://purl.org/dc/terms/> .
@prefix xsd: <http://www.w3.org/2001/XMLSchema#> .
@prefix ns0: <https://schema.org/> .
@prefix ns1: <http://www.w3.org/2003/06/sw-vocab-status/ns#> .
@prefix skos: <http://www.w3.org/2004/02/skos/core#> .
@prefix ns2: <http://purl.org/dc/dcam/> .
@prefix odrl: <http://www.w3.org/ns/odrl/2/> .
@prefix ns3: <http://purl.org/vocab/vann/> .
@prefix cc: <http://creativecommons.org/ns#> .
@prefix bibo: <http://purl.org/ontology/bibo/> .
@prefix ns4: <http://www.w3.org/ns/dx/prof/> .
@prefix foaf: <http://xmlns.com/foaf/0.1/> .
@prefix schema: <http://schema.org/> .
@prefix org: <http://www.w3.org/ns/org#> .
@prefix rdf: <http://www.w3.org/1999/02/22-rdf-syntax-ns#> .
@prefix dcat: <http://www.w3.org/ns/dcat#> .
@prefix vcard: <http://www.w3.org/2006/vcard/ns#> .
@prefix ns5: <http://purl.org/spar/scoro/> .

<https://w3id.org/dpv/owl#AutomatedDecisionMaking>
  a owl:Class ;
  rdfs:subClassOf <https://w3id.org/dpv/owl#DecisionMaking> ;
  dc:contributor _:genid1, _:genid2 ;
  dc:created "2020-11-04"^^xsd:date ;
  dc:modified "2022-09-07"^^xsd:date ;
  dc:source [
    a <https://schema.org/WebPage> ;
    ns0:name "GDPR Art.4-2" ;
    ns0:url "https://eur-lex.europa.eu/eli/reg/2016/679/art_4/par_2/oj"
  ] ;
  ns1:term_status "accepted"@en ;
  skos:definition "Processing that involves automated decision making"@en ;
  skos:prefLabel "Automated Decision Making"@en ;
  skos:scopeNote "Automated decision making can be defined as “the ability to make decisions by technological means without human involvement.” (“Guidelines on Automated individual decision-making and Profiling for the purposes of Regulation 2016/679 (wp251rev.01)”, 2018, p. 8)"@en ;
  owl:sameAs <https://w3id.org/dpv#AutomatedDecisionMaking>, <https://w3id.org/dpv/dpv-owl#AutomatedDecisionMaking> .

<https://w3id.org/dpv/owl#hasDataSubjectScale>
  a owl:ObjectProperty ;
  rdfs:subPropertyOf <https://w3id.org/dpv/owl#hasScale> ;
  ns2:rangeIncludes <https://w3id.org/dpv/owl#DataSubjectScale> ;
  dc:contributor _:genid1 ;
  dc:created "2022-06-22"^^xsd:date ;
  ns1:term_status "accepted"@en ;
  skos:definition "Indicates the scale of data subjects"@en ;
  skos:prefLabel "has data subject scale"@en ;
  ns0:rangeIncludes <https://w3id.org/dpv/owl#DataSubjectScale> ;
  owl:sameAs <https://w3id.org/dpv#hasDataSubjectScale>, <https://w3id.org/dpv/dpv-owl#hasDataSubjectScale> .

<https://w3id.org/dpv/owl#hasRule>
  a owl:ObjectProperty ;
  ns2:domainIncludes <https://w3id.org/dpv/owl#Context> ;
  ns2:rangeIncludes <https://w3id.org/dpv/owl#Rule> ;
  dc:contributor _:genid4, _:genid5, _:genid1, _:genid6 ;
  dc:created "2022-10-19"^^xsd:date ;
  ns1:term_status "accepted"@en ;
  skos:definition "Specifying applicability or inclusion of a rule within specified context"@en ;
  skos:prefLabel "has rule"@en ;
  ns0:domainIncludes <https://w3id.org/dpv/owl#Context> ;
  ns0:rangeIncludes <https://w3id.org/dpv/owl#Rule> ;
  owl:sameAs <https://w3id.org/dpv#hasRule>, <https://w3id.org/dpv/dpv-owl#hasRule> .

<https://w3id.org/dpv/owl#HashMessageAuthenticationCode>
  a owl:Class, owl:NamedIndividual, <https://w3id.org/dpv/owl#TechnicalMeasure> ;
  rdfs:subClassOf <https://w3id.org/dpv/owl#CryptographicAuthentication> ;
  dc:contributor _:genid1 ;
  dc:created "2022-08-17"^^xsd:date ;
  dc:source [
    a ns0:WebPage ;
    ns0:name "ENISA 5G Cybersecurity Standards" ;
    ns0:url "https://www.enisa.europa.eu/publications/5g-cybersecurity-standards"
  ] ;
  ns1:term_status "accepted"@en ;
  skos:definition "Use of HMAC where message authentication code (MAC) utilise a cryptographic hash function and a secret cryptographic key"@en ;
  skos:prefLabel "Hash-based Message Authentication Code (HMAC)"@en ;
  owl:sameAs <https://w3id.org/dpv#HashMessageAuthenticationCode>, <https://w3id.org/dpv/dpv-owl#HashMessageAuthenticationCode> .

odrl:#constraintLeftOperandCommon
  a owl:NamedIndividual, skos:Collection ;
  skos:member odrl:absolutePosition, odrl:absoluteSize, odrl:absoluteSpatialPosition, odrl:absoluteTemporalPosition, odrl:count, odrl:dateTime, odrl:delayPeriod, odrl:deliveryChannel, odrl:elapsedTime, odrl:event, odrl:fileFormat, odrl:industry, odrl:language, odrl:media, odrl:meteredTime, odrl:payAmount, odrl:percentage, odrl:product, odrl:purpose, odrl:recipient, odrl:relativePosition, odrl:relativeSize, odrl:relativeSpatialPosition, odrl:relativeTemporalPosition, odrl:resolution, odrl:spatial, odrl:spatialCoordinates, odrl:systemDevice, odrl:timeInterval, odrl:unitOfCount, odrl:version, odrl:virtualLocation ;
  skos:prefLabel "Constraint Left Operands"@en ;
  skos:scopeNote "ODRL Common Vocabulary Terms"@en .

<https://w3id.org/dpv/owl#CybersecurityTraining>
  a owl:Class, owl:NamedIndividual, <https://w3id.org/dpv/owl#OrganisationalMeasure> ;
  rdfs:subClassOf <https://w3id.org/dpv/owl#StaffTraining> ;
  dc:contributor _:genid1 ;
  dc:created "2022-08-17"^^xsd:date ;
  dc:source [
    a ns0:WebPage ;
    ns0:name "ENISA Reference Incident Classification Taxonomy 2018" ;
    ns0:url "https://www.enisa.europa.eu/publications/reference-incident-classification-taxonomy/"
  ] ;
  ns1:term_status "accepted"@en ;
  skos:definition "Training methods related to cybersecurity"@en ;
  skos:prefLabel "Cybersecurity Training"@en ;
  owl:sameAs <https://w3id.org/dpv#CybersecurityTraining>, <https://w3id.org/dpv/dpv-owl#CybersecurityTraining> .

<https://w3id.org/dpv/owl#EncryptionInTransfer>
  a owl:Class, owl:NamedIndividual, <https://w3id.org/dpv/owl#TechnicalMeasure> ;
  rdfs:subClassOf <https://w3id.org/dpv/owl#Encryption> ;
  dc:contributor _:genid9, _:genid10, _:genid1, _:genid11 ;
  dc:created "2019-04-05"^^xsd:date ;
  ns1:term_status "accepted"@en ;
  skos:definition "Encryption of data in transit e.g. when being transferred from one location to another, including sharing"@en ;
  skos:prefLabel "Encryption in Transfer"@en ;
  owl:sameAs <https://w3id.org/dpv#EncryptionInTransfer>, <https://w3id.org/dpv/dpv-owl#EncryptionInTransfer> .

<https://w3id.org/dpv/owl#SellProductsToDataSubject>
  a owl:Class, owl:NamedIndividual, <https://w3id.org/dpv/owl#Purpose> ;
  rdfs:subClassOf <https://w3id.org/dpv/owl#SellProducts> ;
  dc:contributor _:genid13, _:genid14, _:genid1, _:genid15, _:genid16, _:genid11 ;
  dc:created "2019-04-05"^^xsd:date ;
  ns1:term_status "accepted"@en ;
  skos:definition "Purposes associated with selling products or services to the user, consumer, or data subjects"@en ;
  skos:prefLabel "Sell Products to Data Subject"@en ;
  skos:scopeNote "Sell Products here refers to processing necessary to provide and complete a sale to customers. It should not be confused with providing services with a cost based on an established agreement."@en ;
  owl:sameAs <https://w3id.org/dpv#SellProductsToDataSubject>, <https://w3id.org/dpv/dpv-owl#SellProductsToDataSubject> .

<https://w3id.org/dpv/owl#ConsentInvalidated>
  a owl:Class, owl:NamedIndividual, <https://w3id.org/dpv/owl#ConsentStatus> ;
  rdfs:subClassOf <https://w3id.org/dpv/owl#ConsentStatusInvalidForProcessing> ;
  dc:contributor _:genid4, _:genid1, _:genid17, _:genid6 ;
  dc:created "2022-06-22"^^xsd:date ;
  dc:source [
    a ns0:WebPage ;
    ns0:name "GConsent" ;
    ns0:url "https://w3id.org/GConsent"
  ] ;
  ns1:term_status "accepted"@en ;
  skos:definition "The state where consent has been deemed to be invalid"@en ;
  skos:prefLabel "Consent Invalidated"@en ;
  skos:scopeNote "An example of this state is where an investigating authority or a court finds the collected consent did not meet requirements, and 'invalidates' both prior and future uses of it to carry out processing"@en ;
  owl:sameAs <https://w3id.org/dpv#ConsentInvalidated>, <https://w3id.org/dpv/dpv-owl#ConsentInvalidated> .

<https://w3id.org/dpv/owl#Status>
  a owl:Class ;
  rdfs:subClassOf <https://w3id.org/dpv/owl#Context> ;
  dc:contributor _:genid1 ;
  dc:created "2022-05-18"^^xsd:date ;
  ns1:term_status "accepted"@en ;
  skos:definition "The status or state of something"@en ;
  skos:prefLabel "Status"@en ;
  owl:sameAs <https://w3id.org/dpv#Status>, <https://w3id.org/dpv/dpv-owl#Status> .

odrl:grantUse
  a owl:NamedIndividual, skos:Concept, odrl:Action ;
  odrl:includedIn odrl:use ;
  rdfs:isDefinedBy odrl: ;
  rdfs:label "Grant Use"@en ;
  skos:definition "To grant the use of the Asset to third parties."@en ;
  skos:note "This action enables the assignee to create policies for the use of the Asset for third parties. The nextPolicy is recommended to be agreed with the third party. Use of temporal constraints is recommended."@en ;
  skos:scopeNote "Non-Normative"@en .

<https://w3id.org/dpv/owl#GuardianOfDataSubject>
  a owl:Class, owl:NamedIndividual, <https://w3id.org/dpv/owl#HumanSubject> ;
  rdfs:subClassOf <https://w3id.org/dpv/owl#GuardianOfHuman> ;
  dc:contributor _:genid4 ;
  dc:created "2022-08-03"^^xsd:date ;
  dc:modified "2024-12-17"^^xsd:date ;
  ns1:term_status "modified"@en ;
  skos:definition "Guardian(s) of data subjects such as children"@en ;
  skos:prefLabel "Guardian(s) of Data Subject"@en ;
  owl:sameAs <https://w3id.org/dpv#GuardianOfDataSubject>, <https://w3id.org/dpv/dpv-owl#GuardianOfDataSubject> .

<https://w3id.org/dpv/owl#LocalityScale>
  a owl:Class, owl:NamedIndividual, <https://w3id.org/dpv/owl#GeographicCoverage> ;
  rdfs:subClassOf <https://w3id.org/dpv/owl#GeographicCoverage> ;
  dc:contributor _:genid1 ;
  dc:created "2022-06-15"^^xsd:date ;
  ns1:term_status "accepted"@en ;
  skos:definition "Geographic coverage spanning a specific locality"@en ;
  skos:prefLabel "Locality Scale"@en ;
  skos:scopeNote "For example, geographic scale of a city or an area within a city"@en ;
  owl:sameAs <https://w3id.org/dpv#LocalityScale>, <https://w3id.org/dpv/dpv-owl#LocalityScale> .

odrl:consentedParty
  a owl:ObjectProperty, owl:NamedIndividual, skos:Concept ;
  rdfs:subPropertyOf odrl:function ;
  rdfs:isDefinedBy odrl: ;
  rdfs:label "Consented Party"@en ;
  skos:definition "The Party who obtains the consent."@en ;
  skos:note "Maybe specified as part of the obtainConsent action."@en ;
  skos:scopeNote "Non-Normative"@en .

<https://w3id.org/dpv/owl#DataExporter>
  a owl:Class ;
  rdfs:subClassOf <https://w3id.org/dpv/owl#LegalEntity> ;
  dc:contributor _:genid4, _:genid1, _:genid6, _:genid21 ;
  dc:created "2021-09-08"^^xsd:date ;
  dc:source [
    a ns0:WebPage ;
    ns0:name "EDPB Recommendations 01/2020 on Data Transfers" ;
    ns0:url "https://edpb.europa.eu/our-work-tools/our-documents/recommendations/recommendations-012020-measures-supplement-transfer_en"
  ] ;
  ns3:example <https://w3id.org/dpv/examples/owl#E0035> ;
  ns1:term_status "accepted"@en ;
  skos:definition "An entity that 'exports' data where exporting is considered a form of data transfer"@en ;
  skos:prefLabel "Data Exporter"@en ;
  skos:scopeNote "The term 'Data Exporter' is used by the EU-EDPB as the entity that transfer data across borders. While the EDPB refers to the jurisdictional border of EU, the term within DPV can be used to denote any 'export' or transfer or transmission of data and is thus a broader concept than the EDPB's definition."@en ;
  owl:sameAs <https://w3id.org/dpv#DataExporter>, <https://w3id.org/dpv/dpv-owl#DataExporter> .

<https://w3id.org/dpv/owl#DifferentialPrivacy>
  a owl:Class, owl:NamedIndividual, <https://w3id.org/dpv/owl#TechnicalMeasure> ;
  rdfs:subClassOf <https://w3id.org/dpv/owl#CryptographicMethods> ;
  dc:contributor _:genid1 ;
  dc:created "2022-08-17"^^xsd:date ;
  dc:source [
    a ns0:WebPage ;
    ns0:name "ENISA Data Protection Engineering" ;
    ns0:url "https://www.enisa.europa.eu/publications/data-protection-engineering"
  ] ;
  ns1:term_status "accepted"@en ;
  skos:definition "Utilisation of differential privacy where information is shared as patterns or groups to withhold individual elements"@en ;
  skos:prefLabel "Differential Privacy"@en ;
  owl:sameAs <https://w3id.org/dpv#DifferentialPrivacy>, <https://w3id.org/dpv/dpv-owl#DifferentialPrivacy> .

<https://w3id.org/dpv/owl#ContractAmended>
  a owl:Class, owl:NamedIndividual, <https://w3id.org/dpv/owl#ContractPerformanceStatus> ;
  rdfs:subClassOf <https://w3id.org/dpv/owl#ContractPerformanceStatus> ;
  dc:contributor _:genid4, _:genid1, _:genid17 ;
  dc:created "2025-01-09"^^xsd:date ;
  ns1:term_status "accepted"@en ;
  skos:definition "Status representing contract that has been fully executed and whose terms have been amended through mutual agreement or other means such that the contract is still required to be performed"@en ;
  skos:prefLabel "Contract Amended"@en ;
  owl:sameAs <https://w3id.org/dpv#ContractAmended>, <https://w3id.org/dpv/dpv-owl#ContractAmended> .

<https://w3id.org/dpv/owl#hasImpact>
  a owl:ObjectProperty ;
  rdfs:subPropertyOf <https://w3id.org/dpv/owl#hasConsequence> ;
  ns2:rangeIncludes <https://w3id.org/dpv/owl#Impact> ;
  dc:contributor _:genid4, _:genid5, _:genid1, _:genid17, _:genid15 ;
  dc:created "2022-05-18"^^xsd:date ;
  ns3:example <https://w3id.org/dpv/examples/owl#E0068>, <https://w3id.org/dpv/examples/owl#E0069>, <https://w3id.org/dpv/examples/owl#E0088> ;
  ns1:term_status "accepted"@en ;
  skos:definition "Indicates impact(s) possible or arising as consequences from specified concept"@en ;
  skos:prefLabel "has impact"@en ;
  ns0:rangeIncludes <https://w3id.org/dpv/owl#Impact> ;
  owl:sameAs <https://w3id.org/dpv#hasImpact>, <https://w3id.org/dpv/dpv-owl#hasImpact> .

<https://w3id.org/dpv/owl#Optional>
  a owl:Class, owl:NamedIndividual, <https://w3id.org/dpv/owl#Necessity> ;
  rdfs:subClassOf <https://w3id.org/dpv/owl#Necessity> ;
  dc:contributor _:genid4, _:genid5, _:genid1, _:genid17, _:genid6 ;
  dc:created "2022-02-14"^^xsd:date ;
  ns1:term_status "accepted"@en ;
  skos:definition "Indication of 'optional' or 'voluntary'"@en ;
  skos:prefLabel "Optional"@en ;
  owl:sameAs <https://w3id.org/dpv#Optional>, <https://w3id.org/dpv/dpv-owl#Optional> .

<https://w3id.org/dpv/owl#DataProcessingPolicy>
  a owl:Class, owl:NamedIndividual, <https://w3id.org/dpv/owl#OrganisationalMeasure> ;
  rdfs:subClassOf <https://w3id.org/dpv/owl#Policy> ;
  dc:contributor _:genid1 ;
  dc:created "2024-04-14"^^xsd:date ;
  ns1:term_status "accepted"@en ;
  skos:definition "Policy regarding data processing activities"@en ;
  skos:prefLabel "Data Processing Policy"@en ;
  skos:scopeNote "This only refers to the policy or plan or procedure describing how the data processing should be conducted. To represent the granular details, see further concepts e.g. dpv:DataStoragePolicy to describe policy regarding storage, or dpv:DataStorageCondition to represent information within the policy for how information should be stored"@en ;
  owl:sameAs <https://w3id.org/dpv#DataProcessingPolicy>, <https://w3id.org/dpv/dpv-owl#DataProcessingPolicy> .

<https://w3id.org/dpv/owl#hasPersonalDataHandling>
  a owl:ObjectProperty ;
  ns2:rangeIncludes <https://w3id.org/dpv/owl#PersonalDataHandling> ;
  dc:contributor _:genid4, _:genid1 ;
  dc:created "2022-01-19"^^xsd:date ;
  ns1:term_status "accepted"@en ;
  skos:definition "Indicates association with Personal Data Handling"@en ;
  skos:prefLabel "has personal data handling"@en ;
  ns0:rangeIncludes <https://w3id.org/dpv/owl#PersonalDataHandling> ;
  owl:sameAs <https://w3id.org/dpv#hasPersonalDataHandling>, <https://w3id.org/dpv/dpv-owl#hasPersonalDataHandling> .

<https://w3id.org/dpv/owl#DataSubjectRightsManagement>
  a owl:Class, owl:NamedIndividual, <https://w3id.org/dpv/owl#OrganisationalMeasure> ;
  rdfs:subClassOf <https://w3id.org/dpv/owl#RightsManagement> ;
  dc:contributor _:genid4, _:genid5, _:genid1 ;
  dc:created "2024-04-14"^^xsd:date ;
  dc:source "DGA 12.m"@en ;
  ns1:term_status "accepted"@en ;
  skos:definition "Methods to provide, implement, and exercise data subjects' rights"@en ;
  skos:prefLabel "Data Subject Rights Management"@en ;
  skos:scopeNote "This concept only concerns the organisational management of rights, and does not represent the rights themselves - especially where such 'rights' are legally recognised or defined for the data subject or individual. The concept dpv:DataSubjectRight is provided to represent such legal rights."@en ;
  owl:sameAs <https://w3id.org/dpv#DataSubjectRightsManagement>, <https://w3id.org/dpv/dpv-owl#DataSubjectRightsManagement> .

<https://w3id.org/dpv/owl#NotificationNotNeeded>
  a owl:Class, owl:NamedIndividual, <https://w3id.org/dpv/owl#NotificationStatus> ;
  rdfs:subClassOf <https://w3id.org/dpv/owl#NotificationStatus> ;
  dc:contributor _:genid1 ;
  dc:created "2024-05-19"^^xsd:date ;
  ns1:term_status "accepted"@en ;
  skos:definition "Status indicating notification(s) are not needed"@en ;
  skos:prefLabel "Notification Not Needed"@en ;
  owl:sameAs <https://w3id.org/dpv#NotificationNotNeeded>, <https://w3id.org/dpv/dpv-owl#NotificationNotNeeded> .

<https://w3id.org/dpv/owl#EntityInformedStatus>
  a owl:Class ;
  rdfs:subClassOf <https://w3id.org/dpv/owl#Status> ;
  dc:contributor _:genid4, _:genid1, _:genid25, _:genid6 ;
  dc:created "2024-05-10"^^xsd:date ;
  ns1:term_status "accepted"@en ;
  skos:definition "Status indicating whether an entity is informed or uninformed about specified context"@en ;
  skos:prefLabel "Entity Informed Status"@en ;
  owl:sameAs <https://w3id.org/dpv#EntityInformedStatus>, <https://w3id.org/dpv/dpv-owl#EntityInformedStatus> .

<https://w3id.org/dpv/owl#RightNotice>
  a owl:Class, owl:NamedIndividual, <https://w3id.org/dpv/owl#OrganisationalMeasure> ;
  rdfs:subClassOf <https://w3id.org/dpv/owl#Notice> ;
  dc:contributor _:genid1 ;
  dc:created "2024-06-16"^^xsd:date ;
  ns1:term_status "accepted"@en ;
  skos:definition "Information associated with rights, such as which rights exist, when and where they are applicable, and other relevant information"@en ;
  skos:prefLabel "Right Notice"@en ;
  skos:scopeNote "This concept also covers information about rights exercise, with dpv:RightExerciseNotice specifically representing information provided in connection with exercising of rights. Both notices may be needed, e.g. RightNotice for providing information about existence and exercise of rights, and RightExerciseNotice for providing additional information specifically about exercise of rights - such as to request more information or provide updates on an exercised rights request"@en ;
  owl:sameAs <https://w3id.org/dpv#RightNotice>, <https://w3id.org/dpv/dpv-owl#RightNotice> .

<https://w3id.org/dpv/owl#RecruitmentApplicantInformationAuthentication>
  a owl:Class, owl:NamedIndividual, <https://w3id.org/dpv/owl#Purpose> ;
  rdfs:subClassOf <https://w3id.org/dpv/owl#RecruitmentManagement> ;
  dc:created "2024-12-01"^^xsd:date ;
  ns1:term_status "accepted"@en ;
  skos:definition "Purposes associated with authentication and verification of information as part of recruitment"@en ;
  skos:prefLabel "Recruitment Applicant Information Authentication"@en ;
  owl:sameAs <https://w3id.org/dpv#RecruitmentApplicantInformationAuthentication>, <https://w3id.org/dpv/dpv-owl#RecruitmentApplicantInformationAuthentication> .

<https://w3id.org/dpv/owl#C2CContract>
  a owl:Class, owl:NamedIndividual, <https://w3id.org/dpv/owl#LegalBasis> ;
  rdfs:subClassOf <https://w3id.org/dpv/owl#ContractByEntityType> ;
  dc:created "2024-08-27"^^xsd:date ;
  ns1:term_status "accepted"@en ;
  skos:definition "A contract between two consumers"@en ;
  skos:prefLabel "Consumer-to-Consumer Contract"@en ;
  owl:sameAs <https://w3id.org/dpv#C2CContract>, <https://w3id.org/dpv/dpv-owl#C2CContract> .

<https://w3id.org/dpv/owl#PhysicalSurveillance>
  a owl:Class, owl:NamedIndividual, <https://w3id.org/dpv/owl#PhysicalMeasure> ;
  rdfs:subClassOf <https://w3id.org/dpv/owl#PhysicalMeasure> ;
  dc:contributor _:genid1 ;
  dc:created "2024-04-14"^^xsd:date ;
  dc:source "NIST SP 800-171"@en ;
  ns1:term_status "accepted"@en ;
  skos:definition "Physically monitoring areas via surveillance"@en ;
  skos:prefLabel "Physical Surveillance"@en ;
  owl:sameAs <https://w3id.org/dpv#PhysicalSurveillance>, <https://w3id.org/dpv/dpv-owl#PhysicalSurveillance> .

<https://w3id.org/dpv/owl#RefuseConsent>
  a owl:Class ;
  rdfs:subClassOf <https://w3id.org/dpv/owl#ConsentControl> ;
  dc:created "2024-12-17"^^xsd:date ;
  ns1:term_status "accepted"@en ;
  skos:definition "Control for refusing consent"@en ;
  skos:prefLabel "Refuse Consent"@en ;
  skos:scopeNote "Indicates how the controller (with dpv:ObtainConsent) or data subject (with dpv:ProvideConsent) can reaffirm consent e.g. used with dpv:isExercisedAt"@en ;
  owl:sameAs <https://w3id.org/dpv#RefuseConsent>, <https://w3id.org/dpv/dpv-owl#RefuseConsent> .

<https://w3id.org/dpv/owl#HumanResourceManagement>
  a owl:Class, owl:NamedIndividual, <https://w3id.org/dpv/owl#Purpose> ;
  rdfs:subClassOf <https://w3id.org/dpv/owl#Purpose> ;
  dc:contributor _:genid4, _:genid5, _:genid1, _:genid6, _:genid21 ;
  dc:created "2021-09-01"^^xsd:date ;
  dc:source [
    a ns0:WebPage ;
    ns0:name "Belgian DPA ROPA Template" ;
    ns0:url "https://www.privacycommission.be/nl/model-voor-een-register-van-de-verwerkingsactiviteiten"
  ] ;
  ns1:term_status "accepted"@en ;
  skos:definition "Purposes associated with managing humans and 'human resources' within the organisation for effective and efficient operations."@en ;
  skos:prefLabel "Human Resource Management"@en ;
  skos:scopeNote "HR is a broad concept. Its management includes, amongst others - recruiting employees and intermediaries e.g. brokers, independent representatives; payroll administration, remunerations, commissions, and wages; and application of social legislation."@en ;
  owl:sameAs <https://w3id.org/dpv#HumanResourceManagement>, <https://w3id.org/dpv/dpv-owl#HumanResourceManagement> .

<https://w3id.org/dpv/owl#PartiallyCompliant>
  a owl:Class, owl:NamedIndividual, <https://w3id.org/dpv/owl#ComplianceStatus> ;
  rdfs:subClassOf <https://w3id.org/dpv/owl#ComplianceStatus> ;
  dc:contributor _:genid1 ;
  dc:created "2022-05-18"^^xsd:date ;
  ns1:term_status "accepted"@en ;
  skos:definition "State of partially being compliant i.e. only some objectives have been met, and others have not been in violation"@en ;
  skos:prefLabel "Partially Compliant"@en ;
  owl:sameAs <https://w3id.org/dpv#PartiallyCompliant>, <https://w3id.org/dpv/dpv-owl#PartiallyCompliant> .

<https://w3id.org/dpv/owl#CannotCorrectProcessInput>
  a owl:Class, owl:NamedIndividual, <https://w3id.org/dpv/owl#EntityNonPermissiveInvolvement> ;
  rdfs:subClassOf <https://w3id.org/dpv/owl#EntityNonPermissiveInvolvement> ;
  dc:contributor _:genid1, _:genid25, _:genid19 ;
  dc:created "2024-05-11"^^xsd:date ;
  ns1:term_status "accepted"@en ;
  skos:definition "Involvement where entity cannot correct input of specified context"@en ;
  skos:prefLabel "Cannot Correct Process Input"@en ;
  owl:sameAs <https://w3id.org/dpv#CannotCorrectProcessInput>, <https://w3id.org/dpv/dpv-owl#CannotCorrectProcessInput> .

<https://w3id.org/dpv/owl#VendorPayment>
  a owl:Class, owl:NamedIndividual, <https://w3id.org/dpv/owl#Purpose> ;
  rdfs:subClassOf <https://w3id.org/dpv/owl#VendorManagement> ;
  dc:contributor _:genid4, _:genid1, _:genid6, _:genid21 ;
  dc:created "2021-09-01"^^xsd:date ;
  dc:source [
    a ns0:WebPage ;
    ns0:name "Belgian DPA ROPA Template" ;
    ns0:url "https://www.privacycommission.be/nl/model-voor-een-register-van-de-verwerkingsactiviteiten"
  ] ;
  ns1:term_status "accepted"@en ;
  skos:definition "Purposes associated with managing payment of vendors"@en ;
  skos:prefLabel "Vendor Payment"@en ;
  owl:sameAs <https://w3id.org/dpv#VendorPayment>, <https://w3id.org/dpv/dpv-owl#VendorPayment> .

<https://w3id.org/dpv/owl#CannotReverseProcessOutput>
  a owl:Class, owl:NamedIndividual, <https://w3id.org/dpv/owl#EntityNonPermissiveInvolvement> ;
  rdfs:subClassOf <https://w3id.org/dpv/owl#EntityNonPermissiveInvolvement> ;
  dc:contributor _:genid1, _:genid25, _:genid19 ;
  dc:created "2024-05-11"^^xsd:date ;
  ns1:term_status "accepted"@en ;
  skos:definition "Involvement where entity cannot reverse output of specified context"@en ;
  skos:prefLabel "Cannot Reverse Process Output"@en ;
  owl:sameAs <https://w3id.org/dpv#CannotReverseProcessOutput>, <https://w3id.org/dpv/dpv-owl#CannotReverseProcessOutput> .

<https://w3id.org/dpv/owl#VirtualisationSecurity>
  a owl:Class, owl:NamedIndividual, <https://w3id.org/dpv/owl#TechnicalMeasure> ;
  rdfs:subClassOf <https://w3id.org/dpv/owl#SecurityMethod> ;
  dc:contributor _:genid1 ;
  dc:created "2022-08-17"^^xsd:date ;
  dc:source [
    a ns0:WebPage ;
    ns0:name "ENISA Reference Incident Classification Taxonomy 2018" ;
    ns0:url "https://www.enisa.europa.eu/publications/reference-incident-classification-taxonomy/"
  ] ;
  ns1:term_status "accepted"@en ;
  skos:definition "Security implemented at or through virtualised environments"@en ;
  skos:prefLabel "Virtualisation Security"@en ;
  owl:sameAs <https://w3id.org/dpv#VirtualisationSecurity>, <https://w3id.org/dpv/dpv-owl#VirtualisationSecurity> .

<https://w3id.org/dpv/owl#EntityNotInvolved>
  a owl:Class, owl:NamedIndividual, <https://w3id.org/dpv/owl#EntityInvolvementStatus> ;
  rdfs:subClassOf <https://w3id.org/dpv/owl#EntityInvolvementStatus> ;
  dc:contributor _:genid25 ;
  dc:created "2024-12-01"^^xsd:date ;
  ns1:term_status "accepted"@en ;
  skos:definition "Status indicating the entity is not involved"@en ;
  skos:prefLabel "Entity Not Involved"@en ;
  owl:sameAs <https://w3id.org/dpv#EntityNotInvolved>, <https://w3id.org/dpv/dpv-owl#EntityNotInvolved> .

<https://w3id.org/dpv/owl#Disclose>
  a owl:Class, owl:NamedIndividual, <https://w3id.org/dpv/owl#Processing> ;
  rdfs:subClassOf <https://w3id.org/dpv/owl#Processing> ;
  dc:created "2019-05-07"^^xsd:date ;
  dc:source [
    a ns0:WebPage ;
    ns0:name "GDPR Art.4-2" ;
    ns0:url "https://eur-lex.europa.eu/eli/reg/2016/679/art_4/par_2/oj"
  ] ;
  ns1:term_status "accepted"@en ;
  skos:definition "to make data known"@en ;
  skos:prefLabel "Disclose Data"@en ;
  owl:sameAs <https://w3id.org/dpv#Disclose>, <https://w3id.org/dpv/dpv-owl#Disclose> .

<https://w3id.org/dpv/owl#ContractSignedByParty>
  a owl:Class, owl:NamedIndividual, <https://w3id.org/dpv/owl#ContractExecutionStatus> ;
  rdfs:subClassOf <https://w3id.org/dpv/owl#ContractExecutionStatus> ;
  dc:contributor _:genid4, _:genid1, _:genid17 ;
  dc:created "2025-01-09"^^xsd:date ;
  ns1:term_status "accepted"@en ;
  skos:definition "Status representing contract has been signed by the indicated signing party"@en ;
  skos:prefLabel "Contract Signed By Party"@en ;
  skos:scopeNote "The signing party can be expressed using dpv:hasParty with the status along with metadata such as a timestamp, or the status can be used to list whether each party in the contract has signed or not e.g. it is reviewing the contract"@en ;
  owl:sameAs <https://w3id.org/dpv#ContractSignedByParty>, <https://w3id.org/dpv/dpv-owl#ContractSignedByParty> .

<https://w3id.org/dpv/owl#hasRecipient>
  a owl:ObjectProperty, owl:NamedIndividual, odrl:LeftOperand ;
  rdfs:subPropertyOf <https://w3id.org/dpv/owl#hasEntity> ;
  ns2:domainIncludes <https://w3id.org/dpv/owl#RightExerciseActivity> ;
  ns2:rangeIncludes <https://w3id.org/dpv/owl#Recipient> ;
  dc:contributor _:genid13, _:genid9, _:genid31, _:genid1, _:genid11 ;
  dc:created "2019-04-04"^^xsd:date ;
  dc:modified "2020-11-04"^^xsd:date ;
  dc:source [
    a ns0:WebPage ;
    ns0:name "SPECIAL Project" ;
    ns0:url "https://specialprivacy.ercim.eu/"
  ] ;
  ns1:term_status "accepted"@en ;
  skos:definition "Indicates Recipient of Data"@en ;
  skos:prefLabel "has recipient"@en ;
  skos:scopeNote "Also used to indicate the Recipient of a Right Exercise Activity"@en ;
  ns0:domainIncludes <https://w3id.org/dpv/owl#RightExerciseActivity> ;
  ns0:rangeIncludes <https://w3id.org/dpv/owl#Recipient> ;
  owl:sameAs <https://w3id.org/dpv#hasRecipient>, <https://w3id.org/dpv/dpv-owl#hasRecipient> .

<https://w3id.org/dpv/owl#GovernmentalOrganisation>
  a owl:Class ;
  rdfs:subClassOf <https://w3id.org/dpv/owl#Organisation> ;
  dc:contributor _:genid1 ;
  dc:created "2022-02-02"^^xsd:date ;
  dc:modified "2020-10-05"^^xsd:date ;
  ns1:term_status "accepted"@en ;
  skos:definition "An organisation managed or part of government"@en ;
  skos:prefLabel "Governmental Organisation"@en ;
  owl:sameAs <https://w3id.org/dpv#GovernmentalOrganisation>, <https://w3id.org/dpv/dpv-owl#GovernmentalOrganisation> .

<https://w3id.org/dpv/owl#IdentifyingPersonalData>
  a owl:Class ;
  rdfs:subClassOf <https://w3id.org/dpv/owl#PersonalData> ;
  dc:created "2024-02-14"^^xsd:date ;
  ns1:term_status "accepted"@en ;
  skos:definition "Personal Data that explicitly and by itself is sufficient to identify a person"@en ;
  skos:prefLabel "Identifying Personal Data"@en ;
  skos:scopeNote "DPV does not use PII ('Personally Identifiable Information') as it has varying and conflicting definitions across sources. Instead the concept 'identifying personal data' is intended to provide a clear categorisation of its interpretation. Where multiple data categories can be combined to create an 'identifying' category e.g. fingerprinting, this concept represents the combined category."@en ;
  owl:sameAs <https://w3id.org/dpv#IdentifyingPersonalData>, <https://w3id.org/dpv/dpv-owl#IdentifyingPersonalData> .

<https://w3id.org/dpv/owl#hasServiceConsumer>
  a owl:ObjectProperty ;
  rdfs:subPropertyOf <https://w3id.org/dpv/owl#hasEntity> ;
  ns2:domainIncludes <https://w3id.org/dpv/owl#Service> ;
  ns2:rangeIncludes <https://w3id.org/dpv/owl#ServiceConsumer> ;
  dc:contributor _:genid1 ;
  dc:created "2024-04-20"^^xsd:date ;
  ns1:term_status "accepted"@en ;
  skos:definition "Indicates the entity that consumes or receives the associated service"@en ;
  skos:prefLabel "has service consumer"@en ;
  ns0:domainIncludes <https://w3id.org/dpv/owl#Service> ;
  ns0:rangeIncludes <https://w3id.org/dpv/owl#ServiceConsumer> ;
  owl:sameAs <https://w3id.org/dpv#hasServiceConsumer>, <https://w3id.org/dpv/dpv-owl#hasServiceConsumer> .

<https://w3id.org/dpv/owl#DigitalLiteracy>
  a owl:Class, owl:NamedIndividual, <https://w3id.org/dpv/owl#OrganisationalMeasure> ;
  rdfs:subClassOf <https://w3id.org/dpv/owl#OrganisationalMeasure> ;
  dc:contributor _:genid1 ;
  dc:created "2024-05-17"^^xsd:date ;
  ns1:term_status "accepted"@en ;
  skos:definition "Providing skills, knowledge, and understanding to enable reading, writing, analysing, reasoning, and communicating regarding digital technologies and their implications"@en ;
  skos:prefLabel "Digital Literacy"@en ;
  owl:sameAs <https://w3id.org/dpv#DigitalLiteracy>, <https://w3id.org/dpv/dpv-owl#DigitalLiteracy> .

<https://w3id.org/dpv/owl#ConsentWithdrawn>
  a owl:Class, owl:NamedIndividual, <https://w3id.org/dpv/owl#ConsentStatus> ;
  rdfs:subClassOf <https://w3id.org/dpv/owl#ConsentStatusInvalidForProcessing> ;
  dc:contributor _:genid4, _:genid1, _:genid17, _:genid6 ;
  dc:created "2022-06-22"^^xsd:date ;
  dc:source [
    a ns0:WebPage ;
    ns0:name "GConsent" ;
    ns0:url "https://w3id.org/GConsent"
  ] ;
  ns1:term_status "accepted"@en ;
  skos:definition "The state where the consent is withdrawn or revoked specifically by the data subject and which prevents it from being further used as a valid state"@en ;
  skos:prefLabel "Consent Withdrawn"@en ;
  skos:scopeNote "This state can be considered a form of 'revocation' of consent, where the revocation can only be performed by the data subject. Therefore we suggest using ConsentRevoked when it is a non-data-subject entity, and ConsentWithdrawn when it is the data subject"@en ;
  owl:sameAs <https://w3id.org/dpv#ConsentWithdrawn>, <https://w3id.org/dpv/dpv-owl#ConsentWithdrawn> .

<https://w3id.org/dpv/owl#hasNonPersonalDataProcess>
  a owl:ObjectProperty ;
  ns2:rangeIncludes <https://w3id.org/dpv/owl#NonPersonalDataProcess> ;
  dc:contributor _:genid1 ;
  dc:created "2023-12-12"^^xsd:date ;
  ns1:term_status "accepted"@en ;
  skos:definition "Indicates association with a Non-Personal Data Process"@en ;
  skos:prefLabel "has non-personal data process"@en ;
  ns0:rangeIncludes <https://w3id.org/dpv/owl#NonPersonalDataProcess> ;
  owl:sameAs <https://w3id.org/dpv#hasNonPersonalDataProcess>, <https://w3id.org/dpv/dpv-owl#hasNonPersonalDataProcess> .

<https://w3id.org/dpv/owl#ProcessingContext>
  a owl:Class ;
  rdfs:subClassOf <https://w3id.org/dpv/owl#Context> ;
  dc:contributor _:genid1 ;
  dc:created "2022-02-09"^^xsd:date ;
  ns1:term_status "accepted"@en ;
  skos:definition "Context or conditions within which processing takes place"@en ;
  skos:prefLabel "Processing Context"@en ;
  owl:sameAs <https://w3id.org/dpv#ProcessingContext>, <https://w3id.org/dpv/dpv-owl#ProcessingContext> .

<https://w3id.org/dpv/owl#supportsComplianceWith>
  a owl:ObjectProperty ;
  ns2:domainIncludes <https://w3id.org/dpv/owl#TechnicalOrganisationalMeasure> ;
  dc:contributor _:genid4, _:genid1, _:genid17 ;
  dc:created "2024-04-14"^^xsd:date ;
  ns1:term_status "accepted"@en ;
  skos:definition "Indicate the measure is required for meeting specified requirement or satisfying specified condition/constraint"@en ;
  skos:prefLabel "supports Compliance With"@en ;
  ns0:domainIncludes <https://w3id.org/dpv/owl#TechnicalOrganisationalMeasure> ;
  owl:sameAs <https://w3id.org/dpv#supportsComplianceWith>, <https://w3id.org/dpv/dpv-owl#supportsComplianceWith> .

<https://w3id.org/dpv/owl#ImproveExistingProductsAndServices>
  a owl:Class, owl:NamedIndividual, <https://w3id.org/dpv/owl#Purpose> ;
  rdfs:subClassOf <https://w3id.org/dpv/owl#OptimisationForController> ;
  dc:contributor _:genid13, _:genid14, _:genid1, _:genid15, _:genid16, _:genid11 ;
  dc:created "2019-04-05"^^xsd:date ;
  ns1:term_status "accepted"@en ;
  skos:definition "Purposes associated with improving existing products and services"@en ;
  skos:prefLabel "Improve Existing Products and Services"@en ;
  owl:sameAs <https://w3id.org/dpv#ImproveExistingProductsAndServices>, <https://w3id.org/dpv/dpv-owl#ImproveExistingProductsAndServices> .

<https://w3id.org/dpv/owl#LocationLocality>
  a owl:Class, owl:NamedIndividual, <https://w3id.org/dpv/owl#Location> ;
  rdfs:subClassOf <https://w3id.org/dpv/owl#Location> ;
  dc:contributor _:genid1 ;
  dc:created "2022-06-15"^^xsd:date ;
  dc:modified "2022-10-04"^^xsd:date ;
  ns3:example <https://w3id.org/dpv/examples/owl#E0060> ;
  ns1:term_status "accepted"@en ;
  skos:definition "Locality refers to whether the specified location is local within some context, e.g. for the user"@en ;
  skos:prefLabel "Location Locality"@en ;
  owl:sameAs <https://w3id.org/dpv#LocationLocality>, <https://w3id.org/dpv/dpv-owl#LocationLocality> .

<https://w3id.org/dpv/owl#LegalObligationStatus>
  a owl:Class ;
  rdfs:subClassOf <https://w3id.org/dpv/owl#Status> ;
  dc:created "2024-08-27"^^xsd:date ;
  ns3:example <https://w3id.org/dpv/examples/owl#E0079> ;
  ns1:term_status "accepted"@en ;
  skos:definition "Status associated with use of Legal Obligation as a legal basis"@en ;
  skos:prefLabel "Legal ObligationStatus"@en ;
  owl:sameAs <https://w3id.org/dpv#LegalObligationStatus>, <https://w3id.org/dpv/dpv-owl#LegalObligationStatus> .

<https://w3id.org/dpv/owl#MakeAvailable>
  a owl:Class, owl:NamedIndividual, <https://w3id.org/dpv/owl#Processing> ;
  rdfs:subClassOf <https://w3id.org/dpv/owl#Disclose> ;
  dc:created "2019-05-07"^^xsd:date ;
  dc:source [
    a ns0:WebPage ;
    ns0:name "GDPR Art.4-2" ;
    ns0:url "https://eur-lex.europa.eu/eli/reg/2016/679/art_4/par_2/oj"
  ] ;
  ns1:term_status "accepted"@en ;
  skos:definition "to transform or publish data to be used"@en ;
  skos:prefLabel "Make Data Available"@en ;
  owl:sameAs <https://w3id.org/dpv#MakeAvailable>, <https://w3id.org/dpv/dpv-owl#MakeAvailable> .

<https://w3id.org/dpv/owl#PhysicalAuthentication>
  a owl:Class, owl:NamedIndividual, <https://w3id.org/dpv/owl#PhysicalMeasure> ;
  rdfs:subClassOf <https://w3id.org/dpv/owl#PhysicalMeasure> ;
  dc:contributor _:genid1 ;
  dc:created "2024-04-14"^^xsd:date ;
  dc:source "NIST SP 800-15"@en ;
  ns1:term_status "accepted"@en ;
  skos:definition "Physical implementation of authentication e.g. by matching the person to their ID card"@en ;
  skos:prefLabel "Physical Authentication"@en ;
  owl:sameAs <https://w3id.org/dpv#PhysicalAuthentication>, <https://w3id.org/dpv/dpv-owl#PhysicalAuthentication> .

<https://w3id.org/dpv/owl#FixedOccurrencesDuration>
  a owl:Class ;
  rdfs:subClassOf <https://w3id.org/dpv/owl#Duration> ;
  dc:contributor _:genid1 ;
  dc:created "2022-06-15"^^xsd:date ;
  dc:modified "2020-10-05"^^xsd:date ;
  ns1:term_status "accepted"@en ;
  skos:definition "Duration that takes place a fixed number of times e.g. 3 times"@en ;
  skos:prefLabel "Fixed Occurrences Duration"@en ;
  owl:sameAs <https://w3id.org/dpv#FixedOccurrencesDuration>, <https://w3id.org/dpv/dpv-owl#FixedOccurrencesDuration> .

odrl:watermark
  a owl:NamedIndividual, skos:Concept, odrl:Action ;
  odrl:includedIn odrl:use ;
  rdfs:isDefinedBy odrl: ;
  rdfs:label "Watermark"@en ;
  skos:definition "To apply a watermark to the Asset."@en ;
  skos:scopeNote "Non-Normative"@en .

<https://w3id.org/dpv/owl#SellInsightsFromData>
  a owl:Class, owl:NamedIndividual, <https://w3id.org/dpv/owl#Purpose> ;
  rdfs:subClassOf <https://w3id.org/dpv/owl#SellProducts> ;
  dc:contributor _:genid13, _:genid14, _:genid1, _:genid15, _:genid16, _:genid11 ;
  dc:created "2019-04-05"^^xsd:date ;
  ns1:term_status "accepted"@en ;
  skos:definition "Purposes associated with selling or sharing insights obtained from analysis of data"@en ;
  skos:prefLabel "Sell Insights from Data"@en ;
  skos:scopeNote "Sell here means exchange, submit, or provide in return for direct or indirect compensation. Was subclass of commercial interest, changed to reflect selling something"@en ;
  owl:sameAs <https://w3id.org/dpv#SellInsightsFromData>, <https://w3id.org/dpv/dpv-owl#SellInsightsFromData> .

<https://w3id.org/dpv/owl#Unexpected>
  a owl:Class, owl:NamedIndividual, <https://w3id.org/dpv/owl#ExpectationStatus> ;
  rdfs:subClassOf <https://w3id.org/dpv/owl#ExpectationStatus> ;
  dc:contributor _:genid4, _:genid1, _:genid25, _:genid6 ;
  dc:created "2024-05-10"^^xsd:date ;
  ns1:term_status "accepted"@en ;
  skos:definition "Status indicating the specified context was unexpected i.e. not expected"@en ;
  skos:prefLabel "Unexpected"@en ;
  owl:sameAs <https://w3id.org/dpv#Unexpected>, <https://w3id.org/dpv/dpv-owl#Unexpected> .

<https://w3id.org/dpv/owl#TrackingByThirdParty>
  a owl:Class, owl:NamedIndividual, <https://w3id.org/dpv/owl#Processing> ;
  rdfs:subClassOf <https://w3id.org/dpv/owl#Tracking> ;
  dc:contributor _:genid1 ;
  dc:created "2024-12-17"^^xsd:date ;
  ns1:term_status "accepted"@en ;
  skos:definition "to perform tracking where the performing entity is a third party within the context"@en ;
  skos:prefLabel "Tracking by Third Party"@en ;
  skos:scopeNote "This concept does not strictly only specify the processing operation, but also the relation of the individual with the implementing entity. These concepts may change in the future based on discussions around how to express First and Third Party."@en ;
  owl:sameAs <https://w3id.org/dpv#TrackingByThirdParty>, <https://w3id.org/dpv/dpv-owl#TrackingByThirdParty> .

<https://w3id.org/dpv/owl#hasIntention>
  a owl:ObjectProperty ;
  rdfs:subPropertyOf <https://w3id.org/dpv/owl#hasStatus> ;
  ns2:rangeIncludes <https://w3id.org/dpv/owl#IntentionStatus> ;
  dc:contributor _:genid1 ;
  dc:created "2024-05-10"^^xsd:date ;
  ns1:term_status "accepted"@en ;
  skos:definition "Indicates whether the specified context was intended or unintended"@en ;
  skos:prefLabel "has intention"@en ;
  ns0:rangeIncludes <https://w3id.org/dpv/owl#IntentionStatus> ;
  owl:sameAs <https://w3id.org/dpv#hasIntention>, <https://w3id.org/dpv/dpv-owl#hasIntention> .

<https://w3id.org/dpv/owl#hasJointDataControllers>
  a owl:ObjectProperty ;
  rdfs:subPropertyOf <https://w3id.org/dpv/owl#hasDataController> ;
  ns2:rangeIncludes <https://w3id.org/dpv/owl#JointDataControllers> ;
  dc:contributor _:genid4, _:genid1, _:genid6 ;
  dc:created "2022-02-09"^^xsd:date ;
  ns1:term_status "accepted"@en ;
  skos:definition "Indicates inclusion or applicability of a Joint Data Controller"@en ;
  skos:prefLabel "has joint data controllers"@en ;
  ns0:rangeIncludes <https://w3id.org/dpv/owl#JointDataControllers> ;
  owl:sameAs <https://w3id.org/dpv#hasJointDataControllers>, <https://w3id.org/dpv/dpv-owl#hasJointDataControllers> .

cc:CommercialUse
  a owl:NamedIndividual, skos:Concept, odrl:Action ;
  odrl:includedIn odrl:use ;
  rdfs:isDefinedBy odrl: ;
  rdfs:label "Commercial Use"@en ;
  skos:definition "Exercising rights for commercial purposes."@en ;
  skos:note "This term is defined by Creative Commons."@en ;
  skos:scopeNote "Non-Normative"@en .

<https://w3id.org/dpv/owl#ScoringOfIndividuals>
  a owl:Class, owl:NamedIndividual, <https://w3id.org/dpv/owl#EvaluationScoring> ;
  rdfs:subClassOf <https://w3id.org/dpv/owl#EvaluationScoring> ;
  dc:contributor _:genid1 ;
  dc:created "2022-10-22"^^xsd:date ;
  dc:modified "2022-11-30"^^xsd:date ;
  dc:source [
    a ns0:WebPage ;
    ns0:name "GDPR Art.4-2" ;
    ns0:url "https://eur-lex.europa.eu/eli/reg/2016/679/art_4/par_2/oj"
  ] ;
  ns1:term_status "accepted"@en ;
  skos:definition "Processing that involves scoring of individuals"@en ;
  skos:prefLabel "Scoring of Individuals"@en ;
  owl:sameAs <https://w3id.org/dpv#ScoringOfIndividuals>, <https://w3id.org/dpv/dpv-owl#ScoringOfIndividuals> .

<https://w3id.org/dpv/owl#ChallengingProcessOutput>
  a owl:Class, owl:NamedIndividual, <https://w3id.org/dpv/owl#EntityPermissiveInvolvement> ;
  rdfs:subClassOf <https://w3id.org/dpv/owl#EntityPermissiveInvolvement> ;
  dc:contributor _:genid1, _:genid25, _:genid19 ;
  dc:created "2024-05-11"^^xsd:date ;
  ns1:term_status "accepted"@en ;
  skos:definition "Involvement where entity can challenge the output of specified context"@en ;
  skos:prefLabel "Challenging Process Output"@en ;
  skos:scopeNote "Challenge refers to raising questions about validity, necessity, correctness, or other similar 'trustworthiness' attributes regarding the output of the process or plan or implementation (where output is distinct from the process itself)"@en ;
  owl:sameAs <https://w3id.org/dpv#ChallengingProcessOutput>, <https://w3id.org/dpv/dpv-owl#ChallengingProcessOutput> .

<https://w3id.org/dpv/owl#ContractByDomain>
  a owl:Class, owl:NamedIndividual, <https://w3id.org/dpv/owl#LegalBasis> ;
  rdfs:subClassOf <https://w3id.org/dpv/owl#Contract> ;
  dc:created "2024-12-17"^^xsd:date ;
  ns1:term_status "accepted"@en ;
  skos:definition "A generic concept representing contracts categorised by specific domains which dictate the drafting and interpretation of contracts"@en ;
  skos:prefLabel "Contract by Domain"@en ;
  owl:sameAs <https://w3id.org/dpv#ContractByDomain>, <https://w3id.org/dpv/dpv-owl#ContractByDomain> .

<https://w3id.org/dpv/owl#PrivacyByDefault>
  a owl:Class, owl:NamedIndividual, <https://w3id.org/dpv/owl#OrganisationalMeasure> ;
  rdfs:subClassOf <https://w3id.org/dpv/owl#GuidelinesPrinciple> ;
  dc:contributor _:genid9, _:genid10, _:genid1, _:genid11 ;
  dc:created "2019-04-05"^^xsd:date ;
  dc:modified "2024-04-14"^^xsd:date ;
  ns1:term_status "accepted"@en ;
  skos:definition "Practices regarding setting the default configurations of information and services to implement data protection and privacy (synonymous with Data Protection by Default)"@en ;
  skos:prefLabel "Privacy by Default"@en ;
  owl:sameAs <https://w3id.org/dpv#PrivacyByDefault>, <https://w3id.org/dpv/dpv-owl#PrivacyByDefault> .

<https://w3id.org/dpv/owl#ContractPerformanceStatus>
  a owl:Class ;
  rdfs:subClassOf <https://w3id.org/dpv/owl#ContractStatus> ;
  dc:contributor _:genid4, _:genid1, _:genid17 ;
  dc:created "2025-01-09"^^xsd:date ;
  ns1:term_status "accepted"@en ;
  skos:definition "Status associated with performance of a contract"@en ;
  skos:prefLabel "Contract Performance Status"@en ;
  owl:sameAs <https://w3id.org/dpv#ContractPerformanceStatus>, <https://w3id.org/dpv/dpv-owl#ContractPerformanceStatus> .

<https://w3id.org/dpv/owl#DataQualityManagement>
  a owl:Class, owl:NamedIndividual, <https://w3id.org/dpv/owl#OrganisationalMeasure> ;
  rdfs:subClassOf <https://w3id.org/dpv/owl#DataGovernance> ;
  dc:contributor _:genid1 ;
  dc:created "2024-04-14"^^xsd:date ;
  ns1:term_status "accepted"@en ;
  skos:definition "Measures associated with management of data quality"@en ;
  skos:prefLabel "Data Quality Management"@en ;
  owl:sameAs <https://w3id.org/dpv#DataQualityManagement>, <https://w3id.org/dpv/dpv-owl#DataQualityManagement> .

<https://w3id.org/dpv/owl#DataControllerContract>
  a owl:Class, owl:NamedIndividual, <https://w3id.org/dpv/owl#LegalBasis> ;
  rdfs:subClassOf <https://w3id.org/dpv/owl#DataProcessingAgreement> ;
  dc:created "2023-12-10"^^xsd:date ;
  dc:modified "2024-08-27"^^xsd:date ;
  ns1:term_status "sunset"@en ;
  skos:definition "Creation, completion, fulfilment, or performance of a contract, with Data Controllers as parties being Joint Data Controllers, and involving specified processing of data or technologies. NOTE: This concept is being deprecated - use dpv:JointDataControllersAgreement which has a more explicit definition of the entities involved and the intent of the contract"@en ;
  skos:prefLabel "Data Controller Contract"@en ;
  owl:sameAs <https://w3id.org/dpv#DataControllerContract>, <https://w3id.org/dpv/dpv-owl#DataControllerContract> .

<https://w3id.org/dpv/owl#ThirdParty>
  a owl:Class ;
  rdfs:subClassOf <https://w3id.org/dpv/owl#LegalEntity> ;
  dc:contributor _:genid1 ;
  dc:created "2019-06-04"^^xsd:date ;
  dc:modified "2024-05-21"^^xsd:date ;
  dc:source [
    a ns0:WebPage ;
    ns0:name "GDPR Art.4-10" ;
    ns0:url "https://eur-lex.europa.eu/eli/reg/2016/679/art_4/par_10/oj"
  ] ;
  ns1:term_status "accepted"@en ;
  skos:definition "A ‘third party’ means any natural or legal person other than - the entities directly involved or operating under those directly involved in a process"@en ;
  skos:prefLabel "Third Party"@en ;
  skos:scopeNote "Third Party in the context of personal data processing are entities other than the data subject, controllers, processors, and authorities"@en ;
  owl:sameAs <https://w3id.org/dpv#ThirdParty>, <https://w3id.org/dpv/dpv-owl#ThirdParty> .

<https://w3id.org/dpv/owl#SupportExchangeOfViews>
  a owl:Class, owl:NamedIndividual, <https://w3id.org/dpv/owl#OrganisationalMeasure> ;
  rdfs:subClassOf <https://w3id.org/dpv/owl#SupportEntityDecisionMaking> ;
  dc:contributor _:genid5, _:genid1 ;
  dc:created "2024-04-14"^^xsd:date ;
  dc:source "DGA 2.15"@en ;
  ns1:term_status "accepted"@en ;
  skos:definition "Supporting individuals and entities in exchanging views e.g. regarding data processing purposes for their best interests"@en ;
  skos:prefLabel "Support Exchange of Views"@en ;
  owl:sameAs <https://w3id.org/dpv#SupportExchangeOfViews>, <https://w3id.org/dpv/dpv-owl#SupportExchangeOfViews> .

<https://w3id.org/dpv/owl#HomomorphicEncryption>
  a owl:Class, owl:NamedIndividual, <https://w3id.org/dpv/owl#TechnicalMeasure> ;
  rdfs:subClassOf <https://w3id.org/dpv/owl#CryptographicMethods> ;
  dc:contributor _:genid1 ;
  dc:created "2022-08-17"^^xsd:date ;
  dc:source [
    a ns0:WebPage ;
    ns0:name "ENISA Reference Incident Classification Taxonomy 2018" ;
    ns0:url "https://www.enisa.europa.eu/publications/reference-incident-classification-taxonomy/"
  ] ;
  ns1:term_status "accepted"@en ;
  skos:definition "Use of Homomorphic encryption that permits computations on encrypted data without decrypting it"@en ;
  skos:prefLabel "Homomorphic Encryption"@en ;
  owl:sameAs <https://w3id.org/dpv#HomomorphicEncryption>, <https://w3id.org/dpv/dpv-owl#HomomorphicEncryption> .

<https://w3id.org/dpv/owl#CharityOrganisation>
  a owl:Class ;
  rdfs:subClassOf <https://w3id.org/dpv/owl#LegalEntity> ;
  dc:contributor _:genid4 ;
  dc:created "2024-12-01"^^xsd:date ;
  ns1:term_status "accepted"@en ;
  skos:definition "A nonprofit entity dedicated to providing assistance or raising funds for social, educational, religious, or other philanthropic purposes"@en ;
  skos:prefLabel "Charity Organisation"@en ;
  owl:sameAs <https://w3id.org/dpv#CharityOrganisation>, <https://w3id.org/dpv/dpv-owl#CharityOrganisation> .

<https://w3id.org/dpv/owl#Sector>
  a owl:Class ;
  dc:contributor _:genid13, _:genid14, _:genid1, _:genid15, _:genid16, _:genid11 ;
  dc:created "2019-04-05"^^xsd:date ;
  ns3:example <https://w3id.org/dpv/examples/owl#E0043> ;
  ns1:term_status "accepted"@en ;
  skos:definition "Sector describes the area of application or domain that indicates or restricts scope for interpretation and application of purpose e.g. Agriculture, Banking"@en ;
  skos:prefLabel "Sector"@en ;
  skos:scopeNote "There are various sector codes used commonly to indicate the domain of an organisation or business. Examples include NACE (EU), ISIC (UN), SIC and NAICS (USA)."@en ;
  owl:sameAs <https://w3id.org/dpv#Sector>, <https://w3id.org/dpv/dpv-owl#Sector> .

<https://w3id.org/dpv/owl#AsylumSeeker>
  a owl:Class, owl:NamedIndividual, <https://w3id.org/dpv/owl#HumanSubject> ;
  rdfs:subClassOf <https://w3id.org/dpv/owl#VulnerableHuman> ;
  dc:contributor _:genid4 ;
  dc:created "2022-06-15"^^xsd:date ;
  dc:modified "2024-12-17"^^xsd:date ;
  ns1:term_status "modified"@en ;
  skos:definition "Humans that are asylum seekers"@en ;
  skos:prefLabel "Asylum Seeker"@en ;
  owl:sameAs <https://w3id.org/dpv#AsylumSeeker>, <https://w3id.org/dpv/dpv-owl#AsylumSeeker> .

<https://w3id.org/dpv/owl#OfficialAuthorityExercisePending>
  a owl:Class, owl:NamedIndividual, <https://w3id.org/dpv/owl#OfficialAuthorityExerciseStatus> ;
  rdfs:subClassOf <https://w3id.org/dpv/owl#OfficialAuthorityExerciseStatus> ;
  dc:created "2024-08-27"^^xsd:date ;
  ns1:term_status "accepted"@en ;
  skos:definition "Status where the official authority has not been exercised"@en ;
  skos:prefLabel "Official Authority Exercise Pending"@en ;
  owl:sameAs <https://w3id.org/dpv#OfficialAuthorityExercisePending>, <https://w3id.org/dpv/dpv-owl#OfficialAuthorityExercisePending> .

<https://w3id.org/dpv/owl#DataTransferImpactAssessment>
  a owl:Class, owl:NamedIndividual, <https://w3id.org/dpv/owl#OrganisationalMeasure> ;
  rdfs:subClassOf <https://w3id.org/dpv/owl#ImpactAssessment> ;
  dc:contributor _:genid4, _:genid1, _:genid6 ;
  dc:created "2021-09-08"^^xsd:date ;
  ns1:term_status "accepted"@en ;
  skos:definition "Impact Assessment for conducting data transfers"@en ;
  skos:prefLabel "Data Transfer Impact Assessment"@en ;
  owl:sameAs <https://w3id.org/dpv#DataTransferImpactAssessment>, <https://w3id.org/dpv/dpv-owl#DataTransferImpactAssessment> .

<https://w3id.org/dpv/owl#DeterministicPseudonymisation>
  a owl:Class, owl:NamedIndividual, <https://w3id.org/dpv/owl#TechnicalMeasure> ;
  rdfs:subClassOf <https://w3id.org/dpv/owl#Pseudonymisation> ;
  dc:contributor _:genid1 ;
  dc:created "2022-08-17"^^xsd:date ;
  dc:source [
    a ns0:WebPage ;
    ns0:name "ENISA Data Pseudonymisation: Advanced Techniques and Use Cases" ;
    ns0:url "https://www.enisa.europa.eu/publications/data-pseudonymisation-advanced-techniques-and-use-cases"
  ] ;
  ns1:term_status "accepted"@en ;
  skos:definition "Pseudonymisation achieved through a deterministic function"@en ;
  skos:prefLabel "Deterministic Pseudonymisation"@en ;
  owl:sameAs <https://w3id.org/dpv#DeterministicPseudonymisation>, <https://w3id.org/dpv/dpv-owl#DeterministicPseudonymisation> .

<https://w3id.org/dpv/owl#DataControllerDataSource>
  a owl:Class, owl:NamedIndividual, <https://w3id.org/dpv/owl#DataSource> ;
  rdfs:subClassOf <https://w3id.org/dpv/owl#DataSource> ;
  dc:created "2023-10-12"^^xsd:date ;
  ns1:term_status "accepted"@en ;
  skos:definition "Data Sourced from Data Controller(s), e.g. a Controller inferring data or generating data"@en ;
  skos:prefLabel "Data Controller as Data Source"@en ;
  owl:sameAs <https://w3id.org/dpv#DataControllerDataSource>, <https://w3id.org/dpv/dpv-owl#DataControllerDataSource> .

<https://w3id.org/dpv/owl#Standard>
  a owl:Class, owl:NamedIndividual, <https://w3id.org/dpv/owl#OrganisationalMeasure> ;
  rdfs:subClassOf <https://w3id.org/dpv/owl#GuidelinesPrinciple> ;
  dc:contributor _:genid1, _:genid25 ;
  dc:created "2024-12-01"^^xsd:date ;
  ns1:term_status "accepted"@en ;
  skos:definition "A set of requirements or norms that are agreed upon i.e. they are considered a 'standard'"@en ;
  skos:prefLabel "Standard"@en ;
  skos:scopeNote "DPV does not restrict the notion of 'standard' to those published by specific or 'formal' bodies"@en ;
  owl:sameAs <https://w3id.org/dpv#Standard>, <https://w3id.org/dpv/dpv-owl#Standard> .

<https://w3id.org/dpv/owl#DataSecurityManagement>
  a owl:Class, owl:NamedIndividual, <https://w3id.org/dpv/owl#OrganisationalMeasure> ;
  rdfs:subClassOf <https://w3id.org/dpv/owl#DataGovernance>, <https://w3id.org/dpv/owl#SecurityProcedure> ;
  dc:contributor _:genid1 ;
  dc:created "2024-04-14"^^xsd:date ;
  ns1:term_status "accepted"@en ;
  skos:definition "Measures associated with management of data security"@en ;
  skos:prefLabel "Data Security Management"@en ;
  skos:scopeNote "Examples of data security management are assessing the appropriate security controls such as encryption, testing the implemented security controls, and ensuring it is protected and safeguarded from unintended actions"@en ;
  owl:sameAs <https://w3id.org/dpv#DataSecurityManagement>, <https://w3id.org/dpv/dpv-owl#DataSecurityManagement> .

<https://w3id.org/dpv/owl#CannotOptInToProcess>
  a owl:Class, owl:NamedIndividual, <https://w3id.org/dpv/owl#EntityNonPermissiveInvolvement> ;
  rdfs:subClassOf <https://w3id.org/dpv/owl#EntityNonPermissiveInvolvement> ;
  dc:contributor _:genid1, _:genid25, _:genid19 ;
  dc:created "2024-05-11"^^xsd:date ;
  ns1:term_status "accepted"@en ;
  skos:definition "Involvement where entity cannot opt-in to specified context"@en ;
  skos:prefLabel "Cannot Opt-in to Process"@en ;
  owl:sameAs <https://w3id.org/dpv#CannotOptInToProcess>, <https://w3id.org/dpv/dpv-owl#CannotOptInToProcess> .

<https://w3id.org/dpv/owl#NonCompliant>
  a owl:Class, owl:NamedIndividual, <https://w3id.org/dpv/owl#ComplianceStatus> ;
  rdfs:subClassOf <https://w3id.org/dpv/owl#ComplianceStatus> ;
  dc:contributor _:genid1 ;
  dc:created "2022-05-18"^^xsd:date ;
  dc:modified "2022-09-07"^^xsd:date ;
  ns1:term_status "accepted"@en ;
  skos:definition "State of non-compliance where objectives have not been met, but have not been violated"@en ;
  skos:prefLabel "Non Compliant"@en ;
  skos:scopeNote "Changed from not compliant for consistency in commonly used terms"@en ;
  owl:sameAs <https://w3id.org/dpv#NonCompliant>, <https://w3id.org/dpv/dpv-owl#NonCompliant> .

<https://w3id.org/dpv/owl#ParentLegalEntity>
  a owl:Class ;
  rdfs:subClassOf <https://w3id.org/dpv/owl#Organisation> ;
  dc:contributor _:genid4, _:genid1 ;
  dc:created "2024-04-14"^^xsd:date ;
  ns1:term_status "accepted"@en ;
  skos:definition "A legal entity that has one or more subsidiary entities operating under it"@en ;
  skos:prefLabel "Parent Legal Entity"@en ;
  owl:sameAs <https://w3id.org/dpv#ParentLegalEntity>, <https://w3id.org/dpv/dpv-owl#ParentLegalEntity> .

<https://w3id.org/dpv/owl#hasFrequency>
  a owl:ObjectProperty ;
  ns2:rangeIncludes <https://w3id.org/dpv/owl#Frequency> ;
  dc:contributor _:genid1 ;
  dc:created "2022-02-16"^^xsd:date ;
  ns3:example <https://w3id.org/dpv/examples/owl#E0051> ;
  ns1:term_status "accepted"@en ;
  skos:definition "Indicates the frequency with which something takes place"@en ;
  skos:prefLabel "has frequency"@en ;
  ns0:rangeIncludes <https://w3id.org/dpv/owl#Frequency> ;
  owl:sameAs <https://w3id.org/dpv#hasFrequency>, <https://w3id.org/dpv/dpv-owl#hasFrequency> .

<https://w3id.org/dpv/owl#DataProtectionTraining>
  a owl:Class, owl:NamedIndividual, <https://w3id.org/dpv/owl#OrganisationalMeasure> ;
  rdfs:subClassOf <https://w3id.org/dpv/owl#StaffTraining> ;
  dc:contributor _:genid1 ;
  dc:created "2022-08-17"^^xsd:date ;
  dc:source [
    a ns0:WebPage ;
    ns0:name "ENISA 5G Cybersecurity Standards" ;
    ns0:url "https://www.enisa.europa.eu/publications/5g-cybersecurity-standards"
  ] ;
  ns1:term_status "accepted"@en ;
  skos:definition "Training intended to increase knowledge regarding data protection"@en ;
  skos:prefLabel "Data Protection Training"@en ;
  owl:sameAs <https://w3id.org/dpv#DataProtectionTraining>, <https://w3id.org/dpv/dpv-owl#DataProtectionTraining> .

odrl:dataType
  a owl:ObjectProperty, owl:NamedIndividual, skos:Concept ;
  rdfs:domain odrl:Constraint ;
  rdfs:range rdfs:Datatype ;
  rdfs:isDefinedBy odrl: ;
  rdfs:label "Datatype"@en ;
  skos:definition "The datatype of the value of the rightOperand or rightOperandReference of a Constraint."@en ;
  skos:note "In RDF encodings, use of the rdf:datatype MUST be used. In JSON-LD encoding, the use of @type MUST be used."@en .

<https://w3id.org/dpv/owl#RefuseContract>
  a owl:Class ;
  rdfs:subClassOf <https://w3id.org/dpv/owl#ContractControl> ;
  dc:created "2024-08-27"^^xsd:date ;
  ns1:term_status "accepted"@en ;
  skos:definition "Control for refusing a contract"@en ;
  skos:prefLabel "Refuse Contract"@en ;
  owl:sameAs <https://w3id.org/dpv#RefuseContract>, <https://w3id.org/dpv/dpv-owl#RefuseContract> .

<https://w3id.org/dpv/owl#RandomLocation>
  a owl:Class, owl:NamedIndividual, <https://w3id.org/dpv/owl#LocationFixture> ;
  rdfs:subClassOf <https://w3id.org/dpv/owl#LocationFixture> ;
  dc:contributor _:genid1 ;
  dc:created "2022-06-15"^^xsd:date ;
  dc:modified "2020-10-05"^^xsd:date ;
  ns1:term_status "accepted"@en ;
  skos:definition "Location that is random or unknown"@en ;
  skos:prefLabel "Random Location"@en ;
  owl:sameAs <https://w3id.org/dpv#RandomLocation>, <https://w3id.org/dpv/dpv-owl#RandomLocation> .

<https://w3id.org/dpv/owl#PrivateLocation>
  a owl:Class, owl:NamedIndividual, <https://w3id.org/dpv/owl#Location> ;
  rdfs:subClassOf <https://w3id.org/dpv/owl#LocalLocation> ;
  dc:contributor _:genid1 ;
  dc:created "2022-10-22"^^xsd:date ;
  ns1:term_status "accepted"@en ;
  skos:definition "Location that is not or cannot be accessed by the public and is controlled as a private space"@en ;
  skos:prefLabel "Private Location"@en ;
  owl:sameAs <https://w3id.org/dpv#PrivateLocation>, <https://w3id.org/dpv/dpv-owl#PrivateLocation> .

<https://w3id.org/dpv/owl#EntityNonInvolvement>
  a owl:Class ;
  rdfs:subClassOf <https://w3id.org/dpv/owl#EntityInvolvement> ;
  dc:contributor _:genid25 ;
  dc:created "2024-05-11"^^xsd:date ;
  ns1:term_status "accepted"@en ;
  skos:definition "Indicating entity is not involved"@en ;
  skos:prefLabel "Entity Non-Involvement"@en ;
  owl:sameAs <https://w3id.org/dpv#EntityNonInvolvement>, <https://w3id.org/dpv/dpv-owl#EntityNonInvolvement> .

<https://w3id.org/dpv/owl#DisasterRecoveryProcedures>
  a owl:Class, owl:NamedIndividual, <https://w3id.org/dpv/owl#OrganisationalMeasure> ;
  rdfs:subClassOf <https://w3id.org/dpv/owl#GovernanceProcedures> ;
  dc:contributor _:genid1 ;
  dc:created "2022-08-17"^^xsd:date ;
  dc:source [
    a ns0:WebPage ;
    ns0:name "ENISA 5G Cybersecurity Standards" ;
    ns0:url "https://www.enisa.europa.eu/publications/5g-cybersecurity-standards"
  ] ;
  ns1:term_status "accepted"@en ;
  skos:definition "Procedures related to management of disasters and recovery"@en ;
  skos:prefLabel "Disaster Recovery Procedures"@en ;
  owl:sameAs <https://w3id.org/dpv#DisasterRecoveryProcedures>, <https://w3id.org/dpv/dpv-owl#DisasterRecoveryProcedures> .

<https://w3id.org/dpv/owl#DistributedSystemSecurity>
  a owl:Class, owl:NamedIndividual, <https://w3id.org/dpv/owl#TechnicalMeasure> ;
  rdfs:subClassOf <https://w3id.org/dpv/owl#SecurityMethod> ;
  dc:contributor _:genid1 ;
  dc:created "2022-08-17"^^xsd:date ;
  dc:source [
    a ns0:WebPage ;
    ns0:name "ENISA Reference Incident Classification Taxonomy 2018" ;
    ns0:url "https://www.enisa.europa.eu/publications/reference-incident-classification-taxonomy/"
  ] ;
  ns1:term_status "accepted"@en ;
  skos:definition "Security implementations provided using or over a distributed system"@en ;
  skos:prefLabel "Distributed System Security"@en ;
  owl:sameAs <https://w3id.org/dpv#DistributedSystemSecurity>, <https://w3id.org/dpv/dpv-owl#DistributedSystemSecurity> .

<https://w3id.org/dpv/owl#ContractUnderReview>
  a owl:Class, owl:NamedIndividual, <https://w3id.org/dpv/owl#ContractPreparationStatus> ;
  rdfs:subClassOf <https://w3id.org/dpv/owl#ContractPreparationStatus> ;
  dc:contributor _:genid4, _:genid1, _:genid17 ;
  dc:created "2025-01-09"^^xsd:date ;
  ns1:term_status "accepted"@en ;
  skos:definition "Status representing contract is under review and is being considered for signing"@en ;
  skos:prefLabel "Contract Under Review"@en ;
  owl:sameAs <https://w3id.org/dpv#ContractUnderReview>, <https://w3id.org/dpv/dpv-owl#ContractUnderReview> .

<https://w3id.org/dpv/owl#LawEnforcementOrganisation>
  a owl:Class ;
  rdfs:subClassOf <https://w3id.org/dpv/owl#Organisation> ;
  dc:contributor _:genid25 ;
  dc:created "2024-12-01"^^xsd:date ;
  ns1:term_status "accepted"@en ;
  skos:definition "An organisation that is an agency responsible for enforcing laws, maintaining public order, and ensuring public safety"@en ;
  skos:prefLabel "Law Enforcement Organisation"@en ;
  owl:sameAs <https://w3id.org/dpv#LawEnforcementOrganisation>, <https://w3id.org/dpv/dpv-owl#LawEnforcementOrganisation> .

<https://w3id.org/dpv/owl#hasContext>
  a owl:ObjectProperty ;
  ns2:rangeIncludes <https://w3id.org/dpv/owl#Context> ;
  dc:created "2019-04-05"^^xsd:date ;
  ns1:term_status "accepted"@en ;
  skos:definition "Indicates a purpose is restricted to the specified context(s)"@en ;
  skos:prefLabel "has context"@en ;
  ns0:rangeIncludes <https://w3id.org/dpv/owl#Context> ;
  owl:sameAs <https://w3id.org/dpv#hasContext>, <https://w3id.org/dpv/dpv-owl#hasContext> .

<https://w3id.org/dpv/owl#hasRisk>
  a owl:ObjectProperty, owl:NamedIndividual, odrl:LeftOperand ;
  ns2:rangeIncludes <https://w3id.org/dpv/owl#Risk> ;
  dc:contributor _:genid1 ;
  dc:created "2020-11-18"^^xsd:date ;
  ns3:example <https://w3id.org/dpv/examples/owl#E0068> ;
  ns1:term_status "accepted"@en ;
  skos:definition "Indicates applicability of Risk for this concept"@en ;
  skos:prefLabel "has risk"@en ;
  ns0:rangeIncludes <https://w3id.org/dpv/owl#Risk> ;
  owl:sameAs <https://w3id.org/dpv#hasRisk>, <https://w3id.org/dpv/dpv-owl#hasRisk> .

<https://w3id.org/dpv/owl#hasAlgorithmicLogic>
  a owl:ObjectProperty ;
  ns2:rangeIncludes <https://w3id.org/dpv/owl#AlgorithmicLogic> ;
  dc:contributor _:genid4, _:genid1, _:genid6 ;
  dc:created "2020-11-04"^^xsd:date ;
  dc:modified "2022-06-15"^^xsd:date ;
  ns1:term_status "accepted"@en ;
  skos:definition "Indicates the logic used in processing such as for automated decision making"@en ;
  skos:prefLabel "has algorithmic logic"@en ;
  ns0:rangeIncludes <https://w3id.org/dpv/owl#AlgorithmicLogic> ;
  owl:sameAs <https://w3id.org/dpv#hasAlgorithmicLogic>, <https://w3id.org/dpv/dpv-owl#hasAlgorithmicLogic> .

odrl:Agreement
  a owl:Class, owl:NamedIndividual, skos:Concept ;
  rdfs:subClassOf odrl:Policy ;
  owl:disjointWith odrl:Assertion, odrl:Offer, odrl:Privacy, odrl:Request, odrl:Set, odrl:Ticket ;
  rdfs:isDefinedBy odrl: ;
  rdfs:label "Agreement"@en ;
  skos:definition "A Policy that grants the assignee a Rule over an Asset from an assigner."@en ;
  skos:note "An Agreement Policy MUST contain at least one Permission or Prohibition rule, a Party with Assigner function, and a Party with Assignee function (in the same Permission or Prohibition). The Agreement Policy will grant the terms of the Policy from the Assigner to the Assignee."@en .

<https://w3id.org/dpv/owl#ProvideOfficialStatistics>
  a owl:Class, owl:NamedIndividual, <https://w3id.org/dpv/owl#Purpose> ;
  rdfs:subClassOf <https://w3id.org/dpv/owl#PublicBenefit> ;
  dc:contributor _:genid5, _:genid1 ;
  dc:created "2024-02-14"^^xsd:date ;
  dc:source "DGA 2.16"@en ;
  ns1:term_status "accepted"@en ;
  skos:definition "Purposes associated with facilitating the development, production and dissemination of reliable official statistics"@en ;
  skos:prefLabel "Provide Official Statistics"@en ;
  owl:sameAs <https://w3id.org/dpv#ProvideOfficialStatistics>, <https://w3id.org/dpv/dpv-owl#ProvideOfficialStatistics> .

<https://w3id.org/dpv/owl#DataAltruism>
  a owl:Class, owl:NamedIndividual, <https://w3id.org/dpv/owl#Purpose> ;
  rdfs:subClassOf <https://w3id.org/dpv/owl#PublicBenefit> ;
  dc:contributor _:genid5, _:genid1 ;
  dc:created "2024-02-14"^^xsd:date ;
  dc:source "DGA 2.16"@en ;
  ns1:term_status "accepted"@en ;
  skos:definition "Purposes associated with the voluntary sharing of data for the general interest of the public, such as healthcare or combating climate change"@en ;
  skos:prefLabel "Data Altruism"@en ;
  skos:scopeNote "Data Altruism as a purpose should be combined with other purposes to indicate their altruistic interpretation or application. E.g. improving healthcare and data altruism in combination."@en ;
  owl:sameAs <https://w3id.org/dpv#DataAltruism>, <https://w3id.org/dpv/dpv-owl#DataAltruism> .

<https://w3id.org/dpv/owl#HumanNotInvolved>
  a owl:Class, owl:NamedIndividual, <https://w3id.org/dpv/owl#HumanInvolvement> ;
  rdfs:subClassOf <https://w3id.org/dpv/owl#HumanInvolvement> ;
  dc:created "2023-12-10"^^xsd:date ;
  ns1:term_status "accepted"@en ;
  skos:definition "Humans are not involved in the specified context"@en ;
  skos:prefLabel "Human not involved"@en ;
  skos:scopeNote "This maps to Autonomous and Full Automation models if no humans are involved."@en ;
  owl:sameAs <https://w3id.org/dpv#HumanNotInvolved>, <https://w3id.org/dpv/dpv-owl#HumanNotInvolved> .

odrl:meteredTime
  a owl:NamedIndividual, skos:Concept, odrl:LeftOperand ;
  rdfs:isDefinedBy odrl: ;
  rdfs:label "Metered Time"@en ;
  skos:definition "An accumulated amount of one to many metered time periods which were used for exercising the action of the Rule. Right operand value MUST be an xsd:duration as defined by [[xmlschema11-2]]."@en ;
  skos:note "Only the eq, lt, lteq operators SHOULD be used. See also Elapsed Time. <br />Example: <code>meteredTime lteq P60M</code> indicates an accumulated period of 60 Minutes or less." ;
  skos:scopeNote "Non-Normative"@en .

<https://w3id.org/dpv/owl#OftenFrequency>
  a owl:Class, owl:NamedIndividual, <https://w3id.org/dpv/owl#Frequency> ;
  rdfs:subClassOf <https://w3id.org/dpv/owl#Frequency> ;
  dc:contributor _:genid1 ;
  dc:created "2022-06-15"^^xsd:date ;
  dc:modified "2020-10-05"^^xsd:date ;
  ns1:term_status "accepted"@en ;
  skos:definition "Frequency where occurrences are often or frequent, but not continuous"@en ;
  skos:prefLabel "Often Frequency"@en ;
  owl:sameAs <https://w3id.org/dpv#OftenFrequency>, <https://w3id.org/dpv/dpv-owl#OftenFrequency> .

<https://w3id.org/dpv/owl#ObligationFulfilled>
  a owl:Class, owl:NamedIndividual, <https://w3id.org/dpv/owl#RuleFulfilmentStatus> ;
  rdfs:subClassOf <https://w3id.org/dpv/owl#RuleFulfilled> ;
  dc:contributor _:genid1 ;
  dc:created "2024-09-10"^^xsd:date ;
  ns1:term_status "accepted"@en ;
  skos:definition "Status indicating an obligation has been fulfilled i.e. the activity stated as being required to be carried out has been successfully completed"@en ;
  skos:prefLabel "Obligation Fulfilled"@en ;
  owl:sameAs <https://w3id.org/dpv#ObligationFulfilled>, <https://w3id.org/dpv/dpv-owl#ObligationFulfilled> .

<https://w3id.org/dpv/owl#Match>
  a owl:Class, owl:NamedIndividual, <https://w3id.org/dpv/owl#Processing> ;
  rdfs:subClassOf <https://w3id.org/dpv/owl#Use> ;
  dc:contributor _:genid1 ;
  dc:created "2022-04-20"^^xsd:date ;
  dc:source [
    a ns0:WebPage ;
    ns0:name "A29WP WP 248 rev.01 Guideliens on DPIA" ;
    ns0:url "https://ec.europa.eu/newsroom/article29/items/611236"
  ] ;
  ns1:term_status "accepted"@en ;
  skos:definition "to combine, compare, or match data from different sources"@en ;
  skos:prefLabel "Match Data"@en ;
  owl:sameAs <https://w3id.org/dpv#Match>, <https://w3id.org/dpv/dpv-owl#Match> .

<https://w3id.org/dpv/owl#RecruitmentInterviewManagement>
  a owl:Class, owl:NamedIndividual, <https://w3id.org/dpv/owl#Purpose> ;
  rdfs:subClassOf <https://w3id.org/dpv/owl#RecruitmentManagement> ;
  dc:created "2024-12-01"^^xsd:date ;
  ns1:term_status "accepted"@en ;
  skos:definition "Purposes associated conducting and managing interviews for recruitment"@en ;
  skos:prefLabel "Recruitment Interview Management"@en ;
  owl:sameAs <https://w3id.org/dpv#RecruitmentInterviewManagement>, <https://w3id.org/dpv/dpv-owl#RecruitmentInterviewManagement> .

<https://w3id.org/dpv/owl#hasPermission>
  a owl:ObjectProperty ;
  rdfs:subPropertyOf <https://w3id.org/dpv/owl#hasRule> ;
  ns2:domainIncludes <https://w3id.org/dpv/owl#Context> ;
  ns2:rangeIncludes <https://w3id.org/dpv/owl#Permission> ;
  dc:contributor _:genid4, _:genid5, _:genid1, _:genid6 ;
  dc:created "2022-10-19"^^xsd:date ;
  ns3:example <https://w3id.org/dpv/examples/owl#E0066> ;
  ns1:term_status "accepted"@en ;
  skos:definition "Specifying applicability or inclusion of a permission rule within specified context"@en ;
  skos:prefLabel "has permission"@en ;
  ns0:domainIncludes <https://w3id.org/dpv/owl#Context> ;
  ns0:rangeIncludes <https://w3id.org/dpv/owl#Permission> ;
  owl:sameAs <https://w3id.org/dpv#hasPermission>, <https://w3id.org/dpv/dpv-owl#hasPermission> .

<https://w3id.org/dpv/owl#ProtectionOfPublicSecurity>
  a owl:Class, owl:NamedIndividual, <https://w3id.org/dpv/owl#Purpose> ;
  rdfs:subClassOf <https://w3id.org/dpv/owl#PublicBenefit> ;
  dc:contributor _:genid5, _:genid1 ;
  dc:created "2024-02-14"^^xsd:date ;
  dc:source "DGA 3.2(d)"@en ;
  ns1:term_status "accepted"@en ;
  skos:definition "Purposes associated with the protection of public security"@en ;
  skos:prefLabel "Protection of Public Security"@en ;
  owl:sameAs <https://w3id.org/dpv#ProtectionOfPublicSecurity>, <https://w3id.org/dpv/dpv-owl#ProtectionOfPublicSecurity> .

<https://w3id.org/dpv/owl#Citizen>
  a owl:Class, owl:NamedIndividual, <https://w3id.org/dpv/owl#HumanSubject> ;
  rdfs:subClassOf <https://w3id.org/dpv/owl#HumanSubject> ;
  dc:contributor _:genid4, _:genid5, _:genid1, _:genid17, _:genid6 ;
  dc:created "2022-04-06"^^xsd:date ;
  dc:modified "2024-12-17"^^xsd:date ;
  ns1:term_status "modified"@en ;
  skos:definition "Humans that are citizens (for a jurisdiction)"@en ;
  skos:prefLabel "Citizen"@en ;
  owl:sameAs <https://w3id.org/dpv#Citizen>, <https://w3id.org/dpv/dpv-owl#Citizen> .

<https://w3id.org/dpv/owl#OptimisationForController>
  a owl:Class, owl:NamedIndividual, <https://w3id.org/dpv/owl#Purpose> ;
  rdfs:subClassOf <https://w3id.org/dpv/owl#ServiceOptimisation> ;
  dc:contributor _:genid13, _:genid14, _:genid1, _:genid15, _:genid16, _:genid11 ;
  dc:created "2019-04-05"^^xsd:date ;
  ns1:term_status "accepted"@en ;
  skos:definition "Purposes associated with optimisation of activities and services for provider or controller"@en ;
  skos:prefLabel "Optimisation for Controller"@en ;
  owl:sameAs <https://w3id.org/dpv#OptimisationForController>, <https://w3id.org/dpv/dpv-owl#OptimisationForController> .

<https://w3id.org/dpv/owl#hasHumanSubject>
  a owl:ObjectProperty ;
  rdfs:subPropertyOf <https://w3id.org/dpv/owl#hasEntity> ;
  ns2:rangeIncludes <https://w3id.org/dpv/owl#HumanSubject> ;
  dc:contributor _:genid1 ;
  dc:created "2024-12-17"^^xsd:date ;
  ns3:example <https://w3id.org/dpv/examples/owl#E0074> ;
  ns1:term_status "accepted"@en ;
  skos:definition "Indicates association with Human Subject"@en ;
  skos:prefLabel "has human subject"@en ;
  ns0:rangeIncludes <https://w3id.org/dpv/owl#HumanSubject> ;
  owl:sameAs <https://w3id.org/dpv#hasHumanSubject>, <https://w3id.org/dpv/dpv-owl#hasHumanSubject> .

<https://w3id.org/dpv/owl#ServicePersonalisation>
  a owl:Class, owl:NamedIndividual, <https://w3id.org/dpv/owl#Purpose> ;
  rdfs:subClassOf <https://w3id.org/dpv/owl#Personalisation>, <https://w3id.org/dpv/owl#ServiceProvision> ;
  dc:contributor _:genid13, _:genid14, _:genid1, _:genid15, _:genid16, _:genid11 ;
  dc:created "2019-04-05"^^xsd:date ;
  ns1:term_status "accepted"@en ;
  skos:definition "Purposes associated with providing personalisation within services or product or activities"@en ;
  skos:prefLabel "Service Personalisation"@en ;
  owl:sameAs <https://w3id.org/dpv#ServicePersonalisation>, <https://w3id.org/dpv/dpv-owl#ServicePersonalisation> .

<https://w3id.org/dpv/owl#WithinDevice>
  a owl:Class, owl:NamedIndividual, <https://w3id.org/dpv/owl#Location> ;
  rdfs:subClassOf <https://w3id.org/dpv/owl#LocalLocation> ;
  dc:contributor _:genid1 ;
  dc:created "2022-06-15"^^xsd:date ;
  dc:modified "2020-10-05"^^xsd:date ;
  ns1:term_status "accepted"@en ;
  skos:definition "Location is local and entirely within a device, such as a smartphone"@en ;
  skos:prefLabel "Within Device"@en ;
  owl:sameAs <https://w3id.org/dpv#WithinDevice>, <https://w3id.org/dpv/dpv-owl#WithinDevice> .

odrl:translate
  a owl:NamedIndividual, skos:Concept, odrl:Action ;
  odrl:includedIn odrl:use ;
  rdfs:isDefinedBy odrl: ;
  rdfs:label "Translate"@en ;
  skos:definition "To translate the original natural language of an Asset into another natural language."@en ;
  skos:note "A new derivative Asset is created by that action."@en ;
  skos:scopeNote "Non-Normative"@en .

<https://w3id.org/dpv/owl#AcademicResearch>
  a owl:Class, owl:NamedIndividual, <https://w3id.org/dpv/owl#Purpose> ;
  rdfs:subClassOf <https://w3id.org/dpv/owl#ResearchAndDevelopment> ;
  dc:contributor _:genid13, _:genid14, _:genid1, _:genid15, _:genid16, _:genid11 ;
  dc:created "2019-04-05"^^xsd:date ;
  ns1:term_status "accepted"@en ;
  skos:definition "Purposes associated with conducting or assisting with research conducted in an academic context e.g. within universities"@en ;
  skos:prefLabel "Academic Research"@en ;
  skos:related <https://specialprivacy.ercim.eu/vocabs/purposes#Education> ;
  owl:sameAs <https://w3id.org/dpv#AcademicResearch>, <https://w3id.org/dpv/dpv-owl#AcademicResearch> .

<https://w3id.org/dpv/owl#Location>
  a owl:Class ;
  rdfs:subClassOf rdfs:Class ;
  dc:contributor _:genid4, _:genid1 ;
  dc:created "2022-01-19"^^xsd:date ;
  ns3:example <https://w3id.org/dpv/examples/owl#E0060> ;
  ns1:term_status "accepted"@en ;
  skos:definition "A location is a position, site, or area where something is located"@en ;
  skos:prefLabel "Location"@en ;
  skos:scopeNote "Location may be geographic, physical, or virtual."@en ;
  owl:sameAs <https://w3id.org/dpv#Location>, <https://w3id.org/dpv/dpv-owl#Location> .

<https://w3id.org/dpv/owl#Advertising>
  a owl:Class, owl:NamedIndividual, <https://w3id.org/dpv/owl#Purpose> ;
  rdfs:subClassOf <https://w3id.org/dpv/owl#Marketing> ;
  dc:contributor _:genid4, _:genid5, _:genid1 ;
  dc:created "2020-11-04"^^xsd:date ;
  ns1:term_status "accepted"@en ;
  skos:definition "Purposes associated with conducting advertising i.e. process or artefact used to call attention to a product, service, etc. through announcements, notices, or other forms of communication"@en ;
  skos:prefLabel "Advertising"@en ;
  skos:scopeNote "Advertising is a subset of Marketing. Advertising by itself does not indicate 'personalisation' i.e. personalised ads."@en ;
  owl:sameAs <https://w3id.org/dpv#Advertising>, <https://w3id.org/dpv/dpv-owl#Advertising> .

odrl:informingParty
  a owl:ObjectProperty, owl:NamedIndividual, skos:Concept ;
  rdfs:subPropertyOf odrl:function ;
  rdfs:isDefinedBy odrl: ;
  rdfs:label "Informing Party"@en ;
  skos:definition "The Party who provides the inform use data."@en ;
  skos:note "Maybe specified as part of the inform action."@en ;
  skos:scopeNote "Non-Normative"@en .

<https://w3id.org/dpv/owl#ContractExpired>
  a owl:Class, owl:NamedIndividual, <https://w3id.org/dpv/owl#ContractTerminationStatus> ;
  rdfs:subClassOf <https://w3id.org/dpv/owl#ContractTerminationStatus> ;
  dc:contributor _:genid4, _:genid1, _:genid17 ;
  dc:created "2025-01-09"^^xsd:date ;
  ns1:term_status "accepted"@en ;
  skos:definition "Status representing reaching the expiry defined in the contract, such as when the stated duration or the stated obligations have been completed"@en ;
  skos:prefLabel "Contract Expired"@en ;
  owl:sameAs <https://w3id.org/dpv#ContractExpired>, <https://w3id.org/dpv/dpv-owl#ContractExpired> .

<https://w3id.org/dpv/owl#Transfer>
  a owl:Class, owl:NamedIndividual, <https://w3id.org/dpv/owl#Processing> ;
  rdfs:subClassOf <https://w3id.org/dpv/owl#Processing> ;
  dc:created "2019-05-07"^^xsd:date ;
  dc:source [
    a ns0:WebPage ;
    ns0:name "SPECIAL Project" ;
    ns0:url "https://specialprivacy.ercim.eu/vocabs/processing"
  ] ;
  ns3:example <https://w3id.org/dpv/examples/owl#E0035> ;
  ns1:term_status "accepted"@en ;
  skos:definition "to move data from one place to another"@en ;
  skos:prefLabel "Transfer Data"@en ;
  skos:related <https://specialprivacy.ercim.eu/vocabs/processing#Transfer> ;
  owl:sameAs <https://w3id.org/dpv#Transfer>, <https://w3id.org/dpv/dpv-owl#Transfer> .

<https://w3id.org/dpv/owl#LicenseAgreement>
  a owl:Class, owl:NamedIndividual, <https://w3id.org/dpv/owl#LegalBasis> ;
  rdfs:subClassOf <https://w3id.org/dpv/owl#ContractByDomain> ;
  dc:created "2024-08-27"^^xsd:date ;
  ns1:term_status "accepted"@en ;
  skos:definition "A Legal Document providing permission to utilise data or resource and outlining the conditions under which such use is considered valid"@en ;
  skos:prefLabel "License Agreement"@en ;
  owl:sameAs <https://w3id.org/dpv#LicenseAgreement>, <https://w3id.org/dpv/dpv-owl#LicenseAgreement> .

<https://w3id.org/dpv/owl#hasNoticeLayer>
  a owl:ObjectProperty ;
  ns2:domainIncludes <https://w3id.org/dpv/owl#Notice>, <https://w3id.org/dpv/owl#NoticeLayer> ;
  ns2:rangeIncludes <https://w3id.org/dpv/owl#NoticeLayer> ;
  dc:created "2024-08-17"^^xsd:date ;
  ns3:example <https://w3id.org/dpv/examples/owl#E0072> ;
  ns1:term_status "accepted"@en ;
  skos:definition "Indicates the use of a notice layer within a notice or to associate a layer with another layer"@en ;
  skos:prefLabel "has notice layer"@en ;
  ns0:domainIncludes <https://w3id.org/dpv/owl#Notice>, <https://w3id.org/dpv/owl#NoticeLayer> ;
  ns0:rangeIncludes <https://w3id.org/dpv/owl#NoticeLayer> ;
  owl:sameAs <https://w3id.org/dpv#hasNoticeLayer>, <https://w3id.org/dpv/dpv-owl#hasNoticeLayer> .

<https://w3id.org/dpv/owl#ConsentStatusInvalidForProcessing>
  a owl:Class, owl:NamedIndividual, <https://w3id.org/dpv/owl#ConsentStatus> ;
  rdfs:subClassOf <https://w3id.org/dpv/owl#ConsentStatus> ;
  dc:contributor _:genid4, _:genid1, _:genid17, _:genid6 ;
  dc:created "2022-06-22"^^xsd:date ;
  dc:source [
    a ns0:WebPage ;
    ns0:name "GConsent" ;
    ns0:url "https://w3id.org/GConsent"
  ] ;
  ns1:term_status "accepted"@en ;
  skos:definition "States of consent that cannot be used as valid justifications for processing data"@en ;
  skos:prefLabel "Consent Status Invalid for Processing"@en ;
  skos:scopeNote "This identifies the stages associated with consent that should not be used to process data"@en ;
  owl:sameAs <https://w3id.org/dpv#ConsentStatusInvalidForProcessing>, <https://w3id.org/dpv/dpv-owl#ConsentStatusInvalidForProcessing> .

<http://www.w3.org/ns/dx/prof/hasRole> a owl:AnnotationProperty .
<https://w3id.org/dpv/owl#ConsentRefused>
  a owl:Class, owl:NamedIndividual, <https://w3id.org/dpv/owl#ConsentStatus> ;
  rdfs:subClassOf <https://w3id.org/dpv/owl#ConsentStatusInvalidForProcessing> ;
  dc:contributor _:genid4, _:genid1, _:genid17, _:genid6 ;
  dc:created "2022-06-22"^^xsd:date ;
  dc:source [
    a ns0:WebPage ;
    ns0:name "GConsent" ;
    ns0:url "https://w3id.org/GConsent"
  ] ;
  ns1:term_status "accepted"@en ;
  skos:definition "The state where consent has been refused"@en ;
  skos:prefLabel "Consent Refused"@en ;
  skos:scopeNote "An example of this state is when the individual clicks on a 'disagree' or 'reject' or 'refuse' button, or leaves a checkbox unticked"@en ;
  owl:sameAs <https://w3id.org/dpv#ConsentRefused>, <https://w3id.org/dpv/dpv-owl#ConsentRefused> .

<https://w3id.org/dpv/owl#Permission>
  a owl:Class, owl:NamedIndividual, <https://w3id.org/dpv/owl#Rule> ;
  rdfs:subClassOf <https://w3id.org/dpv/owl#Rule> ;
  dc:contributor _:genid4, _:genid5, _:genid1, _:genid6 ;
  dc:created "2022-10-19"^^xsd:date ;
  ns3:example <https://w3id.org/dpv/examples/owl#E0028>, <https://w3id.org/dpv/examples/owl#E0066> ;
  ns1:term_status "accepted"@en ;
  skos:definition "A rule describing a permission to perform an activity"@en ;
  skos:prefLabel "Permission"@en ;
  owl:sameAs <https://w3id.org/dpv#Permission>, <https://w3id.org/dpv/dpv-owl#Permission> .

<https://w3id.org/dpv/owl#HumanSubject>
  a owl:Class ;
  rdfs:subClassOf <https://w3id.org/dpv/owl#LegalEntity> ;
  dc:contributor _:genid1, _:genid25 ;
  dc:created "2024-12-17"^^xsd:date ;
  ns3:example <https://w3id.org/dpv/examples/owl#E0074> ;
  ns1:term_status "accepted"@en ;
  skos:definition "The individual (or category of individuals) that is the subject within some context such as personal data (dpv:DataSubject) or technology (tech:Subject)"@en ;
  skos:prefLabel "Human Subject"@en ;
  owl:sameAs <https://w3id.org/dpv#HumanSubject>, <https://w3id.org/dpv/dpv-owl#HumanSubject> .

<https://w3id.org/dpv/owl#DataRedaction>
  a owl:Class, owl:NamedIndividual, <https://w3id.org/dpv/owl#TechnicalMeasure> ;
  rdfs:subClassOf <https://w3id.org/dpv/owl#DataSanitisationTechnique> ;
  dc:contributor _:genid1 ;
  dc:created "2020-10-01"^^xsd:date ;
  ns1:term_status "accepted"@en ;
  skos:definition "Removal of sensitive information from a data or document"@en ;
  skos:prefLabel "Data Redaction"@en ;
  owl:sameAs <https://w3id.org/dpv#DataRedaction>, <https://w3id.org/dpv/dpv-owl#DataRedaction> .

<https://w3id.org/dpv/owl#ResidualRisk>
  a owl:Class ;
  rdfs:subClassOf <https://w3id.org/dpv/owl#Risk> ;
  dc:contributor _:genid1 ;
  dc:created "2024-06-16"^^xsd:date ;
  ns3:example <https://w3id.org/dpv/examples/owl#E0068> ;
  ns1:term_status "accepted"@en ;
  skos:definition "Risk remaining after treatment or mitigation"@en ;
  skos:prefLabel "Residual Risk"@en ;
  owl:sameAs <https://w3id.org/dpv#ResidualRisk>, <https://w3id.org/dpv/dpv-owl#ResidualRisk> .

odrl:count
  a owl:NamedIndividual, skos:Concept, odrl:LeftOperand ;
  rdfs:isDefinedBy odrl: ;
  rdfs:label "Count"@en ;
  skos:definition "Numeric count of executions of the action of the Rule."@en ;
  skos:scopeNote "Non-Normative"@en .

<https://w3id.org/dpv/owl#PersonnelBehaviourMonitoring>
  a owl:Class, owl:NamedIndividual, <https://w3id.org/dpv/owl#Purpose> ;
  rdfs:subClassOf <https://w3id.org/dpv/owl#PersonnelMonitoring> ;
  dc:created "2024-12-01"^^xsd:date ;
  ns1:term_status "accepted"@en ;
  skos:definition "Purposes associated with monitoring behaviour of personnel"@en ;
  skos:prefLabel "Personnel Behaviour Monitoring"@en ;
  owl:sameAs <https://w3id.org/dpv#PersonnelBehaviourMonitoring>, <https://w3id.org/dpv/dpv-owl#PersonnelBehaviourMonitoring> .

<https://w3id.org/dpv/owl#DataSubjectRight>
  a owl:Class, owl:NamedIndividual, <https://w3id.org/dpv/owl#Right> ;
  rdfs:subClassOf <https://w3id.org/dpv/owl#Right> ;
  dc:contributor _:genid4, _:genid5, _:genid1 ;
  dc:created "2020-11-18"^^xsd:date ;
  ns1:term_status "accepted"@en ;
  skos:definition "The rights applicable or provided to a Data Subject"@en ;
  skos:prefLabel "Data Subject Right"@en ;
  skos:scopeNote "Based on use of definitions, the notion of 'Data Subject Right' can be equivalent to 'Individual Right' or 'Right of a Person'"@en ;
  owl:sameAs <https://w3id.org/dpv#DataSubjectRight>, <https://w3id.org/dpv/dpv-owl#DataSubjectRight> .

<https://w3id.org/dpv/owl#ContractFullyExecuted>
  a owl:Class, owl:NamedIndividual, <https://w3id.org/dpv/owl#ContractExecutionStatus> ;
  rdfs:subClassOf <https://w3id.org/dpv/owl#ContractExecutionStatus> ;
  dc:contributor _:genid4, _:genid1, _:genid17 ;
  dc:created "2025-01-09"^^xsd:date ;
  ns1:term_status "accepted"@en ;
  skos:definition "Status representing contract has been fully executed i.e. it has been signed by all parties and all other procedural aspects such as exchange of signed contract copies have been completed"@en ;
  skos:prefLabel "Contract Fully Executed"@en ;
  owl:sameAs <https://w3id.org/dpv#ContractFullyExecuted>, <https://w3id.org/dpv/dpv-owl#ContractFullyExecuted> .

<https://w3id.org/dpv/owl#AuthorisationProcedure>
  a owl:Class, owl:NamedIndividual, <https://w3id.org/dpv/owl#OrganisationalMeasure> ;
  rdfs:subClassOf <https://w3id.org/dpv/owl#SecurityProcedure> ;
  dc:contributor _:genid9, _:genid10, _:genid1, _:genid11 ;
  dc:created "2019-04-05"^^xsd:date ;
  ns1:term_status "accepted"@en ;
  skos:definition "Procedures for determining authorisation through permission or authority"@en ;
  skos:prefLabel "Authorisation Procedure"@en ;
  skos:scopeNote "non-technical authorisation procedures: How is it described on an organisational level, who gets access to the data"@en ;
  owl:sameAs <https://w3id.org/dpv#AuthorisationProcedure>, <https://w3id.org/dpv/dpv-owl#AuthorisationProcedure> .

<https://w3id.org/dpv/owl#VitalInterestPending>
  a owl:Class, owl:NamedIndividual, <https://w3id.org/dpv/owl#VitalInterestStatus> ;
  rdfs:subClassOf <https://w3id.org/dpv/owl#VitalInterestStatus> ;
  dc:created "2024-08-27"^^xsd:date ;
  ns1:term_status "accepted"@en ;
  skos:definition "Status where the vital interest activity has not started"@en ;
  skos:prefLabel "Vital Interest Pending"@en ;
  owl:sameAs <https://w3id.org/dpv#VitalInterestPending>, <https://w3id.org/dpv/dpv-owl#VitalInterestPending> .

<https://w3id.org/dpv/owl#SystematicMonitoring>
  a owl:Class, owl:NamedIndividual, <https://w3id.org/dpv/owl#ProcessingContext> ;
  rdfs:subClassOf <https://w3id.org/dpv/owl#ProcessingContext> ;
  dc:contributor _:genid1, _:genid2 ;
  dc:created "2020-11-04"^^xsd:date ;
  dc:source [
    a ns0:WebPage ;
    ns0:name "GDPR Art.4-2" ;
    ns0:url "https://eur-lex.europa.eu/eli/reg/2016/679/art_4/par_2/oj"
  ] ;
  ns1:term_status "accepted"@en ;
  skos:definition "Processing that involves systematic monitoring of individuals"@en ;
  skos:prefLabel "Systematic Monitoring"@en ;
  owl:sameAs <https://w3id.org/dpv#SystematicMonitoring>, <https://w3id.org/dpv/dpv-owl#SystematicMonitoring> .

<https://w3id.org/dpv/owl#NonGovernmentalOrganisation>
  a owl:Class ;
  rdfs:subClassOf <https://w3id.org/dpv/owl#Organisation> ;
  dc:contributor _:genid1 ;
  dc:created "2022-02-02"^^xsd:date ;
  dc:modified "2020-10-05"^^xsd:date ;
  dc:source [
    a ns0:WebPage ;
    ns0:name "ADMS controlled vocabulary" ;
    ns0:url "http://purl.org/adms"
  ] ;
  ns1:term_status "accepted"@en ;
  skos:definition "An organisation not part of or independent from the government"@en ;
  skos:prefLabel "Non-Governmental Organisation"@en ;
  owl:sameAs <https://w3id.org/dpv#NonGovernmentalOrganisation>, <https://w3id.org/dpv/dpv-owl#NonGovernmentalOrganisation> .

<https://w3id.org/dpv/owl#Policy>
  a owl:Class, owl:NamedIndividual, <https://w3id.org/dpv/owl#OrganisationalMeasure> ;
  rdfs:subClassOf <https://w3id.org/dpv/owl#GovernanceProcedures> ;
  dc:contributor _:genid4, _:genid1, _:genid6, _:genid21 ;
  dc:created "2021-09-08"^^xsd:date ;
  ns1:term_status "accepted"@en ;
  skos:definition "A guidance document outlining any of: procedures, plans, principles, decisions, intent, or protocols."@en ;
  skos:prefLabel "Policy"@en ;
  owl:sameAs <https://w3id.org/dpv#Policy>, <https://w3id.org/dpv/dpv-owl#Policy> .

<https://w3id.org/dpv/owl#CustomerRelationshipManagement>
  a owl:Class, owl:NamedIndividual, <https://w3id.org/dpv/owl#Purpose> ;
  rdfs:subClassOf <https://w3id.org/dpv/owl#CustomerManagement> ;
  dc:contributor _:genid4, _:genid5, _:genid1 ;
  dc:created "2021-09-08"^^xsd:date ;
  ns1:term_status "accepted"@en ;
  skos:definition "Customer Relationship Management refers to purposes associated with managing and analysing interactions with past, current, and potential customers"@en ;
  skos:prefLabel "Customer Relationship Management"@en ;
  owl:sameAs <https://w3id.org/dpv#CustomerRelationshipManagement>, <https://w3id.org/dpv/dpv-owl#CustomerRelationshipManagement> .

<https://w3id.org/dpv/owl#RecruitmentApplicantBackgroundCheck>
  a owl:Class, owl:NamedIndividual, <https://w3id.org/dpv/owl#Purpose> ;
  rdfs:subClassOf <https://w3id.org/dpv/owl#RecruitmentManagement> ;
  dc:created "2024-12-01"^^xsd:date ;
  ns1:term_status "accepted"@en ;
  skos:definition "Purposes assocaited with conducting background checks for prospective and current job applicants for recruitment"@en ;
  skos:prefLabel "Recruitment Applicant Background Check"@en ;
  owl:sameAs <https://w3id.org/dpv#RecruitmentApplicantBackgroundCheck>, <https://w3id.org/dpv/dpv-owl#RecruitmentApplicantBackgroundCheck> .

<https://w3id.org/dpv/owl#ProvideProductRecommendations>
  a owl:Class, owl:NamedIndividual, <https://w3id.org/dpv/owl#Purpose> ;
  rdfs:subClassOf <https://w3id.org/dpv/owl#ProvidePersonalisedRecommendations> ;
  dc:contributor _:genid13, _:genid14, _:genid1, _:genid15, _:genid16, _:genid11 ;
  dc:created "2019-04-05"^^xsd:date ;
  dc:modified "2022-10-14"^^xsd:date ;
  ns1:term_status "accepted"@en ;
  skos:definition "Purposes associated with creating and providing product recommendations e.g. suggest similar products"@en ;
  skos:prefLabel "Provide Product Recommendations"@en ;
  skos:related <https://specialprivacy.ercim.eu/vocabs/purposes#Marketing> ;
  owl:sameAs <https://w3id.org/dpv#ProvideProductRecommendations>, <https://w3id.org/dpv/dpv-owl#ProvideProductRecommendations> .

<https://w3id.org/dpv/owl#SensitivityLevel>
  a owl:Class ;
  rdfs:subClassOf <https://w3id.org/dpv/owl#Severity> ;
  dc:contributor _:genid1 ;
  dc:created "2023-08-24"^^xsd:date ;
  ns1:term_status "accepted"@en ;
  skos:definition "Sensitivity' reflects the risk of impact if not secured or utilised with appropriate measures and controls e.g. for sensitive data"@en ;
  skos:prefLabel "Sensitivity Level"@en ;
  skos:scopeNote "ISO/IEC TS 38505-3:2021 defines 'data sensitivity' as the potential harm of unauthorised disclosure. DPV's use of the concept goes beyond disclosure as it refers to the level of safeguards or controls the data requires as a reflection of its 'sensitive' nature. To indicate quantified levels of sensitivity, e.g. \"high sensitivity\", instances of severity can be directly used or specialised"@en ;
  owl:sameAs <https://w3id.org/dpv#SensitivityLevel>, <https://w3id.org/dpv/dpv-owl#SensitivityLevel> .

<https://w3id.org/dpv/owl#hasRight>
  a owl:ObjectProperty, owl:NamedIndividual, odrl:LeftOperand ;
  ns2:rangeIncludes <https://w3id.org/dpv/owl#Right> ;
  dc:contributor _:genid1 ;
  dc:created "2020-11-18"^^xsd:date ;
  ns3:example <https://w3id.org/dpv/examples/owl#E0061>, <https://w3id.org/dpv/examples/owl#E0067> ;
  ns1:term_status "accepted"@en ;
  skos:definition "Indicates use or applicability of Right"@en ;
  skos:prefLabel "has right"@en ;
  ns0:rangeIncludes <https://w3id.org/dpv/owl#Right> ;
  owl:sameAs <https://w3id.org/dpv#hasRight>, <https://w3id.org/dpv/dpv-owl#hasRight> .

<https://w3id.org/dpv/owl#OfficialAuthorityOfController>
  a owl:Class, owl:NamedIndividual, <https://w3id.org/dpv/owl#LegalBasis> ;
  rdfs:subClassOf <https://w3id.org/dpv/owl#LegalBasis> ;
  dc:contributor _:genid4, _:genid1, _:genid6 ;
  dc:created "2021-05-05"^^xsd:date ;
  ns3:example <https://w3id.org/dpv/examples/owl#E0081> ;
  ns1:term_status "accepted"@en ;
  skos:definition "Activities are necessary or authorised through the official authority granted to or vested in the Data Controller"@en ;
  skos:prefLabel "Official Authority of Controller"@en ;
  owl:sameAs <https://w3id.org/dpv#OfficialAuthorityOfController>, <https://w3id.org/dpv/dpv-owl#OfficialAuthorityOfController> .

<https://w3id.org/dpv/owl#ThirdPartyAgreement>
  a owl:Class, owl:NamedIndividual, <https://w3id.org/dpv/owl#LegalBasis>, <https://w3id.org/dpv/owl#LegalMeasure> ;
  rdfs:subClassOf <https://w3id.org/dpv/owl#ThirdPartyContract> ;
  dc:contributor _:genid1 ;
  dc:created "2022-02-09"^^xsd:date ;
  dc:modified "2024-08-27"^^xsd:date ;
  ns1:term_status "modified"@en ;
  skos:definition "An agreement outlining conditions, criteria, obligations, responsibilities, and specifics for carrying out processing of data between a Data Controller or Processor and a Third Party"@en ;
  skos:prefLabel "Third-Party Agreement"@en ;
  owl:sameAs <https://w3id.org/dpv#ThirdPartyAgreement>, <https://w3id.org/dpv/dpv-owl#ThirdPartyAgreement> .

<https://w3id.org/dpv/owl#StorageLocation>
  a owl:Class ;
  rdfs:subClassOf <https://w3id.org/dpv/owl#ProcessingLocation>, <https://w3id.org/dpv/owl#StorageCondition> ;
  dc:contributor _:genid9, _:genid10, _:genid1, _:genid11 ;
  dc:created "2019-04-05"^^xsd:date ;
  ns3:example <https://w3id.org/dpv/examples/owl#E0048> ;
  ns1:term_status "accepted"@en ;
  skos:definition "Location or geospatial scope where the data is stored"@en ;
  skos:prefLabel "Storage Location"@en ;
  owl:sameAs <https://w3id.org/dpv#StorageLocation>, <https://w3id.org/dpv/dpv-owl#StorageLocation> .

<https://w3id.org/dpv/owl#NotRequired>
  a owl:Class, owl:NamedIndividual, <https://w3id.org/dpv/owl#Necessity> ;
  rdfs:subClassOf <https://w3id.org/dpv/owl#Necessity> ;
  dc:contributor _:genid4, _:genid5, _:genid1, _:genid17, _:genid6 ;
  dc:created "2022-02-15"^^xsd:date ;
  ns1:term_status "accepted"@en ;
  skos:definition "Indication of neither being required nor optional i.e. not relevant or needed"@en ;
  skos:prefLabel "Not Required"@en ;
  owl:sameAs <https://w3id.org/dpv#NotRequired>, <https://w3id.org/dpv/dpv-owl#NotRequired> .

<https://w3id.org/dpv/owl#IncidentManagementProcedures>
  a owl:Class, owl:NamedIndividual, <https://w3id.org/dpv/owl#OrganisationalMeasure> ;
  rdfs:subClassOf <https://w3id.org/dpv/owl#GovernanceProcedures> ;
  dc:contributor _:genid1 ;
  dc:created "2022-08-17"^^xsd:date ;
  dc:source [
    a ns0:WebPage ;
    ns0:name "ENISA 5G Cybersecurity Standards" ;
    ns0:url "https://www.enisa.europa.eu/publications/5g-cybersecurity-standards"
  ] ;
  ns1:term_status "accepted"@en ;
  skos:definition "Procedures related to management of incidents"@en ;
  skos:prefLabel "Incident Management Procedures"@en ;
  owl:sameAs <https://w3id.org/dpv#IncidentManagementProcedures>, <https://w3id.org/dpv/dpv-owl#IncidentManagementProcedures> .

<https://w3id.org/dpv/owl#DistributionAgreement>
  a owl:Class, owl:NamedIndividual, <https://w3id.org/dpv/owl#LegalBasis> ;
  rdfs:subClassOf <https://w3id.org/dpv/owl#ContractByDomain> ;
  dc:created "2024-08-27"^^xsd:date ;
  ns1:term_status "accepted"@en ;
  skos:definition "A contract regarding supply of data or technologies between a distributor and a supplier"@en ;
  skos:prefLabel "Distribution Agreement"@en ;
  owl:sameAs <https://w3id.org/dpv#DistributionAgreement>, <https://w3id.org/dpv/dpv-owl#DistributionAgreement> .

<https://w3id.org/dpv/owl#NotificationPlanned>
  a owl:Class, owl:NamedIndividual, <https://w3id.org/dpv/owl#NotificationStatus> ;
  rdfs:subClassOf <https://w3id.org/dpv/owl#NotificationStatus> ;
  dc:contributor _:genid1 ;
  dc:created "2024-05-19"^^xsd:date ;
  ns1:term_status "accepted"@en ;
  skos:definition "Status indicating notification(s) are planned"@en ;
  skos:prefLabel "Notification Planned"@en ;
  owl:sameAs <https://w3id.org/dpv#NotificationPlanned>, <https://w3id.org/dpv/dpv-owl#NotificationPlanned> .

<https://w3id.org/dpv/owl#IdentityVerification>
  a owl:Class, owl:NamedIndividual, <https://w3id.org/dpv/owl#Purpose> ;
  rdfs:subClassOf <https://w3id.org/dpv/owl#Verification> ;
  dc:contributor _:genid13, _:genid14, _:genid1, _:genid15, _:genid16, _:genid11 ;
  dc:created "2019-04-05"^^xsd:date ;
  ns1:term_status "accepted"@en ;
  skos:definition "Purposes associated with verifying or authenticating identity as a form of security"@en ;
  skos:prefLabel "Identity Verification"@en ;
  owl:sameAs <https://w3id.org/dpv#IdentityVerification>, <https://w3id.org/dpv/dpv-owl#IdentityVerification> .

<https://w3id.org/dpv/owl#UseSyntheticData>
  a owl:Class, owl:NamedIndividual, <https://w3id.org/dpv/owl#TechnicalMeasure> ;
  rdfs:subClassOf <https://w3id.org/dpv/owl#SecurityMethod> ;
  dc:contributor _:genid1 ;
  dc:created "2022-08-17"^^xsd:date ;
  dc:source [
    a ns0:WebPage ;
    ns0:name "ENISA Data Protection Engineering" ;
    ns0:url "https://www.enisa.europa.eu/publications/data-protection-engineering"
  ] ;
  ns1:term_status "accepted"@en ;
  skos:definition "Use of synthetic data to preserve privacy, security, or other effects and side-effects"@en ;
  skos:prefLabel "Use of Synthetic Data"@en ;
  owl:sameAs <https://w3id.org/dpv#UseSyntheticData>, <https://w3id.org/dpv/dpv-owl#UseSyntheticData> .

<https://w3id.org/dpv/owl#CorrectingProcessOutput>
  a owl:Class, owl:NamedIndividual, <https://w3id.org/dpv/owl#EntityPermissiveInvolvement> ;
  rdfs:subClassOf <https://w3id.org/dpv/owl#EntityPermissiveInvolvement> ;
  dc:contributor _:genid1, _:genid25, _:genid19 ;
  dc:created "2024-05-11"^^xsd:date ;
  ns1:term_status "accepted"@en ;
  skos:definition "Involvement where entity can correct the output of specified context"@en ;
  skos:prefLabel "Correcting Process Output"@en ;
  skos:scopeNote "Correction of outputs allows modification of the output - implying continuation of the process. This is distinct from reversing of outputs which revert the output back to its previous value and possibly imply not continuing with the process"@en ;
  owl:sameAs <https://w3id.org/dpv#CorrectingProcessOutput>, <https://w3id.org/dpv/dpv-owl#CorrectingProcessOutput> .

<https://w3id.org/dpv/owl#HumanInvolvementForVerification>
  a owl:Class, owl:NamedIndividual, <https://w3id.org/dpv/owl#HumanInvolvement> ;
  rdfs:subClassOf <https://w3id.org/dpv/owl#HumanInvolvement> ;
  dc:contributor _:genid1 ;
  dc:created "2022-09-07"^^xsd:date ;
  dc:modified "2023-12-10"^^xsd:date ;
  ns1:term_status "accepted"@en ;
  skos:definition "Human involvement for the purposes of verification of specified context to ensure its operations, inputs, or outputs are correct or are acceptable."@en ;
  skos:prefLabel "Human Involvement for Verification"@en ;
  skos:scopeNote "Verification by itself does not imply ability to Control, Intervene, or having Oversight."@en ;
  owl:sameAs <https://w3id.org/dpv#HumanInvolvementForVerification>, <https://w3id.org/dpv/dpv-owl#HumanInvolvementForVerification> .

<https://w3id.org/dpv/owl#AssistiveAutomation>
  a owl:Class, owl:NamedIndividual, <https://w3id.org/dpv/owl#AutomationLevel> ;
  rdfs:subClassOf <https://w3id.org/dpv/owl#AutomationLevel> ;
  dc:contributor _:genid1, _:genid25 ;
  dc:created "2023-12-10"^^xsd:date ;
  dc:modified "2024-04-20"^^xsd:date ;
  dc:source [
    a ns0:WebPage ;
    ns0:name "ISO/IEC 22989:2022 Artificial intelligence concepts and terminology" ;
    ns0:url "https://www.iso.org/standard/74296.html"
  ] ;
  ns1:term_status "accepted"@en ;
  skos:definition "Level of automation corresponding to Level 1 in ISO/IEC 22989:2022 where automation is limited to parts of the system or a specific part of the system in a manner that does not change the control of the human in using/driving the system"@en ;
  skos:prefLabel "Assistive Automation"@en ;
  skos:scopeNote "Human Involvement is implied here, specifically the ability to make decisions regarding operations, but also possibly for intervention, oversight, and verification"@en ;
  owl:sameAs <https://w3id.org/dpv#AssistiveAutomation>, <https://w3id.org/dpv/dpv-owl#AssistiveAutomation> .

odrl:
  a owl:Ontology ;
  dc:bibliographicCitation "Harshvardhan J. Pandit, Beatriz Esteves, Georg P. Krog, Paul Ryan, Delaram Golpayegani, Julian Flake (2025) Data Privacy Vocabulary (DPV) – Version 2.0. In: Demartini, G., et al. The Semantic Web – ISWC 2024. ISWC 2024. Lecture Notes in Computer Science, vol 15233. Springer, Cham. https://doi.org/10.1007/978-3-031-77847-6_10" ;
  dc:conformsTo <http://www.w3.org/2002/07/owl>, "http://www.w3.org/2000/01/rdf-schema", "http://www.w3.org/2004/02/skos/core" ;
  dc:contributor _:genid13, _:genid64, _:genid14, _:genid65, _:genid4, _:genid5, _:genid9, _:genid31, _:genid10, _:genid66, _:genid56, _:genid1, _:genid67, _:genid25, _:genid17, _:genid19, _:genid6, _:genid15, _:genid16, _:genid11, _:genid2, _:genid68, _:genid21, "W3C Permissions & Obligations Expression Working Group" ;
  dc:created "2022-08-18"@en ;
  dc:creator _:genid4, _:genid5, _:genid1, _:genid25, _:genid17, _:genid6, "Michael Steidl", "Renato Iannella", "Stuart Myles", "Víctor Rodríguez-Doncel" ;
  dc:description "The Data Privacy Vocabulary (DPV) provides terms (classes and properties) to represent information about processing of personal data, for example - purposes, processing operations, personal data, technical and organisational measures."@en, "The ODRL Vocabulary and Expression defines a set of concepts and terms (the vocabulary) and encoding mechanism (the expression) for permissions and obligations statements describing digital content usage based on the ODRL Information Model."@en ;
  dc:identifier "https://w3id.org/dpv" ;
  dc:issued "2022-08-18"@en ;
  dc:license <https://www.w3.org/Consortium/Legal/2002/ipr-notice-20021231#Copyright/>, <https://www.w3.org/copyright/document-license-2023/> ;
  dc:modified "2025-02-01"@en ;
  dc:publisher <https://www.w3.org/> ;
  dc:source <https://www.w3.org/groups/cg/dpvcg/> ;
  dc:title "Data Privacy Vocabulary (DPV)"@en ;
  bibo:doi "10.5281/zenodo.12505841" ;
  bibo:status "http://purl.org/ontology/bibo/status/published" ;
  ns3:preferredNamespacePrefix "dpv" ;
  ns3:preferredNamespaceUri "https://w3id.org/dpv#" ;
  rdfs:comment "This is the RDF ontology for ODRL Version 2.2."@en ;
  rdfs:label "DPV"@en, "ODRL Version 2.2"@en ;
  owl:versionInfo "2.1", "2.2" ;
  ns4:hasResource <https://w3id.org/dpv/examples>, <https://w3id.org/dpv/guides>, <https://w3id.org/dpv/primer>, <https://w3id.org/dpv/owl#serialisation-html>, <https://w3id.org/dpv/owl#serialisation-jsonld>, <https://w3id.org/dpv/owl#serialisation-n3>, <https://w3id.org/dpv/owl#serialisation-rdf>, <https://w3id.org/dpv/owl#serialisation-ttl> ;
  ns4:isProfileOf <http://www.w3.org/2002/07/owl> ;
  foaf:logo <https://w3id.org/dpv/media/logo.png> ;
  ns0:version "2.1" .

<https://w3id.org/dpv/owl#UntilTimeDuration>
  a owl:Class ;
  rdfs:subClassOf <https://w3id.org/dpv/owl#Duration> ;
  dc:contributor _:genid1 ;
  dc:created "2022-06-15"^^xsd:date ;
  dc:modified "2020-10-05"^^xsd:date ;
  ns1:term_status "accepted"@en ;
  skos:definition "Duration that has a fixed end date e.g. 2022-12-31"@en ;
  skos:prefLabel "Until Time Duration"@en ;
  owl:sameAs <https://w3id.org/dpv#UntilTimeDuration>, <https://w3id.org/dpv/dpv-owl#UntilTimeDuration> .

<https://w3id.org/dpv/owl#ProhibitionViolated>
  a owl:Class, owl:NamedIndividual, <https://w3id.org/dpv/owl#RuleFulfilmentStatus> ;
  rdfs:subClassOf <https://w3id.org/dpv/owl#RuleViolated> ;
  dc:contributor _:genid1 ;
  dc:created "2024-09-10"^^xsd:date ;
  ns1:term_status "accepted"@en ;
  skos:definition "Status indicating a prohibition has been violated i.e. the activity stated as being prohibited has been carried out"@en ;
  skos:prefLabel "Prohibition Violated"@en ;
  owl:sameAs <https://w3id.org/dpv#ProhibitionViolated>, <https://w3id.org/dpv/dpv-owl#ProhibitionViolated> .

<https://w3id.org/dpv/owl#ElderlyHuman>
  a owl:Class, owl:NamedIndividual, <https://w3id.org/dpv/owl#HumanSubject> ;
  rdfs:subClassOf <https://w3id.org/dpv/owl#VulnerableHuman> ;
  dc:contributor _:genid1 ;
  dc:created "2024-12-17"^^xsd:date ;
  ns1:term_status "accepted"@en ;
  skos:definition "Humans that are considered elderly (i.e. based on age)"@en ;
  skos:prefLabel "Elderly Human"@en ;
  owl:sameAs <https://w3id.org/dpv#ElderlyHuman>, <https://w3id.org/dpv/dpv-owl#ElderlyHuman> .

<https://w3id.org/dpv/owl#isRepresentativeFor>
  a owl:ObjectProperty ;
  rdfs:subPropertyOf <https://w3id.org/dpv/owl#hasEntity> ;
  ns2:domainIncludes <https://w3id.org/dpv/owl#Representative> ;
  ns2:rangeIncludes <https://w3id.org/dpv/owl#Entity> ;
  dc:contributor _:genid1 ;
  dc:created "2022-11-09"^^xsd:date ;
  ns1:term_status "accepted"@en ;
  skos:definition "Indicates the entity is a representative for specified entity"@en ;
  skos:prefLabel "is representative for"@en ;
  ns0:domainIncludes <https://w3id.org/dpv/owl#Representative> ;
  ns0:rangeIncludes <https://w3id.org/dpv/owl#Entity> ;
  owl:sameAs <https://w3id.org/dpv#isRepresentativeFor>, <https://w3id.org/dpv/dpv-owl#isRepresentativeFor> .

<https://w3id.org/dpv/owl#Obtain>
  a owl:Class, owl:NamedIndividual, <https://w3id.org/dpv/owl#Processing> ;
  rdfs:subClassOf <https://w3id.org/dpv/owl#Processing> ;
  dc:created "2019-05-07"^^xsd:date ;
  dc:source [
    a ns0:WebPage ;
    ns0:name "GDPR Art.4-2" ;
    ns0:url "https://eur-lex.europa.eu/eli/reg/2016/679/art_4/par_2/oj"
  ] ;
  ns1:term_status "accepted"@en ;
  skos:definition "to solicit or gather data from someone"@en ;
  skos:prefLabel "Obtain Data"@en ;
  owl:sameAs <https://w3id.org/dpv#Obtain>, <https://w3id.org/dpv/dpv-owl#Obtain> .

<https://w3id.org/dpv/owl#PersonnelPayment>
  a owl:Class, owl:NamedIndividual, <https://w3id.org/dpv/owl#Purpose> ;
  rdfs:subClassOf <https://w3id.org/dpv/owl#PersonnelManagement> ;
  dc:contributor _:genid1 ;
  dc:created "2022-04-20"^^xsd:date ;
  ns1:term_status "accepted"@en ;
  skos:definition "Purposes associated with management and execution of payment of personnel"@en ;
  skos:prefLabel "Personnel Payment"@en ;
  owl:sameAs <https://w3id.org/dpv#PersonnelPayment>, <https://w3id.org/dpv/dpv-owl#PersonnelPayment> .

<https://w3id.org/dpv/owl#ContractControl>
  a owl:Class ;
  rdfs:subClassOf <https://w3id.org/dpv/owl#EntityInvolvement> ;
  dc:created "2024-08-27"^^xsd:date ;
  ns1:term_status "accepted"@en ;
  skos:definition "The control or activity associated with accepting, refusing, and other actions associated with a contract"@en ;
  skos:prefLabel "Contract Control"@en ;
  owl:sameAs <https://w3id.org/dpv#ContractControl>, <https://w3id.org/dpv/dpv-owl#ContractControl> .

<https://w3id.org/dpv/owl#ReviewImpactAssessment>
  a owl:Class, owl:NamedIndividual, <https://w3id.org/dpv/owl#OrganisationalMeasure> ;
  rdfs:subClassOf <https://w3id.org/dpv/owl#ImpactAssessment>, <https://w3id.org/dpv/owl#ReviewProcedure> ;
  dc:contributor _:genid4, _:genid1 ;
  dc:created "2022-10-22"^^xsd:date ;
  ns1:term_status "accepted"@en ;
  skos:definition "Procedures to review impact assessments in terms of continued validity, adequacy for intended purposes, and conformance of processes with findings"@en ;
  skos:prefLabel "Review Impact Assessment"@en ;
  owl:sameAs <https://w3id.org/dpv#ReviewImpactAssessment>, <https://w3id.org/dpv/dpv-owl#ReviewImpactAssessment> .

<https://w3id.org/dpv/owl#Consumer>
  a owl:Class, owl:NamedIndividual, <https://w3id.org/dpv/owl#HumanSubject> ;
  rdfs:subClassOf <https://w3id.org/dpv/owl#HumanSubject> ;
  dc:contributor _:genid4, _:genid5, _:genid1, _:genid17, _:genid6 ;
  dc:created "2022-04-06"^^xsd:date ;
  dc:modified "2024-12-17"^^xsd:date ;
  ns1:term_status "modified"@en ;
  skos:definition "Humans that consume goods or services for direct use"@en ;
  skos:prefLabel "Consumer"@en ;
  owl:sameAs <https://w3id.org/dpv#Consumer>, <https://w3id.org/dpv/dpv-owl#Consumer> .

<https://w3id.org/dpv/owl#Share>
  a owl:Class, owl:NamedIndividual, <https://w3id.org/dpv/owl#Processing> ;
  rdfs:subClassOf <https://w3id.org/dpv/owl#Disclose> ;
  dc:created "2019-05-07"^^xsd:date ;
  dc:source [
    a ns0:WebPage ;
    ns0:name "GDPR Art.4-2" ;
    ns0:url "https://eur-lex.europa.eu/eli/reg/2016/679/art_4/par_2/oj"
  ] ;
  ns1:term_status "accepted"@en ;
  skos:definition "to give data (or a portion of it) to others"@en ;
  skos:prefLabel "Share Data"@en ;
  owl:sameAs <https://w3id.org/dpv#Share>, <https://w3id.org/dpv/dpv-owl#Share> .

<https://w3id.org/dpv/owl#ContractPartiallySigned>
  a owl:Class, owl:NamedIndividual, <https://w3id.org/dpv/owl#ContractExecutionStatus> ;
  rdfs:subClassOf <https://w3id.org/dpv/owl#ContractExecutionStatus> ;
  dc:contributor _:genid4, _:genid1, _:genid17 ;
  dc:created "2025-01-09"^^xsd:date ;
  ns1:term_status "accepted"@en ;
  skos:definition "Status representing contract has been partially signed by parties i.e. some parties have signed the contract and others are yet to make a decision to sign it"@en ;
  skos:prefLabel "Contract Partially Signed"@en ;
  owl:sameAs <https://w3id.org/dpv#ContractPartiallySigned>, <https://w3id.org/dpv/dpv-owl#ContractPartiallySigned> .

odrl:spatial
  a owl:NamedIndividual, skos:Concept, odrl:LeftOperand ;
  rdfs:isDefinedBy odrl: ;
  rdfs:label "Geospatial Named Area"@en ;
  skos:definition "A named and identified geospatial area with defined borders which is used for exercising the action of the Rule. An IRI MUST be used to represent this value."@en ;
  skos:note "A code value for the area and source of the code must be presented in the Right Operand. <br />Example: the [[iso3166]] Country Codes or the Getty Thesaurus of Geographic Names. "@en ;
  skos:scopeNote "Non-Normative"@en .

<https://w3id.org/dpv/owl#VulnerableDataSubject>
  a owl:Class, owl:NamedIndividual, <https://w3id.org/dpv/owl#HumanSubject> ;
  rdfs:subClassOf <https://w3id.org/dpv/owl#VulnerableHuman> ;
  dc:contributor _:genid4, _:genid1, _:genid6 ;
  dc:created "2020-11-04"^^xsd:date ;
  dc:modified "2024-12-17"^^xsd:date ;
  ns1:term_status "modified"@en ;
  skos:definition "Humans which should be considered 'vulnerable' and therefore would require additional measures and safeguards"@en ;
  skos:prefLabel "Vulnerable Data Subject"@en ;
  skos:scopeNote "This concept denotes a Data Subject or a group are vulnerable, but not what vulnerability they possess or its context. This information can be provided additionally as comments, or as separate concepts and relations. Proposals for this are welcome."@en ;
  owl:sameAs <https://w3id.org/dpv#VulnerableDataSubject>, <https://w3id.org/dpv/dpv-owl#VulnerableDataSubject> .

<https://w3id.org/dpv/owl#hasAuditStatus>
  a owl:ObjectProperty ;
  rdfs:subPropertyOf <https://w3id.org/dpv/owl#hasStatus> ;
  ns2:rangeIncludes <https://w3id.org/dpv/owl#AuditStatus> ;
  dc:contributor _:genid1 ;
  dc:created "2022-06-22"^^xsd:date ;
  ns3:example <https://w3id.org/dpv/examples/owl#E0056>, <https://w3id.org/dpv/examples/owl#E0057> ;
  ns1:term_status "accepted"@en ;
  skos:definition "Indicates the status of audit associated with specified concept"@en ;
  skos:prefLabel "has audit status"@en ;
  ns0:rangeIncludes <https://w3id.org/dpv/owl#AuditStatus> ;
  owl:sameAs <https://w3id.org/dpv#hasAuditStatus>, <https://w3id.org/dpv/dpv-owl#hasAuditStatus> .

<https://w3id.org/dpv/owl#Retrieve>
  a owl:Class, owl:NamedIndividual, <https://w3id.org/dpv/owl#Processing> ;
  rdfs:subClassOf <https://w3id.org/dpv/owl#Use> ;
  dc:created "2019-05-07"^^xsd:date ;
  dc:source [
    a ns0:WebPage ;
    ns0:name "GDPR Art.4-2" ;
    ns0:url "https://eur-lex.europa.eu/eli/reg/2016/679/art_4/par_2/oj"
  ] ;
  ns1:term_status "accepted"@en ;
  skos:definition "to retrieve data, often in an automated manner"@en ;
  skos:prefLabel "Retrieve Data"@en ;
  owl:sameAs <https://w3id.org/dpv#Retrieve>, <https://w3id.org/dpv/dpv-owl#Retrieve> .

odrl:isNoneOf
  a owl:NamedIndividual, skos:Concept, odrl:Operator ;
  rdfs:isDefinedBy odrl: ;
  rdfs:label "Is none of"@en ;
  skos:definition "A set-based operator indicating that a given value is none of the right operand of the Constraint."@en .

<https://w3id.org/dpv/owl#Applicant>
  a owl:Class, owl:NamedIndividual, <https://w3id.org/dpv/owl#HumanSubject> ;
  rdfs:subClassOf <https://w3id.org/dpv/owl#HumanSubject> ;
  dc:contributor _:genid4, _:genid5, _:genid1, _:genid17, _:genid6 ;
  dc:created "2022-04-06"^^xsd:date ;
  dc:modified "2024-12-17"^^xsd:date ;
  ns1:term_status "modified"@en ;
  skos:definition "Humans that are applicants in some context"@en ;
  skos:prefLabel "Applicant"@en ;
  owl:sameAs <https://w3id.org/dpv#Applicant>, <https://w3id.org/dpv/dpv-owl#Applicant> .

<https://w3id.org/dpv/owl#hasActivityStatus>
  a owl:ObjectProperty ;
  rdfs:subPropertyOf <https://w3id.org/dpv/owl#hasStatus> ;
  ns2:rangeIncludes <https://w3id.org/dpv/owl#ActivityStatus> ;
  dc:contributor _:genid1 ;
  dc:created "2022-05-18"^^xsd:date ;
  ns3:example <https://w3id.org/dpv/examples/owl#E0054> ;
  ns1:term_status "accepted"@en ;
  skos:definition "Indicates the status of activity of specified concept"@en ;
  skos:prefLabel "has activity status"@en ;
  ns0:rangeIncludes <https://w3id.org/dpv/owl#ActivityStatus> ;
  owl:sameAs <https://w3id.org/dpv#hasActivityStatus>, <https://w3id.org/dpv/dpv-owl#hasActivityStatus> .

<https://w3id.org/dpv/owl#SmallScaleOfDataSubjects>
  a owl:Class, owl:NamedIndividual, <https://w3id.org/dpv/owl#DataSubjectScale> ;
  rdfs:subClassOf <https://w3id.org/dpv/owl#DataSubjectScale> ;
  dc:contributor _:genid1 ;
  dc:created "2022-06-15"^^xsd:date ;
  ns1:term_status "accepted"@en ;
  skos:definition "Scale of data subjects considered small or limited within the context"@en ;
  skos:prefLabel "Small Scale Of Data Subjects"@en ;
  owl:sameAs <https://w3id.org/dpv#SmallScaleOfDataSubjects>, <https://w3id.org/dpv/dpv-owl#SmallScaleOfDataSubjects> .

<https://w3id.org/dpv/owl#hasExpectation>
  a owl:ObjectProperty ;
  rdfs:subPropertyOf <https://w3id.org/dpv/owl#hasStatus> ;
  ns2:rangeIncludes <https://w3id.org/dpv/owl#ExpectationStatus> ;
  dc:contributor _:genid1 ;
  dc:created "2024-05-10"^^xsd:date ;
  dc:modified "2024-06-10"^^xsd:date ;
  ns1:term_status "accepted"@en ;
  skos:definition "Indicates whether the specified context was expected or unexpected"@en ;
  skos:prefLabel "has expectation"@en ;
  ns0:rangeIncludes <https://w3id.org/dpv/owl#ExpectationStatus> ;
  owl:sameAs <https://w3id.org/dpv#hasExpectation>, <https://w3id.org/dpv/dpv-owl#hasExpectation> .

<https://w3id.org/dpv/owl#ConsentUnknown>
  a owl:Class, owl:NamedIndividual, <https://w3id.org/dpv/owl#ConsentStatus> ;
  rdfs:subClassOf <https://w3id.org/dpv/owl#ConsentStatusInvalidForProcessing> ;
  dc:contributor _:genid4, _:genid1, _:genid17, _:genid6 ;
  dc:created "2022-06-22"^^xsd:date ;
  dc:source [
    a ns0:WebPage ;
    ns0:name "GConsent" ;
    ns0:url "https://w3id.org/GConsent"
  ] ;
  ns1:term_status "accepted"@en ;
  skos:definition "State where information about consent is not available or is unknown"@en ;
  skos:prefLabel "Consent Unknown"@en ;
  skos:scopeNote "Consent states can be unknown, for example, when information is not available, or cannot be trusted, or is known to be inaccurate"@en ;
  owl:sameAs <https://w3id.org/dpv#ConsentUnknown>, <https://w3id.org/dpv/dpv-owl#ConsentUnknown> .

<https://w3id.org/dpv/owl#hasInformedStatus>
  a owl:ObjectProperty ;
  rdfs:subPropertyOf <https://w3id.org/dpv/owl#hasStatus> ;
  ns2:rangeIncludes <https://w3id.org/dpv/owl#EntityInformedStatus> ;
  dc:contributor _:genid1 ;
  dc:created "2024-05-10"^^xsd:date ;
  ns1:term_status "accepted"@en ;
  skos:definition "Indicates whether an entity was informed or uninformed"@en ;
  skos:prefLabel "has informed status"@en ;
  ns0:rangeIncludes <https://w3id.org/dpv/owl#EntityInformedStatus> ;
  owl:sameAs <https://w3id.org/dpv#hasInformedStatus>, <https://w3id.org/dpv/dpv-owl#hasInformedStatus> .

<https://w3id.org/dpv/owl#Risk>
  a owl:Class ;
  rdfs:subClassOf <https://w3id.org/dpv/owl#RiskConcept> ;
  dc:contributor _:genid1 ;
  dc:created "2020-11-18"^^xsd:date ;
  dc:modified "2024-08-16"^^xsd:date ;
  ns3:example <https://w3id.org/dpv/examples/owl#E0027>, <https://w3id.org/dpv/examples/owl#E0068>, <https://w3id.org/dpv/examples/owl#E0071> ;
  ns1:term_status "accepted"@en ;
  skos:definition "A risk or possibility or uncertainty of negative effects, impacts, or consequences"@en ;
  skos:prefLabel "Risk"@en ;
  skos:scopeNote "Risks can be associated with one or more different concepts such as purpose, processing, personal data, technical or organisational measure"@en ;
  owl:sameAs <https://w3id.org/dpv#Risk>, <https://w3id.org/dpv/dpv-owl#Risk> .

<https://w3id.org/dpv/owl#ImproveTransportMobility>
  a owl:Class, owl:NamedIndividual, <https://w3id.org/dpv/owl#Purpose> ;
  rdfs:subClassOf <https://w3id.org/dpv/owl#PublicBenefit> ;
  dc:contributor _:genid5, _:genid1 ;
  dc:created "2024-02-14"^^xsd:date ;
  dc:source "DGA 2.16"@en ;
  ns1:term_status "accepted"@en ;
  skos:definition "Purposes associated with improving traffic, public transport systems or costs for drivers"@en ;
  skos:prefLabel "Improve Transport and Mobility"@en ;
  owl:sameAs <https://w3id.org/dpv#ImproveTransportMobility>, <https://w3id.org/dpv/dpv-owl#ImproveTransportMobility> .

odrl:dateTime
  a owl:NamedIndividual, skos:Concept, odrl:LeftOperand ;
  rdfs:isDefinedBy odrl: ;
  rdfs:label "Datetime"@en ;
  skos:definition "The date (and optional time and timezone) of exercising the action of the Rule. Right operand value MUST be an xsd:date or xsd:dateTime as defined by [[xmlschema11-2]]."@en ;
  skos:note "The use of Timezone information is strongly recommended. The Rule may be exercised before (with operator lt/lteq) or after (with operator gt/gteq) the date(time) defined by the Right operand. <br />Example: <code>dateTime gteq 2017-12-31T06:00Z</code> means the Rule can only be exercised after (and including) 6:00AM on the 31st Decemeber 2017 UTC time."@en ;
  skos:scopeNote "Non-Normative"@en .

<https://w3id.org/dpv/owl#Justification>
  a owl:Class ;
  rdfs:subClassOf <https://w3id.org/dpv/owl#Context> ;
  dc:contributor _:genid1 ;
  dc:created "2022-06-15"^^xsd:date ;
  ns3:example <https://w3id.org/dpv/examples/owl#E0057>, <https://w3id.org/dpv/examples/owl#E0058>, <https://w3id.org/dpv/examples/owl#E0059>, <https://w3id.org/dpv/examples/owl#E0061>, <https://w3id.org/dpv/examples/owl#E0062>, <https://w3id.org/dpv/examples/owl#E0063> ;
  ns1:term_status "accepted"@en ;
  skos:definition "A form of documentation providing reasons, explanations, or justifications"@en ;
  skos:prefLabel "Justification"@en ;
  owl:sameAs <https://w3id.org/dpv#Justification>, <https://w3id.org/dpv/dpv-owl#Justification> .

<https://w3id.org/dpv/owl#ServiceOptimisation>
  a owl:Class, owl:NamedIndividual, <https://w3id.org/dpv/owl#Purpose> ;
  rdfs:subClassOf <https://w3id.org/dpv/owl#ServiceProvision> ;
  dc:contributor _:genid13, _:genid14, _:genid1, _:genid15, _:genid16, _:genid11 ;
  dc:created "2019-04-05"^^xsd:date ;
  ns1:term_status "accepted"@en ;
  skos:definition "Purposes associated with optimisation of services or activities"@en ;
  skos:prefLabel "Service Optimisation"@en ;
  skos:scopeNote "Subclass of ServiceProvision since optimisation is usually considered part of providing services"@en ;
  owl:sameAs <https://w3id.org/dpv#ServiceOptimisation>, <https://w3id.org/dpv/dpv-owl#ServiceOptimisation> .

<https://w3id.org/dpv/owl#Importance>
  a owl:Class ;
  rdfs:subClassOf <https://w3id.org/dpv/owl#Context> ;
  dc:contributor _:genid4, _:genid5, _:genid1, _:genid17, _:genid6 ;
  dc:created "2022-02-09"^^xsd:date ;
  ns1:term_status "accepted"@en ;
  skos:definition "An indication of 'importance' within a context"@en ;
  skos:prefLabel "Importance"@en ;
  skos:scopeNote "Importance can be used to express importance, desirability, relevance, or significance as a context."@en ;
  owl:sameAs <https://w3id.org/dpv#Importance>, <https://w3id.org/dpv/dpv-owl#Importance> .

<https://w3id.org/dpv/owl#Aggregate>
  a owl:Class, owl:NamedIndividual, <https://w3id.org/dpv/owl#Processing> ;
  rdfs:subClassOf <https://w3id.org/dpv/owl#Alter> ;
  dc:contributor _:genid5, _:genid1 ;
  dc:created "2024-04-14"^^xsd:date ;
  dc:source [
    a ns0:WebPage ;
    ns0:name "SPECIAL Project" ;
    ns0:url "https://specialprivacy.ercim.eu/vocabs/processing"
  ] ;
  ns1:term_status "accepted"@en ;
  skos:definition "to aggregate data"@en ;
  skos:prefLabel "Aggregate Data"@en ;
  skos:related <https://specialprivacy.ercim.eu/vocabs/processing#Aggregate> ;
  owl:sameAs <https://w3id.org/dpv#Aggregate>, <https://w3id.org/dpv/dpv-owl#Aggregate> .

<https://w3id.org/dpv/owl#PersonnelPerformanceEvaluation>
  a owl:Class, owl:NamedIndividual, <https://w3id.org/dpv/owl#Purpose> ;
  rdfs:subClassOf <https://w3id.org/dpv/owl#PersonnelPerformanceManagement> ;
  dc:created "2024-12-01"^^xsd:date ;
  ns1:term_status "accepted"@en ;
  skos:definition "Purposes associated with evaluation or assessment of performance of employees"@en ;
  skos:prefLabel "Personnel Performance Evaluation"@en ;
  owl:sameAs <https://w3id.org/dpv#PersonnelPerformanceEvaluation>, <https://w3id.org/dpv/dpv-owl#PersonnelPerformanceEvaluation> .

<https://w3id.org/dpv/owl#UnverifiedData>
  a owl:Class ;
  rdfs:subClassOf <https://w3id.org/dpv/owl#Data> ;
  dc:contributor _:genid1 ;
  dc:created "2022-11-02"^^xsd:date ;
  ns1:term_status "accepted"@en ;
  skos:definition "Data that has not been verified in terms of accuracy, inconsistency, or quality"@en ;
  skos:prefLabel "Unverified Data"@en ;
  owl:sameAs <https://w3id.org/dpv#UnverifiedData>, <https://w3id.org/dpv/dpv-owl#UnverifiedData> .

<https://w3id.org/dpv/owl#DataController>
  a owl:Class ;
  rdfs:subClassOf <https://w3id.org/dpv/owl#LegalEntity> ;
  dc:contributor _:genid13, _:genid11 ;
  dc:created "2019-04-05"^^xsd:date ;
  dc:modified "2020-11-04"^^xsd:date ;
  dc:source [
    a ns0:WebPage ;
    ns0:name "GDPR Art.4-7g" ;
    ns0:url "https://eur-lex.europa.eu/eli/reg/2016/679/art_4/par_7/oj"
  ] ;
  ns3:example <https://w3id.org/dpv/examples/owl#E0032>, <https://w3id.org/dpv/examples/owl#E0033> ;
  ns1:term_status "accepted"@en ;
  skos:definition "The individual or organisation that decides (or controls) the purpose(s) of processing personal data."@en ;
  skos:prefLabel "Data Controller"@en ;
  skos:scopeNote "The terms 'Controller', 'Data Controller', and 'PII Controller' refer to the same concept"@en ;
  owl:sameAs <https://w3id.org/dpv#DataController>, <https://w3id.org/dpv/dpv-owl#DataController> .

<https://w3id.org/dpv/owl#ContractBeingPerformed>
  a owl:Class, owl:NamedIndividual, <https://w3id.org/dpv/owl#ContractPerformanceStatus> ;
  rdfs:subClassOf <https://w3id.org/dpv/owl#ContractPerformanceStatus> ;
  dc:contributor _:genid4, _:genid1, _:genid17 ;
  dc:created "2025-01-09"^^xsd:date ;
  ns1:term_status "accepted"@en ;
  skos:definition "Status representing contract that has been fully executed and whose terms are being carried out i.e. the contract is being performed"@en ;
  skos:prefLabel "Contract Being Performed"@en ;
  owl:sameAs <https://w3id.org/dpv#ContractBeingPerformed>, <https://w3id.org/dpv/dpv-owl#ContractBeingPerformed> .

<https://w3id.org/dpv/owl#DataInteroperabilityAssessment>
  a owl:Class, owl:NamedIndividual, <https://w3id.org/dpv/owl#OrganisationalMeasure> ;
  rdfs:subClassOf <https://w3id.org/dpv/owl#Assessment>, <https://w3id.org/dpv/owl#DataInteroperabilityManagement> ;
  dc:contributor _:genid1 ;
  dc:created "2024-04-14"^^xsd:date ;
  ns1:term_status "accepted"@en ;
  skos:definition "Measures associated with assessment of data interoperability"@en ;
  skos:prefLabel "Data Interoperability Assessment"@en ;
  owl:sameAs <https://w3id.org/dpv#DataInteroperabilityAssessment>, <https://w3id.org/dpv/dpv-owl#DataInteroperabilityAssessment> .

<https://w3id.org/dpv/owl#ServiceConsumer>
  a owl:Class ;
  rdfs:subClassOf <https://w3id.org/dpv/owl#LegalEntity> ;
  dc:contributor _:genid1 ;
  dc:created "2024-04-20"^^xsd:date ;
  ns1:term_status "accepted"@en ;
  skos:definition "The entity that consumes or receives the service"@en ;
  skos:prefLabel "Service Consumer"@en ;
  owl:sameAs <https://w3id.org/dpv#ServiceConsumer>, <https://w3id.org/dpv/dpv-owl#ServiceConsumer> .

<https://w3id.org/dpv/owl#DataSubjectInformed>
  a owl:Class, owl:NamedIndividual, <https://w3id.org/dpv/owl#EntityInformedStatus> ;
  rdfs:subClassOf <https://w3id.org/dpv/owl#EntityInformed> ;
  dc:contributor _:genid4, _:genid1, _:genid25, _:genid6 ;
  dc:created "2024-05-10"^^xsd:date ;
  ns1:term_status "accepted"@en ;
  skos:definition "Status indicating DataSubject has been informed about the specified context"@en ;
  skos:prefLabel "Data Subject Informed"@en ;
  owl:sameAs <https://w3id.org/dpv#DataSubjectInformed>, <https://w3id.org/dpv/dpv-owl#DataSubjectInformed> .

<https://w3id.org/dpv/owl#ActivityCompleted>
  a owl:Class, owl:NamedIndividual, <https://w3id.org/dpv/owl#ActivityStatus> ;
  rdfs:subClassOf <https://w3id.org/dpv/owl#ActivityStatus> ;
  dc:contributor _:genid1 ;
  dc:created "2022-05-18"^^xsd:date ;
  ns1:term_status "accepted"@en ;
  skos:definition "State of an activity that has completed i.e. is fully in the past"@en ;
  skos:prefLabel "Activity Completed"@en ;
  owl:sameAs <https://w3id.org/dpv#ActivityCompleted>, <https://w3id.org/dpv/dpv-owl#ActivityCompleted> .

<https://w3id.org/dpv/owl#FixedLocation>
  a owl:Class, owl:NamedIndividual, <https://w3id.org/dpv/owl#LocationFixture> ;
  rdfs:subClassOf <https://w3id.org/dpv/owl#LocationFixture> ;
  dc:contributor _:genid1 ;
  dc:created "2022-06-15"^^xsd:date ;
  dc:modified "2020-10-05"^^xsd:date ;
  ns1:term_status "accepted"@en ;
  skos:definition "Location that is fixed i.e. known to occur at a specific place"@en ;
  skos:prefLabel "Fixed Location"@en ;
  owl:sameAs <https://w3id.org/dpv#FixedLocation>, <https://w3id.org/dpv/dpv-owl#FixedLocation> .

odrl:#constraints
  a owl:NamedIndividual, skos:Collection ;
  skos:member odrl:Constraint, odrl:LeftOperand, odrl:Operator, odrl:RightOperand, odrl:constraint, odrl:dataType, odrl:leftOperand, odrl:operator, odrl:refinement, odrl:rightOperand, odrl:rightOperandReference, odrl:status, odrl:unit ;
  skos:prefLabel "Constraint"@en ;
  skos:scopeNote "ODRL Core Vocabulary Terms"@en .

<https://w3id.org/dpv/owl#CustomerCare>
  a owl:Class, owl:NamedIndividual, <https://w3id.org/dpv/owl#Purpose> ;
  rdfs:subClassOf <https://w3id.org/dpv/owl#CustomerManagement> ;
  dc:contributor _:genid13, _:genid14, _:genid1, _:genid15, _:genid16, _:genid11 ;
  dc:created "2019-04-05"^^xsd:date ;
  ns1:term_status "accepted"@en ;
  skos:definition "Customer Care refers to purposes associated with purposes for providing assistance, resolving issues, ensuring satisfaction, etc. in relation to services provided"@en ;
  skos:prefLabel "Customer Care"@en ;
  skos:related <https://specialprivacy.ercim.eu/vocabs/purposes#Feedback> ;
  owl:sameAs <https://w3id.org/dpv#CustomerCare>, <https://w3id.org/dpv/dpv-owl#CustomerCare> .

<https://w3id.org/dpv/owl#NotApplicable>
  a owl:Class, owl:NamedIndividual, <https://w3id.org/dpv/owl#Applicability> ;
  rdfs:subClassOf <https://w3id.org/dpv/owl#Applicability> ;
  dc:contributor _:genid1 ;
  dc:created "2023-08-24"^^xsd:date ;
  ns1:term_status "accepted"@en ;
  skos:definition "Concept indicating the information or context is not applicable"@en ;
  skos:prefLabel "Not Applicable"@en ;
  skos:scopeNote "This relates to a 'Stop' state as distinct from a 'Halt' state. It makes no comments on whether the Activity can be resumed or continued towards completion."@en ;
  owl:sameAs <https://w3id.org/dpv#NotApplicable>, <https://w3id.org/dpv/dpv-owl#NotApplicable> .

<https://w3id.org/dpv/owl#Destruct>
  a owl:Class, owl:NamedIndividual, <https://w3id.org/dpv/owl#Processing> ;
  rdfs:subClassOf <https://w3id.org/dpv/owl#Remove> ;
  dc:created "2019-05-07"^^xsd:date ;
  dc:source [
    a ns0:WebPage ;
    ns0:name "GDPR Art.4-2" ;
    ns0:url "https://eur-lex.europa.eu/eli/reg/2016/679/art_4/par_2/oj"
  ] ;
  ns1:term_status "accepted"@en ;
  skos:definition "to process data in a way it no longer exists or cannot be repaired"@en ;
  skos:prefLabel "Destruct Data"@en ;
  owl:sameAs <https://w3id.org/dpv#Destruct>, <https://w3id.org/dpv/dpv-owl#Destruct> .

<https://w3id.org/dpv/owl#RightsManagement>
  a owl:Class, owl:NamedIndividual, <https://w3id.org/dpv/owl#OrganisationalMeasure> ;
  rdfs:subClassOf <https://w3id.org/dpv/owl#OrganisationalMeasure> ;
  dc:contributor _:genid4, _:genid5, _:genid1 ;
  dc:created "2024-04-14"^^xsd:date ;
  ns1:term_status "accepted"@en ;
  skos:definition "Methods associated with rights management where 'rights' refer to controlling who can do what with a resource"@en ;
  skos:prefLabel "Rights Management"@en ;
  owl:sameAs <https://w3id.org/dpv#RightsManagement>, <https://w3id.org/dpv/dpv-owl#RightsManagement> .

<https://w3id.org/dpv/owl#NoticeUnused>
  a owl:Class, owl:NamedIndividual, <https://w3id.org/dpv/owl#NoticeStatus> ;
  rdfs:subClassOf <https://w3id.org/dpv/owl#NoticeStatus> ;
  dc:contributor _:genid4, _:genid1 ;
  dc:created "2024-12-01"^^xsd:date ;
  ns1:term_status "accepted"@en ;
  skos:definition "Status indicating the notice has been communicated but has not yet been used e.g. the recipient has not acknowledged it or has not taken the intended action"@en ;
  skos:prefLabel "Notice Unused"@en ;
  owl:sameAs <https://w3id.org/dpv#NoticeUnused>, <https://w3id.org/dpv/dpv-owl#NoticeUnused> .

<https://w3id.org/dpv/owl#EvaluationScoring>
  a owl:Class ;
  rdfs:subClassOf <https://w3id.org/dpv/owl#ProcessingContext> ;
  dc:contributor _:genid1, _:genid2 ;
  dc:created "2020-11-04"^^xsd:date ;
  dc:source [
    a ns0:WebPage ;
    ns0:name "GDPR Art.4-2" ;
    ns0:url "https://eur-lex.europa.eu/eli/reg/2016/679/art_4/par_2/oj"
  ] ;
  ns1:term_status "accepted"@en ;
  skos:definition "Processing that involves evaluation and scoring of individuals"@en ;
  skos:prefLabel "Evaluation and Scoring"@en ;
  owl:sameAs <https://w3id.org/dpv#EvaluationScoring>, <https://w3id.org/dpv/dpv-owl#EvaluationScoring> .

<https://w3id.org/dpv/owl#Analyse>
  a owl:Class, owl:NamedIndividual, <https://w3id.org/dpv/owl#Processing> ;
  rdfs:subClassOf <https://w3id.org/dpv/owl#Use> ;
  dc:created "2019-05-07"^^xsd:date ;
  dc:source [
    a ns0:WebPage ;
    ns0:name "SPECIAL Project" ;
    ns0:url "https://specialprivacy.ercim.eu/vocabs/processing"
  ] ;
  ns1:term_status "accepted"@en ;
  skos:definition "to study or examine the data in detail"@en ;
  skos:prefLabel "Analyse Data"@en ;
  skos:related <https://specialprivacy.ercim.eu/vocabs/processing#Analyse> ;
  owl:sameAs <https://w3id.org/dpv#Analyse>, <https://w3id.org/dpv/dpv-owl#Analyse> .

<https://w3id.org/dpv/owl#ApprovalProcedure>
  a owl:Class, owl:NamedIndividual, <https://w3id.org/dpv/owl#OrganisationalMeasure> ;
  rdfs:subClassOf <https://w3id.org/dpv/owl#GovernanceProcedures> ;
  dc:contributor _:genid25 ;
  dc:created "2024-12-01"^^xsd:date ;
  ns1:term_status "accepted"@en ;
  skos:definition "A procedure or process for determining and managing approvals for activities as part of governance"@en ;
  skos:prefLabel "Approval Procedure"@en ;
  owl:sameAs <https://w3id.org/dpv#ApprovalProcedure>, <https://w3id.org/dpv/dpv-owl#ApprovalProcedure> .

<https://w3id.org/dpv/owl#Obligation>
  a owl:Class, owl:NamedIndividual, <https://w3id.org/dpv/owl#Rule> ;
  rdfs:subClassOf <https://w3id.org/dpv/owl#Rule> ;
  dc:contributor _:genid4, _:genid5, _:genid1, _:genid6 ;
  dc:created "2022-10-19"^^xsd:date ;
  ns1:term_status "accepted"@en ;
  skos:definition "A rule describing an obligation for performing an activity"@en ;
  skos:prefLabel "Obligation"@en ;
  owl:sameAs <https://w3id.org/dpv#Obligation>, <https://w3id.org/dpv/dpv-owl#Obligation> .

<https://w3id.org/dpv/owl#hasConsentControl>
  a owl:ObjectProperty ;
  ns2:rangeIncludes <https://w3id.org/dpv/owl#ConsentControl> ;
  dc:created "2024-05-11"^^xsd:date ;
  ns1:term_status "accepted"@en ;
  skos:definition "Specific a control associated with consent"@en ;
  skos:prefLabel "has consent control"@en ;
  ns0:rangeIncludes <https://w3id.org/dpv/owl#ConsentControl> ;
  owl:sameAs <https://w3id.org/dpv#hasConsentControl>, <https://w3id.org/dpv/dpv-owl#hasConsentControl> .

<https://w3id.org/dpv/owl#LocationFixture>
  a owl:Class ;
  rdfs:subClassOf rdfs:Class ;
  dc:contributor _:genid1 ;
  dc:created "2022-06-15"^^xsd:date ;
  ns3:example <https://w3id.org/dpv/examples/owl#E0060> ;
  ns1:term_status "accepted"@en ;
  skos:definition "The fixture of location refers to whether the location is fixed"@en ;
  skos:prefLabel "Location Fixture"@en ;
  owl:sameAs <https://w3id.org/dpv#LocationFixture>, <https://w3id.org/dpv/dpv-owl#LocationFixture> .

<https://w3id.org/dpv/owl#QuantumCryptography>
  a owl:Class, owl:NamedIndividual, <https://w3id.org/dpv/owl#TechnicalMeasure> ;
  rdfs:subClassOf <https://w3id.org/dpv/owl#CryptographicMethods> ;
  dc:contributor _:genid1 ;
  dc:created "2022-08-17"^^xsd:date ;
  dc:source [
    a ns0:WebPage ;
    ns0:name "ENISA Reference Incident Classification Taxonomy 2018" ;
    ns0:url "https://www.enisa.europa.eu/publications/reference-incident-classification-taxonomy/"
  ] ;
  ns1:term_status "accepted"@en ;
  skos:definition "Cryptographic methods that utilise quantum mechanical properties to perform cryptographic tasks"@en ;
  skos:prefLabel "Quantum Cryptography"@en ;
  owl:sameAs <https://w3id.org/dpv#QuantumCryptography>, <https://w3id.org/dpv/dpv-owl#QuantumCryptography> .

<https://w3id.org/dpv/owl#CertificationSeal>
  a owl:Class, owl:NamedIndividual, <https://w3id.org/dpv/owl#OrganisationalMeasure> ;
  rdfs:subClassOf <https://w3id.org/dpv/owl#OrganisationalMeasure> ;
  dc:contributor _:genid9, _:genid10, _:genid1, _:genid11 ;
  dc:created "2019-04-05"^^xsd:date ;
  ns1:term_status "accepted"@en ;
  skos:definition "Certifications, seals, and marks indicating compliance to regulations or practices"@en ;
  skos:prefLabel "Certification and Seal"@en ;
  owl:sameAs <https://w3id.org/dpv#CertificationSeal>, <https://w3id.org/dpv/dpv-owl#CertificationSeal> .

<https://w3id.org/dpv/owl#FRIA>
  a owl:Class, owl:NamedIndividual, <https://w3id.org/dpv/owl#OrganisationalMeasure> ;
  rdfs:subClassOf <https://w3id.org/dpv/owl#RightsImpactAssessment> ;
  dc:contributor _:genid1 ;
  dc:created "2024-04-14"^^xsd:date ;
  dc:source "AI Act Art.27"@en ;
  ns1:term_status "accepted"@en ;
  skos:definition "Impact assessment which assesses the potential and actual impact on fundamental rights occuring due to processing activities"@en ;
  skos:prefLabel "Fundamental Rights Impact Assessment (FRIA)"@en ;
  skos:scopeNote "The fundamental rights and freedoms may be those defined in law or other norms, and may be bound to a jurisdiction - for example see EU Charter of Fundamental Rights"@en ;
  owl:sameAs <https://w3id.org/dpv#FRIA>, <https://w3id.org/dpv/dpv-owl#FRIA> .

<https://w3id.org/dpv/owl#hasDataImporter>
  a owl:ObjectProperty ;
  rdfs:subPropertyOf <https://w3id.org/dpv/owl#hasRecipient> ;
  ns2:rangeIncludes <https://w3id.org/dpv/owl#DataImporter> ;
  dc:contributor _:genid4, _:genid1, _:genid6 ;
  dc:created "2022-02-09"^^xsd:date ;
  ns1:term_status "accepted"@en ;
  skos:definition "Indicates inclusion or applicability of a LegalEntity in the role of Data Importer"@en ;
  skos:prefLabel "has data importer"@en ;
  ns0:rangeIncludes <https://w3id.org/dpv/owl#DataImporter> ;
  owl:sameAs <https://w3id.org/dpv#hasDataImporter>, <https://w3id.org/dpv/dpv-owl#hasDataImporter> .

<https://w3id.org/dpv/owl#EntityNonPermissiveInvolvement>
  a owl:Class ;
  rdfs:subClassOf <https://w3id.org/dpv/owl#EntityInvolvement> ;
  dc:contributor _:genid1, _:genid25 ;
  dc:created "2024-05-11"^^xsd:date ;
  ns1:term_status "accepted"@en ;
  skos:definition "Involvement of an entity in specific context where it is not permitted or able to do something"@en ;
  skos:prefLabel "Entity Non-Permissive Involvement"@en ;
  owl:sameAs <https://w3id.org/dpv#EntityNonPermissiveInvolvement>, <https://w3id.org/dpv/dpv-owl#EntityNonPermissiveInvolvement> .

<https://w3id.org/dpv/owl#SecurityAudit>
  a owl:Class, owl:NamedIndividual, <https://w3id.org/dpv/owl#OrganisationalMeasure> ;
  rdfs:subClassOf <https://w3id.org/dpv/owl#Audit> ;
  dc:contributor _:genid1 ;
  dc:created "2024-12-17"^^xsd:date ;
  ns1:term_status "accepted"@en ;
  skos:definition "An audit that systematically examines the existence and use of security risks and measures within information systems, networks, and security policies to identify vulnerabilities, risks, and gaps"@en ;
  skos:prefLabel "Security Audit"@en ;
  owl:sameAs <https://w3id.org/dpv#SecurityAudit>, <https://w3id.org/dpv/dpv-owl#SecurityAudit> .

<https://w3id.org/dpv/owl#Record>
  a owl:Class, owl:NamedIndividual, <https://w3id.org/dpv/owl#Processing> ;
  rdfs:subClassOf <https://w3id.org/dpv/owl#Obtain> ;
  dc:created "2019-05-07"^^xsd:date ;
  dc:source [
    a ns0:WebPage ;
    ns0:name "GDPR Art.4-2" ;
    ns0:url "https://eur-lex.europa.eu/eli/reg/2016/679/art_4/par_2/oj"
  ] ;
  ns1:term_status "accepted"@en ;
  skos:definition "to make a record (especially media)"@en ;
  skos:prefLabel "Record Data"@en ;
  owl:sameAs <https://w3id.org/dpv#Record>, <https://w3id.org/dpv/dpv-owl#Record> .

odrl:Offer
  a owl:Class, owl:NamedIndividual, skos:Concept ;
  rdfs:subClassOf odrl:Policy ;
  owl:disjointWith odrl:Privacy, odrl:Request, odrl:Set, odrl:Ticket ;
  rdfs:isDefinedBy odrl: ;
  rdfs:label "Offer"@en ;
  skos:definition "A Policy that proposes a Rule over an Asset from an assigner."@en ;
  skos:note "An Offer Policy MUST contain at least one Permission or Prohibition rule and a Party with Assigner function (in the same Permission or Prohibition). The Offer Policy MAY contain a Party with Assignee function, but MUST not grant any privileges to that Party."@en .

<https://w3id.org/dpv/owl#ContractNegotiated>
  a owl:Class, owl:NamedIndividual, <https://w3id.org/dpv/owl#ContractPreparationStatus> ;
  rdfs:subClassOf <https://w3id.org/dpv/owl#ContractPreparationStatus> ;
  dc:contributor _:genid4, _:genid1, _:genid17 ;
  dc:created "2025-01-09"^^xsd:date ;
  ns1:term_status "accepted"@en ;
  skos:definition "Status representing contract has been successfully negotiated by involved parties"@en ;
  skos:prefLabel "Contract Negotiated"@en ;
  owl:sameAs <https://w3id.org/dpv#ContractNegotiated>, <https://w3id.org/dpv/dpv-owl#ContractNegotiated> .

<https://w3id.org/dpv/owl#SupportInformedConsentDecision>
  a owl:Class, owl:NamedIndividual, <https://w3id.org/dpv/owl#OrganisationalMeasure> ;
  rdfs:subClassOf <https://w3id.org/dpv/owl#SupportEntityDecisionMaking> ;
  dc:contributor _:genid5, _:genid1 ;
  dc:created "2024-04-14"^^xsd:date ;
  dc:source "DGA 2.15"@en ;
  ns1:term_status "accepted"@en ;
  skos:definition "Supporting individuals with making a decision regarding their informed consent"@en ;
  skos:prefLabel "Support Informed Consent Decision"@en ;
  owl:sameAs <https://w3id.org/dpv#SupportInformedConsentDecision>, <https://w3id.org/dpv/dpv-owl#SupportInformedConsentDecision> .

<https://w3id.org/dpv/owl#hasIndicationMethod>
  a owl:ObjectProperty ;
  dc:contributor _:genid4, _:genid1, _:genid17, _:genid6 ;
  dc:created "2022-06-21"^^xsd:date ;
  ns1:term_status "accepted"@en ;
  skos:definition "Specifies the method by which an entity has indicated the specific context"@en ;
  skos:prefLabel "has indication method"@en ;
  owl:sameAs <https://w3id.org/dpv#hasIndicationMethod>, <https://w3id.org/dpv/dpv-owl#hasIndicationMethod> .

<https://w3id.org/dpv/owl#SecureMultiPartyComputation>
  a owl:Class, owl:NamedIndividual, <https://w3id.org/dpv/owl#TechnicalMeasure> ;
  rdfs:subClassOf <https://w3id.org/dpv/owl#CryptographicMethods> ;
  dc:contributor _:genid1 ;
  dc:created "2022-08-17"^^xsd:date ;
  dc:source [
    a ns0:WebPage ;
    ns0:name "ENISA Reference Incident Classification Taxonomy 2018" ;
    ns0:url "https://www.enisa.europa.eu/publications/reference-incident-classification-taxonomy/"
  ] ;
  ns1:term_status "accepted"@en ;
  skos:definition "Use of cryptographic methods for entities to jointly compute functions without revealing inputs"@en ;
  skos:prefLabel "Secure Multi-Party Computation"@en ;
  owl:sameAs <https://w3id.org/dpv#SecureMultiPartyComputation>, <https://w3id.org/dpv/dpv-owl#SecureMultiPartyComputation> .

<https://w3id.org/dpv/owl#FullAutomation>
  a owl:Class, owl:NamedIndividual, <https://w3id.org/dpv/owl#AutomationLevel> ;
  rdfs:subClassOf <https://w3id.org/dpv/owl#AutomationLevel> ;
  dc:contributor _:genid1, _:genid25 ;
  dc:created "2023-12-10"^^xsd:date ;
  dc:modified "2024-04-20"^^xsd:date ;
  dc:source [
    a ns0:WebPage ;
    ns0:name "ISO/IEC 22989:2022 Artificial intelligence concepts and terminology" ;
    ns0:url "https://www.iso.org/standard/74296.html"
  ] ;
  ns1:term_status "accepted"@en ;
  skos:definition "Level of automation corresponding to Level 5 in ISO/IEC 22989:2022 where the automation in system is capable of performing all its tasks regardless of the conditions without human involvement"@en ;
  skos:prefLabel "Full Automation"@en ;
  skos:scopeNote "Though Fully Automated such operations can still be associated with dpv:HumanInvolved e.g. for inputs, oversight or verification"@en ;
  owl:sameAs <https://w3id.org/dpv#FullAutomation>, <https://w3id.org/dpv/dpv-owl#FullAutomation> .

<https://w3id.org/dpv/owl#ActivityOngoing>
  a owl:Class, owl:NamedIndividual, <https://w3id.org/dpv/owl#ActivityStatus> ;
  rdfs:subClassOf <https://w3id.org/dpv/owl#ActivityStatus> ;
  dc:contributor _:genid1 ;
  dc:created "2022-05-18"^^xsd:date ;
  ns1:term_status "accepted"@en ;
  skos:definition "State of an activity occurring in continuation i.e. currently ongoing"@en ;
  skos:prefLabel "Activity Ongoing"@en ;
  owl:sameAs <https://w3id.org/dpv#ActivityOngoing>, <https://w3id.org/dpv/dpv-owl#ActivityOngoing> .

<https://w3id.org/dpv/owl#hasJustification>
  a owl:ObjectProperty ;
  ns2:domainIncludes <https://w3id.org/dpv/owl#RightExerciseActivity> ;
  ns2:rangeIncludes <https://w3id.org/dpv/owl#Justification> ;
  dc:contributor _:genid1 ;
  dc:created "2022-06-15"^^xsd:date ;
  ns3:example <https://w3id.org/dpv/examples/owl#E0057>, <https://w3id.org/dpv/examples/owl#E0058>, <https://w3id.org/dpv/examples/owl#E0059>, <https://w3id.org/dpv/examples/owl#E0061>, <https://w3id.org/dpv/examples/owl#E0062>, <https://w3id.org/dpv/examples/owl#E0063> ;
  ns1:term_status "accepted"@en ;
  skos:definition "Indicates a justification for specified concept or context"@en ;
  skos:prefLabel "has justification"@en ;
  skos:scopeNote "Also used for specifying a justification for non-fulfilment of Right Exercise"@en ;
  ns0:domainIncludes <https://w3id.org/dpv/owl#RightExerciseActivity> ;
  ns0:rangeIncludes <https://w3id.org/dpv/owl#Justification> ;
  owl:sameAs <https://w3id.org/dpv#hasJustification>, <https://w3id.org/dpv/dpv-owl#hasJustification> .

<https://w3id.org/dpv/owl#GuidelinesPrinciple>
  a owl:Class, owl:NamedIndividual, <https://w3id.org/dpv/owl#OrganisationalMeasure> ;
  rdfs:subClassOf <https://w3id.org/dpv/owl#OrganisationalMeasure> ;
  dc:contributor _:genid9, _:genid10, _:genid1, _:genid11 ;
  dc:created "2019-04-05"^^xsd:date ;
  ns1:term_status "accepted"@en ;
  skos:definition "Guidelines or Principles regarding processing and operational measures"@en ;
  skos:prefLabel "Guidelines Principle"@en ;
  owl:sameAs <https://w3id.org/dpv#GuidelinesPrinciple>, <https://w3id.org/dpv/dpv-owl#GuidelinesPrinciple> .

odrl:attributedParty
  a owl:ObjectProperty, owl:NamedIndividual, skos:Concept ;
  rdfs:subPropertyOf odrl:function ;
  rdfs:isDefinedBy odrl: ;
  rdfs:label "Attributed Party"@en ;
  skos:definition "The Party to be attributed."@en ;
  skos:note "Maybe specified as part of the attribute action."@en ;
  skos:scopeNote "Non-Normative"@en .

<https://w3id.org/dpv/owl#hasPersonalData>
  a owl:ObjectProperty ;
  rdfs:subPropertyOf <https://w3id.org/dpv/owl#hasData> ;
  ns2:rangeIncludes <https://w3id.org/dpv/owl#PersonalData> ;
  dc:contributor _:genid1 ;
  dc:created "2022-01-19"^^xsd:date ;
  ns3:example <https://w3id.org/dpv/examples/owl#E0044> ;
  ns1:term_status "accepted"@en ;
  skos:definition "Indicates association with Personal Data"@en ;
  skos:prefLabel "has personal data"@en ;
  ns0:rangeIncludes <https://w3id.org/dpv/owl#PersonalData> ;
  owl:sameAs <https://w3id.org/dpv#hasPersonalData>, <https://w3id.org/dpv/dpv-owl#hasPersonalData> .

<https://w3id.org/dpv/owl#RecruitmentTargetedAdvertising>
  a owl:Class, owl:NamedIndividual, <https://w3id.org/dpv/owl#Purpose> ;
  rdfs:subClassOf <https://w3id.org/dpv/owl#RecruitmentAdvertising>, <https://w3id.org/dpv/owl#TargetedAdvertising> ;
  dc:created "2024-12-01"^^xsd:date ;
  ns1:term_status "accepted"@en ;
  skos:definition "Purposes associated with targeted advertisement for Recruitments and personnel hiring"@en ;
  skos:prefLabel "Targeted Recruitment Advertising"@en ;
  owl:sameAs <https://w3id.org/dpv#RecruitmentTargetedAdvertising>, <https://w3id.org/dpv/dpv-owl#RecruitmentTargetedAdvertising> .

<https://w3id.org/dpv/owl#MisusePreventionAndDetection>
  a owl:Class, owl:NamedIndividual, <https://w3id.org/dpv/owl#Purpose> ;
  rdfs:subClassOf <https://w3id.org/dpv/owl#EnforceSecurity> ;
  dc:created "2024-05-09"^^xsd:date ;
  dc:source "DGA 22.1(a)"@en ;
  ns1:term_status "accepted"@en ;
  skos:definition "Prevention and Detection of Misuse or Abuse of services"@en ;
  skos:prefLabel "Misuse, Prevention and Detection"@en ;
  owl:sameAs <https://w3id.org/dpv#MisusePreventionAndDetection>, <https://w3id.org/dpv/dpv-owl#MisusePreventionAndDetection> .

<https://w3id.org/dpv/owl#ImproveInternalCRMProcesses>
  a owl:Class, owl:NamedIndividual, <https://w3id.org/dpv/owl#Purpose> ;
  rdfs:subClassOf <https://w3id.org/dpv/owl#CustomerRelationshipManagement>, <https://w3id.org/dpv/owl#OptimisationForController> ;
  dc:contributor _:genid13, _:genid14, _:genid1, _:genid15, _:genid16, _:genid11 ;
  dc:created "2019-04-05"^^xsd:date ;
  ns1:term_status "accepted"@en ;
  skos:definition "Purposes associated with improving customer-relationship management (CRM) processes"@en ;
  skos:prefLabel "Improve Internal CRM Processes"@en ;
  owl:sameAs <https://w3id.org/dpv#ImproveInternalCRMProcesses>, <https://w3id.org/dpv/dpv-owl#ImproveInternalCRMProcesses> .

<https://w3id.org/dpv/owl#RecruitmentManagement>
  a owl:Class, owl:NamedIndividual, <https://w3id.org/dpv/owl#Purpose> ;
  rdfs:subClassOf <https://w3id.org/dpv/owl#PersonnelHiring> ;
  dc:created "2024-12-01"^^xsd:date ;
  ns1:term_status "accepted"@en ;
  skos:definition "Purposes assocaited with recruitment of personnel, which includes identifying, sourcing, screening, filtering, shortlisting, and interviewing candidates"@en ;
  skos:prefLabel "Recruitment Management"@en ;
  owl:sameAs <https://w3id.org/dpv#RecruitmentManagement>, <https://w3id.org/dpv/dpv-owl#RecruitmentManagement> .

odrl:archive
  a owl:NamedIndividual, skos:Concept, odrl:Action ;
  odrl:includedIn odrl:use ;
  rdfs:isDefinedBy odrl: ;
  rdfs:label "Archive"@en ;
  skos:definition "To store the Asset (in a non-transient form)."@en ;
  skos:note "Temporal constraints may be used for temporal conditions."@en ;
  skos:scopeNote "Non-Normative"@en .

<https://w3id.org/dpv/owl#Encryption>
  a owl:Class, owl:NamedIndividual, <https://w3id.org/dpv/owl#TechnicalMeasure> ;
  rdfs:subClassOf <https://w3id.org/dpv/owl#TechnicalMeasure> ;
  dc:contributor _:genid9, _:genid10, _:genid1, _:genid11 ;
  dc:created "2019-04-05"^^xsd:date ;
  ns3:example <https://w3id.org/dpv/examples/owl#E0020> ;
  ns1:term_status "accepted"@en ;
  skos:definition "Technical measures consisting of encryption"@en ;
  skos:prefLabel "Encryption"@en ;
  owl:sameAs <https://w3id.org/dpv#Encryption>, <https://w3id.org/dpv/dpv-owl#Encryption> .

<https://w3id.org/dpv/owl#OfficialAuthorityExerciseCompleted>
  a owl:Class, owl:NamedIndividual, <https://w3id.org/dpv/owl#OfficialAuthorityExerciseStatus> ;
  rdfs:subClassOf <https://w3id.org/dpv/owl#OfficialAuthorityExerciseStatus> ;
  dc:created "2024-08-27"^^xsd:date ;
  ns1:term_status "accepted"@en ;
  skos:definition "Status where the official authority has been exercised to completion"@en ;
  skos:prefLabel "Official Authority Exercise Completed"@en ;
  owl:sameAs <https://w3id.org/dpv#OfficialAuthorityExerciseCompleted>, <https://w3id.org/dpv/dpv-owl#OfficialAuthorityExerciseCompleted> .

odrl:remedy
  a owl:ObjectProperty, owl:NamedIndividual, skos:Concept ;
  rdfs:subPropertyOf odrl:failure ;
  rdfs:domain odrl:Prohibition ;
  rdfs:range odrl:Duty ;
  rdfs:isDefinedBy odrl: ;
  rdfs:label "Remedy"@en ;
  skos:definition "Relates an individual remedy Duty to a Prohibition."@en ;
  skos:note "The remedy property expresses an agreed Duty that must be fulfilled in case that a Prohibition has been violated by being exercised."@en .

<https://w3id.org/dpv/owl#Disseminate>
  a owl:Class, owl:NamedIndividual, <https://w3id.org/dpv/owl#Processing> ;
  rdfs:subClassOf <https://w3id.org/dpv/owl#Disclose> ;
  dc:created "2019-05-07"^^xsd:date ;
  dc:source [
    a ns0:WebPage ;
    ns0:name "GDPR Art.4-2" ;
    ns0:url "https://eur-lex.europa.eu/eli/reg/2016/679/art_4/par_2/oj"
  ] ;
  ns1:term_status "accepted"@en ;
  skos:definition "to spread data throughout"@en ;
  skos:prefLabel "Disseminate Data"@en ;
  owl:sameAs <https://w3id.org/dpv#Disseminate>, <https://w3id.org/dpv/dpv-owl#Disseminate> .

<https://w3id.org/dpv/owl#SubsidiaryLegalEntity>
  a owl:Class ;
  rdfs:subClassOf <https://w3id.org/dpv/owl#Organisation> ;
  dc:contributor _:genid4, _:genid1 ;
  dc:created "2024-04-14"^^xsd:date ;
  ns1:term_status "accepted"@en ;
  skos:definition "A legal entity that operates as a subsidiary of another legal entity"@en ;
  skos:prefLabel "Subsidiary Legal Entity"@en ;
  owl:sameAs <https://w3id.org/dpv#SubsidiaryLegalEntity>, <https://w3id.org/dpv/dpv-owl#SubsidiaryLegalEntity> .

<https://w3id.org/dpv/owl#EstablishContractualAgreement>
  a owl:Class, owl:NamedIndividual, <https://w3id.org/dpv/owl#Purpose> ;
  rdfs:subClassOf <https://w3id.org/dpv/owl#Purpose> ;
  dc:contributor _:genid4, _:genid1 ;
  dc:created "2022-11-09"^^xsd:date ;
  ns1:term_status "accepted"@en ;
  skos:definition "Purposes associated with carrying out data processing to establish an agreement, such as for entering into a contract"@en ;
  skos:prefLabel "Establish Contractual Agreement"@en ;
  owl:sameAs <https://w3id.org/dpv#EstablishContractualAgreement>, <https://w3id.org/dpv/dpv-owl#EstablishContractualAgreement> .

<https://w3id.org/dpv/owl#DataSubjectScale>
  a owl:Class ;
  rdfs:subClassOf <https://w3id.org/dpv/owl#Scale> ;
  dc:contributor _:genid65, _:genid4, _:genid1 ;
  dc:created "2022-06-15"^^xsd:date ;
  ns3:example <https://w3id.org/dpv/examples/owl#E0049> ;
  ns1:term_status "accepted"@en ;
  skos:definition "Scale of Data Subject(s)"@en ;
  skos:prefLabel "Data Subject Scale"@en ;
  owl:sameAs <https://w3id.org/dpv#DataSubjectScale>, <https://w3id.org/dpv/dpv-owl#DataSubjectScale> .

<https://w3id.org/dpv/owl#RecruitmentInterviewScheduling>
  a owl:Class, owl:NamedIndividual, <https://w3id.org/dpv/owl#Purpose> ;
  rdfs:subClassOf <https://w3id.org/dpv/owl#RecruitmentInterviewManagement> ;
  dc:created "2024-12-01"^^xsd:date ;
  ns1:term_status "accepted"@en ;
  skos:definition "Purposes associated with scheduling interviews for recruitment"@en ;
  skos:prefLabel "Recruitment Interview Scheduling"@en ;
  owl:sameAs <https://w3id.org/dpv#RecruitmentInterviewScheduling>, <https://w3id.org/dpv/dpv-owl#RecruitmentInterviewScheduling> .

<https://w3id.org/dpv/owl#ReversingProcessOutput>
  a owl:Class, owl:NamedIndividual, <https://w3id.org/dpv/owl#EntityPermissiveInvolvement> ;
  rdfs:subClassOf <https://w3id.org/dpv/owl#EntityPermissiveInvolvement> ;
  dc:contributor _:genid1, _:genid25, _:genid19 ;
  dc:created "2024-05-11"^^xsd:date ;
  ns1:term_status "accepted"@en ;
  skos:definition "Involvement where entity can reverse output of specified context"@en ;
  skos:prefLabel "Reversing Process Output"@en ;
  skos:scopeNote "Reversing of outputs indicate discarding the output and going back to the previous output. This is different from correction of output which allows modification of the output - implying continuation of the process."@en ;
  owl:sameAs <https://w3id.org/dpv#ReversingProcessOutput>, <https://w3id.org/dpv/dpv-owl#ReversingProcessOutput> .

<https://w3id.org/dpv/owl#AILiteracy>
  a owl:Class, owl:NamedIndividual, <https://w3id.org/dpv/owl#OrganisationalMeasure> ;
  rdfs:subClassOf <https://w3id.org/dpv/owl#DigitalLiteracy> ;
  dc:contributor _:genid1 ;
  dc:created "2024-05-17"^^xsd:date ;
  ns1:term_status "accepted"@en ;
  skos:definition "Providing skills, knowledge, and understanding to enable reading, writing, analysing, reasoning, and communicating regarding AI"@en ;
  skos:prefLabel "AI Literacy"@en ;
  owl:sameAs <https://w3id.org/dpv#AILiteracy>, <https://w3id.org/dpv/dpv-owl#AILiteracy> .

<https://w3id.org/dpv/owl#ReaffirmConsent>
  a owl:Class ;
  rdfs:subClassOf <https://w3id.org/dpv/owl#ConsentControl> ;
  dc:created "2024-05-11"^^xsd:date ;
  ns1:term_status "accepted"@en ;
  skos:definition "Control for affirming consent"@en ;
  skos:prefLabel "Reaffirm Consent"@en ;
  skos:scopeNote "Indicates how the controller (with dpv:ObtainConsent) or data subject (with dpv:ProvideConsent) can reaffirm consent e.g. used with dpv:isExercisedAt"@en ;
  owl:sameAs <https://w3id.org/dpv#ReaffirmConsent>, <https://w3id.org/dpv/dpv-owl#ReaffirmConsent> .

<https://w3id.org/dpv/owl#OptimiseUserInterface>
  a owl:Class, owl:NamedIndividual, <https://w3id.org/dpv/owl#Purpose> ;
  rdfs:subClassOf <https://w3id.org/dpv/owl#OptimisationForConsumer> ;
  dc:contributor _:genid13, _:genid14, _:genid1, _:genid15, _:genid16, _:genid11 ;
  dc:created "2019-04-05"^^xsd:date ;
  ns1:term_status "accepted"@en ;
  skos:definition "Purposes associated with optimisation of interfaces presented to the user"@en ;
  skos:prefLabel "Optimise User Interface"@en ;
  owl:sameAs <https://w3id.org/dpv#OptimiseUserInterface>, <https://w3id.org/dpv/dpv-owl#OptimiseUserInterface> .

odrl:#policySubClasses
  a owl:NamedIndividual, skos:Collection ;
  skos:member odrl:Agreement, odrl:Offer, odrl:Set ;
  skos:prefLabel "Policy Subclasses"@en ;
  skos:scopeNote "ODRL Core Vocabulary Terms"@en .

<https://w3id.org/dpv/owl#Compliant>
  a owl:Class, owl:NamedIndividual, <https://w3id.org/dpv/owl#ComplianceStatus> ;
  rdfs:subClassOf <https://w3id.org/dpv/owl#ComplianceStatus> ;
  dc:contributor _:genid1 ;
  dc:created "2022-05-18"^^xsd:date ;
  ns1:term_status "accepted"@en ;
  skos:definition "State of being fully compliant"@en ;
  skos:prefLabel "Compliant"@en ;
  owl:sameAs <https://w3id.org/dpv#Compliant>, <https://w3id.org/dpv/dpv-owl#Compliant> .

<https://w3id.org/dpv/owl#RequestAcknowledged>
  a owl:Class, owl:NamedIndividual, <https://w3id.org/dpv/owl#RequestStatus> ;
  rdfs:subClassOf <https://w3id.org/dpv/owl#RequestStatus> ;
  dc:contributor _:genid1 ;
  dc:created "2022-11-30"^^xsd:date ;
  ns1:term_status "accepted"@en ;
  skos:definition "State of a request being acknowledged"@en ;
  skos:prefLabel "Request Acknowledged"@en ;
  owl:sameAs <https://w3id.org/dpv#RequestAcknowledged>, <https://w3id.org/dpv/dpv-owl#RequestAcknowledged> .

<https://w3id.org/dpv/owl#RightNonFulfilmentNotice>
  a owl:Class, owl:NamedIndividual, <https://w3id.org/dpv/owl#OrganisationalMeasure> ;
  rdfs:subClassOf <https://w3id.org/dpv/owl#RightExerciseNotice> ;
  dc:contributor _:genid5, _:genid1 ;
  dc:created "2022-11-02"^^xsd:date ;
  ns3:example <https://w3id.org/dpv/examples/owl#E0058>, <https://w3id.org/dpv/examples/owl#E0061> ;
  ns1:term_status "accepted"@en ;
  skos:definition "Notice provided regarding non-fulfilment of a right"@en ;
  skos:prefLabel "Right Non-Fulfilment Notice"@en ;
  skos:scopeNote "This notice is associated with situations where information is provided with the intention of communicating non-fulfilment of a right. For example, to provide justifications on why a right could not be fulfilled or providing information about another entity  who should be approached for exercising this right."@en ;
  owl:sameAs <https://w3id.org/dpv#RightNonFulfilmentNotice>, <https://w3id.org/dpv/dpv-owl#RightNonFulfilmentNotice> .

<https://w3id.org/dpv/owl#Member>
  a owl:Class, owl:NamedIndividual, <https://w3id.org/dpv/owl#HumanSubject> ;
  rdfs:subClassOf <https://w3id.org/dpv/owl#HumanSubject> ;
  dc:contributor _:genid4, _:genid5, _:genid1, _:genid17, _:genid6 ;
  dc:created "2022-04-06"^^xsd:date ;
  dc:modified "2024-12-17"^^xsd:date ;
  ns1:term_status "modified"@en ;
  skos:definition "Humans that are members of a group, organisation, or other collectives"@en ;
  skos:prefLabel "Member"@en ;
  owl:sameAs <https://w3id.org/dpv#Member>, <https://w3id.org/dpv/dpv-owl#Member> .

<https://w3id.org/dpv/owl#AssetManagementProcedures>
  a owl:Class, owl:NamedIndividual, <https://w3id.org/dpv/owl#OrganisationalMeasure> ;
  rdfs:subClassOf <https://w3id.org/dpv/owl#GovernanceProcedures> ;
  dc:contributor _:genid1 ;
  dc:created "2022-08-17"^^xsd:date ;
  dc:source [
    a ns0:WebPage ;
    ns0:name "ENISA 5G Cybersecurity Standards" ;
    ns0:url "https://www.enisa.europa.eu/publications/5g-cybersecurity-standards"
  ] ;
  ns1:term_status "accepted"@en ;
  skos:definition "Procedures related to management of assets"@en ;
  skos:prefLabel "Asset Management Procedures"@en ;
  owl:sameAs <https://w3id.org/dpv#AssetManagementProcedures>, <https://w3id.org/dpv/dpv-owl#AssetManagementProcedures> .

<https://w3id.org/dpv/owl#EnvironmentalProtection>
  a owl:Class, owl:NamedIndividual, <https://w3id.org/dpv/owl#PhysicalMeasure> ;
  rdfs:subClassOf <https://w3id.org/dpv/owl#PhysicalMeasure> ;
  dc:contributor _:genid1 ;
  dc:created "2024-04-14"^^xsd:date ;
  dc:source "NIST SP 800-13"@en ;
  ns1:term_status "accepted"@en ;
  skos:definition "Physical protection against environmental threats such as fire, floods, storms, etc."@en ;
  skos:prefLabel "Environmental Protection"@en ;
  owl:sameAs <https://w3id.org/dpv#EnvironmentalProtection>, <https://w3id.org/dpv/dpv-owl#EnvironmentalProtection> .

<https://w3id.org/dpv/owl#LocalLocation>
  a owl:Class, owl:NamedIndividual, <https://w3id.org/dpv/owl#Location> ;
  rdfs:subClassOf <https://w3id.org/dpv/owl#LocationLocality> ;
  dc:contributor _:genid1 ;
  dc:created "2022-06-15"^^xsd:date ;
  dc:modified "2020-10-05"^^xsd:date ;
  ns1:term_status "accepted"@en ;
  skos:definition "Location is local"@en ;
  skos:prefLabel "Local Location"@en ;
  owl:sameAs <https://w3id.org/dpv#LocalLocation>, <https://w3id.org/dpv/dpv-owl#LocalLocation> .

<https://w3id.org/dpv/owl#ProtectionOfNationalSecurity>
  a owl:Class, owl:NamedIndividual, <https://w3id.org/dpv/owl#Purpose> ;
  rdfs:subClassOf <https://w3id.org/dpv/owl#PublicBenefit> ;
  dc:contributor _:genid5, _:genid1 ;
  dc:created "2024-02-14"^^xsd:date ;
  dc:source "DGA 1.5"@en ;
  ns1:term_status "accepted"@en ;
  skos:definition "Purposes associated with the protection of national security"@en ;
  skos:prefLabel "Protection of National Security"@en ;
  owl:sameAs <https://w3id.org/dpv#ProtectionOfNationalSecurity>, <https://w3id.org/dpv/dpv-owl#ProtectionOfNationalSecurity> .

odrl:#actionsCommon
  a owl:NamedIndividual, skos:Collection ;
  skos:member cc:Attribution, cc:CommercialUse, cc:DerivativeWorks, cc:Distribution, cc:Notice, cc:Reproduction, cc:ShareAlike, cc:Sharing, cc:SourceCode, odrl:acceptTracking, odrl:aggregate, odrl:annotate, odrl:anonymize, odrl:archive, odrl:attribute, odrl:compensate, odrl:concurrentUse, odrl:delete, odrl:derive, odrl:digitize, odrl:display, odrl:distribute, odrl:ensureExclusivity, odrl:execute, odrl:extract, odrl:give, odrl:grantUse, odrl:include, odrl:index, odrl:inform, odrl:install, odrl:modify, odrl:move, odrl:nextPolicy, odrl:obtainConsent, odrl:play, odrl:present, odrl:print, odrl:read, odrl:reproduce, odrl:reviewPolicy, odrl:sell, odrl:stream, odrl:synchronize, odrl:textToSpeech, odrl:transform, odrl:translate, odrl:uninstall, odrl:watermark ;
  skos:prefLabel "Actions for Rules"@en ;
  skos:scopeNote "ODRL Common Vocabulary Terms"@en .

<https://w3id.org/dpv/owl#isMitigatedByMeasure>
  a owl:ObjectProperty ;
  rdfs:subPropertyOf <https://w3id.org/dpv/owl#hasTechnicalOrganisationalMeasure> ;
  ns2:domainIncludes <https://w3id.org/dpv/owl#Risk> ;
  ns2:rangeIncludes <https://w3id.org/dpv/owl#RiskMitigationMeasure> ;
  dc:contributor _:genid1 ;
  dc:created "2022-02-09"^^xsd:date ;
  ns3:example <https://w3id.org/dpv/examples/owl#E0068> ;
  ns1:term_status "accepted"@en ;
  skos:definition "Indicate a risk is mitigated by specified measure"@en ;
  skos:prefLabel "is mitigated by measure"@en ;
  ns0:domainIncludes <https://w3id.org/dpv/owl#Risk> ;
  ns0:rangeIncludes <https://w3id.org/dpv/owl#RiskMitigationMeasure> ;
  owl:sameAs <https://w3id.org/dpv#isMitigatedByMeasure>, <https://w3id.org/dpv/dpv-owl#isMitigatedByMeasure> .

<https://w3id.org/dpv/owl#Derive>
  a owl:Class, owl:NamedIndividual, <https://w3id.org/dpv/owl#Processing> ;
  rdfs:subClassOf <https://w3id.org/dpv/owl#Obtain> ;
  dc:created "2019-05-07"^^xsd:date ;
  dc:source [
    a ns0:WebPage ;
    ns0:name "SPECIAL Project" ;
    ns0:url "https://specialprivacy.ercim.eu/vocabs/processing"
  ] ;
  ns3:example <https://w3id.org/dpv/examples/owl#E0009> ;
  ns1:term_status "accepted"@en ;
  skos:definition "to create new derivative data from the original data"@en ;
  skos:prefLabel "Derive Data"@en ;
  skos:related <https://specialprivacy.ercim.eu/vocabs/processing#Derive> ;
  skos:scopeNote "Derive indicates data is present or obtainable from existing data. For data that is created without such existence, see Infer."@en ;
  owl:sameAs <https://w3id.org/dpv#Derive>, <https://w3id.org/dpv/dpv-owl#Derive> .

<https://w3id.org/dpv/owl#LegitimateInterestOfThirdParty>
  a owl:Class, owl:NamedIndividual, <https://w3id.org/dpv/owl#LegalBasis> ;
  rdfs:subClassOf <https://w3id.org/dpv/owl#LegitimateInterest> ;
  dc:contributor _:genid4, _:genid1, _:genid6 ;
  dc:created "2021-05-19"^^xsd:date ;
  ns1:term_status "accepted"@en ;
  skos:definition "Legitimate Interests of a Third Party in conducting specified activities"@en ;
  skos:prefLabel "Legitimate Interest of Third Party"@en ;
  owl:sameAs <https://w3id.org/dpv#LegitimateInterestOfThirdParty>, <https://w3id.org/dpv/dpv-owl#LegitimateInterestOfThirdParty> .

<https://w3id.org/dpv/owl#NoticeUpdated>
  a owl:Class, owl:NamedIndividual, <https://w3id.org/dpv/owl#NoticeStatus> ;
  rdfs:subClassOf <https://w3id.org/dpv/owl#NoticeStatus> ;
  dc:contributor _:genid4, _:genid1 ;
  dc:created "2024-12-01"^^xsd:date ;
  ns1:term_status "accepted"@en ;
  skos:definition "Status indicating the notice has been updated and its contents or implications have changed"@en ;
  skos:prefLabel "Notice Updated"@en ;
  owl:sameAs <https://w3id.org/dpv#NoticeUpdated>, <https://w3id.org/dpv/dpv-owl#NoticeUpdated> .

<https://w3id.org/dpv/owl#isAuthorityFor>
  a owl:ObjectProperty ;
  ns2:domainIncludes <https://w3id.org/dpv/owl#Authority> ;
  dc:contributor _:genid4, _:genid1 ;
  dc:created "2022-01-19"^^xsd:date ;
  ns1:term_status "accepted"@en ;
  skos:definition "Indicates area, scope, or applicability of an Authority"@en ;
  skos:prefLabel "is authority for"@en ;
  ns0:domainIncludes <https://w3id.org/dpv/owl#Authority> ;
  owl:sameAs <https://w3id.org/dpv#isAuthorityFor>, <https://w3id.org/dpv/dpv-owl#isAuthorityFor> .

<https://w3id.org/dpv/owl#ThirdPartyContract>
  a owl:Class, owl:NamedIndividual, <https://w3id.org/dpv/owl#LegalBasis> ;
  rdfs:subClassOf <https://w3id.org/dpv/owl#DataProcessingAgreement> ;
  dc:created "2023-12-10"^^xsd:date ;
  dc:modified "2024-08-27"^^xsd:date ;
  ns1:term_status "sunset"@en ;
  skos:definition "Creation, completion, fulfilment, or performance of a contract, with the Data Controller and Third Party as parties, and involving specified processing of data or technologies. NOTE: This concept is being deprecated - use dpv:ThirdPartyAgreement which has a more explicit definition of the entities involved and the intent of the contract"@en ;
  skos:prefLabel "Third Party Contract"@en ;
  owl:sameAs <https://w3id.org/dpv#ThirdPartyContract>, <https://w3id.org/dpv/dpv-owl#ThirdPartyContract> .

<https://w3id.org/dpv/owl#VitalInterestCompleted>
  a owl:Class, owl:NamedIndividual, <https://w3id.org/dpv/owl#VitalInterestStatus> ;
  rdfs:subClassOf <https://w3id.org/dpv/owl#VitalInterestStatus> ;
  dc:created "2024-08-27"^^xsd:date ;
  ns1:term_status "accepted"@en ;
  skos:definition "Status where the vital interest activity has been completed"@en ;
  skos:prefLabel "Vital Interest Completed"@en ;
  owl:sameAs <https://w3id.org/dpv#VitalInterestCompleted>, <https://w3id.org/dpv/dpv-owl#VitalInterestCompleted> .

<https://w3id.org/dpv/owl#Organisation>
  a owl:Class ;
  rdfs:subClassOf <https://w3id.org/dpv/owl#LegalEntity> ;
  dc:contributor _:genid1 ;
  dc:created "2022-02-02"^^xsd:date ;
  ns1:term_status "accepted"@en ;
  skos:definition "A general term reflecting a company or a business or a group acting as a unit"@en ;
  skos:prefLabel "Organisation"@en ;
  owl:sameAs <https://w3id.org/dpv#Organisation>, <https://w3id.org/dpv/dpv-owl#Organisation> .

<https://w3id.org/dpv/owl#hasApplicability>
  a owl:ObjectProperty ;
  ns2:rangeIncludes <https://w3id.org/dpv/owl#Applicability> ;
  dc:contributor _:genid1 ;
  dc:created "2023-08-24"^^xsd:date ;
  ns3:example <https://w3id.org/dpv/examples/owl#E0053> ;
  ns1:term_status "accepted"@en ;
  skos:definition "Indicates situations where the context is not applicable, information is not available, or this is unknown. An appropriate instance of dpv:Applicability should be used with this relation to express the situation"@en ;
  skos:prefLabel "has applicability"@en ;
  ns0:rangeIncludes <https://w3id.org/dpv/owl#Applicability> ;
  owl:sameAs <https://w3id.org/dpv#hasApplicability>, <https://w3id.org/dpv/dpv-owl#hasApplicability> .

<https://w3id.org/dpv/owl#SecondaryImportance>
  a owl:Class, owl:NamedIndividual, <https://w3id.org/dpv/owl#Importance> ;
  rdfs:subClassOf <https://w3id.org/dpv/owl#Importance> ;
  dc:contributor _:genid4, _:genid5, _:genid1, _:genid17, _:genid6 ;
  dc:created "2022-02-11"^^xsd:date ;
  ns1:term_status "accepted"@en ;
  skos:definition "Indication of 'secondary' or 'minor' or 'auxiliary' importance"@en ;
  skos:prefLabel "Secondary Importance"@en ;
  owl:sameAs <https://w3id.org/dpv#SecondaryImportance>, <https://w3id.org/dpv/dpv-owl#SecondaryImportance> .

odrl:Asset
  a owl:Class, owl:NamedIndividual, skos:Concept ;
  rdfs:isDefinedBy odrl: ;
  rdfs:label "Asset"@en ;
  skos:definition "A resource or a collection of resources that are the subject of a Rule."@en ;
  skos:note "The Asset entity can be any form of identifiable resource, such as data/information, content/media, applications, or services. Furthermore, it can be used to represent other Asset entities that are needed to undertake the Policy expression, such as with the Duty entity. To describe more details about the Asset, it is recommended to use Dublin Core [[dcterms]] elements or other content metadata."@en .

<https://w3id.org/dpv/owl#VulnerableHuman>
  a owl:Class, owl:NamedIndividual, <https://w3id.org/dpv/owl#HumanSubject> ;
  rdfs:subClassOf <https://w3id.org/dpv/owl#HumanSubject> ;
  dc:contributor _:genid1 ;
  dc:created "2024-12-17"^^xsd:date ;
  ns1:term_status "accepted"@en ;
  skos:definition "Human(s) which should be considered 'vulnerable' within the context"@en ;
  skos:prefLabel "Vulnerable Human"@en ;
  owl:sameAs <https://w3id.org/dpv#VulnerableHuman>, <https://w3id.org/dpv/dpv-owl#VulnerableHuman> .

odrl:obligation
  a owl:ObjectProperty, owl:NamedIndividual, skos:Concept ;
  rdfs:domain odrl:Policy ;
  rdfs:range odrl:Duty ;
  rdfs:isDefinedBy odrl: ;
  rdfs:label "Obligation"@en ;
  skos:definition "Relates an individual Duty to a Policy."@en ;
  skos:note "The Duty is a requirement which must be fulfilled."@en .

<https://w3id.org/dpv/owl#RequestAccepted>
  a owl:Class, owl:NamedIndividual, <https://w3id.org/dpv/owl#RequestStatus> ;
  rdfs:subClassOf <https://w3id.org/dpv/owl#RequestStatus> ;
  dc:contributor _:genid1 ;
  dc:created "2022-11-30"^^xsd:date ;
  ns1:term_status "accepted"@en ;
  skos:definition "State of a request being accepted towards fulfilment"@en ;
  skos:prefLabel "Request Accepted"@en ;
  owl:sameAs <https://w3id.org/dpv#RequestAccepted>, <https://w3id.org/dpv/dpv-owl#RequestAccepted> .

<https://w3id.org/dpv/owl#VitalInterestObjected>
  a owl:Class, owl:NamedIndividual, <https://w3id.org/dpv/owl#VitalInterestStatus> ;
  rdfs:subClassOf <https://w3id.org/dpv/owl#VitalInterestStatus> ;
  dc:created "2024-08-27"^^xsd:date ;
  ns1:term_status "accepted"@en ;
  skos:definition "Status where the vital interest activity was objected to by the Data Subject or another relevant entity"@en ;
  skos:prefLabel "Vital Interest Objected"@en ;
  owl:sameAs <https://w3id.org/dpv#VitalInterestObjected>, <https://w3id.org/dpv/dpv-owl#VitalInterestObjected> .

<https://w3id.org/dpv/owl#ComplianceViolation>
  a owl:Class, owl:NamedIndividual, <https://w3id.org/dpv/owl#ComplianceStatus> ;
  rdfs:subClassOf <https://w3id.org/dpv/owl#ComplianceStatus> ;
  dc:contributor _:genid1 ;
  dc:created "2022-05-18"^^xsd:date ;
  dc:modified "2022-09-07"^^xsd:date ;
  ns1:term_status "accepted"@en ;
  skos:definition "State where compliance cannot be achieved due to requirements being violated"@en ;
  skos:prefLabel "Compliance Violation"@en ;
  skos:scopeNote "Changed from \"violation of compliance\" for consistency with other terms"@en ;
  owl:sameAs <https://w3id.org/dpv#ComplianceViolation>, <https://w3id.org/dpv/dpv-owl#ComplianceViolation> .

<https://w3id.org/dpv/owl#SecurityMethod>
  a owl:Class, owl:NamedIndividual, <https://w3id.org/dpv/owl#TechnicalMeasure> ;
  rdfs:subClassOf <https://w3id.org/dpv/owl#TechnicalMeasure> ;
  dc:contributor _:genid1 ;
  dc:created "2022-08-24"^^xsd:date ;
  ns1:term_status "accepted"@en ;
  skos:definition "Methods that relate to creating and providing security"@en ;
  skos:prefLabel "Security Method"@en ;
  owl:sameAs <https://w3id.org/dpv#SecurityMethod>, <https://w3id.org/dpv/dpv-owl#SecurityMethod> .

<https://w3id.org/dpv/owl#EntityInformed>
  a owl:Class, owl:NamedIndividual, <https://w3id.org/dpv/owl#EntityInformedStatus> ;
  rdfs:subClassOf <https://w3id.org/dpv/owl#EntityInformedStatus> ;
  dc:contributor _:genid4, _:genid1, _:genid25, _:genid6 ;
  dc:created "2024-05-10"^^xsd:date ;
  ns1:term_status "accepted"@en ;
  skos:definition "Status indicating entity has been informed about specified context"@en ;
  skos:prefLabel "Entity Informed"@en ;
  owl:sameAs <https://w3id.org/dpv#EntityInformed>, <https://w3id.org/dpv/dpv-owl#EntityInformed> .

<https://w3id.org/dpv/owl#LegalObligationPending>
  a owl:Class, owl:NamedIndividual, <https://w3id.org/dpv/owl#LegalObligationStatus> ;
  rdfs:subClassOf <https://w3id.org/dpv/owl#LegalObligationStatus> ;
  dc:created "2024-08-27"^^xsd:date ;
  ns1:term_status "accepted"@en ;
  skos:definition "Status where the legal obligation has not been started"@en ;
  skos:prefLabel "Legal ObligationPending"@en ;
  owl:sameAs <https://w3id.org/dpv#LegalObligationPending>, <https://w3id.org/dpv/dpv-owl#LegalObligationPending> .

<https://w3id.org/dpv/owl#IPRManagement>
  a owl:Class, owl:NamedIndividual, <https://w3id.org/dpv/owl#OrganisationalMeasure> ;
  rdfs:subClassOf <https://w3id.org/dpv/owl#RightsManagement> ;
  dc:contributor _:genid4, _:genid5, _:genid1 ;
  dc:created "2024-04-14"^^xsd:date ;
  dc:source "DGA 3.1.c"@en ;
  ns1:term_status "accepted"@en ;
  skos:definition "Management of Intellectual Property Rights with a view to identify and safeguard and enforce them"@en ;
  skos:prefLabel "Intellectual Property Rights Management"@en ;
  owl:sameAs <https://w3id.org/dpv#IPRManagement>, <https://w3id.org/dpv/dpv-owl#IPRManagement> .

<https://w3id.org/dpv/owl#ContractJurisdictionClause>
  a owl:Class, owl:NamedIndividual, <https://w3id.org/dpv/owl#ContractualClause> ;
  rdfs:subClassOf <https://w3id.org/dpv/owl#ContractualClause> ;
  dc:created "2024-08-27"^^xsd:date ;
  ns1:term_status "accepted"@en ;
  skos:definition "A provision specifying the legal jurisdiction or court where disputes related to the contract will be resolved"@en ;
  skos:prefLabel "Contract Jurisdiction Clause"@en ;
  owl:sameAs <https://w3id.org/dpv#ContractJurisdictionClause>, <https://w3id.org/dpv/dpv-owl#ContractJurisdictionClause> .

<https://w3id.org/dpv/owl#Scale>
  a owl:Class ;
  rdfs:subClassOf <https://w3id.org/dpv/owl#ProcessingContext> ;
  dc:contributor _:genid65, _:genid4, _:genid1 ;
  dc:created "2022-06-15"^^xsd:date ;
  ns1:term_status "accepted"@en ;
  skos:definition "A measurement along some dimension"@en ;
  skos:prefLabel "Scale"@en ;
  skos:scopeNote "Scales are subjective concepts that need to be defined and interpreted within the context of their application. For example, what would be small within one context could be large within another."@en ;
  owl:sameAs <https://w3id.org/dpv#Scale>, <https://w3id.org/dpv/dpv-owl#Scale> .

odrl:action
  a owl:ObjectProperty, owl:NamedIndividual, skos:Concept ;
  rdfs:domain [
    a owl:Class ;
    owl:unionOf (
     odrl:Policy
     odrl:Rule
   )
  ] ;
  rdfs:range odrl:Action ;
  rdfs:isDefinedBy odrl: ;
  rdfs:label "Has Action"@en ;
  skos:definition "The operation relating to the Asset for which the Rule is being subjected."@en .

<https://w3id.org/dpv/owl#InvolvementStatus>
  a owl:Class ;
  rdfs:subClassOf <https://w3id.org/dpv/owl#Status> ;
  dc:contributor _:genid4, _:genid1, _:genid25, _:genid6 ;
  dc:created "2024-05-10"^^xsd:date ;
  ns1:term_status "accepted"@en ;
  skos:definition "Status indicating whether the involvement of specified context"@en ;
  skos:prefLabel "Involvement Status"@en ;
  owl:sameAs <https://w3id.org/dpv#InvolvementStatus>, <https://w3id.org/dpv/dpv-owl#InvolvementStatus> .

<https://w3id.org/dpv/owl#LegalObligation>
  a owl:Class, owl:NamedIndividual, <https://w3id.org/dpv/owl#LegalBasis> ;
  rdfs:subClassOf <https://w3id.org/dpv/owl#LegalBasis> ;
  dc:contributor _:genid1 ;
  dc:created "2021-04-07"^^xsd:date ;
  ns3:example <https://w3id.org/dpv/examples/owl#E0042>, <https://w3id.org/dpv/examples/owl#E0079> ;
  ns1:term_status "accepted"@en ;
  skos:definition "Legal Obligation to conduct the specified activities"@en ;
  skos:prefLabel "Legal Obligation"@en ;
  owl:sameAs <https://w3id.org/dpv#LegalObligation>, <https://w3id.org/dpv/dpv-owl#LegalObligation> .

<https://w3id.org/dpv/owl#Consent>
  a owl:Class, owl:NamedIndividual, <https://w3id.org/dpv/owl#LegalBasis> ;
  rdfs:subClassOf <https://w3id.org/dpv/owl#LegalBasis> ;
  dc:contributor _:genid1 ;
  dc:created "2021-04-07"^^xsd:date ;
  ns3:example <https://w3id.org/dpv/examples/owl#E0015>, <https://w3id.org/dpv/examples/owl#E0018> ;
  ns1:term_status "accepted"@en ;
  skos:definition "Consent of the Data Subject for specified process or activity"@en ;
  skos:prefLabel "Consent"@en ;
  owl:sameAs <https://w3id.org/dpv#Consent>, <https://w3id.org/dpv/dpv-owl#Consent> .

<https://w3id.org/dpv/owl#NoticeCommunicated>
  a owl:Class, owl:NamedIndividual, <https://w3id.org/dpv/owl#NoticeStatus> ;
  rdfs:subClassOf <https://w3id.org/dpv/owl#NoticeStatus> ;
  dc:contributor _:genid4, _:genid1 ;
  dc:created "2024-12-01"^^xsd:date ;
  ns1:term_status "accepted"@en ;
  skos:definition "Status indicating the notice has been communicated"@en ;
  skos:prefLabel "Notice Communicated"@en ;
  owl:sameAs <https://w3id.org/dpv#NoticeCommunicated>, <https://w3id.org/dpv/dpv-owl#NoticeCommunicated> .

<https://w3id.org/dpv/owl#PublicDataSource>
  a owl:Class, owl:NamedIndividual, <https://w3id.org/dpv/owl#DataSource> ;
  rdfs:subClassOf <https://w3id.org/dpv/owl#DataSource> ;
  dc:contributor _:genid4, _:genid5, _:genid1, _:genid17, _:genid6 ;
  dc:created "2022-01-26"^^xsd:date ;
  ns1:term_status "accepted"@en ;
  skos:definition "A source of data that is publicly accessible or available"@en ;
  skos:prefLabel "Public Data Source"@en ;
  skos:scopeNote "The term 'Public' is used here in a broad sense. Actual consideration of what is 'Public Data' can vary based on several contextual or jurisdictional factors such as  definition of open, methods of access, permissions and licenses."@en ;
  owl:sameAs <https://w3id.org/dpv#PublicDataSource>, <https://w3id.org/dpv/dpv-owl#PublicDataSource> .

<https://w3id.org/dpv/owl#ContractOffered>
  a owl:Class, owl:NamedIndividual, <https://w3id.org/dpv/owl#ContractPreparationStatus> ;
  rdfs:subClassOf <https://w3id.org/dpv/owl#ContractPreparationStatus> ;
  dc:contributor _:genid4, _:genid1, _:genid17 ;
  dc:created "2025-01-09"^^xsd:date ;
  ns1:term_status "accepted"@en ;
  skos:definition "Status representing contract has been offered to a party or to parties for reviewing and signing"@en ;
  skos:prefLabel "Contract Offered"@en ;
  owl:sameAs <https://w3id.org/dpv#ContractOffered>, <https://w3id.org/dpv/dpv-owl#ContractOffered> .

<https://w3id.org/dpv/owl#HumanInvolvementForInput>
  a owl:Class, owl:NamedIndividual, <https://w3id.org/dpv/owl#HumanInvolvement> ;
  rdfs:subClassOf <https://w3id.org/dpv/owl#HumanInvolvement> ;
  dc:contributor _:genid1 ;
  dc:created "2022-09-07"^^xsd:date ;
  dc:modified "2023-12-10"^^xsd:date ;
  ns1:term_status "accepted"@en ;
  skos:definition "Human involvement for the purposes of providing inputs to the specified context"@en ;
  skos:prefLabel "Human Involvement for Input"@en ;
  skos:scopeNote "Inputs can be in the form of data or other resources."@en ;
  owl:sameAs <https://w3id.org/dpv#HumanInvolvementForInput>, <https://w3id.org/dpv/dpv-owl#HumanInvolvementForInput> .

<https://w3id.org/dpv/owl#isImplementedByEntity>
  a owl:ObjectProperty ;
  ns2:domainIncludes <https://w3id.org/dpv/owl#RightExerciseActivity> ;
  ns2:rangeIncludes <https://w3id.org/dpv/owl#Entity> ;
  dc:contributor _:genid5, _:genid1, _:genid17, _:genid6, _:genid11 ;
  dc:created "2019-05-07"^^xsd:date ;
  dc:modified "2022-01-26"^^xsd:date ;
  ns3:example <https://w3id.org/dpv/examples/owl#E0037>, <https://w3id.org/dpv/examples/owl#E0085> ;
  ns1:term_status "accepted"@en ;
  skos:definition "Indicates implementation details such as entities or agents"@en ;
  skos:prefLabel "is implemented by entity"@en ;
  skos:scopeNote "Also used to indicate the Entity that implements or performs a Right Exercise Activity"@en, "The use of 'entity' is inclusive of entities (e.g. Data Processor) as well as 'agent' (e.g. DPO). For indicating technological implementation, the property isImplementedByTechnology should be used."@en ;
  ns0:domainIncludes <https://w3id.org/dpv/owl#RightExerciseActivity> ;
  ns0:rangeIncludes <https://w3id.org/dpv/owl#Entity> ;
  owl:sameAs <https://w3id.org/dpv#isImplementedByEntity>, <https://w3id.org/dpv/dpv-owl#isImplementedByEntity> .

<https://w3id.org/dpv/owl#LayeredNotice>
  a owl:Class, owl:NamedIndividual, <https://w3id.org/dpv/owl#OrganisationalMeasure> ;
  rdfs:subClassOf <https://w3id.org/dpv/owl#Notice> ;
  dc:created "2024-08-17"^^xsd:date ;
  dc:source [
    a ns0:WebPage ;
    ns0:name "ICO - What methods can we use to provide privacy information?" ;
    ns0:url "https://ico.org.uk/for-organisations/uk-gdpr-guidance-and-resources/individual-rights/the-right-to-be-informed/what-methods-can-we-use-to-provide-privacy-information/"
  ] ;
  ns1:term_status "accepted"@en ;
  skos:definition "A notice that contains layered elements"@en ;
  skos:prefLabel "Layered Notice"@en ;
  owl:sameAs <https://w3id.org/dpv#LayeredNotice>, <https://w3id.org/dpv/dpv-owl#LayeredNotice> .

<https://w3id.org/dpv/owl#Transmit>
  a owl:Class, owl:NamedIndividual, <https://w3id.org/dpv/owl#Processing> ;
  rdfs:subClassOf <https://w3id.org/dpv/owl#Disclose> ;
  dc:created "2019-05-07"^^xsd:date ;
  dc:source [
    a ns0:WebPage ;
    ns0:name "GDPR Art.4-2" ;
    ns0:url "https://eur-lex.europa.eu/eli/reg/2016/679/art_4/par_2/oj"
  ] ;
  ns1:term_status "accepted"@en ;
  skos:definition "to send out data"@en ;
  skos:prefLabel "Transmit Data"@en ;
  owl:sameAs <https://w3id.org/dpv#Transmit>, <https://w3id.org/dpv/dpv-owl#Transmit> .

<https://w3id.org/dpv/owl#JobApplicant>
  a owl:Class, owl:NamedIndividual, <https://w3id.org/dpv/owl#HumanSubject> ;
  rdfs:subClassOf <https://w3id.org/dpv/owl#HumanSubject> ;
  dc:contributor _:genid4, _:genid5, _:genid1, _:genid17, _:genid6 ;
  dc:created "2022-04-06"^^xsd:date ;
  dc:modified "2024-12-17"^^xsd:date ;
  ns1:term_status "modified"@en ;
  skos:definition "Humans that apply for jobs or employments"@en ;
  skos:prefLabel "Job Applicant"@en ;
  owl:sameAs <https://w3id.org/dpv#JobApplicant>, <https://w3id.org/dpv/dpv-owl#JobApplicant> .

odrl:Assertion
  a owl:Class, owl:NamedIndividual, skos:Concept ;
  rdfs:subClassOf odrl:Policy ;
  owl:disjointWith odrl:Offer, odrl:Privacy, odrl:Request, odrl:Set, odrl:Ticket ;
  rdfs:isDefinedBy odrl: ;
  rdfs:label "Assertion"@en ;
  skos:definition "A Policy that asserts a Rule over an Asset from parties."@en ;
  skos:note "For example, a party (an assignee or assigner) can claim what terms they have over an Asset. An Assertion Policy does not grant such permissions/prohibitions but only asserts the parties claims. An Assetion Policy  MUST contain a target Asset, a Party with any functional role, and at least one of a Permission or Prohibition rule."@en ;
  skos:scopeNote "Non-Normative"@en .

odrl:constraint
  a owl:ObjectProperty, owl:NamedIndividual, skos:Concept ;
  rdfs:domain [
    a owl:Class ;
    owl:unionOf (
     odrl:Policy
     odrl:Rule
   )
  ] ;
  rdfs:range [
    a owl:Class ;
    owl:unionOf (
     odrl:Constraint
     odrl:LogicalConstraint
   )
  ] ;
  rdfs:isDefinedBy odrl: ;
  rdfs:label "Has Constraint"@en ;
  skos:definition "Constraint applied to a Rule"@en ;
  skos:note "Constraints on Rules are used to determine if a rule is Active or not. Example: the Permission rule is only active during the year 2018."@en .

<https://w3id.org/dpv/owl#EntityUninformed>
  a owl:Class ;
  rdfs:subClassOf <https://w3id.org/dpv/owl#EntityInformedStatus> ;
  dc:contributor _:genid4, _:genid1, _:genid25, _:genid6 ;
  dc:created "2024-05-10"^^xsd:date ;
  ns1:term_status "accepted"@en ;
  skos:definition "Status indicating entity is uninformed i.e. has been not been informed about specified context"@en ;
  skos:prefLabel "Entity Uninformed"@en ;
  owl:sameAs <https://w3id.org/dpv#EntityUninformed>, <https://w3id.org/dpv/dpv-owl#EntityUninformed> .

odrl:uninstall
  a owl:NamedIndividual, skos:Concept, odrl:Action ;
  odrl:includedIn odrl:use ;
  rdfs:isDefinedBy odrl: ;
  rdfs:label "Uninstall"@en ;
  skos:definition "To unload and delete the computer program Asset from a storage device and disable its readiness for operation."@en ;
  skos:note "The Asset is no longer accessible to the assignees after it has been used."@en ;
  skos:scopeNote "Non-Normative"@en .

<https://w3id.org/dpv/owl#LegalComplianceAudit>
  a owl:Class, owl:NamedIndividual, <https://w3id.org/dpv/owl#OrganisationalMeasure> ;
  rdfs:subClassOf <https://w3id.org/dpv/owl#Audit> ;
  dc:contributor _:genid1 ;
  dc:created "2024-12-17"^^xsd:date ;
  ns1:term_status "accepted"@en ;
  skos:definition "An audit that systematically examines the state of legal compliance by reviewing policies and procedures related to obligations and compliance requirements for specific laws and regulations"@en ;
  skos:prefLabel "Legal Compliance Audit"@en ;
  owl:sameAs <https://w3id.org/dpv#LegalComplianceAudit>, <https://w3id.org/dpv/dpv-owl#LegalComplianceAudit> .

<https://eu-upcast.github.io/vocabulary/index-en.html#hasApprovalFrom>
  a owl:ObjectProperty ;
  rdfs:domain odrl:purpose ;
  rdfs:comment "Defines the party, tool or organisation that agrees to or approves a specific purpose." ;
  rdfs:label "has approval from"@en .

<https://w3id.org/dpv/owl#isIndicatedBy>
  a owl:ObjectProperty ;
  ns2:rangeIncludes <https://w3id.org/dpv/owl#Entity> ;
  dc:contributor _:genid4, _:genid1, _:genid17, _:genid6 ;
  dc:created "2022-06-21"^^xsd:date ;
  ns1:term_status "accepted"@en ;
  skos:definition "Specifies entity who indicates the specific context"@en ;
  skos:prefLabel "is indicated by"@en ;
  ns0:rangeIncludes <https://w3id.org/dpv/owl#Entity> ;
  owl:sameAs <https://w3id.org/dpv#isIndicatedBy>, <https://w3id.org/dpv/dpv-owl#isIndicatedBy> .

<https://w3id.org/dpv/owl#ContinuousFrequency>
  a owl:Class, owl:NamedIndividual, <https://w3id.org/dpv/owl#Frequency> ;
  rdfs:subClassOf <https://w3id.org/dpv/owl#Frequency> ;
  dc:contributor _:genid1 ;
  dc:created "2022-06-15"^^xsd:date ;
  dc:modified "2020-10-05"^^xsd:date ;
  ns1:term_status "accepted"@en ;
  skos:definition "Frequency where occurrences are continuous"@en ;
  skos:prefLabel "Continuous Frequency"@en ;
  owl:sameAs <https://w3id.org/dpv#ContinuousFrequency>, <https://w3id.org/dpv/dpv-owl#ContinuousFrequency> .

odrl:Set
  a owl:Class, owl:NamedIndividual, skos:Concept ;
  rdfs:subClassOf odrl:Policy ;
  owl:disjointWith odrl:Ticket ;
  rdfs:isDefinedBy odrl: ;
  rdfs:label "Set"@en ;
  skos:definition "A Policy that expresses a Rule over an Asset."@en ;
  skos:note "A Set Policy MUST contain a target Asset, and at least one Rule. A Set Policy is the default Policy subclass. The Set is aimed at scenarios where there is an open criteria for the semantics of the policy expressions and typically refined by other systems/profiles that process the information at a later time. No privileges are granted to any Party (if defined)."@en .

<https://w3id.org/dpv/owl#MultiFactorAuthentication>
  a owl:Class, owl:NamedIndividual, <https://w3id.org/dpv/owl#TechnicalMeasure> ;
  rdfs:subClassOf <https://w3id.org/dpv/owl#AuthenticationProtocols> ;
  dc:contributor _:genid1 ;
  dc:created "2022-08-17"^^xsd:date ;
  dc:source [
    a ns0:WebPage ;
    ns0:name "ENISA Reference Incident Classification Taxonomy 2018" ;
    ns0:url "https://www.enisa.europa.eu/publications/reference-incident-classification-taxonomy/"
  ] ;
  ns1:term_status "accepted"@en ;
  skos:definition "An authentication system that uses two or more methods to authenticate"@en ;
  skos:prefLabel "Multi-Factor Authentication (MFA)"@en ;
  owl:sameAs <https://w3id.org/dpv#MultiFactorAuthentication>, <https://w3id.org/dpv/dpv-owl#MultiFactorAuthentication> .

<https://w3id.org/dpv/owl#NotAutomated>
  a owl:Class, owl:NamedIndividual, <https://w3id.org/dpv/owl#AutomationLevel> ;
  rdfs:subClassOf <https://w3id.org/dpv/owl#AutomationLevel> ;
  dc:contributor _:genid1, _:genid25 ;
  dc:created "2023-12-10"^^xsd:date ;
  dc:modified "2024-04-20"^^xsd:date ;
  dc:source [
    a ns0:WebPage ;
    ns0:name "ISO/IEC 22989:2022 Artificial intelligence concepts and terminology" ;
    ns0:url "https://www.iso.org/standard/74296.html"
  ] ;
  ns1:term_status "accepted"@en ;
  skos:definition "Level of automation corresponding to Level 0 in ISO/IEC 22989:2022 where there is no automation in the system"@en ;
  skos:prefLabel "Not Automated"@en ;
  skos:scopeNote "Human Involvement is necessary here as there is no automation"@en ;
  owl:sameAs <https://w3id.org/dpv#NotAutomated>, <https://w3id.org/dpv/dpv-owl#NotAutomated> .

<https://w3id.org/dpv/owl#Prohibition>
  a owl:Class, owl:NamedIndividual, <https://w3id.org/dpv/owl#Rule> ;
  rdfs:subClassOf <https://w3id.org/dpv/owl#Rule> ;
  dc:contributor _:genid4, _:genid5, _:genid1, _:genid6 ;
  dc:created "2022-10-19"^^xsd:date ;
  ns3:example <https://w3id.org/dpv/examples/owl#E0029>, <https://w3id.org/dpv/examples/owl#E0066> ;
  ns1:term_status "accepted"@en ;
  skos:definition "A rule describing a prohibition to perform an activity"@en ;
  skos:prefLabel "Prohibition"@en ;
  owl:sameAs <https://w3id.org/dpv#Prohibition>, <https://w3id.org/dpv/dpv-owl#Prohibition> .

<https://w3id.org/dpv/owl#Move>
  a owl:Class, owl:NamedIndividual, <https://w3id.org/dpv/owl#Processing> ;
  rdfs:subClassOf <https://w3id.org/dpv/owl#Transfer> ;
  dc:created "2019-05-07"^^xsd:date ;
  dc:source [
    a ns0:WebPage ;
    ns0:name "SPECIAL Project" ;
    ns0:url "https://specialprivacy.ercim.eu/vocabs/processing"
  ] ;
  ns1:term_status "accepted"@en ;
  skos:definition "to move data from one location to another including deleting the original copy"@en ;
  skos:prefLabel "Move Data"@en ;
  skos:related <https://specialprivacy.ercim.eu/vocabs/processing#Move> ;
  owl:sameAs <https://w3id.org/dpv#Move>, <https://w3id.org/dpv/dpv-owl#Move> .

<https://w3id.org/dpv/owl#AutomationLevel>
  a owl:Class ;
  rdfs:subClassOf <https://w3id.org/dpv/owl#ProcessingContext> ;
  dc:contributor _:genid1, _:genid25 ;
  dc:created "2023-12-10"^^xsd:date ;
  dc:modified "2024-04-20"^^xsd:date ;
  dc:source [
    a ns0:WebPage ;
    ns0:name "ISO/IEC 22989:2022 Artificial intelligence concepts and terminology" ;
    ns0:url "https://www.iso.org/standard/74296.html"
  ] ;
  ns3:example <https://w3id.org/dpv/examples/owl#E0013> ;
  ns1:term_status "accepted"@en ;
  skos:definition "Indication of degree or level of automation associated with specified context"@en ;
  skos:prefLabel "Automation Level"@en ;
  skos:scopeNote "This concept was called 'Automation' in previous versions"@en ;
  owl:sameAs <https://w3id.org/dpv#AutomationLevel>, <https://w3id.org/dpv/dpv-owl#AutomationLevel> .

odrl:relativeSize
  a owl:NamedIndividual, skos:Concept, odrl:LeftOperand ;
  rdfs:isDefinedBy odrl: ;
  rdfs:label "Relative Asset Size"@en ;
  skos:definition "Measure(s) of one or two axes for 2D-objects or measure(s) of one to tree axes for 3D-objects - expressed as percentages of full values - of the target Asset."@en ;
  skos:note "Example: The image can be resized in width to a maximum of 200%. Note: See the Left Operand absoluteSize. "@en ;
  skos:scopeNote "Non-Normative"@en .

<https://w3id.org/dpv/owl#ContractExtended>
  a owl:Class, owl:NamedIndividual, <https://w3id.org/dpv/owl#ContractTerminationStatus> ;
  rdfs:subClassOf <https://w3id.org/dpv/owl#ContractTerminationStatus> ;
  dc:contributor _:genid4, _:genid1, _:genid17 ;
  dc:created "2025-01-09"^^xsd:date ;
  ns1:term_status "accepted"@en ;
  skos:definition "Status representing the duration associated with a contract being extended through mutual agreement or by a party"@en ;
  skos:prefLabel "Contract Extended"@en ;
  owl:sameAs <https://w3id.org/dpv#ContractExtended>, <https://w3id.org/dpv/dpv-owl#ContractExtended> .

<https://w3id.org/dpv/owl#hasOrganisationalUnit>
  a owl:ObjectProperty ;
  rdfs:subPropertyOf <https://w3id.org/dpv/owl#hasEntity> ;
  ns2:domainIncludes <https://w3id.org/dpv/owl#Entity> ;
  ns2:rangeIncludes <https://w3id.org/dpv/owl#OrganisationalUnit> ;
  dc:contributor _:genid1 ;
  dc:created "2024-06-10"^^xsd:date ;
  ns1:term_status "accepted"@en ;
  skos:definition "Indicates the specified entity is a unit of the organisation"@en ;
  skos:prefLabel "has organisational unit"@en ;
  ns0:domainIncludes <https://w3id.org/dpv/owl#Entity> ;
  ns0:rangeIncludes <https://w3id.org/dpv/owl#OrganisationalUnit> ;
  owl:sameAs <https://w3id.org/dpv#hasOrganisationalUnit>, <https://w3id.org/dpv/dpv-owl#hasOrganisationalUnit> .

<https://w3id.org/dpv/owl#ExpectationStatus>
  a owl:Class ;
  dc:contributor _:genid4, _:genid1, _:genid25, _:genid6 ;
  dc:created "2024-05-10"^^xsd:date ;
  ns1:term_status "accepted"@en ;
  skos:definition "Status indicating whether the specified context was intended or unintended"@en ;
  skos:prefLabel "Expectation Status"@en ;
  skos:scopeNote "Expectation is associated with the outcome of a goal or purpose for what is expected to happen i.e. an ex-post indication of what was expected to happen in the specified context. Intention and Expectation are closely related terms. We recommend using Intention when the entity has the ability to control the implementation and Expectation for when the entity does not have control or for what happens after or beyond the exercise of control."@en ;
  owl:sameAs <https://w3id.org/dpv#ExpectationStatus>, <https://w3id.org/dpv/dpv-owl#ExpectationStatus> .

<https://w3id.org/dpv/owl#NegotiateContract>
  a owl:Class ;
  rdfs:subClassOf <https://w3id.org/dpv/owl#ContractControl> ;
  dc:created "2024-08-27"^^xsd:date ;
  ns1:term_status "accepted"@en ;
  skos:definition "Control for negotiating a contract"@en ;
  skos:prefLabel "Negotiate Contract"@en ;
  owl:sameAs <https://w3id.org/dpv#NegotiateContract>, <https://w3id.org/dpv/dpv-owl#NegotiateContract> .

<https://w3id.org/dpv/owl#PersonnelPromotionManagement>
  a owl:Class, owl:NamedIndividual, <https://w3id.org/dpv/owl#Purpose> ;
  rdfs:subClassOf <https://w3id.org/dpv/owl#PersonnelManagement> ;
  dc:created "2024-12-01"^^xsd:date ;
  ns1:term_status "accepted"@en ;
  skos:definition "Purposes associated with determination and management of promotion of personnel"@en ;
  skos:prefLabel "Personnel Promotion Management"@en ;
  owl:sameAs <https://w3id.org/dpv#PersonnelPromotionManagement>, <https://w3id.org/dpv/dpv-owl#PersonnelPromotionManagement> .

<https://w3id.org/dpv/owl#TrustedExecutionEnvironment>
  a owl:Class, owl:NamedIndividual, <https://w3id.org/dpv/owl#TechnicalMeasure> ;
  rdfs:subClassOf <https://w3id.org/dpv/owl#CryptographicMethods> ;
  dc:contributor _:genid1 ;
  dc:created "2022-08-17"^^xsd:date ;
  dc:modified "2024-04-14"^^xsd:date ;
  dc:source [
    a ns0:WebPage ;
    ns0:name "ENISA Data Protection Engineering" ;
    ns0:url "https://www.enisa.europa.eu/publications/data-protection-engineering"
  ] ;
  ns1:term_status "accepted"@en ;
  skos:definition "Use of cryptographic methods to restrict access and execution to trusted parties and code within a dedicated execution environment"@en ;
  skos:prefLabel "Trusted Execution Environment"@en ;
  owl:sameAs <https://w3id.org/dpv#TrustedExecutionEnvironment>, <https://w3id.org/dpv/dpv-owl#TrustedExecutionEnvironment> .

<https://w3id.org/dpv/owl#ConsentRequested>
  a owl:Class, owl:NamedIndividual, <https://w3id.org/dpv/owl#ConsentStatus> ;
  rdfs:subClassOf <https://w3id.org/dpv/owl#ConsentStatusInvalidForProcessing> ;
  dc:contributor _:genid4, _:genid1, _:genid17, _:genid6 ;
  dc:created "2022-06-22"^^xsd:date ;
  dc:source [
    a ns0:WebPage ;
    ns0:name "GConsent" ;
    ns0:url "https://w3id.org/GConsent"
  ] ;
  ns1:term_status "accepted"@en ;
  skos:definition "State where a request for consent has been made and is awaiting a decision"@en ;
  skos:prefLabel "Consent Requested"@en ;
  skos:scopeNote "An example of this state is when a notice has been presented to the individual but they have not made a decision"@en ;
  owl:sameAs <https://w3id.org/dpv#ConsentRequested>, <https://w3id.org/dpv/dpv-owl#ConsentRequested> .

<https://w3id.org/dpv/owl#RightExerciseNotice>
  a owl:Class, owl:NamedIndividual, <https://w3id.org/dpv/owl#OrganisationalMeasure> ;
  rdfs:subClassOf <https://w3id.org/dpv/owl#RightNotice> ;
  dc:contributor _:genid4, _:genid5, _:genid1, _:genid6 ;
  dc:created "2022-10-22"^^xsd:date ;
  ns1:term_status "accepted"@en ;
  skos:definition "Information associated with exercising of an active right such as where and how to exercise the right, information required for it, or updates on an exercised rights request"@en ;
  skos:prefLabel "Right Exercise Notice"@en ;
  skos:scopeNote "This concept is intended for providing information regarding a right exercise. For specific instances of such exercises, see RightExerciseActivity and RightExerciseRecord."@en ;
  owl:sameAs <https://w3id.org/dpv#RightExerciseNotice>, <https://w3id.org/dpv/dpv-owl#RightExerciseNotice> .

<https://w3id.org/dpv/owl#MaintainFraudDatabase>
  a owl:Class, owl:NamedIndividual, <https://w3id.org/dpv/owl#Purpose> ;
  rdfs:subClassOf <https://w3id.org/dpv/owl#FraudPreventionAndDetection> ;
  dc:contributor _:genid4, _:genid1 ;
  dc:created "2022-06-15"^^xsd:date ;
  ns1:term_status "accepted"@en ;
  skos:definition "Purposes associated with maintaining a database related to identifying and identified fraud risks and fraud incidents"@en ;
  skos:prefLabel "Maintain Fraud Database"@en ;
  owl:sameAs <https://w3id.org/dpv#MaintainFraudDatabase>, <https://w3id.org/dpv/dpv-owl#MaintainFraudDatabase> .

<https://w3id.org/dpv/owl#AuditConditionallyApproved>
  a owl:Class, owl:NamedIndividual, <https://w3id.org/dpv/owl#AuditStatus> ;
  rdfs:subClassOf <https://w3id.org/dpv/owl#AuditStatus> ;
  dc:contributor _:genid6 ;
  dc:created "2022-06-29"^^xsd:date ;
  ns1:term_status "accepted"@en ;
  skos:definition "State of being conditionally approved through the audit"@en ;
  skos:prefLabel "Audit Conditionally Approved"@en ;
  skos:scopeNote "A \"conditional approval\" is intended to reflect states where the audit has identified further changes which must be implemented before considering the audit has been 'passed', without requiring another audit to validate them. This is distinct from the case where an audit has state 'rejected', which means changes must be made and submitted for review. The requirements of a 'conditional acceptance' are expected to be minor or not significant enough to warrant another audit to review them."@en ;
  owl:sameAs <https://w3id.org/dpv#AuditConditionallyApproved>, <https://w3id.org/dpv/dpv-owl#AuditConditionallyApproved> .

<https://w3id.org/dpv/owl#DataGovernance>
  a owl:Class, owl:NamedIndividual, <https://w3id.org/dpv/owl#OrganisationalMeasure> ;
  rdfs:subClassOf <https://w3id.org/dpv/owl#OrganisationGovernance> ;
  dc:contributor _:genid1 ;
  dc:created "2024-04-14"^^xsd:date ;
  ns1:term_status "accepted"@en ;
  skos:definition "Measures associated with topics typically considered to be part of 'Data Governance'"@en ;
  skos:prefLabel "Data Governance"@en ;
  owl:sameAs <https://w3id.org/dpv#DataGovernance>, <https://w3id.org/dpv/dpv-owl#DataGovernance> .

<https://w3id.org/dpv/owl#PublicSectorBody>
  a owl:Class ;
  rdfs:subClassOf <https://w3id.org/dpv/owl#LegalEntity> ;
  dc:contributor _:genid4 ;
  dc:created "2024-12-01"^^xsd:date ;
  ns1:term_status "accepted"@en ;
  skos:definition "A government-controlled organisation that provides services or goods to the public"@en ;
  skos:prefLabel "Public Sector Body"@en ;
  owl:sameAs <https://w3id.org/dpv#PublicSectorBody>, <https://w3id.org/dpv/dpv-owl#PublicSectorBody> .

<https://w3id.org/dpv/owl#Unlawful>
  a owl:Class, owl:NamedIndividual, <https://w3id.org/dpv/owl#Lawfulness> ;
  rdfs:subClassOf <https://w3id.org/dpv/owl#Lawfulness> ;
  dc:contributor _:genid1 ;
  dc:created "2022-10-19"^^xsd:date ;
  ns1:term_status "accepted"@en ;
  skos:definition "State of being unlawful or legally non-compliant"@en ;
  skos:prefLabel "Unlawful"@en ;
  owl:sameAs <https://w3id.org/dpv#Unlawful>, <https://w3id.org/dpv/dpv-owl#Unlawful> .

<https://w3id.org/dpv/owl#Visitor>
  a owl:Class, owl:NamedIndividual, <https://w3id.org/dpv/owl#HumanSubject> ;
  rdfs:subClassOf <https://w3id.org/dpv/owl#HumanSubject> ;
  dc:contributor _:genid4, _:genid5, _:genid1, _:genid17, _:genid6 ;
  dc:created "2022-04-06"^^xsd:date ;
  dc:modified "2024-12-17"^^xsd:date ;
  ns1:term_status "modified"@en ;
  skos:definition "Humans that are temporary visitors"@en ;
  skos:prefLabel "Visitor"@en ;
  owl:sameAs <https://w3id.org/dpv#Visitor>, <https://w3id.org/dpv/dpv-owl#Visitor> .

<https://w3id.org/dpv/owl#PublicInterestObjected>
  a owl:Class, owl:NamedIndividual, <https://w3id.org/dpv/owl#PublicInterestStatus> ;
  rdfs:subClassOf <https://w3id.org/dpv/owl#PublicInterestStatus> ;
  dc:created "2024-08-27"^^xsd:date ;
  ns1:term_status "accepted"@en ;
  skos:definition "Status where the public interest activity was objected to by the Data Subject or another relevant entity"@en ;
  skos:prefLabel "Public Interest Objected"@en ;
  owl:sameAs <https://w3id.org/dpv#PublicInterestObjected>, <https://w3id.org/dpv/dpv-owl#PublicInterestObjected> .

<https://w3id.org/dpv/owl#VitalInterest>
  a owl:Class, owl:NamedIndividual, <https://w3id.org/dpv/owl#LegalBasis> ;
  rdfs:subClassOf <https://w3id.org/dpv/owl#LegalBasis> ;
  dc:contributor _:genid1 ;
  dc:created "2021-04-21"^^xsd:date ;
  ns3:example <https://w3id.org/dpv/examples/owl#E0083> ;
  ns1:term_status "accepted"@en ;
  skos:definition "Activities are necessary or required to protect vital interests of a data subject or other natural person"@en ;
  skos:prefLabel "Vital Interest"@en ;
  owl:sameAs <https://w3id.org/dpv#VitalInterest>, <https://w3id.org/dpv/dpv-owl#VitalInterest> .

<https://w3id.org/dpv/owl#ContractNotFulfiled>
  a owl:Class, owl:NamedIndividual, <https://w3id.org/dpv/owl#ContractFulfilmentStatus> ;
  rdfs:subClassOf <https://w3id.org/dpv/owl#ContractFulfilmentStatus> ;
  dc:contributor _:genid4, _:genid1, _:genid17 ;
  dc:created "2025-01-09"^^xsd:date ;
  ns1:term_status "accepted"@en ;
  skos:definition "Status representing contract where none of its terms have been fulfiled in a manner that does not constitutea violation or breach of the contract i.e. there is still time and opportunity to complete the terms"@en ;
  skos:prefLabel "Contract Not Fulfiled"@en ;
  owl:sameAs <https://w3id.org/dpv#ContractNotFulfiled>, <https://w3id.org/dpv/dpv-owl#ContractNotFulfiled> .

odrl:inheritFrom
  a owl:ObjectProperty, owl:NamedIndividual, skos:Concept ;
  rdfs:domain odrl:Policy ;
  rdfs:range odrl:Policy ;
  rdfs:isDefinedBy odrl: ;
  rdfs:label "Inherits From"@en ;
  skos:definition "Relates a (child) policy to another (parent) policy from which terms are inherited."@en ;
  skos:note "The child policy will inherit Rules from the parent policy"@en .

<https://w3id.org/dpv/owl#hasNecessity>
  a owl:ObjectProperty ;
  ns2:rangeIncludes <https://w3id.org/dpv/owl#Necessity> ;
  dc:contributor _:genid1 ;
  dc:created "2024-04-13"^^xsd:date ;
  ns3:example <https://w3id.org/dpv/examples/owl#E0052> ;
  ns1:term_status "accepted"@en ;
  skos:definition "Indicates the necessity for specified context or criteria"@en ;
  skos:prefLabel "has necessity"@en ;
  ns0:rangeIncludes <https://w3id.org/dpv/owl#Necessity> ;
  owl:sameAs <https://w3id.org/dpv#hasNecessity>, <https://w3id.org/dpv/dpv-owl#hasNecessity> .

<https://w3id.org/dpv/owl#ContractViolated>
  a owl:Class, owl:NamedIndividual, <https://w3id.org/dpv/owl#ContractFulfilmentStatus> ;
  rdfs:subClassOf <https://w3id.org/dpv/owl#ContractFulfilmentStatus> ;
  dc:contributor _:genid4, _:genid1, _:genid17 ;
  dc:created "2025-01-09"^^xsd:date ;
  ns1:term_status "accepted"@en ;
  skos:definition "Status representing contract where one or more terms have not been fulfiled or have been fulfiled, where either is considered a violation of the terms"@en ;
  skos:prefLabel "Contract Violated"@en ;
  owl:sameAs <https://w3id.org/dpv#ContractViolated>, <https://w3id.org/dpv/dpv-owl#ContractViolated> .

<https://w3id.org/dpv/owl#isResidualRiskOf>
  a owl:ObjectProperty ;
  ns2:domainIncludes <https://w3id.org/dpv/owl#ResidualRisk> ;
  ns2:rangeIncludes <https://w3id.org/dpv/owl#Risk> ;
  dc:contributor _:genid4, _:genid1, _:genid17, _:genid6 ;
  dc:created "2022-07-20"^^xsd:date ;
  ns1:term_status "accepted"@en ;
  skos:definition "Indicates this risk is the remaining or residual risk from applying mitigation measures or treatments to specified risk"@en ;
  skos:prefLabel "is residual risk of"@en ;
  ns0:domainIncludes <https://w3id.org/dpv/owl#ResidualRisk> ;
  ns0:rangeIncludes <https://w3id.org/dpv/owl#Risk> ;
  owl:sameAs <https://w3id.org/dpv#isResidualRiskOf>, <https://w3id.org/dpv/dpv-owl#isResidualRiskOf> .

<https://w3id.org/dpv/owl#Recipient>
  a owl:Class ;
  rdfs:subClassOf <https://w3id.org/dpv/owl#LegalEntity> ;
  dc:contributor _:genid13, _:genid11 ;
  dc:created "2019-04-05"^^xsd:date ;
  dc:modified "2024-05-21"^^xsd:date ;
  dc:source [
    a ns0:WebPage ;
    ns0:name "GDPR Art.4-9g" ;
    ns0:url "https://eur-lex.europa.eu/eli/reg/2016/679/art_4/par_9/oj"
  ] ;
  ns1:term_status "accepted"@en ;
  skos:definition "Entities that receive data or technologies"@en ;
  skos:prefLabel "Recipient"@en ;
  skos:related <https://specialprivacy.ercim.eu/langs/usage-policy#AnyRecipient> ;
  skos:scopeNote "Recipients that receive personal data can be a Third Party, Data Controller, or Data Processor."@en ;
  owl:sameAs <https://w3id.org/dpv#Recipient>, <https://w3id.org/dpv/dpv-owl#Recipient> .

<https://w3id.org/dpv/owl#DataDeletionPolicy>
  a owl:Class, owl:NamedIndividual, <https://w3id.org/dpv/owl#OrganisationalMeasure> ;
  rdfs:subClassOf <https://w3id.org/dpv/owl#DataProcessingPolicy> ;
  dc:contributor _:genid4, _:genid1 ;
  dc:created "2024-04-14"^^xsd:date ;
  ns1:term_status "accepted"@en ;
  skos:definition "Policy regarding deletion of data"@en ;
  skos:prefLabel "Data Deletion Policy"@en ;
  skos:scopeNote "Deletion and Erasure are distinct activities where deletion refers to logical removal of data with the possibility of retrieval whereas erasure refers to destruction of data such that it cannot be retrieved. See dpv:DataErasurePolicy"@en ;
  owl:sameAs <https://w3id.org/dpv#DataDeletionPolicy>, <https://w3id.org/dpv/dpv-owl#DataDeletionPolicy> .

<https://w3id.org/dpv/owl#SporadicScaleOfDataSubjects>
  a owl:Class, owl:NamedIndividual, <https://w3id.org/dpv/owl#DataSubjectScale> ;
  rdfs:subClassOf <https://w3id.org/dpv/owl#DataSubjectScale> ;
  dc:contributor _:genid1 ;
  dc:created "2022-06-15"^^xsd:date ;
  ns1:term_status "accepted"@en ;
  skos:definition "Scale of data subjects considered sporadic or sparse within the context"@en ;
  skos:prefLabel "Sporadic Scale Of Data Subjects"@en ;
  owl:sameAs <https://w3id.org/dpv#SporadicScaleOfDataSubjects>, <https://w3id.org/dpv/dpv-owl#SporadicScaleOfDataSubjects> .

<https://w3id.org/dpv/owl#FullyRandomisedPseudonymisation>
  a owl:Class, owl:NamedIndividual, <https://w3id.org/dpv/owl#TechnicalMeasure> ;
  rdfs:subClassOf <https://w3id.org/dpv/owl#Pseudonymisation> ;
  dc:contributor _:genid1 ;
  dc:created "2022-08-17"^^xsd:date ;
  dc:source [
    a ns0:WebPage ;
    ns0:name "ENISA Data Pseudonymisation: Advanced Techniques and Use Cases" ;
    ns0:url "https://www.enisa.europa.eu/publications/data-pseudonymisation-advanced-techniques-and-use-cases"
  ] ;
  ns1:term_status "accepted"@en ;
  skos:definition "Use of randomised pseudonymisation where the same elements are assigned different values each time they occur"@en ;
  skos:prefLabel "Fully Randomised Pseudonymisation"@en ;
  owl:sameAs <https://w3id.org/dpv#FullyRandomisedPseudonymisation>, <https://w3id.org/dpv/dpv-owl#FullyRandomisedPseudonymisation> .

<https://w3id.org/dpv/owl#Observe>
  a owl:Class, owl:NamedIndividual, <https://w3id.org/dpv/owl#Processing> ;
  rdfs:subClassOf <https://w3id.org/dpv/owl#Obtain> ;
  dc:contributor _:genid4, _:genid1 ;
  dc:created "2022-06-15"^^xsd:date ;
  ns1:term_status "accepted"@en ;
  skos:definition "to obtain data through observation"@en ;
  skos:prefLabel "Observe Data"@en ;
  owl:sameAs <https://w3id.org/dpv#Observe>, <https://w3id.org/dpv/dpv-owl#Observe> .

<https://w3id.org/dpv/owl#hasRequestStatus>
  a owl:ObjectProperty ;
  ns2:rangeIncludes <https://w3id.org/dpv/owl#RequestStatus> ;
  dc:contributor _:genid1 ;
  dc:created "2024-06-10"^^xsd:date ;
  ns1:term_status "accepted"@en ;
  skos:definition "Indicates the status associated with a request"@en ;
  skos:prefLabel "has request status"@en ;
  ns0:rangeIncludes <https://w3id.org/dpv/owl#RequestStatus> ;
  owl:sameAs <https://w3id.org/dpv#hasRequestStatus>, <https://w3id.org/dpv/dpv-owl#hasRequestStatus> .

<https://w3id.org/dpv/owl#hasObligation>
  a owl:ObjectProperty ;
  rdfs:subPropertyOf <https://w3id.org/dpv/owl#hasRule> ;
  ns2:domainIncludes <https://w3id.org/dpv/owl#Context> ;
  ns2:rangeIncludes <https://w3id.org/dpv/owl#Obligation> ;
  dc:contributor _:genid4, _:genid5, _:genid1, _:genid6 ;
  dc:created "2022-10-19"^^xsd:date ;
  ns1:term_status "accepted"@en ;
  skos:definition "Specifying applicability or inclusion of an obligation rule within specified context"@en ;
  skos:prefLabel "has obligation"@en ;
  ns0:domainIncludes <https://w3id.org/dpv/owl#Context> ;
  ns0:rangeIncludes <https://w3id.org/dpv/owl#Obligation> ;
  owl:sameAs <https://w3id.org/dpv#hasObligation>, <https://w3id.org/dpv/dpv-owl#hasObligation> .

<https://w3id.org/dpv/owl#ConsentNotice>
  a owl:Class, owl:NamedIndividual, <https://w3id.org/dpv/owl#OrganisationalMeasure> ;
  rdfs:subClassOf <https://w3id.org/dpv/owl#PrivacyNotice> ;
  dc:contributor _:genid4, _:genid1, _:genid17, _:genid6 ;
  dc:created "2022-06-21"^^xsd:date ;
  ns3:example <https://w3id.org/dpv/examples/owl#E0072> ;
  ns1:term_status "accepted"@en ;
  skos:definition "A Notice for information provision associated with Consent"@en ;
  skos:prefLabel "Consent Notice"@en ;
  owl:sameAs <https://w3id.org/dpv#ConsentNotice>, <https://w3id.org/dpv/dpv-owl#ConsentNotice> .

<https://w3id.org/dpv/owl#NonCommercialPurpose>
  a owl:Class, owl:NamedIndividual, <https://w3id.org/dpv/owl#Purpose> ;
  rdfs:subClassOf <https://w3id.org/dpv/owl#Purpose> ;
  dc:contributor _:genid5, _:genid1 ;
  dc:created "2024-02-14"^^xsd:date ;
  dc:source "DGA 4.4"@en ;
  ns1:term_status "accepted"@en ;
  skos:definition "Purposes associated with processing activities performed in a non-commercial setting or without intention to commercialise"@en ;
  skos:prefLabel "Non-commercial Purpose"@en ;
  owl:sameAs <https://w3id.org/dpv#NonCommercialPurpose>, <https://w3id.org/dpv/dpv-owl#NonCommercialPurpose> .

odrl:xone
  a owl:ObjectProperty, owl:NamedIndividual, skos:Concept ;
  rdfs:subPropertyOf odrl:operand ;
  rdfs:isDefinedBy odrl: ;
  rdfs:label "Only One"@en ;
  skos:definition "The relation is satisfied when only one, and not more, of the Constaints is satisfied"@en ;
  skos:note "This property MUST only be used for Logical Constraints, and the list of operand values MUST be Constraint instances."@en .

odrl:#ruleConcepts
  a owl:NamedIndividual, skos:Collection ;
  skos:member odrl:Rule, odrl:failure, odrl:function, odrl:relation ;
  skos:prefLabel "Rule"@en ;
  skos:scopeNote "ODRL Core Vocabulary Terms"@en .

<https://w3id.org/dpv/owl#hasApplicableLaw>
  a owl:ObjectProperty, owl:NamedIndividual, odrl:LeftOperand ;
  ns2:rangeIncludes <https://w3id.org/dpv/owl#Law> ;
  dc:contributor _:genid1 ;
  dc:created "2022-01-19"^^xsd:date ;
  ns1:term_status "accepted"@en ;
  skos:definition "Indicates applicability of a Law"@en ;
  skos:prefLabel "has applicable law"@en ;
  ns0:rangeIncludes <https://w3id.org/dpv/owl#Law> ;
  owl:sameAs <https://w3id.org/dpv#hasApplicableLaw>, <https://w3id.org/dpv/dpv-owl#hasApplicableLaw> .

<https://w3id.org/dpv/owl#AnonymisedData>
  a owl:Class ;
  rdfs:subClassOf <https://w3id.org/dpv/owl#NonPersonalData> ;
  dc:contributor _:genid2 ;
  dc:created "2022-01-19"^^xsd:date ;
  ns1:term_status "accepted"@en ;
  skos:definition "Personal Data that has been (fully and completely) anonymised so that it is no longer considered Personal Data"@en ;
  skos:prefLabel "Anonymised Data"@en ;
  skos:scopeNote "It is advised to carefully consider indicating data is fully or completely anonymised by determining whether the data by itself or in combination with other data can identify a person. Failing this condition, the data should be denoted as PseudonymisedData. To indicate data is anonymised only for a specified entity (e.g. within an organisation), the concept ContextuallyAnonymisedData (as subclass of PseudonymisedData) should be used instead of AnonymisedData."@en ;
  owl:sameAs <https://w3id.org/dpv#AnonymisedData>, <https://w3id.org/dpv/dpv-owl#AnonymisedData> .

<https://w3id.org/dpv/owl#SymmetricCryptography>
  a owl:Class, owl:NamedIndividual, <https://w3id.org/dpv/owl#TechnicalMeasure> ;
  rdfs:subClassOf <https://w3id.org/dpv/owl#CryptographicMethods> ;
  dc:contributor _:genid1 ;
  dc:created "2022-08-17"^^xsd:date ;
  dc:source [
    a ns0:WebPage ;
    ns0:name "ENISA Reference Incident Classification Taxonomy 2018" ;
    ns0:url "https://www.enisa.europa.eu/publications/reference-incident-classification-taxonomy/"
  ] ;
  ns1:term_status "accepted"@en ;
  skos:definition "Use of cryptography where the same keys are utilised for encryption and decryption of information"@en ;
  skos:prefLabel "Symmetric Cryptography"@en ;
  owl:sameAs <https://w3id.org/dpv#SymmetricCryptography>, <https://w3id.org/dpv/dpv-owl#SymmetricCryptography> .

<https://w3id.org/dpv/owl#DataProcessingRecord>
  a owl:Class, owl:NamedIndividual, <https://w3id.org/dpv/owl#OrganisationalMeasure> ;
  rdfs:subClassOf <https://w3id.org/dpv/owl#RecordsOfActivities> ;
  dc:contributor _:genid1 ;
  dc:created "2021-09-08"^^xsd:date ;
  ns1:term_status "accepted"@en ;
  skos:definition "Record of data processing, whether ex-ante or ex-post"@en ;
  skos:prefLabel "Data Processing Record"@en ;
  owl:sameAs <https://w3id.org/dpv#DataProcessingRecord>, <https://w3id.org/dpv/dpv-owl#DataProcessingRecord> .

<https://w3id.org/dpv/owl#hasSeverity>
  a owl:ObjectProperty ;
  ns2:rangeIncludes <https://w3id.org/dpv/owl#Severity> ;
  dc:contributor _:genid4, _:genid1, _:genid17, _:genid6 ;
  dc:created "2022-07-20"^^xsd:date ;
  ns3:example <https://w3id.org/dpv/examples/owl#E0068> ;
  ns1:term_status "accepted"@en ;
  skos:definition "Indicates the severity associated with a concept"@en ;
  skos:prefLabel "has severity"@en ;
  ns0:rangeIncludes <https://w3id.org/dpv/owl#Severity> ;
  owl:sameAs <https://w3id.org/dpv#hasSeverity>, <https://w3id.org/dpv/dpv-owl#hasSeverity> .

<https://w3id.org/dpv/owl#hasNotice>
  a owl:ObjectProperty ;
  rdfs:subPropertyOf <https://w3id.org/dpv/owl#hasOrganisationalMeasure> ;
  ns2:rangeIncludes <https://w3id.org/dpv/owl#Notice> ;
  dc:contributor _:genid4, _:genid1, _:genid17, _:genid6 ;
  dc:created "2022-06-22"^^xsd:date ;
  ns1:term_status "accepted"@en ;
  skos:definition "Indicates the use or applicability of a Notice for the specified context"@en ;
  skos:prefLabel "has notice"@en ;
  ns0:rangeIncludes <https://w3id.org/dpv/owl#Notice> ;
  owl:sameAs <https://w3id.org/dpv#hasNotice>, <https://w3id.org/dpv/dpv-owl#hasNotice> .

<https://w3id.org/dpv/owl#VendorRecordsManagement>
  a owl:Class, owl:NamedIndividual, <https://w3id.org/dpv/owl#Purpose> ;
  rdfs:subClassOf <https://w3id.org/dpv/owl#VendorManagement> ;
  dc:contributor _:genid4, _:genid1, _:genid6, _:genid21 ;
  dc:created "2021-09-01"^^xsd:date ;
  dc:source [
    a ns0:WebPage ;
    ns0:name "Belgian DPA ROPA Template" ;
    ns0:url "https://www.privacycommission.be/nl/model-voor-een-register-van-de-verwerkingsactiviteiten"
  ] ;
  ns1:term_status "accepted"@en ;
  skos:definition "Purposes associated with managing records and orders related to vendors"@en ;
  skos:prefLabel "Vendor Records Management"@en ;
  owl:sameAs <https://w3id.org/dpv#VendorRecordsManagement>, <https://w3id.org/dpv/dpv-owl#VendorRecordsManagement> .

<https://w3id.org/dpv/owl#RequestedServiceProvision>
  a owl:Class, owl:NamedIndividual, <https://w3id.org/dpv/owl#Purpose> ;
  rdfs:subClassOf <https://w3id.org/dpv/owl#ServiceProvision> ;
  dc:contributor _:genid4, _:genid5, _:genid1 ;
  dc:created "2021-09-08"^^xsd:date ;
  ns1:term_status "accepted"@en ;
  skos:definition "Purposes associated with delivering services as requested by user or consumer"@en ;
  skos:prefLabel "Requested Service Provision"@en ;
  skos:scopeNote "The use of 'request' here includes where an user explicitly asks for the service and also when an established contract requires the provision of the service"@en ;
  owl:sameAs <https://w3id.org/dpv#RequestedServiceProvision>, <https://w3id.org/dpv/dpv-owl#RequestedServiceProvision> .

odrl:relativeTemporalPosition
  a owl:NamedIndividual, skos:Concept, odrl:LeftOperand ;
  rdfs:isDefinedBy odrl: ;
  rdfs:label "Relative Temporal Asset Position"@en ;
  skos:broaderTransitive odrl:relativePosition ;
  skos:definition "A point in space or time defined with coordinates relative to full measures the positioning of the target Asset."@en ;
  skos:note "See also Absolute Temporal Asset Position. <br />Example: The MP3 music file must be positioned between the positions at 33% and 48% of the temporal length of a stream. "@en ;
  skos:scopeNote "Non-Normative"@en .

<https://w3id.org/dpv/owl#RNGPseudonymisation>
  a owl:Class, owl:NamedIndividual, <https://w3id.org/dpv/owl#TechnicalMeasure> ;
  rdfs:subClassOf <https://w3id.org/dpv/owl#Pseudonymisation> ;
  dc:contributor _:genid1 ;
  dc:created "2022-08-17"^^xsd:date ;
  dc:modified "2022-10-13"^^xsd:date ;
  dc:source [
    a ns0:WebPage ;
    ns0:name "ENISA Data Pseudonymisation: Advanced Techniques and Use Cases" ;
    ns0:url "https://www.enisa.europa.eu/publications/data-pseudonymisation-advanced-techniques-and-use-cases"
  ] ;
  ns1:term_status "accepted"@en ;
  skos:definition "A pseudonymisation method where identifiers are substituted by a number chosen by a Random Number Generator (RNG)"@en ;
  skos:prefLabel "RNG Pseudonymisation"@en ;
  owl:sameAs <https://w3id.org/dpv#RNGPseudonymisation>, <https://w3id.org/dpv/dpv-owl#RNGPseudonymisation> .

<https://w3id.org/dpv/owl#HugeScaleOfDataSubjects>
  a owl:Class, owl:NamedIndividual, <https://w3id.org/dpv/owl#DataSubjectScale> ;
  rdfs:subClassOf <https://w3id.org/dpv/owl#DataSubjectScale> ;
  dc:contributor _:genid1 ;
  dc:created "2022-06-15"^^xsd:date ;
  ns1:term_status "accepted"@en ;
  skos:definition "Scale of data subjects considered huge or more than large within the context"@en ;
  skos:prefLabel "Huge Scale Of Data Subjects"@en ;
  owl:sameAs <https://w3id.org/dpv#HugeScaleOfDataSubjects>, <https://w3id.org/dpv/dpv-owl#HugeScaleOfDataSubjects> .

<https://w3id.org/dpv/owl#JointDataControllersAgreement>
  a owl:Class, owl:NamedIndividual, <https://w3id.org/dpv/owl#LegalBasis>, <https://w3id.org/dpv/owl#LegalMeasure> ;
  rdfs:subClassOf <https://w3id.org/dpv/owl#DataControllerContract> ;
  dc:contributor _:genid4, _:genid5, _:genid1, _:genid17, _:genid6 ;
  dc:created "2022-01-26"^^xsd:date ;
  dc:modified "2024-08-27"^^xsd:date ;
  ns1:term_status "modified"@en ;
  skos:definition "An agreement outlining conditions, criteria, obligations, responsibilities, and specifics for carrying out processing of data between Controllers within a Joint Controllers relationship"@en ;
  skos:prefLabel "Joint Data Controllers Agreement"@en ;
  owl:sameAs <https://w3id.org/dpv#JointDataControllersAgreement>, <https://w3id.org/dpv/dpv-owl#JointDataControllersAgreement> .

<https://w3id.org/dpv/owl#RightExerciseActivity>
  a owl:Class, owl:NamedIndividual, <https://w3id.org/dpv/owl#OrganisationalMeasure> ;
  rdfs:subClassOf <https://w3id.org/dpv/owl#OrganisationalMeasure> ;
  dc:contributor _:genid4, _:genid5, _:genid1, _:genid6 ;
  dc:created "2022-11-02"^^xsd:date ;
  ns3:example <https://w3id.org/dpv/examples/owl#E0059> ;
  ns1:term_status "accepted"@en ;
  skos:definition "An activity representing an exercising of an active right"@en ;
  skos:prefLabel "Right Exercise Activity"@en ;
  skos:scopeNote "There may be multiple activities associated with exercising and fulfilling rights. See the RightExerciseRecord concept for record-keeping of such activities in a cohesive manner."@en ;
  owl:sameAs <https://w3id.org/dpv#RightExerciseActivity>, <https://w3id.org/dpv/dpv-owl#RightExerciseActivity> .

<https://w3id.org/dpv/owl#ConsentGiven>
  a owl:Class, owl:NamedIndividual, <https://w3id.org/dpv/owl#ConsentStatus> ;
  rdfs:subClassOf <https://w3id.org/dpv/owl#ConsentStatusValidForProcessing> ;
  dc:contributor _:genid4, _:genid1, _:genid17, _:genid6 ;
  dc:created "2022-06-22"^^xsd:date ;
  dc:source [
    a ns0:WebPage ;
    ns0:name "GConsent" ;
    ns0:url "https://w3id.org/GConsent"
  ] ;
  ns1:term_status "accepted"@en ;
  skos:definition "The state where consent has been given"@en ;
  skos:prefLabel "Consent Given"@en ;
  skos:scopeNote "An example of this state is when the individual clicks on a button, ticks a checkbox, verbally agrees - or any other form that communicates their decision agreeing to the processing of data"@en ;
  owl:sameAs <https://w3id.org/dpv#ConsentGiven>, <https://w3id.org/dpv/dpv-owl#ConsentGiven> .

<https://w3id.org/dpv/owl#FeeRequirement>
  a owl:Class ;
  rdfs:subClassOf <https://w3id.org/dpv/owl#Context> ;
  dc:created "2024-08-27"^^xsd:date ;
  ns1:term_status "accepted"@en ;
  skos:definition "Concept indicating whether a fee is required"@en ;
  skos:prefLabel "Fee Requirement"@en ;
  owl:sameAs <https://w3id.org/dpv#FeeRequirement>, <https://w3id.org/dpv/dpv-owl#FeeRequirement> .

<https://w3id.org/dpv/owl#PrivateSectorBody>
  a owl:Class ;
  rdfs:subClassOf <https://w3id.org/dpv/owl#LegalEntity> ;
  dc:contributor _:genid4 ;
  dc:created "2024-12-01"^^xsd:date ;
  ns1:term_status "accepted"@en ;
  skos:definition "An organisation owned and operated by private individuals or companies"@en ;
  skos:prefLabel "Private Sector Body"@en ;
  owl:sameAs <https://w3id.org/dpv#PrivateSectorBody>, <https://w3id.org/dpv/dpv-owl#PrivateSectorBody> .

<https://w3id.org/dpv/owl#hasIdentifier>
  a owl:ObjectProperty ;
  dc:contributor _:genid4, _:genid5, _:genid1, _:genid6 ;
  dc:created "2020-11-25"^^xsd:date ;
  ns1:term_status "accepted"@en ;
  skos:definition "Indicates an identifier associated for identification or reference"@en ;
  skos:prefLabel "has identifier"@en ;
  owl:sameAs <https://w3id.org/dpv#hasIdentifier>, <https://w3id.org/dpv/dpv-owl#hasIdentifier> .

<https://w3id.org/dpv/owl#DPIA>
  a owl:Class, owl:NamedIndividual, <https://w3id.org/dpv/owl#OrganisationalMeasure> ;
  rdfs:subClassOf <https://w3id.org/dpv/owl#RightsImpactAssessment> ;
  dc:contributor _:genid4, _:genid1, _:genid6 ;
  dc:created "2020-11-04"^^xsd:date ;
  dc:modified "2024-04-14"^^xsd:date ;
  dc:source "GDPR Art. 35"@en ;
  ns3:example <https://w3id.org/dpv/examples/owl#E0056> ;
  ns1:term_status "accepted"@en ;
  skos:definition "Impact assessment determining the potential and actual impact of processing activities on individuals or groups of individuals and taking into account the impacts of activities on their rights and freedoms"@en ;
  skos:prefLabel "Data Protection Impact Assessment (DPIA)"@en ;
  skos:scopeNote "Specific requirements and procedures for DPIA are defined in GDPR Art.35"@en ;
  owl:sameAs <https://w3id.org/dpv#DPIA>, <https://w3id.org/dpv/dpv-owl#DPIA> .

odrl:#deprecatedTerms
  a owl:NamedIndividual, skos:Collection ;
  skos:member odrl:All, odrl:All2ndConnections, odrl:AllConnections, odrl:AllGroups, odrl:AssetScope, odrl:Group, odrl:Individual, odrl:PartyScope, odrl:UndefinedTerm, odrl:adHocShare, odrl:append, odrl:appendTo, odrl:attachPolicy, odrl:attachSource, odrl:commercialize, odrl:copy, odrl:device, odrl:export, odrl:extractChar, odrl:extractPage, odrl:extractWord, odrl:ignore, odrl:inheritAllowed, odrl:inheritRelation, odrl:lease, odrl:lend, odrl:license, odrl:pay, odrl:payeeParty, odrl:preview, odrl:proximity, odrl:scope, odrl:secondaryUse, odrl:share, odrl:shareAlike, odrl:support, odrl:system, odrl:timedCount, odrl:undefined, odrl:write, odrl:writeTo ;
  skos:prefLabel "Deprecated Terms"@en .

odrl:systemDevice
  a owl:NamedIndividual, skos:Concept, odrl:LeftOperand ;
  rdfs:isDefinedBy odrl: ;
  rdfs:label "System Device"@en ;
  skos:definition "An identified computing system or computing device used for exercising the action of the Rule."@en ;
  skos:exactMatch odrl:device, odrl:system ;
  skos:note "Example: The system device can be identified by a unique code created from the used hardware."@en ;
  skos:scopeNote "Non-Normative"@en .

<https://w3id.org/dpv/owl#hasDataProtectionOfficer>
  a owl:ObjectProperty ;
  rdfs:subPropertyOf <https://w3id.org/dpv/owl#hasRepresentative> ;
  ns2:rangeIncludes <https://w3id.org/dpv/owl#DataProtectionOfficer> ;
  dc:contributor _:genid10, _:genid6 ;
  dc:created "2022-03-02"^^xsd:date ;
  ns1:term_status "accepted"@en ;
  skos:definition "Specifies an associated data protection officer"@en ;
  skos:prefLabel "has data protection officer"@en ;
  ns0:rangeIncludes <https://w3id.org/dpv/owl#DataProtectionOfficer> ;
  owl:sameAs <https://w3id.org/dpv#hasDataProtectionOfficer>, <https://w3id.org/dpv/dpv-owl#hasDataProtectionOfficer> .

<https://w3id.org/dpv/owl#hasJurisdiction>
  a owl:ObjectProperty, owl:NamedIndividual, odrl:LeftOperand ;
  ns2:rangeIncludes <https://w3id.org/dpv/owl#Location> ;
  dc:contributor _:genid1 ;
  dc:created "2022-01-19"^^xsd:date ;
  ns1:term_status "accepted"@en ;
  skos:definition "Indicates applicability of specified jurisdiction"@en ;
  skos:prefLabel "has jurisdiction"@en ;
  ns0:rangeIncludes <https://w3id.org/dpv/owl#Location> ;
  owl:sameAs <https://w3id.org/dpv#hasJurisdiction>, <https://w3id.org/dpv/dpv-owl#hasJurisdiction> .

<https://w3id.org/dpv/owl#SecurityKnowledgeTraining>
  a owl:Class, owl:NamedIndividual, <https://w3id.org/dpv/owl#OrganisationalMeasure> ;
  rdfs:subClassOf <https://w3id.org/dpv/owl#StaffTraining> ;
  dc:contributor _:genid1 ;
  dc:created "2022-08-17"^^xsd:date ;
  dc:source [
    a ns0:WebPage ;
    ns0:name "ENISA 5G Cybersecurity Standards" ;
    ns0:url "https://www.enisa.europa.eu/publications/5g-cybersecurity-standards"
  ] ;
  ns1:term_status "accepted"@en ;
  skos:definition "Training intended to increase knowledge regarding security"@en ;
  skos:prefLabel "Security Knowledge Training"@en ;
  owl:sameAs <https://w3id.org/dpv#SecurityKnowledgeTraining>, <https://w3id.org/dpv/dpv-owl#SecurityKnowledgeTraining> .

dc:hasPart
  a owl:ObjectProperty ;
  ns2:domainIncludes <https://w3id.org/dpv/owl#RightExerciseRecord> ;
  ns2:rangeIncludes <https://w3id.org/dpv/owl#RightExerciseActivity> ;
  skos:prefLabel "dct:hasPart"@en ;
  skos:scopeNote "Also used for specifying a RightExerciseRecord has RightExerciseActivity as part of its records"@en ;
  ns0:domainIncludes <https://w3id.org/dpv/owl#RightExerciseRecord> ;
  ns0:rangeIncludes <https://w3id.org/dpv/owl#RightExerciseActivity> .

<https://w3id.org/dpv/owl#NotificationStatus>
  a owl:Class ;
  rdfs:subClassOf <https://w3id.org/dpv/owl#Status> ;
  dc:contributor _:genid1 ;
  dc:created "2024-05-19"^^xsd:date ;
  ns1:term_status "accepted"@en ;
  skos:definition "Status indicating whether notification(s) are planned, completed, or failed"@en ;
  skos:prefLabel "Notification Status"@en ;
  owl:sameAs <https://w3id.org/dpv#NotificationStatus>, <https://w3id.org/dpv/dpv-owl#NotificationStatus> .

<https://w3id.org/dpv/owl#Access>
  a owl:Class, owl:NamedIndividual, <https://w3id.org/dpv/owl#Processing> ;
  rdfs:subClassOf <https://w3id.org/dpv/owl#Use> ;
  dc:contributor _:genid4, _:genid1 ;
  dc:created "2022-06-15"^^xsd:date ;
  ns1:term_status "accepted"@en ;
  skos:definition "to access data"@en ;
  skos:prefLabel "Access Data"@en ;
  owl:sameAs <https://w3id.org/dpv#Access>, <https://w3id.org/dpv/dpv-owl#Access> .

<https://w3id.org/dpv/owl#GlobalScale>
  a owl:Class, owl:NamedIndividual, <https://w3id.org/dpv/owl#GeographicCoverage> ;
  rdfs:subClassOf <https://w3id.org/dpv/owl#GeographicCoverage> ;
  dc:contributor _:genid1 ;
  dc:created "2022-06-15"^^xsd:date ;
  ns1:term_status "accepted"@en ;
  skos:definition "Geographic coverage spanning the entire globe"@en ;
  skos:prefLabel "Global Scale"@en ;
  owl:sameAs <https://w3id.org/dpv#GlobalScale>, <https://w3id.org/dpv/dpv-owl#GlobalScale> .

<https://w3id.org/dpv/owl#EducationalTraining>
  a owl:Class, owl:NamedIndividual, <https://w3id.org/dpv/owl#OrganisationalMeasure> ;
  rdfs:subClassOf <https://w3id.org/dpv/owl#StaffTraining> ;
  dc:contributor _:genid1 ;
  dc:created "2022-08-17"^^xsd:date ;
  dc:source [
    a ns0:WebPage ;
    ns0:name "ENISA Reference Incident Classification Taxonomy 2018" ;
    ns0:url "https://www.enisa.europa.eu/publications/reference-incident-classification-taxonomy/"
  ] ;
  ns1:term_status "accepted"@en ;
  skos:definition "Training methods that are intended to provide education on topic(s)"@en ;
  skos:prefLabel "Educational Training"@en ;
  owl:sameAs <https://w3id.org/dpv#EducationalTraining>, <https://w3id.org/dpv/dpv-owl#EducationalTraining> .

<https://w3id.org/dpv/owl#HumanInvolvementForIntervention>
  a owl:Class, owl:NamedIndividual, <https://w3id.org/dpv/owl#HumanInvolvement> ;
  rdfs:subClassOf <https://w3id.org/dpv/owl#HumanInvolvement> ;
  dc:created "2022-09-05"^^xsd:date ;
  dc:modified "2023-12-10"^^xsd:date ;
  ns1:term_status "accepted"@en ;
  skos:definition "Human involvement for the purposes of exercising interventions over the specified operations in context"@en ;
  skos:prefLabel "Human Involvement for intervention"@en ;
  skos:scopeNote "Intervention indicates the ability to intervene in operations, which can be at various stages. It maps to Conditional and High automation models."@en ;
  owl:sameAs <https://w3id.org/dpv#HumanInvolvementForIntervention>, <https://w3id.org/dpv/dpv-owl#HumanInvolvementForIntervention> .

<https://w3id.org/dpv/owl#Deidentification>
  a owl:Class, owl:NamedIndividual, <https://w3id.org/dpv/owl#TechnicalMeasure> ;
  rdfs:subClassOf <https://w3id.org/dpv/owl#DataSanitisationTechnique> ;
  dc:contributor _:genid9, _:genid10, _:genid1, _:genid11 ;
  dc:created "2019-04-05"^^xsd:date ;
  dc:modified "2022-11-24"^^xsd:date ;
  dc:source [
    a ns0:WebPage ;
    ns0:name "NISTIR 8053" ;
    ns0:url "https://nvlpubs.nist.gov/nistpubs/ir/2015/NIST.IR.8053.pdf"
  ] ;
  ns1:term_status "accepted"@en ;
  skos:definition "Removal of identity or information to reduce identifiability"@en ;
  skos:prefLabel "De-Identification"@en ;
  owl:sameAs <https://w3id.org/dpv#Deidentification>, <https://w3id.org/dpv/dpv-owl#Deidentification> .

<https://w3id.org/dpv/owl#Immigrant>
  a owl:Class, owl:NamedIndividual, <https://w3id.org/dpv/owl#HumanSubject> ;
  rdfs:subClassOf <https://w3id.org/dpv/owl#HumanSubject> ;
  dc:contributor _:genid4, _:genid5, _:genid1, _:genid17, _:genid6 ;
  dc:created "2022-04-06"^^xsd:date ;
  dc:modified "2024-12-17"^^xsd:date ;
  ns1:term_status "modified"@en ;
  skos:definition "Humans that are immigrants (for a jurisdiction)"@en ;
  skos:prefLabel "Immigrant"@en ;
  owl:sameAs <https://w3id.org/dpv#Immigrant>, <https://w3id.org/dpv/dpv-owl#Immigrant> .

<https://w3id.org/dpv/owl#PersonnelHiring>
  a owl:Class, owl:NamedIndividual, <https://w3id.org/dpv/owl#Purpose> ;
  rdfs:subClassOf <https://w3id.org/dpv/owl#PersonnelManagement> ;
  dc:contributor _:genid1 ;
  dc:created "2022-04-20"^^xsd:date ;
  ns1:term_status "accepted"@en ;
  skos:definition "Purposes associated with management and execution of hiring processes of personnel"@en ;
  skos:prefLabel "Personnel Hiring"@en ;
  owl:sameAs <https://w3id.org/dpv#PersonnelHiring>, <https://w3id.org/dpv/dpv-owl#PersonnelHiring> .

<https://w3id.org/dpv/owl#StorageDeletion>
  a owl:Class ;
  rdfs:subClassOf <https://w3id.org/dpv/owl#StorageCondition> ;
  dc:contributor _:genid9, _:genid10, _:genid1, _:genid11 ;
  dc:created "2019-04-05"^^xsd:date ;
  ns3:example <https://w3id.org/dpv/examples/owl#E0048> ;
  ns1:term_status "accepted"@en ;
  skos:definition "Deletion or Erasure of data including any deletion guarantees"@en ;
  skos:prefLabel "Storage Deletion"@en ;
  owl:sameAs <https://w3id.org/dpv#StorageDeletion>, <https://w3id.org/dpv/dpv-owl#StorageDeletion> .

<https://w3id.org/dpv/owl#ActiveRight>
  a owl:Class, owl:NamedIndividual, <https://w3id.org/dpv/owl#Right> ;
  rdfs:subClassOf <https://w3id.org/dpv/owl#Right> ;
  dc:contributor _:genid4, _:genid5, _:genid1, _:genid6 ;
  dc:created "2022-10-22"^^xsd:date ;
  ns1:term_status "accepted"@en ;
  skos:definition "The right(s) applicable, provided, or expected that need to be (actively) exercised"@en ;
  skos:prefLabel "Active Right"@en ;
  skos:scopeNote "Active rights require the entity to expressly exercise them. For example, a Data Subject exercising their right to withdraw their consent."@en ;
  owl:sameAs <https://w3id.org/dpv#ActiveRight>, <https://w3id.org/dpv/dpv-owl#ActiveRight> .

<https://w3id.org/dpv/owl#SupportContractNegotiation>
  a owl:Class, owl:NamedIndividual, <https://w3id.org/dpv/owl#OrganisationalMeasure> ;
  rdfs:subClassOf <https://w3id.org/dpv/owl#SupportEntityDecisionMaking> ;
  dc:contributor _:genid5, _:genid1 ;
  dc:created "2024-04-14"^^xsd:date ;
  dc:source "DGA 2.15"@en ;
  ns1:term_status "accepted"@en ;
  skos:definition "Supporting entities, including individuals, with negotiating a contract and its terms and conditions"@en ;
  skos:prefLabel "Support Contract Negotiation"@en ;
  owl:sameAs <https://w3id.org/dpv#SupportContractNegotiation>, <https://w3id.org/dpv/dpv-owl#SupportContractNegotiation> .

<https://w3id.org/dpv/owl#PrivacyPreservingProtocol>
  a owl:Class, owl:NamedIndividual, <https://w3id.org/dpv/owl#TechnicalMeasure> ;
  rdfs:subClassOf <https://w3id.org/dpv/owl#CryptographicMethods> ;
  dc:contributor _:genid1 ;
  dc:created "2022-08-17"^^xsd:date ;
  dc:source [
    a ns0:WebPage ;
    ns0:name "ENISA Reference Incident Classification Taxonomy 2018" ;
    ns0:url "https://www.enisa.europa.eu/publications/reference-incident-classification-taxonomy/"
  ] ;
  ns1:term_status "accepted"@en ;
  skos:definition "Use of protocols designed with the intention of provided additional guarantees regarding privacy"@en ;
  skos:prefLabel "Privacy Preserving Protocol"@en ;
  owl:sameAs <https://w3id.org/dpv#PrivacyPreservingProtocol>, <https://w3id.org/dpv/dpv-owl#PrivacyPreservingProtocol> .

<https://w3id.org/dpv/owl#EntityUnintendedInvolvement>
  a owl:Class, owl:NamedIndividual, <https://w3id.org/dpv/owl#EntityInvolvementStatus> ;
  rdfs:subClassOf <https://w3id.org/dpv/owl#EntityInvolvement>, <https://w3id.org/dpv/owl#Unintended> ;
  dc:contributor _:genid25 ;
  dc:created "2024-12-01"^^xsd:date ;
  ns1:term_status "accepted"@en ;
  skos:definition "Status indicating the involvement of the entity is not intended"@en ;
  skos:prefLabel "Entity Unintended Involvement"@en ;
  owl:sameAs <https://w3id.org/dpv#EntityUnintendedInvolvement>, <https://w3id.org/dpv/dpv-owl#EntityUnintendedInvolvement> .

odrl:reviewPolicy
  a owl:NamedIndividual, skos:Concept, odrl:Action ;
  odrl:includedIn odrl:use ;
  rdfs:isDefinedBy odrl: ;
  rdfs:label "Review Policy"@en ;
  skos:definition "To review the Policy applicable to the Asset."@en ;
  skos:note "Used when human intervention is required to review the Policy. May link to an Asset which represents the full Policy information."@en ;
  skos:scopeNote "Non-Normative"@en .

<https://w3id.org/dpv/owl#StorageCondition>
  a owl:Class ;
  rdfs:subClassOf <https://w3id.org/dpv/owl#ProcessingCondition> ;
  dc:contributor _:genid9, _:genid10, _:genid1, _:genid11 ;
  dc:created "2019-04-05"^^xsd:date ;
  ns3:example <https://w3id.org/dpv/examples/owl#E0011>, <https://w3id.org/dpv/examples/owl#E0048> ;
  ns1:term_status "accepted"@en ;
  skos:definition "Conditions required or followed regarding storage of data"@en ;
  skos:prefLabel "Storage Condition"@en ;
  owl:sameAs <https://w3id.org/dpv#StorageCondition>, <https://w3id.org/dpv/dpv-owl#StorageCondition> .

<https://w3id.org/dpv/owl#PrivacyNotice>
  a owl:Class, owl:NamedIndividual, <https://w3id.org/dpv/owl#OrganisationalMeasure> ;
  rdfs:subClassOf <https://w3id.org/dpv/owl#Notice> ;
  dc:contributor _:genid4, _:genid1, _:genid6, _:genid21 ;
  dc:created "2021-09-08"^^xsd:date ;
  ns3:example <https://w3id.org/dpv/examples/owl#E0017>, <https://w3id.org/dpv/examples/owl#E0022> ;
  ns1:term_status "accepted"@en ;
  skos:definition "Represents a notice or document outlining information regarding privacy"@en ;
  skos:prefLabel "Privacy Notice"@en ;
  owl:sameAs <https://w3id.org/dpv#PrivacyNotice>, <https://w3id.org/dpv/dpv-owl#PrivacyNotice> .

odrl:contractingParty
  a owl:ObjectProperty, owl:NamedIndividual, skos:Concept ;
  rdfs:subPropertyOf odrl:function ;
  rdfs:isDefinedBy odrl: ;
  rdfs:label "Contracting Party"@en ;
  skos:definition "The Party who is offering the contract."@en ;
  skos:scopeNote "Non-Normative"@en .

<https://w3id.org/dpv/owl#RecipientUninformed>
  a owl:Class, owl:NamedIndividual, <https://w3id.org/dpv/owl#EntityInformedStatus> ;
  rdfs:subClassOf <https://w3id.org/dpv/owl#EntityUninformed> ;
  dc:contributor _:genid4, _:genid1, _:genid25, _:genid6 ;
  dc:created "2024-05-10"^^xsd:date ;
  ns1:term_status "accepted"@en ;
  skos:definition "Status indicating Recipient is uninformed i.e. has not been informed about the specified context"@en ;
  skos:prefLabel "Recipient Uninformed"@en ;
  owl:sameAs <https://w3id.org/dpv#RecipientUninformed>, <https://w3id.org/dpv/dpv-owl#RecipientUninformed> .

<https://w3id.org/dpv/owl#HashFunctions>
  a owl:Class, owl:NamedIndividual, <https://w3id.org/dpv/owl#TechnicalMeasure> ;
  rdfs:subClassOf <https://w3id.org/dpv/owl#CryptographicMethods> ;
  dc:contributor _:genid1 ;
  dc:created "2022-08-17"^^xsd:date ;
  dc:source [
    a ns0:WebPage ;
    ns0:name "ENISA Reference Incident Classification Taxonomy 2018" ;
    ns0:url "https://www.enisa.europa.eu/publications/reference-incident-classification-taxonomy/"
  ] ;
  ns1:term_status "accepted"@en ;
  skos:definition "Use of hash functions to map information or to retrieve a prior categorisation"@en ;
  skos:prefLabel "Hash Functions"@en ;
  owl:sameAs <https://w3id.org/dpv#HashFunctions>, <https://w3id.org/dpv/dpv-owl#HashFunctions> .

<https://w3id.org/dpv/owl#JITNotice>
  a owl:Class, owl:NamedIndividual, <https://w3id.org/dpv/owl#OrganisationalMeasure> ;
  rdfs:subClassOf <https://w3id.org/dpv/owl#Notice> ;
  dc:created "2024-08-17"^^xsd:date ;
  dc:source [
    a ns0:WebPage ;
    ns0:name "ICO - What methods can we use to provide privacy information?" ;
    ns0:url "https://ico.org.uk/for-organisations/uk-gdpr-guidance-and-resources/individual-rights/the-right-to-be-informed/what-methods-can-we-use-to-provide-privacy-information/"
  ] ;
  ns1:term_status "accepted"@en ;
  skos:definition "A notice that is provided \"just in time\" when collecting information or performing an activity"@en ;
  skos:prefLabel "Just-in-time Notice"@en ;
  owl:sameAs <https://w3id.org/dpv#JITNotice>, <https://w3id.org/dpv/dpv-owl#JITNotice> .

<https://w3id.org/dpv/owl#Align>
  a owl:Class, owl:NamedIndividual, <https://w3id.org/dpv/owl#Processing> ;
  rdfs:subClassOf <https://w3id.org/dpv/owl#Transform> ;
  dc:created "2019-05-07"^^xsd:date ;
  dc:source [
    a ns0:WebPage ;
    ns0:name "GDPR Art.4-2" ;
    ns0:url "https://eur-lex.europa.eu/eli/reg/2016/679/art_4/par_2/oj"
  ] ;
  ns1:term_status "accepted"@en ;
  skos:definition "to adjust the data to be in relation to another data"@en ;
  skos:prefLabel "Align Data"@en ;
  owl:sameAs <https://w3id.org/dpv#Align>, <https://w3id.org/dpv/dpv-owl#Align> .

<https://w3id.org/dpv/owl#ManagementStandard>
  a owl:Class, owl:NamedIndividual, <https://w3id.org/dpv/owl#OrganisationalMeasure> ;
  rdfs:subClassOf <https://w3id.org/dpv/owl#Standard> ;
  dc:contributor _:genid1 ;
  dc:created "2024-12-01"^^xsd:date ;
  ns1:term_status "accepted"@en ;
  skos:definition "A management standard is a standard that establishes norms or requirements regarding the management operations and processes e.g. in an organisation"@en ;
  skos:prefLabel "Management Standard"@en ;
  owl:sameAs <https://w3id.org/dpv#ManagementStandard>, <https://w3id.org/dpv/dpv-owl#ManagementStandard> .

<https://w3id.org/dpv/owl#Transform>
  a owl:Class, owl:NamedIndividual, <https://w3id.org/dpv/owl#Processing> ;
  rdfs:subClassOf <https://w3id.org/dpv/owl#Processing> ;
  dc:created "2019-05-07"^^xsd:date ;
  dc:source [
    a ns0:WebPage ;
    ns0:name "GDPR Art.4-2" ;
    ns0:url "https://eur-lex.europa.eu/eli/reg/2016/679/art_4/par_2/oj"
  ] ;
  ns1:term_status "accepted"@en ;
  skos:definition "to change the form or nature of data"@en ;
  skos:prefLabel "Transform Data"@en ;
  owl:sameAs <https://w3id.org/dpv#Transform>, <https://w3id.org/dpv/dpv-owl#Transform> .

<https://w3id.org/dpv/owl#RuleFulfilled>
  a owl:Class, owl:NamedIndividual, <https://w3id.org/dpv/owl#RuleFulfilmentStatus> ;
  rdfs:subClassOf <https://w3id.org/dpv/owl#RuleFulfilmentStatus> ;
  dc:contributor _:genid1 ;
  dc:created "2024-09-10"^^xsd:date ;
  ns1:term_status "accepted"@en ;
  skos:definition "Status indicating a rule has been fulfilled, completed, or satisfied"@en ;
  skos:prefLabel "Rule Fulfilled"@en ;
  owl:sameAs <https://w3id.org/dpv#RuleFulfilled>, <https://w3id.org/dpv/dpv-owl#RuleFulfilled> .

<https://w3id.org/dpv/owl#PhysicalNetworkSecurity>
  a owl:Class, owl:NamedIndividual, <https://w3id.org/dpv/owl#PhysicalMeasure> ;
  rdfs:subClassOf <https://w3id.org/dpv/owl#PhysicalMeasure> ;
  dc:contributor _:genid1 ;
  dc:created "2024-04-14"^^xsd:date ;
  dc:source "NIST SP 800-17"@en ;
  ns1:term_status "accepted"@en ;
  skos:definition "Physical protection for networks and networking related infrastructure e.g. by isolating networking equipments"@en ;
  skos:prefLabel "Physical Network Security"@en ;
  owl:sameAs <https://w3id.org/dpv#PhysicalNetworkSecurity>, <https://w3id.org/dpv/dpv-owl#PhysicalNetworkSecurity> .

<https://w3id.org/dpv/owl#isImplementedUsingTechnology>
  a owl:ObjectProperty ;
  ns2:rangeIncludes <https://w3id.org/dpv/owl#Technology> ;
  dc:contributor _:genid5, _:genid1, _:genid17, _:genid6 ;
  dc:created "2022-01-26"^^xsd:date ;
  dc:modified "2022-06-15"^^xsd:date ;
  ns3:example <https://w3id.org/dpv/examples/owl#E0064>, <https://w3id.org/dpv/examples/owl#E0085> ;
  ns1:term_status "accepted"@en ;
  skos:definition "Indicates implementation details such as technologies or processes"@en ;
  skos:prefLabel "is implemented using technology"@en ;
  skos:scopeNote "The term 'technology' is inclusive of technologies, processes, and methods."@en ;
  ns0:rangeIncludes <https://w3id.org/dpv/owl#Technology> ;
  owl:sameAs <https://w3id.org/dpv#isImplementedUsingTechnology>, <https://w3id.org/dpv/dpv-owl#isImplementedUsingTechnology> .

<https://w3id.org/dpv/owl#DataImporter>
  a owl:Class ;
  rdfs:subClassOf <https://w3id.org/dpv/owl#Recipient> ;
  dc:contributor _:genid4, _:genid1, _:genid6, _:genid21 ;
  dc:created "2021-09-08"^^xsd:date ;
  dc:source [
    a ns0:WebPage ;
    ns0:name "EDPB Recommendations 01/2020 on Data Transfers" ;
    ns0:url "https://edpb.europa.eu/our-work-tools/our-documents/recommendations/recommendations-012020-measures-supplement-transfer_en"
  ] ;
  ns3:example <https://w3id.org/dpv/examples/owl#E0035> ;
  ns1:term_status "accepted"@en ;
  skos:definition "An entity that 'imports' data where importing is considered a form of data transfer"@en ;
  skos:prefLabel "Data Importer"@en ;
  skos:scopeNote "The term 'Data Importer' is used by the EU-EDPB as the entity that receives transferred data across borders. While the EDPB refers to the jurisdictional border of EU, the term within DPV can be used to denote any 'import' or reception of transfer or transmission of data and is thus a broader concept than the EDPB's definition."@en ;
  owl:sameAs <https://w3id.org/dpv#DataImporter>, <https://w3id.org/dpv/dpv-owl#DataImporter> .

<https://w3id.org/dpv/owl#Personalisation>
  a owl:Class, owl:NamedIndividual, <https://w3id.org/dpv/owl#Purpose> ;
  rdfs:subClassOf <https://w3id.org/dpv/owl#Purpose> ;
  dc:contributor _:genid1 ;
  dc:created "2021-09-01"^^xsd:date ;
  ns1:term_status "accepted"@en ;
  skos:definition "Purposes associated with creating and providing customisation based on attributes and/or needs of person(s) or context(s)."@en ;
  skos:prefLabel "Personalisation"@en ;
  skos:scopeNote "This term is a blanket purpose category for indicating personalisation of some other purpose, e.g. by creating a subclass of the other concept and Personalisation"@en ;
  owl:sameAs <https://w3id.org/dpv#Personalisation>, <https://w3id.org/dpv/dpv-owl#Personalisation> .

<https://w3id.org/dpv/owl#Infer>
  a owl:Class, owl:NamedIndividual, <https://w3id.org/dpv/owl#Processing> ;
  rdfs:subClassOf <https://w3id.org/dpv/owl#Derive> ;
  dc:contributor _:genid1 ;
  dc:created "2022-04-20"^^xsd:date ;
  dc:modified "2022-10-14"^^xsd:date ;
  ns3:example <https://w3id.org/dpv/examples/owl#E0009> ;
  ns1:term_status "accepted"@en ;
  skos:definition "to infer data from existing data"@en ;
  skos:prefLabel "Infer Data"@en ;
  skos:scopeNote "Infer indicates data that is derived without it being present or obtainable from existing data. For data that is presented, and is 'extracted' or 'obtained' from existing data, see Derive."@en ;
  owl:sameAs <https://w3id.org/dpv#Infer>, <https://w3id.org/dpv/dpv-owl#Infer> .

odrl:function
  a owl:ObjectProperty, owl:NamedIndividual, skos:Concept ;
  rdfs:domain [
    a owl:Class ;
    owl:unionOf (
     odrl:Policy
     odrl:Rule
   )
  ] ;
  rdfs:range odrl:Party ;
  rdfs:isDefinedBy odrl: ;
  rdfs:label "Function"@en ;
  skos:definition "Function is an abstract property whose sub-properties define the functional roles which may be fulfilled by a party in relation to a Rule."@en .

odrl:language
  a owl:NamedIndividual, skos:Concept, odrl:LeftOperand ;
  rdfs:isDefinedBy odrl: ;
  rdfs:label "Language"@en ;
  skos:definition "A natural language used by the target Asset."@en ;
  skos:note "Example: the asset can only be translated into Greek. Must use [[bcp47]] codes for language values."@en ;
  skos:scopeNote "Non-Normative"@en .

<https://w3id.org/dpv/owl#PublicPolicyMaking>
  a owl:Class, owl:NamedIndividual, <https://w3id.org/dpv/owl#Purpose> ;
  rdfs:subClassOf <https://w3id.org/dpv/owl#PublicBenefit> ;
  dc:contributor _:genid5, _:genid1 ;
  dc:created "2024-02-14"^^xsd:date ;
  dc:source "DGA 2.16"@en ;
  ns1:term_status "accepted"@en ;
  skos:definition "Purposes associated with public policy making, such as the development of new laws"@en ;
  skos:prefLabel "Public Policy Making"@en ;
  owl:sameAs <https://w3id.org/dpv#PublicPolicyMaking>, <https://w3id.org/dpv/dpv-owl#PublicPolicyMaking> .

<https://w3id.org/dpv/owl#HighAutomation>
  a owl:Class, owl:NamedIndividual, <https://w3id.org/dpv/owl#AutomationLevel> ;
  rdfs:subClassOf <https://w3id.org/dpv/owl#AutomationLevel> ;
  dc:contributor _:genid1, _:genid25 ;
  dc:created "2023-12-10"^^xsd:date ;
  dc:modified "2024-04-20"^^xsd:date ;
  dc:source [
    a ns0:WebPage ;
    ns0:name "ISO/IEC 22989:2022 Artificial intelligence concepts and terminology" ;
    ns0:url "https://www.iso.org/standard/74296.html"
  ] ;
  ns1:term_status "accepted"@en ;
  skos:definition "Level of automation corresponding to Level 4 in ISO/IEC 22989:2022 where the automation in system is capable of performing all its tasks within specific controlled conditions without human involvement"@en ;
  skos:prefLabel "High Automation"@en ;
  skos:scopeNote "Human Involvement is implied here, e.g. for intervention, input, decisions"@en ;
  owl:sameAs <https://w3id.org/dpv#HighAutomation>, <https://w3id.org/dpv/dpv-owl#HighAutomation> .

<https://w3id.org/dpv/owl#hasNonInvolvedEntity>
  a owl:ObjectProperty ;
  rdfs:subPropertyOf <https://w3id.org/dpv/owl#hasEntity> ;
  ns2:rangeIncludes <https://w3id.org/dpv/owl#Entity> ;
  dc:created "2024-05-11"^^xsd:date ;
  ns1:term_status "accepted"@en ;
  skos:definition "indicates the entity is not involved in specified context"@en ;
  skos:prefLabel "has non-involved entity"@en ;
  ns0:rangeIncludes <https://w3id.org/dpv/owl#Entity> ;
  owl:sameAs <https://w3id.org/dpv#hasNonInvolvedEntity>, <https://w3id.org/dpv/dpv-owl#hasNonInvolvedEntity> .

<https://w3id.org/dpv/owl#DataTransferRecord>
  a owl:Class, owl:NamedIndividual, <https://w3id.org/dpv/owl#OrganisationalMeasure> ;
  rdfs:subClassOf <https://w3id.org/dpv/owl#DataProcessingRecord> ;
  dc:contributor _:genid1 ;
  dc:created "2024-04-14"^^xsd:date ;
  ns1:term_status "accepted"@en ;
  skos:definition "Record of data transfer activities"@en ;
  skos:prefLabel "Data Transfer Record"@en ;
  owl:sameAs <https://w3id.org/dpv#DataTransferRecord>, <https://w3id.org/dpv/dpv-owl#DataTransferRecord> .

skos:Concept a owl:Class .
<https://w3id.org/dpv/owl#RequestFulfilled>
  a owl:Class, owl:NamedIndividual, <https://w3id.org/dpv/owl#RequestStatus> ;
  rdfs:subClassOf <https://w3id.org/dpv/owl#RequestStatus> ;
  dc:contributor _:genid1 ;
  dc:created "2022-11-30"^^xsd:date ;
  ns1:term_status "accepted"@en ;
  skos:definition "State of a request being fulfilled"@en ;
  skos:prefLabel "Request Fulfilled"@en ;
  owl:sameAs <https://w3id.org/dpv#RequestFulfilled>, <https://w3id.org/dpv/dpv-owl#RequestFulfilled> .

<https://w3id.org/dpv/owl#OfficialAuthorityExerciseStatus>
  a owl:Class ;
  rdfs:subClassOf <https://w3id.org/dpv/owl#Status> ;
  dc:created "2024-08-27"^^xsd:date ;
  ns3:example <https://w3id.org/dpv/examples/owl#E0081> ;
  ns1:term_status "accepted"@en ;
  skos:definition "Status associated with use of Official Authority as a legal basis"@en ;
  skos:prefLabel "Official Authority Exercise Status"@en ;
  owl:sameAs <https://w3id.org/dpv#OfficialAuthorityExerciseStatus>, <https://w3id.org/dpv/dpv-owl#OfficialAuthorityExerciseStatus> .

<https://w3id.org/dpv/owl#hasThirdCountry>
  a owl:ObjectProperty ;
  rdfs:subPropertyOf <https://w3id.org/dpv/owl#hasCountry> ;
  ns2:rangeIncludes <https://w3id.org/dpv/owl#ThirdCountry> ;
  dc:contributor _:genid4, _:genid1 ;
  dc:created "2022-02-09"^^xsd:date ;
  ns1:term_status "accepted"@en ;
  skos:definition "Indicates applicability or relevance of a 'third country'"@en ;
  skos:prefLabel "has third country"@en ;
  ns0:rangeIncludes <https://w3id.org/dpv/owl#ThirdCountry> ;
  owl:sameAs <https://w3id.org/dpv#hasThirdCountry>, <https://w3id.org/dpv/dpv-owl#hasThirdCountry> .

<https://w3id.org/dpv/owl#TerminateContract>
  a owl:Class ;
  rdfs:subClassOf <https://w3id.org/dpv/owl#ContractControl> ;
  dc:created "2024-08-27"^^xsd:date ;
  ns1:term_status "accepted"@en ;
  skos:definition "Control for terminating a contract"@en ;
  skos:prefLabel "Terminate Contract"@en ;
  owl:sameAs <https://w3id.org/dpv#TerminateContract>, <https://w3id.org/dpv/dpv-owl#TerminateContract> .

<https://w3id.org/dpv/owl#InformationAudit>
  a owl:Class, owl:NamedIndividual, <https://w3id.org/dpv/owl#OrganisationalMeasure> ;
  rdfs:subClassOf <https://w3id.org/dpv/owl#Audit> ;
  dc:contributor _:genid1, _:genid6 ;
  dc:created "2024-12-17"^^xsd:date ;
  ns1:term_status "accepted"@en ;
  skos:definition "An audit that systematically examines the existence and use of information along with its associated resources (e.g. where it is stored) and flows (e.g. where it originates and with whom it is being shared)"@en ;
  skos:prefLabel "Information Audit"@en ;
  owl:sameAs <https://w3id.org/dpv#InformationAudit>, <https://w3id.org/dpv/dpv-owl#InformationAudit> .

<https://w3id.org/dpv/owl#LegitimateInterest>
  a owl:Class, owl:NamedIndividual, <https://w3id.org/dpv/owl#LegalBasis> ;
  rdfs:subClassOf <https://w3id.org/dpv/owl#LegalBasis> ;
  dc:contributor _:genid1 ;
  dc:created "2021-05-19"^^xsd:date ;
  ns3:example <https://w3id.org/dpv/examples/owl#E0065>, <https://w3id.org/dpv/examples/owl#E0080> ;
  ns1:term_status "accepted"@en ;
  skos:definition "Legitimate Interests of a Party as justification for specified activities"@en ;
  skos:prefLabel "Legitimate Interest"@en ;
  owl:sameAs <https://w3id.org/dpv#LegitimateInterest>, <https://w3id.org/dpv/dpv-owl#LegitimateInterest> .

<https://w3id.org/dpv/owl#EducationalOrganisation>
  a owl:Class ;
  rdfs:subClassOf <https://w3id.org/dpv/owl#Organisation> ;
  dc:contributor _:genid25 ;
  dc:created "2024-12-01"^^xsd:date ;
  ns1:term_status "accepted"@en ;
  skos:definition "An organisation focused on delivering formal or informal education, training, or research"@en ;
  skos:prefLabel "Educational Organisation"@en ;
  owl:sameAs <https://w3id.org/dpv#EducationalOrganisation>, <https://w3id.org/dpv/dpv-owl#EducationalOrganisation> .

<https://w3id.org/dpv/owl#hasDataExporter>
  a owl:ObjectProperty ;
  rdfs:subPropertyOf <https://w3id.org/dpv/owl#hasEntity> ;
  ns2:rangeIncludes <https://w3id.org/dpv/owl#DataExporter> ;
  dc:contributor _:genid4, _:genid1, _:genid6 ;
  dc:created "2022-02-09"^^xsd:date ;
  ns1:term_status "accepted"@en ;
  skos:definition "Indicates inclusion or applicability of a LegalEntity in the role of Data Exporter"@en ;
  skos:prefLabel "has data exporter"@en ;
  ns0:rangeIncludes <https://w3id.org/dpv/owl#DataExporter> ;
  owl:sameAs <https://w3id.org/dpv#hasDataExporter>, <https://w3id.org/dpv/dpv-owl#hasDataExporter> .

<https://w3id.org/dpv/primer>
  a owl:NamedIndividual, ns4:ResourceDescriptor ;
  dc:format <https://www.iana.org/assignments/media-types/text/html> ;
  dc:conformsTo <https://www.w3.org/TR/html/> ;
  dc:title "Primer for Data Privacy Vocabulary" ;
  ns4:hasArtifact <https://w3id.org/dpv/primer> ;
  ns4:hasRole <http://www.w3.org/ns/dx/prof/role/guidance> .

<https://w3id.org/dpv/owl#SubProcessorAgreement>
  a owl:Class, owl:NamedIndividual, <https://w3id.org/dpv/owl#LegalBasis>, <https://w3id.org/dpv/owl#LegalMeasure> ;
  rdfs:subClassOf <https://w3id.org/dpv/owl#DataProcessingAgreement> ;
  dc:contributor _:genid4, _:genid5, _:genid1, _:genid17, _:genid6 ;
  dc:created "2022-01-26"^^xsd:date ;
  dc:modified "2024-08-27"^^xsd:date ;
  ns1:term_status "modified"@en ;
  skos:definition "An agreement outlining conditions, criteria, obligations, responsibilities, and specifics for carrying out processing of data between a Data Processor and a Data (Sub-)Processor"@en ;
  skos:prefLabel "Sub-Processor Agreement"@en ;
  owl:sameAs <https://w3id.org/dpv#SubProcessorAgreement>, <https://w3id.org/dpv/dpv-owl#SubProcessorAgreement> .

<https://w3id.org/dpv/owl#SupraNationalUnion>
  a owl:Class ;
  rdfs:subClassOf <https://w3id.org/dpv/owl#Location> ;
  dc:contributor _:genid1 ;
  dc:created "2022-01-19"^^xsd:date ;
  ns1:term_status "accepted"@en ;
  skos:definition "A political union of two or more countries with an establishment of common authority"@en ;
  skos:prefLabel "Supranational Union"@en ;
  owl:sameAs <https://w3id.org/dpv#SupraNationalUnion>, <https://w3id.org/dpv/dpv-owl#SupraNationalUnion> .

odrl:relation
  a owl:ObjectProperty, owl:NamedIndividual, skos:Concept ;
  rdfs:domain [
    a owl:Class ;
    owl:unionOf (
     odrl:Policy
     odrl:Rule
   )
  ] ;
  rdfs:range odrl:Asset ;
  rdfs:isDefinedBy odrl: ;
  rdfs:label "Relation"@en ;
  skos:definition "Relation is an abstract property which creates an explicit link between an Action and an Asset."@en ;
  skos:note "Sub-properties of relation are used to define the nature of that link."@en .

<https://w3id.org/dpv/owl#OptimisationForConsumer>
  a owl:Class, owl:NamedIndividual, <https://w3id.org/dpv/owl#Purpose> ;
  rdfs:subClassOf <https://w3id.org/dpv/owl#ServiceOptimisation> ;
  dc:contributor _:genid13, _:genid14, _:genid1, _:genid15, _:genid16, _:genid11 ;
  dc:created "2019-04-05"^^xsd:date ;
  ns1:term_status "accepted"@en ;
  skos:definition "Purposes associated with optimisation of activities and services for consumer or user"@en ;
  skos:prefLabel "Optimisation for Consumer"@en ;
  skos:related <https://specialprivacy.ercim.eu/vocabs/purposes#Custom> ;
  skos:scopeNote "The term optimisation here refers to the efficiency of the service in terms of technical provision (or similar means) with benefits for everybody. Personalisation implies making changes that benefit the current user or persona."@en ;
  owl:sameAs <https://w3id.org/dpv#OptimisationForConsumer>, <https://w3id.org/dpv/dpv-owl#OptimisationForConsumer> .

<https://w3id.org/dpv/owl#SellDataToThirdParties>
  a owl:Class, owl:NamedIndividual, <https://w3id.org/dpv/owl#Purpose> ;
  rdfs:subClassOf <https://w3id.org/dpv/owl#SellProducts> ;
  dc:contributor _:genid13, _:genid14, _:genid1, _:genid15, _:genid16, _:genid11 ;
  dc:created "2019-04-05"^^xsd:date ;
  ns1:term_status "accepted"@en ;
  skos:definition "Purposes associated with selling or sharing data or information to third parties"@en ;
  skos:prefLabel "Sell Data to Third Parties"@en ;
  skos:scopeNote "Sell here means exchange, submit, or provide in return for direct or indirect compensation. Was subclass of commercial interest, changed to reflect selling something"@en ;
  owl:sameAs <https://w3id.org/dpv#SellDataToThirdParties>, <https://w3id.org/dpv/dpv-owl#SellDataToThirdParties> .

<https://w3id.org/dpv/owl#LawfulnessUnkown>
  a owl:Class, owl:NamedIndividual, <https://w3id.org/dpv/owl#Lawfulness> ;
  rdfs:subClassOf <https://w3id.org/dpv/owl#Lawfulness> ;
  dc:contributor _:genid1 ;
  dc:created "2022-10-19"^^xsd:date ;
  ns1:term_status "accepted"@en ;
  skos:definition "State of the lawfulness not being known"@en ;
  skos:prefLabel "Lawfulness Unknown"@en ;
  owl:sameAs <https://w3id.org/dpv#LawfulnessUnkown>, <https://w3id.org/dpv/dpv-owl#LawfulnessUnkown> .

<https://w3id.org/dpv/owl#NotificationCompleted>
  a owl:Class, owl:NamedIndividual, <https://w3id.org/dpv/owl#NotificationStatus> ;
  rdfs:subClassOf <https://w3id.org/dpv/owl#NotificationStatus> ;
  dc:contributor _:genid1 ;
  dc:created "2024-05-19"^^xsd:date ;
  ns1:term_status "accepted"@en ;
  skos:definition "Status indicating notification(s) are completed"@en ;
  skos:prefLabel "Notification Completed"@en ;
  owl:sameAs <https://w3id.org/dpv#NotificationCompleted>, <https://w3id.org/dpv/dpv-owl#NotificationCompleted> .

odrl:neq
  a owl:NamedIndividual, skos:Concept, odrl:Operator ;
  rdfs:isDefinedBy odrl: ;
  rdfs:label "Not equal to"@en ;
  skos:definition "Indicating that a given value is not equal to the right operand of the Constraint."@en .

<https://w3id.org/dpv/owl#hasLegalBasis>
  a owl:ObjectProperty, owl:NamedIndividual, odrl:LeftOperand ;
  ns2:rangeIncludes <https://w3id.org/dpv/owl#LegalBasis> ;
  dc:contributor _:genid13, _:genid11 ;
  dc:created "2019-04-04"^^xsd:date ;
  dc:modified "2020-11-04"^^xsd:date ;
  ns1:term_status "accepted"@en ;
  skos:definition "Indicates use or applicability of a Legal Basis"@en ;
  skos:prefLabel "has legal basis"@en ;
  ns0:rangeIncludes <https://w3id.org/dpv/owl#LegalBasis> ;
  owl:sameAs <https://w3id.org/dpv#hasLegalBasis>, <https://w3id.org/dpv/dpv-owl#hasLegalBasis> .

<https://w3id.org/dpv/owl#PublicInterestStatus>
  a owl:Class ;
  rdfs:subClassOf <https://w3id.org/dpv/owl#Status> ;
  dc:created "2024-08-27"^^xsd:date ;
  ns3:example <https://w3id.org/dpv/examples/owl#E0082> ;
  ns1:term_status "accepted"@en ;
  skos:definition "Status associated with use of Public Interest as a legal basis"@en ;
  skos:prefLabel "Public Interest Status"@en ;
  owl:sameAs <https://w3id.org/dpv#PublicInterestStatus>, <https://w3id.org/dpv/dpv-owl#PublicInterestStatus> .

<https://w3id.org/dpv/owl#PassiveRight>
  a owl:Class, owl:NamedIndividual, <https://w3id.org/dpv/owl#Right> ;
  rdfs:subClassOf <https://w3id.org/dpv/owl#Right> ;
  dc:contributor _:genid4, _:genid5, _:genid1, _:genid6 ;
  dc:created "2022-10-22"^^xsd:date ;
  ns1:term_status "accepted"@en ;
  skos:definition "The right(s) applicable, provided, or expected that are always (passively) applicable"@en ;
  skos:prefLabel "Passive Right"@en ;
  skos:scopeNote "Passive rights do not require the entity to request or exercise them. They are considered to be always applicable. For example, the Right to Privacy (in EU) does not require an exercise for it to be fulfilled."@en ;
  owl:sameAs <https://w3id.org/dpv#PassiveRight>, <https://w3id.org/dpv/dpv-owl#PassiveRight> .

<https://w3id.org/dpv/owl#SecurityAssessment>
  a owl:Class, owl:NamedIndividual, <https://w3id.org/dpv/owl#OrganisationalMeasure> ;
  rdfs:subClassOf <https://w3id.org/dpv/owl#RiskAssessment> ;
  dc:contributor _:genid1 ;
  dc:created "2022-08-17"^^xsd:date ;
  dc:source [
    a ns0:WebPage ;
    ns0:name "ENISA 5G Cybersecurity Standards" ;
    ns0:url "https://www.enisa.europa.eu/publications/5g-cybersecurity-standards"
  ] ;
  ns1:term_status "accepted"@en ;
  skos:definition "Assessment of security intended to identity gaps, vulnerabilities, risks, and effectiveness of controls"@en ;
  skos:prefLabel "Security Assessment"@en ;
  owl:sameAs <https://w3id.org/dpv#SecurityAssessment>, <https://w3id.org/dpv/dpv-owl#SecurityAssessment> .

<https://w3id.org/dpv/owl#FeeNotRequired>
  a owl:Class, owl:NamedIndividual, <https://w3id.org/dpv/owl#FeeRequirement> ;
  rdfs:subClassOf <https://w3id.org/dpv/owl#FeeRequirement> ;
  dc:created "2024-08-27"^^xsd:date ;
  ns1:term_status "accepted"@en ;
  skos:definition "Concept indicating a fee is not required. This is distinct from a Fee of zero as it indicates a fee is not applicable in the context"@en ;
  skos:prefLabel "Fee Not Required"@en ;
  owl:sameAs <https://w3id.org/dpv#FeeNotRequired>, <https://w3id.org/dpv/dpv-owl#FeeNotRequired> .

<https://w3id.org/dpv/owl#InnovativeUseOfNewTechnologies>
  a owl:Class, owl:NamedIndividual, <https://w3id.org/dpv/owl#InnovativeUseOfTechnology> ;
  rdfs:subClassOf <https://w3id.org/dpv/owl#InnovativeUseOfTechnology> ;
  dc:contributor _:genid1, _:genid2 ;
  dc:created "2020-11-04"^^xsd:date ;
  dc:modified "2023-12-10"^^xsd:date ;
  dc:source [
    a ns0:WebPage ;
    ns0:name "GDPR Art.4-2" ;
    ns0:url "https://eur-lex.europa.eu/eli/reg/2016/679/art_4/par_2/oj"
  ] ;
  ns1:term_status "accepted"@en ;
  skos:definition "Involvement of a new (innovative) technologies"@en ;
  skos:prefLabel "Innovative Use of New Technologies"@en ;
  skos:scopeNote "New technologies are by definition considered innovative"@en ;
  owl:sameAs <https://w3id.org/dpv#InnovativeUseOfNewTechnologies>, <https://w3id.org/dpv/dpv-owl#InnovativeUseOfNewTechnologies> .

<https://w3id.org/dpv/owl#Alter>
  a owl:Class, owl:NamedIndividual, <https://w3id.org/dpv/owl#Processing> ;
  rdfs:subClassOf <https://w3id.org/dpv/owl#Transform> ;
  dc:created "2019-05-07"^^xsd:date ;
  dc:source [
    a ns0:WebPage ;
    ns0:name "GDPR Art.4-2" ;
    ns0:url "https://eur-lex.europa.eu/eli/reg/2016/679/art_4/par_2/oj"
  ] ;
  ns1:term_status "accepted"@en ;
  skos:definition "to change the data without changing it into something else"@en ;
  skos:prefLabel "Alter Data"@en ;
  owl:sameAs <https://w3id.org/dpv#Alter>, <https://w3id.org/dpv/dpv-owl#Alter> .

<https://w3id.org/dpv/owl#hasRecordOfActivity>
  a owl:ObjectProperty ;
  rdfs:subPropertyOf <https://w3id.org/dpv/owl#hasOrganisationalMeasure> ;
  ns2:rangeIncludes <https://w3id.org/dpv/owl#RecordsOfActivities> ;
  dc:contributor _:genid1 ;
  dc:created "2024-05-05"^^xsd:date ;
  ns1:term_status "accepted"@en ;
  skos:definition "Indicates a relevant record of activity"@en ;
  skos:prefLabel "has record of activity"@en ;
  ns0:rangeIncludes <https://w3id.org/dpv/owl#RecordsOfActivities> ;
  owl:sameAs <https://w3id.org/dpv#hasRecordOfActivity>, <https://w3id.org/dpv/dpv-owl#hasRecordOfActivity> .

<https://w3id.org/dpv/owl#DesignStandard>
  a owl:Class, owl:NamedIndividual, <https://w3id.org/dpv/owl#OrganisationalMeasure> ;
  rdfs:subClassOf <https://w3id.org/dpv/owl#Standard> ;
  dc:contributor _:genid9, _:genid10, _:genid1, _:genid11 ;
  dc:created "2019-04-05"^^xsd:date ;
  ns1:term_status "accepted"@en ;
  skos:definition "A set of rules or guidelines outlining criterias for design"@en ;
  skos:prefLabel "Design Standard"@en ;
  owl:sameAs <https://w3id.org/dpv#DesignStandard>, <https://w3id.org/dpv/dpv-owl#DesignStandard> .

<https://w3id.org/dpv/owl#Student>
  a owl:Class, owl:NamedIndividual, <https://w3id.org/dpv/owl#HumanSubject> ;
  rdfs:subClassOf <https://w3id.org/dpv/owl#HumanSubject> ;
  dc:contributor _:genid4, _:genid5, _:genid1, _:genid17, _:genid6 ;
  dc:created "2022-04-06"^^xsd:date ;
  dc:modified "2024-12-17"^^xsd:date ;
  ns1:term_status "modified"@en ;
  skos:definition "Humans that are students"@en ;
  skos:prefLabel "Student"@en ;
  owl:sameAs <https://w3id.org/dpv#Student>, <https://w3id.org/dpv/dpv-owl#Student> .

odrl:index
  a owl:NamedIndividual, skos:Concept, odrl:Action ;
  odrl:includedIn odrl:use ;
  rdfs:isDefinedBy odrl: ;
  rdfs:label "Index"@en ;
  skos:definition "To record the Asset in an index."@en ;
  skos:note "For example, to include a link to the Asset in a search engine database."@en ;
  skos:scopeNote "Non-Normative"@en .

<https://w3id.org/dpv/owl#ControllerDataSubjectAgreement>
  a owl:Class, owl:NamedIndividual, <https://w3id.org/dpv/owl#LegalBasis>, <https://w3id.org/dpv/owl#LegalMeasure> ;
  rdfs:subClassOf <https://w3id.org/dpv/owl#DataSubjectContract> ;
  dc:created "2024-08-27"^^xsd:date ;
  dc:modified "2024-08-27"^^xsd:date ;
  ns1:term_status "modified"@en ;
  skos:definition "An agreement outlining conditions, criteria, obligations, responsibilities, and specifics for carrying out processing of data between a Data Controller and a Data Subject"@en ;
  skos:prefLabel "Controller-Data Subject Agreement"@en ;
  owl:sameAs <https://w3id.org/dpv#ControllerDataSubjectAgreement>, <https://w3id.org/dpv/dpv-owl#ControllerDataSubjectAgreement> .

odrl:compensatingParty
  a owl:ObjectProperty, owl:NamedIndividual, skos:Concept ;
  rdfs:subPropertyOf odrl:function ;
  rdfs:isDefinedBy odrl: ;
  rdfs:label "Compensating Party"@en ;
  skos:definition "The Party that is the provider of the compensation."@en ;
  skos:note "Maybe specified as part of the compensate duty action."@en ;
  skos:scopeNote "Non-Normative"@en .

<https://w3id.org/dpv/owl#ScientificResearch>
  a owl:Class, owl:NamedIndividual, <https://w3id.org/dpv/owl#Purpose> ;
  rdfs:subClassOf <https://w3id.org/dpv/owl#ResearchAndDevelopment> ;
  dc:contributor _:genid5, _:genid1 ;
  dc:created "2024-02-14"^^xsd:date ;
  dc:source "DGA 2.16"@en ;
  ns1:term_status "accepted"@en ;
  skos:definition "Purposes associated with scientific research"@en ;
  skos:prefLabel "Scientific Research"@en ;
  owl:sameAs <https://w3id.org/dpv#ScientificResearch>, <https://w3id.org/dpv/dpv-owl#ScientificResearch> .

<https://w3id.org/dpv/owl#RiskMitigationMeasure>
  a owl:Class ;
  rdfs:subClassOf <https://w3id.org/dpv/owl#TechnicalOrganisationalMeasure> ;
  dc:contributor _:genid4, _:genid1, _:genid6 ;
  dc:created "2020-11-04"^^xsd:date ;
  ns3:example <https://w3id.org/dpv/examples/owl#E0068> ;
  ns1:term_status "accepted"@en ;
  skos:definition "Measures intended to mitigate, minimise, or prevent risk."@en ;
  skos:prefLabel "Risk Mitigation Measure"@en ;
  owl:sameAs <https://w3id.org/dpv#RiskMitigationMeasure>, <https://w3id.org/dpv/dpv-owl#RiskMitigationMeasure> .

odrl:operand
  a owl:ObjectProperty, owl:NamedIndividual, skos:Concept ;
  rdfs:domain odrl:LogicalConstraint ;
  rdfs:isDefinedBy odrl: ;
  rdfs:label "Operand"@en ;
  skos:definition "Operand is an abstract property for a logical relationship."@en ;
  skos:note "Sub-properties of operand are used for Logical Constraints."@en .

odrl:absolutePosition
  a owl:NamedIndividual, skos:Concept, odrl:LeftOperand ;
  rdfs:isDefinedBy odrl: ;
  rdfs:label "Absolute Asset Position"@en ;
  skos:definition "A point in space or time defined with absolute coordinates for the positioning of the target Asset."@en ;
  skos:note "Example: The upper left corner of a picture may be constrained to a specific position of the canvas rendering it."@en ;
  skos:scopeNote "Non-Normative"@en .

<https://w3id.org/dpv/owl#CannotWithdrawFromProcess>
  a owl:Class, owl:NamedIndividual, <https://w3id.org/dpv/owl#EntityNonPermissiveInvolvement> ;
  rdfs:subClassOf <https://w3id.org/dpv/owl#EntityNonPermissiveInvolvement> ;
  dc:contributor _:genid1, _:genid25, _:genid19 ;
  dc:created "2024-05-11"^^xsd:date ;
  ns1:term_status "accepted"@en ;
  skos:definition "Involvement where entity cannot withdraw a previously given assent from specified context"@en ;
  skos:prefLabel "Cannot Withdraw from Process"@en ;
  owl:sameAs <https://w3id.org/dpv#CannotWithdrawFromProcess>, <https://w3id.org/dpv/dpv-owl#CannotWithdrawFromProcess> .

<https://w3id.org/dpv/owl#ContractDrafted>
  a owl:Class, owl:NamedIndividual, <https://w3id.org/dpv/owl#ContractPreparationStatus> ;
  rdfs:subClassOf <https://w3id.org/dpv/owl#ContractPreparationStatus> ;
  dc:contributor _:genid4, _:genid1, _:genid17 ;
  dc:created "2025-01-09"^^xsd:date ;
  ns1:term_status "accepted"@en ;
  skos:definition "Status representing the drafting of contract text has been completed and it can now be offered for signing"@en ;
  skos:prefLabel "Contract Drafted"@en ;
  owl:sameAs <https://w3id.org/dpv#ContractDrafted>, <https://w3id.org/dpv/dpv-owl#ContractDrafted> .

<https://w3id.org/dpv/owl#OrganisationComplianceManagement>
  a owl:Class, owl:NamedIndividual, <https://w3id.org/dpv/owl#Purpose> ;
  rdfs:subClassOf <https://w3id.org/dpv/owl#OrganisationGovernance> ;
  dc:contributor _:genid4, _:genid1, _:genid6, _:genid21 ;
  dc:created "2021-09-01"^^xsd:date ;
  ns1:term_status "accepted"@en ;
  skos:definition "Purposes associated with managing compliance for organisation in relation to internal policies"@en ;
  skos:prefLabel "Organisation Compliance Management"@en ;
  skos:scopeNote "Note that this concept relates to internal organisational compliance. The concept LegalCompliance should be used for external legal or regulatory compliance."@en ;
  owl:sameAs <https://w3id.org/dpv#OrganisationComplianceManagement>, <https://w3id.org/dpv/dpv-owl#OrganisationComplianceManagement> .

<https://w3id.org/dpv/owl#Verification>
  a owl:Class, owl:NamedIndividual, <https://w3id.org/dpv/owl#Purpose> ;
  rdfs:subClassOf <https://w3id.org/dpv/owl#EnforceSecurity> ;
  dc:contributor _:genid5, _:genid1 ;
  dc:created "2024-02-14"^^xsd:date ;
  ns1:term_status "accepted"@en ;
  skos:definition "Purposes association with verification e.g. information, identity, integrity"@en ;
  skos:prefLabel "Verification"@en ;
  owl:sameAs <https://w3id.org/dpv#Verification>, <https://w3id.org/dpv/dpv-owl#Verification> .

odrl:Action
  a owl:Class, owl:NamedIndividual, skos:Concept ;
  rdfs:subClassOf schema:Action ;
  rdfs:isDefinedBy odrl: ;
  rdfs:label "Action"@en ;
  skos:definition "An operation on an Asset."@en ;
  skos:note "Actions may be allowed by Permissions, disallowed by Prohibitions, or made mandatory by Duties."@en .

<https://w3id.org/dpv/owl#Authentication-ABC>
  a owl:Class, owl:NamedIndividual, <https://w3id.org/dpv/owl#TechnicalMeasure> ;
  rdfs:subClassOf <https://w3id.org/dpv/owl#CryptographicAuthentication> ;
  dc:contributor _:genid1 ;
  dc:created "2022-08-17"^^xsd:date ;
  dc:source [
    a ns0:WebPage ;
    ns0:name "ENISA Data Protection Engineering" ;
    ns0:url "https://www.enisa.europa.eu/publications/data-protection-engineering"
  ] ;
  ns1:term_status "accepted"@en ;
  skos:definition "Use of Attribute Based Credentials (ABC) to perform and manage authentication"@en ;
  skos:prefLabel "Authentication using ABC"@en ;
  owl:sameAs <https://w3id.org/dpv#Authentication-ABC>, <https://w3id.org/dpv/dpv-owl#Authentication-ABC> .

odrl:play
  a owl:NamedIndividual, skos:Concept, odrl:Action ;
  odrl:includedIn odrl:use ;
  rdfs:isDefinedBy odrl: ;
  rdfs:label "Play"@en ;
  skos:definition "To create a sequential and transient rendition of an Asset."@en ;
  skos:note "For example, to play a video or audio track. If the action is to be performed to a wider audience than just the Assignees, then the Recipient constraint is recommended to be used." ;
  skos:scopeNote "Non-Normative"@en .

<https://w3id.org/dpv/owl#ConsultationWithDataSubject>
  a owl:Class, owl:NamedIndividual, <https://w3id.org/dpv/owl#OrganisationalMeasure> ;
  rdfs:subClassOf <https://w3id.org/dpv/owl#Consultation> ;
  dc:contributor _:genid4, _:genid1 ;
  dc:created "2022-06-15"^^xsd:date ;
  ns1:term_status "accepted"@en ;
  skos:definition "Consultation with data subject(s) or their representative(s)"@en ;
  skos:prefLabel "Consultation with Data Subject"@en ;
  owl:sameAs <https://w3id.org/dpv#ConsultationWithDataSubject>, <https://w3id.org/dpv/dpv-owl#ConsultationWithDataSubject> .

<https://w3id.org/dpv/owl#DataQualityAssessment>
  a owl:Class, owl:NamedIndividual, <https://w3id.org/dpv/owl#OrganisationalMeasure> ;
  rdfs:subClassOf <https://w3id.org/dpv/owl#Assessment>, <https://w3id.org/dpv/owl#DataQualityManagement> ;
  dc:contributor _:genid1 ;
  dc:created "2024-04-14"^^xsd:date ;
  ns1:term_status "accepted"@en ;
  skos:definition "Measures associated with assessment of data quality"@en ;
  skos:prefLabel "Data Quality Assessment"@en ;
  owl:sameAs <https://w3id.org/dpv#DataQualityAssessment>, <https://w3id.org/dpv/dpv-owl#DataQualityAssessment> .

<https://w3id.org/dpv/owl#ContractStatus>
  a owl:Class ;
  rdfs:subClassOf <https://w3id.org/dpv/owl#Status> ;
  dc:contributor _:genid1 ;
  dc:created "2024-08-27"^^xsd:date ;
  ns3:example <https://w3id.org/dpv/examples/owl#E0077> ;
  ns1:term_status "accepted"@en ;
  skos:definition "Status associated with a contract"@en ;
  skos:prefLabel "Contract Status"@en ;
  owl:sameAs <https://w3id.org/dpv#ContractStatus>, <https://w3id.org/dpv/dpv-owl#ContractStatus> .

<https://w3id.org/dpv/owl#LegitimateInterestAssessment>
  a owl:Class, owl:NamedIndividual, <https://w3id.org/dpv/owl#OrganisationalMeasure> ;
  rdfs:subClassOf <https://w3id.org/dpv/owl#Assessment> ;
  dc:contributor _:genid4, _:genid1, _:genid6 ;
  dc:created "2021-09-08"^^xsd:date ;
  ns1:term_status "accepted"@en ;
  skos:definition "Indicates an assessment regarding the use of legitimate interest as a lawful basis by the data controller"@en ;
  skos:prefLabel "Legitimate Interest Assessment"@en ;
  owl:sameAs <https://w3id.org/dpv#LegitimateInterestAssessment>, <https://w3id.org/dpv/dpv-owl#LegitimateInterestAssessment> .

<https://w3id.org/dpv/owl#WithinVirtualEnvironment>
  a owl:Class, owl:NamedIndividual, <https://w3id.org/dpv/owl#Location> ;
  rdfs:subClassOf <https://w3id.org/dpv/owl#LocalLocation> ;
  dc:contributor _:genid1 ;
  dc:created "2020-10-06"^^xsd:date ;
  ns1:term_status "accepted"@en ;
  skos:definition "Location is local and entirely within a virtual environment, such as a shared network directory"@en ;
  skos:prefLabel "Within Virtual Environment"@en ;
  owl:sameAs <https://w3id.org/dpv#WithinVirtualEnvironment>, <https://w3id.org/dpv/dpv-owl#WithinVirtualEnvironment> .

<https://w3id.org/dpv/owl#ConfidentialData>
  a owl:Class ;
  rdfs:subClassOf <https://w3id.org/dpv/owl#Data> ;
  dc:created "2024-02-14"^^xsd:date ;
  dc:source "DGA 5.10"@en ;
  ns1:term_status "accepted"@en ;
  skos:definition "Data deemed confidential"@en ;
  skos:prefLabel "Confidential Data"@en ;
  owl:sameAs <https://w3id.org/dpv#ConfidentialData>, <https://w3id.org/dpv/dpv-owl#ConfidentialData> .

<https://w3id.org/dpv/owl#hasName>
  a owl:ObjectProperty ;
  ns2:domainIncludes <https://w3id.org/dpv/owl#Entity> ;
  dc:contributor _:genid4, _:genid5, _:genid1, _:genid6 ;
  dc:created "2020-11-04"^^xsd:date ;
  ns1:term_status "accepted"@en ;
  skos:definition "Specifies name of a legal entity"@en ;
  skos:prefLabel "has name"@en ;
  ns0:domainIncludes <https://w3id.org/dpv/owl#Entity> ;
  owl:sameAs <https://w3id.org/dpv#hasName>, <https://w3id.org/dpv/dpv-owl#hasName> .

dc:isPartOf
  a owl:ObjectProperty ;
  ns2:domainIncludes <https://w3id.org/dpv/owl#RightExerciseActivity> ;
  ns2:rangeIncludes <https://w3id.org/dpv/owl#RightExerciseRecord> ;
  skos:prefLabel "dct:isPartOf"@en ;
  skos:scopeNote "Also used for specifying a RightExerciseActivity is part of a RightExerciseRecord"@en ;
  ns0:domainIncludes <https://w3id.org/dpv/owl#RightExerciseActivity> ;
  ns0:rangeIncludes <https://w3id.org/dpv/owl#RightExerciseRecord> .

<https://w3id.org/dpv/owl#DataLiteracy>
  a owl:Class, owl:NamedIndividual, <https://w3id.org/dpv/owl#OrganisationalMeasure> ;
  rdfs:subClassOf <https://w3id.org/dpv/owl#DigitalLiteracy> ;
  dc:contributor _:genid1 ;
  dc:created "2024-05-17"^^xsd:date ;
  ns1:term_status "accepted"@en ;
  skos:definition "Providing skills, knowledge, and understanding to enable reading, writing, analysing, reasoning, and communicating regarding data"@en ;
  skos:prefLabel "Data Literacy"@en ;
  owl:sameAs <https://w3id.org/dpv#DataLiteracy>, <https://w3id.org/dpv/dpv-owl#DataLiteracy> .

<https://w3id.org/dpv/owl#Erase>
  a owl:Class, owl:NamedIndividual, <https://w3id.org/dpv/owl#Processing> ;
  rdfs:subClassOf <https://w3id.org/dpv/owl#Remove> ;
  dc:created "2019-05-07"^^xsd:date ;
  dc:source [
    a ns0:WebPage ;
    ns0:name "GDPR Art.4-2" ;
    ns0:url "https://eur-lex.europa.eu/eli/reg/2016/679/art_4/par_2/oj"
  ] ;
  ns1:term_status "accepted"@en ;
  skos:definition "to remove data from existence i.e. without the possibility of retrieval"@en ;
  skos:prefLabel "Erase Data"@en ;
  owl:sameAs <https://w3id.org/dpv#Erase>, <https://w3id.org/dpv/dpv-owl#Erase> .

<https://w3id.org/dpv/owl#CannotReverseProcessInput>
  a owl:Class, owl:NamedIndividual, <https://w3id.org/dpv/owl#EntityNonPermissiveInvolvement> ;
  rdfs:subClassOf <https://w3id.org/dpv/owl#EntityNonPermissiveInvolvement> ;
  dc:contributor _:genid1, _:genid25, _:genid19 ;
  dc:created "2024-05-11"^^xsd:date ;
  ns1:term_status "accepted"@en ;
  skos:definition "Involvement where entity cannot reverse input of specified context"@en ;
  skos:prefLabel "Cannot Reverse Process Input"@en ;
  skos:scopeNote "Reversion can be considered a form of correction in some instances. We welcome inputs to further explore and define this relation between correction and reversion concepts."@en ;
  owl:sameAs <https://w3id.org/dpv#CannotReverseProcessInput>, <https://w3id.org/dpv/dpv-owl#CannotReverseProcessInput> .

<https://w3id.org/dpv/owl#ContractInactive>
  a owl:Class, owl:NamedIndividual, <https://w3id.org/dpv/owl#ContractActivationStatus> ;
  rdfs:subClassOf <https://w3id.org/dpv/owl#ContractActivationStatus> ;
  dc:contributor _:genid4, _:genid1, _:genid17 ;
  dc:created "2025-01-09"^^xsd:date ;
  ns1:term_status "accepted"@en ;
  skos:definition "Status representing contract that has been fully executed and whose terms are not yet active i.e. they need to be performed at a later time"@en ;
  skos:prefLabel "Contract Inactive"@en ;
  skos:scopeNote "An example of an inactive contract is where its terms need to be fulfiled at a later date, at which point the contract will become active"@en ;
  owl:sameAs <https://w3id.org/dpv#ContractInactive>, <https://w3id.org/dpv/dpv-owl#ContractInactive> .

<https://w3id.org/dpv/owl#SecureProcessingEnvironment>
  a owl:Class, owl:NamedIndividual, <https://w3id.org/dpv/owl#OrganisationalMeasure> ;
  rdfs:subClassOf <https://w3id.org/dpv/owl#SecurityProcedure> ;
  dc:contributor _:genid5, _:genid1 ;
  dc:created "2024-04-14"^^xsd:date ;
  dc:source "DGA 2.20"@en ;
  ns1:term_status "accepted"@en ;
  skos:definition "A physical or virtual environment supported by organisational means that integrates security and compliance requirements and allows supervising data processing actions"@en ;
  skos:prefLabel "Secure Processing Environment"@en ;
  owl:sameAs <https://w3id.org/dpv#SecureProcessingEnvironment>, <https://w3id.org/dpv/dpv-owl#SecureProcessingEnvironment> .

<https://w3id.org/dpv/owl#hasImpactOn>
  a owl:ObjectProperty ;
  rdfs:subPropertyOf <https://w3id.org/dpv/owl#hasConsequenceOn> ;
  ns2:domainIncludes <https://w3id.org/dpv/owl#Impact> ;
  dc:contributor _:genid4, _:genid5, _:genid1, _:genid17, _:genid15 ;
  dc:created "2022-05-18"^^xsd:date ;
  ns3:example <https://w3id.org/dpv/examples/owl#E0068> ;
  ns1:term_status "accepted"@en ;
  skos:definition "Indicates the thing (e.g. plan, process, or entity) affected by an impact"@en ;
  skos:prefLabel "has impact on"@en ;
  ns0:domainIncludes <https://w3id.org/dpv/owl#Impact> ;
  owl:sameAs <https://w3id.org/dpv#hasImpactOn>, <https://w3id.org/dpv/dpv-owl#hasImpactOn> .

<https://w3id.org/dpv/owl#G2CContract>
  a owl:Class, owl:NamedIndividual, <https://w3id.org/dpv/owl#LegalBasis> ;
  rdfs:subClassOf <https://w3id.org/dpv/owl#ContractByEntityType> ;
  dc:created "2024-08-27"^^xsd:date ;
  ns1:term_status "accepted"@en ;
  skos:definition "A contract between a government and consumers"@en ;
  skos:prefLabel "Government-to-Consumer Contract"@en ;
  owl:sameAs <https://w3id.org/dpv#G2CContract>, <https://w3id.org/dpv/dpv-owl#G2CContract> .

<https://w3id.org/dpv/owl#Applicability>
  a owl:Class ;
  rdfs:subClassOf <https://w3id.org/dpv/owl#Context> ;
  dc:contributor _:genid1 ;
  dc:created "2023-08-24"^^xsd:date ;
  ns3:example <https://w3id.org/dpv/examples/owl#E0053> ;
  ns1:term_status "accepted"@en ;
  skos:definition "Concept provided to represent indication of cases where the information or context is not applicable (N/A) or not available or this is not known or determined yet. If the information is applicable and available, this concept should not be used."@en ;
  skos:prefLabel "Applicability"@en ;
  skos:scopeNote "These concepts are useful in closed-world interpretations, for example in forms where a field must have a value to explicitly denote it is not applicable or the information is not available yet."@en ;
  owl:sameAs <https://w3id.org/dpv#Applicability>, <https://w3id.org/dpv/dpv-owl#Applicability> .

<https://w3id.org/dpv/owl#FulfilmentOfObligation>
  a owl:Class, owl:NamedIndividual, <https://w3id.org/dpv/owl#Purpose> ;
  rdfs:subClassOf <https://w3id.org/dpv/owl#Purpose> ;
  dc:contributor _:genid4, _:genid1 ;
  dc:created "2022-11-09"^^xsd:date ;
  ns1:term_status "accepted"@en ;
  skos:definition "Purposes associated with carrying out data processing to fulfill an obligation"@en ;
  skos:prefLabel "Fulfilment of Obligation"@en ;
  owl:sameAs <https://w3id.org/dpv#FulfilmentOfObligation>, <https://w3id.org/dpv/dpv-owl#FulfilmentOfObligation> .

<https://w3id.org/dpv/owl#ContractualTerms>
  a owl:Class, owl:NamedIndividual, <https://w3id.org/dpv/owl#LegalMeasure> ;
  rdfs:subClassOf <https://w3id.org/dpv/owl#LegalMeasure> ;
  dc:contributor _:genid9, _:genid10, _:genid1, _:genid11 ;
  dc:created "2019-04-05"^^xsd:date ;
  dc:modified "2024-08-27"^^xsd:date ;
  ns1:term_status "sunset"@en ;
  skos:definition "Contractual terms governing data handling within or with an entity"@en ;
  skos:prefLabel "Contractual Terms"@en ;
  owl:sameAs <https://w3id.org/dpv#ContractualTerms>, <https://w3id.org/dpv/dpv-owl#ContractualTerms> .

<https://w3id.org/dpv/owl#MetadataManagement>
  a owl:Class, owl:NamedIndividual, <https://w3id.org/dpv/owl#OrganisationalMeasure> ;
  rdfs:subClassOf <https://w3id.org/dpv/owl#DataGovernance> ;
  dc:contributor _:genid1 ;
  dc:created "2024-04-14"^^xsd:date ;
  ns1:term_status "accepted"@en ;
  skos:definition "Measures associated with management of metadata"@en ;
  skos:prefLabel "Metadata Management"@en ;
  skos:scopeNote "Examples of metadata management include assessing which metadata are required or being used by technology, assessing their potential inclusion as personal data, and implementing a metadata based solution to manage data"@en ;
  owl:sameAs <https://w3id.org/dpv#MetadataManagement>, <https://w3id.org/dpv/dpv-owl#MetadataManagement> .

<https://w3id.org/dpv/owl#IntentionStatus>
  a owl:Class ;
  rdfs:subClassOf <https://w3id.org/dpv/owl#Status> ;
  dc:contributor _:genid4, _:genid1, _:genid25, _:genid6 ;
  dc:created "2024-05-10"^^xsd:date ;
  ns1:term_status "accepted"@en ;
  skos:definition "Status indicating whether the specified context was intended or unintended"@en ;
  skos:prefLabel "Intention Status"@en ;
  skos:scopeNote "Intention is associated with the goal or purpose for what is about to happen i.e. an ex-ante indication of whether the specified context is/was planned or intended. Intention and Expectation are closely related terms. We recommend using Intention when the entity has the ability to control the implementation and Expectation for when the entity does not have control or for what happens after or beyond the exercise of control."@en ;
  owl:sameAs <https://w3id.org/dpv#IntentionStatus>, <https://w3id.org/dpv/dpv-owl#IntentionStatus> .

<https://w3id.org/dpv/owl#serialisation-n3>
  a owl:NamedIndividual, ns4:ResourceDescriptor ;
  dc:format <https://www.iana.org/assignments/media-types/text/n3> ;
  dc:conformsTo <https://www.w3.org/TeamSubmission/n3/> ;
  dc:title "Data Privacy Vocabulary (DPV) - N3 serialiation" ;
  ns4:hasArtifact <https://w3id.org/dpv/dpv/dpv-owl.n3> ;
  ns4:hasRole <http://www.w3.org/ns/dx/prof/role/vocabulary> ;
  owl:sameAs <https://w3id.org/dpv#serialisation-n3>, <https://w3id.org/dpv/dpv-owl#serialisation-n3> .

<https://w3id.org/dpv/owl#NotificationOngoing>
  a owl:Class, owl:NamedIndividual, <https://w3id.org/dpv/owl#NotificationStatus> ;
  rdfs:subClassOf <https://w3id.org/dpv/owl#NotificationStatus> ;
  dc:contributor _:genid1 ;
  dc:created "2024-05-19"^^xsd:date ;
  ns1:term_status "accepted"@en ;
  skos:definition "Status indicating notification(s) are ongoing"@en ;
  skos:prefLabel "Notification Ongoing"@en ;
  owl:sameAs <https://w3id.org/dpv#NotificationOngoing>, <https://w3id.org/dpv/dpv-owl#NotificationOngoing> .

<https://w3id.org/dpv/owl#Duration>
  a owl:Class ;
  rdfs:subClassOf <https://w3id.org/dpv/owl#Context> ;
  dc:contributor _:genid1 ;
  dc:created "2022-02-09"^^xsd:date ;
  ns3:example <https://w3id.org/dpv/examples/owl#E0050>, <https://w3id.org/dpv/examples/owl#E0070> ;
  ns1:term_status "accepted"@en ;
  skos:definition "The duration or temporal limitation"@en ;
  skos:prefLabel "Duration"@en ;
  owl:sameAs <https://w3id.org/dpv#Duration>, <https://w3id.org/dpv/dpv-owl#Duration> .

<https://w3id.org/dpv/owl#CommunicationForCustomerCare>
  a owl:Class, owl:NamedIndividual, <https://w3id.org/dpv/owl#Purpose> ;
  rdfs:subClassOf <https://w3id.org/dpv/owl#CommunicationManagement>, <https://w3id.org/dpv/owl#CustomerCare> ;
  dc:contributor _:genid4, _:genid5, _:genid1 ;
  dc:created "2020-11-04"^^xsd:date ;
  ns1:term_status "accepted"@en ;
  skos:definition "Customer Care Communication refers to purposes associated with communicating with customers for assisting them, resolving issues, ensuring satisfaction, etc. in relation to services provided"@en ;
  skos:prefLabel "Communication for Customer Care"@en ;
  owl:sameAs <https://w3id.org/dpv#CommunicationForCustomerCare>, <https://w3id.org/dpv/dpv-owl#CommunicationForCustomerCare> .

<https://w3id.org/dpv/owl#SecurityProcedure>
  a owl:Class, owl:NamedIndividual, <https://w3id.org/dpv/owl#OrganisationalMeasure> ;
  rdfs:subClassOf <https://w3id.org/dpv/owl#OrganisationalMeasure> ;
  dc:contributor _:genid1 ;
  dc:created "2022-08-24"^^xsd:date ;
  ns1:term_status "accepted"@en ;
  skos:definition "Procedures associated with assessing, implementing, and evaluating security"@en ;
  skos:prefLabel "Security Procedure"@en ;
  owl:sameAs <https://w3id.org/dpv#SecurityProcedure>, <https://w3id.org/dpv/dpv-owl#SecurityProcedure> .

<https://w3id.org/dpv/owl#RemoteLocation>
  a owl:Class, owl:NamedIndividual, <https://w3id.org/dpv/owl#Location> ;
  rdfs:subClassOf <https://w3id.org/dpv/owl#LocationLocality> ;
  dc:contributor _:genid1 ;
  dc:created "2022-06-15"^^xsd:date ;
  dc:modified "2020-10-05"^^xsd:date ;
  ns1:term_status "accepted"@en ;
  skos:definition "Location is remote i.e. not local"@en ;
  skos:prefLabel "Remote Location"@en ;
  owl:sameAs <https://w3id.org/dpv#RemoteLocation>, <https://w3id.org/dpv/dpv-owl#RemoteLocation> .

<https://w3id.org/dpv/owl#RiskConcept>
  a owl:Class ;
  dc:contributor _:genid10, _:genid1, _:genid25 ;
  dc:created "2024-08-16"^^xsd:date ;
  ns1:term_status "accepted"@en ;
  skos:definition "Parent concept for combining concepts associated with risk assessment such as actual and potential Risk, Risk Source, Consequences, and Impacts"@en ;
  skos:prefLabel "Risk Concept"@en ;
  skos:scopeNote "RiskConcept is a generic concept used for creation of specific taxonomies in the RISK extension to provide guidance on how a concept can potentially be a risk, risk source, consequence, and impact. It is not intended to be used directly and is only created for organisation of concepts in DPV vocabularies"@en ;
  owl:sameAs <https://w3id.org/dpv#RiskConcept>, <https://w3id.org/dpv/dpv-owl#RiskConcept> .

<https://w3id.org/dpv/owl#VitalInterestOfDataSubject>
  a owl:Class, owl:NamedIndividual, <https://w3id.org/dpv/owl#LegalBasis> ;
  rdfs:subClassOf <https://w3id.org/dpv/owl#VitalInterestOfNaturalPerson> ;
  dc:contributor _:genid4, _:genid1, _:genid6 ;
  dc:created "2021-04-21"^^xsd:date ;
  ns1:term_status "accepted"@en ;
  skos:definition "Activities are necessary or required to protect vital interests of a data subject"@en ;
  skos:prefLabel "Vital Interest of Data Subject"@en ;
  owl:sameAs <https://w3id.org/dpv#VitalInterestOfDataSubject>, <https://w3id.org/dpv/dpv-owl#VitalInterestOfDataSubject> .

<https://w3id.org/dpv/owl#Autonomous>
  a owl:Class, owl:NamedIndividual, <https://w3id.org/dpv/owl#AutomationLevel> ;
  rdfs:subClassOf <https://w3id.org/dpv/owl#AutomationLevel> ;
  dc:contributor _:genid1, _:genid25 ;
  dc:created "2023-12-10"^^xsd:date ;
  dc:modified "2024-04-20"^^xsd:date ;
  dc:source [
    a ns0:WebPage ;
    ns0:name "ISO/IEC 22989:2022 Artificial intelligence concepts and terminology" ;
    ns0:url "https://www.iso.org/standard/74296.html"
  ] ;
  ns1:term_status "accepted"@en ;
  skos:definition "Level of automation corresponding to Level 6 in ISO/IEC 22989:2022 where the automation in system is capable of modifying its operation domain or its goals without external intervention, control or oversight"@en ;
  skos:prefLabel "Autonomous"@en ;
  skos:scopeNote "Though Autonomous, such operations can still be associated with dpv:HumanInvolved e.g. for inputs, oversight or verification"@en ;
  owl:sameAs <https://w3id.org/dpv#Autonomous>, <https://w3id.org/dpv/dpv-owl#Autonomous> .

<https://w3id.org/dpv/owl#ProvidedData>
  a owl:Class ;
  rdfs:subClassOf <https://w3id.org/dpv/owl#CollectedData> ;
  dc:contributor _:genid1, _:genid6 ;
  dc:created "2024-04-20"^^xsd:date ;
  ns1:term_status "accepted"@en ;
  skos:definition "Data that has been provided by an entity"@en ;
  skos:prefLabel "Provided Data"@en ;
  skos:scopeNote "Provided data involves one entity explicitly providing the data, which the other entity then collects"@en ;
  owl:sameAs <https://w3id.org/dpv#ProvidedData>, <https://w3id.org/dpv/dpv-owl#ProvidedData> .

<https://w3id.org/dpv/owl#CrossBorderTransfer>
  a owl:Class, owl:NamedIndividual, <https://w3id.org/dpv/owl#Processing> ;
  rdfs:subClassOf <https://w3id.org/dpv/owl#Transfer> ;
  dc:contributor _:genid1 ;
  dc:created "2024-04-14"^^xsd:date ;
  ns1:term_status "accepted"@en ;
  skos:definition "to move data from one jurisdiction (border) to another"@en ;
  skos:prefLabel "Cross-Border Data Transfer"@en ;
  owl:sameAs <https://w3id.org/dpv#CrossBorderTransfer>, <https://w3id.org/dpv/dpv-owl#CrossBorderTransfer> .

<https://w3id.org/dpv/owl#CommercialResearch>
  a owl:Class, owl:NamedIndividual, <https://w3id.org/dpv/owl#Purpose> ;
  rdfs:subClassOf <https://w3id.org/dpv/owl#CommercialPurpose>, <https://w3id.org/dpv/owl#ResearchAndDevelopment> ;
  dc:contributor _:genid13, _:genid14, _:genid1, _:genid15, _:genid16, _:genid11 ;
  dc:created "2019-04-05"^^xsd:date ;
  dc:modified "2024-04-14"^^xsd:date ;
  ns1:term_status "accepted"@en ;
  skos:definition "Purposes associated with conducting research in a commercial setting or with intention to commercialise e.g. in a company or sponsored by a company"@en ;
  skos:prefLabel "Commercial Research"@en ;
  skos:related <https://specialprivacy.ercim.eu/vocabs/purposes#Develop> ;
  owl:sameAs <https://w3id.org/dpv#CommercialResearch>, <https://w3id.org/dpv/dpv-owl#CommercialResearch> .

<https://w3id.org/dpv/owl#ProtectionOfIPR>
  a owl:Class, owl:NamedIndividual, <https://w3id.org/dpv/owl#Purpose> ;
  rdfs:subClassOf <https://w3id.org/dpv/owl#FulfilmentOfObligation> ;
  dc:contributor _:genid5, _:genid1 ;
  dc:created "2024-02-14"^^xsd:date ;
  dc:source "DGA 3.1(c)"@en ;
  ns1:term_status "accepted"@en ;
  skos:definition "Purposes associated with the protection of intellectual property rights"@en ;
  skos:prefLabel "Protection of Intellectual Property Rights"@en ;
  owl:sameAs <https://w3id.org/dpv#ProtectionOfIPR>, <https://w3id.org/dpv/dpv-owl#ProtectionOfIPR> .

<https://w3id.org/dpv/owl#ContractPreparationStatus>
  a owl:Class ;
  rdfs:subClassOf <https://w3id.org/dpv/owl#ContractStatus> ;
  dc:contributor _:genid4, _:genid1, _:genid17 ;
  dc:created "2025-01-09"^^xsd:date ;
  ns1:term_status "accepted"@en ;
  skos:definition "Status associated with preparation of contracts before they are signed or accepted or executed"@en ;
  skos:prefLabel "Contract Preparation Status"@en ;
  owl:sameAs <https://w3id.org/dpv#ContractPreparationStatus>, <https://w3id.org/dpv/dpv-owl#ContractPreparationStatus> .

<https://w3id.org/dpv/owl#DataInteroperabilityImprovement>
  a owl:Class, owl:NamedIndividual, <https://w3id.org/dpv/owl#OrganisationalMeasure> ;
  rdfs:subClassOf <https://w3id.org/dpv/owl#DataInteroperabilityManagement> ;
  dc:contributor _:genid5, _:genid1 ;
  dc:created "2024-04-14"^^xsd:date ;
  dc:source "DGA 12.d"@en ;
  ns1:term_status "accepted"@en ;
  skos:definition "Measures associated with improvement of data interoperability"@en ;
  skos:prefLabel "Data Interoperability Improvement"@en ;
  owl:sameAs <https://w3id.org/dpv#DataInteroperabilityImprovement>, <https://w3id.org/dpv/dpv-owl#DataInteroperabilityImprovement> .

<https://w3id.org/dpv/owl#Copy>
  a owl:Class, owl:NamedIndividual, <https://w3id.org/dpv/owl#Processing> ;
  rdfs:subClassOf <https://w3id.org/dpv/owl#Processing> ;
  dc:created "2019-05-07"^^xsd:date ;
  dc:source [
    a ns0:WebPage ;
    ns0:name "SPECIAL Project" ;
    ns0:url "https://specialprivacy.ercim.eu/vocabs/processing"
  ] ;
  ns1:term_status "accepted"@en ;
  skos:definition "to produce an exact reproduction of the data"@en ;
  skos:prefLabel "Copy Data"@en ;
  skos:related <https://specialprivacy.ercim.eu/vocabs/processing#Copy> ;
  owl:sameAs <https://w3id.org/dpv#Copy>, <https://w3id.org/dpv/dpv-owl#Copy> .

<https://w3id.org/dpv/owl#AlgorithmicLogic>
  a owl:Class ;
  rdfs:subClassOf <https://w3id.org/dpv/owl#ProcessingContext> ;
  dc:contributor _:genid1 ;
  dc:created "2022-01-26"^^xsd:date ;
  dc:modified "2023-12-10"^^xsd:date ;
  ns1:term_status "accepted"@en ;
  skos:definition "The algorithmic logic applied or used"@en ;
  skos:prefLabel "Algorithmic Logic"@en ;
  skos:scopeNote "Algorithmic Logic is intended as a broad concept for explaining the use of algorithms and automated decisions making within Processing. To describe the actual algorithm, see the Algorithm concept."@en ;
  owl:sameAs <https://w3id.org/dpv#AlgorithmicLogic>, <https://w3id.org/dpv/dpv-owl#AlgorithmicLogic> .

<https://w3id.org/dpv/owl#ConsentRecord>
  a owl:Class, owl:NamedIndividual, <https://w3id.org/dpv/owl#OrganisationalMeasure> ;
  rdfs:subClassOf <https://w3id.org/dpv/owl#DataProcessingRecord> ;
  dc:contributor _:genid4, _:genid1, _:genid17, _:genid6 ;
  dc:created "2022-06-22"^^xsd:date ;
  ns3:example <https://w3id.org/dpv/examples/owl#E0016>, <https://w3id.org/dpv/examples/owl#E0023> ;
  ns1:term_status "accepted"@en ;
  skos:definition "A Record of Consent or Consent related activities"@en ;
  skos:prefLabel "Consent Record"@en ;
  owl:sameAs <https://w3id.org/dpv#ConsentRecord>, <https://w3id.org/dpv/dpv-owl#ConsentRecord> .

<https://w3id.org/dpv/owl#TemporalDuration>
  a owl:Class ;
  rdfs:subClassOf <https://w3id.org/dpv/owl#Duration> ;
  dc:contributor _:genid1 ;
  dc:created "2022-06-15"^^xsd:date ;
  dc:modified "2020-10-05"^^xsd:date ;
  ns1:term_status "accepted"@en ;
  skos:definition "Duration that has a fixed temporal duration e.g. 6 months"@en ;
  skos:prefLabel "Temporal Duration"@en ;
  owl:sameAs <https://w3id.org/dpv#TemporalDuration>, <https://w3id.org/dpv/dpv-owl#TemporalDuration> .

<https://w3id.org/dpv/owl#IncreaseServiceRobustness>
  a owl:Class, owl:NamedIndividual, <https://w3id.org/dpv/owl#Purpose> ;
  rdfs:subClassOf <https://w3id.org/dpv/owl#OptimisationForController> ;
  dc:contributor _:genid13, _:genid14, _:genid1, _:genid15, _:genid16, _:genid11 ;
  dc:created "2019-04-05"^^xsd:date ;
  ns1:term_status "accepted"@en ;
  skos:definition "Purposes associated with improving robustness and resilience of services"@en ;
  skos:prefLabel "Increase Service Robustness"@en ;
  owl:sameAs <https://w3id.org/dpv#IncreaseServiceRobustness>, <https://w3id.org/dpv/dpv-owl#IncreaseServiceRobustness> .

odrl:Prohibition
  a owl:Class, owl:NamedIndividual, skos:Concept ;
  rdfs:subClassOf odrl:Rule ;
  rdfs:isDefinedBy odrl: ;
  rdfs:label "Prohibition"@en ;
  skos:definition "The inability to perform an Action over an Asset."@en .

<https://w3id.org/dpv/owl#hasAssessment>
  a owl:ObjectProperty ;
  rdfs:subPropertyOf <https://w3id.org/dpv/owl#hasOrganisationalMeasure> ;
  ns2:rangeIncludes <https://w3id.org/dpv/owl#Assessment> ;
  dc:contributor _:genid1 ;
  dc:created "2024-04-14"^^xsd:date ;
  ns1:term_status "accepted"@en ;
  skos:definition "Indicates a relevant assessment associated with the specific context"@en ;
  skos:prefLabel "has assessment"@en ;
  ns0:rangeIncludes <https://w3id.org/dpv/owl#Assessment> ;
  owl:sameAs <https://w3id.org/dpv#hasAssessment>, <https://w3id.org/dpv/dpv-owl#hasAssessment> .

<https://w3id.org/dpv/owl#LoggingPolicy>
  a owl:Class, owl:NamedIndividual, <https://w3id.org/dpv/owl#OrganisationalMeasure> ;
  rdfs:subClassOf <https://w3id.org/dpv/owl#Policy> ;
  dc:contributor _:genid1 ;
  dc:created "2022-08-17"^^xsd:date ;
  dc:modified "2024-04-14"^^xsd:date ;
  dc:source [
    a ns0:WebPage ;
    ns0:name "ENISA 5G Cybersecurity Standards" ;
    ns0:url "https://www.enisa.europa.eu/publications/5g-cybersecurity-standards"
  ] ;
  ns1:term_status "accepted"@en ;
  skos:definition "Policy for logging of information"@en ;
  skos:prefLabel "Logging Policy"@en ;
  owl:sameAs <https://w3id.org/dpv#LoggingPolicy>, <https://w3id.org/dpv/dpv-owl#LoggingPolicy> .

<https://w3id.org/dpv/owl#CryptographicMethods>
  a owl:Class, owl:NamedIndividual, <https://w3id.org/dpv/owl#TechnicalMeasure> ;
  rdfs:subClassOf <https://w3id.org/dpv/owl#TechnicalMeasure> ;
  dc:contributor _:genid1 ;
  dc:created "2022-08-17"^^xsd:date ;
  dc:source [
    a ns0:WebPage ;
    ns0:name "ENISA Reference Incident Classification Taxonomy 2018" ;
    ns0:url "https://www.enisa.europa.eu/publications/reference-incident-classification-taxonomy/"
  ] ;
  ns1:term_status "accepted"@en ;
  skos:definition "Use of cryptographic methods to perform tasks"@en ;
  skos:prefLabel "Cryptographic Methods"@en ;
  owl:sameAs <https://w3id.org/dpv#CryptographicMethods>, <https://w3id.org/dpv/dpv-owl#CryptographicMethods> .

<https://w3id.org/dpv/owl#hasDuration>
  a owl:ObjectProperty ;
  ns2:rangeIncludes <https://w3id.org/dpv/owl#Duration> ;
  dc:contributor _:genid9, _:genid10, _:genid1, _:genid11 ;
  dc:created "2019-04-05"^^xsd:date ;
  dc:source [
    a ns0:WebPage ;
    ns0:name "SPECIAL Project" ;
    ns0:url "https://specialprivacy.ercim.eu/"
  ] ;
  ns3:example <https://w3id.org/dpv/examples/owl#E0050>, <https://w3id.org/dpv/examples/owl#E0070> ;
  ns1:term_status "accepted"@en ;
  skos:definition "Indicates information about duration"@en ;
  skos:prefLabel "has duration"@en ;
  ns0:rangeIncludes <https://w3id.org/dpv/owl#Duration> ;
  owl:sameAs <https://w3id.org/dpv#hasDuration>, <https://w3id.org/dpv/dpv-owl#hasDuration> .

<https://w3id.org/dpv/owl#RiskAssessment>
  a owl:Class, owl:NamedIndividual, <https://w3id.org/dpv/owl#OrganisationalMeasure> ;
  rdfs:subClassOf <https://w3id.org/dpv/owl#Assessment> ;
  dc:contributor _:genid1 ;
  dc:created "2024-04-14"^^xsd:date ;
  ns1:term_status "accepted"@en ;
  skos:definition "Assessment involving identification, analysis, and evaluation of risk"@en ;
  skos:prefLabel "Risk Assessment"@en ;
  owl:sameAs <https://w3id.org/dpv#RiskAssessment>, <https://w3id.org/dpv/dpv-owl#RiskAssessment> .

<https://w3id.org/dpv/owl#Subscriber>
  a owl:Class, owl:NamedIndividual, <https://w3id.org/dpv/owl#HumanSubject> ;
  rdfs:subClassOf <https://w3id.org/dpv/owl#HumanSubject> ;
  dc:contributor _:genid4, _:genid5, _:genid1, _:genid17, _:genid6 ;
  dc:created "2022-04-06"^^xsd:date ;
  dc:modified "2024-12-17"^^xsd:date ;
  ns1:term_status "modified"@en ;
  skos:definition "Humans that subscribe to service(s)"@en ;
  skos:prefLabel "Subscriber"@en ;
  skos:scopeNote "note: subscriber can be customer or consumer"@en ;
  owl:sameAs <https://w3id.org/dpv#Subscriber>, <https://w3id.org/dpv/dpv-owl#Subscriber> .

<https://w3id.org/dpv/owl#DataPublishedByDataSubject>
  a owl:Class, owl:NamedIndividual, <https://w3id.org/dpv/owl#DataSubjectDataSource> ;
  rdfs:subClassOf <https://w3id.org/dpv/owl#DataSubjectDataSource> ;
  dc:contributor _:genid17 ;
  dc:created "2022-08-24"^^xsd:date ;
  dc:modified "2023-12-10"^^xsd:date ;
  ns1:term_status "accepted"@en ;
  skos:definition "Data is published by the data subject"@en ;
  skos:prefLabel "Data published by Data Subject"@en ;
  skos:scopeNote "This refers to where that data was made publicly available by the data subject. An example of this would be a social media profile that the data subject has made publicly accessible."@en ;
  owl:sameAs <https://w3id.org/dpv#DataPublishedByDataSubject>, <https://w3id.org/dpv/dpv-owl#DataPublishedByDataSubject> .

<https://w3id.org/dpv/owl#EffectivenessDeterminationProcedures>
  a owl:Class, owl:NamedIndividual, <https://w3id.org/dpv/owl#OrganisationalMeasure> ;
  rdfs:subClassOf <https://w3id.org/dpv/owl#Assessment> ;
  dc:contributor _:genid1 ;
  dc:created "2022-08-17"^^xsd:date ;
  dc:source [
    a ns0:WebPage ;
    ns0:name "ENISA 5G Cybersecurity Standards" ;
    ns0:url "https://www.enisa.europa.eu/publications/5g-cybersecurity-standards"
  ] ;
  ns1:term_status "accepted"@en ;
  skos:definition "Procedures intended to determine effectiveness of other measures"@en ;
  skos:prefLabel "Effectiveness Determination Procedures"@en ;
  owl:sameAs <https://w3id.org/dpv#EffectivenessDeterminationProcedures>, <https://w3id.org/dpv/dpv-owl#EffectivenessDeterminationProcedures> .

<https://w3id.org/dpv/owl#PublicInterest>
  a owl:Class, owl:NamedIndividual, <https://w3id.org/dpv/owl#LegalBasis> ;
  rdfs:subClassOf <https://w3id.org/dpv/owl#LegalBasis> ;
  dc:contributor _:genid1 ;
  dc:created "2021-04-21"^^xsd:date ;
  ns3:example <https://w3id.org/dpv/examples/owl#E0082> ;
  ns1:term_status "accepted"@en ;
  skos:definition "Activities are necessary or beneficial for interest of the public or society at large"@en ;
  skos:prefLabel "Public Interest"@en ;
  owl:sameAs <https://w3id.org/dpv#PublicInterest>, <https://w3id.org/dpv/dpv-owl#PublicInterest> .

<https://w3id.org/dpv/owl#ContractPreamble>
  a owl:Class, owl:NamedIndividual, <https://w3id.org/dpv/owl#ContractualClause> ;
  rdfs:subClassOf <https://w3id.org/dpv/owl#ContractualClause> ;
  dc:created "2024-08-27"^^xsd:date ;
  ns1:term_status "accepted"@en ;
  skos:definition "An introductory section outlining the background, context, and purpose of the contract"@en ;
  skos:prefLabel "Contract Preamble"@en ;
  owl:sameAs <https://w3id.org/dpv#ContractPreamble>, <https://w3id.org/dpv/dpv-owl#ContractPreamble> .

<https://w3id.org/dpv/owl#isNotApplicableFor>
  a owl:ObjectProperty ;
  ns2:rangeIncludes <https://w3id.org/dpv/owl#Scope> ;
  dc:contributor _:genid4, _:genid5, _:genid1, _:genid6 ;
  dc:created "2024-04-13"^^xsd:date ;
  ns1:term_status "accepted"@en ;
  skos:definition "Indicates the concept or information is not applicable for specified context"@en ;
  skos:prefLabel "is not applicable for"@en ;
  ns0:rangeIncludes <https://w3id.org/dpv/owl#Scope> ;
  owl:sameAs <https://w3id.org/dpv#isNotApplicableFor>, <https://w3id.org/dpv/dpv-owl#isNotApplicableFor> .

<https://w3id.org/dpv/owl#Rule>
  a owl:Class ;
  dc:contributor _:genid4, _:genid5, _:genid1, _:genid6 ;
  dc:created "2022-10-19"^^xsd:date ;
  ns3:example <https://w3id.org/dpv/examples/owl#E0030> ;
  ns1:term_status "accepted"@en ;
  skos:definition "A rule describing a process or control that directs or determines if and how an activity should be conducted"@en ;
  skos:prefLabel "Rule"@en ;
  owl:sameAs <https://w3id.org/dpv#Rule>, <https://w3id.org/dpv/dpv-owl#Rule> .

<https://w3id.org/dpv/owl#MultiNationalScale>
  a owl:Class, owl:NamedIndividual, <https://w3id.org/dpv/owl#GeographicCoverage> ;
  rdfs:subClassOf <https://w3id.org/dpv/owl#GeographicCoverage> ;
  dc:contributor _:genid1 ;
  dc:created "2022-06-15"^^xsd:date ;
  ns1:term_status "accepted"@en ;
  skos:definition "Geographic coverage spanning multiple nations"@en ;
  skos:prefLabel "Multi National Scale"@en ;
  owl:sameAs <https://w3id.org/dpv#MultiNationalScale>, <https://w3id.org/dpv/dpv-owl#MultiNationalScale> .

odrl:or
  a owl:ObjectProperty, owl:NamedIndividual, skos:Concept ;
  rdfs:subPropertyOf odrl:operand ;
  rdfs:isDefinedBy odrl: ;
  rdfs:label "Or"@en ;
  skos:definition "The relation is satisfied when at least one of the Constraints is satisfied."@en ;
  skos:note "This property MUST only be used for Logical Constraints, and the list of operand values MUST be Constraint instances."@en .

<https://w3id.org/dpv/owl#ContractualClauseFulfiled>
  a owl:Class, owl:NamedIndividual, <https://w3id.org/dpv/owl#ContractualClauseFulfilmentStatus> ;
  rdfs:subClassOf <https://w3id.org/dpv/owl#ContractualClauseFulfilmentStatus> ;
  dc:created "2024-08-27"^^xsd:date ;
  ns1:term_status "accepted"@en ;
  skos:definition "Status indicating the terms of the contractual clause are fulfiled i.e. they have been succesfully completed without violation"@en ;
  skos:prefLabel "Contractual Clause Fulfiled"@en ;
  owl:sameAs <https://w3id.org/dpv#ContractualClauseFulfiled>, <https://w3id.org/dpv/dpv-owl#ContractualClauseFulfiled> .

<https://w3id.org/dpv/owl#hasConsequenceOn>
  a owl:ObjectProperty ;
  ns2:domainIncludes <https://w3id.org/dpv/owl#Consequence> ;
  dc:contributor _:genid4, _:genid1 ;
  dc:created "2022-11-24"^^xsd:date ;
  ns1:term_status "accepted"@en ;
  skos:definition "Indicates the thing (e.g. plan, process, or entity) affected by a consequence"@en ;
  skos:prefLabel "has consequence on"@en ;
  ns0:domainIncludes <https://w3id.org/dpv/owl#Consequence> ;
  owl:sameAs <https://w3id.org/dpv#hasConsequenceOn>, <https://w3id.org/dpv/dpv-owl#hasConsequenceOn> .

<https://w3id.org/dpv/owl#hasOutcome>
  a owl:ObjectProperty ;
  dc:contributor _:genid1 ;
  dc:created "2022-05-18"^^xsd:date ;
  ns1:term_status "accepted"@en ;
  skos:definition "Indicates an outcome of specified concept or context"@en ;
  skos:prefLabel "has outcome"@en ;
  owl:sameAs <https://w3id.org/dpv#hasOutcome>, <https://w3id.org/dpv/dpv-owl#hasOutcome> .

<https://w3id.org/dpv/owl#hasStorageCondition>
  a owl:ObjectProperty ;
  rdfs:subPropertyOf <https://w3id.org/dpv/owl#hasProcessingCondition> ;
  ns2:rangeIncludes <https://w3id.org/dpv/owl#StorageCondition> ;
  dc:contributor _:genid9, _:genid10, _:genid1, _:genid11 ;
  dc:created "2022-08-13"^^xsd:date ;
  dc:source [
    a ns0:WebPage ;
    ns0:name "SPECIAL Project" ;
    ns0:url "https://specialprivacy.ercim.eu/"
  ] ;
  ns1:term_status "accepted"@en ;
  skos:definition "Indicates information about storage condition"@en ;
  skos:prefLabel "has storage condition"@en ;
  ns0:rangeIncludes <https://w3id.org/dpv/owl#StorageCondition> ;
  owl:sameAs <https://w3id.org/dpv#hasStorageCondition>, <https://w3id.org/dpv/dpv-owl#hasStorageCondition> .

<https://w3id.org/dpv/owl#hasCountry>
  a owl:ObjectProperty ;
  rdfs:subPropertyOf <https://w3id.org/dpv/owl#hasLocation> ;
  ns2:rangeIncludes <https://w3id.org/dpv/owl#Country> ;
  dc:contributor _:genid4, _:genid1 ;
  dc:created "2022-01-19"^^xsd:date ;
  ns1:term_status "accepted"@en ;
  skos:definition "Indicates applicability of specified country"@en ;
  skos:prefLabel "has country"@en ;
  ns0:rangeIncludes <https://w3id.org/dpv/owl#Country> ;
  owl:sameAs <https://w3id.org/dpv#hasCountry>, <https://w3id.org/dpv/dpv-owl#hasCountry> .

<https://w3id.org/dpv/owl#DataBreachRecord>
  a owl:Class, owl:NamedIndividual, <https://w3id.org/dpv/owl#OrganisationalMeasure> ;
  rdfs:subClassOf <https://w3id.org/dpv/owl#RecordsOfActivities> ;
  dc:contributor _:genid1 ;
  dc:created "2024-04-14"^^xsd:date ;
  ns1:term_status "accepted"@en ;
  skos:definition "Record of a data breach incident"@en ;
  skos:prefLabel "Data Breach Record"@en ;
  owl:sameAs <https://w3id.org/dpv#DataBreachRecord>, <https://w3id.org/dpv/dpv-owl#DataBreachRecord> .

<https://w3id.org/dpv/owl#RecruitmentAdvertising>
  a owl:Class, owl:NamedIndividual, <https://w3id.org/dpv/owl#Purpose> ;
  rdfs:subClassOf <https://w3id.org/dpv/owl#Advertising>, <https://w3id.org/dpv/owl#PersonnelHiring> ;
  dc:created "2024-12-01"^^xsd:date ;
  ns1:term_status "accepted"@en ;
  skos:definition "Purposes associated with advertisement for Recruitments and personnel hiring"@en ;
  skos:prefLabel "Recruitment Advertising"@en ;
  owl:sameAs <https://w3id.org/dpv#RecruitmentAdvertising>, <https://w3id.org/dpv/dpv-owl#RecruitmentAdvertising> .

<https://w3id.org/dpv/owl#ContractTerminationClause>
  a owl:Class, owl:NamedIndividual, <https://w3id.org/dpv/owl#ContractualClause> ;
  rdfs:subClassOf <https://w3id.org/dpv/owl#ContractualClause> ;
  dc:created "2024-08-27"^^xsd:date ;
  ns1:term_status "accepted"@en ;
  skos:definition "A provision outlining the conditions under which the contract can be terminated before its completion, including any penalties or obligations"@en ;
  skos:prefLabel "Contract Termination Clause"@en ;
  owl:sameAs <https://w3id.org/dpv#ContractTerminationClause>, <https://w3id.org/dpv/dpv-owl#ContractTerminationClause> .

<https://w3id.org/dpv/owl#ReversingProcessInput>
  a owl:Class, owl:NamedIndividual, <https://w3id.org/dpv/owl#EntityPermissiveInvolvement> ;
  rdfs:subClassOf <https://w3id.org/dpv/owl#EntityPermissiveInvolvement> ;
  dc:contributor _:genid1, _:genid25, _:genid19 ;
  dc:created "2024-05-11"^^xsd:date ;
  ns1:term_status "accepted"@en ;
  skos:definition "Involvement where entity can reverse input of specified context"@en ;
  skos:prefLabel "Reversing Process Input"@en ;
  skos:scopeNote "Reversion can be considered a form of correction in some instances. We welcome inputs to further explore and define this relation between correction and reversion concepts."@en ;
  owl:sameAs <https://w3id.org/dpv#ReversingProcessInput>, <https://w3id.org/dpv/dpv-owl#ReversingProcessInput> .

<https://w3id.org/dpv/owl#SensitivePersonalData>
  a owl:Class ;
  rdfs:subClassOf <https://w3id.org/dpv/owl#PersonalData>, <https://w3id.org/dpv/owl#SensitiveData> ;
  dc:contributor _:genid1 ;
  dc:created "2022-01-19"^^xsd:date ;
  ns3:example <https://w3id.org/dpv/examples/owl#E0010>, <https://w3id.org/dpv/examples/owl#E0045> ;
  ns1:term_status "accepted"@en ;
  skos:definition "Personal data that is considered 'sensitive' in terms of privacy and/or impact, and therefore requires additional considerations and/or protection"@en ;
  skos:prefLabel "Sensitive Personal Data"@en ;
  skos:scopeNote "Sensitivity' is a matter of context, and may be defined within legal frameworks. For GDPR, Special categories of personal data are considered a subset of sensitive data. To illustrate the difference between the two, consider the situation where Location data is collected, and which is considered 'sensitive' but not 'special'. As a probable rule, sensitive data require additional considerations whereas special category data requires additional legal basis / justifications."@en ;
  owl:sameAs <https://w3id.org/dpv#SensitivePersonalData>, <https://w3id.org/dpv/dpv-owl#SensitivePersonalData> .

<https://w3id.org/dpv/owl#PublicInterestCompleted>
  a owl:Class, owl:NamedIndividual, <https://w3id.org/dpv/owl#PublicInterestStatus> ;
  rdfs:subClassOf <https://w3id.org/dpv/owl#PublicInterestStatus> ;
  dc:created "2024-08-27"^^xsd:date ;
  ns1:term_status "accepted"@en ;
  skos:definition "Status where the public interest activity has been completed"@en ;
  skos:prefLabel "Public Interest Completed"@en ;
  owl:sameAs <https://w3id.org/dpv#PublicInterestCompleted>, <https://w3id.org/dpv/dpv-owl#PublicInterestCompleted> .

odrl:lteq
  a owl:NamedIndividual, skos:Concept, odrl:Operator ;
  rdfs:isDefinedBy odrl: ;
  rdfs:label "Less than or equal to"@en ;
  skos:definition "Indicating that a given value is less than or equal to the right operand of the Constraint."@en .

<https://w3id.org/dpv/owl#Generate>
  a owl:Class, owl:NamedIndividual, <https://w3id.org/dpv/owl#Processing> ;
  rdfs:subClassOf <https://w3id.org/dpv/owl#Obtain> ;
  dc:contributor _:genid1 ;
  dc:created "2022-04-20"^^xsd:date ;
  ns1:term_status "accepted"@en ;
  skos:definition "to generate or create data"@en ;
  skos:prefLabel "Generate Data"@en ;
  owl:sameAs <https://w3id.org/dpv#Generate>, <https://w3id.org/dpv/dpv-owl#Generate> .

<https://w3id.org/dpv/owl#RequestRequiredActionPerformed>
  a owl:Class, owl:NamedIndividual, <https://w3id.org/dpv/owl#RequestStatus> ;
  rdfs:subClassOf <https://w3id.org/dpv/owl#RequestStatus> ;
  dc:contributor _:genid1 ;
  dc:created "2022-11-30"^^xsd:date ;
  ns1:term_status "accepted"@en ;
  skos:definition "State of a request's required action having been performed by the other party"@en ;
  skos:prefLabel "Request Required Action Performed"@en ;
  owl:sameAs <https://w3id.org/dpv#RequestRequiredActionPerformed>, <https://w3id.org/dpv/dpv-owl#RequestRequiredActionPerformed> .

odrl:leftOperand
  a owl:ObjectProperty, owl:NamedIndividual, skos:Concept ;
  rdfs:domain odrl:Constraint ;
  rdfs:range odrl:LeftOperand ;
  rdfs:isDefinedBy odrl: ;
  rdfs:label "Has Left Operand"@en ;
  skos:definition "The left operand in a constraint expression."@en .

<https://w3id.org/dpv/owl#DataTransferLegalBasis>
  a owl:Class, owl:NamedIndividual, <https://w3id.org/dpv/owl#LegalBasis> ;
  rdfs:subClassOf <https://w3id.org/dpv/owl#LegalBasis> ;
  dc:contributor _:genid4, _:genid21 ;
  dc:created "2021-09-08"^^xsd:date ;
  ns1:term_status "accepted"@en ;
  skos:definition "Specific or special categories and instances of legal basis intended for justifying data transfers"@en ;
  skos:prefLabel "Data Transfer Legal Basis"@en ;
  owl:sameAs <https://w3id.org/dpv#DataTransferLegalBasis>, <https://w3id.org/dpv/dpv-owl#DataTransferLegalBasis> .

<https://w3id.org/dpv/owl#StandardFormContract>
  a owl:Class, owl:NamedIndividual, <https://w3id.org/dpv/owl#LegalBasis> ;
  rdfs:subClassOf <https://w3id.org/dpv/owl#ContractByNegotiationType> ;
  dc:created "2024-08-27"^^xsd:date ;
  ns1:term_status "accepted"@en ;
  skos:definition "A contract where the terms and conditions are determined by one or more of the parties, and the other parties have negligible or no ability to negotiate the terms and conditions"@en ;
  skos:prefLabel "Standard Form Contract"@en ;
  skos:scopeNote "Such a contract results in the unempowered parties being in a \"take it or leave it\" position as they can only accept or reject the contract. Standard form contracts are also known as \"Adhesion contract\" or \"Boilerplate contract\""@en ;
  owl:sameAs <https://w3id.org/dpv#StandardFormContract>, <https://w3id.org/dpv/dpv-owl#StandardFormContract> .

<https://w3id.org/dpv/owl#AcademicScientificOrganisation>
  a owl:Class ;
  rdfs:subClassOf <https://w3id.org/dpv/owl#Organisation> ;
  dc:contributor _:genid1 ;
  dc:created "2022-02-02"^^xsd:date ;
  dc:modified "2020-10-05"^^xsd:date ;
  dc:source [
    a ns0:WebPage ;
    ns0:name "ADMS controlled vocabulary" ;
    ns0:url "http://purl.org/adms"
  ] ;
  ns1:term_status "accepted"@en ;
  skos:definition "Organisations related to academia or scientific pursuits e.g. Universities, Schools, Research Bodies"@en ;
  skos:prefLabel "Academic or Scientific Organisation"@en ;
  owl:sameAs <https://w3id.org/dpv#AcademicScientificOrganisation>, <https://w3id.org/dpv/dpv-owl#AcademicScientificOrganisation> .

<https://w3id.org/dpv/owl#DataJurisdictionPolicy>
  a owl:Class, owl:NamedIndividual, <https://w3id.org/dpv/owl#OrganisationalMeasure> ;
  rdfs:subClassOf <https://w3id.org/dpv/owl#DataProcessingPolicy> ;
  dc:contributor _:genid1 ;
  dc:created "2024-04-14"^^xsd:date ;
  ns1:term_status "accepted"@en ;
  skos:definition "Policy specifying jurisdictional requirements for data processing"@en ;
  skos:prefLabel "Data Jurisdiction Policy"@en ;
  skos:scopeNote "Jurisdictional requirements can refer to data being stored within specific jurisdictions, or that data must be in line with jurisdictional laws and norms"@en ;
  owl:sameAs <https://w3id.org/dpv#DataJurisdictionPolicy>, <https://w3id.org/dpv/dpv-owl#DataJurisdictionPolicy> .

odrl:#constraintRightOpCommon
  a owl:NamedIndividual, skos:Collection ;
  skos:member odrl:policyUsage ;
  skos:prefLabel "Constraint Right Operands"@en ;
  skos:scopeNote "ODRL Common Vocabulary Terms"@en .

<https://w3id.org/dpv/owl#JudicialOrganisation>
  a owl:Class ;
  rdfs:subClassOf <https://w3id.org/dpv/owl#Organisation> ;
  dc:contributor _:genid25 ;
  dc:created "2024-12-01"^^xsd:date ;
  ns1:term_status "accepted"@en ;
  skos:definition "An organisation involved in interpreting and applying the law, resolving disputes, and administering justice as part of the judicial system"@en ;
  skos:prefLabel "Judicial Organisation"@en ;
  owl:sameAs <https://w3id.org/dpv#JudicialOrganisation>, <https://w3id.org/dpv/dpv-owl#JudicialOrganisation> .

odrl:rightOperand
  a owl:ObjectProperty, owl:DatatypeProperty, owl:NamedIndividual, skos:Concept ;
  rdfs:domain odrl:Constraint ;
  rdfs:range [
    a owl:Class ;
    owl:unionOf (
     rdfs:Literal
     xsd:anyURI
     odrl:RightOperand
   )
  ] ;
  rdfs:isDefinedBy odrl: ;
  rdfs:label "Has Right Operand"@en ;
  skos:definition "The value of the right operand in a constraint expression."@en ;
  skos:note "When used with set-based operators, a list of values may be used."@en .

<https://w3id.org/dpv/owl#Reformat>
  a owl:Class, owl:NamedIndividual, <https://w3id.org/dpv/owl#Processing> ;
  rdfs:subClassOf <https://w3id.org/dpv/owl#Format> ;
  dc:contributor _:genid5 ;
  dc:created "2024-04-14"^^xsd:date ;
  dc:source "DGA 12.d"@en ;
  ns1:term_status "accepted"@en ;
  skos:definition "to rearrange or restructure data to change its form"@en ;
  skos:prefLabel "Reformat Data"@en ;
  owl:sameAs <https://w3id.org/dpv#Reformat>, <https://w3id.org/dpv/dpv-owl#Reformat> .

<https://w3id.org/dpv/owl#SymmetricEncryption>
  a owl:Class, owl:NamedIndividual, <https://w3id.org/dpv/owl#TechnicalMeasure> ;
  rdfs:subClassOf <https://w3id.org/dpv/owl#Encryption> ;
  dc:contributor _:genid1 ;
  dc:created "2022-08-17"^^xsd:date ;
  dc:source [
    a ns0:WebPage ;
    ns0:name "ENISA Data Pseudonymisation: Advanced Techniques and Use Cases" ;
    ns0:url "https://www.enisa.europa.eu/publications/data-pseudonymisation-advanced-techniques-and-use-cases"
  ] ;
  ns1:term_status "accepted"@en ;
  skos:definition "Use of symmetric cryptography to encrypt data"@en ;
  skos:prefLabel "Symmetric Encryption"@en ;
  owl:sameAs <https://w3id.org/dpv#SymmetricEncryption>, <https://w3id.org/dpv/dpv-owl#SymmetricEncryption> .

<https://w3id.org/dpv/owl#NonPublicDataSource>
  a owl:Class, owl:NamedIndividual, <https://w3id.org/dpv/owl#DataSource> ;
  rdfs:subClassOf <https://w3id.org/dpv/owl#DataSource> ;
  dc:contributor _:genid4, _:genid5, _:genid1, _:genid17, _:genid6 ;
  dc:created "2022-01-26"^^xsd:date ;
  ns1:term_status "accepted"@en ;
  skos:definition "A source of data that is not publicly accessible or available"@en ;
  skos:prefLabel "Non-Public Data Source"@en ;
  owl:sameAs <https://w3id.org/dpv#NonPublicDataSource>, <https://w3id.org/dpv/dpv-owl#NonPublicDataSource> .

<https://w3id.org/dpv/owl#Customer>
  a owl:Class, owl:NamedIndividual, <https://w3id.org/dpv/owl#HumanSubject> ;
  rdfs:subClassOf <https://w3id.org/dpv/owl#HumanSubject> ;
  dc:contributor _:genid4, _:genid5, _:genid1, _:genid17, _:genid6 ;
  dc:created "2022-04-06"^^xsd:date ;
  dc:modified "2024-12-17"^^xsd:date ;
  ns1:term_status "modified"@en ;
  skos:definition "Humans that purchase goods or services"@en ;
  skos:prefLabel "Customer"@en ;
  skos:scopeNote "note: for B2B relations where customers are organisations, this concept only applies for data subjects"@en ;
  owl:sameAs <https://w3id.org/dpv#Customer>, <https://w3id.org/dpv/dpv-owl#Customer> .

<https://w3id.org/dpv/owl#Consultation>
  a owl:Class, owl:NamedIndividual, <https://w3id.org/dpv/owl#OrganisationalMeasure> ;
  rdfs:subClassOf <https://w3id.org/dpv/owl#OrganisationalMeasure> ;
  dc:contributor _:genid4, _:genid1, _:genid6 ;
  dc:created "2020-11-04"^^xsd:date ;
  ns1:term_status "accepted"@en ;
  skos:definition "Consultation is a process of receiving feedback, advice, or opinion from an external agency"@en ;
  skos:prefLabel "Consultation"@en ;
  owl:sameAs <https://w3id.org/dpv#Consultation>, <https://w3id.org/dpv/dpv-owl#Consultation> .

<https://w3id.org/dpv/owl#DecisionMaking>
  a owl:Class ;
  rdfs:subClassOf <https://w3id.org/dpv/owl#ProcessingContext> ;
  dc:contributor _:genid1 ;
  dc:created "2022-09-07"^^xsd:date ;
  ns1:term_status "accepted"@en ;
  skos:definition "Processing that involves decision making"@en ;
  skos:prefLabel "Decision Making"@en ;
  owl:sameAs <https://w3id.org/dpv#DecisionMaking>, <https://w3id.org/dpv/dpv-owl#DecisionMaking> .

<https://w3id.org/dpv/owl#DeliveryOfGoods>
  a owl:Class, owl:NamedIndividual, <https://w3id.org/dpv/owl#Purpose> ;
  rdfs:subClassOf <https://w3id.org/dpv/owl#RequestedServiceProvision> ;
  dc:contributor _:genid13, _:genid14, _:genid1, _:genid15, _:genid16, _:genid11 ;
  dc:created "2019-04-05"^^xsd:date ;
  ns1:term_status "accepted"@en ;
  skos:definition "Purposes associated with delivering goods and services requested or asked by consumer"@en ;
  skos:prefLabel "Delivery of Goods"@en ;
  skos:related <https://specialprivacy.ercim.eu/vocabs/purposes#Delivery> ;
  owl:sameAs <https://w3id.org/dpv#DeliveryOfGoods>, <https://w3id.org/dpv/dpv-owl#DeliveryOfGoods> .

<https://w3id.org/dpv/owl#NoticeUsed>
  a owl:Class, owl:NamedIndividual, <https://w3id.org/dpv/owl#NoticeStatus> ;
  rdfs:subClassOf <https://w3id.org/dpv/owl#NoticeStatus> ;
  dc:contributor _:genid4, _:genid1 ;
  dc:created "2024-12-01"^^xsd:date ;
  ns1:term_status "accepted"@en ;
  skos:definition "Status indicating the notice has been communicated and has been used e.g. the recipient has acknowledged it or taken the intended action"@en ;
  skos:prefLabel "Notice Used"@en ;
  owl:sameAs <https://w3id.org/dpv#NoticeUsed>, <https://w3id.org/dpv/dpv-owl#NoticeUsed> .

<https://w3id.org/dpv/owl#SellProducts>
  a owl:Class, owl:NamedIndividual, <https://w3id.org/dpv/owl#Purpose> ;
  rdfs:subClassOf <https://w3id.org/dpv/owl#ServiceProvision> ;
  dc:contributor _:genid4, _:genid5, _:genid1 ;
  dc:created "2021-09-08"^^xsd:date ;
  ns1:term_status "accepted"@en ;
  skos:definition "Purposes associated with selling products or services"@en ;
  skos:prefLabel "Sell Products"@en ;
  skos:scopeNote "Sell here means exchange, submit, or provide in return for direct or indirect compensation."@en ;
  owl:sameAs <https://w3id.org/dpv#SellProducts>, <https://w3id.org/dpv/dpv-owl#SellProducts> .

<https://w3id.org/dpv/owl#DataHandlingClause>
  a owl:Class, owl:NamedIndividual, <https://w3id.org/dpv/owl#LegalMeasure> ;
  rdfs:subClassOf <https://w3id.org/dpv/owl#ContractualTerms> ;
  dc:created "2024-08-27"^^xsd:date ;
  ns1:term_status "accepted"@en ;
  skos:definition "Conctractual clauses governing handling of data within or by an entity"@en ;
  skos:prefLabel "Data Handling Clause"@en ;
  owl:sameAs <https://w3id.org/dpv#DataHandlingClause>, <https://w3id.org/dpv/dpv-owl#DataHandlingClause> .

<https://w3id.org/dpv/owl#hasRepresentative>
  a owl:ObjectProperty ;
  rdfs:subPropertyOf <https://w3id.org/dpv/owl#hasEntity> ;
  ns2:domainIncludes <https://w3id.org/dpv/owl#Entity> ;
  ns2:rangeIncludes <https://w3id.org/dpv/owl#Representative> ;
  dc:contributor _:genid4, _:genid5, _:genid1, _:genid6 ;
  dc:created "2020-11-04"^^xsd:date ;
  ns1:term_status "accepted"@en ;
  skos:definition "Specifies representative of the legal entity"@en ;
  skos:prefLabel "has representative"@en ;
  ns0:domainIncludes <https://w3id.org/dpv/owl#Entity> ;
  ns0:rangeIncludes <https://w3id.org/dpv/owl#Representative> ;
  owl:sameAs <https://w3id.org/dpv#hasRepresentative>, <https://w3id.org/dpv/dpv-owl#hasRepresentative> .

<https://w3id.org/dpv/owl#VitalInterestOngoing>
  a owl:Class, owl:NamedIndividual, <https://w3id.org/dpv/owl#VitalInterestStatus> ;
  rdfs:subClassOf <https://w3id.org/dpv/owl#VitalInterestStatus> ;
  dc:created "2024-08-27"^^xsd:date ;
  ns1:term_status "accepted"@en ;
  skos:definition "Status where the vital interest activity is ongoing"@en ;
  skos:prefLabel "Vital Interest Ongoing"@en ;
  owl:sameAs <https://w3id.org/dpv#VitalInterestOngoing>, <https://w3id.org/dpv/dpv-owl#VitalInterestOngoing> .

<https://w3id.org/dpv/owl#DataSource>
  a owl:Class ;
  rdfs:subClassOf <https://w3id.org/dpv/owl#ProcessingContext> ;
  dc:contributor _:genid4, _:genid5, _:genid1 ;
  dc:created "2020-11-04"^^xsd:date ;
  ns3:example <https://w3id.org/dpv/examples/owl#E0012> ;
  ns1:term_status "accepted"@en ;
  skos:definition "The source or origin of data"@en ;
  skos:prefLabel "Data Source"@en ;
  skos:scopeNote "Source' is the direct point of data collection; 'origin' would indicate the original/others points of where the data originates from."@en ;
  owl:sameAs <https://w3id.org/dpv#DataSource>, <https://w3id.org/dpv/dpv-owl#DataSource> .

<https://w3id.org/dpv/owl#InternalResourceOptimisation>
  a owl:Class, owl:NamedIndividual, <https://w3id.org/dpv/owl#Purpose> ;
  rdfs:subClassOf <https://w3id.org/dpv/owl#OptimisationForController> ;
  dc:contributor _:genid13, _:genid14, _:genid1, _:genid15, _:genid16, _:genid11 ;
  dc:created "2019-04-05"^^xsd:date ;
  ns1:term_status "accepted"@en ;
  skos:definition "Purposes associated with optimisation of internal resource availability and usage for organisation"@en ;
  skos:prefLabel "Internal Resource Optimisation"@en ;
  owl:sameAs <https://w3id.org/dpv#InternalResourceOptimisation>, <https://w3id.org/dpv/dpv-owl#InternalResourceOptimisation> .

<https://w3id.org/dpv/owl#CustomerSolvencyMonitoring>
  a owl:Class, owl:NamedIndividual, <https://w3id.org/dpv/owl#Purpose> ;
  rdfs:subClassOf <https://w3id.org/dpv/owl#CustomerManagement> ;
  dc:contributor _:genid4, _:genid5, _:genid1 ;
  dc:created "2021-09-08"^^xsd:date ;
  dc:source [
    a ns0:WebPage ;
    ns0:name "Belgian DPA ROPA Template" ;
    ns0:url "https://www.privacycommission.be/nl/model-voor-een-register-van-de-verwerkingsactiviteiten"
  ] ;
  ns1:term_status "accepted"@en ;
  skos:definition "Customer Solvency Monitoring refers to purposes associated with monitor solvency of customers for financial diligence"@en ;
  skos:prefLabel "Customer Solvency Monitoring"@en ;
  owl:sameAs <https://w3id.org/dpv#CustomerSolvencyMonitoring>, <https://w3id.org/dpv/dpv-owl#CustomerSolvencyMonitoring> .

<https://w3id.org/dpv/owl#ProcessingLocation>
  a owl:Class ;
  rdfs:subClassOf <https://w3id.org/dpv/owl#Location>, <https://w3id.org/dpv/owl#ProcessingCondition> ;
  dc:created "2023-12-10"^^xsd:date ;
  dc:modified "2024-05-11"^^xsd:date ;
  ns3:example <https://w3id.org/dpv/examples/owl#E0047> ;
  ns1:term_status "accepted"@en ;
  skos:definition "Conditions regarding location or geospatial scope where processing takes places"@en ;
  skos:prefLabel "Processing Location"@en ;
  owl:sameAs <https://w3id.org/dpv#ProcessingLocation>, <https://w3id.org/dpv/dpv-owl#ProcessingLocation> .

odrl:execute
  a owl:NamedIndividual, skos:Concept, odrl:Action ;
  odrl:includedIn odrl:use ;
  rdfs:isDefinedBy odrl: ;
  rdfs:label "Execute"@en ;
  skos:definition "To run the computer program Asset."@en ;
  skos:note "For example, machine executable code or Java such as a game or application."@en ;
  skos:scopeNote "Non-Normative"@en .

<https://w3id.org/dpv/owl#ConsentManagement>
  a owl:Class, owl:NamedIndividual, <https://w3id.org/dpv/owl#OrganisationalMeasure> ;
  rdfs:subClassOf <https://w3id.org/dpv/owl#PermissionManagement> ;
  dc:contributor _:genid4, _:genid5, _:genid1 ;
  dc:created "2024-04-14"^^xsd:date ;
  dc:source "DGA 12.n"@en ;
  ns1:term_status "accepted"@en ;
  skos:definition "Methods to obtain, provide, modify, and withdraw consent along with maintaining a record of consent, retrieving records, and processing changes in consent states"@en ;
  skos:prefLabel "Consent Management"@en ;
  owl:sameAs <https://w3id.org/dpv#ConsentManagement>, <https://w3id.org/dpv/dpv-owl#ConsentManagement> .

<https://w3id.org/dpv/owl#ServiceProvider>
  a owl:Class ;
  rdfs:subClassOf <https://w3id.org/dpv/owl#LegalEntity> ;
  dc:contributor _:genid1 ;
  dc:created "2024-04-20"^^xsd:date ;
  ns1:term_status "accepted"@en ;
  skos:definition "The entity that provides a service"@en ;
  skos:prefLabel "Service Provider"@en ;
  owl:sameAs <https://w3id.org/dpv#ServiceProvider>, <https://w3id.org/dpv/dpv-owl#ServiceProvider> .

<https://w3id.org/dpv/owl#HardwareSecurityProtocols>
  a owl:Class, owl:NamedIndividual, <https://w3id.org/dpv/owl#TechnicalMeasure> ;
  rdfs:subClassOf <https://w3id.org/dpv/owl#SecurityMethod> ;
  dc:contributor _:genid1 ;
  dc:created "2022-08-17"^^xsd:date ;
  dc:source [
    a ns0:WebPage ;
    ns0:name "ENISA Reference Incident Classification Taxonomy 2018" ;
    ns0:url "https://www.enisa.europa.eu/publications/reference-incident-classification-taxonomy/"
  ] ;
  ns1:term_status "accepted"@en ;
  skos:definition "Security protocols implemented at or within hardware"@en ;
  skos:prefLabel "Hardware Security Protocols"@en ;
  owl:sameAs <https://w3id.org/dpv#HardwareSecurityProtocols>, <https://w3id.org/dpv/dpv-owl#HardwareSecurityProtocols> .

<https://w3id.org/dpv/owl#Lawfulness>
  a owl:Class ;
  rdfs:subClassOf <https://w3id.org/dpv/owl#ComplianceStatus> ;
  dc:contributor _:genid1 ;
  dc:created "2022-10-19"^^xsd:date ;
  ns1:term_status "accepted"@en ;
  skos:definition "Status associated with expressing lawfulness or legal compliance"@en ;
  skos:prefLabel "Lawfulness"@en ;
  owl:sameAs <https://w3id.org/dpv#Lawfulness>, <https://w3id.org/dpv/dpv-owl#Lawfulness> .

<https://w3id.org/dpv/owl#Assess>
  a owl:Class, owl:NamedIndividual, <https://w3id.org/dpv/owl#Processing> ;
  rdfs:subClassOf <https://w3id.org/dpv/owl#Use> ;
  dc:contributor _:genid4, _:genid1 ;
  dc:created "2022-06-15"^^xsd:date ;
  ns1:term_status "accepted"@en ;
  skos:definition "to assess data for some criteria"@en ;
  skos:prefLabel "Assess Data"@en ;
  owl:sameAs <https://w3id.org/dpv#Assess>, <https://w3id.org/dpv/dpv-owl#Assess> .

<https://w3id.org/dpv/owl#Notice>
  a owl:Class, owl:NamedIndividual, <https://w3id.org/dpv/owl#OrganisationalMeasure> ;
  rdfs:subClassOf <https://w3id.org/dpv/owl#OrganisationalMeasure> ;
  dc:contributor _:genid4, _:genid1, _:genid6, _:genid21 ;
  dc:created "2021-09-08"^^xsd:date ;
  ns3:example <https://w3id.org/dpv/examples/owl#E0017> ;
  ns1:term_status "accepted"@en ;
  skos:definition "A notice is an artefact for providing information, choices, or controls"@en ;
  skos:prefLabel "Notice"@en ;
  skos:scopeNote "Notice refers to the information whereas Notification refers to the provision of that notice. In several cases, they are used interchangeably - for example Privacy Notice as a measure or control refers to both the information as well as the act of making it available. For 'active' contexts where this distinction is important, e.g. data breach notifications, see Notification concept."@en ;
  owl:sameAs <https://w3id.org/dpv#Notice>, <https://w3id.org/dpv/dpv-owl#Notice> .

<https://w3id.org/dpv/owl#hasConsentStatus>
  a owl:ObjectProperty ;
  ns2:rangeIncludes <https://w3id.org/dpv/owl#ConsentStatus> ;
  dc:contributor _:genid4, _:genid1, _:genid17, _:genid6 ;
  dc:created "2022-06-21"^^xsd:date ;
  ns1:term_status "accepted"@en ;
  skos:definition "Specifies the state or status of consent"@en ;
  skos:prefLabel "has consent status"@en ;
  ns0:rangeIncludes <https://w3id.org/dpv/owl#ConsentStatus> ;
  owl:sameAs <https://w3id.org/dpv#hasConsentStatus>, <https://w3id.org/dpv/dpv-owl#hasConsentStatus> .

<https://w3id.org/dpv/owl#ProcessingScale>
  a owl:Class ;
  rdfs:subClassOf <https://w3id.org/dpv/owl#Scale> ;
  dc:contributor _:genid1, _:genid2 ;
  dc:created "2022-09-07"^^xsd:date ;
  ns3:example <https://w3id.org/dpv/examples/owl#E0049> ;
  ns1:term_status "accepted"@en ;
  skos:definition "Scale of Processing"@en ;
  skos:prefLabel "Processing Scale"@en ;
  skos:scopeNote "The exact definition of what constitutes \"scale\" depends on use of jurisdictional, domain-specific, or other forms of externally defined criterias. Where possible, this should be reflected by extending the scales provided with the appropriate context."@en ;
  owl:sameAs <https://w3id.org/dpv#ProcessingScale>, <https://w3id.org/dpv/dpv-owl#ProcessingScale> .

<https://w3id.org/dpv/owl#CannotCorrectProcessOutput>
  a owl:Class, owl:NamedIndividual, <https://w3id.org/dpv/owl#EntityNonPermissiveInvolvement> ;
  rdfs:subClassOf <https://w3id.org/dpv/owl#EntityNonPermissiveInvolvement> ;
  dc:contributor _:genid1, _:genid25, _:genid19 ;
  dc:created "2024-05-11"^^xsd:date ;
  ns1:term_status "accepted"@en ;
  skos:definition "Involvement where entity cannot correct the output of specified context"@en ;
  skos:prefLabel "Cannot Correct Process Output"@en ;
  owl:sameAs <https://w3id.org/dpv#CannotCorrectProcessOutput>, <https://w3id.org/dpv/dpv-owl#CannotCorrectProcessOutput> .

<https://w3id.org/dpv/owl#FireDepartment>
  a owl:Class ;
  rdfs:subClassOf <https://w3id.org/dpv/owl#EmergencyServiceProvider> ;
  dc:contributor _:genid25 ;
  dc:created "2024-12-01"^^xsd:date ;
  ns1:term_status "accepted"@en ;
  skos:definition "An organisation that is an emergency service provider for fire prevention, firefighting, and rescue services"@en ;
  skos:prefLabel "Fire Department"@en ;
  owl:sameAs <https://w3id.org/dpv#FireDepartment>, <https://w3id.org/dpv/dpv-owl#FireDepartment> .

<https://w3id.org/dpv/owl#ActivityPlanned>
  a owl:Class, owl:NamedIndividual, <https://w3id.org/dpv/owl#ActivityStatus> ;
  rdfs:subClassOf <https://w3id.org/dpv/owl#ActivityStatus> ;
  dc:contributor _:genid1 ;
  dc:created "2024-05-19"^^xsd:date ;
  ns1:term_status "accepted"@en ;
  skos:definition "State of an activity being planned with concrete plans for implementation"@en ;
  skos:prefLabel "Activity Planned"@en ;
  owl:sameAs <https://w3id.org/dpv#ActivityPlanned>, <https://w3id.org/dpv/dpv-owl#ActivityPlanned> .

<https://w3id.org/dpv/owl#Likelihood>
  a owl:Class ;
  dc:contributor _:genid1 ;
  dc:created "2022-07-22"^^xsd:date ;
  ns3:example <https://w3id.org/dpv/examples/owl#E0068> ;
  ns1:term_status "accepted"@en ;
  skos:definition "The likelihood or probability or chance of something taking place or occuring"@en ;
  skos:prefLabel "Likelihood"@en ;
  skos:scopeNote "Likelihood can be expressed in a subjective manner, such as 'Unlikely', or in a quantitative manner such as \"Twice in a Day\" (frequency per period). The suggestion is to use quantitative values, or to associate them with subjective terms used so as to enable accurate interpretations and interoperability. See the concepts related to Frequency and Duration for possible uses as a combination to express Likelihood."@en ;
  owl:sameAs <https://w3id.org/dpv#Likelihood>, <https://w3id.org/dpv/dpv-owl#Likelihood> .

<https://w3id.org/dpv/owl#Pseudonymisation>
  a owl:Class, owl:NamedIndividual, <https://w3id.org/dpv/owl#TechnicalMeasure> ;
  rdfs:subClassOf <https://w3id.org/dpv/owl#Deidentification> ;
  dc:contributor _:genid64, _:genid9, _:genid10, _:genid1, _:genid11, _:genid68 ;
  dc:created "2019-04-05"^^xsd:date ;
  dc:modified "2022-11-24"^^xsd:date ;
  dc:source [
    a ns0:WebPage ;
    ns0:name "GDPR Art.4-5" ;
    ns0:url "https://eur-lex.europa.eu/eli/reg/2016/679/art_4/par_5/oj"
  ] ;
  ns1:term_status "accepted"@en ;
  skos:definition "Pseudonymisation means the processing of personal data in such a manner that the personal data can no longer be attributed to a specific data subject without the use of additional information, provided that such additional information is kept separately and is subject to technical and organisational measures to ensure that the personal data are not attributed to an identified or identifiable natural person;"@en ;
  skos:prefLabel "Pseudonymisation"@en ;
  owl:sameAs <https://w3id.org/dpv#Pseudonymisation>, <https://w3id.org/dpv/dpv-owl#Pseudonymisation> .

odrl:transfer
  a owl:NamedIndividual, skos:Concept, odrl:Action ;
  rdfs:isDefinedBy odrl: ;
  rdfs:label "Transfer Ownership"@en ;
  skos:definition "To transfer the ownership of the Asset in perpetuity."@en .

<https://w3id.org/dpv/owl#GeneratedPersonalData>
  a owl:Class ;
  rdfs:subClassOf <https://w3id.org/dpv/owl#PersonalData> ;
  dc:contributor _:genid1 ;
  dc:created "2022-03-30"^^xsd:date ;
  dc:modified "2023-12-10"^^xsd:date ;
  ns1:term_status "accepted"@en ;
  skos:definition "Personal Data that is generated or brought into existence without relation to existing data i.e. it is not derived or inferred from other data"@en ;
  skos:prefLabel "Generated Personal Data"@en ;
  skos:scopeNote "Generated Data is used to indicate data that is produced and is not derived or inferred from other data"@en ;
  owl:sameAs <https://w3id.org/dpv#GeneratedPersonalData>, <https://w3id.org/dpv/dpv-owl#GeneratedPersonalData> .

<https://w3id.org/dpv/owl#HumanInvolvementForDecision>
  a owl:Class, owl:NamedIndividual, <https://w3id.org/dpv/owl#HumanInvolvement> ;
  rdfs:subClassOf <https://w3id.org/dpv/owl#HumanInvolvement> ;
  dc:created "2022-09-06"^^xsd:date ;
  dc:modified "2023-12-10"^^xsd:date ;
  ns1:term_status "accepted"@en ;
  skos:definition "Human involvement for the purposes of exercising decisions over the specified operations in context"@en ;
  skos:prefLabel "Human Involvement for decision"@en ;
  skos:scopeNote "Decisions are about exercising control over the operation, and are distinct from input (data or parameters)."@en ;
  owl:sameAs <https://w3id.org/dpv#HumanInvolvementForDecision>, <https://w3id.org/dpv/dpv-owl#HumanInvolvementForDecision> .

<https://w3id.org/dpv/owl#DataSubjectDataSource>
  a owl:Class, owl:NamedIndividual, <https://w3id.org/dpv/owl#DataSource> ;
  rdfs:subClassOf <https://w3id.org/dpv/owl#DataSource> ;
  dc:created "2023-10-12"^^xsd:date ;
  ns1:term_status "accepted"@en ;
  skos:definition "Data Sourced from Data Subject(s), e.g. when data is collected via a form or observed from their activities"@en ;
  skos:prefLabel "Data Subject as Data Source"@en ;
  owl:sameAs <https://w3id.org/dpv#DataSubjectDataSource>, <https://w3id.org/dpv/dpv-owl#DataSubjectDataSource> .

<https://w3id.org/dpv/owl#PersonalDataHandling>
  a owl:Class ;
  rdfs:subClassOf <https://w3id.org/dpv/owl#Process> ;
  dc:contributor _:genid13, _:genid11 ;
  dc:created "2019-04-05"^^xsd:date ;
  dc:modified "2023-12-10"^^xsd:date ;
  ns1:term_status "sunset"@en ;
  skos:definition "An abstract concept describing 'personal data handling'"@en ;
  skos:prefLabel "Personal Data Handling"@en ;
  skos:scopeNote "This concept will be deprecated in future updates. It is recommended to use dpv:Process as the equivalent alternative which is better aligned with legal and operational terminology."@en ;
  owl:sameAs <https://w3id.org/dpv#PersonalDataHandling>, <https://w3id.org/dpv/dpv-owl#PersonalDataHandling> .

<https://w3id.org/dpv/owl#LegitimateInterestOfController>
  a owl:Class, owl:NamedIndividual, <https://w3id.org/dpv/owl#LegalBasis> ;
  rdfs:subClassOf <https://w3id.org/dpv/owl#LegitimateInterest> ;
  dc:contributor _:genid4, _:genid1, _:genid6 ;
  dc:created "2021-05-19"^^xsd:date ;
  ns3:example <https://w3id.org/dpv/examples/owl#E0065> ;
  ns1:term_status "accepted"@en ;
  skos:definition "Legitimate Interests of a Data Controller in conducting specified activities"@en ;
  skos:prefLabel "Legitimate Interest of Controller"@en ;
  owl:sameAs <https://w3id.org/dpv#LegitimateInterestOfController>, <https://w3id.org/dpv/dpv-owl#LegitimateInterestOfController> .

<https://w3id.org/dpv/owl#NonPersonalData>
  a owl:Class ;
  rdfs:subClassOf <https://w3id.org/dpv/owl#Data> ;
  dc:contributor _:genid1 ;
  dc:created "2022-01-19"^^xsd:date ;
  ns1:term_status "accepted"@en ;
  skos:definition "Data that is not Personal Data"@en ;
  skos:prefLabel "Non-Personal Data"@en ;
  skos:scopeNote "The term NonPersonalData is provided to distinguish between PersonalData and other data, e.g. for indicating which data is regulated by privacy laws. To specify personal data that has been anonymised, the concept AnonymisedData should be used as the anonymisation process has a risk of not being fully effective and such anonymous data may be found to be personal data depending on circumstances."@en ;
  owl:sameAs <https://w3id.org/dpv#NonPersonalData>, <https://w3id.org/dpv/dpv-owl#NonPersonalData> .

<https://w3id.org/dpv/owl#PrintedNotice>
  a owl:Class, owl:NamedIndividual, <https://w3id.org/dpv/owl#OrganisationalMeasure> ;
  rdfs:subClassOf <https://w3id.org/dpv/owl#Notice> ;
  dc:created "2024-08-17"^^xsd:date ;
  dc:source [
    a ns0:WebPage ;
    ns0:name "ICO - What methods can we use to provide privacy information?" ;
    ns0:url "https://ico.org.uk/for-organisations/uk-gdpr-guidance-and-resources/individual-rights/the-right-to-be-informed/what-methods-can-we-use-to-provide-privacy-information/"
  ] ;
  ns1:term_status "accepted"@en ;
  skos:definition "A notice that is provided in a printed form on or along with a device"@en ;
  skos:prefLabel "Printed Notice"@en ;
  owl:sameAs <https://w3id.org/dpv#PrintedNotice>, <https://w3id.org/dpv/dpv-owl#PrintedNotice> .

<https://w3id.org/dpv/owl#SporadicDataVolume>
  a owl:Class, owl:NamedIndividual, <https://w3id.org/dpv/owl#DataVolume> ;
  rdfs:subClassOf <https://w3id.org/dpv/owl#DataVolume> ;
  dc:contributor _:genid1 ;
  dc:created "2022-06-15"^^xsd:date ;
  ns1:term_status "accepted"@en ;
  skos:definition "Data volume that is considered sporadic or sparse within the context"@en ;
  skos:prefLabel "Sporadic Data Volume"@en ;
  owl:sameAs <https://w3id.org/dpv#SporadicDataVolume>, <https://w3id.org/dpv/dpv-owl#SporadicDataVolume> .

<https://w3id.org/dpv/owl#StartupOrganisation>
  a owl:Class ;
  rdfs:subClassOf <https://w3id.org/dpv/owl#LegalEntity> ;
  dc:contributor _:genid4 ;
  dc:created "2024-12-01"^^xsd:date ;
  ns1:term_status "accepted"@en ;
  skos:definition "An organisation that is newly established and is nascent in terms of available resources"@en ;
  skos:prefLabel "Startup Organisation"@en ;
  owl:sameAs <https://w3id.org/dpv#StartupOrganisation>, <https://w3id.org/dpv/dpv-owl#StartupOrganisation> .

<https://w3id.org/dpv/owl#OrganisationRiskManagement>
  a owl:Class, owl:NamedIndividual, <https://w3id.org/dpv/owl#Purpose> ;
  rdfs:subClassOf <https://w3id.org/dpv/owl#OrganisationGovernance> ;
  dc:contributor _:genid4, _:genid1, _:genid6, _:genid21 ;
  dc:created "2021-09-01"^^xsd:date ;
  ns1:term_status "accepted"@en ;
  skos:definition "Purposes associated with managing risk for organisation's activities"@en ;
  skos:prefLabel "Organisation Risk Management"@en ;
  owl:sameAs <https://w3id.org/dpv#OrganisationRiskManagement>, <https://w3id.org/dpv/dpv-owl#OrganisationRiskManagement> .

<https://w3id.org/dpv/owl#AuthorityUninformed>
  a owl:Class, owl:NamedIndividual, <https://w3id.org/dpv/owl#EntityInformedStatus> ;
  rdfs:subClassOf <https://w3id.org/dpv/owl#EntityUninformed> ;
  dc:contributor _:genid4, _:genid1, _:genid25, _:genid6 ;
  dc:created "2024-05-10"^^xsd:date ;
  ns1:term_status "accepted"@en ;
  skos:definition "Status indicating Authority is uninformed i.e. has not been informed about the specified context"@en ;
  skos:prefLabel "Authority Uninformed"@en ;
  owl:sameAs <https://w3id.org/dpv#AuthorityUninformed>, <https://w3id.org/dpv/dpv-owl#AuthorityUninformed> .

<https://w3id.org/dpv/owl#LegalComplianceAssessment>
  a owl:Class, owl:NamedIndividual, <https://w3id.org/dpv/owl#OrganisationalMeasure> ;
  rdfs:subClassOf <https://w3id.org/dpv/owl#ComplianceAssessment> ;
  dc:contributor _:genid4, _:genid1 ;
  dc:created "2024-04-14"^^xsd:date ;
  ns1:term_status "accepted"@en ;
  skos:definition "Assessment regarding legal compliance"@en ;
  skos:prefLabel "Legal Compliance Assessment"@en ;
  owl:sameAs <https://w3id.org/dpv#LegalComplianceAssessment>, <https://w3id.org/dpv/dpv-owl#LegalComplianceAssessment> .

<https://w3id.org/dpv/owl#ManageConsent>
  a owl:Class ;
  rdfs:subClassOf <https://w3id.org/dpv/owl#ProvideConsent>, <https://w3id.org/dpv/owl#ReaffirmConsent>, <https://w3id.org/dpv/owl#WithdrawConsent> ;
  dc:created "2024-12-17"^^xsd:date ;
  ns1:term_status "accepted"@en ;
  skos:definition "Control for managing a given consent in terms of providing, reaffirming, or withdrawing it"@en ;
  skos:prefLabel "Manage Consent"@en ;
  skos:scopeNote "Indicates how the data subject can manage their consent in terms of providing it, or reaffirming or withdrawing a given consent. This concept is useful to represent a single location or interface where multiple controls are provided for consent"@en ;
  owl:sameAs <https://w3id.org/dpv#ManageConsent>, <https://w3id.org/dpv/dpv-owl#ManageConsent> .

odrl:#constraintLogicalOperands
  a owl:NamedIndividual, skos:Collection ;
  skos:member odrl:and, odrl:andSequence, odrl:or, odrl:xone ;
  skos:prefLabel "Logical Constraint Operands"@en ;
  skos:scopeNote "ODRL Core Vocabulary Terms"@en .

<https://w3id.org/dpv/owl#Processing>
  a owl:Class ;
  rdfs:subClassOf odrl:Action ;
  dc:contributor _:genid13, _:genid11 ;
  dc:created "2019-04-05"^^xsd:date ;
  dc:modified "2020-11-04"^^xsd:date ;
  dc:source [
    a ns0:WebPage ;
    ns0:name "SPECIAL Project" ;
    ns0:url "https://specialprivacy.ercim.eu/"
  ] ;
  ns3:example <https://w3id.org/dpv/examples/owl#E0085> ;
  ns1:term_status "accepted"@en ;
  skos:definition "Operations or 'processing' performed on data"@en ;
  skos:prefLabel "Processing Data"@en ;
  skos:related <https://specialprivacy.ercim.eu/langs/usage-policy#AnyProcessing> ;
  owl:sameAs <https://w3id.org/dpv#Processing>, <https://w3id.org/dpv/dpv-owl#Processing> .

<https://w3id.org/dpv/owl#Modify>
  a owl:Class, owl:NamedIndividual, <https://w3id.org/dpv/owl#Processing> ;
  rdfs:subClassOf <https://w3id.org/dpv/owl#Alter> ;
  dc:contributor _:genid4, _:genid1 ;
  dc:created "2022-06-15"^^xsd:date ;
  ns1:term_status "accepted"@en ;
  skos:definition "to modify or change data"@en ;
  skos:prefLabel "Modify Data"@en ;
  owl:sameAs <https://w3id.org/dpv#Modify>, <https://w3id.org/dpv/dpv-owl#Modify> .

<https://w3id.org/dpv/owl#FileSystemSecurity>
  a owl:Class, owl:NamedIndividual, <https://w3id.org/dpv/owl#TechnicalMeasure> ;
  rdfs:subClassOf <https://w3id.org/dpv/owl#SecurityMethod> ;
  dc:contributor _:genid1 ;
  dc:created "2022-08-17"^^xsd:date ;
  dc:source [
    a ns0:WebPage ;
    ns0:name "ENISA Reference Incident Classification Taxonomy 2018" ;
    ns0:url "https://www.enisa.europa.eu/publications/reference-incident-classification-taxonomy/"
  ] ;
  ns1:term_status "accepted"@en ;
  skos:definition "Security implemented over a file system"@en ;
  skos:prefLabel "File System Security"@en ;
  owl:sameAs <https://w3id.org/dpv#FileSystemSecurity>, <https://w3id.org/dpv/dpv-owl#FileSystemSecurity> .

<https://w3id.org/dpv/owl#hasLawfulness>
  a owl:ObjectProperty ;
  rdfs:subPropertyOf <https://w3id.org/dpv/owl#hasComplianceStatus> ;
  ns2:rangeIncludes <https://w3id.org/dpv/owl#Lawfulness> ;
  dc:contributor _:genid1 ;
  dc:created "2022-10-22"^^xsd:date ;
  ns1:term_status "accepted"@en ;
  skos:definition "Indicates the status of being lawful or legally compliant"@en ;
  skos:prefLabel "has lawfulness"@en ;
  ns0:rangeIncludes <https://w3id.org/dpv/owl#Lawfulness> ;
  owl:sameAs <https://w3id.org/dpv#hasLawfulness>, <https://w3id.org/dpv/dpv-owl#hasLawfulness> .

<https://w3id.org/dpv/owl#FixedSingularLocation>
  a owl:Class, owl:NamedIndividual, <https://w3id.org/dpv/owl#LocationFixture> ;
  rdfs:subClassOf <https://w3id.org/dpv/owl#FixedLocation> ;
  dc:contributor _:genid1 ;
  dc:created "2022-06-15"^^xsd:date ;
  dc:modified "2020-10-05"^^xsd:date ;
  ns1:term_status "accepted"@en ;
  skos:definition "Location that is fixed at a specific place e.g. a city"@en ;
  skos:prefLabel "Fixed Singular Location"@en ;
  owl:sameAs <https://w3id.org/dpv#FixedSingularLocation>, <https://w3id.org/dpv/dpv-owl#FixedSingularLocation> .

<https://w3id.org/dpv/owl#Principle>
  a owl:Class, owl:NamedIndividual, <https://w3id.org/dpv/owl#OrganisationalMeasure> ;
  rdfs:subClassOf <https://w3id.org/dpv/owl#GuidelinesPrinciple> ;
  dc:contributor _:genid1 ;
  dc:created "2024-05-12"^^xsd:date ;
  ns1:term_status "accepted"@en ;
  skos:definition "A representation of values or norms that must be taken into consideration when conducting activities"@en ;
  skos:prefLabel "Principle"@en ;
  owl:sameAs <https://w3id.org/dpv#Principle>, <https://w3id.org/dpv/dpv-owl#Principle> .

<https://w3id.org/dpv/owl#PublicRegisterOfEntities>
  a owl:Class ;
  rdfs:subClassOf rdfs:Class ;
  dc:contributor _:genid5 ;
  dc:created "2024-06-11"^^xsd:date ;
  ns1:term_status "accepted"@en ;
  skos:definition "A publicly available list of entities e.g. to indicate which entities perform a certain activity within a certain location or jurisdiction"@en ;
  skos:prefLabel "Public Register of Entities"@en ;
  owl:sameAs <https://w3id.org/dpv#PublicRegisterOfEntities>, <https://w3id.org/dpv/dpv-owl#PublicRegisterOfEntities> .

<https://w3id.org/dpv/owl#Child>
  a owl:Class, owl:NamedIndividual, <https://w3id.org/dpv/owl#HumanSubject> ;
  rdfs:subClassOf <https://w3id.org/dpv/owl#VulnerableHuman> ;
  dc:contributor _:genid1 ;
  dc:created "2020-11-25"^^xsd:date ;
  dc:modified "2024-12-17"^^xsd:date ;
  ns1:term_status "modified"@en ;
  skos:definition "A 'child' is a natural legal person who is below a certain legal age depending on the legal jurisdiction."@en ;
  skos:prefLabel "Child"@en ;
  skos:scopeNote "The legality of age defining a child varies by jurisdiction. In addition, 'child' is distinct from a 'minor'. For example, the legal age for consumption of alcohol can be 21, which makes a person of age 20 a 'minor' in this context. In other cases, 'minor' and 'child' are used interchangeably to refer to a person below some legally defined age."@en ;
  owl:sameAs <https://w3id.org/dpv#Child>, <https://w3id.org/dpv/dpv-owl#Child> .

<https://w3id.org/dpv/owl#RequestActionDelayed>
  a owl:Class, owl:NamedIndividual, <https://w3id.org/dpv/owl#RequestStatus> ;
  rdfs:subClassOf <https://w3id.org/dpv/owl#RequestStatus> ;
  dc:contributor _:genid1 ;
  dc:created "2022-11-30"^^xsd:date ;
  ns3:example <https://w3id.org/dpv/examples/owl#E0058> ;
  ns1:term_status "accepted"@en ;
  skos:definition "State of a request being delayed towards fulfilment"@en ;
  skos:prefLabel "Request Action Delayed"@en ;
  owl:sameAs <https://w3id.org/dpv#RequestActionDelayed>, <https://w3id.org/dpv/dpv-owl#RequestActionDelayed> .

skos:member a owl:AnnotationProperty .
<https://w3id.org/dpv/owl#CryptographicKeyManagement>
  a owl:Class, owl:NamedIndividual, <https://w3id.org/dpv/owl#TechnicalMeasure> ;
  rdfs:subClassOf <https://w3id.org/dpv/owl#CryptographicMethods> ;
  dc:contributor _:genid1 ;
  dc:created "2022-08-17"^^xsd:date ;
  dc:source [
    a ns0:WebPage ;
    ns0:name "ENISA Reference Incident Classification Taxonomy 2018" ;
    ns0:url "https://www.enisa.europa.eu/publications/reference-incident-classification-taxonomy/"
  ] ;
  ns1:term_status "accepted"@en ;
  skos:definition "Management of cryptographic keys, including their generation, storage, assessment, and safekeeping"@en ;
  skos:prefLabel "Cryptographic Key Management"@en ;
  owl:sameAs <https://w3id.org/dpv#CryptographicKeyManagement>, <https://w3id.org/dpv/dpv-owl#CryptographicKeyManagement> .

<https://w3id.org/dpv/owl#ContractDisputed>
  a owl:Class, owl:NamedIndividual, <https://w3id.org/dpv/owl#ContractTerminationStatus> ;
  rdfs:subClassOf <https://w3id.org/dpv/owl#ContractTerminationStatus> ;
  dc:contributor _:genid4, _:genid1, _:genid17 ;
  dc:created "2025-01-09"^^xsd:date ;
  ns1:term_status "accepted"@en ;
  skos:definition "Status representing contract being disputed where one or more parties have an issue regarding the interpretation and performance of the contract"@en ;
  skos:prefLabel "Contract Disputed"@en ;
  owl:sameAs <https://w3id.org/dpv#ContractDisputed>, <https://w3id.org/dpv/dpv-owl#ContractDisputed> .

<https://w3id.org/dpv/owl#NationalScale>
  a owl:Class, owl:NamedIndividual, <https://w3id.org/dpv/owl#GeographicCoverage> ;
  rdfs:subClassOf <https://w3id.org/dpv/owl#GeographicCoverage> ;
  dc:contributor _:genid1 ;
  dc:created "2022-06-15"^^xsd:date ;
  ns1:term_status "accepted"@en ;
  skos:definition "Geographic coverage spanning a nation"@en ;
  skos:prefLabel "National Scale"@en ;
  owl:sameAs <https://w3id.org/dpv#NationalScale>, <https://w3id.org/dpv/dpv-owl#NationalScale> .

<https://w3id.org/dpv/owl#DataVolume>
  a owl:Class ;
  rdfs:subClassOf <https://w3id.org/dpv/owl#Scale> ;
  dc:contributor _:genid65, _:genid4, _:genid1 ;
  dc:created "2022-06-15"^^xsd:date ;
  ns3:example <https://w3id.org/dpv/examples/owl#E0049> ;
  ns1:term_status "accepted"@en ;
  skos:definition "Volume or Scale of Data"@en ;
  skos:prefLabel "Data Volume"@en ;
  owl:sameAs <https://w3id.org/dpv#DataVolume>, <https://w3id.org/dpv/dpv-owl#DataVolume> .

odrl:perm
  a owl:NamedIndividual, skos:Concept, odrl:ConflictTerm ;
  rdfs:isDefinedBy odrl: ;
  rdfs:label "Prefer Permissions"@en ;
  skos:definition "Permissions take preference over prohibitions."@en ;
  skos:note "Used to determine policy conflict outcomes."@en .

<https://w3id.org/dpv/owl#hasHumanInvolvement>
  a owl:ObjectProperty ;
  ns2:rangeIncludes <https://w3id.org/dpv/owl#HumanInvolvement> ;
  dc:contributor _:genid4, _:genid1, _:genid6 ;
  dc:created "2020-11-04"^^xsd:date ;
  ns3:example <https://w3id.org/dpv/examples/owl#E0074> ;
  ns1:term_status "accepted"@en ;
  skos:definition "Indicates Involvement of humans in processing such as within automated decision making process"@en ;
  skos:prefLabel "has human involvement"@en ;
  skos:scopeNote "Human involvement is also relevant to 'human in the loop'"@en ;
  ns0:rangeIncludes <https://w3id.org/dpv/owl#HumanInvolvement> ;
  owl:sameAs <https://w3id.org/dpv#hasHumanInvolvement>, <https://w3id.org/dpv/dpv-owl#hasHumanInvolvement> .

<https://w3id.org/dpv/owl#isPolicyFor>
  a owl:ObjectProperty ;
  ns2:domainIncludes <https://w3id.org/dpv/owl#Policy> ;
  dc:contributor _:genid1 ;
  dc:created "2022-01-26"^^xsd:date ;
  ns1:term_status "accepted"@en ;
  skos:definition "Indicates the context or application of policy"@en ;
  skos:prefLabel "is policy for"@en ;
  ns0:domainIncludes <https://w3id.org/dpv/owl#Policy> ;
  owl:sameAs <https://w3id.org/dpv#isPolicyFor>, <https://w3id.org/dpv/dpv-owl#isPolicyFor> .

<https://w3id.org/dpv/owl#hasLocation>
  a owl:ObjectProperty, owl:NamedIndividual, odrl:LeftOperand ;
  ns2:rangeIncludes <https://w3id.org/dpv/owl#Location> ;
  dc:contributor _:genid9, _:genid10, _:genid1, _:genid11 ;
  dc:created "2019-04-05"^^xsd:date ;
  dc:source [
    a ns0:WebPage ;
    ns0:name "SPECIAL Project" ;
    ns0:url "https://specialprivacy.ercim.eu/"
  ] ;
  ns3:example <https://w3id.org/dpv/examples/owl#E0060> ;
  ns1:term_status "accepted"@en ;
  skos:definition "Indicates information about location"@en ;
  skos:prefLabel "has location"@en ;
  ns0:rangeIncludes <https://w3id.org/dpv/owl#Location> ;
  owl:sameAs <https://w3id.org/dpv#hasLocation>, <https://w3id.org/dpv/dpv-owl#hasLocation> .

<https://w3id.org/dpv/owl#NotificationFailed>
  a owl:Class, owl:NamedIndividual, <https://w3id.org/dpv/owl#NotificationStatus> ;
  rdfs:subClassOf <https://w3id.org/dpv/owl#NotificationStatus> ;
  dc:contributor _:genid1 ;
  dc:created "2024-05-19"^^xsd:date ;
  ns1:term_status "accepted"@en ;
  skos:definition "Status indicating notification(s) could not be completed due to a failure"@en ;
  skos:prefLabel "Notification Failed"@en ;
  owl:sameAs <https://w3id.org/dpv#NotificationFailed>, <https://w3id.org/dpv/dpv-owl#NotificationFailed> .

<https://w3id.org/dpv/owl#ProvidedPersonalData>
  a owl:Class ;
  rdfs:subClassOf <https://w3id.org/dpv/owl#CollectedPersonalData>, <https://w3id.org/dpv/owl#ProvidedData> ;
  dc:contributor _:genid1, _:genid6 ;
  dc:created "2024-04-20"^^xsd:date ;
  ns3:example <https://w3id.org/dpv/examples/owl#E0046> ;
  ns1:term_status "accepted"@en ;
  skos:definition "Personal Data that has been provided by an entity such as the Data Subject"@en ;
  skos:prefLabel "Provided Personal Data"@en ;
  skos:scopeNote "Provided personal data involves one entity (e.g. data subject) explicitly providing the data, which the other entity (e.g. data controller) then collects"@en ;
  owl:sameAs <https://w3id.org/dpv#ProvidedPersonalData>, <https://w3id.org/dpv/dpv-owl#ProvidedPersonalData> .

<https://w3id.org/dpv/owl#hasStatus>
  a owl:ObjectProperty ;
  ns2:domainIncludes <https://w3id.org/dpv/owl#RightExerciseActivity> ;
  ns2:rangeIncludes <https://w3id.org/dpv/owl#Status> ;
  dc:contributor _:genid1 ;
  dc:created "2022-05-18"^^xsd:date ;
  ns3:example <https://w3id.org/dpv/examples/owl#E0069> ;
  ns1:term_status "accepted"@en ;
  skos:definition "Indicates the status of specified concept"@en ;
  skos:prefLabel "has status"@en ;
  skos:scopeNote "Also used to Indicate the status of a Right Exercise Activity"@en ;
  ns0:domainIncludes <https://w3id.org/dpv/owl#RightExerciseActivity> ;
  ns0:rangeIncludes <https://w3id.org/dpv/owl#Status> ;
  owl:sameAs <https://w3id.org/dpv#hasStatus>, <https://w3id.org/dpv/dpv-owl#hasStatus> .

odrl:andSequence
  a owl:ObjectProperty, owl:NamedIndividual, skos:Concept ;
  rdfs:subPropertyOf odrl:operand ;
  rdfs:isDefinedBy odrl: ;
  rdfs:label "And Sequence"@en ;
  skos:definition "The relation is satisfied when each of the Constraints are satisfied in the order specified."@en ;
  skos:note "This property MUST only be used for Logical Constraints, and the list of operand values MUST be Constraint instances. The order of the list MUST be preserved. The andSequence operator is an example where there may be temporal conditional requirements between the operands. This may lead to situations where the outcome is unresolvable, such as deadlock if one of the Constraints is unable to be satisfied. ODRL Processing systems SHOULD plan for these scenarios and implement mechanisms to resolve them."@en .

<https://w3id.org/dpv/owl#hasPersonalDataProcess>
  a owl:ObjectProperty ;
  ns2:rangeIncludes <https://w3id.org/dpv/owl#PersonalDataProcess> ;
  dc:contributor _:genid1 ;
  dc:created "2023-12-11"^^xsd:date ;
  ns1:term_status "accepted"@en ;
  skos:definition "Indicates association with a Personal Data Process"@en ;
  skos:prefLabel "has personal data process"@en ;
  ns0:rangeIncludes <https://w3id.org/dpv/owl#PersonalDataProcess> ;
  owl:sameAs <https://w3id.org/dpv#hasPersonalDataProcess>, <https://w3id.org/dpv/dpv-owl#hasPersonalDataProcess> .

<https://w3id.org/dpv/owl#ContractTerminated>
  a owl:Class, owl:NamedIndividual, <https://w3id.org/dpv/owl#ContractTerminationStatus> ;
  rdfs:subClassOf <https://w3id.org/dpv/owl#ContractTerminationStatus> ;
  dc:contributor _:genid4, _:genid1, _:genid17 ;
  dc:created "2025-01-09"^^xsd:date ;
  ns1:term_status "accepted"@en ;
  skos:definition "Status representing contract being terminated by one or more parties"@en ;
  skos:prefLabel "Contract Terminated"@en ;
  owl:sameAs <https://w3id.org/dpv#ContractTerminated>, <https://w3id.org/dpv/dpv-owl#ContractTerminated> .

<https://w3id.org/dpv/owl#FederatedLocations>
  a owl:Class, owl:NamedIndividual, <https://w3id.org/dpv/owl#LocationFixture> ;
  rdfs:subClassOf <https://w3id.org/dpv/owl#LocationFixture> ;
  dc:contributor _:genid1 ;
  dc:created "2022-06-15"^^xsd:date ;
  dc:modified "2020-10-05"^^xsd:date ;
  ns1:term_status "accepted"@en ;
  skos:definition "Location that is federated across multiple separate areas with designation of a primary or central location"@en ;
  skos:prefLabel "Federated Locations"@en ;
  owl:sameAs <https://w3id.org/dpv#FederatedLocations>, <https://w3id.org/dpv/dpv-owl#FederatedLocations> .

<https://w3id.org/dpv/owl#isOrganistionalUnitOf>
  a owl:ObjectProperty ;
  rdfs:subPropertyOf <https://w3id.org/dpv/owl#hasEntity> ;
  ns2:domainIncludes <https://w3id.org/dpv/owl#OrganisationalUnit> ;
  ns2:rangeIncludes <https://w3id.org/dpv/owl#Entity> ;
  dc:contributor _:genid1 ;
  dc:created "2024-06-10"^^xsd:date ;
  ns1:term_status "accepted"@en ;
  skos:definition "Indicates this entity is an organisational unit of the specified entity"@en ;
  skos:prefLabel "is organisational unit of"@en ;
  ns0:domainIncludes <https://w3id.org/dpv/owl#OrganisationalUnit> ;
  ns0:rangeIncludes <https://w3id.org/dpv/owl#Entity> ;
  owl:sameAs <https://w3id.org/dpv#isOrganistionalUnitOf>, <https://w3id.org/dpv/dpv-owl#isOrganistionalUnitOf> .

odrl:compensatedParty
  a owl:ObjectProperty, owl:NamedIndividual, skos:Concept ;
  rdfs:subPropertyOf odrl:function ;
  rdfs:isDefinedBy odrl: ;
  rdfs:label "Compensated Party"@en ;
  skos:definition "The Party is the recipient of the compensation."@en ;
  skos:note "Maybe specified as part of the compensate duty action."@en ;
  skos:scopeNote "Non-Normative"@en .

<https://w3id.org/dpv/owl#EnforceAccessControl>
  a owl:Class, owl:NamedIndividual, <https://w3id.org/dpv/owl#Purpose> ;
  rdfs:subClassOf <https://w3id.org/dpv/owl#EnforceSecurity> ;
  dc:contributor _:genid13, _:genid14, _:genid1, _:genid15, _:genid16, _:genid11 ;
  dc:created "2019-04-05"^^xsd:date ;
  ns1:term_status "accepted"@en ;
  skos:definition "Purposes associated with conducting or enforcing access control as a form of security"@en ;
  skos:prefLabel "Enforce Access Control"@en ;
  skos:related <https://specialprivacy.ercim.eu/vocabs/purposes#Login> ;
  skos:scopeNote "Was previously \"Access Control\". Prefixed to distinguish from Technical Measure."@en ;
  owl:sameAs <https://w3id.org/dpv#EnforceAccessControl>, <https://w3id.org/dpv/dpv-owl#EnforceAccessControl> .

<https://w3id.org/dpv/owl#RecruitmentApplicantSelection>
  a owl:Class, owl:NamedIndividual, <https://w3id.org/dpv/owl#Purpose> ;
  rdfs:subClassOf <https://w3id.org/dpv/owl#RecruitmentManagement> ;
  dc:created "2024-12-01"^^xsd:date ;
  ns1:term_status "accepted"@en ;
  skos:definition "Purposes associated with determination or selection of candidates, whether for a specific job or job pool, or for a specific stage as part of recruitment"@en ;
  skos:prefLabel "Recruitment Applicant Selection"@en ;
  owl:sameAs <https://w3id.org/dpv#RecruitmentApplicantSelection>, <https://w3id.org/dpv/dpv-owl#RecruitmentApplicantSelection> .

<https://w3id.org/dpv/owl#RightExerciseRecord>
  a owl:Class, owl:NamedIndividual, <https://w3id.org/dpv/owl#OrganisationalMeasure> ;
  rdfs:subClassOf <https://w3id.org/dpv/owl#Record> ;
  dc:contributor _:genid4, _:genid5, _:genid1, _:genid6 ;
  dc:created "2022-11-02"^^xsd:date ;
  ns3:example <https://w3id.org/dpv/examples/owl#E0057> ;
  ns1:term_status "accepted"@en ;
  skos:definition "Record of a Right being exercised"@en ;
  skos:prefLabel "Right Exercise Record Data"@en ;
  skos:scopeNote "This concept represents a record of one or more right exercise activities, such as those associated with a single data subject or service or entity"@en ;
  owl:sameAs <https://w3id.org/dpv#RightExerciseRecord>, <https://w3id.org/dpv/dpv-owl#RightExerciseRecord> .

<https://w3id.org/dpv/owl#Process>
  a owl:Class ;
  dc:contributor _:genid1 ;
  dc:created "2024-05-09"^^xsd:date ;
  ns3:example <https://w3id.org/dpv/examples/owl#E0005>, <https://w3id.org/dpv/examples/owl#E0006>, <https://w3id.org/dpv/examples/owl#E0031>, <https://w3id.org/dpv/examples/owl#E0041> ;
  ns1:term_status "accepted"@en ;
  skos:definition "An action, activity, or method"@en ;
  skos:prefLabel "Process"@en ;
  owl:sameAs <https://w3id.org/dpv#Process>, <https://w3id.org/dpv/dpv-owl#Process> .

<https://w3id.org/dpv/owl#ConsentExpired>
  a owl:Class, owl:NamedIndividual, <https://w3id.org/dpv/owl#ConsentStatus> ;
  rdfs:subClassOf <https://w3id.org/dpv/owl#ConsentStatusInvalidForProcessing> ;
  dc:contributor _:genid4, _:genid1, _:genid17, _:genid6 ;
  dc:created "2022-06-22"^^xsd:date ;
  dc:source [
    a ns0:WebPage ;
    ns0:name "GConsent" ;
    ns0:url "https://w3id.org/GConsent"
  ] ;
  ns1:term_status "accepted"@en ;
  skos:definition "The state where the temporal or contextual validity of consent has 'expired'"@en ;
  skos:prefLabel "Consent Expired"@en ;
  skos:scopeNote "An example of this state is when the obtained consent has been assigned a duration - which has lapsed or 'expired', making it invalid to be used further for processing data"@en ;
  owl:sameAs <https://w3id.org/dpv#ConsentExpired>, <https://w3id.org/dpv/dpv-owl#ConsentExpired> .

<https://w3id.org/dpv/owl#DataSubjectUninformed>
  a owl:Class, owl:NamedIndividual, <https://w3id.org/dpv/owl#EntityInformedStatus> ;
  rdfs:subClassOf <https://w3id.org/dpv/owl#EntityUninformed> ;
  dc:contributor _:genid4, _:genid1, _:genid25, _:genid6 ;
  dc:created "2024-05-10"^^xsd:date ;
  ns1:term_status "accepted"@en ;
  skos:definition "Status indicating DataSubject is uninformed i.e. has not been informed about the specified context"@en ;
  skos:prefLabel "Data Subject Uninformed"@en ;
  owl:sameAs <https://w3id.org/dpv#DataSubjectUninformed>, <https://w3id.org/dpv/dpv-owl#DataSubjectUninformed> .

<https://w3id.org/dpv/owl#RecordManagement>
  a owl:Class, owl:NamedIndividual, <https://w3id.org/dpv/owl#Purpose> ;
  rdfs:subClassOf <https://w3id.org/dpv/owl#Purpose> ;
  dc:contributor _:genid4, _:genid1, _:genid6, _:genid21 ;
  dc:created "2021-09-01"^^xsd:date ;
  ns1:term_status "accepted"@en ;
  skos:definition "Purposes associated with manage creation, storage, and use of records relevant to operations, events, and processes e.g. to store logs or access requests"@en ;
  skos:prefLabel "Record Management"@en ;
  skos:scopeNote "This purpose relates specifically for record creation and management. This can be combined or used along with other purposes to express intentions such as records for legal compliance or vendor payments."@en ;
  owl:sameAs <https://w3id.org/dpv#RecordManagement>, <https://w3id.org/dpv/dpv-owl#RecordManagement> .

<https://w3id.org/dpv/owl#CustomerClaimsManagement>
  a owl:Class, owl:NamedIndividual, <https://w3id.org/dpv/owl#Purpose> ;
  rdfs:subClassOf <https://w3id.org/dpv/owl#CustomerManagement> ;
  dc:contributor _:genid4, _:genid5, _:genid1 ;
  dc:created "2021-09-08"^^xsd:date ;
  dc:source [
    a ns0:WebPage ;
    ns0:name "Belgian DPA ROPA Template" ;
    ns0:url "https://www.privacycommission.be/nl/model-voor-een-register-van-de-verwerkingsactiviteiten"
  ] ;
  ns1:term_status "accepted"@en ;
  skos:definition "Customer Claims Management refers to purposes associated with managing claims, including repayment of monies owed"@en ;
  skos:prefLabel "Customer Claims Management"@en ;
  owl:sameAs <https://w3id.org/dpv#CustomerClaimsManagement>, <https://w3id.org/dpv/dpv-owl#CustomerClaimsManagement> .

odrl:Privacy
  a owl:Class, owl:NamedIndividual, skos:Concept ;
  rdfs:subClassOf odrl:Policy ;
  owl:disjointWith odrl:Request, odrl:Set, odrl:Ticket ;
  rdfs:isDefinedBy odrl: ;
  rdfs:label "Privacy Policy"@en ;
  skos:definition "A Policy that expresses a Rule over an Asset containing personal information."@en ;
  skos:note "A Privacy Policy  MUST contain a target Asset, a Party with Assigner  is, a Party with Assignee function, and at least one of a Permission or Prohibition rule that MUST include a Duty. The target Asset SHOULD contain or relate to personal information about the Assignee. The Duty MUST describe obligations on the Assigner about managing the Asset. The Assignee is being granted the terms of the Privacy policy from the Assigner."@en ;
  skos:scopeNote "Non-Normative"@en .

<https://w3id.org/dpv/owl#NonCitizen>
  a owl:Class, owl:NamedIndividual, <https://w3id.org/dpv/owl#HumanSubject> ;
  rdfs:subClassOf <https://w3id.org/dpv/owl#HumanSubject> ;
  dc:contributor _:genid4, _:genid5, _:genid1, _:genid17, _:genid6 ;
  dc:created "2022-04-06"^^xsd:date ;
  dc:modified "2024-12-17"^^xsd:date ;
  ns1:term_status "modified"@en ;
  skos:definition "Humans that are not citizens (for a jurisdiction)"@en ;
  skos:prefLabel "Non-Citizen"@en ;
  owl:sameAs <https://w3id.org/dpv#NonCitizen>, <https://w3id.org/dpv/dpv-owl#NonCitizen> .

<https://w3id.org/dpv/owl#hasRecipientThirdParty>
  a owl:ObjectProperty ;
  rdfs:subPropertyOf <https://w3id.org/dpv/owl#hasRecipient> ;
  ns2:rangeIncludes <https://w3id.org/dpv/owl#ThirdParty> ;
  dc:contributor _:genid4, _:genid1, _:genid6 ;
  dc:created "2022-02-09"^^xsd:date ;
  ns1:term_status "accepted"@en ;
  skos:definition "Indiciates inclusion or applicability of a Third Party as a Recipient of persona data"@en ;
  skos:prefLabel "has recipient third party"@en ;
  ns0:rangeIncludes <https://w3id.org/dpv/owl#ThirdParty> ;
  owl:sameAs <https://w3id.org/dpv#hasRecipientThirdParty>, <https://w3id.org/dpv/dpv-owl#hasRecipientThirdParty> .

<https://w3id.org/dpv/owl#ConsultationWithDataSubjectRepresentative>
  a owl:Class, owl:NamedIndividual, <https://w3id.org/dpv/owl#OrganisationalMeasure> ;
  rdfs:subClassOf <https://w3id.org/dpv/owl#ConsultationWithDataSubject> ;
  dc:contributor _:genid4, _:genid1 ;
  dc:created "2022-10-22"^^xsd:date ;
  ns1:term_status "accepted"@en ;
  skos:definition "Consultation with representative of data subject(s)"@en ;
  skos:prefLabel "Consultation with Data Subject Representative"@en ;
  owl:sameAs <https://w3id.org/dpv#ConsultationWithDataSubjectRepresentative>, <https://w3id.org/dpv/dpv-owl#ConsultationWithDataSubjectRepresentative> .

odrl:PartyCollection
  a owl:Class, owl:NamedIndividual, skos:Concept ;
  rdfs:subClassOf odrl:Party ;
  rdfs:isDefinedBy odrl: ;
  rdfs:label "Party Collection"@en ;
  skos:definition "A Party that is a group of individual entities"@en .

odrl:#assetRelations
  a owl:NamedIndividual, skos:Collection ;
  skos:member odrl:hasPolicy, odrl:target ;
  skos:prefLabel "Asset Relations"@en ;
  skos:scopeNote "ODRL Core Vocabulary Terms"@en .

<https://w3id.org/dpv/owl#DataTransferNotice>
  a owl:Class, owl:NamedIndividual, <https://w3id.org/dpv/owl#OrganisationalMeasure> ;
  rdfs:subClassOf <https://w3id.org/dpv/owl#Notice> ;
  dc:contributor _:genid4, _:genid5, _:genid1, _:genid6, _:genid21 ;
  dc:created "2024-04-14"^^xsd:date ;
  dc:source "DGA 5.9"@en ;
  ns1:term_status "accepted"@en ;
  skos:definition "Notice for the legal entity for the transfer of its data"@en ;
  skos:prefLabel "Data Transfer Notice"@en ;
  owl:sameAs <https://w3id.org/dpv#DataTransferNotice>, <https://w3id.org/dpv/dpv-owl#DataTransferNotice> .

<https://w3id.org/dpv/owl#DecentralisedLocations>
  a owl:Class, owl:NamedIndividual, <https://w3id.org/dpv/owl#LocationFixture> ;
  rdfs:subClassOf <https://w3id.org/dpv/owl#LocationFixture> ;
  dc:contributor _:genid1 ;
  dc:created "2022-06-15"^^xsd:date ;
  dc:modified "2020-10-05"^^xsd:date ;
  ns1:term_status "accepted"@en ;
  skos:definition "Location that is spread across multiple separate areas with no distinction between their importance"@en ;
  skos:prefLabel "Decentralised Locations"@en ;
  owl:sameAs <https://w3id.org/dpv#DecentralisedLocations>, <https://w3id.org/dpv/dpv-owl#DecentralisedLocations> .

<https://w3id.org/dpv/owl#DirectMarketing>
  a owl:Class, owl:NamedIndividual, <https://w3id.org/dpv/owl#Purpose> ;
  rdfs:subClassOf <https://w3id.org/dpv/owl#Marketing> ;
  dc:contributor _:genid4, _:genid5, _:genid1 ;
  dc:created "2020-11-04"^^xsd:date ;
  ns1:term_status "accepted"@en ;
  skos:definition "Purposes associated with conducting direct marketing i.e. marketing communicated directly to the individual"@en ;
  skos:prefLabel "Direct Marketing"@en ;
  owl:sameAs <https://w3id.org/dpv#DirectMarketing>, <https://w3id.org/dpv/dpv-owl#DirectMarketing> .

<https://w3id.org/dpv/owl#DataProtectionAuthority>
  a owl:Class ;
  rdfs:subClassOf <https://w3id.org/dpv/owl#Authority> ;
  dc:contributor _:genid4, _:genid1, _:genid6 ;
  dc:created "2020-11-04"^^xsd:date ;
  ns3:example <https://w3id.org/dpv/examples/owl#E0036> ;
  ns1:term_status "accepted"@en ;
  skos:definition "An authority tasked with overseeing legal compliance regarding privacy and data protection laws."@en ;
  skos:prefLabel "Data Protection Authority"@en ;
  owl:sameAs <https://w3id.org/dpv#DataProtectionAuthority>, <https://w3id.org/dpv/dpv-owl#DataProtectionAuthority> .

<https://w3id.org/dpv/owl#RecruitmentInterviewAnalysis>
  a owl:Class, owl:NamedIndividual, <https://w3id.org/dpv/owl#Purpose> ;
  rdfs:subClassOf <https://w3id.org/dpv/owl#RecruitmentInterviewManagement> ;
  dc:created "2024-12-01"^^xsd:date ;
  ns1:term_status "accepted"@en ;
  skos:definition "Purposes associated with analysis of interviews, including the people and involved, for recruitment"@en ;
  skos:prefLabel "Recruitment Interview Analysis"@en ;
  owl:sameAs <https://w3id.org/dpv#RecruitmentInterviewAnalysis>, <https://w3id.org/dpv/dpv-owl#RecruitmentInterviewAnalysis> .

<https://w3id.org/dpv/owl#isAfter>
  a owl:ObjectProperty ;
  ns2:domainIncludes <https://w3id.org/dpv/owl#RightExerciseActivity> ;
  ns2:rangeIncludes <https://w3id.org/dpv/owl#RightExerciseActivity> ;
  dc:contributor _:genid4, _:genid1, _:genid17 ;
  dc:created "2022-03-02"^^xsd:date ;
  ns1:term_status "accepted"@en ;
  skos:definition "Indicates the specified concepts is 'after' this concept in some context"@en ;
  skos:prefLabel "is after"@en ;
  skos:scopeNote "Also used for specifying a RightExerciseActivity occurs before another RightExerciseActivity"@en ;
  ns0:domainIncludes <https://w3id.org/dpv/owl#RightExerciseActivity> ;
  ns0:rangeIncludes <https://w3id.org/dpv/owl#RightExerciseActivity> ;
  owl:sameAs <https://w3id.org/dpv#isAfter>, <https://w3id.org/dpv/dpv-owl#isAfter> .

<https://w3id.org/dpv/owl#LegitimateInterestOfDataSubject>
  a owl:Class, owl:NamedIndividual, <https://w3id.org/dpv/owl#LegalBasis> ;
  rdfs:subClassOf <https://w3id.org/dpv/owl#LegitimateInterest> ;
  dc:contributor _:genid4 ;
  dc:created "2022-10-22"^^xsd:date ;
  ns1:term_status "accepted"@en ;
  skos:definition "Legitimate Interests of the Data Subject in conducting specified activities"@en ;
  skos:prefLabel "Legitimate Interest of Data Subject"@en ;
  owl:sameAs <https://w3id.org/dpv#LegitimateInterestOfDataSubject>, <https://w3id.org/dpv/dpv-owl#LegitimateInterestOfDataSubject> .

<https://w3id.org/dpv/owl#OfficialAuthorityExerciseOngoing>
  a owl:Class, owl:NamedIndividual, <https://w3id.org/dpv/owl#OfficialAuthorityExerciseStatus> ;
  rdfs:subClassOf <https://w3id.org/dpv/owl#OfficialAuthorityExerciseStatus> ;
  dc:created "2024-08-27"^^xsd:date ;
  ns1:term_status "accepted"@en ;
  skos:definition "Status where the official authority is being exercised"@en ;
  skos:prefLabel "Official Authority Exercise Ongoing"@en ;
  owl:sameAs <https://w3id.org/dpv#OfficialAuthorityExerciseOngoing>, <https://w3id.org/dpv/dpv-owl#OfficialAuthorityExerciseOngoing> .

<https://w3id.org/dpv/owl#CloudLocation>
  a owl:Class, owl:NamedIndividual, <https://w3id.org/dpv/owl#Location> ;
  rdfs:subClassOf <https://w3id.org/dpv/owl#RemoteLocation> ;
  dc:contributor _:genid1 ;
  dc:created "2022-06-15"^^xsd:date ;
  dc:modified "2020-10-05"^^xsd:date ;
  ns1:term_status "accepted"@en ;
  skos:definition "Location that is in the 'cloud' i.e. a logical location operated over the internet"@en ;
  skos:prefLabel "Cloud Location"@en ;
  owl:sameAs <https://w3id.org/dpv#CloudLocation>, <https://w3id.org/dpv/dpv-owl#CloudLocation> .

<https://w3id.org/dpv/owl#PoliticalCampaign>
  a owl:Class, owl:NamedIndividual, <https://w3id.org/dpv/owl#Purpose> ;
  rdfs:subClassOf <https://w3id.org/dpv/owl#Advertising>, <https://w3id.org/dpv/owl#Personalisation> ;
  dc:created "2024-12-01"^^xsd:date ;
  ns1:term_status "accepted"@en ;
  skos:definition "Purposes associated with political campaign activities related to promotion and advertisement of positions and candidates in elections at local, state or regional, or national and international levels"@en ;
  skos:prefLabel "Political Campaign"@en ;
  owl:sameAs <https://w3id.org/dpv#PoliticalCampaign>, <https://w3id.org/dpv/dpv-owl#PoliticalCampaign> .

<https://w3id.org/dpv/owl#NaturalPerson>
  a owl:Class ;
  rdfs:subClassOf <https://w3id.org/dpv/owl#Entity> ;
  dc:contributor _:genid1 ;
  dc:created "2022-02-09"^^xsd:date ;
  ns1:term_status "accepted"@en ;
  skos:definition "A human"@en ;
  skos:prefLabel "Natural Person"@en ;
  owl:sameAs <https://w3id.org/dpv#NaturalPerson>, <https://w3id.org/dpv/dpv-owl#NaturalPerson> .

<https://w3id.org/dpv/owl#PersonnelMonitoring>
  a owl:Class, owl:NamedIndividual, <https://w3id.org/dpv/owl#Purpose> ;
  rdfs:subClassOf <https://w3id.org/dpv/owl#PersonnelManagement> ;
  dc:created "2024-12-01"^^xsd:date ;
  ns1:term_status "accepted"@en ;
  skos:definition "Purposes associated with monitoring of personnel"@en ;
  skos:prefLabel "Personnel Monitoring"@en ;
  owl:sameAs <https://w3id.org/dpv#PersonnelMonitoring>, <https://w3id.org/dpv/dpv-owl#PersonnelMonitoring> .

<https://w3id.org/dpv/owl#RegionalScale>
  a owl:Class, owl:NamedIndividual, <https://w3id.org/dpv/owl#GeographicCoverage> ;
  rdfs:subClassOf <https://w3id.org/dpv/owl#GeographicCoverage> ;
  dc:contributor _:genid1 ;
  dc:created "2022-06-15"^^xsd:date ;
  ns1:term_status "accepted"@en ;
  skos:definition "Geographic coverage spanning a specific region or regions"@en ;
  skos:prefLabel "Regional Scale"@en ;
  owl:sameAs <https://w3id.org/dpv#RegionalScale>, <https://w3id.org/dpv/dpv-owl#RegionalScale> .

<https://w3id.org/dpv/owl#Patient>
  a owl:Class, owl:NamedIndividual, <https://w3id.org/dpv/owl#HumanSubject> ;
  rdfs:subClassOf <https://w3id.org/dpv/owl#HumanSubject> ;
  dc:contributor _:genid4, _:genid5, _:genid1, _:genid17, _:genid6 ;
  dc:created "2022-04-06"^^xsd:date ;
  dc:modified "2024-12-17"^^xsd:date ;
  ns1:term_status "modified"@en ;
  skos:definition "Humans that receive medical attention, treatment, care, advice, or other health related services"@en ;
  skos:prefLabel "Patient"@en ;
  owl:sameAs <https://w3id.org/dpv#Patient>, <https://w3id.org/dpv/dpv-owl#Patient> .

<https://w3id.org/dpv/owl#Notification>
  a owl:Class, owl:NamedIndividual, <https://w3id.org/dpv/owl#OrganisationalMeasure> ;
  rdfs:subClassOf <https://w3id.org/dpv/owl#OrganisationalMeasure> ;
  dc:contributor _:genid1 ;
  dc:created "2024-04-14"^^xsd:date ;
  ns1:term_status "accepted"@en ;
  skos:definition "Notification represents the provision of a notice i.e. notifying"@en ;
  skos:prefLabel "Notification"@en ;
  skos:scopeNote "Notice refers to the information whereas Notification refers to the provision of that notice. The distinction is important as there are specific obligations associated with notice and notifications. For example, a data breach notice refers to the information about the breach intended to be provided to another entity, whereas notification refers to the act of providing the entity with the notice"@en ;
  owl:sameAs <https://w3id.org/dpv#Notification>, <https://w3id.org/dpv/dpv-owl#Notification> .

<https://w3id.org/dpv/owl#ContractActivationStatus>
  a owl:Class ;
  rdfs:subClassOf <https://w3id.org/dpv/owl#ContractStatus> ;
  dc:contributor _:genid4, _:genid1, _:genid17 ;
  dc:created "2025-01-09"^^xsd:date ;
  ns1:term_status "accepted"@en ;
  skos:definition "Status associated with activation of a contract i.e. whether its terms are active and are required to be performed"@en ;
  skos:prefLabel "Contract Activation Status"@en ;
  owl:sameAs <https://w3id.org/dpv#ContractActivationStatus>, <https://w3id.org/dpv/dpv-owl#ContractActivationStatus> .

<https://w3id.org/dpv/owl#Tracking>
  a owl:Class, owl:NamedIndividual, <https://w3id.org/dpv/owl#Processing> ;
  rdfs:subClassOf <https://w3id.org/dpv/owl#Use> ;
  dc:contributor _:genid5, _:genid56, _:genid1 ;
  dc:created "2024-12-17"^^xsd:date ;
  ns3:example <https://w3id.org/dpv/examples/owl#E0075> ;
  ns1:term_status "accepted"@en ;
  skos:definition "to use data to track a specific factor (e.g. a human or their activities) across multiple distinct contexts"@en ;
  skos:prefLabel "Tracking"@en ;
  skos:scopeNote "Tracking is a widely used (and abused) concept and therefore carries several distinct interpretations, for example see Do Not Track which defines tracking in the context of the web, and where other forms of tracking such as location tracking or physical biometric tracking may exist which are defined differently. For this concept, DPVCG defines Tracking in the broadest possible sense and strongly recommends adopters to provide their specific definition or interpretation by either extending this concept, through a usage note, or by contributing the specific term back to DPVCG for inclusion in DPV or an extension. This concept may change in the future based on developments in privacy and legal spaces. In DPV, Tracking is defined as a type of processing operation that may collect and/or may use data - which covers both initial collection and usage as well as subsequent use of existing data to track an individual. The classification of Tracking as a processing operation also implies that it is not sufficient as a Purpose on its own and therefore a suitable purpose from the DPV taxonomy should be used to justify it."@en ;
  owl:sameAs <https://w3id.org/dpv#Tracking>, <https://w3id.org/dpv/dpv-owl#Tracking> .

<https://w3id.org/dpv/owl#hasLikelihood>
  a owl:ObjectProperty ;
  ns2:rangeIncludes <https://w3id.org/dpv/owl#Likelihood> ;
  dc:contributor _:genid4, _:genid1, _:genid17, _:genid6 ;
  dc:created "2022-07-20"^^xsd:date ;
  ns3:example <https://w3id.org/dpv/examples/owl#E0068> ;
  ns1:term_status "accepted"@en ;
  skos:definition "Indicates the likelihood associated with a concept"@en ;
  skos:prefLabel "has likelihood"@en ;
  ns0:rangeIncludes <https://w3id.org/dpv/owl#Likelihood> ;
  owl:sameAs <https://w3id.org/dpv#hasLikelihood>, <https://w3id.org/dpv/dpv-owl#hasLikelihood> .

cc:Sharing
  a owl:NamedIndividual, skos:Concept, odrl:Action ;
  odrl:includedIn odrl:use ;
  rdfs:isDefinedBy odrl: ;
  rdfs:label "Sharing"@en ;
  skos:definition "Permits commercial derivatives, but only non-commercial distribution."@en ;
  skos:note "This term is defined by Creative Commons."@en ;
  skos:scopeNote "Non-Normative"@en .

<https://w3id.org/dpv/owl#CannotChallengeProcessInput>
  a owl:Class, owl:NamedIndividual, <https://w3id.org/dpv/owl#EntityNonPermissiveInvolvement> ;
  rdfs:subClassOf <https://w3id.org/dpv/owl#EntityNonPermissiveInvolvement> ;
  dc:contributor _:genid1, _:genid25, _:genid19 ;
  dc:created "2024-05-11"^^xsd:date ;
  ns1:term_status "accepted"@en ;
  skos:definition "Involvement where entity cannot challenge input of specified context"@en ;
  skos:prefLabel "Cannot Challenge Process Input"@en ;
  owl:sameAs <https://w3id.org/dpv#CannotChallengeProcessInput>, <https://w3id.org/dpv/dpv-owl#CannotChallengeProcessInput> .

<https://w3id.org/dpv/owl#PersonalisedBenefits>
  a owl:Class, owl:NamedIndividual, <https://w3id.org/dpv/owl#Purpose> ;
  rdfs:subClassOf <https://w3id.org/dpv/owl#ServicePersonalisation> ;
  dc:contributor _:genid13, _:genid14, _:genid1, _:genid15, _:genid16, _:genid11 ;
  dc:created "2019-04-05"^^xsd:date ;
  ns1:term_status "accepted"@en ;
  skos:definition "Purposes associated with creating and providing personalised benefits for a service"@en ;
  skos:prefLabel "Personalised Benefits"@en ;
  owl:sameAs <https://w3id.org/dpv#PersonalisedBenefits>, <https://w3id.org/dpv/dpv-owl#PersonalisedBenefits> .

<https://w3id.org/dpv/owl#Certification>
  a owl:Class, owl:NamedIndividual, <https://w3id.org/dpv/owl#OrganisationalMeasure> ;
  rdfs:subClassOf <https://w3id.org/dpv/owl#CertificationSeal> ;
  dc:contributor _:genid9, _:genid10, _:genid1, _:genid11 ;
  dc:created "2019-04-05"^^xsd:date ;
  ns1:term_status "accepted"@en ;
  skos:definition "Certification mechanisms, seals, and marks for the purpose of demonstrating compliance"@en ;
  skos:prefLabel "Certification"@en ;
  owl:sameAs <https://w3id.org/dpv#Certification>, <https://w3id.org/dpv/dpv-owl#Certification> .

<https://w3id.org/dpv/owl#hasNotificationStatus>
  a owl:ObjectProperty ;
  ns2:rangeIncludes <https://w3id.org/dpv/owl#NotificationStatus> ;
  dc:contributor _:genid1 ;
  dc:created "2024-06-10"^^xsd:date ;
  ns1:term_status "accepted"@en ;
  skos:definition "Indicates the status associated with a notice"@en ;
  skos:prefLabel "has notification status"@en ;
  ns0:rangeIncludes <https://w3id.org/dpv/owl#NotificationStatus> ;
  owl:sameAs <https://w3id.org/dpv#hasNotificationStatus>, <https://w3id.org/dpv/dpv-owl#hasNotificationStatus> .

<https://w3id.org/dpv/owl#ObjectingToProcess>
  a owl:Class, owl:NamedIndividual, <https://w3id.org/dpv/owl#EntityPermissiveInvolvement> ;
  rdfs:subClassOf <https://w3id.org/dpv/owl#EntityPermissiveInvolvement> ;
  dc:contributor _:genid1, _:genid25, _:genid19 ;
  dc:created "2024-05-11"^^xsd:date ;
  ns1:term_status "accepted"@en ;
  skos:definition "Involvement where entity can object to process of specified context"@en ;
  skos:prefLabel "Objecting to Process"@en ;
  owl:sameAs <https://w3id.org/dpv#ObjectingToProcess>, <https://w3id.org/dpv/dpv-owl#ObjectingToProcess> .

<https://w3id.org/dpv/owl#hasTechnicalMeasure>
  a owl:ObjectProperty ;
  rdfs:subPropertyOf <https://w3id.org/dpv/owl#hasTechnicalOrganisationalMeasure> ;
  ns2:rangeIncludes <https://w3id.org/dpv/owl#TechnicalMeasure> ;
  dc:contributor _:genid1 ;
  dc:created "2022-02-09"^^xsd:date ;
  ns3:example <https://w3id.org/dpv/examples/owl#E0064>, <https://w3id.org/dpv/examples/owl#E0070> ;
  ns1:term_status "accepted"@en ;
  skos:definition "Indicates use or applicability of Technical measure"@en ;
  skos:prefLabel "has technical measure"@en ;
  ns0:rangeIncludes <https://w3id.org/dpv/owl#TechnicalMeasure> ;
  owl:sameAs <https://w3id.org/dpv#hasTechnicalMeasure>, <https://w3id.org/dpv/dpv-owl#hasTechnicalMeasure> .

odrl:contractedParty
  a owl:ObjectProperty, owl:NamedIndividual, skos:Concept ;
  rdfs:subPropertyOf odrl:function ;
  rdfs:isDefinedBy odrl: ;
  rdfs:label "Contracted Party"@en ;
  skos:definition "The Party who is being contracted."@en ;
  skos:scopeNote "Non-Normative"@en .

<https://w3id.org/dpv/owl#NegotiatedContract>
  a owl:Class, owl:NamedIndividual, <https://w3id.org/dpv/owl#LegalBasis> ;
  rdfs:subClassOf <https://w3id.org/dpv/owl#ContractByNegotiationType> ;
  dc:created "2024-08-27"^^xsd:date ;
  ns1:term_status "accepted"@en ;
  skos:definition "A contract where the terms and conditions are determined with all parties having the ability to negotiate the terms and conditions"@en ;
  skos:prefLabel "Negotiated Contract"@en ;
  skos:scopeNote "Negotiation here refers to the opportunity for a party on their own initiative to modify or dictate terms and conditions within a contract. If the party is provided a set of options to choose from or in other ways is dictated which terms and conditions can be present in the contract, neither of these should be considered a negotiation"@en ;
  owl:sameAs <https://w3id.org/dpv#NegotiatedContract>, <https://w3id.org/dpv/dpv-owl#NegotiatedContract> .

<https://w3id.org/dpv/owl#RenewedConsentGiven>
  a owl:Class, owl:NamedIndividual, <https://w3id.org/dpv/owl#ConsentStatus> ;
  rdfs:subClassOf <https://w3id.org/dpv/owl#ConsentStatusValidForProcessing> ;
  dc:contributor _:genid4, _:genid1, _:genid17, _:genid6 ;
  dc:created "2022-06-22"^^xsd:date ;
  dc:source [
    a ns0:WebPage ;
    ns0:name "GConsent" ;
    ns0:url "https://w3id.org/GConsent"
  ] ;
  ns1:term_status "accepted"@en ;
  skos:definition "The state where a previously given consent has been 'renewed' or 'refreshed' or 'reaffirmed' to form a new instance of given consent"@en ;
  skos:prefLabel "Renewed Consent Given"@en ;
  skos:scopeNote "An example of this state is when a previously given consent has expired, and the individual is presented a notice regarding continuing associated processing operations - to which they agree. This state can be useful to keep track of 'reconfirmed' or 'refreshed' consent within consent records, assist notices and contextual agents to create better consenting dialogues, and assist with specific legal obligations related to subsequent consenting"@en ;
  owl:sameAs <https://w3id.org/dpv#RenewedConsentGiven>, <https://w3id.org/dpv/dpv-owl#RenewedConsentGiven> .

<https://w3id.org/dpv/owl#SingularScaleOfDataSubjects>
  a owl:Class, owl:NamedIndividual, <https://w3id.org/dpv/owl#DataSubjectScale> ;
  rdfs:subClassOf <https://w3id.org/dpv/owl#DataSubjectScale> ;
  dc:contributor _:genid1 ;
  dc:created "2022-06-15"^^xsd:date ;
  ns1:term_status "accepted"@en ;
  skos:definition "Scale of data subjects considered singular i.e. a specific data subject"@en ;
  skos:prefLabel "Singular Scale Of Data Subjects"@en ;
  owl:sameAs <https://w3id.org/dpv#SingularScaleOfDataSubjects>, <https://w3id.org/dpv/dpv-owl#SingularScaleOfDataSubjects> .

<https://w3id.org/dpv/owl#PhysicalAuthorisation>
  a owl:Class, owl:NamedIndividual, <https://w3id.org/dpv/owl#PhysicalMeasure> ;
  rdfs:subClassOf <https://w3id.org/dpv/owl#PhysicalMeasure> ;
  dc:contributor _:genid1 ;
  dc:created "2024-04-14"^^xsd:date ;
  dc:source "NIST SP 800-16"@en ;
  ns1:term_status "accepted"@en ;
  skos:definition "Physical implementation of authorisation e.g. by stamping a visitor pass"@en ;
  skos:prefLabel "Physical Authorisation"@en ;
  owl:sameAs <https://w3id.org/dpv#PhysicalAuthorisation>, <https://w3id.org/dpv/dpv-owl#PhysicalAuthorisation> .

<https://w3id.org/dpv/owl#CustomerManagement>
  a owl:Class, owl:NamedIndividual, <https://w3id.org/dpv/owl#Purpose> ;
  rdfs:subClassOf <https://w3id.org/dpv/owl#Purpose> ;
  dc:contributor _:genid4, _:genid5, _:genid1 ;
  dc:created "2021-09-08"^^xsd:date ;
  ns1:term_status "accepted"@en ;
  skos:definition "Customer Management refers to purposes associated with managing activities related with past, current, and future customers"@en ;
  skos:prefLabel "Customer Management"@en ;
  owl:sameAs <https://w3id.org/dpv#CustomerManagement>, <https://w3id.org/dpv/dpv-owl#CustomerManagement> .

<https://w3id.org/dpv/owl#Right>
  a owl:Class ;
  dc:contributor _:genid4, _:genid5, _:genid1 ;
  dc:created "2020-11-18"^^xsd:date ;
  ns3:example <https://w3id.org/dpv/examples/owl#E0067> ;
  ns1:term_status "accepted"@en ;
  skos:definition "The right(s) applicable, provided, or expected"@en ;
  skos:prefLabel "Right"@en ;
  skos:scopeNote "A 'right' is a legal, social, or ethical principle of freedom or entitlement which dictate the norms regarding what is allowed or owed. Rights as a concept encompass a broad area of norms and entities, and are not specific to Individuals or Data Protection / Privacy. For individual specific rights, see dpv:DataSubjectRight"@en ;
  owl:sameAs <https://w3id.org/dpv#Right>, <https://w3id.org/dpv/dpv-owl#Right> .

<https://w3id.org/dpv/owl#EncryptionInUse>
  a owl:Class, owl:NamedIndividual, <https://w3id.org/dpv/owl#TechnicalMeasure> ;
  rdfs:subClassOf <https://w3id.org/dpv/owl#Encryption> ;
  dc:contributor _:genid1 ;
  dc:created "2022-10-22"^^xsd:date ;
  ns1:term_status "accepted"@en ;
  skos:definition "Encryption of data when it is being used"@en ;
  skos:prefLabel "Encryption in Use"@en ;
  owl:sameAs <https://w3id.org/dpv#EncryptionInUse>, <https://w3id.org/dpv/dpv-owl#EncryptionInUse> .

<https://w3id.org/dpv/owl#ComplianceUnknown>
  a owl:Class, owl:NamedIndividual, <https://w3id.org/dpv/owl#ComplianceStatus> ;
  rdfs:subClassOf <https://w3id.org/dpv/owl#ComplianceStatus> ;
  dc:contributor _:genid1 ;
  dc:created "2022-09-07"^^xsd:date ;
  ns1:term_status "accepted"@en ;
  skos:definition "State where the status of compliance is unknown"@en ;
  skos:prefLabel "Compliance Unknown"@en ;
  owl:sameAs <https://w3id.org/dpv#ComplianceUnknown>, <https://w3id.org/dpv/dpv-owl#ComplianceUnknown> .

odrl:includedIn
  a owl:ObjectProperty, owl:TransitiveProperty, owl:NamedIndividual, skos:Concept ;
  rdfs:domain odrl:Action ;
  rdfs:range odrl:Action ;
  rdfs:isDefinedBy odrl: ;
  rdfs:label "Included In"@en ;
  skos:definition "An Action transitively asserts that another Action that encompasses its operational semantics."@en ;
  skos:note "The purpose is to explicitly assert that the semantics of the referenced instance of an other Action encompasses (includes) the semantics of this instance of Action. The includedIn property is transitive, and as such, the Actions form ancestor relationships."@en .

<https://w3id.org/dpv/owl#RecertificationPolicy>
  a owl:Class, owl:NamedIndividual, <https://w3id.org/dpv/owl#OrganisationalMeasure> ;
  rdfs:subClassOf <https://w3id.org/dpv/owl#Policy> ;
  dc:created "2019-04-05"^^xsd:date ;
  dc:modified "2024-04-14"^^xsd:date ;
  ns1:term_status "accepted"@en ;
  skos:definition "Policy regarding repetition or renewal of existing certification(s)"@en ;
  skos:prefLabel "Recertification Policy"@en ;
  owl:sameAs <https://w3id.org/dpv#RecertificationPolicy>, <https://w3id.org/dpv/dpv-owl#RecertificationPolicy> .

odrl:LeftOperand
  a owl:Class, owl:NamedIndividual, skos:Concept ;
  rdfs:isDefinedBy odrl: ;
  rdfs:label "Left Operand"@en ;
  skos:definition "Left operand for a constraint expression."@en ;
  skos:note "Instances of the LeftOperand class are used as the leftOperand of a Constraint."@en .

<https://w3id.org/dpv/owl#isDeterminedByEntity>
  a owl:ObjectProperty ;
  rdfs:subPropertyOf <https://w3id.org/dpv/owl#hasEntity> ;
  ns2:rangeIncludes <https://w3id.org/dpv/owl#Entity> ;
  dc:contributor _:genid1 ;
  dc:created "2024-05-10"^^xsd:date ;
  ns1:term_status "accepted"@en ;
  skos:definition "Indicates the context is determined by the specified entity"@en ;
  skos:prefLabel "is determined by entity"@en ;
  ns0:rangeIncludes <https://w3id.org/dpv/owl#Entity> ;
  owl:sameAs <https://w3id.org/dpv#isDeterminedByEntity>, <https://w3id.org/dpv/dpv-owl#isDeterminedByEntity> .

<https://w3id.org/dpv/owl#EvaluationOfIndividuals>
  a owl:Class, owl:NamedIndividual, <https://w3id.org/dpv/owl#EvaluationScoring> ;
  rdfs:subClassOf <https://w3id.org/dpv/owl#EvaluationScoring> ;
  dc:contributor _:genid1 ;
  dc:created "2022-10-22"^^xsd:date ;
  dc:modified "2022-11-30"^^xsd:date ;
  dc:source [
    a ns0:WebPage ;
    ns0:name "GDPR Art.4-2" ;
    ns0:url "https://eur-lex.europa.eu/eli/reg/2016/679/art_4/par_2/oj"
  ] ;
  ns1:term_status "accepted"@en ;
  skos:definition "Processing that involves evaluation of individuals"@en ;
  skos:prefLabel "Evaluation of Individuals"@en ;
  owl:sameAs <https://w3id.org/dpv#EvaluationOfIndividuals>, <https://w3id.org/dpv/dpv-owl#EvaluationOfIndividuals> .

<https://w3id.org/dpv/owl#hasDataController>
  a owl:ObjectProperty ;
  rdfs:subPropertyOf <https://w3id.org/dpv/owl#hasEntity> ;
  ns2:rangeIncludes <https://w3id.org/dpv/owl#DataController> ;
  dc:contributor _:genid13, _:genid9, _:genid31, _:genid1, _:genid11 ;
  dc:created "2019-04-04"^^xsd:date ;
  dc:modified "2020-11-04"^^xsd:date ;
  ns1:term_status "accepted"@en ;
  skos:definition "Indicates association with Data Controller"@en ;
  skos:prefLabel "has data controller"@en ;
  ns0:rangeIncludes <https://w3id.org/dpv/owl#DataController> ;
  owl:sameAs <https://w3id.org/dpv#hasDataController>, <https://w3id.org/dpv/dpv-owl#hasDataController> .

odrl:extract
  a owl:NamedIndividual, skos:Concept, odrl:Action ;
  odrl:includedIn odrl:reproduce ;
  rdfs:isDefinedBy odrl: ;
  rdfs:label "Extract"@en ;
  skos:definition "To extract parts of the Asset and to use it as a new Asset."@en ;
  skos:note "A new asset is created and may have very little in common with the original Asset. (Note that the notion of whether or not the change is significant enough to qualify as a new asset is subjective). To the extracted Asset a next policy may be applied."@en ;
  skos:scopeNote "Non-Normative"@en .

<https://w3id.org/dpv/owl#VerifiedData>
  a owl:Class ;
  rdfs:subClassOf <https://w3id.org/dpv/owl#Data> ;
  dc:contributor _:genid1 ;
  dc:created "2022-11-02"^^xsd:date ;
  ns1:term_status "accepted"@en ;
  skos:definition "Data that has been verified in terms of accuracy, consistency, or quality"@en ;
  skos:prefLabel "Verified Data"@en ;
  owl:sameAs <https://w3id.org/dpv#VerifiedData>, <https://w3id.org/dpv/dpv-owl#VerifiedData> .

<https://w3id.org/dpv/owl#Context>
  a owl:Class ;
  dc:contributor _:genid13, _:genid14, _:genid1, _:genid15, _:genid16, _:genid11 ;
  dc:created "2019-04-05"^^xsd:date ;
  dc:modified "2022-06-15"^^xsd:date ;
  ns1:term_status "accepted"@en ;
  skos:definition "Contextually relevant information"@en ;
  skos:prefLabel "Context"@en ;
  skos:scopeNote "Context is a catch-all concept for information of relevance not possible to represent through other core concepts. DPV offers specific contextual concepts such as Necessity, Frequency, and Duration. More can be created by extending Context within use-cases."@en ;
  owl:sameAs <https://w3id.org/dpv#Context>, <https://w3id.org/dpv/dpv-owl#Context> .

odrl:Permission
  a owl:Class, owl:NamedIndividual, skos:Concept ;
  rdfs:subClassOf odrl:Rule ;
  owl:disjointWith odrl:Prohibition ;
  rdfs:isDefinedBy odrl: ;
  rdfs:label "Permission"@en ;
  skos:definition "The ability to perform an Action over an Asset."@en .

<https://w3id.org/dpv/owl#Query>
  a owl:Class, owl:NamedIndividual, <https://w3id.org/dpv/owl#Processing> ;
  rdfs:subClassOf <https://w3id.org/dpv/owl#Consult> ;
  dc:contributor _:genid1 ;
  dc:created "2022-06-15"^^xsd:date ;
  ns1:term_status "accepted"@en ;
  skos:definition "to query or make enquiries over data"@en ;
  skos:prefLabel "Query Data"@en ;
  owl:sameAs <https://w3id.org/dpv#Query>, <https://w3id.org/dpv/dpv-owl#Query> .

<https://eu-upcast.github.io/vocabulary/index-en.html#hasFinishTime>
  a owl:DatatypeProperty ;
  rdfs:subPropertyOf owl:topDataProperty ;
  rdfs:domain odrl:Action ;
  rdfs:range xsd:dateTime ;
  rdfs:label "finish time"@en .

<https://w3id.org/dpv/owl#WithinPhysicalEnvironment>
  a owl:Class, owl:NamedIndividual, <https://w3id.org/dpv/owl#Location> ;
  rdfs:subClassOf <https://w3id.org/dpv/owl#LocalLocation> ;
  dc:contributor _:genid1 ;
  dc:created "2020-10-06"^^xsd:date ;
  ns1:term_status "accepted"@en ;
  skos:definition "Location is local and entirely within a physical environment, such as a room"@en ;
  skos:prefLabel "Within Physical Environment"@en ;
  owl:sameAs <https://w3id.org/dpv#WithinPhysicalEnvironment>, <https://w3id.org/dpv/dpv-owl#WithinPhysicalEnvironment> .

<https://w3id.org/dpv/owl#OrganisationGovernance>
  a owl:Class, owl:NamedIndividual, <https://w3id.org/dpv/owl#Purpose> ;
  rdfs:subClassOf <https://w3id.org/dpv/owl#Purpose> ;
  dc:contributor _:genid4, _:genid1, _:genid6, _:genid21 ;
  dc:created "2021-09-01"^^xsd:date ;
  dc:source [
    a ns0:WebPage ;
    ns0:name "Belgian DPA ROPA Template" ;
    ns0:url "https://www.privacycommission.be/nl/model-voor-een-register-van-de-verwerkingsactiviteiten"
  ] ;
  ns1:term_status "accepted"@en ;
  skos:definition "Purposes associated with conducting activities and functions for governance of an organisation"@en ;
  skos:prefLabel "Organisation Governance"@en ;
  owl:sameAs <https://w3id.org/dpv#OrganisationGovernance>, <https://w3id.org/dpv/dpv-owl#OrganisationGovernance> .

<https://w3id.org/dpv/owl#PublicBenefit>
  a owl:Class, owl:NamedIndividual, <https://w3id.org/dpv/owl#Purpose> ;
  rdfs:subClassOf <https://w3id.org/dpv/owl#Purpose> ;
  dc:contributor _:genid1 ;
  dc:created "2024-02-14"^^xsd:date ;
  ns1:term_status "accepted"@en ;
  skos:definition "Purposes undertaken and intended to provide benefit to public or society"@en ;
  skos:prefLabel "Public Benefit"@en ;
  owl:sameAs <https://w3id.org/dpv#PublicBenefit>, <https://w3id.org/dpv/dpv-owl#PublicBenefit> .

odrl:transform
  a owl:NamedIndividual, skos:Concept, odrl:Action ;
  odrl:includedIn odrl:use ;
  rdfs:isDefinedBy odrl: ;
  rdfs:label "Transform"@en ;
  skos:definition "To convert the Asset into a different format."@en ;
  skos:note "Typically used to convert the Asset into a different format for consumption on/transfer to a third party system."@en ;
  skos:scopeNote "Non-Normative"@en .

<https://w3id.org/dpv/owl#UserInterfacePersonalisation>
  a owl:Class, owl:NamedIndividual, <https://w3id.org/dpv/owl#Purpose> ;
  rdfs:subClassOf <https://w3id.org/dpv/owl#ServicePersonalisation> ;
  dc:contributor _:genid13, _:genid14, _:genid1, _:genid15, _:genid16, _:genid11 ;
  dc:created "2019-04-05"^^xsd:date ;
  ns1:term_status "accepted"@en ;
  skos:definition "Purposes associated with personalisation of interfaces presented to the user"@en ;
  skos:prefLabel "User Interface Personalisation"@en ;
  skos:scopeNote "Examples of user-interface personalisation include changing the language to match the locale"@en ;
  owl:sameAs <https://w3id.org/dpv#UserInterfacePersonalisation>, <https://w3id.org/dpv/dpv-owl#UserInterfacePersonalisation> .

<https://w3id.org/dpv/owl#NoticeLatest>
  a owl:Class, owl:NamedIndividual, <https://w3id.org/dpv/owl#NoticeStatus> ;
  rdfs:subClassOf <https://w3id.org/dpv/owl#NoticeStatus> ;
  dc:contributor _:genid4, _:genid1 ;
  dc:created "2024-12-01"^^xsd:date ;
  ns1:term_status "accepted"@en ;
  skos:definition "Status indicating the notice is currently at its latest iteration"@en ;
  skos:prefLabel "Notice Latest"@en ;
  owl:sameAs <https://w3id.org/dpv#NoticeLatest>, <https://w3id.org/dpv/dpv-owl#NoticeLatest> .

<https://w3id.org/dpv/owl#CredentialManagement>
  a owl:Class, owl:NamedIndividual, <https://w3id.org/dpv/owl#OrganisationalMeasure> ;
  rdfs:subClassOf <https://w3id.org/dpv/owl#AuthorisationProcedure> ;
  dc:contributor _:genid4 ;
  dc:created "2022-06-15"^^xsd:date ;
  ns1:term_status "accepted"@en ;
  skos:definition "Management of credentials and their use in authorisations"@en ;
  skos:prefLabel "Credential Management"@en ;
  owl:sameAs <https://w3id.org/dpv#CredentialManagement>, <https://w3id.org/dpv/dpv-owl#CredentialManagement> .

odrl:absoluteSize
  a owl:NamedIndividual, skos:Concept, odrl:LeftOperand ;
  rdfs:isDefinedBy odrl: ;
  rdfs:label "Absolute Asset Size"@en ;
  skos:definition "Measure(s) of one or two axes for 2D-objects or measure(s) of one to tree axes for 3D-objects of the target Asset."@en ;
  skos:note "Example: The image can be resized in width to a maximum of 1000px."@en ;
  skos:scopeNote "Non-Normative"@en .

<https://w3id.org/dpv/owl#ParentOfHuman>
  a owl:Class, owl:NamedIndividual, <https://w3id.org/dpv/owl#HumanSubject> ;
  rdfs:subClassOf <https://w3id.org/dpv/owl#HumanSubject> ;
  dc:contributor _:genid1 ;
  dc:created "2024-12-17"^^xsd:date ;
  ns1:term_status "accepted"@en ;
  skos:definition "Parent(s) of humans"@en ;
  skos:prefLabel "Parent of Human"@en ;
  owl:sameAs <https://w3id.org/dpv#ParentOfHuman>, <https://w3id.org/dpv/dpv-owl#ParentOfHuman> .

<https://w3id.org/dpv/owl#Intended>
  a owl:Class, owl:NamedIndividual, <https://w3id.org/dpv/owl#IntentionStatus> ;
  rdfs:subClassOf <https://w3id.org/dpv/owl#IntentionStatus> ;
  dc:contributor _:genid4, _:genid1, _:genid25, _:genid6 ;
  dc:created "2024-05-10"^^xsd:date ;
  ns1:term_status "accepted"@en ;
  skos:definition "Status indicating the specified context was intended"@en ;
  skos:prefLabel "Intended"@en ;
  owl:sameAs <https://w3id.org/dpv#Intended>, <https://w3id.org/dpv/dpv-owl#Intended> .

<https://w3id.org/dpv/owl#FulfilmentOfContractualObligation>
  a owl:Class, owl:NamedIndividual, <https://w3id.org/dpv/owl#Purpose> ;
  rdfs:subClassOf <https://w3id.org/dpv/owl#FulfilmentOfObligation> ;
  dc:contributor _:genid4, _:genid1 ;
  dc:created "2022-11-09"^^xsd:date ;
  ns1:term_status "accepted"@en ;
  skos:definition "Purposes associated with carrying out data processing to fulfill a contractual obligation"@en ;
  skos:prefLabel "Fulfilment of Contractual Obligation"@en ;
  owl:sameAs <https://w3id.org/dpv#FulfilmentOfContractualObligation>, <https://w3id.org/dpv/dpv-owl#FulfilmentOfContractualObligation> .

odrl:proximity a owl:DatatypeProperty, owl:NamedIndividual, skos:Concept .
<https://w3id.org/dpv/owl#Anonymise>
  a owl:Class, owl:NamedIndividual, <https://w3id.org/dpv/owl#Processing> ;
  rdfs:subClassOf <https://w3id.org/dpv/owl#Transform> ;
  dc:created "2019-05-07"^^xsd:date ;
  dc:source [
    a ns0:WebPage ;
    ns0:name "SPECIAL Project" ;
    ns0:url "https://specialprivacy.ercim.eu/vocabs/processing"
  ] ;
  ns1:term_status "accepted"@en ;
  skos:definition "to irreversibly alter personal data in such a way that an unique data subject can no longer be identified directly or indirectly or in combination with other data"@en ;
  skos:prefLabel "Anonymise Data"@en ;
  skos:related <https://specialprivacy.ercim.eu/vocabs/processing#Anonymise> ;
  owl:sameAs <https://w3id.org/dpv#Anonymise>, <https://w3id.org/dpv/dpv-owl#Anonymise> .

<https://w3id.org/dpv/owl#SupportEntityDecisionMaking>
  a owl:Class, owl:NamedIndividual, <https://w3id.org/dpv/owl#OrganisationalMeasure> ;
  rdfs:subClassOf <https://w3id.org/dpv/owl#OrganisationalMeasure> ;
  dc:contributor _:genid5, _:genid1 ;
  dc:created "2024-04-14"^^xsd:date ;
  dc:source "DGA 2.15"@en ;
  ns1:term_status "accepted"@en ;
  skos:definition "Supporting entities, including individuals, in making decisions"@en ;
  skos:prefLabel "Support Entity Decision Making"@en ;
  owl:sameAs <https://w3id.org/dpv#SupportEntityDecisionMaking>, <https://w3id.org/dpv/dpv-owl#SupportEntityDecisionMaking> .

<https://w3id.org/dpv/owl#CollectedPersonalData>
  a owl:Class ;
  rdfs:subClassOf <https://w3id.org/dpv/owl#CollectedData>, <https://w3id.org/dpv/owl#PersonalData> ;
  dc:contributor _:genid1 ;
  dc:created "2022-03-30"^^xsd:date ;
  dc:modified "2023-12-10"^^xsd:date ;
  ns3:example <https://w3id.org/dpv/examples/owl#E0046> ;
  ns1:term_status "accepted"@en ;
  skos:definition "Personal Data that has been collected from another source such as the Data Subject"@en ;
  skos:prefLabel "Collected Personal Data"@en ;
  skos:scopeNote "To indicate the source of data, use the DataSource concept with the hasDataSource relation"@en ;
  owl:sameAs <https://w3id.org/dpv#CollectedPersonalData>, <https://w3id.org/dpv/dpv-owl#CollectedPersonalData> .

<https://w3id.org/dpv/owl#hasProcess>
  a owl:ObjectProperty ;
  ns2:rangeIncludes <https://w3id.org/dpv/owl#Process> ;
  dc:contributor _:genid1 ;
  dc:created "2023-12-10"^^xsd:date ;
  ns1:term_status "accepted"@en ;
  skos:definition "Indicates association with a Process"@en ;
  skos:prefLabel "has process"@en ;
  ns0:rangeIncludes <https://w3id.org/dpv/owl#Process> ;
  owl:sameAs <https://w3id.org/dpv#hasProcess>, <https://w3id.org/dpv/dpv-owl#hasProcess> .

<https://w3id.org/dpv/owl#Structure>
  a owl:Class, owl:NamedIndividual, <https://w3id.org/dpv/owl#Processing> ;
  rdfs:subClassOf <https://w3id.org/dpv/owl#Organise> ;
  dc:created "2019-05-07"^^xsd:date ;
  dc:source [
    a ns0:WebPage ;
    ns0:name "GDPR Art.4-2" ;
    ns0:url "https://eur-lex.europa.eu/eli/reg/2016/679/art_4/par_2/oj"
  ] ;
  ns1:term_status "accepted"@en ;
  skos:definition "to arrange data according to a structure"@en ;
  skos:prefLabel "Structure Data"@en ;
  owl:sameAs <https://w3id.org/dpv#Structure>, <https://w3id.org/dpv/dpv-owl#Structure> .

<https://w3id.org/dpv/owl#Download>
  a owl:Class, owl:NamedIndividual, <https://w3id.org/dpv/owl#Processing> ;
  rdfs:subClassOf <https://w3id.org/dpv/owl#Disclose> ;
  dc:contributor _:genid5 ;
  dc:created "2024-04-14"^^xsd:date ;
  dc:source " 2.20"@en, "DGA 2.13"@en ;
  ns1:term_status "accepted"@en ;
  skos:definition "to provide a copy or to receive a copy of data over a network or internet"@en ;
  skos:prefLabel "Download Data"@en ;
  owl:sameAs <https://w3id.org/dpv#Download>, <https://w3id.org/dpv/dpv-owl#Download> .

<https://w3id.org/dpv/owl#hasInvolvement>
  a owl:ObjectProperty ;
  rdfs:subPropertyOf <https://w3id.org/dpv/owl#hasStatus> ;
  ns2:rangeIncludes <https://w3id.org/dpv/owl#InvolvementStatus> ;
  dc:contributor _:genid1 ;
  dc:created "2024-05-10"^^xsd:date ;
  ns1:term_status "accepted"@en ;
  skos:definition "Indicates the involvement status for the specified context"@en ;
  skos:prefLabel "has involvement"@en ;
  ns0:rangeIncludes <https://w3id.org/dpv/owl#InvolvementStatus> ;
  owl:sameAs <https://w3id.org/dpv#hasInvolvement>, <https://w3id.org/dpv/dpv-owl#hasInvolvement> .

<https://w3id.org/dpv/owl#Adult>
  a owl:Class, owl:NamedIndividual, <https://w3id.org/dpv/owl#HumanSubject> ;
  rdfs:subClassOf <https://w3id.org/dpv/owl#HumanSubject> ;
  dc:contributor _:genid4 ;
  dc:created "2022-03-30"^^xsd:date ;
  dc:modified "2024-12-17"^^xsd:date ;
  ns1:term_status "modified"@en ;
  skos:definition "A natural person that is not a child i.e. has attained some legally specified age of adulthood"@en ;
  skos:prefLabel "Adult"@en ;
  owl:sameAs <https://w3id.org/dpv#Adult>, <https://w3id.org/dpv/dpv-owl#Adult> .

odrl:assignee
  a owl:ObjectProperty, owl:NamedIndividual, skos:Concept ;
  rdfs:subPropertyOf odrl:function ;
  rdfs:domain [
    a owl:Class ;
    owl:unionOf (
     odrl:Policy
     odrl:Rule
   )
  ] ;
  rdfs:range odrl:Party ;
  rdfs:isDefinedBy odrl: ;
  rdfs:label "Assignee"@en ;
  skos:definition "The Party is the recipient of the Rule."@en .

<https://w3id.org/dpv/owl#LargeScaleOfDataSubjects>
  a owl:Class, owl:NamedIndividual, <https://w3id.org/dpv/owl#DataSubjectScale> ;
  rdfs:subClassOf <https://w3id.org/dpv/owl#DataSubjectScale> ;
  dc:contributor _:genid1 ;
  dc:created "2022-06-15"^^xsd:date ;
  ns1:term_status "accepted"@en ;
  skos:definition "Scale of data subjects considered large within the context"@en ;
  skos:prefLabel "Large Scale Of Data Subjects"@en ;
  owl:sameAs <https://w3id.org/dpv#LargeScaleOfDataSubjects>, <https://w3id.org/dpv/dpv-owl#LargeScaleOfDataSubjects> .

<https://w3id.org/dpv/owl#RecruitmentApplicationManagement>
  a owl:Class, owl:NamedIndividual, <https://w3id.org/dpv/owl#Purpose> ;
  rdfs:subClassOf <https://w3id.org/dpv/owl#RecruitmentManagement> ;
  dc:created "2024-12-01"^^xsd:date ;
  ns1:term_status "accepted"@en ;
  skos:definition "Purposes associated with managing job applications for recruitment"@en ;
  skos:prefLabel "Recruitment Application Management"@en ;
  owl:sameAs <https://w3id.org/dpv#RecruitmentApplicationManagement>, <https://w3id.org/dpv/dpv-owl#RecruitmentApplicationManagement> .

<https://w3id.org/dpv/owl#PhysicalSecureStorage>
  a owl:Class, owl:NamedIndividual, <https://w3id.org/dpv/owl#PhysicalMeasure> ;
  rdfs:subClassOf <https://w3id.org/dpv/owl#PhysicalMeasure> ;
  dc:contributor _:genid1 ;
  dc:created "2024-04-14"^^xsd:date ;
  dc:source "NIST SP 800-171"@en ;
  ns1:term_status "accepted"@en ;
  skos:definition "Physical protection for storage of information or equipment e.g. secure storage for files"@en ;
  skos:prefLabel "Physical Secure Storage"@en ;
  owl:sameAs <https://w3id.org/dpv#PhysicalSecureStorage>, <https://w3id.org/dpv/dpv-owl#PhysicalSecureStorage> .

odrl:prohibit
  a owl:NamedIndividual, skos:Concept, odrl:ConflictTerm ;
  rdfs:isDefinedBy odrl: ;
  rdfs:label "Prefer Prohibitions"@en ;
  skos:definition "Prohibitions take preference over permissions."@en ;
  skos:note "Used to determine policy conflict outcomes."@en .

<https://w3id.org/dpv/owl#CybersecurityAssessment>
  a owl:Class, owl:NamedIndividual, <https://w3id.org/dpv/owl#OrganisationalMeasure> ;
  rdfs:subClassOf <https://w3id.org/dpv/owl#SecurityAssessment> ;
  dc:contributor _:genid1 ;
  dc:created "2022-08-17"^^xsd:date ;
  dc:source [
    a ns0:WebPage ;
    ns0:name "ENISA 5G Cybersecurity Standards" ;
    ns0:url "https://www.enisa.europa.eu/publications/5g-cybersecurity-standards"
  ] ;
  ns1:term_status "accepted"@en ;
  skos:definition "Assessment of cybersecurity capabilities in terms of vulnerabilities and effectiveness of controls"@en ;
  skos:prefLabel "Cybersecurity Assessment"@en ;
  owl:sameAs <https://w3id.org/dpv#CybersecurityAssessment>, <https://w3id.org/dpv/dpv-owl#CybersecurityAssessment> .

<https://w3id.org/dpv/owl#MediumScaleProcessing>
  a owl:Class, owl:NamedIndividual, <https://w3id.org/dpv/owl#ProcessingScale> ;
  rdfs:subClassOf <https://w3id.org/dpv/owl#ProcessingScale> ;
  dc:contributor _:genid1 ;
  dc:created "2022-09-07"^^xsd:date ;
  ns1:term_status "accepted"@en ;
  skos:definition "Processing that takes place at medium scales (as specified by some criteria)"@en ;
  skos:prefLabel "Medium Scale Processing"@en ;
  owl:sameAs <https://w3id.org/dpv#MediumScaleProcessing>, <https://w3id.org/dpv/dpv-owl#MediumScaleProcessing> .

<https://w3id.org/dpv/owl#PrivacyByDesign>
  a owl:Class, owl:NamedIndividual, <https://w3id.org/dpv/owl#OrganisationalMeasure> ;
  rdfs:subClassOf <https://w3id.org/dpv/owl#GuidelinesPrinciple> ;
  dc:contributor _:genid9, _:genid10, _:genid1, _:genid11 ;
  dc:created "2019-04-05"^^xsd:date ;
  ns1:term_status "accepted"@en ;
  skos:definition "Practices regarding incorporating data protection and privacy in the design of information and services (synonymous with Data Protection by Design)"@en ;
  skos:prefLabel "Privacy by Design"@en ;
  owl:sameAs <https://w3id.org/dpv#PrivacyByDesign>, <https://w3id.org/dpv/dpv-owl#PrivacyByDesign> .

<https://w3id.org/dpv/owl#Guideline>
  a owl:Class, owl:NamedIndividual, <https://w3id.org/dpv/owl#OrganisationalMeasure> ;
  rdfs:subClassOf <https://w3id.org/dpv/owl#GuidelinesPrinciple> ;
  dc:contributor _:genid1 ;
  dc:created "2024-05-12"^^xsd:date ;
  ns1:term_status "accepted"@en ;
  skos:definition "Practices that specify how activities must be conducted"@en ;
  skos:prefLabel "Guideline"@en ;
  owl:sameAs <https://w3id.org/dpv#Guideline>, <https://w3id.org/dpv/dpv-owl#Guideline> .

<https://w3id.org/dpv/owl#Remove>
  a owl:Class, owl:NamedIndividual, <https://w3id.org/dpv/owl#Processing> ;
  rdfs:subClassOf <https://w3id.org/dpv/owl#Processing> ;
  dc:created "2019-05-07"^^xsd:date ;
  dc:source [
    a ns0:WebPage ;
    ns0:name "GDPR Art.4-2" ;
    ns0:url "https://eur-lex.europa.eu/eli/reg/2016/679/art_4/par_2/oj"
  ] ;
  ns1:term_status "accepted"@en ;
  skos:definition "to destruct or erase data"@en ;
  skos:prefLabel "Remove Data"@en ;
  owl:sameAs <https://w3id.org/dpv#Remove>, <https://w3id.org/dpv/dpv-owl#Remove> .

<https://w3id.org/dpv/owl#ContractApproved>
  a owl:Class, owl:NamedIndividual, <https://w3id.org/dpv/owl#ContractPreparationStatus> ;
  rdfs:subClassOf <https://w3id.org/dpv/owl#ContractPreparationStatus> ;
  dc:contributor _:genid4, _:genid1, _:genid17 ;
  dc:created "2025-01-09"^^xsd:date ;
  ns1:term_status "accepted"@en ;
  skos:definition "Status representing contract has been approved and can be used for signing"@en ;
  skos:prefLabel "Contract Approved"@en ;
  owl:sameAs <https://w3id.org/dpv#ContractApproved>, <https://w3id.org/dpv/dpv-owl#ContractApproved> .

cc:SourceCode
  a owl:NamedIndividual, skos:Concept, odrl:Action ;
  odrl:includedIn odrl:use ;
  rdfs:isDefinedBy odrl: ;
  rdfs:label "Source Code"@en ;
  skos:definition "Source code (the preferred form for making modifications) must be provided when exercising some rights granted by the license."@en ;
  skos:note "This term is defined by Creative Commons."@en ;
  skos:scopeNote "Non-Normative"@en .

odrl:#partyRolesCommon
  a owl:NamedIndividual, skos:Collection ;
  skos:member odrl:attributedParty, odrl:attributingParty, odrl:compensatedParty, odrl:compensatingParty, odrl:consentedParty, odrl:consentingParty, odrl:contractedParty, odrl:contractingParty, odrl:informedParty, odrl:informingParty, odrl:trackedParty, odrl:trackingParty ;
  skos:prefLabel "Party Functions"@en ;
  skos:scopeNote "ODRL Common Vocabulary Terms"@en .

<https://w3id.org/dpv/owl#ContractTemporarilySuspended>
  a owl:Class, owl:NamedIndividual, <https://w3id.org/dpv/owl#ContractPerformanceStatus> ;
  rdfs:subClassOf <https://w3id.org/dpv/owl#ContractPerformanceStatus> ;
  dc:contributor _:genid4, _:genid1, _:genid17 ;
  dc:created "2025-01-09"^^xsd:date ;
  ns1:term_status "accepted"@en ;
  skos:definition "Status representing contract that has been temporarily suspended through mutual agreement or by some parties"@en ;
  skos:prefLabel "Contract Temporarily Suspended"@en ;
  owl:sameAs <https://w3id.org/dpv#ContractTemporarilySuspended>, <https://w3id.org/dpv/dpv-owl#ContractTemporarilySuspended> .

<https://w3id.org/dpv/owl#ObservedData>
  a owl:Class ;
  rdfs:subClassOf <https://w3id.org/dpv/owl#CollectedData> ;
  dc:created "2023-12-10"^^xsd:date ;
  ns1:term_status "accepted"@en ;
  skos:definition "Data that has been obtained through observations of a source"@en ;
  skos:prefLabel "Observed Data"@en ;
  owl:sameAs <https://w3id.org/dpv#ObservedData>, <https://w3id.org/dpv/dpv-owl#ObservedData> .

skos:related a owl:AnnotationProperty .
<https://w3id.org/dpv/owl#StaffTraining>
  a owl:Class, owl:NamedIndividual, <https://w3id.org/dpv/owl#OrganisationalMeasure> ;
  rdfs:subClassOf <https://w3id.org/dpv/owl#OrganisationalMeasure> ;
  dc:contributor _:genid9, _:genid10, _:genid1, _:genid11 ;
  dc:created "2019-04-05"^^xsd:date ;
  ns3:example <https://w3id.org/dpv/examples/owl#E0021> ;
  ns1:term_status "accepted"@en ;
  skos:definition "Practices and policies regarding training of staff members"@en ;
  skos:prefLabel "Staff Training"@en ;
  owl:sameAs <https://w3id.org/dpv#StaffTraining>, <https://w3id.org/dpv/dpv-owl#StaffTraining> .

odrl:version
  a owl:NamedIndividual, skos:Concept, odrl:LeftOperand ;
  rdfs:isDefinedBy odrl: ;
  rdfs:label "Version"@en ;
  skos:definition "The version of the target Asset."@en ;
  skos:note "Example: Single Paperback or Multiple Issues or version 2.0 or higher."@en ;
  skos:scopeNote "Non-Normative"@en .

<https://w3id.org/dpv/owl#hasScope>
  a owl:ObjectProperty ;
  ns2:rangeIncludes <https://w3id.org/dpv/owl#Scope> ;
  dc:contributor _:genid1 ;
  dc:created "2022-06-15"^^xsd:date ;
  ns1:term_status "accepted"@en ;
  skos:definition "Indicates the scope of specified concept or context"@en ;
  skos:prefLabel "has scope"@en ;
  ns0:rangeIncludes <https://w3id.org/dpv/owl#Scope> ;
  owl:sameAs <https://w3id.org/dpv#hasScope>, <https://w3id.org/dpv/dpv-owl#hasScope> .

odrl:gteq
  a owl:NamedIndividual, skos:Concept, odrl:Operator ;
  rdfs:isDefinedBy odrl: ;
  rdfs:label "Greater than or equal to"@en ;
  skos:definition "Indicating that a given value is greater than or equal to the right operand of the Constraint."@en .

<https://w3id.org/dpv/owl#DerivedData>
  a owl:Class ;
  rdfs:subClassOf <https://w3id.org/dpv/owl#Data> ;
  dc:created "2023-12-10"^^xsd:date ;
  ns1:term_status "accepted"@en ;
  skos:definition "Data that has been obtained through derivations of other data"@en ;
  skos:prefLabel "Derived Data"@en ;
  owl:sameAs <https://w3id.org/dpv#DerivedData>, <https://w3id.org/dpv/dpv-owl#DerivedData> .

<https://w3id.org/dpv/owl#ControllerProcessorAgreement>
  a owl:Class, owl:NamedIndividual, <https://w3id.org/dpv/owl#LegalBasis>, <https://w3id.org/dpv/owl#LegalMeasure> ;
  rdfs:subClassOf <https://w3id.org/dpv/owl#DataProcessorContract> ;
  dc:contributor _:genid4, _:genid5, _:genid1, _:genid17, _:genid6 ;
  dc:created "2022-01-26"^^xsd:date ;
  dc:modified "2024-08-27"^^xsd:date ;
  ns3:example <https://w3id.org/dpv/examples/owl#E0024> ;
  ns1:term_status "modified"@en ;
  skos:definition "An agreement outlining conditions, criteria, obligations, responsibilities, and specifics for carrying out processing of data between a Data Controller and a Data Processor"@en ;
  skos:prefLabel "Controller-Processor Agreement"@en ;
  owl:sameAs <https://w3id.org/dpv#ControllerProcessorAgreement>, <https://w3id.org/dpv/dpv-owl#ControllerProcessorAgreement> .

<https://w3id.org/dpv/owl#ServiceUsageAnalytics>
  a owl:Class, owl:NamedIndividual, <https://w3id.org/dpv/owl#Purpose> ;
  rdfs:subClassOf <https://w3id.org/dpv/owl#ServiceProvision> ;
  dc:contributor _:genid4, _:genid5, _:genid1 ;
  dc:created "2020-11-04"^^xsd:date ;
  dc:modified "2022-10-05"^^xsd:date ;
  ns1:term_status "accepted"@en ;
  skos:definition "Purposes associated with conducting analysis and reporting related to usage of services or products"@en ;
  skos:prefLabel "Service Usage Analytics"@en ;
  skos:scopeNote "Was \"UsageAnalytics\", prefixed with Service to better reflect scope"@en ;
  owl:sameAs <https://w3id.org/dpv#ServiceUsageAnalytics>, <https://w3id.org/dpv/dpv-owl#ServiceUsageAnalytics> .

<https://w3id.org/dpv/owl#VendorSelectionAssessment>
  a owl:Class, owl:NamedIndividual, <https://w3id.org/dpv/owl#Purpose> ;
  rdfs:subClassOf <https://w3id.org/dpv/owl#VendorManagement> ;
  dc:contributor _:genid4, _:genid1, _:genid6, _:genid21 ;
  dc:created "2021-09-01"^^xsd:date ;
  dc:source [
    a ns0:WebPage ;
    ns0:name "Belgian DPA ROPA Template" ;
    ns0:url "https://www.privacycommission.be/nl/model-voor-een-register-van-de-verwerkingsactiviteiten"
  ] ;
  ns1:term_status "accepted"@en ;
  skos:definition "Purposes associated with managing selection, assessment, and evaluation related to vendors"@en ;
  skos:prefLabel "Vendor Selection Assessment"@en ;
  owl:sameAs <https://w3id.org/dpv#VendorSelectionAssessment>, <https://w3id.org/dpv/dpv-owl#VendorSelectionAssessment> .

<https://w3id.org/dpv/owl#MemberPartnerManagement>
  a owl:Class, owl:NamedIndividual, <https://w3id.org/dpv/owl#Purpose> ;
  rdfs:subClassOf <https://w3id.org/dpv/owl#OrganisationGovernance> ;
  dc:contributor _:genid4, _:genid1, _:genid6, _:genid21 ;
  dc:created "2021-09-01"^^xsd:date ;
  dc:source [
    a ns0:WebPage ;
    ns0:name "Belgian DPA ROPA Template" ;
    ns0:url "https://www.privacycommission.be/nl/model-voor-een-register-van-de-verwerkingsactiviteiten"
  ] ;
  ns1:term_status "accepted"@en ;
  skos:definition "Purposes associated with maintaining a registry of shareholders, members, or partners for governance, administration, and management functions"@en ;
  skos:prefLabel "Members and Partners Management"@en ;
  owl:sameAs <https://w3id.org/dpv#MemberPartnerManagement>, <https://w3id.org/dpv/dpv-owl#MemberPartnerManagement> .

odrl:attributingParty
  a owl:ObjectProperty, owl:NamedIndividual, skos:Concept ;
  rdfs:subPropertyOf odrl:function ;
  rdfs:isDefinedBy odrl: ;
  rdfs:label "Attributing Party"@en ;
  skos:definition "The Party who undertakes the attribution."@en ;
  skos:note "Maybe specified as part of the attribute action."@en ;
  skos:scopeNote "Non-Normative"@en .

<https://w3id.org/dpv/owl#hasServiceProvider>
  a owl:ObjectProperty ;
  rdfs:subPropertyOf <https://w3id.org/dpv/owl#hasEntity> ;
  ns2:domainIncludes <https://w3id.org/dpv/owl#Service> ;
  ns2:rangeIncludes <https://w3id.org/dpv/owl#ServiceProvider> ;
  dc:contributor _:genid1 ;
  dc:created "2024-04-20"^^xsd:date ;
  ns1:term_status "accepted"@en ;
  skos:definition "Indicates the entity that provides the associated service"@en ;
  skos:prefLabel "has service provider"@en ;
  ns0:domainIncludes <https://w3id.org/dpv/owl#Service> ;
  ns0:rangeIncludes <https://w3id.org/dpv/owl#ServiceProvider> ;
  owl:sameAs <https://w3id.org/dpv#hasServiceProvider>, <https://w3id.org/dpv/dpv-owl#hasServiceProvider> .

<https://w3id.org/dpv/owl#MediumScaleOfDataSubjects>
  a owl:Class, owl:NamedIndividual, <https://w3id.org/dpv/owl#DataSubjectScale> ;
  rdfs:subClassOf <https://w3id.org/dpv/owl#DataSubjectScale> ;
  dc:contributor _:genid4, _:genid1, _:genid6 ;
  dc:created "2022-06-15"^^xsd:date ;
  ns1:term_status "accepted"@en ;
  skos:definition "Scale of data subjects considered medium i.e. neither large nor small within the context"@en ;
  skos:prefLabel "Medium Scale Of Data Subjects"@en ;
  owl:sameAs <https://w3id.org/dpv#MediumScaleOfDataSubjects>, <https://w3id.org/dpv/dpv-owl#MediumScaleOfDataSubjects> .

odrl:event
  a owl:NamedIndividual, skos:Concept, odrl:LeftOperand ;
  rdfs:isDefinedBy odrl: ;
  rdfs:label "Event"@en ;
  skos:definition "An identified event setting a context for exercising the action of the Rule."@en ;
  skos:note "Events are temporal periods of time, and operators can be used to signal before (lt), during (eq) or after (gt) the event. <br />Example: May be taken during the “FIFA World Cup 2020” only."@en ;
  skos:scopeNote "Non-Normative"@en .

odrl:core
  a owl:Thing, owl:NamedIndividual, skos:Concept ;
  rdfs:isDefinedBy odrl: ;
  rdfs:label "ODRL Core Profile"@en ;
  skos:definition "Identifier for the ODRL Core Profile"@en .

<https://w3id.org/dpv/owl#hasRelationWithDataSubject>
  a owl:ObjectProperty ;
  rdfs:subPropertyOf <https://w3id.org/dpv/owl#hasEntity> ;
  ns2:domainIncludes <https://w3id.org/dpv/owl#Entity> ;
  dc:contributor _:genid4, _:genid1, _:genid17, _:genid6 ;
  dc:created "2022-06-21"^^xsd:date ;
  ns1:term_status "accepted"@en ;
  skos:definition "Indicates the relation between specified Entity and Data Subject"@en ;
  skos:prefLabel "has relation with data subject"@en ;
  ns0:domainIncludes <https://w3id.org/dpv/owl#Entity> ;
  owl:sameAs <https://w3id.org/dpv#hasRelationWithDataSubject>, <https://w3id.org/dpv/dpv-owl#hasRelationWithDataSubject> .

<https://w3id.org/dpv/owl#hasRiskLevel>
  a owl:ObjectProperty ;
  ns2:domainIncludes <https://w3id.org/dpv/owl#Risk> ;
  ns2:rangeIncludes <https://w3id.org/dpv/owl#RiskLevel> ;
  dc:contributor _:genid4, _:genid1, _:genid17, _:genid6 ;
  dc:created "2022-07-20"^^xsd:date ;
  ns3:example <https://w3id.org/dpv/examples/owl#E0068>, <https://w3id.org/dpv/examples/owl#E0071> ;
  ns1:term_status "accepted"@en ;
  skos:definition "Indicates the associated risk level associated with a risk"@en ;
  skos:prefLabel "has risk level"@en ;
  ns0:domainIncludes <https://w3id.org/dpv/owl#Risk> ;
  ns0:rangeIncludes <https://w3id.org/dpv/owl#RiskLevel> ;
  owl:sameAs <https://w3id.org/dpv#hasRiskLevel>, <https://w3id.org/dpv/dpv-owl#hasRiskLevel> .

<https://w3id.org/dpv/owl#SecretSharingSchemes>
  a owl:Class, owl:NamedIndividual, <https://w3id.org/dpv/owl#TechnicalMeasure> ;
  rdfs:subClassOf <https://w3id.org/dpv/owl#CryptographicMethods> ;
  dc:contributor _:genid1 ;
  dc:created "2022-08-17"^^xsd:date ;
  dc:source [
    a ns0:WebPage ;
    ns0:name "ENISA Data Pseudonymisation: Advanced Techniques and Use Cases" ;
    ns0:url "https://www.enisa.europa.eu/publications/data-pseudonymisation-advanced-techniques-and-use-cases"
  ] ;
  ns1:term_status "accepted"@en ;
  skos:definition "Use of secret sharing schemes where the secret can only be reconstructed through combination of sufficient number of individuals"@en ;
  skos:prefLabel "Secret Sharing Schemes"@en ;
  owl:sameAs <https://w3id.org/dpv#SecretSharingSchemes>, <https://w3id.org/dpv/dpv-owl#SecretSharingSchemes> .

odrl:obtainConsent
  a owl:NamedIndividual, skos:Concept, odrl:Action ;
  odrl:includedIn odrl:use ;
  rdfs:isDefinedBy odrl: ;
  rdfs:label "Obtain Consent"@en ;
  skos:definition "To obtain verifiable consent to perform the requested action in relation to the Asset."@en ;
  skos:note "May be used as a Duty to ensure that the Assigner or a Party is authorized to approve such actions on a case-by-case basis. May link to a Party with the role “consentingParty” function."@en ;
  skos:scopeNote "Non-Normative"@en .

<https://w3id.org/dpv/owl#Required>
  a owl:Class, owl:NamedIndividual, <https://w3id.org/dpv/owl#Necessity> ;
  rdfs:subClassOf <https://w3id.org/dpv/owl#Necessity> ;
  dc:contributor _:genid4, _:genid5, _:genid1, _:genid17, _:genid6 ;
  dc:created "2022-02-13"^^xsd:date ;
  ns1:term_status "accepted"@en ;
  skos:definition "Indication of 'required' or 'necessary'"@en ;
  skos:prefLabel "Required"@en ;
  owl:sameAs <https://w3id.org/dpv#Required>, <https://w3id.org/dpv/dpv-owl#Required> .

<https://w3id.org/dpv/owl#hasImportance>
  a owl:ObjectProperty ;
  ns2:rangeIncludes <https://w3id.org/dpv/owl#Importance> ;
  dc:contributor _:genid1 ;
  dc:created "2024-04-13"^^xsd:date ;
  ns1:term_status "accepted"@en ;
  skos:definition "Indicates the importance for specified context or criteria"@en ;
  skos:prefLabel "has importance"@en ;
  ns0:rangeIncludes <https://w3id.org/dpv/owl#Importance> ;
  owl:sameAs <https://w3id.org/dpv#hasImportance>, <https://w3id.org/dpv/dpv-owl#hasImportance> .

<https://w3id.org/dpv/owl#ZeroKnowledgeAuthentication>
  a owl:Class, owl:NamedIndividual, <https://w3id.org/dpv/owl#TechnicalMeasure> ;
  rdfs:subClassOf <https://w3id.org/dpv/owl#AuthenticationProtocols>, <https://w3id.org/dpv/owl#CryptographicMethods> ;
  dc:contributor _:genid1 ;
  dc:created "2022-08-17"^^xsd:date ;
  dc:source [
    a ns0:WebPage ;
    ns0:name "ENISA Data Protection Engineering" ;
    ns0:url "https://www.enisa.europa.eu/publications/data-protection-engineering"
  ] ;
  ns1:term_status "accepted"@en ;
  skos:definition "Authentication using Zero-Knowledge proofs"@en ;
  skos:prefLabel "Zero Knowledge Authentication"@en ;
  owl:sameAs <https://w3id.org/dpv#ZeroKnowledgeAuthentication>, <https://w3id.org/dpv/dpv-owl#ZeroKnowledgeAuthentication> .

<https://w3id.org/dpv/owl#IntrusionDetectionSystem>
  a owl:Class, owl:NamedIndividual, <https://w3id.org/dpv/owl#TechnicalMeasure> ;
  rdfs:subClassOf <https://w3id.org/dpv/owl#SecurityMethod> ;
  dc:contributor _:genid1 ;
  dc:created "2022-08-17"^^xsd:date ;
  dc:source [
    a ns0:WebPage ;
    ns0:name "ENISA Reference Incident Classification Taxonomy 2018" ;
    ns0:url "https://www.enisa.europa.eu/publications/reference-incident-classification-taxonomy/"
  ] ;
  ns1:term_status "accepted"@en ;
  skos:definition "Use of measures to detect intrusions and other unauthorised attempts to gain access to a system"@en ;
  skos:prefLabel "Intrusion Detection System"@en ;
  owl:sameAs <https://w3id.org/dpv#IntrusionDetectionSystem>, <https://w3id.org/dpv/dpv-owl#IntrusionDetectionSystem> .

odrl:lt
  a owl:NamedIndividual, skos:Concept, odrl:Operator ;
  rdfs:isDefinedBy odrl: ;
  rdfs:label "Less than"@en ;
  skos:definition "Indicating that a given value is less than the right operand of the Constraint."@en .

<https://w3id.org/dpv/owl#Employee>
  a owl:Class, owl:NamedIndividual, <https://w3id.org/dpv/owl#HumanSubject> ;
  rdfs:subClassOf <https://w3id.org/dpv/owl#HumanSubject> ;
  dc:contributor _:genid4, _:genid5, _:genid1, _:genid17, _:genid6 ;
  dc:created "2022-04-06"^^xsd:date ;
  dc:modified "2024-12-17"^^xsd:date ;
  ns1:term_status "modified"@en ;
  skos:definition "Humans that are employees"@en ;
  skos:prefLabel "Employee"@en ;
  owl:sameAs <https://w3id.org/dpv#Employee>, <https://w3id.org/dpv/dpv-owl#Employee> .

cc:Attribution
  a owl:NamedIndividual, skos:Concept, odrl:Action ;
  odrl:includedIn odrl:use ;
  rdfs:isDefinedBy odrl: ;
  rdfs:label "Attribution"@en ;
  skos:definition "Credit be given to copyright holder and/or author."@en ;
  skos:note "This term is defined by Creative Commons."@en ;
  skos:scopeNote "Non-Normative"@en .

<https://w3id.org/dpv/owl#CannotObjectToProcess>
  a owl:Class, owl:NamedIndividual, <https://w3id.org/dpv/owl#EntityNonPermissiveInvolvement> ;
  rdfs:subClassOf <https://w3id.org/dpv/owl#EntityNonPermissiveInvolvement> ;
  dc:contributor _:genid1, _:genid25, _:genid19 ;
  dc:created "2024-05-11"^^xsd:date ;
  ns1:term_status "accepted"@en ;
  skos:definition "Involvement where entity cannot object to process of specified context"@en ;
  skos:prefLabel "Cannot Object to Process"@en ;
  owl:sameAs <https://w3id.org/dpv#CannotObjectToProcess>, <https://w3id.org/dpv/dpv-owl#CannotObjectToProcess> .

<https://w3id.org/dpv/owl#EnforceSecurity>
  a owl:Class, owl:NamedIndividual, <https://w3id.org/dpv/owl#Purpose> ;
  rdfs:subClassOf <https://w3id.org/dpv/owl#Purpose> ;
  dc:contributor _:genid13, _:genid14, _:genid1, _:genid15, _:genid16, _:genid11 ;
  dc:created "2019-04-05"^^xsd:date ;
  ns1:term_status "accepted"@en ;
  skos:definition "Purposes associated with ensuring and enforcing security for data, personnel, or other related matters"@en ;
  skos:prefLabel "Enforce Security"@en ;
  skos:scopeNote "Was previous \"Security\". Prefixed to distinguish from TechOrg measures."@en ;
  owl:sameAs <https://w3id.org/dpv#EnforceSecurity>, <https://w3id.org/dpv/dpv-owl#EnforceSecurity> .

<https://w3id.org/dpv/owl#ReviewProcedure>
  a owl:Class, owl:NamedIndividual, <https://w3id.org/dpv/owl#OrganisationalMeasure> ;
  rdfs:subClassOf <https://w3id.org/dpv/owl#GovernanceProcedures> ;
  dc:contributor _:genid4, _:genid1 ;
  dc:created "2022-10-22"^^xsd:date ;
  ns1:term_status "accepted"@en ;
  skos:definition "A procedure or process that reviews the correctness and validity of other procedures and policies e.g. to ensure continued validity, adequacy for intended purposes, and conformance of processes with findings"@en ;
  skos:prefLabel "Review Procedure"@en ;
  owl:sameAs <https://w3id.org/dpv#ReviewProcedure>, <https://w3id.org/dpv/dpv-owl#ReviewProcedure> .

<https://w3id.org/dpv/owl#WithdrawingFromProcess>
  a owl:Class, owl:NamedIndividual, <https://w3id.org/dpv/owl#EntityPermissiveInvolvement> ;
  rdfs:subClassOf <https://w3id.org/dpv/owl#EntityPermissiveInvolvement> ;
  dc:contributor _:genid1, _:genid25, _:genid19 ;
  dc:created "2024-05-11"^^xsd:date ;
  ns1:term_status "accepted"@en ;
  skos:definition "Involvement where entity can withdraw a previously given assent from specified context"@en ;
  skos:prefLabel "Withdrawing from Process"@en ;
  owl:sameAs <https://w3id.org/dpv#WithdrawingFromProcess>, <https://w3id.org/dpv/dpv-owl#WithdrawingFromProcess> .

<https://w3id.org/dpv/owl#HugeDataVolume>
  a owl:Class, owl:NamedIndividual, <https://w3id.org/dpv/owl#DataVolume> ;
  rdfs:subClassOf <https://w3id.org/dpv/owl#DataVolume> ;
  dc:contributor _:genid1 ;
  dc:created "2022-06-15"^^xsd:date ;
  ns1:term_status "accepted"@en ;
  skos:definition "Data volume that is considered huge or more than large within the context"@en ;
  skos:prefLabel "Huge Data Volume"@en ;
  owl:sameAs <https://w3id.org/dpv#HugeDataVolume>, <https://w3id.org/dpv/dpv-owl#HugeDataVolume> .

<https://w3id.org/dpv/owl#TrackingByFirstParty>
  a owl:Class, owl:NamedIndividual, <https://w3id.org/dpv/owl#Processing> ;
  rdfs:subClassOf <https://w3id.org/dpv/owl#Tracking> ;
  dc:contributor _:genid1 ;
  dc:created "2024-12-17"^^xsd:date ;
  ns1:term_status "accepted"@en ;
  skos:definition "to perform tracking where the performing entity is a first party within the context"@en ;
  skos:prefLabel "Tracking by First Party"@en ;
  skos:scopeNote "This concept does not strictly only specify the processing operation, but also the relation of the individual with the implementing entity. These concepts may change in the future based on discussions around how to express First and Third Party."@en ;
  owl:sameAs <https://w3id.org/dpv#TrackingByFirstParty>, <https://w3id.org/dpv/dpv-owl#TrackingByFirstParty> .

<https://w3id.org/dpv/owl#GraphicalNotice>
  a owl:Class, owl:NamedIndividual, <https://w3id.org/dpv/owl#OrganisationalMeasure> ;
  rdfs:subClassOf <https://w3id.org/dpv/owl#Notice> ;
  dc:created "2024-08-17"^^xsd:date ;
  dc:source [
    a ns0:WebPage ;
    ns0:name "ICO - What methods can we use to provide privacy information?" ;
    ns0:url "https://ico.org.uk/for-organisations/uk-gdpr-guidance-and-resources/individual-rights/the-right-to-be-informed/what-methods-can-we-use-to-provide-privacy-information/"
  ] ;
  ns1:term_status "accepted"@en ;
  skos:definition "A notice that uses graphical elements such as visualisations and icons"@en ;
  skos:prefLabel "Graphical Notice"@en ;
  owl:sameAs <https://w3id.org/dpv#GraphicalNotice>, <https://w3id.org/dpv/dpv-owl#GraphicalNotice> .

odrl:read
  a owl:NamedIndividual, skos:Concept, odrl:Action ;
  odrl:includedIn odrl:use ;
  rdfs:isDefinedBy odrl: ;
  rdfs:label "Read"@en ;
  skos:definition "To obtain data from the Asset."@en ;
  skos:note "For example, the ability to read a record from a database (the Asset)."@en ;
  skos:scopeNote "Non-Normative"@en .

<https://w3id.org/dpv/owl#PhysicalAccessControlMethod>
  a owl:Class, owl:NamedIndividual, <https://w3id.org/dpv/owl#PhysicalMeasure> ;
  rdfs:subClassOf <https://w3id.org/dpv/owl#AccessControlMethod> ;
  dc:contributor _:genid4 ;
  dc:created "2022-06-15"^^xsd:date ;
  dc:source "NIST SP 800-12"@en ;
  ns1:term_status "accepted"@en ;
  skos:definition "Access control applied for physical access e.g. premises or equipment"@en ;
  skos:prefLabel "Physical Access Control Method"@en ;
  owl:sameAs <https://w3id.org/dpv#PhysicalAccessControlMethod>, <https://w3id.org/dpv/dpv-owl#PhysicalAccessControlMethod> .

<https://w3id.org/dpv/owl#ContractualClauseFulfilmentStatus>
  a owl:Class ;
  rdfs:subClassOf <https://w3id.org/dpv/owl#ContractStatus> ;
  dc:created "2024-08-27"^^xsd:date ;
  ns1:term_status "accepted"@en ;
  skos:definition "Status associated with fulfilment of a contractual clause"@en ;
  skos:prefLabel "Contractual Clause Fulfilment Status"@en ;
  owl:sameAs <https://w3id.org/dpv#ContractualClauseFulfilmentStatus>, <https://w3id.org/dpv/dpv-owl#ContractualClauseFulfilmentStatus> .

<https://w3id.org/dpv/owl#RuleUnfulfilled>
  a owl:Class, owl:NamedIndividual, <https://w3id.org/dpv/owl#RuleFulfilmentStatus> ;
  rdfs:subClassOf <https://w3id.org/dpv/owl#RuleFulfilmentStatus> ;
  dc:contributor _:genid1 ;
  dc:created "2024-09-10"^^xsd:date ;
  ns1:term_status "accepted"@en ;
  skos:definition "Status indicating a rule has not been fulfilled nor violated"@en ;
  skos:prefLabel "Rule Unfulfilled"@en ;
  owl:sameAs <https://w3id.org/dpv#RuleUnfulfilled>, <https://w3id.org/dpv/dpv-owl#RuleUnfulfilled> .

<https://w3id.org/dpv/owl#Profiling>
  a owl:Class, owl:NamedIndividual, <https://w3id.org/dpv/owl#Processing> ;
  rdfs:subClassOf <https://w3id.org/dpv/owl#Use> ;
  dc:created "2019-05-07"^^xsd:date ;
  dc:source [
    a ns0:WebPage ;
    ns0:name "GDPR Art.4-2" ;
    ns0:url "https://eur-lex.europa.eu/eli/reg/2016/679/art_4/par_2/oj"
  ] ;
  ns3:example <https://w3id.org/dpv/examples/owl#E0075> ;
  ns1:term_status "accepted"@en ;
  skos:definition "to create a profile that describes or represents a person"@en ;
  skos:prefLabel "Profiling"@en ;
  owl:sameAs <https://w3id.org/dpv#Profiling>, <https://w3id.org/dpv/dpv-owl#Profiling> .

<https://w3id.org/dpv/owl#DataProcessorContract>
  a owl:Class, owl:NamedIndividual, <https://w3id.org/dpv/owl#LegalBasis> ;
  rdfs:subClassOf <https://w3id.org/dpv/owl#DataProcessingAgreement> ;
  dc:created "2023-12-10"^^xsd:date ;
  dc:modified "2024-08-27"^^xsd:date ;
  ns1:term_status "sunset"@en ;
  skos:definition "Creation, completion, fulfilment, or performance of a contract, with the Data Controller and Data Processor as parties, and involving specified processing of data or technologies. NOTE: This concept is being deprecated - use dpv:ControllerProcessorAgreement which has a more explicit definition of the entities involved and the intent of the contract"@en ;
  skos:prefLabel "Data Processor Contract"@en ;
  owl:sameAs <https://w3id.org/dpv#DataProcessorContract>, <https://w3id.org/dpv/dpv-owl#DataProcessorContract> .

<https://w3id.org/dpv/owl#RequestRequiresAction>
  a owl:Class, owl:NamedIndividual, <https://w3id.org/dpv/owl#RequestStatus> ;
  rdfs:subClassOf <https://w3id.org/dpv/owl#RequestStatus> ;
  dc:contributor _:genid1 ;
  dc:created "2022-11-30"^^xsd:date ;
  ns1:term_status "accepted"@en ;
  skos:definition "State of a request requiring an action to be performed from another party"@en ;
  skos:prefLabel "Request Requires Action"@en ;
  owl:sameAs <https://w3id.org/dpv#RequestRequiresAction>, <https://w3id.org/dpv/dpv-owl#RequestRequiresAction> .

<https://w3id.org/dpv/owl#InferredData>
  a owl:Class ;
  rdfs:subClassOf <https://w3id.org/dpv/owl#DerivedData> ;
  dc:created "2023-12-10"^^xsd:date ;
  ns1:term_status "accepted"@en ;
  skos:definition "Data that has been obtained through inferences of other data"@en ;
  skos:prefLabel "Inferred Data"@en ;
  owl:sameAs <https://w3id.org/dpv#InferredData>, <https://w3id.org/dpv/dpv-owl#InferredData> .

<https://w3id.org/dpv/owl#NoticeGenerated>
  a owl:Class, owl:NamedIndividual, <https://w3id.org/dpv/owl#NoticeStatus> ;
  rdfs:subClassOf <https://w3id.org/dpv/owl#NoticeStatus> ;
  dc:contributor _:genid4, _:genid1 ;
  dc:created "2024-12-01"^^xsd:date ;
  ns1:term_status "accepted"@en ;
  skos:definition "Status indicating the notice has been generated"@en ;
  skos:prefLabel "Notice Generated"@en ;
  owl:sameAs <https://w3id.org/dpv#NoticeGenerated>, <https://w3id.org/dpv/dpv-owl#NoticeGenerated> .

<https://w3id.org/dpv/owl#DataStoragePolicy>
  a owl:Class, owl:NamedIndividual, <https://w3id.org/dpv/owl#OrganisationalMeasure> ;
  rdfs:subClassOf <https://w3id.org/dpv/owl#DataProcessingPolicy> ;
  dc:contributor _:genid4, _:genid1 ;
  dc:created "2024-04-14"^^xsd:date ;
  ns1:term_status "accepted"@en ;
  skos:definition "Policy regarding storage of data, including the manner, duration, location, and conditions for storage"@en ;
  skos:prefLabel "Data Storage Policy"@en ;
  owl:sameAs <https://w3id.org/dpv#DataStoragePolicy>, <https://w3id.org/dpv/dpv-owl#DataStoragePolicy> .

<https://w3id.org/dpv/owl#RightsImpactAssessment>
  a owl:Class, owl:NamedIndividual, <https://w3id.org/dpv/owl#OrganisationalMeasure> ;
  rdfs:subClassOf <https://w3id.org/dpv/owl#ImpactAssessment> ;
  dc:contributor _:genid1 ;
  dc:created "2024-04-14"^^xsd:date ;
  ns1:term_status "accepted"@en ;
  skos:definition "Impact assessment which involves determining the impact on rights and freedoms"@en ;
  skos:prefLabel "Rights Impact Assessment"@en ;
  skos:scopeNote "The rights and freedoms may be those defined in law or other norms, and may be bound to a jurisdiction"@en ;
  owl:sameAs <https://w3id.org/dpv#RightsImpactAssessment>, <https://w3id.org/dpv/dpv-owl#RightsImpactAssessment> .

odrl:unit
  a owl:AnnotationProperty ;
  rdfs:isDefinedBy odrl: ;
  rdfs:label "Unit"@en ;
  skos:definition "The unit of measurement of the value of the rightOperand or rightOperandReference of a Constraint."@en ;
  rdfs:domain odrl:Constraint .

<https://w3id.org/dpv/owl#hasDataSubject>
  a owl:ObjectProperty ;
  rdfs:subPropertyOf <https://w3id.org/dpv/owl#hasHumanSubject> ;
  ns2:rangeIncludes <https://w3id.org/dpv/owl#DataSubject> ;
  dc:contributor _:genid13, _:genid9, _:genid31, _:genid1, _:genid11 ;
  dc:created "2019-04-04"^^xsd:date ;
  dc:modified "2024-12-17"^^xsd:date ;
  ns3:example <https://w3id.org/dpv/examples/owl#E0074> ;
  ns1:term_status "modified"@en ;
  skos:definition "Indicates association with Data Subject"@en ;
  skos:prefLabel "has data subject"@en ;
  ns0:rangeIncludes <https://w3id.org/dpv/owl#DataSubject> ;
  owl:sameAs <https://w3id.org/dpv#hasDataSubject>, <https://w3id.org/dpv/dpv-owl#hasDataSubject> .

<https://w3id.org/dpv/owl#CannotCorrectProcess>
  a owl:Class, owl:NamedIndividual, <https://w3id.org/dpv/owl#EntityNonPermissiveInvolvement> ;
  rdfs:subClassOf <https://w3id.org/dpv/owl#EntityNonPermissiveInvolvement> ;
  dc:contributor _:genid1, _:genid25, _:genid19 ;
  dc:created "2024-05-11"^^xsd:date ;
  ns1:term_status "accepted"@en ;
  skos:definition "Involvement where entity cannot correct the process of specified context"@en ;
  skos:prefLabel "Cannot Correct Process"@en ;
  owl:sameAs <https://w3id.org/dpv#CannotCorrectProcess>, <https://w3id.org/dpv/dpv-owl#CannotCorrectProcess> .

<https://w3id.org/dpv/owl#PersonnelPerformanceManagement>
  a owl:Class, owl:NamedIndividual, <https://w3id.org/dpv/owl#Purpose> ;
  rdfs:subClassOf <https://w3id.org/dpv/owl#PersonnelManagement>, <https://w3id.org/dpv/owl#PersonnelMonitoring> ;
  dc:created "2024-12-01"^^xsd:date ;
  ns1:term_status "accepted"@en ;
  skos:definition "Purposes associated with management of performance of personnel"@en ;
  skos:prefLabel "Personnel Performance Management"@en ;
  owl:sameAs <https://w3id.org/dpv#PersonnelPerformanceManagement>, <https://w3id.org/dpv/dpv-owl#PersonnelPerformanceManagement> .

<https://w3id.org/dpv/owl#B2CContract>
  a owl:Class, owl:NamedIndividual, <https://w3id.org/dpv/owl#LegalBasis> ;
  rdfs:subClassOf <https://w3id.org/dpv/owl#ContractByEntityType> ;
  dc:created "2024-08-27"^^xsd:date ;
  ns1:term_status "accepted"@en ;
  skos:definition "A contract between a business and a consumer where the business provides goods or services to the consumer"@en ;
  skos:prefLabel "Business-to-Consumer Contract"@en ;
  owl:sameAs <https://w3id.org/dpv#B2CContract>, <https://w3id.org/dpv/dpv-owl#B2CContract> .

<https://w3id.org/dpv/owl#FraudPreventionAndDetection>
  a owl:Class, owl:NamedIndividual, <https://w3id.org/dpv/owl#Purpose> ;
  rdfs:subClassOf <https://w3id.org/dpv/owl#MisusePreventionAndDetection> ;
  dc:contributor _:genid13, _:genid14, _:genid1, _:genid15, _:genid16, _:genid11 ;
  dc:created "2019-04-05"^^xsd:date ;
  ns1:term_status "accepted"@en ;
  skos:definition "Purposes associated with fraud detection, prevention, and mitigation"@en ;
  skos:prefLabel "Fraud Prevention and Detection"@en ;
  skos:related <https://specialprivacy.ercim.eu/vocabs/purposes#Government> ;
  owl:sameAs <https://w3id.org/dpv#FraudPreventionAndDetection>, <https://w3id.org/dpv/dpv-owl#FraudPreventionAndDetection> .

<https://w3id.org/dpv/owl#CommunicationManagement>
  a owl:Class, owl:NamedIndividual, <https://w3id.org/dpv/owl#Purpose> ;
  rdfs:subClassOf <https://w3id.org/dpv/owl#Purpose> ;
  dc:contributor _:genid4, _:genid1, _:genid6, _:genid21 ;
  dc:created "2021-09-01"^^xsd:date ;
  ns1:term_status "accepted"@en ;
  skos:definition "Communication Management refers to purposes associated with providing or managing communication activities e.g. to send an email for notifying some information"@en ;
  skos:prefLabel "Communication Management"@en ;
  skos:scopeNote "This purpose by itself does not sufficiently and clearly indicate what the communication is about. As such, it is recommended to combine it with another purpose to indicate the application. For example, Communication of Payment."@en ;
  owl:sameAs <https://w3id.org/dpv#CommunicationManagement>, <https://w3id.org/dpv/dpv-owl#CommunicationManagement> .

odrl:refinement
  a owl:ObjectProperty, owl:NamedIndividual, skos:Concept ;
  rdfs:domain [
    a owl:Class ;
    owl:unionOf (
     odrl:Action
     odrl:AssetCollection
     odrl:PartyCollection
   )
  ] ;
  rdfs:range [
    a owl:Class ;
    owl:unionOf (
     odrl:Constraint
     odrl:LogicalConstraint
   )
  ] ;
  rdfs:isDefinedBy odrl: ;
  rdfs:label "Refinement"@en ;
  skos:definition "Constraint used to refine the semantics of an Action, or Party/Asset Collection"@en ;
  skos:note "Example: the Action print is only permitted on 50% of the asset."@en .

odrl:inheritRelation a owl:ObjectProperty, owl:NamedIndividual, skos:Concept .
<https://w3id.org/dpv/owl#RequestInitiated>
  a owl:Class, owl:NamedIndividual, <https://w3id.org/dpv/owl#RequestStatus> ;
  rdfs:subClassOf <https://w3id.org/dpv/owl#RequestStatus> ;
  dc:contributor _:genid1 ;
  dc:created "2022-11-30"^^xsd:date ;
  ns1:term_status "accepted"@en ;
  skos:definition "State of a request being initiated"@en ;
  skos:prefLabel "Request Initiated"@en ;
  owl:sameAs <https://w3id.org/dpv#RequestInitiated>, <https://w3id.org/dpv/dpv-owl#RequestInitiated> .

odrl:prohibition
  a owl:ObjectProperty, owl:NamedIndividual, skos:Concept ;
  rdfs:domain odrl:Policy ;
  rdfs:range odrl:Prohibition ;
  rdfs:isDefinedBy odrl: ;
  rdfs:label "Has Prohibition"@en ;
  skos:definition "Relates an individual Prohibition to a Policy."@en .

<https://w3id.org/dpv/owl#HumanInvolved>
  a owl:Class, owl:NamedIndividual, <https://w3id.org/dpv/owl#HumanInvolvement> ;
  rdfs:subClassOf <https://w3id.org/dpv/owl#HumanInvolvement> ;
  dc:created "2022-09-03"^^xsd:date ;
  dc:modified "2023-12-10"^^xsd:date ;
  ns1:term_status "accepted"@en ;
  skos:definition "Humans are involved in the specified context"@en ;
  skos:prefLabel "Human involved"@en ;
  skos:scopeNote "This concept only indicates that humans are involved. For specific involvement, see specialised concepts e.g. involved for input, oversight."@en ;
  owl:sameAs <https://w3id.org/dpv#HumanInvolved>, <https://w3id.org/dpv/dpv-owl#HumanInvolved> .

odrl:absoluteSpatialPosition
  a owl:NamedIndividual, skos:Concept, odrl:LeftOperand ;
  rdfs:isDefinedBy odrl: ;
  rdfs:label "Absolute Spatial Asset Position"@en ;
  skos:broaderTransitive odrl:absolutePosition ;
  skos:definition "The absolute spatial positions of four corners of a rectangle on a 2D-canvas or the eight corners of a cuboid in a 3D-space for the target Asset to fit."@en ;
  skos:note "Example: The upper left corner of a picture may be constrained to a specific position of the canvas rendering it. Note: see also the Left Operand Relative Spatial Asset Position. "@en ;
  skos:scopeNote "Non-Normative"@en .

<https://w3id.org/dpv/owl#Assessment>
  a owl:Class, owl:NamedIndividual, <https://w3id.org/dpv/owl#OrganisationalMeasure> ;
  rdfs:subClassOf <https://w3id.org/dpv/owl#OrganisationalMeasure> ;
  dc:contributor _:genid1 ;
  dc:created "2021-09-08"^^xsd:date ;
  ns1:term_status "accepted"@en ;
  skos:definition "The document, plan, or process for assessment or determination towards a purpose e.g. assessment of legality or impact assessments"@en ;
  skos:prefLabel "Assessment"@en ;
  owl:sameAs <https://w3id.org/dpv#Assessment>, <https://w3id.org/dpv/dpv-owl#Assessment> .

<https://w3id.org/dpv/owl#TermsOfService>
  a owl:Class, owl:NamedIndividual, <https://w3id.org/dpv/owl#ContractualClause> ;
  rdfs:subClassOf <https://w3id.org/dpv/owl#ContractualClause> ;
  dc:contributor _:genid4 ;
  dc:created "2024-08-27"^^xsd:date ;
  ns1:term_status "accepted"@en ;
  skos:definition "Contractual clauses outlining the terms and conditions regarding the provision of a service, typically between a service provider and a service consumer, also know as 'Terms of Use' and 'Terms and Conditions' and commonly abbreviated as TOS, ToS, ToU, or T&C"@en ;
  skos:prefLabel "Terms of Service"@en ;
  owl:sameAs <https://w3id.org/dpv#TermsOfService>, <https://w3id.org/dpv/dpv-owl#TermsOfService> .

<https://w3id.org/dpv/owl#Contract>
  a owl:Class, owl:NamedIndividual, <https://w3id.org/dpv/owl#LegalBasis> ;
  rdfs:subClassOf <https://w3id.org/dpv/owl#LegalBasis> ;
  dc:contributor _:genid1 ;
  dc:created "2021-04-07"^^xsd:date ;
  dc:modified "2024-12-17"^^xsd:date ;
  ns3:example <https://w3id.org/dpv/examples/owl#E0076>, <https://w3id.org/dpv/examples/owl#E0077> ;
  ns1:term_status "modified"@en ;
  skos:definition "Creation, completion, fulfilment, or performance of a contract involving specified processing of data or technologies"@en ;
  skos:prefLabel "Contract"@en ;
  owl:sameAs <https://w3id.org/dpv#Contract>, <https://w3id.org/dpv/dpv-owl#Contract> .

<https://w3id.org/dpv/owl#hasProcessing>
  a owl:ObjectProperty ;
  ns2:rangeIncludes <https://w3id.org/dpv/owl#Processing> ;
  dc:contributor _:genid13, _:genid9, _:genid31, _:genid1, _:genid11 ;
  dc:created "2019-04-04"^^xsd:date ;
  dc:modified "2020-11-04"^^xsd:date ;
  dc:source [
    a ns0:WebPage ;
    ns0:name "SPECIAL Project" ;
    ns0:url "https://specialprivacy.ercim.eu/"
  ] ;
  ns3:example <https://w3id.org/dpv/examples/owl#E0085> ;
  ns1:term_status "accepted"@en ;
  skos:definition "Indicates association with Processing"@en ;
  skos:prefLabel "has processing"@en ;
  ns0:rangeIncludes <https://w3id.org/dpv/owl#Processing> ;
  owl:sameAs <https://w3id.org/dpv#hasProcessing>, <https://w3id.org/dpv/dpv-owl#hasProcessing> .

<https://w3id.org/dpv/owl#LegalObligationCompleted>
  a owl:Class, owl:NamedIndividual, <https://w3id.org/dpv/owl#LegalObligationStatus> ;
  rdfs:subClassOf <https://w3id.org/dpv/owl#LegalObligationStatus> ;
  dc:created "2024-08-27"^^xsd:date ;
  ns1:term_status "accepted"@en ;
  skos:definition "Status where the legal obligation has been completed"@en ;
  skos:prefLabel "Legal ObligationCompleted"@en ;
  owl:sameAs <https://w3id.org/dpv#LegalObligationCompleted>, <https://w3id.org/dpv/dpv-owl#LegalObligationCompleted> .

<https://w3id.org/dpv/owl#InformationSecurityPolicy>
  a owl:Class, owl:NamedIndividual, <https://w3id.org/dpv/owl#OrganisationalMeasure> ;
  rdfs:subClassOf <https://w3id.org/dpv/owl#Policy> ;
  dc:contributor _:genid1 ;
  dc:created "2022-08-17"^^xsd:date ;
  dc:modified "2024-04-14"^^xsd:date ;
  dc:source [
    a ns0:WebPage ;
    ns0:name "ENISA 5G Cybersecurity Standards" ;
    ns0:url "https://www.enisa.europa.eu/publications/5g-cybersecurity-standards"
  ] ;
  ns1:term_status "accepted"@en ;
  skos:definition "Policy regarding security of information"@en ;
  skos:prefLabel "Information Security Policy"@en ;
  owl:sameAs <https://w3id.org/dpv#InformationSecurityPolicy>, <https://w3id.org/dpv/dpv-owl#InformationSecurityPolicy> .

odrl:inform
  a owl:NamedIndividual, skos:Concept, odrl:Action ;
  odrl:includedIn odrl:use ;
  rdfs:isDefinedBy odrl: ;
  rdfs:label "Inform"@en ;
  skos:definition "To inform that an action has been performed on or in relation to the Asset."@en ;
  skos:note "May link to a Party with the role 'informedParty' function."@en ;
  skos:scopeNote "Non-Normative"@en .

<https://w3id.org/dpv/owl#ContractDisputeResolutionClause>
  a owl:Class, owl:NamedIndividual, <https://w3id.org/dpv/owl#ContractualClause> ;
  rdfs:subClassOf <https://w3id.org/dpv/owl#ContractualClause> ;
  dc:created "2024-08-27"^^xsd:date ;
  ns1:term_status "accepted"@en ;
  skos:definition "A provision detailing the methods and procedures for resolving disagreements or conflicts arising from the contract"@en ;
  skos:prefLabel "Contract DisputeResolution Clause"@en ;
  owl:sameAs <https://w3id.org/dpv#ContractDisputeResolutionClause>, <https://w3id.org/dpv/dpv-owl#ContractDisputeResolutionClause> .

<https://w3id.org/dpv/owl#DocumentSecurity>
  a owl:Class, owl:NamedIndividual, <https://w3id.org/dpv/owl#TechnicalMeasure> ;
  rdfs:subClassOf <https://w3id.org/dpv/owl#SecurityMethod> ;
  dc:contributor _:genid1 ;
  dc:created "2022-08-17"^^xsd:date ;
  dc:source [
    a ns0:WebPage ;
    ns0:name "ENISA Reference Incident Classification Taxonomy 2018" ;
    ns0:url "https://www.enisa.europa.eu/publications/reference-incident-classification-taxonomy/"
  ] ;
  ns1:term_status "accepted"@en ;
  skos:definition "Security measures enacted over documents to protect against tampering or restrict access"@en ;
  skos:prefLabel "Document Security"@en ;
  owl:sameAs <https://w3id.org/dpv#DocumentSecurity>, <https://w3id.org/dpv/dpv-owl#DocumentSecurity> .

<https://w3id.org/dpv/owl#ObligationViolated>
  a owl:Class, owl:NamedIndividual, <https://w3id.org/dpv/owl#RuleFulfilmentStatus> ;
  rdfs:subClassOf <https://w3id.org/dpv/owl#RuleViolated> ;
  dc:contributor _:genid1 ;
  dc:created "2024-09-10"^^xsd:date ;
  ns1:term_status "accepted"@en ;
  skos:definition "Status indicating an obligation has been violated i.e. the activity stated as being required to be carried out has not been carried out and this is considered as a violation i.e. the activity can no longer be carried out to fulfil the obligation"@en ;
  skos:prefLabel "Obligation Violated"@en ;
  owl:sameAs <https://w3id.org/dpv#ObligationViolated>, <https://w3id.org/dpv/dpv-owl#ObligationViolated> .

<https://w3id.org/dpv/owl#ContractFullySigned>
  a owl:Class, owl:NamedIndividual, <https://w3id.org/dpv/owl#ContractExecutionStatus> ;
  rdfs:subClassOf <https://w3id.org/dpv/owl#ContractExecutionStatus> ;
  dc:contributor _:genid4, _:genid1, _:genid17 ;
  dc:created "2025-01-09"^^xsd:date ;
  ns1:term_status "accepted"@en ;
  skos:definition "Status representing contract has been signed by all concerned parties"@en ;
  skos:prefLabel "Contract Fully Signed"@en ;
  owl:sameAs <https://w3id.org/dpv#ContractFullySigned>, <https://w3id.org/dpv/dpv-owl#ContractFullySigned> .

<https://w3id.org/dpv/owl#ConsumerStandardFormContract>
  a owl:Class, owl:NamedIndividual, <https://w3id.org/dpv/owl#LegalBasis> ;
  rdfs:subClassOf <https://w3id.org/dpv/owl#StandardFormContract> ;
  dc:created "2024-08-27"^^xsd:date ;
  ns1:term_status "accepted"@en ;
  skos:definition "A contract where the terms and conditions are determined by parties in the role of a 'consumer' - whether an entity or an individual, and the other parties have negligible or no ability to negotiate the terms and conditions"@en ;
  skos:prefLabel "Consumer Standard Form Contract"@en ;
  owl:sameAs <https://w3id.org/dpv#ConsumerStandardFormContract>, <https://w3id.org/dpv/dpv-owl#ConsumerStandardFormContract> .

<https://w3id.org/dpv/owl#ConsentReceipt>
  a owl:Class, owl:NamedIndividual, <https://w3id.org/dpv/owl#OrganisationalMeasure> ;
  rdfs:subClassOf <https://w3id.org/dpv/owl#ConsentRecord> ;
  dc:contributor _:genid1 ;
  dc:created "2022-06-22"^^xsd:date ;
  ns1:term_status "accepted"@en ;
  skos:definition "A record of consent or consent related activities that is provided to another entity"@en ;
  skos:prefLabel "Consent Receipt"@en ;
  owl:sameAs <https://w3id.org/dpv#ConsentReceipt>, <https://w3id.org/dpv/dpv-owl#ConsentReceipt> .

<https://w3id.org/dpv/owl#ReligiousAssociations>
  a owl:Class ;
  rdfs:subClassOf <https://w3id.org/dpv/owl#Organisation> ;
  dc:contributor _:genid4 ;
  dc:created "2024-12-01"^^xsd:date ;
  ns1:term_status "accepted"@en ;
  skos:definition "An organisations that supports the practice, promotion, and management of religious activities and beliefs"@en ;
  skos:prefLabel "Religious Associations"@en ;
  owl:sameAs <https://w3id.org/dpv#ReligiousAssociations>, <https://w3id.org/dpv/dpv-owl#ReligiousAssociations> .

<https://w3id.org/dpv/owl#Technology>
  a owl:Class ;
  dc:contributor _:genid1 ;
  dc:created "2022-01-26"^^xsd:date ;
  ns1:term_status "accepted"@en ;
  skos:definition "The technology, technological implementation, or any techniques, skills, methods, and processes used or applied"@en ;
  skos:prefLabel "Technology"@en ;
  skos:scopeNote "Examples (non-exhaustive) include: Algorithm, Process, Method, Skill, Database, Cookies, Server, Device"@en ;
  owl:sameAs <https://w3id.org/dpv#Technology>, <https://w3id.org/dpv/dpv-owl#Technology> .

<https://w3id.org/dpv/owl#ImprovePublicServices>
  a owl:Class, owl:NamedIndividual, <https://w3id.org/dpv/owl#Purpose> ;
  rdfs:subClassOf <https://w3id.org/dpv/owl#PublicBenefit> ;
  dc:contributor _:genid5, _:genid1 ;
  dc:created "2024-02-14"^^xsd:date ;
  dc:source "DGA 2.16"@en ;
  ns1:term_status "accepted"@en ;
  skos:definition "Purposes associated with improving the provision of public services, such as public safety, education or law enforcement"@en ;
  skos:prefLabel "Improve Public Services"@en ;
  owl:sameAs <https://w3id.org/dpv#ImprovePublicServices>, <https://w3id.org/dpv/dpv-owl#ImprovePublicServices> .

<https://w3id.org/dpv/owl#Anonymisation>
  a owl:Class, owl:NamedIndividual, <https://w3id.org/dpv/owl#TechnicalMeasure> ;
  rdfs:subClassOf <https://w3id.org/dpv/owl#Deidentification> ;
  dc:contributor _:genid64, _:genid9, _:genid10, _:genid1, _:genid11, _:genid68 ;
  dc:created "2019-04-05"^^xsd:date ;
  dc:modified "2022-11-24"^^xsd:date ;
  dc:source [
    a ns0:WebPage ;
    ns0:name "ISO 29100:2011" ;
    ns0:url "https://www.iso.org/standard/45123.html"
  ] ;
  ns1:term_status "accepted"@en ;
  skos:definition "Anonymisation is the process by which data is irreversibly altered in such a way that a data subject can no longer be identified directly or indirectly, either by the entity holding the data alone or in collaboration with other entities and information sources"@en ;
  skos:prefLabel "Anonymisation"@en ;
  owl:sameAs <https://w3id.org/dpv#Anonymisation>, <https://w3id.org/dpv/dpv-owl#Anonymisation> .

<https://w3id.org/dpv/owl#isBefore>
  a owl:ObjectProperty ;
  ns2:domainIncludes <https://w3id.org/dpv/owl#RightExerciseActivity> ;
  ns2:rangeIncludes <https://w3id.org/dpv/owl#RightExerciseActivity> ;
  dc:contributor _:genid4, _:genid1, _:genid17 ;
  dc:created "2022-03-02"^^xsd:date ;
  ns1:term_status "accepted"@en ;
  skos:definition "Indicates the specified concepts is 'before' this concept in some context"@en ;
  skos:prefLabel "is before"@en ;
  skos:scopeNote "Also used for specifying a RightExerciseActivity occurs before another RightExerciseActivity"@en ;
  ns0:domainIncludes <https://w3id.org/dpv/owl#RightExerciseActivity> ;
  ns0:rangeIncludes <https://w3id.org/dpv/owl#RightExerciseActivity> ;
  owl:sameAs <https://w3id.org/dpv#isBefore>, <https://w3id.org/dpv/dpv-owl#isBefore> .

<https://w3id.org/dpv/owl#ComplianceStatus>
  a owl:Class ;
  rdfs:subClassOf <https://w3id.org/dpv/owl#Status> ;
  dc:contributor _:genid1 ;
  dc:created "2022-05-18"^^xsd:date ;
  ns3:example <https://w3id.org/dpv/examples/owl#E0055> ;
  ns1:term_status "accepted"@en ;
  skos:definition "Status associated with Compliance with some norms, objectives, or requirements"@en ;
  skos:prefLabel "Compliance Status"@en ;
  owl:sameAs <https://w3id.org/dpv#ComplianceStatus>, <https://w3id.org/dpv/dpv-owl#ComplianceStatus> .

<https://w3id.org/dpv/owl#Acquire>
  a owl:Class, owl:NamedIndividual, <https://w3id.org/dpv/owl#Processing> ;
  rdfs:subClassOf <https://w3id.org/dpv/owl#Obtain> ;
  dc:created "2019-05-07"^^xsd:date ;
  dc:source [
    a ns0:WebPage ;
    ns0:name "GDPR Art.4-2" ;
    ns0:url "https://eur-lex.europa.eu/eli/reg/2016/679/art_4/par_2/oj"
  ] ;
  ns1:term_status "accepted"@en ;
  skos:definition "to come into possession or control of the data"@en ;
  skos:prefLabel "Acquire Data"@en ;
  owl:sameAs <https://w3id.org/dpv#Acquire>, <https://w3id.org/dpv/dpv-owl#Acquire> .

<https://w3id.org/dpv/owl#SecurityIncidentRecord>
  a owl:Class, owl:NamedIndividual, <https://w3id.org/dpv/owl#OrganisationalMeasure> ;
  rdfs:subClassOf <https://w3id.org/dpv/owl#RecordsOfActivities> ;
  dc:contributor _:genid1 ;
  dc:created "2024-04-14"^^xsd:date ;
  ns1:term_status "accepted"@en ;
  skos:definition "Record of a security incident"@en ;
  skos:prefLabel "Security Incident Record"@en ;
  owl:sameAs <https://w3id.org/dpv#SecurityIncidentRecord>, <https://w3id.org/dpv/dpv-owl#SecurityIncidentRecord> .

<https://w3id.org/dpv/owl#ProvideConsent>
  a owl:Class ;
  rdfs:subClassOf <https://w3id.org/dpv/owl#ConsentControl>, <https://w3id.org/dpv/owl#OptingInToProcess> ;
  dc:created "2024-05-11"^^xsd:date ;
  ns1:term_status "accepted"@en ;
  skos:definition "Control for providing consent"@en ;
  skos:prefLabel "Provide Consent"@en ;
  skos:scopeNote "Indicates how the data subject can provide consent e.g. used with dpv:isExercisedAt"@en ;
  owl:sameAs <https://w3id.org/dpv#ProvideConsent>, <https://w3id.org/dpv/dpv-owl#ProvideConsent> .

odrl:operator
  a owl:ObjectProperty, owl:NamedIndividual, skos:Concept ;
  rdfs:domain odrl:Constraint ;
  rdfs:range odrl:Operator ;
  rdfs:isDefinedBy odrl: ;
  rdfs:label "Has Operator"@en ;
  skos:definition "The operator function applied to operands of a Constraint"@en .

<https://w3id.org/dpv/examples>
  a owl:NamedIndividual, ns4:ResourceDescriptor ;
  dc:format <https://www.iana.org/assignments/media-types/text/html> ;
  dc:conformsTo <https://www.w3.org/TR/html/> ;
  dc:title "Examples for Data Privacy Vocabulary" ;
  ns4:hasArtifact <https://w3id.org/dpv/examples> ;
  ns4:hasRole <http://www.w3.org/ns/dx/prof/role/guidance> .

<https://w3id.org/dpv/owl#ServiceLevelAgreement>
  a owl:Class, owl:NamedIndividual, <https://w3id.org/dpv/owl#LegalBasis> ;
  rdfs:subClassOf <https://w3id.org/dpv/owl#ContractByDomain> ;
  dc:created "2024-08-27"^^xsd:date ;
  ns1:term_status "accepted"@en ;
  skos:definition "A contract regarding the provision of a service which outlines the acceptable metrics and performance of the service for the consumer"@en ;
  skos:prefLabel "Service Legvel Agreement (SLA)"@en ;
  owl:sameAs <https://w3id.org/dpv#ServiceLevelAgreement>, <https://w3id.org/dpv/dpv-owl#ServiceLevelAgreement> .

odrl:#assetParty
  a owl:NamedIndividual, skos:Collection ;
  skos:member odrl:partOf, odrl:source ;
  skos:prefLabel "Asset and Party"@en ;
  skos:scopeNote "ODRL Core Vocabulary Terms"@en .

<https://w3id.org/dpv/owl#PublicLocation>
  a owl:Class, owl:NamedIndividual, <https://w3id.org/dpv/owl#Location> ;
  rdfs:subClassOf <https://w3id.org/dpv/owl#LocalLocation> ;
  dc:contributor _:genid4 ;
  dc:created "2022-10-22"^^xsd:date ;
  ns1:term_status "accepted"@en ;
  skos:definition "Location that is or can be accessed by the public"@en ;
  skos:prefLabel "Public Location"@en ;
  owl:sameAs <https://w3id.org/dpv#PublicLocation>, <https://w3id.org/dpv/dpv-owl#PublicLocation> .

foaf:Agent a owl:Class .
<https://w3id.org/dpv/owl#LargeDataVolume>
  a owl:Class, owl:NamedIndividual, <https://w3id.org/dpv/owl#DataVolume> ;
  rdfs:subClassOf <https://w3id.org/dpv/owl#DataVolume> ;
  dc:contributor _:genid1 ;
  dc:created "2022-06-15"^^xsd:date ;
  ns1:term_status "accepted"@en ;
  skos:definition "Data volume that is considered large within the context"@en ;
  skos:prefLabel "Large Data Volume"@en ;
  owl:sameAs <https://w3id.org/dpv#LargeDataVolume>, <https://w3id.org/dpv/dpv-owl#LargeDataVolume> .

<https://w3id.org/dpv/owl#AuditStatus>
  a owl:Class ;
  rdfs:subClassOf <https://w3id.org/dpv/owl#Status> ;
  dc:contributor _:genid1 ;
  dc:created "2022-05-18"^^xsd:date ;
  ns3:example <https://w3id.org/dpv/examples/owl#E0056>, <https://w3id.org/dpv/examples/owl#E0057> ;
  ns1:term_status "accepted"@en ;
  skos:definition "Status associated with Auditing or Investigation"@en ;
  skos:prefLabel "Audit Status"@en ;
  owl:sameAs <https://w3id.org/dpv#AuditStatus>, <https://w3id.org/dpv/dpv-owl#AuditStatus> .

<https://w3id.org/dpv/owl#IntellectualPropertyData>
  a owl:Class ;
  rdfs:subClassOf <https://w3id.org/dpv/owl#ConfidentialData> ;
  dc:created "2024-02-14"^^xsd:date ;
  dc:source "DGA 5.10"@en ;
  ns1:term_status "accepted"@en ;
  skos:definition "Data protected by Intellectual Property rights and regulations"@en ;
  skos:prefLabel "Intellectual Property Data"@en ;
  owl:sameAs <https://w3id.org/dpv#IntellectualPropertyData>, <https://w3id.org/dpv/dpv-owl#IntellectualPropertyData> .

<https://w3id.org/dpv/owl#hasSector>
  a owl:ObjectProperty ;
  ns2:rangeIncludes <https://w3id.org/dpv/owl#Sector> ;
  dc:created "2019-04-05"^^xsd:date ;
  ns1:term_status "accepted"@en ;
  skos:definition "Indicates the purpose is associated with activities in the indicated (Economic) Sector(s)"@en ;
  skos:prefLabel "has sector"@en ;
  ns0:rangeIncludes <https://w3id.org/dpv/owl#Sector> ;
  owl:sameAs <https://w3id.org/dpv#hasSector>, <https://w3id.org/dpv/dpv-owl#hasSector> .

odrl:display
  a owl:NamedIndividual, skos:Concept, odrl:Action ;
  odrl:includedIn odrl:play ;
  rdfs:isDefinedBy odrl: ;
  rdfs:label "Display"@en ;
  skos:definition "To create a static and transient rendition of an Asset."@en ;
  skos:note "For example, displaying an image on a screen. If the action is to be performed to a wider audience than just the Assignees, then the Recipient constraint is recommended to be used."@en ;
  skos:scopeNote "Non-Normative"@en .

<https://w3id.org/dpv/owl#StatisticalConfidentialityAgreement>
  a owl:Class, owl:NamedIndividual, <https://w3id.org/dpv/owl#LegalMeasure> ;
  rdfs:subClassOf <https://w3id.org/dpv/owl#LegalAgreement> ;
  dc:created "2022-02-09"^^xsd:date ;
  dc:modified "2024-08-27"^^xsd:date ;
  ns1:term_status "accepted"@en ;
  skos:definition "An agreement outlining conditions, criteria, obligations, responsibilities, and specifics for classification and management of 'confidential data' based on a statistical framework"@en ;
  skos:prefLabel "Statistical Confidentiality Agreement"@en ;
  owl:sameAs <https://w3id.org/dpv#StatisticalConfidentialityAgreement>, <https://w3id.org/dpv/dpv-owl#StatisticalConfidentialityAgreement> .

<https://w3id.org/dpv/owl#UntilEventDuration>
  a owl:Class ;
  rdfs:subClassOf <https://w3id.org/dpv/owl#Duration> ;
  dc:contributor _:genid1 ;
  dc:created "2022-06-15"^^xsd:date ;
  dc:modified "2020-10-05"^^xsd:date ;
  ns1:term_status "accepted"@en ;
  skos:definition "Duration that takes place until a specific event occurs e.g. Account Closure"@en ;
  skos:prefLabel "Until Event Duration"@en ;
  owl:sameAs <https://w3id.org/dpv#UntilEventDuration>, <https://w3id.org/dpv/dpv-owl#UntilEventDuration> .

<https://w3id.org/dpv/owl#MentallyVulnerableDataSubject>
  a owl:Class, owl:NamedIndividual, <https://w3id.org/dpv/owl#HumanSubject> ;
  rdfs:subClassOf <https://w3id.org/dpv/owl#MentallyVulnerableHuman>, <https://w3id.org/dpv/owl#VulnerableDataSubject> ;
  dc:contributor _:genid4 ;
  dc:created "2022-06-15"^^xsd:date ;
  dc:modified "2024-12-17"^^xsd:date ;
  ns1:term_status "modified"@en ;
  skos:definition "Data subjects that are considered mentally vulnerable"@en ;
  skos:prefLabel "Mentally Vulnerable Data Subject"@en ;
  owl:sameAs <https://w3id.org/dpv#MentallyVulnerableDataSubject>, <https://w3id.org/dpv/dpv-owl#MentallyVulnerableDataSubject> .

<https://w3id.org/dpv/owl#hasAutomationLevel>
  a owl:ObjectProperty ;
  ns2:rangeIncludes <https://w3id.org/dpv/owl#AutomationLevel> ;
  dc:contributor _:genid1 ;
  dc:created "2022-08-13"^^xsd:date ;
  dc:modified "2024-04-20"^^xsd:date ;
  ns1:term_status "accepted"@en ;
  skos:definition "Indicates the level of automation involved in implementation of the specified context"@en ;
  skos:prefLabel "has automation level"@en ;
  ns0:rangeIncludes <https://w3id.org/dpv/owl#AutomationLevel> ;
  owl:sameAs <https://w3id.org/dpv#hasAutomationLevel>, <https://w3id.org/dpv/dpv-owl#hasAutomationLevel> .

<https://w3id.org/dpv/owl#NotAvailable>
  a owl:Class, owl:NamedIndividual, <https://w3id.org/dpv/owl#Applicability> ;
  rdfs:subClassOf <https://w3id.org/dpv/owl#Applicability> ;
  dc:contributor _:genid1 ;
  dc:created "2023-08-24"^^xsd:date ;
  ns1:term_status "accepted"@en ;
  skos:definition "Concept indicating the information or context is applicable but information is not yet available"@en ;
  skos:prefLabel "Not Available"@en ;
  skos:scopeNote "This concept is useful when describing situations where information is required but is not available (yet). For example, if in a form a field asks about whether a process X was completed, and it is correct to interpret that process X is applicable and must be completed, but the information is not yet available as to whether this was done - then NotAvailable is useful to represent this."@en ;
  owl:sameAs <https://w3id.org/dpv#NotAvailable>, <https://w3id.org/dpv/dpv-owl#NotAvailable> .

<https://w3id.org/dpv/owl#Expected>
  a owl:Class, owl:NamedIndividual, <https://w3id.org/dpv/owl#ExpectationStatus> ;
  rdfs:subClassOf <https://w3id.org/dpv/owl#ExpectationStatus> ;
  dc:contributor _:genid4, _:genid1, _:genid25, _:genid6 ;
  dc:created "2024-05-10"^^xsd:date ;
  ns1:term_status "accepted"@en ;
  skos:definition "Status indicating the specified context was expected"@en ;
  skos:prefLabel "Expected"@en ;
  owl:sameAs <https://w3id.org/dpv#Expected>, <https://w3id.org/dpv/dpv-owl#Expected> .

odrl:output
  a owl:ObjectProperty, owl:NamedIndividual, skos:Concept ;
  rdfs:subPropertyOf odrl:relation ;
  rdfs:domain odrl:Rule ;
  rdfs:range odrl:Asset ;
  rdfs:isDefinedBy odrl: ;
  rdfs:label "Output"@en ;
  skos:definition "The output property specifies the Asset which is created from the output of the Action."@en ;
  skos:scopeNote "Non-Normative"@en .

<https://w3id.org/dpv/owl#SensitiveData>
  a owl:Class ;
  rdfs:subClassOf <https://w3id.org/dpv/owl#Data> ;
  dc:created "2024-02-14"^^xsd:date ;
  ns1:term_status "accepted"@en ;
  skos:definition "Data deemed sensitive"@en ;
  skos:prefLabel "Sensitive Data"@en ;
  owl:sameAs <https://w3id.org/dpv#SensitiveData>, <https://w3id.org/dpv/dpv-owl#SensitiveData> .

<https://w3id.org/dpv/owl#SMEOrganisation>
  a owl:Class ;
  rdfs:subClassOf <https://w3id.org/dpv/owl#LegalEntity> ;
  dc:contributor _:genid4 ;
  dc:created "2024-12-01"^^xsd:date ;
  ns1:term_status "accepted"@en ;
  skos:definition "An organisation that is characterised as a Small or Medium-sized Enterprise based on limited staff and revenue"@en ;
  skos:prefLabel "SME Organisation"@en ;
  owl:sameAs <https://w3id.org/dpv#SMEOrganisation>, <https://w3id.org/dpv/dpv-owl#SMEOrganisation> .

<https://w3id.org/dpv/owl#hasResidualRisk>
  a owl:ObjectProperty ;
  ns2:domainIncludes <https://w3id.org/dpv/owl#Risk> ;
  ns2:rangeIncludes <https://w3id.org/dpv/owl#ResidualRisk> ;
  dc:contributor _:genid4, _:genid1, _:genid17, _:genid6 ;
  dc:created "2022-07-20"^^xsd:date ;
  ns3:example <https://w3id.org/dpv/examples/owl#E0068> ;
  ns1:term_status "accepted"@en ;
  skos:definition "Indicates the associated risk is the remaining or residual risk from applying mitigation measures or treatments to this risk"@en ;
  skos:prefLabel "has residual risk"@en ;
  ns0:domainIncludes <https://w3id.org/dpv/owl#Risk> ;
  ns0:rangeIncludes <https://w3id.org/dpv/owl#ResidualRisk> ;
  owl:sameAs <https://w3id.org/dpv#hasResidualRisk>, <https://w3id.org/dpv/dpv-owl#hasResidualRisk> .

odrl:source
  a owl:AnnotationProperty, owl:NamedIndividual, skos:Concept ;
  rdfs:domain odrl:_:genid-nodeid-Nd32909520d984eb2acc8591f722fbf67 ;
  rdfs:isDefinedBy odrl: ;
  rdfs:label "Source"@en ;
  skos:definition "Reference to a Asset/PartyCollection"@en ;
  skos:note "Used by AssetCollection and PartyCollection when constraints are applied."@en .

<https://w3id.org/dpv/owl#GuardianOfHuman>
  a owl:Class, owl:NamedIndividual, <https://w3id.org/dpv/owl#HumanSubject> ;
  rdfs:subClassOf <https://w3id.org/dpv/owl#HumanSubject> ;
  dc:contributor _:genid1 ;
  dc:created "2024-12-17"^^xsd:date ;
  ns1:term_status "accepted"@en ;
  skos:definition "Guardian(s) of humans"@en ;
  skos:prefLabel "Guardian(s) of Human"@en ;
  owl:sameAs <https://w3id.org/dpv#GuardianOfHuman>, <https://w3id.org/dpv/dpv-owl#GuardianOfHuman> .

odrl:assigneeOf
  a owl:ObjectProperty, owl:NamedIndividual, skos:Concept ;
  rdfs:domain odrl:Party ;
  rdfs:range odrl:Policy ;
  rdfs:isDefinedBy odrl: ;
  rdfs:label "Assignee Of"@en ;
  skos:definition "Identifies an ODRL Policy for which the identified Party undertakes the assignee functional role."@en ;
  skos:note "When assigneeOf has been asserted between a metadata expression and an ODRL Policy, the Party being identified MUST be inferred to undertake the assignee functional role of all the Rules of that Policy."@en .

odrl:invalid
  a owl:NamedIndividual, skos:Concept, odrl:ConflictTerm ;
  rdfs:isDefinedBy odrl: ;
  rdfs:label "Void Policy"@en ;
  skos:definition "The policy is void."@en ;
  skos:note "Used to indicate the policy is void for Conflict Strategy."@en ;
  skos:scopeNote "Non-Normative"@en .

<https://w3id.org/dpv/owl#NoticeIcon>
  a owl:Class ;
  dc:created "2024-08-17"^^xsd:date ;
  dc:source [
    a ns0:WebPage ;
    ns0:name "ICO - What methods can we use to provide privacy information?" ;
    ns0:url "https://ico.org.uk/for-organisations/uk-gdpr-guidance-and-resources/individual-rights/the-right-to-be-informed/what-methods-can-we-use-to-provide-privacy-information/"
  ] ;
  ns3:example <https://w3id.org/dpv/examples/owl#E0072> ;
  ns1:term_status "accepted"@en ;
  skos:definition "An icon within a notice associated with specific information or elements"@en ;
  skos:prefLabel "Notice Icon"@en ;
  owl:sameAs <https://w3id.org/dpv#NoticeIcon>, <https://w3id.org/dpv/dpv-owl#NoticeIcon> .

odrl:unitOfCount
  a owl:NamedIndividual, skos:Concept, odrl:LeftOperand ;
  rdfs:isDefinedBy odrl: ;
  rdfs:label "Unit Of Count"@en ;
  skos:definition "The unit of measure used for counting the executions of the action of the Rule."@en ;
  skos:note "Note: Typically used with Duties to indicate the unit entity to be counted of the Action. <br />Example: A duty to compensate and a unitOfCount constraint of 'perUser' would indicate that the compensation by multiplied by the 'number of users'."@en ;
  skos:scopeNote "Non-Normative"@en .

<https://w3id.org/dpv/owl#AuditRequired>
  a owl:Class, owl:NamedIndividual, <https://w3id.org/dpv/owl#AuditStatus> ;
  rdfs:subClassOf <https://w3id.org/dpv/owl#AuditStatus> ;
  dc:contributor _:genid1 ;
  dc:created "2022-05-18"^^xsd:date ;
  ns1:term_status "accepted"@en ;
  skos:definition "State where an audit is determined as being required but has not been conducted"@en ;
  skos:prefLabel "Audit Required"@en ;
  owl:sameAs <https://w3id.org/dpv#AuditRequired>, <https://w3id.org/dpv/dpv-owl#AuditRequired> .

odrl:assigner
  a owl:ObjectProperty, owl:NamedIndividual, skos:Concept ;
  rdfs:subPropertyOf odrl:function ;
  rdfs:domain [
    a owl:Class ;
    owl:unionOf (
     odrl:Policy
     odrl:Rule
   )
  ] ;
  rdfs:range odrl:Party ;
  rdfs:isDefinedBy odrl: ;
  rdfs:label "Assigner"@en ;
  skos:definition "The Party is the issuer of the Rule."@en .

odrl:ConflictTerm
  a owl:Class, owl:NamedIndividual, skos:Concept ;
  rdfs:isDefinedBy odrl: ;
  rdfs:label "Conflict Strategy Preference"@en ;
  skos:definition "Used to establish strategies to resolve conflicts that arise from the merging of Policies or conflicts between Permissions and Prohibitions in the same Policy."@en ;
  skos:note "Instances of ConflictTerm describe strategies for resolving conflicts."@en .

<https://w3id.org/dpv/owl#ImpliedConsent>
  a owl:Class, owl:NamedIndividual, <https://w3id.org/dpv/owl#LegalBasis> ;
  rdfs:subClassOf <https://w3id.org/dpv/owl#InformedConsent> ;
  dc:contributor _:genid4, _:genid1, _:genid17, _:genid6 ;
  dc:created "2022-06-21"^^xsd:date ;
  ns1:term_status "accepted"@en ;
  skos:definition "Consent that is implied indirectly through an action not associated solely with conveying a consenting decision"@en ;
  skos:prefLabel "Implied Consent"@en ;
  skos:scopeNote "Implied consent is expected to also be Informed Consent. An example is a CCTV notice outside a monitored area that informs the individuals that by walking in they would be consenting to the use of camera for surveillance."@en ;
  owl:sameAs <https://w3id.org/dpv#ImpliedConsent>, <https://w3id.org/dpv/dpv-owl#ImpliedConsent> .

odrl:annotate
  a owl:NamedIndividual, skos:Concept, odrl:Action ;
  odrl:includedIn odrl:use ;
  rdfs:isDefinedBy odrl: ;
  rdfs:label "Annotate"@en ;
  skos:definition "To add explanatory notations/commentaries to the Asset without modifying the Asset in any other way."@en ;
  skos:scopeNote "Non-Normative"@en .

<https://w3id.org/dpv/owl#DataErasurePolicy>
  a owl:Class, owl:NamedIndividual, <https://w3id.org/dpv/owl#OrganisationalMeasure> ;
  rdfs:subClassOf <https://w3id.org/dpv/owl#DataProcessingPolicy> ;
  dc:contributor _:genid1 ;
  dc:created "2024-04-14"^^xsd:date ;
  ns1:term_status "accepted"@en ;
  skos:definition "Policy regarding erasure of data"@en ;
  skos:prefLabel "Data Erasure Policy"@en ;
  skos:scopeNote "Erasure or data destruction or secure removal of data refers to irreversible erasure of data. See dpv:DataDeletion for reversible or logical deletion of data"@en ;
  owl:sameAs <https://w3id.org/dpv#DataErasurePolicy>, <https://w3id.org/dpv/dpv-owl#DataErasurePolicy> .

<https://w3id.org/dpv/owl#Participant>
  a owl:Class, owl:NamedIndividual, <https://w3id.org/dpv/owl#HumanSubject> ;
  rdfs:subClassOf <https://w3id.org/dpv/owl#HumanSubject> ;
  dc:contributor _:genid4, _:genid5, _:genid1, _:genid17, _:genid6 ;
  dc:created "2022-04-06"^^xsd:date ;
  dc:modified "2024-12-17"^^xsd:date ;
  ns1:term_status "modified"@en ;
  skos:definition "Humans that participate in some context such as volunteers in a function"@en ;
  skos:prefLabel "Participant"@en ;
  owl:sameAs <https://w3id.org/dpv#Participant>, <https://w3id.org/dpv/dpv-owl#Participant> .

odrl:trackedParty
  a owl:ObjectProperty, owl:NamedIndividual, skos:Concept ;
  rdfs:subPropertyOf odrl:function ;
  rdfs:isDefinedBy odrl: ;
  rdfs:label "Tracked Party"@en ;
  skos:definition "The Party whose usage is being tracked."@en ;
  skos:note "May be specified as part of the acceptTracking action."@en ;
  skos:scopeNote "Non-Normative"@en .

<https://w3id.org/dpv/owl#DataBreachNotice>
  a owl:Class, owl:NamedIndividual, <https://w3id.org/dpv/owl#OrganisationalMeasure> ;
  rdfs:subClassOf <https://w3id.org/dpv/owl#SecurityIncidentNotice> ;
  dc:contributor _:genid4, _:genid5, _:genid1, _:genid6, _:genid21 ;
  dc:created "2024-04-14"^^xsd:date ;
  dc:source " DGA 21.5 GDPR 33"@en, " GDPR 34"@en, "DGA 12.k"@en ;
  ns1:term_status "accepted"@en ;
  skos:definition "A notice providing information about data breach(es) i.e. unauthorised transfer, access, use, or modification of data"@en ;
  skos:prefLabel "Data Breach Notice"@en ;
  owl:sameAs <https://w3id.org/dpv#DataBreachNotice>, <https://w3id.org/dpv/dpv-owl#DataBreachNotice> .

<https://w3id.org/dpv/owl#ImpactAssessment>
  a owl:Class, owl:NamedIndividual, <https://w3id.org/dpv/owl#OrganisationalMeasure> ;
  rdfs:subClassOf <https://w3id.org/dpv/owl#RiskAssessment> ;
  dc:contributor _:genid4, _:genid1, _:genid6 ;
  dc:created "2020-11-04"^^xsd:date ;
  ns1:term_status "accepted"@en ;
  skos:definition "Calculating or determining the likelihood of impact of an existing or proposed process, which can involve risks or detriments."@en ;
  skos:prefLabel "Impact Assessment"@en ;
  owl:sameAs <https://w3id.org/dpv#ImpactAssessment>, <https://w3id.org/dpv/dpv-owl#ImpactAssessment> .

<https://w3id.org/dpv/owl#hasDataSource>
  a owl:ObjectProperty ;
  ns2:rangeIncludes <https://w3id.org/dpv/owl#DataSource> ;
  dc:contributor _:genid4, _:genid1, _:genid6 ;
  dc:created "2020-11-04"^^xsd:date ;
  ns1:term_status "accepted"@en ;
  skos:definition "Indicates the source or origin of data being processed"@en ;
  skos:prefLabel "has data source"@en ;
  ns0:rangeIncludes <https://w3id.org/dpv/owl#DataSource> ;
  owl:sameAs <https://w3id.org/dpv#hasDataSource>, <https://w3id.org/dpv/dpv-owl#hasDataSource> .

<https://w3id.org/dpv/owl#hasProhibition>
  a owl:ObjectProperty ;
  rdfs:subPropertyOf <https://w3id.org/dpv/owl#hasRule> ;
  ns2:domainIncludes <https://w3id.org/dpv/owl#Context> ;
  ns2:rangeIncludes <https://w3id.org/dpv/owl#Prohibition> ;
  dc:contributor _:genid4, _:genid5, _:genid1, _:genid6 ;
  dc:created "2022-10-19"^^xsd:date ;
  ns3:example <https://w3id.org/dpv/examples/owl#E0066> ;
  ns1:term_status "accepted"@en ;
  skos:definition "Specifying applicability or inclusion of a prohibition rule within specified context"@en ;
  skos:prefLabel "has prohibition"@en ;
  ns0:domainIncludes <https://w3id.org/dpv/owl#Context> ;
  ns0:rangeIncludes <https://w3id.org/dpv/owl#Prohibition> ;
  owl:sameAs <https://w3id.org/dpv#hasProhibition>, <https://w3id.org/dpv/dpv-owl#hasProhibition> .

odrl:isAnyOf
  a owl:NamedIndividual, skos:Concept, odrl:Operator ;
  rdfs:isDefinedBy odrl: ;
  rdfs:label "Is any of"@en ;
  skos:definition "A set-based operator indicating that a given value is any of the right operand of the Constraint."@en .

<https://w3id.org/dpv/owl#PenetrationTestingMethods>
  a owl:Class, owl:NamedIndividual, <https://w3id.org/dpv/owl#TechnicalMeasure> ;
  rdfs:subClassOf <https://w3id.org/dpv/owl#SecurityMethod> ;
  dc:contributor _:genid1 ;
  dc:created "2022-08-17"^^xsd:date ;
  dc:source [
    a ns0:WebPage ;
    ns0:name "ENISA Reference Incident Classification Taxonomy 2018" ;
    ns0:url "https://www.enisa.europa.eu/publications/reference-incident-classification-taxonomy/"
  ] ;
  ns1:term_status "accepted"@en ;
  skos:definition "Use of penetration testing to identify weaknesses and vulnerabilities through simulations"@en ;
  skos:prefLabel "Penetration Testing Methods"@en ;
  owl:sameAs <https://w3id.org/dpv#PenetrationTestingMethods>, <https://w3id.org/dpv/dpv-owl#PenetrationTestingMethods> .

<https://w3id.org/dpv/owl#ConfidentialityAgreement>
  a owl:Class, owl:NamedIndividual, <https://w3id.org/dpv/owl#LegalMeasure> ;
  rdfs:subClassOf <https://w3id.org/dpv/owl#LegalAgreement> ;
  dc:created "2022-02-09"^^xsd:date ;
  dc:modified "2024-08-27"^^xsd:date ;
  dc:source "DGA 3.1.a"@en ;
  ns1:term_status "accepted"@en ;
  skos:definition "Agreements that enforce confidentiality for e.g. to protect business, professional, or company secrets"@en ;
  skos:prefLabel "Confidentiality Agreement"@en ;
  owl:sameAs <https://w3id.org/dpv#ConfidentialityAgreement>, <https://w3id.org/dpv/dpv-owl#ConfidentialityAgreement> .

<https://w3id.org/dpv/owl#DeviceNotice>
  a owl:Class, owl:NamedIndividual, <https://w3id.org/dpv/owl#OrganisationalMeasure> ;
  rdfs:subClassOf <https://w3id.org/dpv/owl#Notice> ;
  dc:created "2024-08-17"^^xsd:date ;
  dc:source [
    a ns0:WebPage ;
    ns0:name "ICO - What methods can we use to provide privacy information?" ;
    ns0:url "https://ico.org.uk/for-organisations/uk-gdpr-guidance-and-resources/individual-rights/the-right-to-be-informed/what-methods-can-we-use-to-provide-privacy-information/"
  ] ;
  ns1:term_status "accepted"@en ;
  skos:definition "A notice provided using the functionality provided by a device e.g. using the popup or alert feature"@en ;
  skos:prefLabel "Device Notice"@en ;
  owl:sameAs <https://w3id.org/dpv#DeviceNotice>, <https://w3id.org/dpv/dpv-owl#DeviceNotice> .

<https://w3id.org/dpv/owl#HumanInvolvement>
  a owl:Class ;
  rdfs:subClassOf <https://w3id.org/dpv/owl#EntityInvolvement> ;
  dc:contributor _:genid1 ;
  dc:created "2022-01-26"^^xsd:date ;
  dc:modified "2024-04-20"^^xsd:date ;
  ns3:example <https://w3id.org/dpv/examples/owl#E0013>, <https://w3id.org/dpv/examples/owl#E0074> ;
  ns1:term_status "accepted"@en ;
  skos:definition "The involvement of humans in specified context"@en ;
  skos:prefLabel "Human Involvement"@en ;
  skos:scopeNote "Human Involvement here broadly refers to any involvement by a human in the context of carrying out processing. This may include verification of outcomes, providing input data for making decisions, or overseeing activities. To indicate whether humans are involved or not, see relevant concepts of dpv:HumanInvolved and dpv:HumanNotInvolved. The term 'Human in the loop' and its varieties are absent from DPV due to their contradictory and non-compatible use across different sources."@en ;
  owl:sameAs <https://w3id.org/dpv#HumanInvolvement>, <https://w3id.org/dpv/dpv-owl#HumanInvolvement> .

<https://w3id.org/dpv/owl#RecruitmentApplicationAnalysis>
  a owl:Class, owl:NamedIndividual, <https://w3id.org/dpv/owl#Purpose> ;
  rdfs:subClassOf <https://w3id.org/dpv/owl#RecruitmentApplicationManagement> ;
  dc:created "2024-12-01"^^xsd:date ;
  ns1:term_status "accepted"@en ;
  skos:definition "Purposes assocaited with analysis of job applications or job candidates for recruitment"@en ;
  skos:prefLabel "Recruitment Application Analysis"@en ;
  owl:sameAs <https://w3id.org/dpv#RecruitmentApplicationAnalysis>, <https://w3id.org/dpv/dpv-owl#RecruitmentApplicationAnalysis> .

<https://w3id.org/dpv/owl#LegalObligationOngoing>
  a owl:Class, owl:NamedIndividual, <https://w3id.org/dpv/owl#LegalObligationStatus> ;
  rdfs:subClassOf <https://w3id.org/dpv/owl#LegalObligationStatus> ;
  dc:created "2024-08-27"^^xsd:date ;
  ns1:term_status "accepted"@en ;
  skos:definition "Status where the legal obligation is being fulfiled"@en ;
  skos:prefLabel "Legal ObligationOngoing"@en ;
  owl:sameAs <https://w3id.org/dpv#LegalObligationOngoing>, <https://w3id.org/dpv/dpv-owl#LegalObligationOngoing> .

<https://w3id.org/dpv/owl#Use>
  a owl:Class, owl:NamedIndividual, <https://w3id.org/dpv/owl#Processing> ;
  rdfs:subClassOf <https://w3id.org/dpv/owl#Processing> ;
  dc:created "2019-05-07"^^xsd:date ;
  dc:source [
    a ns0:WebPage ;
    ns0:name "GDPR Art.4-2" ;
    ns0:url "https://eur-lex.europa.eu/eli/reg/2016/679/art_4/par_2/oj"
  ] ;
  ns1:term_status "accepted"@en ;
  skos:definition "to use data"@en ;
  skos:prefLabel "Use Data"@en ;
  owl:sameAs <https://w3id.org/dpv#Use>, <https://w3id.org/dpv/dpv-owl#Use> .

<https://w3id.org/dpv/owl#PublicRelations>
  a owl:Class, owl:NamedIndividual, <https://w3id.org/dpv/owl#Purpose> ;
  rdfs:subClassOf <https://w3id.org/dpv/owl#Marketing> ;
  dc:contributor _:genid4, _:genid1, _:genid6, _:genid21 ;
  dc:created "2021-09-01"^^xsd:date ;
  dc:source [
    a ns0:WebPage ;
    ns0:name "Belgian DPA ROPA Template" ;
    ns0:url "https://www.privacycommission.be/nl/model-voor-een-register-van-de-verwerkingsactiviteiten"
  ] ;
  ns1:term_status "accepted"@en ;
  skos:definition "Purposes associated with managing and conducting public relations processes, including creating goodwill for the organisation"@en ;
  skos:prefLabel "Public Relations"@en ;
  owl:sameAs <https://w3id.org/dpv#PublicRelations>, <https://w3id.org/dpv/dpv-owl#PublicRelations> .

odrl:AssetCollection
  a owl:Class, owl:NamedIndividual, skos:Concept ;
  rdfs:subClassOf odrl:Asset ;
  rdfs:isDefinedBy odrl: ;
  rdfs:label "Asset Collection"@en ;
  skos:definition "An Asset that is collection of individual resources"@en .

<https://w3id.org/dpv/owl#RecordsOfActivities>
  a owl:Class, owl:NamedIndividual, <https://w3id.org/dpv/owl#OrganisationalMeasure> ;
  rdfs:subClassOf <https://w3id.org/dpv/owl#OrganisationalMeasure> ;
  dc:contributor _:genid4, _:genid1, _:genid6 ;
  dc:created "2021-09-08"^^xsd:date ;
  dc:modified "2024-05-05"^^xsd:date ;
  ns1:term_status "accepted"@en ;
  skos:definition "Records of activities within some context such as maintenance tasks or governance functions"@en ;
  skos:prefLabel "Records of Activities"@en ;
  skos:scopeNote "Records can be any information associated with the activity e.g. logs, summaries."@en ;
  owl:sameAs <https://w3id.org/dpv#RecordsOfActivities>, <https://w3id.org/dpv/dpv-owl#RecordsOfActivities> .

<https://w3id.org/dpv/owl#SearchFunctionalities>
  a owl:Class, owl:NamedIndividual, <https://w3id.org/dpv/owl#Purpose> ;
  rdfs:subClassOf <https://w3id.org/dpv/owl#ServiceProvision> ;
  dc:contributor _:genid4 ;
  dc:created "2022-11-09"^^xsd:date ;
  ns1:term_status "accepted"@en ;
  skos:definition "Purposes associated with providing searching, querying, or other forms of information retrieval related functionalities"@en ;
  skos:prefLabel "Search Functionalities"@en ;
  owl:sameAs <https://w3id.org/dpv#SearchFunctionalities>, <https://w3id.org/dpv/dpv-owl#SearchFunctionalities> .

<https://w3id.org/dpv/owl#PhysicalInterruptionProtection>
  a owl:Class, owl:NamedIndividual, <https://w3id.org/dpv/owl#PhysicalMeasure> ;
  rdfs:subClassOf <https://w3id.org/dpv/owl#PhysicalMeasure> ;
  dc:contributor _:genid1 ;
  dc:created "2024-04-14"^^xsd:date ;
  dc:source "NIST SP 800-18"@en ;
  ns1:term_status "accepted"@en ;
  skos:definition "Physical protection against interruptions e.g. electrical supply interruption"@en ;
  skos:prefLabel "Physical Interruption Protection"@en ;
  owl:sameAs <https://w3id.org/dpv#PhysicalInterruptionProtection>, <https://w3id.org/dpv/dpv-owl#PhysicalInterruptionProtection> .

<https://w3id.org/dpv/owl#LegitimateInterestObjected>
  a owl:Class, owl:NamedIndividual, <https://w3id.org/dpv/owl#LegitimateInterestStatus> ;
  rdfs:subClassOf <https://w3id.org/dpv/owl#LegitimateInterestStatus> ;
  dc:created "2024-08-27"^^xsd:date ;
  ns1:term_status "accepted"@en ;
  skos:definition "Status where the use of Legitimate Interest was objected to"@en ;
  skos:prefLabel "Legitimate InterestObjected"@en ;
  owl:sameAs <https://w3id.org/dpv#LegitimateInterestObjected>, <https://w3id.org/dpv/dpv-owl#LegitimateInterestObjected> .

odrl:#policyConcepts
  a owl:NamedIndividual, skos:Collection ;
  skos:member odrl:Policy, odrl:inheritFrom, odrl:profile, odrl:uid ;
  skos:prefLabel "Policy"@en ;
  skos:scopeNote "ODRL Core Vocabulary Terms"@en .

<https://w3id.org/dpv/owl#ActivityStatus>
  a owl:Class ;
  rdfs:subClassOf <https://w3id.org/dpv/owl#Status> ;
  dc:contributor _:genid1 ;
  dc:created "2022-05-18"^^xsd:date ;
  ns3:example <https://w3id.org/dpv/examples/owl#E0054> ;
  ns1:term_status "accepted"@en ;
  skos:definition "Status associated with activity operations and lifecycles"@en ;
  skos:prefLabel "Activity Status"@en ;
  owl:sameAs <https://w3id.org/dpv#ActivityStatus>, <https://w3id.org/dpv/dpv-owl#ActivityStatus> .

odrl:synchronize
  a owl:NamedIndividual, skos:Concept, odrl:Action ;
  odrl:includedIn odrl:use ;
  rdfs:isDefinedBy odrl: ;
  rdfs:label "Synchronize"@en ;
  skos:definition "To use the Asset in timed relations with media (audio/visual) elements of another Asset."@en ;
  skos:scopeNote "Non-Normative"@en .

<https://w3id.org/dpv/owl#NonCommercialResearch>
  a owl:Class, owl:NamedIndividual, <https://w3id.org/dpv/owl#Purpose> ;
  rdfs:subClassOf <https://w3id.org/dpv/owl#NonCommercialPurpose>, <https://w3id.org/dpv/owl#ResearchAndDevelopment> ;
  dc:contributor _:genid13, _:genid14, _:genid1, _:genid15, _:genid16, _:genid11 ;
  dc:created "2019-04-05"^^xsd:date ;
  dc:modified "2024-04-14"^^xsd:date ;
  ns1:term_status "accepted"@en ;
  skos:definition "Purposes associated with conducting research in a non-commercial setting e.g. for a non-profit-organisation (NGO)"@en ;
  skos:prefLabel "Non-Commercial Research"@en ;
  owl:sameAs <https://w3id.org/dpv#NonCommercialResearch>, <https://w3id.org/dpv/dpv-owl#NonCommercialResearch> .

<https://w3id.org/dpv/owl#SafeguardForDataTransfer>
  a owl:Class, owl:NamedIndividual, <https://w3id.org/dpv/owl#OrganisationalMeasure> ;
  rdfs:subClassOf <https://w3id.org/dpv/owl#Safeguard> ;
  dc:contributor _:genid4, _:genid1, _:genid6, _:genid21 ;
  dc:created "2021-09-22"^^xsd:date ;
  ns1:term_status "accepted"@en ;
  skos:definition "Represents a safeguard used for data transfer. Can include technical or organisational measures."@en ;
  skos:prefLabel "Safeguard for Data Transfer"@en ;
  owl:sameAs <https://w3id.org/dpv#SafeguardForDataTransfer>, <https://w3id.org/dpv/dpv-owl#SafeguardForDataTransfer> .

<https://w3id.org/dpv/owl#ConsequenceOfFailure>
  a owl:Class ;
  rdfs:subClassOf <https://w3id.org/dpv/owl#Consequence> ;
  dc:contributor _:genid4, _:genid1 ;
  dc:created "2022-03-23"^^xsd:date ;
  ns1:term_status "accepted"@en ;
  skos:definition "The consequence(s) possible or arising from failure of specified context"@en ;
  skos:prefLabel "Consequence of Failure"@en ;
  owl:sameAs <https://w3id.org/dpv#ConsequenceOfFailure>, <https://w3id.org/dpv/dpv-owl#ConsequenceOfFailure> .

<https://w3id.org/dpv/owl#ReversingProcessEffects>
  a owl:Class, owl:NamedIndividual, <https://w3id.org/dpv/owl#EntityPermissiveInvolvement> ;
  rdfs:subClassOf <https://w3id.org/dpv/owl#EntityPermissiveInvolvement> ;
  dc:contributor _:genid1, _:genid25, _:genid19 ;
  dc:created "2024-05-11"^^xsd:date ;
  ns1:term_status "accepted"@en ;
  skos:definition "Involvement where entity can reverse effects of specified context"@en ;
  skos:prefLabel "Reversing Process Effects"@en ;
  skos:scopeNote "Effects refer to consequences and impacts arising from the process or from the outputs of a process"@en ;
  owl:sameAs <https://w3id.org/dpv#ReversingProcessEffects>, <https://w3id.org/dpv/dpv-owl#ReversingProcessEffects> .

<https://w3id.org/dpv/owl#DataSubProcessor>
  a owl:Class ;
  rdfs:subClassOf <https://w3id.org/dpv/owl#DataProcessor> ;
  dc:contributor _:genid1 ;
  dc:created "2020-11-25"^^xsd:date ;
  ns1:term_status "accepted"@en ;
  skos:definition "A 'sub-processor' is a processor engaged by another processor"@en ;
  skos:prefLabel "Data Sub-Processor"@en ;
  skos:scopeNote "A 'Sub-Processor' is always a 'Processor' with the distinction of not directly being appointed by the 'Controller'"@en ;
  owl:sameAs <https://w3id.org/dpv#DataSubProcessor>, <https://w3id.org/dpv/dpv-owl#DataSubProcessor> .

<https://w3id.org/dpv/owl#DataProcessingAgreement>
  a owl:Class, owl:NamedIndividual, <https://w3id.org/dpv/owl#LegalBasis>, <https://w3id.org/dpv/owl#LegalMeasure> ;
  rdfs:subClassOf <https://w3id.org/dpv/owl#Contract> ;
  dc:contributor _:genid4, _:genid5, _:genid1, _:genid17, _:genid6 ;
  dc:created "2022-01-26"^^xsd:date ;
  dc:modified "2024-12-17"^^xsd:date ;
  ns1:term_status "modified"@en ;
  skos:definition "An agreement outlining conditions, criteria, obligations, responsibilities, and specifics for carrying out processing of data"@en ;
  skos:prefLabel "Data Processing Agreement"@en ;
  skos:scopeNote "For specific role-based data processing agreements, see concepts for Processors and JointDataController agreements."@en ;
  owl:sameAs <https://w3id.org/dpv#DataProcessingAgreement>, <https://w3id.org/dpv/dpv-owl#DataProcessingAgreement> .

odrl:consequence
  a owl:ObjectProperty, owl:NamedIndividual, skos:Concept ;
  rdfs:subPropertyOf odrl:failure ;
  rdfs:domain odrl:Duty ;
  rdfs:range odrl:Duty ;
  rdfs:isDefinedBy odrl: ;
  rdfs:label "Consequence"@en ;
  skos:definition "Relates a Duty to another Duty, the latter being a consequence of not fulfilling the former."@en ;
  skos:note "The consequence property is utilised to express the repercussions of not fulfilling an agreed Policy obligation or duty for a Permission. If either of these fails to be fulfilled, then this will result in the consequence Duty also becoming a new requirement, meaning that the original obligation or duty, as well as the consequence Duty must all be fulfilled"@en .

<https://w3id.org/dpv/owl#SingularDataVolume>
  a owl:Class, owl:NamedIndividual, <https://w3id.org/dpv/owl#DataVolume> ;
  rdfs:subClassOf <https://w3id.org/dpv/owl#DataVolume> ;
  dc:contributor _:genid1 ;
  dc:created "2022-06-15"^^xsd:date ;
  ns1:term_status "accepted"@en ;
  skos:definition "Data volume that is considered singular i.e. a specific instance or single item"@en ;
  skos:prefLabel "Singular Data Volume"@en ;
  owl:sameAs <https://w3id.org/dpv#SingularDataVolume>, <https://w3id.org/dpv/dpv-owl#SingularDataVolume> .

<https://w3id.org/dpv/owl#hasFulfillmentsStatus>
  a owl:ObjectProperty ;
  rdfs:subPropertyOf <https://w3id.org/dpv/owl#hasStatus> ;
  ns2:domainIncludes <https://w3id.org/dpv/owl#Context> ;
  ns2:rangeIncludes <https://w3id.org/dpv/owl#Rule> ;
  dc:contributor _:genid1 ;
  dc:created "2024-09-10"^^xsd:date ;
  ns1:term_status "accepted"@en ;
  skos:definition "Specifying the fulfillment status associated with a rule"@en ;
  skos:prefLabel "has fulfillment status"@en ;
  ns0:domainIncludes <https://w3id.org/dpv/owl#Context> ;
  ns0:rangeIncludes <https://w3id.org/dpv/owl#Rule> ;
  owl:sameAs <https://w3id.org/dpv#hasFulfillmentsStatus>, <https://w3id.org/dpv/dpv-owl#hasFulfillmentsStatus> .

<https://w3id.org/dpv/owl#PersonnelTerminationManagement>
  a owl:Class, owl:NamedIndividual, <https://w3id.org/dpv/owl#Purpose> ;
  rdfs:subClassOf <https://w3id.org/dpv/owl#PersonnelManagement> ;
  dc:created "2024-12-01"^^xsd:date ;
  ns1:term_status "accepted"@en ;
  skos:definition "Purposes associated with determination and management of termination of personnel"@en ;
  skos:prefLabel "Personnel Termination Management"@en ;
  owl:sameAs <https://w3id.org/dpv#PersonnelTerminationManagement>, <https://w3id.org/dpv/dpv-owl#PersonnelTerminationManagement> .

odrl:nextPolicy
  a owl:NamedIndividual, skos:Concept, odrl:Action ;
  odrl:includedIn odrl:use ;
  rdfs:isDefinedBy odrl: ;
  rdfs:label "Next Policy"@en ;
  skos:definition "To grant the specified Policy to a third party for their use of the Asset."@en ;
  skos:note "Useful for downstream policies."@en ;
  skos:scopeNote "Non-Normative"@en .

<https://w3id.org/dpv/owl#ActivelyInvolved>
  a owl:Class, owl:NamedIndividual, <https://w3id.org/dpv/owl#InvolvementStatus> ;
  rdfs:subClassOf <https://w3id.org/dpv/owl#InvolvementStatus> ;
  dc:contributor _:genid4, _:genid1, _:genid25, _:genid6 ;
  dc:created "2024-05-10"^^xsd:date ;
  ns1:term_status "accepted"@en ;
  skos:definition "Status indicating the specified context is 'actively' involved"@en ;
  skos:prefLabel "Actively Involved"@en ;
  skos:scopeNote "An example of active involvement is a person directly using a system to enter information"@en ;
  owl:sameAs <https://w3id.org/dpv#ActivelyInvolved>, <https://w3id.org/dpv/dpv-owl#ActivelyInvolved> .

<https://w3id.org/dpv/owl#PersonalDataProcess>
  a owl:Class ;
  rdfs:subClassOf <https://w3id.org/dpv/owl#Process> ;
  dc:contributor _:genid1 ;
  dc:created "2024-05-09"^^xsd:date ;
  ns1:term_status "accepted"@en ;
  skos:definition "An action, activity, or method involving personal data"@en ;
  skos:prefLabel "Personal Data Process"@en ;
  owl:sameAs <https://w3id.org/dpv#PersonalDataProcess>, <https://w3id.org/dpv/dpv-owl#PersonalDataProcess> .

<https://w3id.org/dpv/owl#hasProcessingCondition>
  a owl:ObjectProperty ;
  ns2:rangeIncludes <https://w3id.org/dpv/owl#ProcessingCondition> ;
  dc:contributor _:genid1 ;
  dc:created "2023-12-10"^^xsd:date ;
  ns1:term_status "accepted"@en ;
  skos:definition "Indicates information about processing condition"@en ;
  skos:prefLabel "has processing condition"@en ;
  ns0:rangeIncludes <https://w3id.org/dpv/owl#ProcessingCondition> ;
  owl:sameAs <https://w3id.org/dpv#hasProcessingCondition>, <https://w3id.org/dpv/dpv-owl#hasProcessingCondition> .

<https://w3id.org/dpv/owl#InformationFlowControl>
  a owl:Class, owl:NamedIndividual, <https://w3id.org/dpv/owl#TechnicalMeasure> ;
  rdfs:subClassOf <https://w3id.org/dpv/owl#TechnicalMeasure> ;
  dc:contributor _:genid1 ;
  dc:created "2022-08-17"^^xsd:date ;
  dc:source [
    a ns0:WebPage ;
    ns0:name "ENISA Reference Incident Classification Taxonomy 2018" ;
    ns0:url "https://www.enisa.europa.eu/publications/reference-incident-classification-taxonomy/"
  ] ;
  ns1:term_status "accepted"@en ;
  skos:definition "Use of measures to control information flows"@en ;
  skos:prefLabel "Information Flow Control"@en ;
  owl:sameAs <https://w3id.org/dpv#InformationFlowControl>, <https://w3id.org/dpv/dpv-owl#InformationFlowControl> .

foaf:Organization a owl:Class .
<https://w3id.org/dpv/owl#DataInventoryManagement>
  a owl:Class, owl:NamedIndividual, <https://w3id.org/dpv/owl#OrganisationalMeasure> ;
  rdfs:subClassOf <https://w3id.org/dpv/owl#DataGovernance> ;
  dc:contributor _:genid1 ;
  dc:created "2024-04-14"^^xsd:date ;
  ns1:term_status "accepted"@en ;
  skos:definition "Measures associated with management of data inventory or a data asset list"@en ;
  skos:prefLabel "Data Inventory Management"@en ;
  owl:sameAs <https://w3id.org/dpv#DataInventoryManagement>, <https://w3id.org/dpv/dpv-owl#DataInventoryManagement> .

<https://w3id.org/dpv/owl#Audit>
  a owl:Class, owl:NamedIndividual, <https://w3id.org/dpv/owl#OrganisationalMeasure> ;
  rdfs:subClassOf <https://w3id.org/dpv/owl#OrganisationalMeasure> ;
  dc:contributor _:genid1 ;
  dc:created "2024-12-17"^^xsd:date ;
  ns1:term_status "accepted"@en ;
  skos:definition "An audit is a systematic examination or evaluation of records, processes, or systems towards a specific objective such as to assess accuracy, compliance, effectiveness, or performance"@en ;
  skos:prefLabel "Audit"@en ;
  owl:sameAs <https://w3id.org/dpv#Audit>, <https://w3id.org/dpv/dpv-owl#Audit> .

odrl:include
  a owl:NamedIndividual, skos:Concept, odrl:Action ;
  odrl:includedIn odrl:use ;
  rdfs:isDefinedBy odrl: ;
  rdfs:label "Include"@en ;
  skos:definition "To include other related assets in the Asset."@en ;
  skos:note "For example: bio picture must be included in the attribution. Use of a relation sub-property is required for the related assets."@en ;
  skos:scopeNote "Non-Normative"@en .

<https://w3id.org/dpv/owl#NetworkSecurityProtocols>
  a owl:Class, owl:NamedIndividual, <https://w3id.org/dpv/owl#TechnicalMeasure> ;
  rdfs:subClassOf <https://w3id.org/dpv/owl#SecurityMethod> ;
  dc:contributor _:genid1 ;
  dc:created "2022-08-17"^^xsd:date ;
  dc:source [
    a ns0:WebPage ;
    ns0:name "ENISA Reference Incident Classification Taxonomy 2018" ;
    ns0:url "https://www.enisa.europa.eu/publications/reference-incident-classification-taxonomy/"
  ] ;
  ns1:term_status "accepted"@en ;
  skos:definition "Security implemented at or over networks protocols"@en ;
  skos:prefLabel "Network Security Protocols"@en ;
  owl:sameAs <https://w3id.org/dpv#NetworkSecurityProtocols>, <https://w3id.org/dpv/dpv-owl#NetworkSecurityProtocols> .

<https://w3id.org/dpv/owl#ConsentRevoked>
  a owl:Class, owl:NamedIndividual, <https://w3id.org/dpv/owl#ConsentStatus> ;
  rdfs:subClassOf <https://w3id.org/dpv/owl#ConsentStatusInvalidForProcessing> ;
  dc:contributor _:genid4, _:genid1, _:genid17, _:genid6 ;
  dc:created "2022-06-22"^^xsd:date ;
  dc:source [
    a ns0:WebPage ;
    ns0:name "GConsent" ;
    ns0:url "https://w3id.org/GConsent"
  ] ;
  ns1:term_status "accepted"@en ;
  skos:definition "The state where the consent is revoked by an entity other than the data subject and which prevents it from being further used as a valid state"@en ;
  skos:prefLabel "Consent Revoked"@en ;
  skos:scopeNote "An example of this state is when a Data Controller stops utilising previously obtaining consent, such as when that service no longer exists"@en ;
  owl:sameAs <https://w3id.org/dpv#ConsentRevoked>, <https://w3id.org/dpv/dpv-owl#ConsentRevoked> .

odrl:hasPolicy
  a owl:ObjectProperty, owl:NamedIndividual, skos:Concept ;
  rdfs:domain odrl:Asset ;
  rdfs:range odrl:Policy ;
  rdfs:isDefinedBy odrl: ;
  rdfs:label "Target Policy"@en ;
  skos:definition "Identifies an ODRL Policy for which the identified Asset is the target Asset to all the Rules."@en ;
  skos:note "The Asset being identified MUST be inferred to be the target Asset of all of the Rules of the Policy."@en .

<https://w3id.org/dpv/owl#Purpose>
  a owl:Class ;
  rdfs:subClassOf odrl:purpose ;
  dc:contributor _:genid13, _:genid1, _:genid25, _:genid11 ;
  dc:created "2019-04-05"^^xsd:date ;
  dc:modified "2024-04-14"^^xsd:date ;
  dc:source [
    a ns0:WebPage ;
    ns0:name "SPECIAL Project" ;
    ns0:url "https://specialprivacy.ercim.eu/"
  ] ;
  ns3:example <https://w3id.org/dpv/examples/owl#E0003>, <https://w3id.org/dpv/examples/owl#E0004>, <https://w3id.org/dpv/examples/owl#E0007>, <https://w3id.org/dpv/examples/owl#E0008>, <https://w3id.org/dpv/examples/owl#E0040>, <https://w3id.org/dpv/examples/owl#E0041>, <https://w3id.org/dpv/examples/owl#E0042>, <https://w3id.org/dpv/examples/owl#E0043> ;
  ns1:term_status "accepted"@en ;
  skos:definition "Purpose or (broader) Goal associated with data or technology"@en ;
  skos:prefLabel "Purpose"@en ;
  skos:related <https://specialprivacy.ercim.eu/langs/usage-policy#AnyPurpose> ;
  skos:scopeNote "The purpose or goal here is intended to sufficiently describe the intention or objective of why the data or technology is being used, and should be broader than mere technical descriptions of achieving a capability. For example, \"Analyse Data\" is an abstract purpose with no indication of what the analyses is for as compared to a purpose such as \"Marketing\" or \"Service Provision\" which provide clarity and comprehension of the 'purpose' and can be enhanced with additional descriptions. Such modelling is in line with regulatory requirements regarding the specificity of purposes, for example in GDPR"@en ;
  owl:sameAs <https://w3id.org/dpv#Purpose>, <https://w3id.org/dpv/dpv-owl#Purpose> .

odrl:consentingParty
  a owl:ObjectProperty, owl:NamedIndividual, skos:Concept ;
  rdfs:subPropertyOf odrl:function ;
  rdfs:isDefinedBy odrl: ;
  rdfs:label "Consenting Party"@en ;
  skos:definition "The Party to obtain consent from."@en ;
  skos:note "Maybe specified as part of the obtainConsent action."@en ;
  skos:scopeNote "Non-Normative"@en .

<https://w3id.org/dpv/owl#Seal>
  a owl:Class, owl:NamedIndividual, <https://w3id.org/dpv/owl#OrganisationalMeasure> ;
  rdfs:subClassOf <https://w3id.org/dpv/owl#CertificationSeal> ;
  dc:contributor _:genid9, _:genid10, _:genid1, _:genid11 ;
  dc:created "2019-04-05"^^xsd:date ;
  ns1:term_status "accepted"@en ;
  skos:definition "A seal or a mark indicating proof of certification to some certification or standard"@en ;
  skos:prefLabel "Seal"@en ;
  owl:sameAs <https://w3id.org/dpv#Seal>, <https://w3id.org/dpv/dpv-owl#Seal> .

<https://w3id.org/dpv/owl#B2BContract>
  a owl:Class, owl:NamedIndividual, <https://w3id.org/dpv/owl#LegalBasis> ;
  rdfs:subClassOf <https://w3id.org/dpv/owl#ContractByEntityType> ;
  dc:created "2024-08-27"^^xsd:date ;
  ns1:term_status "accepted"@en ;
  skos:definition "A contract between two businesses"@en ;
  skos:prefLabel "Business-to-Business Contract"@en ;
  owl:sameAs <https://w3id.org/dpv#B2BContract>, <https://w3id.org/dpv/dpv-owl#B2BContract> .

<https://w3id.org/dpv/owl#ChallengingProcessInput>
  a owl:Class, owl:NamedIndividual, <https://w3id.org/dpv/owl#EntityPermissiveInvolvement> ;
  rdfs:subClassOf <https://w3id.org/dpv/owl#EntityPermissiveInvolvement> ;
  dc:contributor _:genid1, _:genid25, _:genid19 ;
  dc:created "2024-05-11"^^xsd:date ;
  ns1:term_status "accepted"@en ;
  skos:definition "Involvement where entity can challenge input of specified context"@en ;
  skos:prefLabel "Challenging Process Input"@en ;
  owl:sameAs <https://w3id.org/dpv#ChallengingProcessInput>, <https://w3id.org/dpv/dpv-owl#ChallengingProcessInput> .

<https://w3id.org/dpv/owl#ConsultationWithAuthority>
  a owl:Class, owl:NamedIndividual, <https://w3id.org/dpv/owl#OrganisationalMeasure> ;
  rdfs:subClassOf <https://w3id.org/dpv/owl#Consultation> ;
  dc:contributor _:genid4, _:genid1, _:genid6 ;
  dc:created "2020-11-04"^^xsd:date ;
  ns1:term_status "accepted"@en ;
  skos:definition "Consultation with an authority or authoritative entity"@en ;
  skos:prefLabel "Consultation with Authority"@en ;
  owl:sameAs <https://w3id.org/dpv#ConsultationWithAuthority>, <https://w3id.org/dpv/dpv-owl#ConsultationWithAuthority> .

<https://w3id.org/dpv/owl#LegitimateInterestInformed>
  a owl:Class, owl:NamedIndividual, <https://w3id.org/dpv/owl#LegitimateInterestStatus> ;
  rdfs:subClassOf <https://w3id.org/dpv/owl#LegitimateInterestStatus> ;
  dc:created "2024-08-27"^^xsd:date ;
  ns1:term_status "accepted"@en ;
  skos:definition "Status where the Legitimate Interest was informed to the data subject or other relevant entities"@en ;
  skos:prefLabel "Legitimate InterestInformed"@en ;
  owl:sameAs <https://w3id.org/dpv#LegitimateInterestInformed>, <https://w3id.org/dpv/dpv-owl#LegitimateInterestInformed> .

org:memberOf a owl:AnnotationProperty .
<https://w3id.org/dpv/owl#PermissionUtilised>
  a owl:Class, owl:NamedIndividual, <https://w3id.org/dpv/owl#RuleFulfilmentStatus> ;
  rdfs:subClassOf <https://w3id.org/dpv/owl#RuleFulfilled> ;
  dc:contributor _:genid1 ;
  dc:created "2024-09-10"^^xsd:date ;
  ns1:term_status "accepted"@en ;
  skos:definition "Status indicating a permission has been utilised i.e. the activity stated as being permitted has been carried out"@en ;
  skos:prefLabel "Permission Utilised"@en ;
  owl:sameAs <https://w3id.org/dpv#PermissionUtilised>, <https://w3id.org/dpv/dpv-owl#PermissionUtilised> .

<https://w3id.org/dpv/owl#ConformanceStatus>
  a owl:Class ;
  rdfs:subClassOf <https://w3id.org/dpv/owl#Status> ;
  dc:contributor _:genid1 ;
  dc:created "2022-10-22"^^xsd:date ;
  ns1:term_status "accepted"@en ;
  skos:definition "Status associated with conformance to a standard, guideline, code, or recommendation"@en ;
  skos:prefLabel "Conformance Status"@en ;
  owl:sameAs <https://w3id.org/dpv#ConformanceStatus>, <https://w3id.org/dpv/dpv-owl#ConformanceStatus> .

<https://w3id.org/dpv/owl#PrivateInformationRetrieval>
  a owl:Class, owl:NamedIndividual, <https://w3id.org/dpv/owl#TechnicalMeasure> ;
  rdfs:subClassOf <https://w3id.org/dpv/owl#CryptographicMethods> ;
  dc:contributor _:genid1 ;
  dc:created "2022-08-17"^^xsd:date ;
  dc:source [
    a ns0:WebPage ;
    ns0:name "ENISA Data Protection Engineering" ;
    ns0:url "https://www.enisa.europa.eu/publications/data-protection-engineering"
  ] ;
  ns1:term_status "accepted"@en ;
  skos:definition "Use of cryptographic methods to retrieve a record from a system without revealing which record is retrieved"@en ;
  skos:prefLabel "Private Information Retrieval"@en ;
  owl:sameAs <https://w3id.org/dpv#PrivateInformationRetrieval>, <https://w3id.org/dpv/dpv-owl#PrivateInformationRetrieval> .

<https://w3id.org/dpv/owl#ContractActive>
  a owl:Class, owl:NamedIndividual, <https://w3id.org/dpv/owl#ContractActivationStatus> ;
  rdfs:subClassOf <https://w3id.org/dpv/owl#ContractActivationStatus> ;
  dc:contributor _:genid4, _:genid1, _:genid17 ;
  dc:created "2025-01-09"^^xsd:date ;
  ns1:term_status "accepted"@en ;
  skos:definition "Status representing contract that has been fully executed and whose terms are considered active i.e. they are applicable and are required to be performed"@en ;
  skos:prefLabel "Contract Active"@en ;
  skos:scopeNote "A contract being active only refers to its terms now being required to be fulfiled, while dpv:ContractBeingPerformed states that they are being performed"@en ;
  owl:sameAs <https://w3id.org/dpv#ContractActive>, <https://w3id.org/dpv/dpv-owl#ContractActive> .

<https://w3id.org/dpv/owl#AcceptContract>
  a owl:Class ;
  rdfs:subClassOf <https://w3id.org/dpv/owl#ContractControl> ;
  dc:created "2024-08-27"^^xsd:date ;
  ns1:term_status "accepted"@en ;
  skos:definition "Control for accepting a contract"@en ;
  skos:prefLabel "Accept Contract"@en ;
  owl:sameAs <https://w3id.org/dpv#AcceptContract>, <https://w3id.org/dpv/dpv-owl#AcceptContract> .

<https://w3id.org/dpv/owl#MediumDataVolume>
  a owl:Class, owl:NamedIndividual, <https://w3id.org/dpv/owl#DataVolume> ;
  rdfs:subClassOf <https://w3id.org/dpv/owl#DataVolume> ;
  dc:contributor _:genid4, _:genid1, _:genid6 ;
  dc:created "2022-06-15"^^xsd:date ;
  ns1:term_status "accepted"@en ;
  skos:definition "Data volume that is considered medium i.e. neither large nor small within the context"@en ;
  skos:prefLabel "Medium Data Volume"@en ;
  owl:sameAs <https://w3id.org/dpv#MediumDataVolume>, <https://w3id.org/dpv/dpv-owl#MediumDataVolume> .

<https://w3id.org/dpv/owl#SecurityIncidentNotification>
  a owl:Class, owl:NamedIndividual, <https://w3id.org/dpv/owl#OrganisationalMeasure> ;
  rdfs:subClassOf <https://w3id.org/dpv/owl#Notification> ;
  dc:contributor _:genid1 ;
  dc:created "2024-04-14"^^xsd:date ;
  ns1:term_status "accepted"@en ;
  skos:definition "Notification of information about security incident(s)"@en ;
  skos:prefLabel "Security Incident Notification"@en ;
  owl:sameAs <https://w3id.org/dpv#SecurityIncidentNotification>, <https://w3id.org/dpv/dpv-owl#SecurityIncidentNotification> .

<https://w3id.org/dpv/owl#RequestUnfulfilled>
  a owl:Class, owl:NamedIndividual, <https://w3id.org/dpv/owl#RequestStatus> ;
  rdfs:subClassOf <https://w3id.org/dpv/owl#RequestStatus> ;
  dc:contributor _:genid1 ;
  dc:created "2022-11-30"^^xsd:date ;
  ns1:term_status "accepted"@en ;
  skos:definition "State of a request being unfulfilled"@en ;
  skos:prefLabel "Request Unfulfilled"@en ;
  owl:sameAs <https://w3id.org/dpv#RequestUnfulfilled>, <https://w3id.org/dpv/dpv-owl#RequestUnfulfilled> .

<https://w3id.org/dpv/owl#VulnerabilityTestingMethods>
  a owl:Class, owl:NamedIndividual, <https://w3id.org/dpv/owl#TechnicalMeasure> ;
  rdfs:subClassOf <https://w3id.org/dpv/owl#SecurityMethod> ;
  dc:contributor _:genid1 ;
  dc:created "2022-08-17"^^xsd:date ;
  dc:source [
    a ns0:WebPage ;
    ns0:name "ENISA Reference Incident Classification Taxonomy 2018" ;
    ns0:url "https://www.enisa.europa.eu/publications/reference-incident-classification-taxonomy/"
  ] ;
  ns1:term_status "accepted"@en ;
  skos:definition "Methods that assess or discover vulnerabilities in a system"@en ;
  skos:prefLabel "Vulnerability Testing Methods"@en ;
  owl:sameAs <https://w3id.org/dpv#VulnerabilityTestingMethods>, <https://w3id.org/dpv/dpv-owl#VulnerabilityTestingMethods> .

odrl:give
  a owl:NamedIndividual, skos:Concept, odrl:Action ;
  odrl:includedIn odrl:transfer ;
  rdfs:isDefinedBy odrl: ;
  rdfs:label "Give"@en ;
  skos:definition "To transfer the ownership of the Asset to a third party without compensation and while deleting the original asset."@en ;
  skos:scopeNote "Non-Normative"@en .

<https://w3id.org/dpv/owl#AccountManagement>
  a owl:Class, owl:NamedIndividual, <https://w3id.org/dpv/owl#Purpose> ;
  rdfs:subClassOf <https://w3id.org/dpv/owl#Purpose> ;
  dc:contributor _:genid4, _:genid5, _:genid1 ;
  dc:created "2021-09-08"^^xsd:date ;
  ns1:term_status "accepted"@en ;
  skos:definition "Account Management refers to purposes associated with account management, such as to create, provide, maintain, and manage accounts"@en ;
  skos:prefLabel "Account Management"@en ;
  owl:sameAs <https://w3id.org/dpv#AccountManagement>, <https://w3id.org/dpv/dpv-owl#AccountManagement> .

<https://w3id.org/dpv/owl#NoticeStale>
  a owl:Class, owl:NamedIndividual, <https://w3id.org/dpv/owl#NoticeStatus> ;
  rdfs:subClassOf <https://w3id.org/dpv/owl#NoticeStatus> ;
  dc:contributor _:genid4, _:genid1 ;
  dc:created "2024-12-01"^^xsd:date ;
  ns1:term_status "accepted"@en ;
  skos:definition "Status indicating the notice is stale or not up to date or not the latest version"@en ;
  skos:prefLabel "Notice Stale"@en ;
  owl:sameAs <https://w3id.org/dpv#NoticeStale>, <https://w3id.org/dpv/dpv-owl#NoticeStale> .

<https://w3id.org/dpv/owl#ConsultationWithDPO>
  a owl:Class, owl:NamedIndividual, <https://w3id.org/dpv/owl#OrganisationalMeasure> ;
  rdfs:subClassOf <https://w3id.org/dpv/owl#Consultation> ;
  dc:contributor _:genid4, _:genid1 ;
  dc:created "2022-06-15"^^xsd:date ;
  ns1:term_status "accepted"@en ;
  skos:definition "Consultation with Data Protection Officer(s)"@en ;
  skos:prefLabel "Consultation with DPO"@en ;
  owl:sameAs <https://w3id.org/dpv#ConsultationWithDPO>, <https://w3id.org/dpv/dpv-owl#ConsultationWithDPO> .

<https://w3id.org/dpv/owl#NonProfitOrganisation>
  a owl:Class ;
  rdfs:subClassOf <https://w3id.org/dpv/owl#Organisation> ;
  dc:contributor _:genid1 ;
  dc:created "2022-02-02"^^xsd:date ;
  dc:modified "2020-10-05"^^xsd:date ;
  dc:source [
    a ns0:WebPage ;
    ns0:name "ADMS controlled vocabulary" ;
    ns0:url "http://purl.org/adms"
  ] ;
  ns1:term_status "accepted"@en ;
  skos:definition "An organisation that does not aim to achieve profit as its primary goal"@en ;
  skos:prefLabel "Non-Profit Organisation"@en ;
  owl:sameAs <https://w3id.org/dpv#NonProfitOrganisation>, <https://w3id.org/dpv/dpv-owl#NonProfitOrganisation> .

<https://w3id.org/dpv/owl#AuditRejected>
  a owl:Class, owl:NamedIndividual, <https://w3id.org/dpv/owl#AuditStatus> ;
  rdfs:subClassOf <https://w3id.org/dpv/owl#AuditStatus> ;
  dc:contributor _:genid1 ;
  dc:created "2022-05-18"^^xsd:date ;
  ns1:term_status "accepted"@en ;
  skos:definition "State of not being approved or being rejected through the audit"@en ;
  skos:prefLabel "Audit Rejected"@en ;
  owl:sameAs <https://w3id.org/dpv#AuditRejected>, <https://w3id.org/dpv/dpv-owl#AuditRejected> .

<https://w3id.org/dpv/owl#ObtainConsent>
  a owl:Class ;
  rdfs:subClassOf <https://w3id.org/dpv/owl#ConsentControl> ;
  dc:created "2024-05-11"^^xsd:date ;
  ns1:term_status "accepted"@en ;
  skos:definition "Control for obtaining consent"@en ;
  skos:prefLabel "Obtain Consent"@en ;
  skos:scopeNote "Indicates how the controller or entity can obtain consent e.g. used with dpv:isExercisedAt"@en ;
  owl:sameAs <https://w3id.org/dpv#ObtainConsent>, <https://w3id.org/dpv/dpv-owl#ObtainConsent> .

<https://w3id.org/dpv/owl#hasEntityInvolvement>
  a owl:ObjectProperty ;
  ns2:rangeIncludes <https://w3id.org/dpv/owl#EntityInvolvement> ;
  dc:created "2024-05-11"^^xsd:date ;
  ns1:term_status "accepted"@en ;
  skos:definition "Indicates involvement of an entity in specified context"@en ;
  skos:prefLabel "has entity involvement"@en ;
  ns0:rangeIncludes <https://w3id.org/dpv/owl#EntityInvolvement> ;
  owl:sameAs <https://w3id.org/dpv#hasEntityInvolvement>, <https://w3id.org/dpv/dpv-owl#hasEntityInvolvement> .

<https://w3id.org/dpv/owl#IncidentReportingCommunication>
  a owl:Class, owl:NamedIndividual, <https://w3id.org/dpv/owl#OrganisationalMeasure> ;
  rdfs:subClassOf <https://w3id.org/dpv/owl#GovernanceProcedures> ;
  dc:contributor _:genid1 ;
  dc:created "2022-08-17"^^xsd:date ;
  dc:source [
    a ns0:WebPage ;
    ns0:name "ENISA 5G Cybersecurity Standards" ;
    ns0:url "https://www.enisa.europa.eu/publications/5g-cybersecurity-standards"
  ] ;
  ns1:term_status "accepted"@en ;
  skos:definition "Procedures related to management of incident reporting"@en ;
  skos:prefLabel "Incident Reporting Communication"@en ;
  owl:sameAs <https://w3id.org/dpv#IncidentReportingCommunication>, <https://w3id.org/dpv/dpv-owl#IncidentReportingCommunication> .

odrl:#duties
  a owl:NamedIndividual, skos:Collection ;
  skos:member odrl:Duty, odrl:consequence, odrl:duty, odrl:obligation, odrl:remedy ;
  skos:prefLabel "Duty"@en ;
  skos:scopeNote "ODRL Core Vocabulary Terms"@en .

<https://w3id.org/dpv/owl#Marketing>
  a owl:Class, owl:NamedIndividual, <https://w3id.org/dpv/owl#Purpose> ;
  rdfs:subClassOf <https://w3id.org/dpv/owl#Purpose> ;
  dc:contributor _:genid4, _:genid5, _:genid1 ;
  dc:created "2020-11-04"^^xsd:date ;
  ns1:term_status "accepted"@en ;
  skos:definition "Purposes associated with conducting marketing in relation to organisation or products or services e.g. promoting, selling, and distributing"@en ;
  skos:prefLabel "Marketing"@en ;
  skos:scopeNote "Was commercial interest, changed to consider Marketing a separate Purpose category by itself"@en ;
  owl:sameAs <https://w3id.org/dpv#Marketing>, <https://w3id.org/dpv/dpv-owl#Marketing> .

<https://w3id.org/dpv/owl#LegalCompliance>
  a owl:Class, owl:NamedIndividual, <https://w3id.org/dpv/owl#Purpose> ;
  rdfs:subClassOf <https://w3id.org/dpv/owl#FulfilmentOfObligation> ;
  dc:contributor _:genid4, _:genid5, _:genid1 ;
  dc:created "2020-11-04"^^xsd:date ;
  dc:modified "2022-11-09"^^xsd:date ;
  ns1:term_status "accepted"@en ;
  skos:definition "Purposes associated with carrying out data processing to fulfill a legal or statutory obligation"@en ;
  skos:prefLabel "Legal Compliance"@en ;
  skos:scopeNote "This purpose only refers to processing that is additionally required in order to fulfill the obligations and requirements associated with a law. For example, the use of consent would have its own separate purposes, with this purpose addressing a legal requirement for maintaining consent record (along with RecordManagement). This purpose will typically be used with Legal Obligation as the legal basis."@en ;
  owl:sameAs <https://w3id.org/dpv#LegalCompliance>, <https://w3id.org/dpv/dpv-owl#LegalCompliance> .

<https://w3id.org/dpv/owl#MonitoringPolicy>
  a owl:Class, owl:NamedIndividual, <https://w3id.org/dpv/owl#OrganisationalMeasure> ;
  rdfs:subClassOf <https://w3id.org/dpv/owl#Policy> ;
  dc:contributor _:genid1 ;
  dc:created "2022-08-17"^^xsd:date ;
  dc:modified "2024-04-14"^^xsd:date ;
  dc:source [
    a ns0:WebPage ;
    ns0:name "ENISA 5G Cybersecurity Standards" ;
    ns0:url "https://www.enisa.europa.eu/publications/5g-cybersecurity-standards"
  ] ;
  ns1:term_status "accepted"@en ;
  skos:definition "Policy for monitoring (e.g. progress, performance)"@en ;
  skos:prefLabel "Monitoring Policy"@en ;
  owl:sameAs <https://w3id.org/dpv#MonitoringPolicy>, <https://w3id.org/dpv/dpv-owl#MonitoringPolicy> .

odrl:modify
  a owl:NamedIndividual, skos:Concept, odrl:Action ;
  odrl:includedIn odrl:use ;
  rdfs:isDefinedBy odrl: ;
  rdfs:label "Modify"@en ;
  skos:definition "To change existing content of the Asset. A new asset is not created by this action."@en ;
  skos:note "This action will modify an asset which is typically updated from time to time without creating a new asset. If the result from modifying the asset should be a new asset the actions derive or extract should be used. (Note that the notion of whether or not the change is significant enough to qualify as a new asset is subjective)."@en ;
  skos:scopeNote "Non-Normative"@en .

<https://w3id.org/dpv/owl#B2B2CContract>
  a owl:Class, owl:NamedIndividual, <https://w3id.org/dpv/owl#LegalBasis> ;
  rdfs:subClassOf <https://w3id.org/dpv/owl#B2BContract>, <https://w3id.org/dpv/owl#B2CContract> ;
  dc:contributor _:genid4, _:genid5 ;
  dc:created "2024-08-27"^^xsd:date ;
  ns1:term_status "accepted"@en ;
  skos:definition "A contract between two businesses who partner together to provide services to a consumer"@en ;
  skos:prefLabel "Business-to-Business-to-Consumer Contract"@en ;
  owl:sameAs <https://w3id.org/dpv#B2B2CContract>, <https://w3id.org/dpv/dpv-owl#B2B2CContract> .

<https://w3id.org/dpv/owl#LegalMeasure>
  a owl:Class ;
  rdfs:subClassOf <https://w3id.org/dpv/owl#TechnicalOrganisationalMeasure> ;
  dc:created "2023-12-10"^^xsd:date ;
  dc:modified "2023-12-10"^^xsd:date ;
  dc:source "DGA 12.j"@en ;
  ns1:term_status "accepted"@en ;
  skos:definition "Legal measures used to safeguard and ensure good practices in connection with data and technologies"@en ;
  skos:prefLabel "Legal Measure"@en ;
  owl:sameAs <https://w3id.org/dpv#LegalMeasure>, <https://w3id.org/dpv/dpv-owl#LegalMeasure> .

<https://w3id.org/dpv/owl#hasEntityControl>
  a owl:ObjectProperty ;
  rdfs:subPropertyOf <https://w3id.org/dpv/owl#hasTechnicalOrganisationalMeasure> ;
  ns2:rangeIncludes <https://w3id.org/dpv/owl#EntityControl> ;
  dc:contributor _:genid1 ;
  dc:created "2024-04-14"^^xsd:date ;
  ns1:term_status "accepted"@en ;
  skos:definition "Indicates a control or measure provided for an entity to perform the specified action"@en ;
  skos:prefLabel "has entity control"@en ;
  ns0:rangeIncludes <https://w3id.org/dpv/owl#EntityControl> ;
  owl:sameAs <https://w3id.org/dpv#hasEntityControl>, <https://w3id.org/dpv/dpv-owl#hasEntityControl> .

<https://w3id.org/dpv/owl#LargeScaleProcessing>
  a owl:Class, owl:NamedIndividual, <https://w3id.org/dpv/owl#ProcessingScale> ;
  rdfs:subClassOf <https://w3id.org/dpv/owl#ProcessingScale> ;
  dc:contributor _:genid1, _:genid2 ;
  dc:created "2020-11-04"^^xsd:date ;
  dc:modified "2022-09-07"^^xsd:date ;
  dc:source [
    a ns0:WebPage ;
    ns0:name "GDPR Art.4-2" ;
    ns0:url "https://eur-lex.europa.eu/eli/reg/2016/679/art_4/par_2/oj"
  ] ;
  ns1:term_status "accepted"@en ;
  skos:definition "Processing that takes place at large scales (as specified by some criteria)"@en ;
  skos:prefLabel "Large Scale Processing"@en ;
  skos:scopeNote "The exact definition of what constitutes \"large scale\" depends on use of jurisdictional, domain-specific, or other forms of externally defined criterias. Where possible, this should be reflected by extending this term with the appropriate context."@en ;
  owl:sameAs <https://w3id.org/dpv#LargeScaleProcessing>, <https://w3id.org/dpv/dpv-owl#LargeScaleProcessing> .

<https://w3id.org/dpv/owl#Consult>
  a owl:Class, owl:NamedIndividual, <https://w3id.org/dpv/owl#Processing> ;
  rdfs:subClassOf <https://w3id.org/dpv/owl#Use> ;
  dc:created "2019-05-07"^^xsd:date ;
  dc:source [
    a ns0:WebPage ;
    ns0:name "GDPR Art.4-2" ;
    ns0:url "https://eur-lex.europa.eu/eli/reg/2016/679/art_4/par_2/oj"
  ] ;
  ns1:term_status "accepted"@en ;
  skos:definition "to consult or query data"@en ;
  skos:prefLabel "Consult Data"@en ;
  skos:related <https://specialprivacy.ercim.eu/vocabs/processing#Query> ;
  owl:sameAs <https://w3id.org/dpv#Consult>, <https://w3id.org/dpv/dpv-owl#Consult> .

<https://w3id.org/dpv/owl#hasThirdParty>
  a owl:ObjectProperty ;
  rdfs:subPropertyOf <https://w3id.org/dpv/owl#hasEntity> ;
  ns2:rangeIncludes <https://w3id.org/dpv/owl#ThirdParty> ;
  dc:contributor _:genid1 ;
  dc:created "2025-02-02"^^xsd:date ;
  ns1:term_status "accepted"@en ;
  skos:definition "Indicates association with Third Party"@en ;
  skos:prefLabel "has third party"@en ;
  ns0:rangeIncludes <https://w3id.org/dpv/owl#ThirdParty> ;
  owl:sameAs <https://w3id.org/dpv#hasThirdParty>, <https://w3id.org/dpv/dpv-owl#hasThirdParty> .

<https://w3id.org/dpv/owl#PassivelyInvolved>
  a owl:Class, owl:NamedIndividual, <https://w3id.org/dpv/owl#InvolvementStatus> ;
  rdfs:subClassOf <https://w3id.org/dpv/owl#InvolvementStatus> ;
  dc:contributor _:genid4, _:genid1, _:genid25, _:genid6 ;
  dc:created "2024-05-10"^^xsd:date ;
  ns1:term_status "accepted"@en ;
  skos:definition "Status indicating the specified context is 'passively' involved"@en ;
  skos:prefLabel "Passively Involved"@en ;
  skos:scopeNote "An example of passive involvement is a person being monitored by a CCTV"@en ;
  owl:sameAs <https://w3id.org/dpv#PassivelyInvolved>, <https://w3id.org/dpv/dpv-owl#PassivelyInvolved> .

odrl:#policySubClassesCommon
  a owl:NamedIndividual, skos:Collection ;
  skos:member odrl:Assertion, odrl:Privacy, odrl:Request, odrl:Ticket ;
  skos:prefLabel "Policy Subclasses"@en ;
  skos:scopeNote "ODRL Common Vocabulary Terms"@en .

<https://w3id.org/dpv/owl#UnknownApplicability>
  a owl:Class, owl:NamedIndividual, <https://w3id.org/dpv/owl#Applicability> ;
  rdfs:subClassOf <https://w3id.org/dpv/owl#Applicability> ;
  dc:contributor _:genid1 ;
  dc:created "2023-08-24"^^xsd:date ;
  ns1:term_status "accepted"@en ;
  skos:definition "Concept indicating information or context availability is unknown i.e. it is not known if the information exists or is applicable and therefore statements about its availability cannot be made (yet)"@en ;
  skos:prefLabel "Unknown Applicability"@en ;
  skos:scopeNote "This concept is useful when describing situations where it cannot be stated whether the context applies or whether the information is not available yet. For example, if a form field asks about whether a process X was completed and it is not yet known whether X applies or not and therefore it is also unclear whether X was completed or not. Using UnknownApplicability is a signal that the applicability of X should be assessed, and if applicable, then information about X should be identified and used here."@en ;
  owl:sameAs <https://w3id.org/dpv#UnknownApplicability>, <https://w3id.org/dpv/dpv-owl#UnknownApplicability> .

<https://w3id.org/dpv/owl#ContractUnderNegotiation>
  a owl:Class, owl:NamedIndividual, <https://w3id.org/dpv/owl#ContractPreparationStatus> ;
  rdfs:subClassOf <https://w3id.org/dpv/owl#ContractPreparationStatus> ;
  dc:contributor _:genid4, _:genid1, _:genid17 ;
  dc:created "2025-01-09"^^xsd:date ;
  ns1:term_status "accepted"@en ;
  skos:definition "Status representing contract is under negotiation between parties"@en ;
  skos:prefLabel "Contract Under Negotiation"@en ;
  owl:sameAs <https://w3id.org/dpv#ContractUnderNegotiation>, <https://w3id.org/dpv/dpv-owl#ContractUnderNegotiation> .

<https://w3id.org/dpv/owl#PersonalData>
  a owl:Class ;
  rdfs:subClassOf <https://w3id.org/dpv/owl#Data> ;
  dc:contributor _:genid1 ;
  dc:created "2019-04-05"^^xsd:date ;
  dc:modified "2022-01-19"^^xsd:date ;
  dc:source [
    a ns0:WebPage ;
    ns0:name "GDPR Art.4-1g" ;
    ns0:url "https://eur-lex.europa.eu/eli/reg/2016/679/art_4/par_1/oj"
  ] ;
  ns3:example <https://w3id.org/dpv/examples/owl#E0044> ;
  ns1:term_status "accepted"@en ;
  skos:definition "Data directly or indirectly associated or related to an individual."@en ;
  skos:prefLabel "Personal Data"@en ;
  skos:related <https://specialprivacy.ercim.eu/langs/usage-policy#AnyData> ;
  skos:scopeNote "This definition of personal data encompasses the concepts used in GDPR Art.4-1 for 'personal data' and ISO/IEC 2700 for 'personally identifiable information (PII)'."@en ;
  owl:sameAs <https://w3id.org/dpv#PersonalData>, <https://w3id.org/dpv/dpv-owl#PersonalData> .

<https://w3id.org/dpv/owl#ObligationUnfulfilled>
  a owl:Class, owl:NamedIndividual, <https://w3id.org/dpv/owl#RuleFulfilmentStatus> ;
  rdfs:subClassOf <https://w3id.org/dpv/owl#RuleUnfulfilled> ;
  dc:contributor _:genid1 ;
  dc:created "2024-09-10"^^xsd:date ;
  ns1:term_status "accepted"@en ;
  skos:definition "Status indicating an obligation has not been fulfilled i.e. the activity stated as being required to be carried out has not been carried out but this is not considered as a violation e.g. there is still time to conduct the activity"@en ;
  skos:prefLabel "Obligation Unfulfilled"@en ;
  owl:sameAs <https://w3id.org/dpv#ObligationUnfulfilled>, <https://w3id.org/dpv/dpv-owl#ObligationUnfulfilled> .

<https://w3id.org/dpv/owl#OralNotice>
  a owl:Class, owl:NamedIndividual, <https://w3id.org/dpv/owl#OrganisationalMeasure> ;
  rdfs:subClassOf <https://w3id.org/dpv/owl#Notice> ;
  dc:created "2024-08-17"^^xsd:date ;
  dc:source [
    a ns0:WebPage ;
    ns0:name "ICO - What methods can we use to provide privacy information?" ;
    ns0:url "https://ico.org.uk/for-organisations/uk-gdpr-guidance-and-resources/individual-rights/the-right-to-be-informed/what-methods-can-we-use-to-provide-privacy-information/"
  ] ;
  ns1:term_status "accepted"@en ;
  skos:definition "A notice provided orally or verbally"@en ;
  skos:prefLabel "Oral Notice"@en ;
  owl:sameAs <https://w3id.org/dpv#OralNotice>, <https://w3id.org/dpv/dpv-owl#OralNotice> .

<https://w3id.org/dpv/owl#PostedNotice>
  a owl:Class, owl:NamedIndividual, <https://w3id.org/dpv/owl#OrganisationalMeasure> ;
  rdfs:subClassOf <https://w3id.org/dpv/owl#Notice> ;
  dc:created "2024-08-17"^^xsd:date ;
  dc:source [
    a ns0:WebPage ;
    ns0:name "ICO - What methods can we use to provide privacy information?" ;
    ns0:url "https://ico.org.uk/for-organisations/uk-gdpr-guidance-and-resources/individual-rights/the-right-to-be-informed/what-methods-can-we-use-to-provide-privacy-information/"
  ] ;
  ns1:term_status "accepted"@en ;
  skos:definition "A notice that is posted as a sign or banner"@en ;
  skos:prefLabel "Posted Notice"@en ;
  owl:sameAs <https://w3id.org/dpv#PostedNotice>, <https://w3id.org/dpv/dpv-owl#PostedNotice> .

<https://w3id.org/dpv/owl#Impact>
  a owl:Class ;
  rdfs:subClassOf <https://w3id.org/dpv/owl#Consequence> ;
  dc:contributor _:genid4, _:genid5, _:genid1, _:genid17, _:genid15 ;
  dc:created "2022-03-23"^^xsd:date ;
  dc:modified "2024-08-16"^^xsd:date ;
  ns3:example <https://w3id.org/dpv/examples/owl#E0027>, <https://w3id.org/dpv/examples/owl#E0068>, <https://w3id.org/dpv/examples/owl#E0069> ;
  ns1:term_status "accepted"@en ;
  skos:definition "The impact(s) possible or arising as a consequence from specified context"@en ;
  skos:prefLabel "Impact"@en ;
  skos:scopeNote "Impact is a stronger notion of consequence in terms of influence, change, or effect on something e.g. for impact assessments"@en ;
  owl:sameAs <https://w3id.org/dpv#Impact>, <https://w3id.org/dpv/dpv-owl#Impact> .

<https://w3id.org/dpv/owl#PersonalisedAdvertising>
  a owl:Class, owl:NamedIndividual, <https://w3id.org/dpv/owl#Purpose> ;
  rdfs:subClassOf <https://w3id.org/dpv/owl#Advertising>, <https://w3id.org/dpv/owl#Personalisation> ;
  dc:contributor _:genid4, _:genid5, _:genid1 ;
  dc:created "2020-11-04"^^xsd:date ;
  ns1:term_status "accepted"@en ;
  skos:definition "Purposes associated with creating and providing personalised advertising"@en ;
  skos:prefLabel "Personalised Advertising"@en ;
  owl:sameAs <https://w3id.org/dpv#PersonalisedAdvertising>, <https://w3id.org/dpv/dpv-owl#PersonalisedAdvertising> .

<https://w3id.org/dpv/owl#CommercialPurpose>
  a owl:Class, owl:NamedIndividual, <https://w3id.org/dpv/owl#Purpose> ;
  rdfs:subClassOf <https://w3id.org/dpv/owl#Purpose> ;
  dc:contributor _:genid5, _:genid1 ;
  dc:created "2024-02-14"^^xsd:date ;
  dc:source "DGA 4.4"@en ;
  ns1:term_status "accepted"@en ;
  skos:definition "Purposes associated with processing activities performed in a commercial setting or with intention to commercialise"@en ;
  skos:prefLabel "Commercial Purpose"@en ;
  owl:sameAs <https://w3id.org/dpv#CommercialPurpose>, <https://w3id.org/dpv/dpv-owl#CommercialPurpose> .

<https://w3id.org/dpv/owl#hasContractualFulfilmentStatus>
  a owl:ObjectProperty ;
  rdfs:subPropertyOf <https://w3id.org/dpv/owl#hasContractStatus> ;
  ns2:domainIncludes <https://w3id.org/dpv/owl#Contract>, <https://w3id.org/dpv/owl#ContractualClause> ;
  ns2:rangeIncludes <https://w3id.org/dpv/owl#ContractStatus> ;
  dc:created "2024-08-27"^^xsd:date ;
  ns3:example <https://w3id.org/dpv/examples/owl#E0077>, <https://w3id.org/dpv/examples/owl#E0078> ;
  ns1:term_status "accepted"@en ;
  skos:definition "Indicates the fulfilment status of a contract or a contractual clause"@en ;
  skos:prefLabel "has contractual fulfilment status"@en ;
  ns0:domainIncludes <https://w3id.org/dpv/owl#Contract>, <https://w3id.org/dpv/owl#ContractualClause> ;
  ns0:rangeIncludes <https://w3id.org/dpv/owl#ContractStatus> ;
  owl:sameAs <https://w3id.org/dpv#hasContractualFulfilmentStatus>, <https://w3id.org/dpv/dpv-owl#hasContractualFulfilmentStatus> .

<https://w3id.org/dpv/owl#InnovativeUseOfTechnology>
  a owl:Class ;
  rdfs:subClassOf <https://w3id.org/dpv/owl#ProcessingContext> ;
  dc:created "2023-12-10"^^xsd:date ;
  ns1:term_status "accepted"@en ;
  skos:definition "Indicates that technology is being used in an innovative manner"@en ;
  skos:prefLabel "Innovative use of Technology"@en ;
  skos:scopeNote "Innovative here refers to 'state of the art' rather than the implementing entity, and can be for either new technology or new uses of existing technology"@en ;
  owl:sameAs <https://w3id.org/dpv#InnovativeUseOfTechnology>, <https://w3id.org/dpv/dpv-owl#InnovativeUseOfTechnology> .

<https://w3id.org/dpv/owl#AINotice>
  a owl:Class, owl:NamedIndividual, <https://w3id.org/dpv/owl#OrganisationalMeasure> ;
  rdfs:subClassOf <https://w3id.org/dpv/owl#Notice> ;
  dc:contributor _:genid25 ;
  dc:created "2024-12-01"^^xsd:date ;
  ns1:term_status "accepted"@en ;
  skos:definition "A notice providing information regarding the particulars of an AI system such as its intended purpose and proper use"@en ;
  skos:prefLabel "AI Notice"@en ;
  owl:sameAs <https://w3id.org/dpv#AINotice>, <https://w3id.org/dpv/dpv-owl#AINotice> .

odrl:sell
  a owl:NamedIndividual, skos:Concept, odrl:Action ;
  odrl:includedIn odrl:transfer ;
  rdfs:isDefinedBy odrl: ;
  rdfs:label "Sell"@en ;
  skos:definition "To transfer the ownership of the Asset to a third party with compensation and while deleting the original asset."@en ;
  skos:scopeNote "Non-Normative"@en .

<https://w3id.org/dpv/owl#serialisation-rdf>
  a owl:NamedIndividual, ns4:ResourceDescriptor ;
  dc:format <https://www.iana.org/assignments/media-types/application/rdf+xml> ;
  dc:conformsTo rdf: ;
  dc:title "Data Privacy Vocabulary (DPV) - RDF/XML serialiation" ;
  ns4:hasArtifact <https://w3id.org/dpv/dpv/dpv-owl.rdf> ;
  ns4:hasRole <http://www.w3.org/ns/dx/prof/role/vocabulary> ;
  owl:sameAs <https://w3id.org/dpv#serialisation-rdf>, <https://w3id.org/dpv/dpv-owl#serialisation-rdf> .

<https://w3id.org/dpv/owl#VitalInterestOfNaturalPerson>
  a owl:Class, owl:NamedIndividual, <https://w3id.org/dpv/owl#LegalBasis> ;
  rdfs:subClassOf <https://w3id.org/dpv/owl#VitalInterest> ;
  dc:contributor _:genid4, _:genid1, _:genid6 ;
  dc:created "2021-04-21"^^xsd:date ;
  ns1:term_status "accepted"@en ;
  skos:definition "Activities are necessary or required to protect vital interests of a natural person"@en ;
  skos:prefLabel "Vital Interest of Natural Person"@en ;
  owl:sameAs <https://w3id.org/dpv#VitalInterestOfNaturalPerson>, <https://w3id.org/dpv/dpv-owl#VitalInterestOfNaturalPerson> .

<https://w3id.org/dpv/owl#DiscloseByTransmission>
  a owl:Class, owl:NamedIndividual, <https://w3id.org/dpv/owl#Processing> ;
  rdfs:subClassOf <https://w3id.org/dpv/owl#Disclose> ;
  dc:created "2019-05-07"^^xsd:date ;
  dc:source [
    a ns0:WebPage ;
    ns0:name "GDPR Art.4-2" ;
    ns0:url "https://eur-lex.europa.eu/eli/reg/2016/679/art_4/par_2/oj"
  ] ;
  ns1:term_status "accepted"@en ;
  skos:definition "to disclose data by means of transmission"@en ;
  skos:prefLabel "Disclose Data by Transmission"@en ;
  owl:sameAs <https://w3id.org/dpv#DiscloseByTransmission>, <https://w3id.org/dpv/dpv-owl#DiscloseByTransmission> .

skos:scopeNote a owl:AnnotationProperty .
<https://w3id.org/dpv/owl#Country>
  a owl:Class ;
  rdfs:subClassOf <https://w3id.org/dpv/owl#Location> ;
  dc:contributor _:genid4, _:genid1 ;
  dc:created "2022-01-19"^^xsd:date ;
  ns1:term_status "accepted"@en ;
  skos:definition "A political entity indicative of a sovereign or non-sovereign territorial state comprising of distinct geographical areas"@en ;
  skos:prefLabel "Country"@en ;
  skos:scopeNote "The definition of country is not intended for political interpretation. DPVCG welcomes alternate definitions based in existing sources with global scope, such as UN or ISO."@en ;
  owl:sameAs <https://w3id.org/dpv#Country>, <https://w3id.org/dpv/dpv-owl#Country> .

odrl:#partyConcepts
  a owl:NamedIndividual, skos:Collection ;
  skos:member odrl:Party, odrl:PartyCollection ;
  skos:prefLabel "Party"@en ;
  skos:scopeNote "ODRL Core Vocabulary Terms"@en .

<https://w3id.org/dpv/owl#DataSanitisationTechnique>
  a owl:Class, owl:NamedIndividual, <https://w3id.org/dpv/owl#TechnicalMeasure> ;
  rdfs:subClassOf <https://w3id.org/dpv/owl#TechnicalMeasure> ;
  dc:contributor _:genid1 ;
  dc:created "2022-08-17"^^xsd:date ;
  dc:source [
    a ns0:WebPage ;
    ns0:name "ENISA Reference Incident Classification Taxonomy 2018" ;
    ns0:url "https://www.enisa.europa.eu/publications/reference-incident-classification-taxonomy/"
  ] ;
  ns1:term_status "accepted"@en ;
  skos:definition "Cleaning or any removal or re-organisation of elements in data based on selective criteria"@en ;
  skos:prefLabel "Data Sanitisation Technique"@en ;
  owl:sameAs <https://w3id.org/dpv#DataSanitisationTechnique>, <https://w3id.org/dpv/dpv-owl#DataSanitisationTechnique> .

<https://w3id.org/dpv/owl#ActivityMonitoring>
  a owl:Class, owl:NamedIndividual, <https://w3id.org/dpv/owl#TechnicalMeasure> ;
  rdfs:subClassOf <https://w3id.org/dpv/owl#TechnicalMeasure> ;
  dc:contributor _:genid1 ;
  dc:created "2022-08-17"^^xsd:date ;
  dc:source [
    a ns0:WebPage ;
    ns0:name "ENISA Reference Incident Classification Taxonomy 2018" ;
    ns0:url "https://www.enisa.europa.eu/publications/reference-incident-classification-taxonomy/"
  ] ;
  ns1:term_status "accepted"@en ;
  skos:definition "Monitoring of activities including assessing whether they have been successfully initiated and completed"@en ;
  skos:prefLabel "Activity Monitoring"@en ;
  owl:sameAs <https://w3id.org/dpv#ActivityMonitoring>, <https://w3id.org/dpv/dpv-owl#ActivityMonitoring> .

<https://w3id.org/dpv/owl#LegalAgreement>
  a owl:Class, owl:NamedIndividual, <https://w3id.org/dpv/owl#LegalMeasure> ;
  rdfs:subClassOf odrl:Agreement, <https://w3id.org/dpv/owl#LegalMeasure> ;
  dc:contributor _:genid9, _:genid10, _:genid1, _:genid11 ;
  dc:created "2019-04-05"^^xsd:date ;
  dc:modified "2024-08-27"^^xsd:date ;
  ns1:term_status "sunset"@en ;
  skos:definition "A legally binding agreement"@en ;
  skos:prefLabel "Legal Agreement"@en ;
  owl:sameAs <https://w3id.org/dpv#LegalAgreement>, <https://w3id.org/dpv/dpv-owl#LegalAgreement> .

odrl:isPartOf
  a owl:NamedIndividual, skos:Concept, odrl:Operator ;
  rdfs:isDefinedBy odrl: ;
  rdfs:label "Is part of"@en ;
  skos:definition "A set-based operator indicating that a given value is contained by the right operand of the Constraint."@en .

<https://w3id.org/dpv/owl#DigitalSignatures>
  a owl:Class, owl:NamedIndividual, <https://w3id.org/dpv/owl#TechnicalMeasure> ;
  rdfs:subClassOf <https://w3id.org/dpv/owl#CryptographicMethods> ;
  dc:contributor _:genid1 ;
  dc:created "2022-08-17"^^xsd:date ;
  dc:source [
    a ns0:WebPage ;
    ns0:name "ENISA Reference Incident Classification Taxonomy 2018" ;
    ns0:url "https://www.enisa.europa.eu/publications/reference-incident-classification-taxonomy/"
  ] ;
  ns1:term_status "accepted"@en ;
  skos:definition "Expression and authentication of identity through digital information containing cryptographic signatures"@en ;
  skos:prefLabel "Digital Signatures"@en ;
  owl:sameAs <https://w3id.org/dpv#DigitalSignatures>, <https://w3id.org/dpv/dpv-owl#DigitalSignatures> .

<https://w3id.org/dpv/owl#Organise>
  a owl:Class, owl:NamedIndividual, <https://w3id.org/dpv/owl#Processing> ;
  rdfs:subClassOf <https://w3id.org/dpv/owl#Processing> ;
  dc:created "2019-05-07"^^xsd:date ;
  dc:source [
    a ns0:WebPage ;
    ns0:name "GDPR Art.4-2" ;
    ns0:url "https://eur-lex.europa.eu/eli/reg/2016/679/art_4/par_2/oj"
  ] ;
  ns1:term_status "accepted"@en ;
  skos:definition "to organize data for arranging or classifying"@en ;
  skos:prefLabel "Organise Data"@en ;
  owl:sameAs <https://w3id.org/dpv#Organise>, <https://w3id.org/dpv/dpv-owl#Organise> .

<https://w3id.org/dpv/owl#NotInvolved>
  a owl:Class, owl:NamedIndividual, <https://w3id.org/dpv/owl#InvolvementStatus> ;
  rdfs:subClassOf <https://w3id.org/dpv/owl#InvolvementStatus> ;
  dc:contributor _:genid4, _:genid1, _:genid25, _:genid6 ;
  dc:created "2024-05-10"^^xsd:date ;
  ns1:term_status "accepted"@en ;
  skos:definition "Status indicating the specified context is 'not' involved"@en ;
  skos:prefLabel "Not Involved"@en ;
  owl:sameAs <https://w3id.org/dpv#NotInvolved>, <https://w3id.org/dpv/dpv-owl#NotInvolved> .

odrl:#actionConcepts
  a owl:NamedIndividual, skos:Collection ;
  skos:member odrl:Action, odrl:action, odrl:implies, odrl:includedIn ;
  skos:prefLabel "Action"@en ;
  skos:scopeNote "ODRL Core Vocabulary Terms"@en .

<https://w3id.org/dpv/owl#hasGeographicCoverage>
  a owl:ObjectProperty ;
  rdfs:subPropertyOf <https://w3id.org/dpv/owl#hasScale> ;
  ns2:rangeIncludes <https://w3id.org/dpv/owl#GeographicCoverage> ;
  dc:contributor _:genid1 ;
  dc:created "2022-06-22"^^xsd:date ;
  ns1:term_status "accepted"@en ;
  skos:definition "Indicates the geographic coverage (of specified context)"@en ;
  skos:prefLabel "has geographic coverage"@en ;
  ns0:rangeIncludes <https://w3id.org/dpv/owl#GeographicCoverage> ;
  owl:sameAs <https://w3id.org/dpv#hasGeographicCoverage>, <https://w3id.org/dpv/dpv-owl#hasGeographicCoverage> .

<http://purl.org/spar/scoro/hasORCID> a owl:AnnotationProperty .
<https://w3id.org/dpv/owl#ControllerUninformed>
  a owl:Class, owl:NamedIndividual, <https://w3id.org/dpv/owl#EntityInformedStatus> ;
  rdfs:subClassOf <https://w3id.org/dpv/owl#EntityUninformed> ;
  dc:contributor _:genid4, _:genid1, _:genid25, _:genid6 ;
  dc:created "2024-05-10"^^xsd:date ;
  ns1:term_status "accepted"@en ;
  skos:definition "Status indicating Controller is uninformed i.e. has not been informed about the specified context"@en ;
  skos:prefLabel "Controller Uninformed"@en ;
  owl:sameAs <https://w3id.org/dpv#ControllerUninformed>, <https://w3id.org/dpv/dpv-owl#ControllerUninformed> .

<https://w3id.org/dpv/owl#RegulatorySandbox>
  a owl:Class, owl:NamedIndividual, <https://w3id.org/dpv/owl#OrganisationalMeasure> ;
  rdfs:subClassOf <https://w3id.org/dpv/owl#Safeguard> ;
  dc:contributor _:genid1 ;
  dc:created "2024-05-17"^^xsd:date ;
  dc:source [
    a ns0:WebPage ;
    ns0:name "EU Council Regulatory sandboxes and experimentation clauses as tools for better regulation" ;
    ns0:url "https://www.consilium.europa.eu/en/press/press-releases/2020/11/16/regulatory-sandboxes-and-experimentation-clauses-as-tools-for-better-regulation-council-adopts-conclusions/"
  ] ;
  ns1:term_status "accepted"@en ;
  skos:definition "Mechanism used by regulators and businesses for gauging the compatibility of regulations and innovative products, particularly in the context of digitalisation, in a controlled real-world environment with appropriate safeguards in place"@en ;
  skos:prefLabel "Regulatory Sandbox"@en ;
  owl:sameAs <https://w3id.org/dpv#RegulatorySandbox>, <https://w3id.org/dpv/dpv-owl#RegulatorySandbox> .

<https://w3id.org/dpv/owl#ContractualClauseNotFulfiled>
  a owl:Class, owl:NamedIndividual, <https://w3id.org/dpv/owl#ContractualClauseFulfilmentStatus> ;
  rdfs:subClassOf <https://w3id.org/dpv/owl#ContractualClauseFulfilmentStatus> ;
  dc:created "2024-08-27"^^xsd:date ;
  ns1:term_status "accepted"@en ;
  skos:definition "Status indicating the terms of the contractual clause have not yet been fulfiled in a manner that does not constitute a violation i.e. there is still an opportunity to complete them"@en ;
  skos:prefLabel "Contractual Clause Unfulfiled"@en ;
  owl:sameAs <https://w3id.org/dpv#ContractualClauseNotFulfiled>, <https://w3id.org/dpv/dpv-owl#ContractualClauseNotFulfiled> .

odrl:policyUsage
  a owl:NamedIndividual, skos:Concept, odrl:RightOperand ;
  rdfs:isDefinedBy odrl: ;
  rdfs:label "Policy Rule Usage"@en ;
  skos:definition "Indicates the actual datetime the action of the Rule was exercised."@en ;
  skos:note "This can be used to express constraints with a LeftOperand relative to the time the rule is exercised. Operators indicate before (lt, lteq), during (eq) or after (gt, gteq) the usage of the rule. <br />Example: <code>event lt policyUsage</code> expresses that the identified event must have happened before the action of the rule is exercised."@en ;
  skos:scopeNote "Non-Normative"@en .

<https://w3id.org/dpv/owl#JointDataControllers>
  a owl:Class ;
  rdfs:subClassOf <https://w3id.org/dpv/owl#DataController> ;
  dc:contributor _:genid4, _:genid1 ;
  dc:created "2022-02-02"^^xsd:date ;
  ns1:term_status "accepted"@en ;
  skos:definition "A group of Data Controllers that jointly determine the purposes and means of processing"@en ;
  skos:prefLabel "Joint Data Controllers"@en ;
  skos:scopeNote "While Joint Data Controllers operate together, they are made up of individually distinct legal entities. To indicate the membership of this group, hasDataController should be used to denote each Data Controller. The concept of Joint Data Controllers also allows specifying a single group as the 'Controller' and to specify role and responsibilities within that group for each entity using DPV's concepts (e.g. isImplementedByEntity)"@en ;
  owl:sameAs <https://w3id.org/dpv#JointDataControllers>, <https://w3id.org/dpv/dpv-owl#JointDataControllers> .

<https://w3id.org/dpv/owl#ContractRejected>
  a owl:Class, owl:NamedIndividual, <https://w3id.org/dpv/owl#ContractPreparationStatus> ;
  rdfs:subClassOf <https://w3id.org/dpv/owl#ContractPreparationStatus> ;
  dc:contributor _:genid4, _:genid1, _:genid17 ;
  dc:created "2025-01-09"^^xsd:date ;
  ns1:term_status "accepted"@en ;
  skos:definition "Status representing contract has been rejected and cannot be used for signing"@en ;
  skos:prefLabel "Contract Rejected"@en ;
  owl:sameAs <https://w3id.org/dpv#ContractRejected>, <https://w3id.org/dpv/dpv-owl#ContractRejected> .

<https://w3id.org/dpv/owl#Restrict>
  a owl:Class, owl:NamedIndividual, <https://w3id.org/dpv/owl#Processing> ;
  rdfs:subClassOf <https://w3id.org/dpv/owl#Transform> ;
  dc:created "2019-05-07"^^xsd:date ;
  dc:source [
    a ns0:WebPage ;
    ns0:name "GDPR Art.4-2" ;
    ns0:url "https://eur-lex.europa.eu/eli/reg/2016/679/art_4/par_2/oj"
  ] ;
  ns1:term_status "accepted"@en ;
  skos:definition "to apply a restriction on the processing of specific records"@en ;
  skos:prefLabel "Restrict Data"@en ;
  owl:sameAs <https://w3id.org/dpv#Restrict>, <https://w3id.org/dpv/dpv-owl#Restrict> .

<https://w3id.org/dpv/owl#ProhibitionFulfilled>
  a owl:Class, owl:NamedIndividual, <https://w3id.org/dpv/owl#RuleFulfilmentStatus> ;
  rdfs:subClassOf <https://w3id.org/dpv/owl#RuleFulfilled> ;
  dc:contributor _:genid1 ;
  dc:created "2024-09-10"^^xsd:date ;
  ns1:term_status "accepted"@en ;
  skos:definition "Status indicating a prohibition has been fulfilled i.e. the activity stated as being prohibited has not been carried out"@en ;
  skos:prefLabel "Prohibition Fulfilled"@en ;
  owl:sameAs <https://w3id.org/dpv#ProhibitionFulfilled>, <https://w3id.org/dpv/dpv-owl#ProhibitionFulfilled> .

<https://w3id.org/dpv/owl#FixedMultipleLocations>
  a owl:Class, owl:NamedIndividual, <https://w3id.org/dpv/owl#LocationFixture> ;
  rdfs:subClassOf <https://w3id.org/dpv/owl#FixedLocation> ;
  dc:contributor _:genid1 ;
  dc:created "2022-06-15"^^xsd:date ;
  dc:modified "2020-10-05"^^xsd:date ;
  ns1:term_status "accepted"@en ;
  skos:definition "Location that is fixed with multiple places e.g. multiple cities"@en ;
  skos:prefLabel "Fixed Multiple Locations"@en ;
  owl:sameAs <https://w3id.org/dpv#FixedMultipleLocations>, <https://w3id.org/dpv/dpv-owl#FixedMultipleLocations> .

<https://w3id.org/dpv/owl#ServiceRegistration>
  a owl:Class, owl:NamedIndividual, <https://w3id.org/dpv/owl#Purpose> ;
  rdfs:subClassOf <https://w3id.org/dpv/owl#ServiceProvision> ;
  dc:contributor _:genid4, _:genid5, _:genid1 ;
  dc:created "2020-11-04"^^xsd:date ;
  ns1:term_status "accepted"@en ;
  skos:definition "Purposes associated with registering users and collecting information required for providing a service"@en ;
  skos:prefLabel "Service Registration"@en ;
  skos:scopeNote "An example of service registration is to provide a form that collects information such as preferred language or media format for downloading a movie"@en ;
  owl:sameAs <https://w3id.org/dpv#ServiceRegistration>, <https://w3id.org/dpv/dpv-owl#ServiceRegistration> .

<https://w3id.org/dpv/owl#PIA>
  a owl:Class, owl:NamedIndividual, <https://w3id.org/dpv/owl#OrganisationalMeasure> ;
  rdfs:subClassOf <https://w3id.org/dpv/owl#ImpactAssessment> ;
  dc:contributor _:genid4, _:genid1, _:genid6 ;
  dc:created "2020-11-04"^^xsd:date ;
  ns1:term_status "accepted"@en ;
  skos:definition "Impact assessment regarding privacy risks"@en ;
  skos:prefLabel "Privacy Impact Assessment (PIA)"@en ;
  owl:sameAs <https://w3id.org/dpv#PIA>, <https://w3id.org/dpv/dpv-owl#PIA> .

<https://w3id.org/dpv/owl#PseudonymisedData>
  a owl:Class ;
  rdfs:subClassOf <https://w3id.org/dpv/owl#PersonalData> ;
  dc:contributor _:genid1 ;
  dc:created "2022-01-19"^^xsd:date ;
  ns1:term_status "accepted"@en ;
  skos:definition "Pseudonymised Data is data that has gone a partial or incomplete anonymisation process by replacing the identifiable information with artificial identifiers or 'pseudonyms', and is still considered as personal data"@en ;
  skos:prefLabel "Pseudonymised Data"@en ;
  owl:sameAs <https://w3id.org/dpv#PseudonymisedData>, <https://w3id.org/dpv/dpv-owl#PseudonymisedData> .

<https://w3id.org/dpv/owl#Scope>
  a owl:Class ;
  rdfs:subClassOf <https://w3id.org/dpv/owl#Context> ;
  dc:contributor _:genid1 ;
  dc:created "2022-06-15"^^xsd:date ;
  ns1:term_status "accepted"@en ;
  skos:definition "Indication of the extent or range or boundaries associated with(in) a context"@en ;
  skos:prefLabel "Scope"@en ;
  owl:sameAs <https://w3id.org/dpv#Scope>, <https://w3id.org/dpv/dpv-owl#Scope> .

<https://w3id.org/dpv/owl#hasConsequence>
  a owl:ObjectProperty ;
  ns2:rangeIncludes <https://w3id.org/dpv/owl#Consequence> ;
  dc:contributor _:genid4, _:genid5, _:genid1, _:genid17, _:genid15 ;
  dc:created "2020-11-04"^^xsd:date ;
  dc:modified "2021-09-21"^^xsd:date ;
  ns3:example <https://w3id.org/dpv/examples/owl#E0068>, <https://w3id.org/dpv/examples/owl#E0071> ;
  ns1:term_status "accepted"@en ;
  skos:definition "Indicates consequence(s) possible or arising from specified concept"@en ;
  skos:prefLabel "has consequence"@en ;
  skos:scopeNote "Removed plural suffix for consistency"@en ;
  ns0:rangeIncludes <https://w3id.org/dpv/owl#Consequence> ;
  owl:sameAs <https://w3id.org/dpv#hasConsequence>, <https://w3id.org/dpv/dpv-owl#hasConsequence> .

<https://w3id.org/dpv/owl#EULA>
  a owl:Class, owl:NamedIndividual, <https://w3id.org/dpv/owl#LegalBasis> ;
  rdfs:subClassOf <https://w3id.org/dpv/owl#LicenseAgreement> ;
  dc:created "2024-08-27"^^xsd:date ;
  ns1:term_status "accepted"@en ;
  skos:definition "End User License Agreement is a contract entered into between a software (or service) developer or provider with the (end-)user"@en ;
  skos:prefLabel "End User License Agreement (EULA)"@en ;
  owl:sameAs <https://w3id.org/dpv#EULA>, <https://w3id.org/dpv/dpv-owl#EULA> .

<https://w3id.org/dpv/owl#ControllerInformed>
  a owl:Class, owl:NamedIndividual, <https://w3id.org/dpv/owl#EntityInformedStatus> ;
  rdfs:subClassOf <https://w3id.org/dpv/owl#EntityInformed> ;
  dc:contributor _:genid4, _:genid1, _:genid25, _:genid6 ;
  dc:created "2024-05-10"^^xsd:date ;
  ns1:term_status "accepted"@en ;
  skos:definition "Status indicating Controller has been informed about the specified context"@en ;
  skos:prefLabel "Controller Informed"@en ;
  owl:sameAs <https://w3id.org/dpv#ControllerInformed>, <https://w3id.org/dpv/dpv-owl#ControllerInformed> .

odrl:target
  a owl:ObjectProperty, owl:NamedIndividual, skos:Concept ;
  rdfs:subPropertyOf odrl:relation ;
  rdfs:domain [
    a owl:Class ;
    owl:unionOf (
     odrl:Policy
     odrl:Rule
   )
  ] ;
  rdfs:range odrl:Asset ;
  rdfs:isDefinedBy odrl: ;
  rdfs:label "Target"@en ;
  skos:definition "The target property indicates the Asset that is the primary subject to which the Rule action directly applies."@en .

<https://w3id.org/dpv/owl#hasActiveEntity>
  a owl:ObjectProperty ;
  rdfs:subPropertyOf <https://w3id.org/dpv/owl#hasEntity> ;
  ns2:rangeIncludes <https://w3id.org/dpv/owl#Entity> ;
  dc:created "2024-05-11"^^xsd:date ;
  ns1:term_status "accepted"@en ;
  skos:definition "indicates the entity is actively involved in specified context"@en ;
  skos:prefLabel "has active entity"@en ;
  ns0:rangeIncludes <https://w3id.org/dpv/owl#Entity> ;
  owl:sameAs <https://w3id.org/dpv#hasActiveEntity>, <https://w3id.org/dpv/dpv-owl#hasActiveEntity> .

<https://w3id.org/dpv/owl#ContractAmendmentClause>
  a owl:Class, owl:NamedIndividual, <https://w3id.org/dpv/owl#ContractualClause> ;
  rdfs:subClassOf <https://w3id.org/dpv/owl#ContractualClause> ;
  dc:created "2024-08-27"^^xsd:date ;
  ns1:term_status "accepted"@en ;
  skos:definition "A provision describing how changes or modifications to the contract can be made and the process for implementing them"@en ;
  skos:prefLabel "Contract Amendment Clause"@en ;
  owl:sameAs <https://w3id.org/dpv#ContractAmendmentClause>, <https://w3id.org/dpv/dpv-owl#ContractAmendmentClause> .

<https://w3id.org/dpv/owl#Hospital>
  a owl:Class ;
  rdfs:subClassOf <https://w3id.org/dpv/owl#Organisation> ;
  dc:contributor _:genid25 ;
  dc:created "2024-12-01"^^xsd:date ;
  ns1:term_status "accepted"@en ;
  skos:definition "An organisation that provides comprehensive medical treatment, including emergency care, surgeries, and inpatient services"@en ;
  skos:prefLabel "Hospital"@en ;
  owl:sameAs <https://w3id.org/dpv#Hospital>, <https://w3id.org/dpv/dpv-owl#Hospital> .

<https://w3id.org/dpv/owl#Lawful>
  a owl:Class, owl:NamedIndividual, <https://w3id.org/dpv/owl#Lawfulness> ;
  rdfs:subClassOf <https://w3id.org/dpv/owl#Lawfulness> ;
  dc:contributor _:genid1 ;
  dc:created "2022-10-19"^^xsd:date ;
  ns1:term_status "accepted"@en ;
  skos:definition "State of being lawful or legally compliant"@en ;
  skos:prefLabel "Lawful"@en ;
  owl:sameAs <https://w3id.org/dpv#Lawful>, <https://w3id.org/dpv/dpv-owl#Lawful> .

odrl:ensureExclusivity
  a owl:NamedIndividual, skos:Concept, odrl:Action ;
  odrl:includedIn odrl:use ;
  rdfs:isDefinedBy odrl: ;
  rdfs:label "Ensure Exclusivity"@en ;
  skos:definition "To ensure that the Rule on the Asset is exclusive."@en ;
  skos:note "If used as a Duty, the assignee should be explicitly indicated as the party that is ensuring the exclusivity of the Rule."@en ;
  skos:scopeNote "Non-Normative"@en .

odrl:timeInterval
  a owl:NamedIndividual, skos:Concept, odrl:LeftOperand ;
  rdfs:isDefinedBy odrl: ;
  rdfs:label "Recurring Time Interval"@en ;
  skos:definition "A recurring period of time before the next execution of the action of the Rule. Right operand value MUST be an xsd:duration as defined by [[xmlschema11-2]]."@en ;
  skos:note "Only the eq operator SHOULD be used. <br />Example: <code>timeInterval eq P7D</code> indicates a recurring 7 day period." ;
  skos:scopeNote "Non-Normative"@en .

<https://w3id.org/dpv/owl#Safeguard>
  a owl:Class, owl:NamedIndividual, <https://w3id.org/dpv/owl#OrganisationalMeasure> ;
  rdfs:subClassOf <https://w3id.org/dpv/owl#OrganisationalMeasure> ;
  dc:contributor _:genid4, _:genid1, _:genid6, _:genid21 ;
  dc:created "2021-09-22"^^xsd:date ;
  ns1:term_status "accepted"@en ;
  skos:definition "A safeguard is a precautionary measure for the protection against or mitigation of negative effects"@en ;
  skos:prefLabel "Safeguard"@en ;
  skos:scopeNote "This concept is relevant given the requirement to assert safeguards in cross-border data transfers"@en ;
  owl:sameAs <https://w3id.org/dpv#Safeguard>, <https://w3id.org/dpv/dpv-owl#Safeguard> .

<https://w3id.org/dpv/owl#DataReusePolicy>
  a owl:Class, owl:NamedIndividual, <https://w3id.org/dpv/owl#OrganisationalMeasure> ;
  rdfs:subClassOf <https://w3id.org/dpv/owl#DataProcessingPolicy> ;
  dc:contributor _:genid1 ;
  dc:created "2024-04-14"^^xsd:date ;
  ns1:term_status "accepted"@en ;
  skos:definition "Policy regarding reuse of data i.e. using data for purposes other than its initial purpose"@en ;
  skos:prefLabel "Data Reuse Policy"@en ;
  skos:scopeNote "This policy can be used to describe the procedures associated with undertaking such reuse of data, for example to assess its legality and the compatibility of the initial and subsequent purposes"@en ;
  owl:sameAs <https://w3id.org/dpv#DataReusePolicy>, <https://w3id.org/dpv/dpv-owl#DataReusePolicy> .

<https://w3id.org/dpv/owl#hasDataVolume>
  a owl:ObjectProperty ;
  rdfs:subPropertyOf <https://w3id.org/dpv/owl#hasScale> ;
  ns2:rangeIncludes <https://w3id.org/dpv/owl#DataVolume> ;
  dc:contributor _:genid1 ;
  dc:created "2022-06-22"^^xsd:date ;
  ns1:term_status "accepted"@en ;
  skos:definition "Indicates the volume of data"@en ;
  skos:prefLabel "has data volume"@en ;
  ns0:rangeIncludes <https://w3id.org/dpv/owl#DataVolume> ;
  owl:sameAs <https://w3id.org/dpv#hasDataVolume>, <https://w3id.org/dpv/dpv-owl#hasDataVolume> .

<https://w3id.org/dpv/owl#hasSensitivityLevel>
  a owl:ObjectProperty ;
  ns2:rangeIncludes <https://w3id.org/dpv/owl#SensitivityLevel> ;
  dc:contributor _:genid1 ;
  dc:created "2023-08-24"^^xsd:date ;
  ns1:term_status "accepted"@en ;
  skos:definition "Indicates the associated level of sensitivity"@en ;
  skos:prefLabel "has sensitivity level"@en ;
  ns0:rangeIncludes <https://w3id.org/dpv/owl#SensitivityLevel> ;
  owl:sameAs <https://w3id.org/dpv#hasSensitivityLevel>, <https://w3id.org/dpv/dpv-owl#hasSensitivityLevel> .

odrl:purpose
  a owl:Class, owl:NamedIndividual, skos:Concept, odrl:LeftOperand ;
  rdfs:isDefinedBy odrl: ;
  rdfs:label "Purpose"@en ;
  skos:definition "A defined purpose for exercising the action of the Rule."@en ;
  skos:note "Example: Educational use."@en ;
  skos:scopeNote "Non-Normative"@en .

<https://w3id.org/dpv/owl#ForProfitOrganisation>
  a owl:Class ;
  rdfs:subClassOf <https://w3id.org/dpv/owl#Organisation> ;
  dc:contributor _:genid1 ;
  dc:created "2022-02-02"^^xsd:date ;
  dc:modified "2020-10-05"^^xsd:date ;
  ns1:term_status "accepted"@en ;
  skos:definition "An organisation that aims to achieve profit as its primary goal"@en ;
  skos:prefLabel "For-Profit Organisation"@en ;
  owl:sameAs <https://w3id.org/dpv#ForProfitOrganisation>, <https://w3id.org/dpv/dpv-owl#ForProfitOrganisation> .

odrl:delete
  a owl:NamedIndividual, skos:Concept, odrl:Action ;
  odrl:includedIn odrl:use ;
  rdfs:isDefinedBy odrl: ;
  rdfs:label "Delete"@en ;
  skos:definition "To permanently remove all copies of the Asset after it has been used."@en ;
  skos:note "Use a constraint to define under which conditions the Asset must be deleted."@en ;
  skos:scopeNote "Non-Normative"@en .

<https://w3id.org/dpv/owl#ContractBreached>
  a owl:Class, owl:NamedIndividual, <https://w3id.org/dpv/owl#ContractTerminationStatus> ;
  rdfs:subClassOf <https://w3id.org/dpv/owl#ContractTerminationStatus> ;
  dc:contributor _:genid4, _:genid1, _:genid17 ;
  dc:created "2025-01-09"^^xsd:date ;
  ns1:term_status "accepted"@en ;
  skos:definition "Status representing contract being breached where its terms are not fulfiled or are violated with legal consequences"@en ;
  skos:prefLabel "Contract Breached"@en ;
  owl:sameAs <https://w3id.org/dpv#ContractBreached>, <https://w3id.org/dpv/dpv-owl#ContractBreached> .

<https://w3id.org/dpv/owl#PhysicalMeasure>
  a owl:Class ;
  rdfs:subClassOf <https://w3id.org/dpv/owl#TechnicalOrganisationalMeasure> ;
  dc:created "2023-12-10"^^xsd:date ;
  dc:modified "2023-12-10"^^xsd:date ;
  ns1:term_status "accepted"@en ;
  skos:definition "Physical measures used to safeguard and ensure good practices in connection with data and technologies"@en ;
  skos:prefLabel "Physical Measure"@en ;
  owl:sameAs <https://w3id.org/dpv#PhysicalMeasure>, <https://w3id.org/dpv/dpv-owl#PhysicalMeasure> .

<https://w3id.org/dpv/owl#ContractualClauseViolated>
  a owl:Class, owl:NamedIndividual, <https://w3id.org/dpv/owl#ContractualClauseFulfilmentStatus> ;
  rdfs:subClassOf <https://w3id.org/dpv/owl#ContractualClauseFulfilmentStatus> ;
  dc:created "2024-08-27"^^xsd:date ;
  ns1:term_status "accepted"@en ;
  skos:definition "Status indicating the terms of the contractual clause have been violated"@en ;
  skos:prefLabel "Contractual Clause Breached"@en ;
  owl:sameAs <https://w3id.org/dpv#ContractualClauseViolated>, <https://w3id.org/dpv/dpv-owl#ContractualClauseViolated> .

<https://w3id.org/dpv/owl#AuditRequested>
  a owl:Class, owl:NamedIndividual, <https://w3id.org/dpv/owl#AuditStatus> ;
  rdfs:subClassOf <https://w3id.org/dpv/owl#AuditStatus> ;
  dc:contributor _:genid1 ;
  dc:created "2022-05-18"^^xsd:date ;
  ns1:term_status "accepted"@en ;
  skos:definition "State of an audit being requested whose outcome is not yet known"@en ;
  skos:prefLabel "Audit Requested"@en ;
  owl:sameAs <https://w3id.org/dpv#AuditRequested>, <https://w3id.org/dpv/dpv-owl#AuditRequested> .

<https://w3id.org/dpv/owl#DigitalRightsManagement>
  a owl:Class, owl:NamedIndividual, <https://w3id.org/dpv/owl#TechnicalMeasure> ;
  rdfs:subClassOf <https://w3id.org/dpv/owl#TechnicalMeasure> ;
  dc:contributor _:genid1 ;
  dc:created "2022-08-17"^^xsd:date ;
  dc:source [
    a ns0:WebPage ;
    ns0:name "ENISA Reference Incident Classification Taxonomy 2018" ;
    ns0:url "https://www.enisa.europa.eu/publications/reference-incident-classification-taxonomy/"
  ] ;
  ns1:term_status "accepted"@en ;
  skos:definition "Management of access, use, and other operations associated with digital content"@en ;
  skos:prefLabel "Digital Rights Management"@en ;
  owl:sameAs <https://w3id.org/dpv#DigitalRightsManagement>, <https://w3id.org/dpv/dpv-owl#DigitalRightsManagement> .

<https://w3id.org/dpv/owl#SensitiveNonPersonalData>
  a owl:Class ;
  rdfs:subClassOf <https://w3id.org/dpv/owl#SensitiveData> ;
  dc:created "2024-02-14"^^xsd:date ;
  dc:source "DGA 30(a)"@en ;
  ns1:term_status "accepted"@en ;
  skos:definition "Non-personal data deemed sensitive"@en ;
  skos:prefLabel "Sensitive Non Personal Data"@en ;
  owl:sameAs <https://w3id.org/dpv#SensitiveNonPersonalData>, <https://w3id.org/dpv/dpv-owl#SensitiveNonPersonalData> .

<https://w3id.org/dpv/owl#GovernanceProcedures>
  a owl:Class, owl:NamedIndividual, <https://w3id.org/dpv/owl#OrganisationalMeasure> ;
  rdfs:subClassOf <https://w3id.org/dpv/owl#OrganisationalMeasure> ;
  dc:contributor _:genid1 ;
  dc:created "2022-08-17"^^xsd:date ;
  dc:source [
    a ns0:WebPage ;
    ns0:name "ENISA 5G Cybersecurity Standards" ;
    ns0:url "https://www.enisa.europa.eu/publications/5g-cybersecurity-standards"
  ] ;
  ns1:term_status "accepted"@en ;
  skos:definition "Procedures related to governance (e.g. organisation, unit, team, process, system)"@en ;
  skos:prefLabel "Governance Procedures"@en ;
  owl:sameAs <https://w3id.org/dpv#GovernanceProcedures>, <https://w3id.org/dpv/dpv-owl#GovernanceProcedures> .

<https://w3id.org/dpv/owl#ResearchAndDevelopment>
  a owl:Class, owl:NamedIndividual, <https://w3id.org/dpv/owl#Purpose> ;
  rdfs:subClassOf <https://w3id.org/dpv/owl#Purpose> ;
  dc:contributor _:genid13, _:genid14, _:genid1, _:genid15, _:genid16, _:genid11 ;
  dc:created "2019-04-05"^^xsd:date ;
  ns1:term_status "accepted"@en ;
  skos:definition "Purposes associated with conducting research and development for new methods, products, or services"@en ;
  skos:prefLabel "Research and Development"@en ;
  owl:sameAs <https://w3id.org/dpv#ResearchAndDevelopment>, <https://w3id.org/dpv/dpv-owl#ResearchAndDevelopment> .

odrl:relativeSpatialPosition
  a owl:NamedIndividual, skos:Concept, odrl:LeftOperand ;
  rdfs:isDefinedBy odrl: ;
  rdfs:label "Relative Spatial Asset Position"@en ;
  skos:broaderTransitive odrl:relativePosition ;
  skos:definition "The relative spatial positions - expressed as percentages of full values - of four corners of a rectangle on a 2D-canvas or the eight corners of a cuboid in a 3D-space of the target Asset."@en ;
  skos:note "See also Absolute Spatial Asset Position."@en ;
  skos:scopeNote "Non-Normative"@en .

foaf:homepage a owl:AnnotationProperty .
<https://w3id.org/dpv/owl#CodeOfConduct>
  a owl:Class, owl:NamedIndividual, <https://w3id.org/dpv/owl#OrganisationalMeasure> ;
  rdfs:subClassOf <https://w3id.org/dpv/owl#GuidelinesPrinciple> ;
  dc:contributor _:genid9, _:genid10, _:genid1, _:genid11 ;
  dc:created "2019-04-05"^^xsd:date ;
  ns1:term_status "accepted"@en ;
  skos:definition "A set of rules or procedures outlining the norms and practices for conducting activities"@en ;
  skos:prefLabel "Code of Conduct"@en ;
  owl:sameAs <https://w3id.org/dpv#CodeOfConduct>, <https://w3id.org/dpv/dpv-owl#CodeOfConduct> .

<https://w3id.org/dpv/owl#ServiceProvision>
  a owl:Class, owl:NamedIndividual, <https://w3id.org/dpv/owl#Purpose> ;
  rdfs:subClassOf <https://w3id.org/dpv/owl#Purpose> ;
  dc:contributor _:genid13, _:genid14, _:genid1, _:genid15, _:genid16, _:genid11 ;
  dc:created "2019-04-05"^^xsd:date ;
  ns1:term_status "accepted"@en ;
  skos:definition "Purposes associated with providing service or product or activities"@en ;
  skos:prefLabel "Service Provision"@en ;
  owl:sameAs <https://w3id.org/dpv#ServiceProvision>, <https://w3id.org/dpv/dpv-owl#ServiceProvision> .

odrl:payeeParty a owl:ObjectProperty, owl:NamedIndividual, skos:Concept .
<https://www.iana.org/assignments/media-types/application/rdf+xml> a owl:NamedIndividual .
<https://w3id.org/dpv/owl#PersonnelOffboarding>
  a owl:Class, owl:NamedIndividual, <https://w3id.org/dpv/owl#Purpose> ;
  rdfs:subClassOf <https://w3id.org/dpv/owl#PersonnelManagement> ;
  dc:created "2024-12-01"^^xsd:date ;
  ns1:term_status "accepted"@en ;
  skos:definition "Purposes associated with offboarding of personnel i.e. activities and processes carried out when the person is exiting the company or role"@en ;
  skos:prefLabel "Personnel Offboarding"@en ;
  owl:sameAs <https://w3id.org/dpv#PersonnelOffboarding>, <https://w3id.org/dpv/dpv-owl#PersonnelOffboarding> .

<https://w3id.org/dpv/owl#ConsentRequestDeferred>
  a owl:Class, owl:NamedIndividual, <https://w3id.org/dpv/owl#ConsentStatus> ;
  rdfs:subClassOf <https://w3id.org/dpv/owl#ConsentStatusInvalidForProcessing> ;
  dc:contributor _:genid4, _:genid1, _:genid17, _:genid6 ;
  dc:created "2022-06-22"^^xsd:date ;
  dc:source [
    a ns0:WebPage ;
    ns0:name "GConsent" ;
    ns0:url "https://w3id.org/GConsent"
  ] ;
  ns1:term_status "accepted"@en ;
  skos:definition "State where a request for consent has been deferred without a decision"@en ;
  skos:prefLabel "Consent Request Deferred"@en ;
  skos:scopeNote "An example of this state is when the individual closes or dismisses a notice without making a decision. This state is intended for making the distinction between a notice being provided (as a consent request) and the individual interacting with the notice without making a decision - where the 'ignoring of a notice' is taken as consent being neither given nor refused"@en ;
  owl:sameAs <https://w3id.org/dpv#ConsentRequestDeferred>, <https://w3id.org/dpv/dpv-owl#ConsentRequestDeferred> .

odrl:Operator
  a owl:Class, owl:NamedIndividual, skos:Concept ;
  rdfs:isDefinedBy odrl: ;
  rdfs:label "Operator"@en ;
  skos:definition "Operator for constraint expression."@en ;
  skos:note "Instances of the Operator class representing relational operators."@en .

odrl:duty
  a owl:ObjectProperty, owl:NamedIndividual, skos:Concept ;
  rdfs:domain odrl:Permission ;
  rdfs:range odrl:Duty ;
  rdfs:isDefinedBy odrl: ;
  rdfs:label "Has Duty"@en ;
  skos:definition "Relates an individual Duty to a Permission."@en ;
  skos:note "A Duty is a pre-condition which must be fulfilled in order to receive the Permission."@en .

<https://w3id.org/dpv/owl#IdentityAuthentication>
  a owl:Class, owl:NamedIndividual, <https://w3id.org/dpv/owl#Purpose> ;
  rdfs:subClassOf <https://w3id.org/dpv/owl#EnforceSecurity> ;
  dc:contributor _:genid4, _:genid5, _:genid1 ;
  dc:created "2024-04-14"^^xsd:date ;
  ns1:term_status "accepted"@en ;
  skos:definition "Purposes associated with performing authentication based on identity as a form of security"@en ;
  skos:prefLabel "Identity Authentication"@en ;
  owl:sameAs <https://w3id.org/dpv#IdentityAuthentication>, <https://w3id.org/dpv/dpv-owl#IdentityAuthentication> .

<https://w3id.org/dpv/owl#Delete>
  a owl:Class, owl:NamedIndividual, <https://w3id.org/dpv/owl#Processing> ;
  rdfs:subClassOf <https://w3id.org/dpv/owl#Remove> ;
  dc:contributor _:genid1 ;
  dc:created "2024-04-14"^^xsd:date ;
  ns1:term_status "accepted"@en ;
  skos:definition "to remove data in a logical fashion i.e. with the possibility of retrieval"@en ;
  skos:prefLabel "Delete Data"@en ;
  owl:sameAs <https://w3id.org/dpv#Delete>, <https://w3id.org/dpv/dpv-owl#Delete> .

odrl:#conflictConcepts
  a owl:NamedIndividual, skos:Collection ;
  skos:member odrl:ConflictTerm, odrl:conflict, odrl:invalid, odrl:perm, odrl:prohibit ;
  skos:prefLabel "Policy Conflict Strategy"@en ;
  skos:scopeNote "ODRL Core Vocabulary Terms"@en .

odrl:hasPart
  a owl:NamedIndividual, skos:Concept, odrl:Operator ;
  rdfs:isDefinedBy odrl: ;
  rdfs:label "Has part"@en ;
  skos:definition "A set-based operator indicating that a given value contains the right operand of the Constraint."@en .

<https://w3id.org/dpv/owl#CommerciallyConfidentialData>
  a owl:Class ;
  rdfs:subClassOf <https://w3id.org/dpv/owl#Data> ;
  dc:created "2024-02-14"^^xsd:date ;
  dc:source "DGA 6.5(c)"@en ;
  ns1:term_status "accepted"@en ;
  skos:definition "Data protected through Commercial Confidentiality Agreements"@en ;
  skos:prefLabel "Commercially Confidential Data"@en ;
  owl:sameAs <https://w3id.org/dpv#CommerciallyConfidentialData>, <https://w3id.org/dpv/dpv-owl#CommerciallyConfidentialData> .

<https://w3id.org/dpv/owl#MentallyVulnerableHuman>
  a owl:Class, owl:NamedIndividual, <https://w3id.org/dpv/owl#HumanSubject> ;
  rdfs:subClassOf <https://w3id.org/dpv/owl#VulnerableHuman> ;
  dc:contributor _:genid1 ;
  dc:created "2024-12-17"^^xsd:date ;
  ns1:term_status "accepted"@en ;
  skos:definition "Humans that are considered mentally vulnerable within the context"@en ;
  skos:prefLabel "Mentally Vulnerable Human"@en ;
  owl:sameAs <https://w3id.org/dpv#MentallyVulnerableHuman>, <https://w3id.org/dpv/dpv-owl#MentallyVulnerableHuman> .

<https://w3id.org/dpv/owl#DataSubjectContract>
  a owl:Class, owl:NamedIndividual, <https://w3id.org/dpv/owl#LegalBasis> ;
  rdfs:subClassOf <https://w3id.org/dpv/owl#DataProcessingAgreement> ;
  dc:created "2023-12-10"^^xsd:date ;
  dc:modified "2024-08-27"^^xsd:date ;
  ns1:term_status "sunset"@en ;
  skos:definition "Creation, completion, fulfilment, or performance of a contract, with the Data Controller and Data Subject as parties, and involving specified processing of data or technologies. NOTE: This concept is being deprecated - use dpv:ControllerDataSubjectAgreement which has a more explicit definition of the entities involved and the intent of the contract"@en ;
  skos:prefLabel "Data Subject Contract"@en ;
  owl:sameAs <https://w3id.org/dpv#DataSubjectContract>, <https://w3id.org/dpv/dpv-owl#DataSubjectContract> .

<https://w3id.org/dpv/owl#LegalBasis>
  a owl:Class ;
  dc:created "2019-04-05"^^xsd:date ;
  dc:modified "2020-11-04"^^xsd:date ;
  ns3:example <https://w3id.org/dpv/examples/owl#E0014> ;
  ns1:term_status "accepted"@en ;
  skos:definition "Legal basis used to justify processing of data or use of technology in accordance with a law"@en ;
  skos:prefLabel "Legal Basis"@en ;
  skos:scopeNote "Legal basis (plural: legal bases) are defined by legislations and regulations, whose applicability is usually restricted to specific jurisdictions which can be represented using dpv:hasJurisdiction or dpv:hasLaw. Legal basis can be used without such declarations, e.g. 'Consent', however their interpretation will require association with a law, e.g. 'EU GDPR'."@en ;
  owl:sameAs <https://w3id.org/dpv#LegalBasis>, <https://w3id.org/dpv/dpv-owl#LegalBasis> .

<https://w3id.org/dpv/owl#AuthorityInformed>
  a owl:Class, owl:NamedIndividual, <https://w3id.org/dpv/owl#EntityInformedStatus> ;
  rdfs:subClassOf <https://w3id.org/dpv/owl#EntityInformed> ;
  dc:contributor _:genid4, _:genid1, _:genid25, _:genid6 ;
  dc:created "2024-05-10"^^xsd:date ;
  ns1:term_status "accepted"@en ;
  skos:definition "Status indicating Authority has been informed about the specified context"@en ;
  skos:prefLabel "Authority Informed"@en ;
  owl:sameAs <https://w3id.org/dpv#AuthorityInformed>, <https://w3id.org/dpv/dpv-owl#AuthorityInformed> .

<https://w3id.org/dpv/owl#SpecialCategoryPersonalData>
  a owl:Class ;
  rdfs:subClassOf <https://w3id.org/dpv/owl#SensitivePersonalData> ;
  dc:contributor _:genid1, _:genid15, _:genid16 ;
  dc:created "2019-05-07"^^xsd:date ;
  dc:modified "2022-01-19"^^xsd:date ;
  dc:source [
    a ns0:WebPage ;
    ns0:name "GDPR Art.9-1" ;
    ns0:url "https://eur-lex.europa.eu/eli/reg/2016/679/art_9/par_1/oj"
  ] ;
  ns3:example <https://w3id.org/dpv/examples/owl#E0010>, <https://w3id.org/dpv/examples/owl#E0045> ;
  ns1:term_status "accepted"@en ;
  skos:definition "Sensitive Personal Data whose use requires specific additional legal permission or justification"@en ;
  skos:prefLabel "Special Category Personal Data"@en ;
  skos:scopeNote "The term 'special category' is based on GDPR Art.9, but should not be considered as exclusive to it. DPV considers all Special Categories to also be Sensitive, but whose use is either prohibited or regulated and therefore requires additional legal basis for justification that is separate from that for general personal data."@en ;
  owl:sameAs <https://w3id.org/dpv#SpecialCategoryPersonalData>, <https://w3id.org/dpv/dpv-owl#SpecialCategoryPersonalData> .

odrl:assignerOf
  a owl:ObjectProperty, owl:NamedIndividual, skos:Concept ;
  rdfs:domain odrl:Party ;
  rdfs:range odrl:Policy ;
  rdfs:isDefinedBy odrl: ;
  rdfs:label "Assigner Of"@en ;
  skos:definition "Identifies an ODRL Policy for which the identified Party undertakes the assigner functional role."@en ;
  skos:note "When assignerOf has been asserted between a metadata expression and an ODRL Policy, the Party being identified MUST be inferred to undertake the assigner functional role of all the Rules of that Policy."@en .

<https://w3id.org/dpv/owl#CannotChallengeProcessOutput>
  a owl:Class, owl:NamedIndividual, <https://w3id.org/dpv/owl#EntityNonPermissiveInvolvement> ;
  rdfs:subClassOf <https://w3id.org/dpv/owl#EntityNonPermissiveInvolvement> ;
  dc:contributor _:genid1, _:genid25, _:genid19 ;
  dc:created "2024-05-11"^^xsd:date ;
  ns1:term_status "accepted"@en ;
  skos:definition "Involvement where entity cannot challenge the output of specified context"@en ;
  skos:prefLabel "Cannot Challenge Process Output"@en ;
  skos:scopeNote "Challenge refers to raising questions about validity, necessity, correctness, or other similar 'trustworthiness' attributes regarding the output of the process or plan or implementation (where output is distinct from the process itself)"@en ;
  owl:sameAs <https://w3id.org/dpv#CannotChallengeProcessOutput>, <https://w3id.org/dpv/dpv-owl#CannotChallengeProcessOutput> .

<https://w3id.org/dpv/owl#hasImpactAssessment>
  a owl:ObjectProperty ;
  rdfs:subPropertyOf <https://w3id.org/dpv/owl#hasAssessment> ;
  ns2:rangeIncludes <https://w3id.org/dpv/owl#ImpactAssessment> ;
  dc:contributor _:genid1 ;
  dc:created "2024-04-14"^^xsd:date ;
  ns1:term_status "accepted"@en ;
  skos:definition "Indicates an impact assessment associated with the specific context"@en ;
  skos:prefLabel "has impact assessment"@en ;
  ns0:rangeIncludes <https://w3id.org/dpv/owl#ImpactAssessment> ;
  owl:sameAs <https://w3id.org/dpv#hasImpactAssessment>, <https://w3id.org/dpv/dpv-owl#hasImpactAssessment> .

<https://w3id.org/dpv/owl#RecruitmentInterviewAssessment>
  a owl:Class, owl:NamedIndividual, <https://w3id.org/dpv/owl#Purpose> ;
  rdfs:subClassOf <https://w3id.org/dpv/owl#RecruitmentInterviewManagement> ;
  dc:created "2024-12-01"^^xsd:date ;
  ns1:term_status "accepted"@en ;
  skos:definition "Purposes associated with assessment of interviews, including assessment of people and information, for recruitment"@en ;
  skos:prefLabel "Recruitment Interview Assessment"@en ;
  owl:sameAs <https://w3id.org/dpv#RecruitmentInterviewAssessment>, <https://w3id.org/dpv/dpv-owl#RecruitmentInterviewAssessment> .

<https://eu-upcast.github.io/vocabulary/index-en.html#hasStartTime>
  a owl:DatatypeProperty ;
  rdfs:domain odrl:Action ;
  rdfs:range xsd:dateTime ;
  rdfs:label "start time"@en .

<https://w3id.org/dpv/owl#ImproveHealthcare>
  a owl:Class, owl:NamedIndividual, <https://w3id.org/dpv/owl#Purpose> ;
  rdfs:subClassOf <https://w3id.org/dpv/owl#PublicBenefit> ;
  dc:contributor _:genid5, _:genid1 ;
  dc:created "2024-02-14"^^xsd:date ;
  dc:source "DGA 2.16"@en ;
  ns1:term_status "accepted"@en ;
  skos:definition "Purposes associated with improving healthcare systems such as for personalised treatments and curing chronic diseases"@en ;
  skos:prefLabel "Improve Healthcare"@en ;
  owl:sameAs <https://w3id.org/dpv#ImproveHealthcare>, <https://w3id.org/dpv/dpv-owl#ImproveHealthcare> .

<https://w3id.org/dpv/owl#TechnicalServiceProvision>
  a owl:Class, owl:NamedIndividual, <https://w3id.org/dpv/owl#Purpose> ;
  rdfs:subClassOf <https://w3id.org/dpv/owl#ServiceProvision> ;
  dc:contributor _:genid1 ;
  dc:created "2021-09-08"^^xsd:date ;
  ns1:term_status "accepted"@en ;
  skos:definition "Purposes associated with managing and providing technical processes and functions necessary for delivering services"@en ;
  skos:prefLabel "Technical Service Provision"@en ;
  owl:sameAs <https://w3id.org/dpv#TechnicalServiceProvision>, <https://w3id.org/dpv/dpv-owl#TechnicalServiceProvision> .

<https://w3id.org/dpv/owl#NetworkProxyRouting>
  a owl:Class, owl:NamedIndividual, <https://w3id.org/dpv/owl#TechnicalMeasure> ;
  rdfs:subClassOf <https://w3id.org/dpv/owl#SecurityMethod> ;
  dc:contributor _:genid1 ;
  dc:created "2022-08-17"^^xsd:date ;
  dc:source [
    a ns0:WebPage ;
    ns0:name "ENISA Data Protection Engineering" ;
    ns0:url "https://www.enisa.europa.eu/publications/data-protection-engineering"
  ] ;
  ns1:term_status "accepted"@en ;
  skos:definition "Use of network routing using proxy"@en ;
  skos:prefLabel "Network Proxy Routing"@en ;
  owl:sameAs <https://w3id.org/dpv#NetworkProxyRouting>, <https://w3id.org/dpv/dpv-owl#NetworkProxyRouting> .

<https://w3id.org/dpv/owl#EmergencyServiceProvider>
  a owl:Class ;
  rdfs:subClassOf <https://w3id.org/dpv/owl#Organisation> ;
  dc:contributor _:genid25 ;
  dc:created "2024-12-01"^^xsd:date ;
  ns1:term_status "accepted"@en ;
  skos:definition "An organisation tasked with providing emergency services such as by responding rapidly to urgent situations to protect lives, property, and the environment"@en ;
  skos:prefLabel "Emergency Service Provider"@en ;
  owl:sameAs <https://w3id.org/dpv#EmergencyServiceProvider>, <https://w3id.org/dpv/dpv-owl#EmergencyServiceProvider> .

<https://w3id.org/dpv/owl#NearlyGlobalScale>
  a owl:Class, owl:NamedIndividual, <https://w3id.org/dpv/owl#GeographicCoverage> ;
  rdfs:subClassOf <https://w3id.org/dpv/owl#GeographicCoverage> ;
  dc:contributor _:genid1 ;
  dc:created "2022-06-15"^^xsd:date ;
  ns1:term_status "accepted"@en ;
  skos:definition "Geographic coverage nearly spanning the entire globe"@en ;
  skos:prefLabel "Nearly Global Scale"@en ;
  owl:sameAs <https://w3id.org/dpv#NearlyGlobalScale>, <https://w3id.org/dpv/dpv-owl#NearlyGlobalScale> .

<https://w3id.org/dpv/owl#ContractualClause>
  a owl:Class ;
  dc:created "2024-08-27"^^xsd:date ;
  ns3:example <https://w3id.org/dpv/examples/owl#E0078> ;
  ns1:term_status "accepted"@en ;
  skos:definition "A part or component within a contract that outlines its specifics"@en ;
  skos:prefLabel "Contractual Clause"@en ;
  owl:sameAs <https://w3id.org/dpv#ContractualClause>, <https://w3id.org/dpv/dpv-owl#ContractualClause> .

<https://w3id.org/dpv/owl#ExpressedConsent>
  a owl:Class, owl:NamedIndividual, <https://w3id.org/dpv/owl#LegalBasis> ;
  rdfs:subClassOf <https://w3id.org/dpv/owl#InformedConsent> ;
  dc:contributor _:genid4, _:genid1, _:genid17, _:genid6 ;
  dc:created "2022-06-21"^^xsd:date ;
  ns3:example <https://w3id.org/dpv/examples/owl#E0018> ;
  ns1:term_status "accepted"@en ;
  skos:definition "Consent that is expressed through an action intended to convey a consenting decision"@en ;
  skos:prefLabel "Expressed Consent"@en ;
  skos:scopeNote "Expressed consent requires the individual take a specific and unambiguous action that directly indicates their consent. This action may be a part of other processes such as setting preferences, or agreeing to a contract, or other matters not relating to consent. An example of expressed consent is interacting with a checkbox within a dashboard or clicking a button on a web form"@en ;
  owl:sameAs <https://w3id.org/dpv#ExpressedConsent>, <https://w3id.org/dpv/dpv-owl#ExpressedConsent> .

<https://w3id.org/dpv/owl#EncryptionAtRest>
  a owl:Class, owl:NamedIndividual, <https://w3id.org/dpv/owl#TechnicalMeasure> ;
  rdfs:subClassOf <https://w3id.org/dpv/owl#Encryption> ;
  dc:contributor _:genid9, _:genid10, _:genid1, _:genid11 ;
  dc:created "2019-04-05"^^xsd:date ;
  ns1:term_status "accepted"@en ;
  skos:definition "Encryption of data when being stored (persistent encryption)"@en ;
  skos:prefLabel "Encryption at Rest"@en ;
  owl:sameAs <https://w3id.org/dpv#EncryptionAtRest>, <https://w3id.org/dpv/dpv-owl#EncryptionAtRest> .

<https://w3id.org/dpv/owl#RightFulfilmentNotice>
  a owl:Class, owl:NamedIndividual, <https://w3id.org/dpv/owl#OrganisationalMeasure> ;
  rdfs:subClassOf <https://w3id.org/dpv/owl#RightExerciseNotice> ;
  dc:contributor _:genid5, _:genid1 ;
  dc:created "2022-11-02"^^xsd:date ;
  ns1:term_status "accepted"@en ;
  skos:definition "Notice provided regarding fulfilment of a right"@en ;
  skos:prefLabel "Right Fulfilment Notice"@en ;
  skos:scopeNote "This notice is associated with situations where information is provided with the intention of progressing the fulfilment of a right. For example, a notice asking for more information regarding the scope of the right, or providing information on where to access the data provided under a right."@en ;
  owl:sameAs <https://w3id.org/dpv#RightFulfilmentNotice>, <https://w3id.org/dpv/dpv-owl#RightFulfilmentNotice> .

<https://w3id.org/dpv/owl#EnterIntoContract>
  a owl:Class, owl:NamedIndividual, <https://w3id.org/dpv/owl#LegalBasis> ;
  rdfs:subClassOf <https://w3id.org/dpv/owl#Contract> ;
  dc:contributor _:genid4, _:genid1, _:genid6 ;
  dc:created "2021-04-07"^^xsd:date ;
  ns1:term_status "accepted"@en ;
  skos:definition "Processing necessary to enter into contract"@en ;
  skos:prefLabel "Enter Into Contract"@en ;
  owl:sameAs <https://w3id.org/dpv#EnterIntoContract>, <https://w3id.org/dpv/dpv-owl#EnterIntoContract> .

<https://w3id.org/dpv/owl#OptingOutFromProcess>
  a owl:Class, owl:NamedIndividual, <https://w3id.org/dpv/owl#EntityPermissiveInvolvement> ;
  rdfs:subClassOf <https://w3id.org/dpv/owl#EntityPermissiveInvolvement> ;
  dc:contributor _:genid1, _:genid25, _:genid19 ;
  dc:created "2024-05-11"^^xsd:date ;
  ns1:term_status "accepted"@en ;
  skos:definition "Involvement where entity can opt-out from specified context"@en ;
  skos:prefLabel "Opting out of Process"@en ;
  owl:sameAs <https://w3id.org/dpv#OptingOutFromProcess>, <https://w3id.org/dpv/dpv-owl#OptingOutFromProcess> .

<https://w3id.org/dpv/owl#Service>
  a owl:Class ;
  rdfs:subClassOf <https://w3id.org/dpv/owl#Process> ;
  dc:contributor _:genid1 ;
  dc:created "2024-05-09"^^xsd:date ;
  ns3:example <https://w3id.org/dpv/examples/owl#E0031>, <https://w3id.org/dpv/examples/owl#E0041> ;
  ns1:term_status "accepted"@en ;
  skos:definition "A service is a process where one entity provides some benefit or assistance to another entity"@en ;
  skos:prefLabel "Service"@en ;
  skos:scopeNote "Service Provider and Service Consumer reflect the roles associated with a service. 'Service' as a process is a distinct concept from the use of 'service' as a provision method in Tech extension"@en ;
  owl:sameAs <https://w3id.org/dpv#Service>, <https://w3id.org/dpv/dpv-owl#Service> .

odrl:status
  a owl:AnnotationProperty, owl:NamedIndividual, skos:Concept ;
  rdfs:domain odrl:Constraint ;
  rdfs:isDefinedBy odrl: ;
  rdfs:label "Status"@en ;
  skos:definition "the value generated from the leftOperand action or a value related to the leftOperand set as the reference for the comparison."@en .

<https://w3id.org/dpv/owl#CorrectingProcessInput>
  a owl:Class, owl:NamedIndividual, <https://w3id.org/dpv/owl#EntityPermissiveInvolvement> ;
  rdfs:subClassOf <https://w3id.org/dpv/owl#EntityPermissiveInvolvement> ;
  dc:contributor _:genid1, _:genid25, _:genid19 ;
  dc:created "2024-05-11"^^xsd:date ;
  ns1:term_status "accepted"@en ;
  skos:definition "Involvement where entity can correct input of specified context"@en ;
  skos:prefLabel "Correcting Process Input"@en ;
  owl:sameAs <https://w3id.org/dpv#CorrectingProcessInput>, <https://w3id.org/dpv/dpv-owl#CorrectingProcessInput> .

<https://w3id.org/dpv/owl#StorageRestoration>
  a owl:Class ;
  rdfs:subClassOf <https://w3id.org/dpv/owl#StorageCondition> ;
  dc:contributor _:genid9, _:genid10, _:genid1, _:genid11 ;
  dc:created "2019-04-05"^^xsd:date ;
  ns3:example <https://w3id.org/dpv/examples/owl#E0048> ;
  ns1:term_status "accepted"@en ;
  skos:definition "Regularity and temporal span of data restoration/backup mechanisms that guarantee that data is preserved"@en ;
  skos:prefLabel "Storage Restoration"@en ;
  owl:sameAs <https://w3id.org/dpv#StorageRestoration>, <https://w3id.org/dpv/dpv-owl#StorageRestoration> .

<https://w3id.org/dpv/owl#UsageControl>
  a owl:Class, owl:NamedIndividual, <https://w3id.org/dpv/owl#TechnicalMeasure> ;
  rdfs:subClassOf <https://w3id.org/dpv/owl#AccessControlMethod> ;
  dc:contributor _:genid1 ;
  dc:created "2022-08-17"^^xsd:date ;
  dc:source [
    a ns0:WebPage ;
    ns0:name "ENISA Reference Incident Classification Taxonomy 2018" ;
    ns0:url "https://www.enisa.europa.eu/publications/reference-incident-classification-taxonomy/"
  ] ;
  ns1:term_status "accepted"@en ;
  skos:definition "Management of usage, which is intended to be broader than access control and may cover trust, digital rights, or other relevant controls"@en ;
  skos:prefLabel "Usage Control"@en ;
  owl:sameAs <https://w3id.org/dpv#UsageControl>, <https://w3id.org/dpv/dpv-owl#UsageControl> .

<https://w3id.org/dpv/owl#PersonnelOnboarding>
  a owl:Class, owl:NamedIndividual, <https://w3id.org/dpv/owl#Purpose> ;
  rdfs:subClassOf <https://w3id.org/dpv/owl#PersonnelHiring> ;
  dc:created "2024-12-01"^^xsd:date ;
  ns1:term_status "accepted"@en ;
  skos:definition "Purposes associated with onboarding and integration of personnel within an organisation"@en ;
  skos:prefLabel "Personnel Onboarding"@en ;
  owl:sameAs <https://w3id.org/dpv#PersonnelOnboarding>, <https://w3id.org/dpv/dpv-owl#PersonnelOnboarding> .

<https://w3id.org/dpv/owl#InformedConsent>
  a owl:Class, owl:NamedIndividual, <https://w3id.org/dpv/owl#LegalBasis> ;
  rdfs:subClassOf <https://w3id.org/dpv/owl#Consent> ;
  dc:contributor _:genid4, _:genid1, _:genid17, _:genid6 ;
  dc:created "2022-06-21"^^xsd:date ;
  ns1:term_status "accepted"@en ;
  skos:definition "Consent that is informed i.e. with the requirement to provide sufficient information to make a consenting decision"@en ;
  skos:prefLabel "Informed Consent"@en ;
  skos:scopeNote "The specifics for what information should be provided or made available will depend on the context, use-case, or relevant legal requirements"@en ;
  owl:sameAs <https://w3id.org/dpv#InformedConsent>, <https://w3id.org/dpv/dpv-owl#InformedConsent> .

<https://w3id.org/dpv/owl#MonotonicCounterPseudonymisation>
  a owl:Class, owl:NamedIndividual, <https://w3id.org/dpv/owl#TechnicalMeasure> ;
  rdfs:subClassOf <https://w3id.org/dpv/owl#Pseudonymisation> ;
  dc:contributor _:genid1 ;
  dc:created "2022-08-17"^^xsd:date ;
  dc:modified "2022-10-13"^^xsd:date ;
  dc:source [
    a ns0:WebPage ;
    ns0:name "ENISA Data Pseudonymisation: Advanced Techniques and Use Cases" ;
    ns0:url "https://www.enisa.europa.eu/publications/data-pseudonymisation-advanced-techniques-and-use-cases"
  ] ;
  ns1:term_status "accepted"@en ;
  skos:definition "A simple pseudonymisation method where identifiers are substituted by a number chosen by a monotonic counter"@en ;
  skos:prefLabel "Monotonic Counter Pseudonymisation"@en ;
  owl:sameAs <https://w3id.org/dpv#MonotonicCounterPseudonymisation>, <https://w3id.org/dpv/dpv-owl#MonotonicCounterPseudonymisation> .

<https://w3id.org/dpv/owl#OrganisationalMeasure>
  a owl:Class ;
  rdfs:subClassOf <https://w3id.org/dpv/owl#TechnicalOrganisationalMeasure> ;
  dc:contributor _:genid9, _:genid10, _:genid1, _:genid11 ;
  dc:created "2019-04-05"^^xsd:date ;
  dc:modified "2023-12-10"^^xsd:date ;
  ns3:example <https://w3id.org/dpv/examples/owl#E0021> ;
  ns1:term_status "accepted"@en ;
  skos:definition "Organisational measures used to safeguard and ensure good practices in connection with data and technologies"@en ;
  skos:prefLabel "Organisational Measure"@en ;
  owl:sameAs <https://w3id.org/dpv#OrganisationalMeasure>, <https://w3id.org/dpv/dpv-owl#OrganisationalMeasure> .

<https://w3id.org/dpv/owl#ProcessingCondition>
  a owl:Class ;
  rdfs:subClassOf <https://w3id.org/dpv/owl#ProcessingContext> ;
  dc:created "2023-12-10"^^xsd:date ;
  ns3:example <https://w3id.org/dpv/examples/owl#E0047> ;
  ns1:term_status "accepted"@en ;
  skos:definition "Conditions required or followed regarding processing of data or use of technologies"@en ;
  skos:prefLabel "Processing Condition"@en ;
  owl:sameAs <https://w3id.org/dpv#ProcessingCondition>, <https://w3id.org/dpv/dpv-owl#ProcessingCondition> .

<https://w3id.org/dpv/owl#AccessControlMethod>
  a owl:Class, owl:NamedIndividual, <https://w3id.org/dpv/owl#TechnicalMeasure> ;
  rdfs:subClassOf <https://w3id.org/dpv/owl#TechnicalMeasure> ;
  dc:contributor _:genid9, _:genid10, _:genid1, _:genid11 ;
  dc:created "2019-04-05"^^xsd:date ;
  ns3:example <https://w3id.org/dpv/examples/owl#E0020> ;
  ns1:term_status "accepted"@en ;
  skos:definition "Methods which restrict access to a place or resource"@en ;
  skos:prefLabel "Access Control Method"@en ;
  owl:sameAs <https://w3id.org/dpv#AccessControlMethod>, <https://w3id.org/dpv/dpv-owl#AccessControlMethod> .

<https://w3id.org/dpv/owl#ComplianceAssessment>
  a owl:Class, owl:NamedIndividual, <https://w3id.org/dpv/owl#OrganisationalMeasure> ;
  rdfs:subClassOf <https://w3id.org/dpv/owl#Assessment> ;
  dc:contributor _:genid4, _:genid1 ;
  dc:created "2024-04-14"^^xsd:date ;
  ns1:term_status "accepted"@en ;
  skos:definition "Assessment regarding compliance (e.g. internal policy, regulations)"@en ;
  skos:prefLabel "Compliance Assessment"@en ;
  owl:sameAs <https://w3id.org/dpv#ComplianceAssessment>, <https://w3id.org/dpv/dpv-owl#ComplianceAssessment> .

<https://w3id.org/dpv/owl#ContractFulfiled>
  a owl:Class, owl:NamedIndividual, <https://w3id.org/dpv/owl#ContractFulfilmentStatus> ;
  rdfs:subClassOf <https://w3id.org/dpv/owl#ContractFulfilmentStatus> ;
  dc:contributor _:genid4, _:genid1, _:genid17 ;
  dc:created "2025-01-09"^^xsd:date ;
  ns1:term_status "accepted"@en ;
  skos:definition "Status representing contract where all its terms have been fulfiled in a manner that does not constitute a violation or breach of the contract"@en ;
  skos:prefLabel "Contract Fulfiled"@en ;
  owl:sameAs <https://w3id.org/dpv#ContractFulfiled>, <https://w3id.org/dpv/dpv-owl#ContractFulfiled> .

<https://w3id.org/dpv/owl#WebBrowserSecurity>
  a owl:Class, owl:NamedIndividual, <https://w3id.org/dpv/owl#TechnicalMeasure> ;
  rdfs:subClassOf <https://w3id.org/dpv/owl#SecurityMethod> ;
  dc:contributor _:genid1 ;
  dc:created "2022-08-17"^^xsd:date ;
  dc:source [
    a ns0:WebPage ;
    ns0:name "ENISA Reference Incident Classification Taxonomy 2018" ;
    ns0:url "https://www.enisa.europa.eu/publications/reference-incident-classification-taxonomy/"
  ] ;
  ns1:term_status "accepted"@en ;
  skos:definition "Security implemented at or over web browsers"@en ;
  skos:prefLabel "WebBrowser Security"@en ;
  owl:sameAs <https://w3id.org/dpv#WebBrowserSecurity>, <https://w3id.org/dpv/dpv-owl#WebBrowserSecurity> .

<https://w3id.org/dpv/owl#ThirdPartyDataSource>
  a owl:Class, owl:NamedIndividual, <https://w3id.org/dpv/owl#DataSource> ;
  rdfs:subClassOf <https://w3id.org/dpv/owl#DataSource> ;
  dc:created "2023-10-12"^^xsd:date ;
  ns1:term_status "accepted"@en ;
  skos:definition "Data Sourced from a Third Party, e.g. when data is collected from an entity that is neither the Controller nor the Data Subject"@en ;
  skos:prefLabel "Third Party as Data Source"@en ;
  owl:sameAs <https://w3id.org/dpv#ThirdPartyDataSource>, <https://w3id.org/dpv/dpv-owl#ThirdPartyDataSource> .

<https://w3id.org/dpv/owl#WebSecurityProtocols>
  a owl:Class, owl:NamedIndividual, <https://w3id.org/dpv/owl#TechnicalMeasure> ;
  rdfs:subClassOf <https://w3id.org/dpv/owl#SecurityMethod> ;
  dc:contributor _:genid1 ;
  dc:created "2022-08-17"^^xsd:date ;
  dc:source [
    a ns0:WebPage ;
    ns0:name "ENISA Reference Incident Classification Taxonomy 2018" ;
    ns0:url "https://www.enisa.europa.eu/publications/reference-incident-classification-taxonomy/"
  ] ;
  ns1:term_status "accepted"@en ;
  skos:definition "Security implemented at or over web-based protocols"@en ;
  skos:prefLabel "Web Security Protocols"@en ;
  owl:sameAs <https://w3id.org/dpv#WebSecurityProtocols>, <https://w3id.org/dpv/dpv-owl#WebSecurityProtocols> .

<https://w3id.org/dpv/owl#Client>
  a owl:Class, owl:NamedIndividual, <https://w3id.org/dpv/owl#HumanSubject> ;
  rdfs:subClassOf <https://w3id.org/dpv/owl#Customer> ;
  dc:contributor _:genid4, _:genid5, _:genid1, _:genid17, _:genid6 ;
  dc:created "2022-04-06"^^xsd:date ;
  dc:modified "2024-12-17"^^xsd:date ;
  ns1:term_status "modified"@en ;
  skos:definition "Humans that are clients or recipients of services"@en ;
  skos:prefLabel "Client"@en ;
  owl:sameAs <https://w3id.org/dpv#Client>, <https://w3id.org/dpv/dpv-owl#Client> .

<https://w3id.org/dpv/owl#OptingInToProcess>
  a owl:Class, owl:NamedIndividual, <https://w3id.org/dpv/owl#EntityPermissiveInvolvement> ;
  rdfs:subClassOf <https://w3id.org/dpv/owl#EntityPermissiveInvolvement> ;
  dc:contributor _:genid1, _:genid25, _:genid19 ;
  dc:created "2024-05-11"^^xsd:date ;
  ns1:term_status "accepted"@en ;
  skos:definition "Involvement where entity can opt-in to specified context"@en ;
  skos:prefLabel "Opting in to Process"@en ;
  owl:sameAs <https://w3id.org/dpv#OptingInToProcess>, <https://w3id.org/dpv/dpv-owl#OptingInToProcess> .

dcat:Resource
  a owl:Class ;
  dc:created "2022-11-02"^^xsd:date ;
  skos:prefLabel "dcat:Resource"@en ;
  skos:scopeNote "A dataset, data service, or any other resource associated with Right Exercise - such as for providing a copy of data"@en .

odrl:move
  a owl:NamedIndividual, skos:Concept, odrl:Action ;
  odrl:includedIn odrl:use ;
  rdfs:isDefinedBy odrl: ;
  rdfs:label "Move"@en ;
  skos:definition "To move the Asset from one digital location to another including deleting the original copy."@en ;
  skos:note "After the Asset has been moved, the original copy must be deleted."@en ;
  skos:scopeNote "Non-Normative"@en .

<https://w3id.org/dpv/owl#PersonnelWorkloadManagement>
  a owl:Class, owl:NamedIndividual, <https://w3id.org/dpv/owl#Purpose> ;
  rdfs:subClassOf <https://w3id.org/dpv/owl#PersonnelManagement> ;
  dc:created "2024-12-01"^^xsd:date ;
  ns1:term_status "accepted"@en ;
  skos:definition "Purposes assocaited with determination, scheduling, planning, and carrying out workload management of personnel"@en ;
  skos:prefLabel "Personnel Workload Management"@en ;
  owl:sameAs <https://w3id.org/dpv#PersonnelWorkloadManagement>, <https://w3id.org/dpv/dpv-owl#PersonnelWorkloadManagement> .

<https://w3id.org/dpv/owl#ActivityNotCompleted>
  a owl:Class, owl:NamedIndividual, <https://w3id.org/dpv/owl#ActivityStatus> ;
  rdfs:subClassOf <https://w3id.org/dpv/owl#ActivityStatus> ;
  dc:contributor _:genid1 ;
  dc:created "2022-11-30"^^xsd:date ;
  ns1:term_status "accepted"@en ;
  skos:definition "State of an activity that could not be completed, but has reached some end state"@en ;
  skos:prefLabel "Activity Not Completed"@en ;
  skos:scopeNote "This relates to a 'Stop' state as distinct from a 'Halt' state. It makes no comments on whether the Activity can be resumed or continued towards completion."@en ;
  owl:sameAs <https://w3id.org/dpv#ActivityNotCompleted>, <https://w3id.org/dpv/dpv-owl#ActivityNotCompleted> .

odrl:#partyRoles
  a owl:NamedIndividual, skos:Collection ;
  skos:member odrl:assignee, odrl:assigneeOf, odrl:assigner, odrl:assignerOf ;
  skos:prefLabel "Party Functions"@en ;
  skos:scopeNote "ODRL Core Vocabulary Terms"@en .

<https://w3id.org/dpv/owl#ConsentControl>
  a owl:Class ;
  rdfs:subClassOf <https://w3id.org/dpv/owl#EntityInvolvement> ;
  dc:created "2024-05-11"^^xsd:date ;
  ns1:term_status "accepted"@en ;
  skos:definition "The control or activity associated with obtaining, providing, withdrawing, or reaffirming consent"@en ;
  skos:prefLabel "Consent Control"@en ;
  owl:sameAs <https://w3id.org/dpv#ConsentControl>, <https://w3id.org/dpv/dpv-owl#ConsentControl> .

<https://w3id.org/dpv/owl#PermissionNotUtilised>
  a owl:Class, owl:NamedIndividual, <https://w3id.org/dpv/owl#RuleFulfilmentStatus> ;
  rdfs:subClassOf <https://w3id.org/dpv/owl#RuleFulfilled> ;
  dc:contributor _:genid1 ;
  dc:created "2024-09-10"^^xsd:date ;
  ns1:term_status "accepted"@en ;
  skos:definition "Status indicating a permission has not been utilised i.e. the activity stated as being permitted has not been carried out"@en ;
  skos:prefLabel "Permission Not Utilised"@en ;
  owl:sameAs <https://w3id.org/dpv#PermissionNotUtilised>, <https://w3id.org/dpv/dpv-owl#PermissionNotUtilised> .

odrl:distribute
  a owl:NamedIndividual, skos:Concept, odrl:Action ;
  odrl:includedIn odrl:use ;
  rdfs:isDefinedBy odrl: ;
  rdfs:label "Distribute"@en ;
  skos:definition "To supply the Asset to third-parties."@en ;
  skos:note "It is recommended to use nextPolicy to express the allowable usages by third-parties."@en ;
  skos:scopeNote "Non-Normative"@en .

<https://w3id.org/dpv/owl#Collect>
  a owl:Class, owl:NamedIndividual, <https://w3id.org/dpv/owl#Processing> ;
  rdfs:subClassOf <https://w3id.org/dpv/owl#Obtain> ;
  dc:created "2019-05-07"^^xsd:date ;
  dc:source [
    a ns0:WebPage ;
    ns0:name "GDPR Art.4-2" ;
    ns0:url "https://eur-lex.europa.eu/eli/reg/2016/679/art_4/par_2/oj"
  ] ;
  ns1:term_status "accepted"@en ;
  skos:definition "to gather data from someone"@en ;
  skos:prefLabel "Collect Data"@en ;
  skos:related <https://specialprivacy.ercim.eu/vocabs/processing#Collect> ;
  owl:sameAs <https://w3id.org/dpv#Collect>, <https://w3id.org/dpv/dpv-owl#Collect> .

<https://w3id.org/dpv/owl#SingleSignOn>
  a owl:Class, owl:NamedIndividual, <https://w3id.org/dpv/owl#TechnicalMeasure> ;
  rdfs:subClassOf <https://w3id.org/dpv/owl#AuthenticationProtocols> ;
  dc:contributor _:genid4, _:genid1, _:genid6 ;
  dc:created "2020-11-04"^^xsd:date ;
  ns1:term_status "accepted"@en ;
  skos:definition "Use of credentials or processes that enable using one set of credentials to authenticate multiple contexts."@en ;
  skos:prefLabel "Single Sign On"@en ;
  owl:sameAs <https://w3id.org/dpv#SingleSignOn>, <https://w3id.org/dpv/dpv-owl#SingleSignOn> .

<https://w3id.org/dpv/owl#Representative>
  a owl:Class ;
  rdfs:subClassOf <https://w3id.org/dpv/owl#LegalEntity> ;
  dc:contributor _:genid4, _:genid5, _:genid1, _:genid6 ;
  dc:created "2020-11-04"^^xsd:date ;
  dc:source [
    a ns0:WebPage ;
    ns0:name "GDPR Art.27" ;
    ns0:url "https://eur-lex.europa.eu/eli/reg/2016/679/art_27/oj"
  ] ;
  ns3:example <https://w3id.org/dpv/examples/owl#E0019>, <https://w3id.org/dpv/examples/owl#E0032> ;
  ns1:term_status "accepted"@en ;
  skos:definition "A representative of a legal entity"@en ;
  skos:prefLabel "Representative"@en ;
  owl:sameAs <https://w3id.org/dpv#Representative>, <https://w3id.org/dpv/dpv-owl#Representative> .

odrl:Duty
  a owl:Class, owl:NamedIndividual, skos:Concept ;
  rdfs:subClassOf odrl:Rule ;
  owl:disjointWith odrl:Permission, odrl:Prohibition ;
  rdfs:isDefinedBy odrl: ;
  rdfs:label "Duty"@en ;
  skos:definition "The obligation to perform an Action"@en .

<https://w3id.org/dpv/owl#ProfessionalTraining>
  a owl:Class, owl:NamedIndividual, <https://w3id.org/dpv/owl#OrganisationalMeasure> ;
  rdfs:subClassOf <https://w3id.org/dpv/owl#StaffTraining> ;
  dc:contributor _:genid1 ;
  dc:created "2022-08-17"^^xsd:date ;
  dc:source [
    a ns0:WebPage ;
    ns0:name "ENISA Reference Incident Classification Taxonomy 2018" ;
    ns0:url "https://www.enisa.europa.eu/publications/reference-incident-classification-taxonomy/"
  ] ;
  ns1:term_status "accepted"@en ;
  skos:definition "Training methods that are intended to provide professional knowledge and expertise"@en ;
  skos:prefLabel "Professional Training"@en ;
  owl:sameAs <https://w3id.org/dpv#ProfessionalTraining>, <https://w3id.org/dpv/dpv-owl#ProfessionalTraining> .

<https://w3id.org/dpv/owl#AuthenticationProtocols>
  a owl:Class, owl:NamedIndividual, <https://w3id.org/dpv/owl#TechnicalMeasure> ;
  rdfs:subClassOf <https://w3id.org/dpv/owl#TechnicalMeasure> ;
  dc:contributor _:genid9, _:genid10, _:genid1, _:genid11 ;
  dc:created "2019-04-05"^^xsd:date ;
  ns1:term_status "accepted"@en ;
  skos:definition "Protocols involving validation of identity i.e. authentication of a person or information"@en ;
  skos:prefLabel "Authentication Protocols"@en ;
  owl:sameAs <https://w3id.org/dpv#AuthenticationProtocols>, <https://w3id.org/dpv/dpv-owl#AuthenticationProtocols> .

odrl:isA
  a owl:NamedIndividual, skos:Concept, odrl:Operator ;
  rdfs:isDefinedBy odrl: ;
  rdfs:label "Is a"@en ;
  skos:definition "A set-based operator indicating that a given value is an instance of the right operand of the Constraint."@en .

<https://w3id.org/dpv/owl#ContractByEntityType>
  a owl:Class, owl:NamedIndividual, <https://w3id.org/dpv/owl#LegalBasis> ;
  rdfs:subClassOf <https://w3id.org/dpv/owl#Contract> ;
  dc:created "2024-12-17"^^xsd:date ;
  ns1:term_status "accepted"@en ;
  skos:definition "A generic concept representing contracts categorised by the type of entities involved - such as Businesses (B), Consumers (C), and Governments (G)"@en ;
  skos:prefLabel "Contract by Entity Type"@en ;
  owl:sameAs <https://w3id.org/dpv#ContractByEntityType>, <https://w3id.org/dpv/dpv-owl#ContractByEntityType> .

<https://w3id.org/dpv/owl#serialisation-ttl>
  a owl:NamedIndividual, ns4:ResourceDescriptor ;
  dc:format <https://www.iana.org/assignments/media-types/text/turtle> ;
  dc:conformsTo <https://www.w3.org/TR/turtle/> ;
  dc:title "Data Privacy Vocabulary (DPV) - Turtle serialiation" ;
  ns4:hasArtifact <https://w3id.org/dpv/dpv/dpv-owl.ttl> ;
  ns4:hasRole <http://www.w3.org/ns/dx/prof/role/vocabulary> ;
  owl:sameAs <https://w3id.org/dpv#serialisation-ttl>, <https://w3id.org/dpv/dpv-owl#serialisation-ttl> .

<https://w3id.org/dpv/owl#EntityPermissiveInvolvement>
  a owl:Class ;
  rdfs:subClassOf <https://w3id.org/dpv/owl#EntityInvolvement> ;
  dc:contributor _:genid1, _:genid25 ;
  dc:created "2024-05-11"^^xsd:date ;
  ns1:term_status "accepted"@en ;
  skos:definition "Involvement of an entity in specific context where it is permitted or able to do something"@en ;
  skos:prefLabel "Entity Permissive Involvement"@en ;
  owl:sameAs <https://w3id.org/dpv#EntityPermissiveInvolvement>, <https://w3id.org/dpv/dpv-owl#EntityPermissiveInvolvement> .

<https://w3id.org/dpv/owl#Authority>
  a owl:Class ;
  rdfs:subClassOf <https://w3id.org/dpv/owl#GovernmentalOrganisation> ;
  dc:contributor _:genid4, _:genid1, _:genid6 ;
  dc:created "2020-11-04"^^xsd:date ;
  ns1:term_status "accepted"@en ;
  skos:definition "An authority with the power to create or enforce laws, or determine their compliance."@en ;
  skos:prefLabel "Authority"@en ;
  owl:sameAs <https://w3id.org/dpv#Authority>, <https://w3id.org/dpv/dpv-owl#Authority> .

<https://w3id.org/dpv/owl#hasParty>
  a owl:ObjectProperty ;
  ns2:domainIncludes <https://w3id.org/dpv/owl#Contract> ;
  ns2:rangeIncludes <https://w3id.org/dpv/owl#LegalEntity> ;
  dc:contributor _:genid4, _:genid1, _:genid17 ;
  dc:created "2025-01-14"^^xsd:date ;
  ns1:term_status "accepted"@en ;
  skos:definition "Indicates a legal entity involved as a party in a contract"@en ;
  skos:prefLabel "has party"@en ;
  ns0:domainIncludes <https://w3id.org/dpv/owl#Contract> ;
  ns0:rangeIncludes <https://w3id.org/dpv/owl#LegalEntity> ;
  owl:sameAs <https://w3id.org/dpv#hasParty>, <https://w3id.org/dpv/dpv-owl#hasParty> .

<https://w3id.org/dpv/owl#Filter>
  a owl:Class, owl:NamedIndividual, <https://w3id.org/dpv/owl#Processing> ;
  rdfs:subClassOf <https://w3id.org/dpv/owl#Transform> ;
  dc:contributor _:genid4, _:genid1 ;
  dc:created "2022-06-15"^^xsd:date ;
  ns1:term_status "accepted"@en ;
  skos:definition "to filter or keep data for some criteria"@en ;
  skos:prefLabel "Filter Data"@en ;
  owl:sameAs <https://w3id.org/dpv#Filter>, <https://w3id.org/dpv/dpv-owl#Filter> .

<https://w3id.org/dpv/owl#ROPA>
  a owl:Class, owl:NamedIndividual, <https://w3id.org/dpv/owl#OrganisationalMeasure> ;
  rdfs:subClassOf <https://w3id.org/dpv/owl#DataProcessingRecord> ;
  dc:contributor _:genid4, _:genid1, _:genid6 ;
  dc:created "2021-09-08"^^xsd:date ;
  dc:modified "2024-04-14"^^xsd:date ;
  ns1:term_status "accepted"@en ;
  skos:definition "A Record of Processing Activities (ROPA) is a document detailing processing activities"@en ;
  skos:prefLabel "Records of Processing Activities"@en ;
  skos:scopeNote "ROPA under GDPR Art.30 has specific requirements regarding the information to be maintained. Additionally, Data Protection Authorities also provide additional information guidelines for information to be maintained in a ROPA. For more information see https://w3id.org/dpcat"@en ;
  owl:sameAs <https://w3id.org/dpv#ROPA>, <https://w3id.org/dpv/dpv-owl#ROPA> .

<https://w3id.org/dpv/owl#ProvidePersonalisedRecommendations>
  a owl:Class, owl:NamedIndividual, <https://w3id.org/dpv/owl#Purpose> ;
  rdfs:subClassOf <https://w3id.org/dpv/owl#ServicePersonalisation> ;
  dc:contributor _:genid66, _:genid1 ;
  dc:created "2019-11-26"^^xsd:date ;
  dc:modified "2022-10-14"^^xsd:date ;
  dc:source [
    a ns0:WebPage ;
    ns0:name "SPECIAL Project" ;
    ns0:url "https://specialprivacy.ercim.eu/"
  ] ;
  ns1:term_status "accepted"@en ;
  skos:definition "Purposes associated with creating and providing personalised recommendations"@en ;
  skos:prefLabel "Provide Personalised Recommendations"@en ;
  owl:sameAs <https://w3id.org/dpv#ProvidePersonalisedRecommendations>, <https://w3id.org/dpv/dpv-owl#ProvidePersonalisedRecommendations> .

<https://w3id.org/dpv/owl#RecipientInformed>
  a owl:Class, owl:NamedIndividual, <https://w3id.org/dpv/owl#EntityInformedStatus> ;
  rdfs:subClassOf <https://w3id.org/dpv/owl#EntityInformed> ;
  dc:contributor _:genid4, _:genid1, _:genid25, _:genid6 ;
  dc:created "2024-05-10"^^xsd:date ;
  ns1:term_status "accepted"@en ;
  skos:definition "Status indicating Recipient has been informed about the specified context"@en ;
  skos:prefLabel "Recipient Informed"@en ;
  owl:sameAs <https://w3id.org/dpv#RecipientInformed>, <https://w3id.org/dpv/dpv-owl#RecipientInformed> .

<https://w3id.org/dpv/owl#hasComplianceStatus>
  a owl:ObjectProperty ;
  rdfs:subPropertyOf <https://w3id.org/dpv/owl#hasStatus> ;
  ns2:rangeIncludes <https://w3id.org/dpv/owl#ComplianceStatus> ;
  dc:contributor _:genid1 ;
  dc:created "2022-05-18"^^xsd:date ;
  ns3:example <https://w3id.org/dpv/examples/owl#E0055> ;
  ns1:term_status "accepted"@en ;
  skos:definition "Indicates the status of compliance of specified concept"@en ;
  skos:prefLabel "has compliance status"@en ;
  ns0:rangeIncludes <https://w3id.org/dpv/owl#ComplianceStatus> ;
  owl:sameAs <https://w3id.org/dpv#hasComplianceStatus>, <https://w3id.org/dpv/dpv-owl#hasComplianceStatus> .

odrl:compensate
  a owl:NamedIndividual, skos:Concept, odrl:Action ;
  odrl:includedIn odrl:use ;
  rdfs:isDefinedBy odrl: ;
  rdfs:label "Compensate"@en ;
  skos:definition "To compensate by transfer of some amount of value, if defined, for using or selling the Asset."@en ;
  skos:note "The compensation may use different types of things with a value: (i) the thing is expressed by the value (term) of the Constraint name; (b) the value is expressed by operator, rightOperand, dataType and unit. Typically the assignee will compensate the assigner, but other compensation party roles may be used."@en ;
  skos:scopeNote "Non-Normative"@en .

<https://w3id.org/dpv/owl#PhysicalDeviceSecurity>
  a owl:Class, owl:NamedIndividual, <https://w3id.org/dpv/owl#PhysicalMeasure> ;
  rdfs:subClassOf <https://w3id.org/dpv/owl#PhysicalMeasure> ;
  dc:contributor _:genid1 ;
  dc:created "2024-04-14"^^xsd:date ;
  dc:source "NIST SP 800-19"@en ;
  ns1:term_status "accepted"@en ;
  skos:definition "Physical protection for devices and equipment"@en ;
  skos:prefLabel "Physical Device Security"@en ;
  owl:sameAs <https://w3id.org/dpv#PhysicalDeviceSecurity>, <https://w3id.org/dpv/dpv-owl#PhysicalDeviceSecurity> .

<https://w3id.org/dpv/owl#PersonnelPerformanceMonitoring>
  a owl:Class, owl:NamedIndividual, <https://w3id.org/dpv/owl#Purpose> ;
  rdfs:subClassOf <https://w3id.org/dpv/owl#PersonnelMonitoring>, <https://w3id.org/dpv/owl#PersonnelPerformanceManagement> ;
  dc:created "2024-12-01"^^xsd:date ;
  ns1:term_status "accepted"@en ;
  skos:definition "Purposes associated with monitoring of performance of personnel"@en ;
  skos:prefLabel "Personnel Performance Monitoring"@en ;
  owl:sameAs <https://w3id.org/dpv#PersonnelPerformanceMonitoring>, <https://w3id.org/dpv/dpv-owl#PersonnelPerformanceMonitoring> .

<https://w3id.org/dpv/owl#ContractDefinitions>
  a owl:Class, owl:NamedIndividual, <https://w3id.org/dpv/owl#ContractualClause> ;
  rdfs:subClassOf <https://w3id.org/dpv/owl#ContractualClause> ;
  dc:created "2024-08-27"^^xsd:date ;
  ns1:term_status "accepted"@en ;
  skos:definition "A section specifying the meanings of key terms and phrases used throughout the contract"@en ;
  skos:prefLabel "Contract Definitions"@en ;
  owl:sameAs <https://w3id.org/dpv#ContractDefinitions>, <https://w3id.org/dpv/dpv-owl#ContractDefinitions> .

<https://w3id.org/dpv/owl#PostQuantumCryptography>
  a owl:Class, owl:NamedIndividual, <https://w3id.org/dpv/owl#TechnicalMeasure> ;
  rdfs:subClassOf <https://w3id.org/dpv/owl#CryptographicMethods> ;
  dc:contributor _:genid1 ;
  dc:created "2022-08-17"^^xsd:date ;
  dc:source [
    a ns0:WebPage ;
    ns0:name "ENISA Reference Incident Classification Taxonomy 2018" ;
    ns0:url "https://www.enisa.europa.eu/publications/reference-incident-classification-taxonomy/"
  ] ;
  ns1:term_status "accepted"@en ;
  skos:definition "Use of algorithms that are intended to be secure against cryptanalytic attack by a quantum computer"@en ;
  skos:prefLabel "Post-Quantum Cryptography"@en ;
  owl:sameAs <https://w3id.org/dpv#PostQuantumCryptography>, <https://w3id.org/dpv/dpv-owl#PostQuantumCryptography> .

<https://w3id.org/dpv/owl#MobilePlatformSecurity>
  a owl:Class, owl:NamedIndividual, <https://w3id.org/dpv/owl#TechnicalMeasure> ;
  rdfs:subClassOf <https://w3id.org/dpv/owl#SecurityMethod> ;
  dc:contributor _:genid1 ;
  dc:created "2022-08-17"^^xsd:date ;
  dc:source [
    a ns0:WebPage ;
    ns0:name "ENISA Reference Incident Classification Taxonomy 2018" ;
    ns0:url "https://www.enisa.europa.eu/publications/reference-incident-classification-taxonomy/"
  ] ;
  ns1:term_status "accepted"@en ;
  skos:definition "Security implemented over a mobile platform"@en ;
  skos:prefLabel "Mobile Platform Security"@en ;
  owl:sameAs <https://w3id.org/dpv#MobilePlatformSecurity>, <https://w3id.org/dpv/dpv-owl#MobilePlatformSecurity> .

<https://w3id.org/dpv/owl#Screen>
  a owl:Class, owl:NamedIndividual, <https://w3id.org/dpv/owl#Processing> ;
  rdfs:subClassOf <https://w3id.org/dpv/owl#Transform> ;
  dc:contributor _:genid4, _:genid1 ;
  dc:created "2022-06-15"^^xsd:date ;
  ns1:term_status "accepted"@en ;
  skos:definition "to remove data for some criteria"@en ;
  skos:prefLabel "Screen Data"@en ;
  owl:sameAs <https://w3id.org/dpv#Screen>, <https://w3id.org/dpv/dpv-owl#Screen> .

<https://w3id.org/dpv/owl#ContractFulfilmentStatus>
  a owl:Class ;
  rdfs:subClassOf <https://w3id.org/dpv/owl#ContractStatus> ;
  dc:contributor _:genid4, _:genid1, _:genid17 ;
  dc:created "2025-01-09"^^xsd:date ;
  ns3:example <https://w3id.org/dpv/examples/owl#E0077>, <https://w3id.org/dpv/examples/owl#E0078> ;
  ns1:term_status "accepted"@en ;
  skos:definition "Status associated with fulfilment of a contract"@en ;
  skos:prefLabel "Contract Fulfilment Status"@en ;
  owl:sameAs <https://w3id.org/dpv#ContractFulfilmentStatus>, <https://w3id.org/dpv/dpv-owl#ContractFulfilmentStatus> .

<https://w3id.org/dpv/owl#AsymmetricEncryption>
  a owl:Class, owl:NamedIndividual, <https://w3id.org/dpv/owl#TechnicalMeasure> ;
  rdfs:subClassOf <https://w3id.org/dpv/owl#Encryption> ;
  dc:contributor _:genid1 ;
  dc:created "2022-08-17"^^xsd:date ;
  dc:source [
    a ns0:WebPage ;
    ns0:name "ENISA Data Pseudonymisation: Advanced Techniques and Use Cases" ;
    ns0:url "https://www.enisa.europa.eu/publications/data-pseudonymisation-advanced-techniques-and-use-cases"
  ] ;
  ns1:term_status "accepted"@en ;
  skos:definition "Use of asymmetric cryptography to encrypt data"@en ;
  skos:prefLabel "Asymmetric Encryption"@en ;
  owl:sameAs <https://w3id.org/dpv#AsymmetricEncryption>, <https://w3id.org/dpv/dpv-owl#AsymmetricEncryption> .

odrl:aggregate
  a owl:NamedIndividual, skos:Concept, odrl:Action ;
  odrl:includedIn odrl:use ;
  rdfs:isDefinedBy odrl: ;
  rdfs:label "Aggregate"@en ;
  skos:definition "To use the Asset or parts of it as part of a composite collection."@en ;
  skos:scopeNote "Non-Normative"@en .

<https://w3id.org/dpv/owl#Entity>
  a owl:Class ;
  rdfs:subClassOf odrl:Party ;
  dc:contributor _:genid1 ;
  dc:created "2022-02-02"^^xsd:date ;
  ns1:term_status "accepted"@en ;
  skos:definition "A human or non-human 'thing' that constitutes as an entity"@en ;
  skos:prefLabel "Entity"@en ;
  owl:sameAs <https://w3id.org/dpv#Entity>, <https://w3id.org/dpv/dpv-owl#Entity> .

<https://w3id.org/dpv/owl#NonConformant>
  a owl:Class, owl:NamedIndividual, <https://w3id.org/dpv/owl#ConformanceStatus> ;
  rdfs:subClassOf <https://w3id.org/dpv/owl#ConformanceStatus> ;
  dc:contributor _:genid1 ;
  dc:created "2022-10-22"^^xsd:date ;
  ns1:term_status "accepted"@en ;
  skos:definition "State of being non-conformant"@en ;
  skos:prefLabel "NonConformant"@en ;
  owl:sameAs <https://w3id.org/dpv#NonConformant>, <https://w3id.org/dpv/dpv-owl#NonConformant> .

<https://w3id.org/dpv/owl#NonPersonalDataProcess>
  a owl:Class ;
  rdfs:subClassOf <https://w3id.org/dpv/owl#Process> ;
  dc:contributor _:genid1 ;
  dc:created "2024-05-09"^^xsd:date ;
  ns1:term_status "accepted"@en ;
  skos:definition "An action, activity, or method involving non-personal data, and asserting that no personal data is involved"@en ;
  skos:prefLabel "Non-Personal Data Process"@en ;
  skos:scopeNote "Use of personal data within NonPersonalDataProcess should be considered a violation of the explicit constraint that no personal data is involved."@en ;
  owl:sameAs <https://w3id.org/dpv#NonPersonalDataProcess>, <https://w3id.org/dpv/dpv-owl#NonPersonalDataProcess> .

odrl:anonymize
  a owl:NamedIndividual, skos:Concept, odrl:Action ;
  odrl:includedIn odrl:use ;
  rdfs:isDefinedBy odrl: ;
  rdfs:label "Anonymize"@en ;
  skos:definition "To anonymize all or parts of the Asset."@en ;
  skos:note "For example, to remove identifying particulars for statistical or for other comparable purposes, or to use the Asset without stating the author/source."@en ;
  skos:scopeNote "Non-Normative"@en .

odrl:acceptTracking
  a owl:NamedIndividual, skos:Concept, odrl:Action ;
  odrl:includedIn odrl:use ;
  rdfs:isDefinedBy odrl: ;
  rdfs:label "Accept Tracking"@en ;
  skos:definition "To accept that the use of the Asset may be tracked."@en ;
  skos:note "The collected information may be tracked by the Assigner, or may link to a Party with the role 'trackingParty' function."@en ;
  skos:scopeNote "Non-Normative"@en .

bibo:doi a owl:AnnotationProperty .
<https://w3id.org/dpv/owl#InternationalOrganisation>
  a owl:Class ;
  rdfs:subClassOf <https://w3id.org/dpv/owl#Organisation> ;
  dc:contributor _:genid4, _:genid17 ;
  dc:created "2022-03-23"^^xsd:date ;
  dc:modified "2020-10-05"^^xsd:date ;
  dc:source [
    a ns0:WebPage ;
    ns0:name "GDPR Art.4-26" ;
    ns0:url "https://eur-lex.europa.eu/eli/reg/2016/679/art_4/par_26/oj"
  ] ;
  ns1:term_status "accepted"@en ;
  skos:definition "An organisation and its subordinate bodies governed by public international law, or any other body which is set up by, or on the basis of, an agreement between two or more countries"@en ;
  skos:prefLabel "International Organisation"@en ;
  owl:sameAs <https://w3id.org/dpv#InternationalOrganisation>, <https://w3id.org/dpv/dpv-owl#InternationalOrganisation> .

<https://w3id.org/dpv/owl#hasDataProcessor>
  a owl:ObjectProperty ;
  rdfs:subPropertyOf <https://w3id.org/dpv/owl#hasRecipient> ;
  ns2:rangeIncludes <https://w3id.org/dpv/owl#DataProcessor> ;
  dc:contributor _:genid4, _:genid1, _:genid6 ;
  dc:created "2022-02-09"^^xsd:date ;
  ns1:term_status "accepted"@en ;
  skos:definition "Indiciates inclusion or applicability of a Data Processor"@en ;
  skos:prefLabel "has data processor"@en ;
  ns0:rangeIncludes <https://w3id.org/dpv/owl#DataProcessor> ;
  owl:sameAs <https://w3id.org/dpv#hasDataProcessor>, <https://w3id.org/dpv/dpv-owl#hasDataProcessor> .

<https://w3id.org/dpv/owl#ProvideEventRecommendations>
  a owl:Class, owl:NamedIndividual, <https://w3id.org/dpv/owl#Purpose> ;
  rdfs:subClassOf <https://w3id.org/dpv/owl#ProvidePersonalisedRecommendations> ;
  dc:contributor _:genid66, _:genid1 ;
  dc:created "2019-11-26"^^xsd:date ;
  dc:modified "2022-10-14"^^xsd:date ;
  dc:source [
    a ns0:WebPage ;
    ns0:name "SPECIAL Project" ;
    ns0:url "https://specialprivacy.ercim.eu/"
  ] ;
  ns1:term_status "accepted"@en ;
  skos:definition "Purposes associated with creating and providing personalised recommendations for events"@en ;
  skos:prefLabel "Provide Event Recommendations"@en ;
  owl:sameAs <https://w3id.org/dpv#ProvideEventRecommendations>, <https://w3id.org/dpv/dpv-owl#ProvideEventRecommendations> .

<https://w3id.org/dpv/owl#CorrectingProcess>
  a owl:Class, owl:NamedIndividual, <https://w3id.org/dpv/owl#EntityPermissiveInvolvement> ;
  rdfs:subClassOf <https://w3id.org/dpv/owl#EntityPermissiveInvolvement> ;
  dc:contributor _:genid1, _:genid25, _:genid19 ;
  dc:created "2024-05-11"^^xsd:date ;
  ns1:term_status "accepted"@en ;
  skos:definition "Involvement where entity can correct the process of specified context"@en ;
  skos:prefLabel "Correcting Process"@en ;
  skos:scopeNote "Correction of process refers to the ability to change how the process takes place"@en ;
  owl:sameAs <https://w3id.org/dpv#CorrectingProcess>, <https://w3id.org/dpv/dpv-owl#CorrectingProcess> .

<https://w3id.org/dpv/owl#OfferContract>
  a owl:Class ;
  rdfs:subClassOf <https://w3id.org/dpv/owl#ContractControl> ;
  dc:created "2024-08-27"^^xsd:date ;
  ns1:term_status "accepted"@en ;
  skos:definition "Control for offering a contract"@en ;
  skos:prefLabel "Offer Contract"@en ;
  owl:sameAs <https://w3id.org/dpv#OfferContract>, <https://w3id.org/dpv/dpv-owl#OfferContract> .

<https://w3id.org/dpv/owl#IndustryConsortium>
  a owl:Class ;
  rdfs:subClassOf <https://w3id.org/dpv/owl#Organisation> ;
  dc:contributor _:genid1 ;
  dc:created "2022-02-02"^^xsd:date ;
  dc:modified "2020-10-05"^^xsd:date ;
  dc:source [
    a ns0:WebPage ;
    ns0:name "ADMS controlled vocabulary" ;
    ns0:url "http://purl.org/adms"
  ] ;
  ns1:term_status "accepted"@en ;
  skos:definition "A consortium established and comprising on industry organisations"@en ;
  skos:prefLabel "Industry Consortium"@en ;
  owl:sameAs <https://w3id.org/dpv#IndustryConsortium>, <https://w3id.org/dpv/dpv-owl#IndustryConsortium> .

<https://w3id.org/dpv/owl#RuleFulfilmentStatus>
  a owl:Class ;
  rdfs:subClassOf <https://w3id.org/dpv/owl#Status> ;
  dc:contributor _:genid1 ;
  dc:created "2024-09-10"^^xsd:date ;
  ns3:example <https://w3id.org/dpv/examples/owl#E0084> ;
  ns1:term_status "accepted"@en ;
  skos:definition "Status associated with a rule for indicating whether it is applicable, or has been utilised, and whether the requirements of the rule have been fulfilled or violated"@en ;
  skos:prefLabel "Rule Fulfilment Status"@en ;
  owl:sameAs <https://w3id.org/dpv#RuleFulfilmentStatus>, <https://w3id.org/dpv/dpv-owl#RuleFulfilmentStatus> .

odrl:textToSpeech
  a owl:NamedIndividual, skos:Concept, odrl:Action ;
  odrl:includedIn odrl:use ;
  rdfs:isDefinedBy odrl: ;
  rdfs:label "Text-to-speech"@en ;
  skos:definition "To have a text Asset read out loud."@en ;
  skos:note "If the action is to be performed to a wider audience than just the Assignees, then the recipient constraint is recommended to be used." ;
  skos:scopeNote "Non-Normative"@en .

odrl:elapsedTime
  a owl:NamedIndividual, skos:Concept, odrl:LeftOperand ;
  rdfs:isDefinedBy odrl: ;
  rdfs:label "Elapsed Time"@en ;
  skos:definition "A continuous elapsed time period which may be used for exercising of the action of the Rule. Right operand value MUST be an xsd:duration as defined by [[xmlschema11-2]]."@en ;
  skos:note "Only the eq, lt, lteq operators SHOULD be used. See also Metered Time. <br />Example: <code>elpasedTime eq P60M</code> indicates a total elapsed time of 60 Minutes." ;
  skos:scopeNote "Non-Normative"@en .

odrl:delayPeriod
  a owl:NamedIndividual, skos:Concept, odrl:LeftOperand ;
  rdfs:isDefinedBy odrl: ;
  rdfs:label "Delay Period"@en ;
  skos:definition "A time delay period prior to exercising the action of the Rule. The point in time triggering this period MAY be defined by another temporal Constraint combined by a Logical Constraint (utilising the odrl:andSequence operand). Right operand value MUST be an xsd:duration as defined by [[xmlschema11-2]]."@en ;
  skos:note "Only the eq, gt, gteq operators SHOULD be used. <br />Example: <code>delayPeriod eq P60M</code> indicates a delay of 60 Minutes before exercising the action."@en ;
  skos:scopeNote "Non-Normative"@en .

<https://w3id.org/dpv/owl#SocialMediaMarketing>
  a owl:Class, owl:NamedIndividual, <https://w3id.org/dpv/owl#Purpose> ;
  rdfs:subClassOf <https://w3id.org/dpv/owl#Marketing> ;
  dc:contributor _:genid4, _:genid5, _:genid1 ;
  dc:created "2020-11-04"^^xsd:date ;
  ns1:term_status "accepted"@en ;
  skos:definition "Purposes associated with conducting marketing through social media"@en ;
  skos:prefLabel "Social Media Marketing"@en ;
  owl:sameAs <https://w3id.org/dpv#SocialMediaMarketing>, <https://w3id.org/dpv/dpv-owl#SocialMediaMarketing> .

<https://w3id.org/dpv/owl#AgeVerification>
  a owl:Class, owl:NamedIndividual, <https://w3id.org/dpv/owl#Purpose> ;
  rdfs:subClassOf <https://w3id.org/dpv/owl#Verification> ;
  dc:contributor _:genid5, _:genid1, _:genid67 ;
  dc:created "2024-02-14"^^xsd:date ;
  ns1:term_status "accepted"@en ;
  skos:definition "Purposes associated with verifying or authenticating age or age related information as a form of security"@en ;
  skos:prefLabel "Age Verification"@en ;
  skos:scopeNote "Age Verification can include verification of the exact age, e.g. being 21 years old, a date, e.g. birth date is 01 January 1969, or a condition, e.g. age is over 21 years and the person is an adult. Specific dedicated resources should be used to further express information and processes associated with Age Verification, for example the Age Verification Vocabulary https://w3id.org/age/"@en ;
  owl:sameAs <https://w3id.org/dpv#AgeVerification>, <https://w3id.org/dpv/dpv-owl#AgeVerification> .

odrl:uid
  a owl:AnnotationProperty, owl:NamedIndividual, skos:Concept ;
  rdfs:domain odrl:_:genid-nodeid-Nfcf59089734546b7891bf53bc9cb17f0 ;
  rdfs:isDefinedBy odrl: ;
  rdfs:label "Unique Identifier"@en ;
  skos:definition "An unambiguous identifier"@en ;
  skos:note "Used by the Policy, Rule, Asset, Party, Constraint, and Logical Constraint Classes."@en .

<https://w3id.org/dpv/owl#mitigatesRisk>
  a owl:ObjectProperty ;
  ns2:domainIncludes <https://w3id.org/dpv/owl#RiskMitigationMeasure> ;
  ns2:rangeIncludes <https://w3id.org/dpv/owl#Risk> ;
  dc:contributor _:genid1 ;
  dc:created "2020-11-04"^^xsd:date ;
  ns1:term_status "accepted"@en ;
  skos:definition "Indicates risks mitigated by this concept"@en ;
  skos:prefLabel "mitigates risk"@en ;
  ns0:domainIncludes <https://w3id.org/dpv/owl#RiskMitigationMeasure> ;
  ns0:rangeIncludes <https://w3id.org/dpv/owl#Risk> ;
  owl:sameAs <https://w3id.org/dpv#mitigatesRisk>, <https://w3id.org/dpv/dpv-owl#mitigatesRisk> .

<https://w3id.org/dpv/owl#GeographicCoverage>
  a owl:Class ;
  rdfs:subClassOf <https://w3id.org/dpv/owl#Scale> ;
  dc:contributor _:genid4, _:genid1, _:genid6 ;
  dc:created "2022-06-15"^^xsd:date ;
  ns3:example <https://w3id.org/dpv/examples/owl#E0049> ;
  ns1:term_status "accepted"@en ;
  skos:definition "Indicate of scale in terms of geographic coverage"@en ;
  skos:prefLabel "Geographic Coverage"@en ;
  owl:sameAs <https://w3id.org/dpv#GeographicCoverage>, <https://w3id.org/dpv/dpv-owl#GeographicCoverage> .

<https://w3id.org/dpv/owl#DataSubject>
  a owl:Class ;
  rdfs:subClassOf <https://w3id.org/dpv/owl#HumanSubject> ;
  dc:contributor _:genid13, _:genid11 ;
  dc:created "2019-04-05"^^xsd:date ;
  dc:modified "2024-12-17"^^xsd:date ;
  dc:source [
    a ns0:WebPage ;
    ns0:name "GDPR Art.4-1g" ;
    ns0:url "https://eur-lex.europa.eu/eli/reg/2016/679/art_4/par_1/oj"
  ] ;
  ns3:example <https://w3id.org/dpv/examples/owl#E0039>, <https://w3id.org/dpv/examples/owl#E0074> ;
  ns1:term_status "modified"@en ;
  skos:definition "The individual (or category of individuals) whose personal data is being processed"@en ;
  skos:prefLabel "Data Subject"@en ;
  skos:scopeNote "The term 'data subject' is specific to the GDPR, but is functionally equivalent to the term 'individual associated with data' and the ISO/IEC term 'PII Principle'"@en ;
  owl:sameAs <https://w3id.org/dpv#DataSubject>, <https://w3id.org/dpv/dpv-owl#DataSubject> .

<https://w3id.org/dpv/owl#ActivityProposed>
  a owl:Class, owl:NamedIndividual, <https://w3id.org/dpv/owl#ActivityStatus> ;
  rdfs:subClassOf <https://w3id.org/dpv/owl#ActivityStatus> ;
  dc:contributor _:genid1 ;
  dc:created "2022-05-18"^^xsd:date ;
  dc:modified "2024-05-19"^^xsd:date ;
  ns1:term_status "accepted"@en ;
  skos:definition "State of an activity being proposed without any concrete plans for implementation"@en ;
  skos:prefLabel "Activity Proposed"@en ;
  owl:sameAs <https://w3id.org/dpv#ActivityProposed>, <https://w3id.org/dpv/dpv-owl#ActivityProposed> .

<https://w3id.org/dpv/owl#IndeterminateDuration>
  a owl:Class, owl:NamedIndividual, <https://w3id.org/dpv/owl#Duration> ;
  rdfs:subClassOf <https://w3id.org/dpv/owl#Duration> ;
  dc:contributor _:genid1 ;
  dc:created "2022-11-30"^^xsd:date ;
  ns1:term_status "accepted"@en ;
  skos:definition "Duration that is indeterminate or cannot be determined"@en ;
  skos:prefLabel "Indeterminate Duration"@en ;
  skos:scopeNote "Indeterminate means (exact or otherwise) information about the duration cannot be determined, which is distinct from 'EndlessDuration' where it is known (or decided) that the duration is open-ended or without an end."@en ;
  owl:sameAs <https://w3id.org/dpv#IndeterminateDuration>, <https://w3id.org/dpv/dpv-owl#IndeterminateDuration> .

odrl:relativePosition
  a owl:NamedIndividual, skos:Concept, odrl:LeftOperand ;
  rdfs:isDefinedBy odrl: ;
  rdfs:label "Relative Asset Position"@en ;
  skos:definition "A point in space or time defined with coordinates relative to full measures the positioning of the target Asset."@en ;
  skos:note "Example: The upper left corner of a picture may be constrained to a specific position of the canvas rendering it."@en ;
  skos:scopeNote "Non-Normative"@en .

<https://w3id.org/dpv/owl#ChallengingProcess>
  a owl:Class, owl:NamedIndividual, <https://w3id.org/dpv/owl#EntityPermissiveInvolvement> ;
  rdfs:subClassOf <https://w3id.org/dpv/owl#EntityPermissiveInvolvement> ;
  dc:contributor _:genid1, _:genid25, _:genid19 ;
  dc:created "2024-05-11"^^xsd:date ;
  ns1:term_status "accepted"@en ;
  skos:definition "Involvement where entity can challenge the process of specified context"@en ;
  skos:prefLabel "Challenging Process"@en ;
  skos:scopeNote "Challenge refers to raising questions about validity, necessity, correctness, or other similar 'trustworthiness' attributes regarding the process or plan or implementation"@en ;
  owl:sameAs <https://w3id.org/dpv#ChallengingProcess>, <https://w3id.org/dpv/dpv-owl#ChallengingProcess> .

<https://w3id.org/dpv/owl#Authentication-PABC>
  a owl:Class, owl:NamedIndividual, <https://w3id.org/dpv/owl#TechnicalMeasure> ;
  rdfs:subClassOf <https://w3id.org/dpv/owl#CryptographicAuthentication> ;
  dc:contributor _:genid1 ;
  dc:created "2022-08-17"^^xsd:date ;
  dc:source [
    a ns0:WebPage ;
    ns0:name "ENISA Data Protection Engineering" ;
    ns0:url "https://www.enisa.europa.eu/publications/data-protection-engineering"
  ] ;
  ns1:term_status "accepted"@en ;
  skos:definition "Use of Privacy-enhancing Attribute Based Credentials (ABC) to perform and manage authentication"@en ;
  skos:prefLabel "Authentication using PABC"@en ;
  owl:sameAs <https://w3id.org/dpv#Authentication-PABC>, <https://w3id.org/dpv/dpv-owl#Authentication-PABC> .

<https://w3id.org/dpv/owl#isDuring>
  a owl:ObjectProperty ;
  dc:contributor _:genid1 ;
  dc:created "2024-08-13"^^xsd:date ;
  ns1:term_status "accepted"@en ;
  skos:definition "Indicates the specified concepts occur 'during' this concept in some context"@en ;
  skos:prefLabel "is during"@en ;
  owl:sameAs <https://w3id.org/dpv#isDuring>, <https://w3id.org/dpv/dpv-owl#isDuring> .

<https://w3id.org/dpv/owl#OperatingSystemSecurity>
  a owl:Class, owl:NamedIndividual, <https://w3id.org/dpv/owl#TechnicalMeasure> ;
  rdfs:subClassOf <https://w3id.org/dpv/owl#SecurityMethod> ;
  dc:contributor _:genid1 ;
  dc:created "2022-08-17"^^xsd:date ;
  dc:source [
    a ns0:WebPage ;
    ns0:name "ENISA Reference Incident Classification Taxonomy 2018" ;
    ns0:url "https://www.enisa.europa.eu/publications/reference-incident-classification-taxonomy/"
  ] ;
  ns1:term_status "accepted"@en ;
  skos:definition "Security implemented at or through operating systems"@en ;
  skos:prefLabel "Operating System Security"@en ;
  owl:sameAs <https://w3id.org/dpv#OperatingSystemSecurity>, <https://w3id.org/dpv/dpv-owl#OperatingSystemSecurity> .

<https://w3id.org/dpv/owl#EntityInvolved>
  a owl:Class, owl:NamedIndividual, <https://w3id.org/dpv/owl#EntityInvolvementStatus> ;
  rdfs:subClassOf <https://w3id.org/dpv/owl#EntityInvolvementStatus> ;
  dc:contributor _:genid25 ;
  dc:created "2024-12-01"^^xsd:date ;
  ns1:term_status "accepted"@en ;
  skos:definition "Status indicating the entity is involved"@en ;
  skos:prefLabel "Entity Involved"@en ;
  owl:sameAs <https://w3id.org/dpv#EntityInvolved>, <https://w3id.org/dpv/dpv-owl#EntityInvolved> .

<https://w3id.org/dpv/owl#RequestStatusQuery>
  a owl:Class, owl:NamedIndividual, <https://w3id.org/dpv/owl#RequestStatus> ;
  rdfs:subClassOf <https://w3id.org/dpv/owl#RequestStatus> ;
  dc:contributor _:genid1 ;
  dc:created "2022-11-30"^^xsd:date ;
  ns1:term_status "accepted"@en ;
  skos:definition "State of a request's status being queried"@en ;
  skos:prefLabel "Request Status Query"@en ;
  owl:sameAs <https://w3id.org/dpv#RequestStatusQuery>, <https://w3id.org/dpv/dpv-owl#RequestStatusQuery> .

<https://w3id.org/dpv/owl#OrganisationalUnit>
  a owl:Class ;
  rdfs:subClassOf <https://w3id.org/dpv/owl#Entity> ;
  dc:contributor _:genid1, _:genid6 ;
  dc:created "2022-03-23"^^xsd:date ;
  ns3:example <https://w3id.org/dpv/examples/owl#E0037> ;
  ns1:term_status "accepted"@en ;
  skos:definition "Entity within an organisation that does not constitute as a separate legal entity"@en ;
  skos:prefLabel "Organisational Unit"@en ;
  owl:sameAs <https://w3id.org/dpv#OrganisationalUnit>, <https://w3id.org/dpv/dpv-owl#OrganisationalUnit> .

<https://w3id.org/dpv/owl#EntityIntendedInvolvement>
  a owl:Class, owl:NamedIndividual, <https://w3id.org/dpv/owl#EntityInvolvementStatus> ;
  rdfs:subClassOf <https://w3id.org/dpv/owl#EntityInvolvement>, <https://w3id.org/dpv/owl#Intended> ;
  dc:contributor _:genid25 ;
  dc:created "2024-12-01"^^xsd:date ;
  ns1:term_status "accepted"@en ;
  skos:definition "Status indicating the involvement of the entity is intended"@en ;
  skos:prefLabel "Entity Intended Involvement"@en ;
  owl:sameAs <https://w3id.org/dpv#EntityIntendedInvolvement>, <https://w3id.org/dpv/dpv-owl#EntityIntendedInvolvement> .

<https://w3id.org/dpv/owl#isApplicableFor>
  a owl:ObjectProperty ;
  ns2:rangeIncludes <https://w3id.org/dpv/owl#Scope> ;
  dc:contributor _:genid4, _:genid5, _:genid1, _:genid6 ;
  dc:created "2024-04-13"^^xsd:date ;
  ns1:term_status "accepted"@en ;
  skos:definition "Indicates the concept or information is applicable for specified context"@en ;
  skos:prefLabel "is applicable for"@en ;
  ns0:rangeIncludes <https://w3id.org/dpv/owl#Scope> ;
  owl:sameAs <https://w3id.org/dpv#isApplicableFor>, <https://w3id.org/dpv/dpv-owl#isApplicableFor> .

<https://w3id.org/dpv/owl#DataBackupProtocols>
  a owl:Class, owl:NamedIndividual, <https://w3id.org/dpv/owl#TechnicalMeasure> ;
  rdfs:subClassOf <https://w3id.org/dpv/owl#TechnicalMeasure> ;
  dc:contributor _:genid4 ;
  dc:created "2022-06-15"^^xsd:date ;
  ns1:term_status "accepted"@en ;
  skos:definition "Protocols or plans for backing up of data"@en ;
  skos:prefLabel "Data Backup Protocols"@en ;
  owl:sameAs <https://w3id.org/dpv#DataBackupProtocols>, <https://w3id.org/dpv/dpv-owl#DataBackupProtocols> .

skos:hasTopConcept a owl:AnnotationProperty .
<https://w3id.org/dpv/owl#TechnicalStandard>
  a owl:Class, owl:NamedIndividual, <https://w3id.org/dpv/owl#OrganisationalMeasure> ;
  rdfs:subClassOf <https://w3id.org/dpv/owl#Standard> ;
  dc:contributor _:genid1 ;
  dc:created "2024-12-01"^^xsd:date ;
  ns1:term_status "accepted"@en ;
  skos:definition "A technical standard is a standard that establishes norms or requirements regarding technology or technical processes"@en ;
  skos:prefLabel "Technical Standard"@en ;
  owl:sameAs <https://w3id.org/dpv#TechnicalStandard>, <https://w3id.org/dpv/dpv-owl#TechnicalStandard> .

<https://w3id.org/dpv/owl#isSubsidiaryOf>
  a owl:ObjectProperty ;
  rdfs:subPropertyOf <https://w3id.org/dpv/owl#hasEntity> ;
  ns2:domainIncludes <https://w3id.org/dpv/owl#Organisation> ;
  ns2:rangeIncludes <https://w3id.org/dpv/owl#Organisation> ;
  dc:contributor _:genid4, _:genid1 ;
  dc:created "2024-04-14"^^xsd:date ;
  ns1:term_status "accepted"@en ;
  skos:definition "Indicates this entity is the subsidiary of the specified entity"@en ;
  skos:prefLabel "is subsidiary of"@en ;
  ns0:domainIncludes <https://w3id.org/dpv/owl#Organisation> ;
  ns0:rangeIncludes <https://w3id.org/dpv/owl#Organisation> ;
  owl:sameAs <https://w3id.org/dpv#isSubsidiaryOf>, <https://w3id.org/dpv/dpv-owl#isSubsidiaryOf> .

odrl:resolution
  a owl:NamedIndividual, skos:Concept, odrl:LeftOperand ;
  rdfs:isDefinedBy odrl: ;
  rdfs:label "Rendition Resolution"@en ;
  skos:definition "Resolution of the rendition of the target Asset."@en ;
  skos:note "Example: the image may be printed at 1200dpi."@en ;
  skos:scopeNote "Non-Normative"@en .

<https://w3id.org/dpv/owl#AuditApproved>
  a owl:Class, owl:NamedIndividual, <https://w3id.org/dpv/owl#AuditStatus> ;
  rdfs:subClassOf <https://w3id.org/dpv/owl#AuditStatus> ;
  dc:contributor _:genid1 ;
  dc:created "2022-05-18"^^xsd:date ;
  ns1:term_status "accepted"@en ;
  skos:definition "State of being approved through the audit"@en ;
  skos:prefLabel "Audit Approved"@en ;
  owl:sameAs <https://w3id.org/dpv#AuditApproved>, <https://w3id.org/dpv/dpv-owl#AuditApproved> .

odrl:install
  a owl:NamedIndividual, skos:Concept, odrl:Action ;
  odrl:includedIn odrl:use ;
  rdfs:isDefinedBy odrl: ;
  rdfs:label "Install"@en ;
  skos:definition "To load the computer program Asset onto a storage device which allows operating or running the Asset."@en ;
  skos:scopeNote "Non-Normative"@en .

<https://w3id.org/dpv/owl#hasAuthority>
  a owl:ObjectProperty ;
  ns2:rangeIncludes <https://w3id.org/dpv/owl#Authority> ;
  dc:contributor _:genid4, _:genid1 ;
  dc:created "2022-01-19"^^xsd:date ;
  ns1:term_status "accepted"@en ;
  skos:definition "Indicates applicability of authority for a jurisdiction"@en ;
  skos:prefLabel "has authority"@en ;
  ns0:rangeIncludes <https://w3id.org/dpv/owl#Authority> ;
  owl:sameAs <https://w3id.org/dpv#hasAuthority>, <https://w3id.org/dpv/dpv-owl#hasAuthority> .

odrl:product
  a owl:NamedIndividual, skos:Concept, odrl:LeftOperand ;
  rdfs:isDefinedBy odrl: ;
  rdfs:label "Product Context"@en ;
  skos:definition "Category of product or service setting a context for exercising the action of the Rule."@en ;
  skos:note "Example: May only be used in the XYZ Magazine."@en ;
  skos:scopeNote "Non-Normative"@en .

<https://w3id.org/dpv/owl#ConsentStatusValidForProcessing>
  a owl:Class, owl:NamedIndividual, <https://w3id.org/dpv/owl#ConsentStatus> ;
  rdfs:subClassOf <https://w3id.org/dpv/owl#ConsentStatus> ;
  dc:contributor _:genid4, _:genid1, _:genid17, _:genid6 ;
  dc:created "2022-06-22"^^xsd:date ;
  dc:source [
    a ns0:WebPage ;
    ns0:name "GConsent" ;
    ns0:url "https://w3id.org/GConsent"
  ] ;
  ns1:term_status "accepted"@en ;
  skos:definition "States of consent that can be used as valid justifications for processing data"@en ;
  skos:prefLabel "Consent Status Valid for Processing"@en ;
  skos:scopeNote "Practically, given consent is the only valid state for processing"@en ;
  owl:sameAs <https://w3id.org/dpv#ConsentStatusValidForProcessing>, <https://w3id.org/dpv/dpv-owl#ConsentStatusValidForProcessing> .

<https://w3id.org/dpv/owl#ContextuallyAnonymisedData>
  a owl:Class ;
  rdfs:subClassOf <https://w3id.org/dpv/owl#PseudonymisedData> ;
  dc:contributor _:genid1 ;
  dc:created "2024-06-11"^^xsd:date ;
  ns1:term_status "accepted"@en ;
  skos:definition "Data that can be considered as being fully anonymised within the context but in actuality is not fully anonymised and is still personal data as it can be de-anonymised outside that context"@en ;
  skos:prefLabel "Contextually Anonymised Data"@en ;
  skos:scopeNote "To distinguish between partially anonymised data that can be effectively treated as anonymised data (e.g. in processing) within a context (e.g. an organisation), the concept ContextuallyAnonymisedData should be used instead of AnonymisedData. Transfer of this data outside of the context should consider that it is not fully anonymised and that it is still personal data"@en ;
  owl:sameAs <https://w3id.org/dpv#ContextuallyAnonymisedData>, <https://w3id.org/dpv/dpv-owl#ContextuallyAnonymisedData> .

odrl:LogicalConstraint
  a owl:Class, owl:NamedIndividual, skos:Concept ;
  rdfs:isDefinedBy odrl: ;
  rdfs:label "Logical Constraint"@en ;
  skos:definition "A logical expression that refines the semantics of an Action and Party/Asset Collection or declare the conditions applicable to a Rule."@en .

odrl:Party
  a owl:Class, owl:NamedIndividual, skos:Concept ;
  rdfs:subClassOf [
    a owl:Class ;
    owl:unionOf (
     schema:Organization
     schema:Person
     vcard:Agent
     vcard:Individual
     vcard:Organization
     foaf:Agent
     foaf:Organization
     foaf:Person
   )
  ] ;
  rdfs:isDefinedBy odrl: ;
  rdfs:label "Party"@en ;
  skos:definition "An entity or a collection of entities that undertake Roles in a Rule."@en ;
  skos:note "The Party entity could be a person, group of people, organisation, or agent. An agent is a person or thing that takes an active role or produces a specified effect. To describe more details about the Party, it is recommended to use W3C vCard Ontology [[vcard-rdf]] or FOAF Vocabulary [[foaf]]."@en .

<https://w3id.org/dpv/owl#Conformant>
  a owl:Class, owl:NamedIndividual, <https://w3id.org/dpv/owl#ConformanceStatus> ;
  rdfs:subClassOf <https://w3id.org/dpv/owl#ConformanceStatus> ;
  dc:contributor _:genid1 ;
  dc:created "2022-10-22"^^xsd:date ;
  ns1:term_status "accepted"@en ;
  skos:definition "State of being conformant"@en ;
  skos:prefLabel "Conformant"@en ;
  owl:sameAs <https://w3id.org/dpv#Conformant>, <https://w3id.org/dpv/dpv-owl#Conformant> .

<https://w3id.org/dpv/owl#DataProtectionOfficer>
  a owl:Class ;
  rdfs:subClassOf <https://w3id.org/dpv/owl#Representative> ;
  dc:contributor _:genid4, _:genid6 ;
  dc:created "2020-11-04"^^xsd:date ;
  dc:modified "2021-12-08"^^xsd:date ;
  dc:source [
    a ns0:WebPage ;
    ns0:name "GDPR Art.37" ;
    ns0:url "https://eur-lex.europa.eu/eli/reg/2016/679/art_37/oj"
  ] ;
  ns1:term_status "accepted"@en ;
  skos:definition "An entity within or authorised by an organisation to monitor internal compliance, inform and advise on data protection obligations and act as a contact point for data subjects and the supervisory authority."@en ;
  skos:prefLabel "Data Protection Officer"@en ;
  owl:sameAs <https://w3id.org/dpv#DataProtectionOfficer>, <https://w3id.org/dpv/dpv-owl#DataProtectionOfficer> .

<https://w3id.org/dpv/owl#DataRestorationPolicy>
  a owl:Class, owl:NamedIndividual, <https://w3id.org/dpv/owl#OrganisationalMeasure> ;
  rdfs:subClassOf <https://w3id.org/dpv/owl#DataProcessingPolicy> ;
  dc:contributor _:genid4, _:genid1 ;
  dc:created "2024-04-14"^^xsd:date ;
  ns1:term_status "accepted"@en ;
  skos:definition "Policy regarding restoration of data"@en ;
  skos:prefLabel "Data Restoration Policy"@en ;
  skos:scopeNote "Restoration can refer to how data is restored from a backup"@en ;
  owl:sameAs <https://w3id.org/dpv#DataRestorationPolicy>, <https://w3id.org/dpv/dpv-owl#DataRestorationPolicy> .

<https://w3id.org/dpv/owl#SporadicFrequency>
  a owl:Class, owl:NamedIndividual, <https://w3id.org/dpv/owl#Frequency> ;
  rdfs:subClassOf <https://w3id.org/dpv/owl#Frequency> ;
  dc:contributor _:genid1 ;
  dc:created "2022-06-15"^^xsd:date ;
  dc:modified "2020-10-05"^^xsd:date ;
  ns1:term_status "accepted"@en ;
  skos:definition "Frequency where occurrences are sporadic or infrequent or sparse"@en ;
  skos:prefLabel "Sporadic Frequency"@en ;
  owl:sameAs <https://w3id.org/dpv#SporadicFrequency>, <https://w3id.org/dpv/dpv-owl#SporadicFrequency> .

ns0:url a owl:AnnotationProperty .
<https://w3id.org/dpv/owl#Region>
  a owl:Class ;
  rdfs:subClassOf <https://w3id.org/dpv/owl#Country> ;
  dc:contributor _:genid1 ;
  dc:created "2022-01-19"^^xsd:date ;
  ns1:term_status "accepted"@en ;
  skos:definition "A region is an area or site that is considered a location"@en ;
  skos:prefLabel "Region"@en ;
  owl:sameAs <https://w3id.org/dpv#Region>, <https://w3id.org/dpv/dpv-owl#Region> .

<https://w3id.org/dpv/owl#Combine>
  a owl:Class, owl:NamedIndividual, <https://w3id.org/dpv/owl#Processing> ;
  rdfs:subClassOf <https://w3id.org/dpv/owl#Transform> ;
  dc:created "2019-05-07"^^xsd:date ;
  dc:source [
    a ns0:WebPage ;
    ns0:name "GDPR Art.4-2" ;
    ns0:url "https://eur-lex.europa.eu/eli/reg/2016/679/art_4/par_2/oj"
  ] ;
  ns1:term_status "accepted"@en ;
  skos:definition "to join or merge data"@en ;
  skos:prefLabel "Combine Data"@en ;
  skos:related <https://specialprivacy.ercim.eu/vocabs/processing#Aggregate> ;
  owl:sameAs <https://w3id.org/dpv#Combine>, <https://w3id.org/dpv/dpv-owl#Combine> .

<https://w3id.org/dpv/owl#Store>
  a owl:Class, owl:NamedIndividual, <https://w3id.org/dpv/owl#Processing> ;
  rdfs:subClassOf <https://w3id.org/dpv/owl#Processing> ;
  dc:created "2019-05-07"^^xsd:date ;
  dc:source [
    a ns0:WebPage ;
    ns0:name "GDPR Art.4-2" ;
    ns0:url "https://eur-lex.europa.eu/eli/reg/2016/679/art_4/par_2/oj"
  ] ;
  ns1:term_status "accepted"@en ;
  skos:definition "to keep data for future use"@en ;
  skos:prefLabel "Store Data"@en ;
  owl:sameAs <https://w3id.org/dpv#Store>, <https://w3id.org/dpv/dpv-owl#Store> .

<https://w3id.org/dpv/owl#PublicInterestPending>
  a owl:Class, owl:NamedIndividual, <https://w3id.org/dpv/owl#PublicInterestStatus> ;
  rdfs:subClassOf <https://w3id.org/dpv/owl#PublicInterestStatus> ;
  dc:created "2024-08-27"^^xsd:date ;
  ns1:term_status "accepted"@en ;
  skos:definition "Status where the public interest activity has not started"@en ;
  skos:prefLabel "Public Interest Pending"@en ;
  owl:sameAs <https://w3id.org/dpv#PublicInterestPending>, <https://w3id.org/dpv/dpv-owl#PublicInterestPending> .

<https://w3id.org/dpv/owl#VariableLocation>
  a owl:Class, owl:NamedIndividual, <https://w3id.org/dpv/owl#LocationFixture> ;
  rdfs:subClassOf <https://w3id.org/dpv/owl#LocationFixture> ;
  dc:contributor _:genid1 ;
  dc:created "2022-06-15"^^xsd:date ;
  dc:modified "2020-10-05"^^xsd:date ;
  ns1:term_status "accepted"@en ;
  skos:definition "Location that is known but is variable e.g. somewhere within a given area"@en ;
  skos:prefLabel "Variable Location"@en ;
  owl:sameAs <https://w3id.org/dpv#VariableLocation>, <https://w3id.org/dpv/dpv-owl#VariableLocation> .

odrl:partOf
  a owl:ObjectProperty, owl:NamedIndividual, skos:Concept ;
  rdfs:domain [
    a owl:Class ;
    owl:unionOf (
     odrl:Asset
     odrl:Party
   )
  ] ;
  rdfs:range [
    a owl:Class ;
    owl:unionOf (
     odrl:AssetCollection
     odrl:PartyCollection
   )
  ] ;
  rdfs:isDefinedBy odrl: ;
  rdfs:label "Part Of"@en ;
  skos:definition "Identifies an Asset/PartyCollection that the Asset/Party is a member of."@en .

odrl:use
  a owl:NamedIndividual, skos:Concept, odrl:Action ;
  rdfs:isDefinedBy odrl: ;
  rdfs:label "Use"@en ;
  skos:definition "To use the Asset"@en ;
  skos:note "Use is the most generic action for all non-third-party usage. More specific types of the use action can be expressed by more targetted actions."@en .

<https://w3id.org/dpv/owl#hasEntity>
  a owl:ObjectProperty ;
  ns2:rangeIncludes <https://w3id.org/dpv/owl#Entity> ;
  dc:contributor _:genid1 ;
  dc:created "2022-02-09"^^xsd:date ;
  ns1:term_status "accepted"@en ;
  skos:definition "Indicates inclusion or applicability of an entity to some concept"@en ;
  skos:prefLabel "has entity"@en ;
  skos:scopeNote "parent property for controller, processor, data subject, authority, etc.?"@en ;
  ns0:rangeIncludes <https://w3id.org/dpv/owl#Entity> ;
  owl:sameAs <https://w3id.org/dpv#hasEntity>, <https://w3id.org/dpv/dpv-owl#hasEntity> .

odrl:fileFormat
  a owl:NamedIndividual, skos:Concept, odrl:LeftOperand ;
  rdfs:isDefinedBy odrl: ;
  rdfs:label "File Format"@en ;
  skos:definition "A transformed file format of the target Asset."@en ;
  skos:note "Example: An asset may be transformed into JPEG format."@en ;
  skos:scopeNote "Non-Normative"@en .

<https://w3id.org/dpv/owl#DataQualityImprovement>
  a owl:Class, owl:NamedIndividual, <https://w3id.org/dpv/owl#OrganisationalMeasure> ;
  rdfs:subClassOf <https://w3id.org/dpv/owl#DataQualityManagement> ;
  dc:contributor _:genid1 ;
  dc:created "2024-04-14"^^xsd:date ;
  ns1:term_status "accepted"@en ;
  skos:definition "Measures associated with improvement of data quality"@en ;
  skos:prefLabel "Data Quality Improvement"@en ;
  owl:sameAs <https://w3id.org/dpv#DataQualityImprovement>, <https://w3id.org/dpv/dpv-owl#DataQualityImprovement> .

<https://w3id.org/dpv/owl#DerivedPersonalData>
  a owl:Class ;
  rdfs:subClassOf <https://w3id.org/dpv/owl#DerivedData>, <https://w3id.org/dpv/owl#PersonalData> ;
  dc:contributor _:genid1, _:genid15, _:genid16 ;
  dc:created "2019-05-07"^^xsd:date ;
  dc:modified "2023-12-10"^^xsd:date ;
  dc:source [
    a ns0:WebPage ;
    ns0:name "DPVCG" ;
    ns0:url "https://www.w3.org/community/dpvcg/"
  ] ;
  ns3:example <https://w3id.org/dpv/examples/owl#E0009>, <https://w3id.org/dpv/examples/owl#E0046> ;
  ns1:term_status "accepted"@en ;
  skos:definition "Personal Data that is obtained or derived from other data"@en ;
  skos:prefLabel "Derived Personal Data"@en ;
  skos:related <https://specialprivacy.ercim.eu/vocabs/data#Derived> ;
  skos:scopeNote "Derived Data is data that is obtained through processing of existing data, e.g. deriving first name from full name. To indicate data that is derived but which was not present or evident within the source data, InferredPersonalData should be used."@en ;
  owl:sameAs <https://w3id.org/dpv#DerivedPersonalData>, <https://w3id.org/dpv/dpv-owl#DerivedPersonalData> .

<https://w3id.org/dpv/owl#RuleViolated>
  a owl:Class, owl:NamedIndividual, <https://w3id.org/dpv/owl#RuleFulfilmentStatus> ;
  rdfs:subClassOf <https://w3id.org/dpv/owl#RuleFulfilmentStatus> ;
  dc:contributor _:genid1 ;
  dc:created "2024-09-10"^^xsd:date ;
  ns1:term_status "accepted"@en ;
  skos:definition "Status indicating a rule has been violated, breached, broken, or infracted"@en ;
  skos:prefLabel "Rule Violated"@en ;
  owl:sameAs <https://w3id.org/dpv#RuleViolated>, <https://w3id.org/dpv/dpv-owl#RuleViolated> .

<https://w3id.org/dpv/owl#NationalAuthority>
  a owl:Class ;
  rdfs:subClassOf <https://w3id.org/dpv/owl#Authority> ;
  dc:contributor _:genid1 ;
  dc:created "2022-02-02"^^xsd:date ;
  dc:source [
    a ns0:WebPage ;
    ns0:name "ADMS controlled vocabulary" ;
    ns0:url "http://purl.org/adms"
  ] ;
  ns1:term_status "accepted"@en ;
  skos:definition "An authority tasked with overseeing legal compliance for a nation"@en ;
  skos:prefLabel "National Authority"@en ;
  owl:sameAs <https://w3id.org/dpv#NationalAuthority>, <https://w3id.org/dpv/dpv-owl#NationalAuthority> .

<https://w3id.org/dpv/owl#Display>
  a owl:Class, owl:NamedIndividual, <https://w3id.org/dpv/owl#Processing> ;
  rdfs:subClassOf <https://w3id.org/dpv/owl#Disclose> ;
  dc:contributor _:genid5 ;
  dc:created "2024-04-14"^^xsd:date ;
  dc:source "DGA 2.20"@en ;
  ns1:term_status "accepted"@en ;
  skos:definition "to present or show data"@en ;
  skos:prefLabel "Display Data"@en ;
  owl:sameAs <https://w3id.org/dpv#Display>, <https://w3id.org/dpv/dpv-owl#Display> .

<https://w3id.org/dpv/owl#PermissionManagement>
  a owl:Class, owl:NamedIndividual, <https://w3id.org/dpv/owl#OrganisationalMeasure> ;
  rdfs:subClassOf <https://w3id.org/dpv/owl#RightsManagement> ;
  dc:contributor _:genid4, _:genid5, _:genid1 ;
  dc:created "2024-04-14"^^xsd:date ;
  dc:source "DGA 12.n"@en ;
  ns1:term_status "accepted"@en ;
  skos:definition "Methods to obtain, provide, modify, and withdraw permissions along with maintaining a record of permissions, retrieving records, and processing changes in permission states"@en ;
  skos:prefLabel "Permission Management"@en ;
  skos:scopeNote "Permission is a broader concept than '(Informed) Consent' as consent when used as a legal basis has specific requirements to be valid. For management of consent, see the concept dpv:ConsentManagement"@en ;
  owl:sameAs <https://w3id.org/dpv#PermissionManagement>, <https://w3id.org/dpv/dpv-owl#PermissionManagement> .

<https://w3id.org/dpv/owl#PersonnelPerformancePrediction>
  a owl:Class, owl:NamedIndividual, <https://w3id.org/dpv/owl#Purpose> ;
  rdfs:subClassOf <https://w3id.org/dpv/owl#PersonnelPerformanceManagement> ;
  dc:created "2024-12-01"^^xsd:date ;
  ns1:term_status "accepted"@en ;
  skos:definition "Purposes associated with prediction of performance of personnel"@en ;
  skos:prefLabel "Personnel Performance Prediction"@en ;
  owl:sameAs <https://w3id.org/dpv#PersonnelPerformancePrediction>, <https://w3id.org/dpv/dpv-owl#PersonnelPerformancePrediction> .

<https://w3id.org/dpv/owl#LegitimateInterestUninformed>
  a owl:Class, owl:NamedIndividual, <https://w3id.org/dpv/owl#LegitimateInterestStatus> ;
  rdfs:subClassOf <https://w3id.org/dpv/owl#LegitimateInterestStatus> ;
  dc:created "2024-08-27"^^xsd:date ;
  ns1:term_status "accepted"@en ;
  skos:definition "Status where the Legitimate Interest was not informed to the data subject or other relevant entities"@en ;
  skos:prefLabel "Legitimate InterestUninformed"@en ;
  owl:sameAs <https://w3id.org/dpv#LegitimateInterestUninformed>, <https://w3id.org/dpv/dpv-owl#LegitimateInterestUninformed> .

<https://w3id.org/dpv/owl#EntityInvolvement>
  a owl:Class ;
  rdfs:subClassOf <https://w3id.org/dpv/owl#ProcessingContext> ;
  dc:contributor _:genid1, _:genid25 ;
  dc:created "2024-05-11"^^xsd:date ;
  ns1:term_status "accepted"@en ;
  skos:definition "Involvement of an entity in specific context"@en ;
  skos:prefLabel "Entity Involvement"@en ;
  owl:sameAs <https://w3id.org/dpv#EntityInvolvement>, <https://w3id.org/dpv/dpv-owl#EntityInvolvement> .

<https://w3id.org/dpv/owl#WirelessSecurityProtocols>
  a owl:Class, owl:NamedIndividual, <https://w3id.org/dpv/owl#TechnicalMeasure> ;
  rdfs:subClassOf <https://w3id.org/dpv/owl#SecurityMethod> ;
  dc:contributor _:genid1 ;
  dc:created "2022-08-17"^^xsd:date ;
  dc:source [
    a ns0:WebPage ;
    ns0:name "ENISA Reference Incident Classification Taxonomy 2018" ;
    ns0:url "https://www.enisa.europa.eu/publications/reference-incident-classification-taxonomy/"
  ] ;
  ns1:term_status "accepted"@en ;
  skos:definition "Security implemented at or over wireless communication protocols"@en ;
  skos:prefLabel "Wireless Security Protocols"@en ;
  owl:sameAs <https://w3id.org/dpv#WirelessSecurityProtocols>, <https://w3id.org/dpv/dpv-owl#WirelessSecurityProtocols> .

<https://w3id.org/dpv/owl#PhysicalSupplySecurity>
  a owl:Class, owl:NamedIndividual, <https://w3id.org/dpv/owl#PhysicalMeasure> ;
  rdfs:subClassOf <https://w3id.org/dpv/owl#PhysicalMeasure> ;
  dc:contributor _:genid1 ;
  dc:created "2024-04-14"^^xsd:date ;
  dc:source "NIST SP 800-14"@en ;
  ns1:term_status "accepted"@en ;
  skos:definition "Physically securing the supply of resources"@en ;
  skos:prefLabel "Physical Supply Security"@en ;
  owl:sameAs <https://w3id.org/dpv#PhysicalSupplySecurity>, <https://w3id.org/dpv/dpv-owl#PhysicalSupplySecurity> .

<https://w3id.org/dpv/owl#User>
  a owl:Class, owl:NamedIndividual, <https://w3id.org/dpv/owl#HumanSubject> ;
  rdfs:subClassOf <https://w3id.org/dpv/owl#HumanSubject> ;
  dc:contributor _:genid4, _:genid5, _:genid1, _:genid17, _:genid6 ;
  dc:created "2022-04-06"^^xsd:date ;
  dc:modified "2024-12-17"^^xsd:date ;
  ns1:term_status "modified"@en ;
  skos:definition "Humans that use service(s)"@en ;
  skos:prefLabel "User"@en ;
  owl:sameAs <https://w3id.org/dpv#User>, <https://w3id.org/dpv/dpv-owl#User> .

<https://w3id.org/dpv/owl#hasProcessingScale>
  a owl:ObjectProperty ;
  rdfs:subPropertyOf <https://w3id.org/dpv/owl#hasScale> ;
  ns2:rangeIncludes <https://w3id.org/dpv/owl#ProcessingScale> ;
  dc:contributor _:genid1 ;
  dc:created "2024-12-01"^^xsd:date ;
  ns1:term_status "accepted"@en ;
  skos:definition "Indicates the scale of processing operations"@en ;
  skos:prefLabel "has processing scale"@en ;
  ns0:rangeIncludes <https://w3id.org/dpv/owl#ProcessingScale> ;
  owl:sameAs <https://w3id.org/dpv#hasProcessingScale>, <https://w3id.org/dpv/dpv-owl#hasProcessingScale> .

<https://w3id.org/dpv/owl#RegionalAuthority>
  a owl:Class ;
  rdfs:subClassOf <https://w3id.org/dpv/owl#Authority> ;
  dc:contributor _:genid1 ;
  dc:created "2022-02-02"^^xsd:date ;
  dc:source [
    a ns0:WebPage ;
    ns0:name "ADMS controlled vocabulary" ;
    ns0:url "http://purl.org/adms"
  ] ;
  ns1:term_status "accepted"@en ;
  skos:definition "An authority tasked with overseeing legal compliance for a region"@en ;
  skos:prefLabel "Regional Authority"@en ;
  owl:sameAs <https://w3id.org/dpv#RegionalAuthority>, <https://w3id.org/dpv/dpv-owl#RegionalAuthority> .

<https://w3id.org/dpv/owl#hasRiskAssessment>
  a owl:ObjectProperty ;
  rdfs:subPropertyOf <https://w3id.org/dpv/owl#hasAssessment> ;
  ns2:rangeIncludes <https://w3id.org/dpv/owl#RiskAssessment> ;
  dc:contributor _:genid1 ;
  dc:created "2024-04-14"^^xsd:date ;
  ns1:term_status "accepted"@en ;
  skos:definition "Indicates an associated risk assessment"@en ;
  skos:prefLabel "has risk assessment"@en ;
  ns0:rangeIncludes <https://w3id.org/dpv/owl#RiskAssessment> ;
  owl:sameAs <https://w3id.org/dpv#hasRiskAssessment>, <https://w3id.org/dpv/dpv-owl#hasRiskAssessment> .

<https://w3id.org/dpv/owl#ThirdCountry>
  a owl:Class ;
  rdfs:subClassOf <https://w3id.org/dpv/owl#Country> ;
  dc:contributor _:genid1 ;
  dc:created "2022-02-09"^^xsd:date ;
  ns1:term_status "accepted"@en ;
  skos:definition "Represents a country outside applicable or compatible jurisdiction as outlined in law"@en ;
  skos:prefLabel "Third Country"@en ;
  owl:sameAs <https://w3id.org/dpv#ThirdCountry>, <https://w3id.org/dpv/dpv-owl#ThirdCountry> .

odrl:implies
  a owl:ObjectProperty, owl:NamedIndividual, skos:Concept ;
  rdfs:domain odrl:Action ;
  rdfs:range odrl:Action ;
  rdfs:isDefinedBy odrl: ;
  rdfs:label "Implies"@en ;
  skos:definition "An Action asserts that another Action is not prohibited to enable its operational semantics."@en ;
  skos:note "The property asserts that an instance of Action entails that the other instance of Action is not prohibited."@en .

<https://w3id.org/dpv/owl#ComplianceMonitoring>
  a owl:Class, owl:NamedIndividual, <https://w3id.org/dpv/owl#OrganisationalMeasure> ;
  rdfs:subClassOf <https://w3id.org/dpv/owl#GovernanceProcedures> ;
  dc:contributor _:genid1 ;
  dc:created "2022-08-17"^^xsd:date ;
  dc:source [
    a ns0:WebPage ;
    ns0:name "ENISA 5G Cybersecurity Standards" ;
    ns0:url "https://www.enisa.europa.eu/publications/5g-cybersecurity-standards"
  ] ;
  ns1:term_status "accepted"@en ;
  skos:definition "Monitoring of compliance (e.g. internal policy, regulations)"@en ;
  skos:prefLabel "Compliance Monitoring"@en ;
  owl:sameAs <https://w3id.org/dpv#ComplianceMonitoring>, <https://w3id.org/dpv/dpv-owl#ComplianceMonitoring> .

<https://w3id.org/dpv/owl#PrimaryImportance>
  a owl:Class, owl:NamedIndividual, <https://w3id.org/dpv/owl#Importance> ;
  rdfs:subClassOf <https://w3id.org/dpv/owl#Importance> ;
  dc:contributor _:genid4, _:genid5, _:genid1, _:genid17, _:genid6 ;
  dc:created "2022-02-10"^^xsd:date ;
  ns1:term_status "accepted"@en ;
  skos:definition "Indication of 'primary' or 'main' or 'core' importance"@en ;
  skos:prefLabel "Primary Importance"@en ;
  owl:sameAs <https://w3id.org/dpv#PrimaryImportance>, <https://w3id.org/dpv/dpv-owl#PrimaryImportance> .

<https://w3id.org/dpv/owl#EndlessDuration>
  a owl:Class, owl:NamedIndividual, <https://w3id.org/dpv/owl#Duration> ;
  rdfs:subClassOf <https://w3id.org/dpv/owl#Duration> ;
  dc:contributor _:genid1 ;
  dc:created "2022-06-15"^^xsd:date ;
  dc:modified "2020-10-05"^^xsd:date ;
  ns1:term_status "accepted"@en ;
  skos:definition "Duration that is (known or intended to be) open ended or without an end"@en ;
  skos:prefLabel "Endless Duration"@en ;
  owl:sameAs <https://w3id.org/dpv#EndlessDuration>, <https://w3id.org/dpv/dpv-owl#EndlessDuration> .

odrl:stream
  a owl:NamedIndividual, skos:Concept, odrl:Action ;
  odrl:includedIn odrl:use ;
  rdfs:isDefinedBy odrl: ;
  rdfs:label "Stream"@en ;
  skos:definition "To deliver the Asset in real-time."@en ;
  skos:note "The Asset maybe utilised in real-time as it is being delivered. If the action is to be performed to a wider audience than just the Assignees, then the Recipient constraint is recommended to be used." ;
  skos:scopeNote "Non-Normative"@en .

<https://w3id.org/dpv/owl#ConformanceAssessment>
  a owl:Class, owl:NamedIndividual, <https://w3id.org/dpv/owl#OrganisationalMeasure> ;
  rdfs:subClassOf <https://w3id.org/dpv/owl#Assessment> ;
  dc:contributor _:genid4, _:genid1 ;
  dc:created "2024-04-14"^^xsd:date ;
  ns1:term_status "accepted"@en ;
  skos:definition "Assessment regarding conformance with standards or norms or guidelines or similar instruments"@en ;
  skos:prefLabel "Conformance Assessment"@en ;
  owl:sameAs <https://w3id.org/dpv#ConformanceAssessment>, <https://w3id.org/dpv/dpv-owl#ConformanceAssessment> .

<https://w3id.org/dpv/owl#CombatClimateChange>
  a owl:Class, owl:NamedIndividual, <https://w3id.org/dpv/owl#Purpose> ;
  rdfs:subClassOf <https://w3id.org/dpv/owl#PublicBenefit> ;
  dc:contributor _:genid5, _:genid1 ;
  dc:created "2024-02-14"^^xsd:date ;
  dc:source "DGA 2.16"@en ;
  ns1:term_status "accepted"@en ;
  skos:definition "Purposes associated with combating the causes and consequences of climate change, including reducing gas emissions and fighting emergencies such as floods or wildfires"@en ;
  skos:prefLabel "Combat Climate Change"@en ;
  owl:sameAs <https://w3id.org/dpv#CombatClimateChange>, <https://w3id.org/dpv/dpv-owl#CombatClimateChange> .

<https://w3id.org/dpv/owl#CustomerOrderManagement>
  a owl:Class, owl:NamedIndividual, <https://w3id.org/dpv/owl#Purpose> ;
  rdfs:subClassOf <https://w3id.org/dpv/owl#CustomerManagement> ;
  dc:contributor _:genid4, _:genid5, _:genid1 ;
  dc:created "2021-09-08"^^xsd:date ;
  dc:source [
    a ns0:WebPage ;
    ns0:name "Belgian DPA ROPA Template" ;
    ns0:url "https://www.privacycommission.be/nl/model-voor-een-register-van-de-verwerkingsactiviteiten"
  ] ;
  ns1:term_status "accepted"@en ;
  skos:definition "Customer Order Management refers to purposes associated with managing customer orders i.e. processing of an order related to customer's purchase of good or services"@en ;
  skos:prefLabel "Customer Order Management"@en ;
  owl:sameAs <https://w3id.org/dpv#CustomerOrderManagement>, <https://w3id.org/dpv/dpv-owl#CustomerOrderManagement> .

<https://w3id.org/dpv/owl#serialisation-html>
  a owl:NamedIndividual, ns4:ResourceDescriptor ;
  dc:format <https://www.iana.org/assignments/media-types/text/html> ;
  dc:conformsTo <https://www.w3.org/TR/html/> ;
  dc:title "Data Privacy Vocabulary (DPV) - HTML serialiation" ;
  ns4:hasArtifact <https://w3id.org/dpv/dpv-owl.html> ;
  ns4:hasRole <http://www.w3.org/ns/dx/prof/role/specification> ;
  owl:sameAs <https://w3id.org/dpv#serialisation-html>, <https://w3id.org/dpv/dpv-owl#serialisation-html> .

ns4:ResourceDescriptor a owl:Class .
<https://w3id.org/dpv/owl#isIndicatedAtTime>
  a owl:ObjectProperty ;
  dc:contributor _:genid4, _:genid1, _:genid17, _:genid6 ;
  dc:created "2022-06-21"^^xsd:date ;
  ns1:term_status "accepted"@en ;
  skos:definition "Specifies the temporal information for when the entity has indicated the specific context"@en ;
  skos:prefLabel "is indicated at time"@en ;
  owl:sameAs <https://w3id.org/dpv#isIndicatedAtTime>, <https://w3id.org/dpv/dpv-owl#isIndicatedAtTime> .

<https://w3id.org/dpv/owl#IncorrectData>
  a owl:Class ;
  rdfs:subClassOf <https://w3id.org/dpv/owl#Data> ;
  dc:contributor _:genid1 ;
  dc:created "2022-11-02"^^xsd:date ;
  ns1:term_status "accepted"@en ;
  skos:definition "Data that is known to be incorrect or inconsistent with some requirements"@en ;
  skos:prefLabel "Incorrect Data"@en ;
  owl:sameAs <https://w3id.org/dpv#IncorrectData>, <https://w3id.org/dpv/dpv-owl#IncorrectData> .

odrl:permission
  a owl:ObjectProperty, owl:NamedIndividual, skos:Concept ;
  rdfs:domain odrl:Policy ;
  rdfs:range odrl:Permission ;
  rdfs:isDefinedBy odrl: ;
  rdfs:label "Has Permission"@en ;
  skos:definition "Relates an individual Permission to a Policy."@en .

odrl:Constraint
  a owl:Class, owl:NamedIndividual, skos:Concept ;
  rdfs:isDefinedBy odrl: ;
  rdfs:label "Constraint"@en ;
  skos:definition "A boolean expression that refines the semantics of an Action and Party/Asset Collection or declare the conditions applicable to a Rule."@en .

<https://w3id.org/dpv/owl#hasAddress>
  a owl:ObjectProperty ;
  ns2:domainIncludes <https://w3id.org/dpv/owl#Entity> ;
  dc:contributor _:genid4, _:genid5, _:genid1, _:genid6 ;
  dc:created "2020-11-04"^^xsd:date ;
  ns1:term_status "accepted"@en ;
  skos:definition "Specifies address of a legal entity such as street address or pin code"@en ;
  skos:prefLabel "has address"@en ;
  ns0:domainIncludes <https://w3id.org/dpv/owl#Entity> ;
  owl:sameAs <https://w3id.org/dpv#hasAddress>, <https://w3id.org/dpv/dpv-owl#hasAddress> .

odrl:isAllOf
  a owl:NamedIndividual, skos:Concept, odrl:Operator ;
  rdfs:isDefinedBy odrl: ;
  rdfs:label "Is all of"@en ;
  skos:definition "A set-based operator indicating that a given value is all of the right operand of the Constraint."@en .

<https://w3id.org/dpv/owl#StandardsConformance>
  a owl:Class, owl:NamedIndividual, <https://w3id.org/dpv/owl#OrganisationalMeasure> ;
  rdfs:subClassOf <https://w3id.org/dpv/owl#GovernanceProcedures> ;
  dc:contributor _:genid5, _:genid1 ;
  dc:created "2024-04-14"^^xsd:date ;
  dc:source "DGA 12.d"@en ;
  ns1:term_status "accepted"@en ;
  skos:definition "Purposes associated with activities undertaken to ensure or achieve conformance with standards"@en ;
  skos:prefLabel "Standards Conformance"@en ;
  owl:sameAs <https://w3id.org/dpv#StandardsConformance>, <https://w3id.org/dpv/dpv-owl#StandardsConformance> .

<https://w3id.org/dpv/owl#hasContact>
  a owl:ObjectProperty ;
  ns2:domainIncludes <https://w3id.org/dpv/owl#Entity> ;
  dc:contributor _:genid4, _:genid5, _:genid1, _:genid6 ;
  dc:created "2020-11-04"^^xsd:date ;
  ns1:term_status "accepted"@en ;
  skos:definition "Specifies contact details of a legal entity such as phone  or email"@en ;
  skos:prefLabel "has contact"@en ;
  ns0:domainIncludes <https://w3id.org/dpv/owl#Entity> ;
  owl:sameAs <https://w3id.org/dpv#hasContact>, <https://w3id.org/dpv/dpv-owl#hasContact> .

odrl:industry
  a owl:NamedIndividual, skos:Concept, odrl:LeftOperand ;
  rdfs:isDefinedBy odrl: ;
  rdfs:label "Industry Context"@en ;
  skos:definition "A defined industry sector setting a context for exercising the action of the Rule."@en ;
  skos:note "Example: publishing or financial industry."@en ;
  skos:scopeNote "Non-Normative"@en .

<https://w3id.org/dpv/owl#ContractExecutionStatus>
  a owl:Class ;
  rdfs:subClassOf <https://w3id.org/dpv/owl#ContractStatus> ;
  dc:contributor _:genid4, _:genid1, _:genid17 ;
  dc:created "2025-01-09"^^xsd:date ;
  ns1:term_status "accepted"@en ;
  skos:definition "Status associated with execution of a contract (i.e. signing and procedural aspects before the contract terms come in to effect)"@en ;
  skos:prefLabel "Contract Execution Status"@en ;
  owl:sameAs <https://w3id.org/dpv#ContractExecutionStatus>, <https://w3id.org/dpv/dpv-owl#ContractExecutionStatus> .

odrl:deliveryChannel
  a owl:NamedIndividual, skos:Concept, odrl:LeftOperand ;
  rdfs:isDefinedBy odrl: ;
  rdfs:label "Delivery Channel"@en ;
  skos:definition "The delivery channel used for exercising the action of the Rule."@en ;
  skos:note "Example: the asset may be distributed only on mobile networks."@en ;
  skos:scopeNote "Non-Normative"@en .

<https://w3id.org/dpv/owl#WithdrawConsent>
  a owl:Class ;
  rdfs:subClassOf <https://w3id.org/dpv/owl#ConsentControl>, <https://w3id.org/dpv/owl#WithdrawingFromProcess> ;
  dc:created "2024-05-11"^^xsd:date ;
  ns1:term_status "accepted"@en ;
  skos:definition "Control for withdrawing consent"@en ;
  skos:prefLabel "Withdraw Consent"@en ;
  skos:scopeNote "Indicates how the data subject can withdraw consent e.g. used with dpv:isExercisedAt"@en ;
  owl:sameAs <https://w3id.org/dpv#WithdrawConsent>, <https://w3id.org/dpv/dpv-owl#WithdrawConsent> .

odrl:recipient
  a owl:NamedIndividual, skos:Concept, odrl:LeftOperand ;
  rdfs:isDefinedBy odrl: ;
  rdfs:label "Recipient"@en ;
  skos:definition "The party receiving the result/outcome of exercising the action of the Rule."@en ;
  skos:note "The Right Operand must identify one or more specific Parties or category/ies of the Party."@en ;
  skos:scopeNote "Non-Normative"@en .

<https://w3id.org/dpv/owl#ConsequenceOfSuccess>
  a owl:Class ;
  rdfs:subClassOf <https://w3id.org/dpv/owl#Consequence> ;
  dc:contributor _:genid4, _:genid1 ;
  dc:created "2022-03-23"^^xsd:date ;
  ns1:term_status "accepted"@en ;
  skos:definition "The consequence(s) possible or arising from success of specified context"@en ;
  skos:prefLabel "Consequence of Success"@en ;
  owl:sameAs <https://w3id.org/dpv#ConsequenceOfSuccess>, <https://w3id.org/dpv/dpv-owl#ConsequenceOfSuccess> .

odrl:payAmount
  a owl:NamedIndividual, skos:Concept, odrl:LeftOperand ;
  rdfs:isDefinedBy odrl: ;
  rdfs:label "Payment Amount"@en ;
  skos:definition "The amount of a financial payment. Right operand value MUST be an xsd:decimal. "@en ;
  skos:note "Can be used for compensation duties with the unit property indicating the currency of the payment."@en ;
  skos:scopeNote "Non-Normative"@en .

<https://w3id.org/dpv/owl#ContractRenewed>
  a owl:Class, owl:NamedIndividual, <https://w3id.org/dpv/owl#ContractPerformanceStatus> ;
  rdfs:subClassOf <https://w3id.org/dpv/owl#ContractPerformanceStatus> ;
  dc:contributor _:genid4, _:genid1, _:genid17 ;
  dc:created "2025-01-09"^^xsd:date ;
  ns1:term_status "accepted"@en ;
  skos:definition "Status representing contract being renewed with new duration and/or applicability where the contract has been fully executed in the past"@en ;
  skos:prefLabel "Contract Renewed"@en ;
  owl:sameAs <https://w3id.org/dpv#ContractRenewed>, <https://w3id.org/dpv/dpv-owl#ContractRenewed> .

<https://w3id.org/dpv/owl#Pseudonymise>
  a owl:Class, owl:NamedIndividual, <https://w3id.org/dpv/owl#Processing> ;
  rdfs:subClassOf <https://w3id.org/dpv/owl#Transform> ;
  dc:created "2019-05-07"^^xsd:date ;
  dc:modified "2022-10-14"^^xsd:date ;
  dc:source [
    a ns0:WebPage ;
    ns0:name "GDPR Art.4-2" ;
    ns0:url "https://eur-lex.europa.eu/eli/reg/2016/679/art_4/par_2/oj"
  ] ;
  ns1:term_status "accepted"@en ;
  skos:definition "to replace personal identifiable information by artificial identifiers"@en ;
  skos:prefLabel "Pseudonymise Data"@en ;
  owl:sameAs <https://w3id.org/dpv#Pseudonymise>, <https://w3id.org/dpv/dpv-owl#Pseudonymise> .

<https://w3id.org/dpv/owl#UninformedConsent>
  a owl:Class, owl:NamedIndividual, <https://w3id.org/dpv/owl#LegalBasis> ;
  rdfs:subClassOf <https://w3id.org/dpv/owl#Consent> ;
  dc:contributor _:genid4, _:genid1, _:genid17, _:genid6 ;
  dc:created "2022-06-21"^^xsd:date ;
  ns1:term_status "accepted"@en ;
  skos:definition "Consent that is uninformed i.e. without requirement to provide sufficient information to make a consenting decision"@en ;
  skos:prefLabel "Uninformed Consent"@en ;
  owl:sameAs <https://w3id.org/dpv#UninformedConsent>, <https://w3id.org/dpv/dpv-owl#UninformedConsent> .

<https://w3id.org/dpv/owl#AuditNotRequired>
  a owl:Class, owl:NamedIndividual, <https://w3id.org/dpv/owl#AuditStatus> ;
  rdfs:subClassOf <https://w3id.org/dpv/owl#AuditStatus> ;
  dc:contributor _:genid1 ;
  dc:created "2022-05-18"^^xsd:date ;
  ns1:term_status "accepted"@en ;
  skos:definition "State where an audit is determined as not being required"@en ;
  skos:prefLabel "Audit Not Required"@en ;
  owl:sameAs <https://w3id.org/dpv#AuditNotRequired>, <https://w3id.org/dpv/dpv-owl#AuditNotRequired> .

odrl:#constraintRelationalOperators
  a owl:NamedIndividual, skos:Collection ;
  skos:member odrl:eq, odrl:gt, odrl:gteq, odrl:hasPart, odrl:isA, odrl:isAllOf, odrl:isAnyOf, odrl:isNoneOf, odrl:isPartOf, odrl:lt, odrl:lteq, odrl:neq ;
  skos:prefLabel "Constraint Operators"@en ;
  skos:scopeNote "ODRL Core Vocabulary Terms"@en .

<https://w3id.org/dpv/owl#ProviderStandardFormContract>
  a owl:Class, owl:NamedIndividual, <https://w3id.org/dpv/owl#LegalBasis> ;
  rdfs:subClassOf <https://w3id.org/dpv/owl#StandardFormContract> ;
  dc:created "2024-08-27"^^xsd:date ;
  ns1:term_status "accepted"@en ;
  skos:definition "A contract where the terms and conditions are determined by parties in the role of a 'provider', and the other parties have negligible or no ability to negotiate the terms and conditions"@en ;
  skos:prefLabel "Provider Standard Form Contract"@en ;
  owl:sameAs <https://w3id.org/dpv#ProviderStandardFormContract>, <https://w3id.org/dpv/dpv-owl#ProviderStandardFormContract> .

cc:Reproduction
  a owl:NamedIndividual, skos:Concept, odrl:Action ;
  odrl:includedIn odrl:use ;
  rdfs:isDefinedBy odrl: ;
  rdfs:label "Reproduction"@en ;
  skos:definition "Making multiple copies."@en ;
  skos:note "This term is defined by Creative Commons."@en ;
  skos:scopeNote "Non-Normative"@en .

<https://w3id.org/dpv/owl#TargetedAdvertising>
  a owl:Class, owl:NamedIndividual, <https://w3id.org/dpv/owl#Purpose> ;
  rdfs:subClassOf <https://w3id.org/dpv/owl#PersonalisedAdvertising> ;
  dc:contributor _:genid1 ;
  dc:created "2022-03-30"^^xsd:date ;
  ns1:term_status "accepted"@en ;
  skos:definition "Purposes associated with creating and providing personalised advertisement where the personalisation is targeted to a specific individual or group of individuals"@en ;
  skos:prefLabel "Targeted Advertising"@en ;
  owl:sameAs <https://w3id.org/dpv#TargetedAdvertising>, <https://w3id.org/dpv/dpv-owl#TargetedAdvertising> .

<https://w3id.org/dpv/owl#RecruitmentApplicationScreening>
  a owl:Class, owl:NamedIndividual, <https://w3id.org/dpv/owl#Purpose> ;
  rdfs:subClassOf <https://w3id.org/dpv/owl#RecruitmentApplicationManagement> ;
  dc:created "2024-12-01"^^xsd:date ;
  ns1:term_status "accepted"@en ;
  skos:definition "Purposes associated with screening and filtering of job applications or job candidates for recruitment"@en ;
  skos:prefLabel "Recruitment Application Screening"@en ;
  owl:sameAs <https://w3id.org/dpv#RecruitmentApplicationScreening>, <https://w3id.org/dpv/dpv-owl#RecruitmentApplicationScreening> .

<https://w3id.org/dpv/owl#InferredPersonalData>
  a owl:Class ;
  rdfs:subClassOf <https://w3id.org/dpv/owl#DerivedPersonalData>, <https://w3id.org/dpv/owl#InferredData> ;
  dc:contributor _:genid1 ;
  dc:created "2022-01-19"^^xsd:date ;
  dc:modified "2023-12-10"^^xsd:date ;
  ns3:example <https://w3id.org/dpv/examples/owl#E0009> ;
  ns1:term_status "accepted"@en ;
  skos:definition "Personal Data that is obtained through inference from other data"@en ;
  skos:prefLabel "Inferred Personal Data"@en ;
  skos:scopeNote "Inferred Data is derived data generated from existing data, but which did not originally exist within it, e.g. inferring demographics from browsing history."@en ;
  owl:sameAs <https://w3id.org/dpv#InferredPersonalData>, <https://w3id.org/dpv/dpv-owl#InferredPersonalData> .

<https://w3id.org/dpv/owl#PublicInterestOngoing>
  a owl:Class, owl:NamedIndividual, <https://w3id.org/dpv/owl#PublicInterestStatus> ;
  rdfs:subClassOf <https://w3id.org/dpv/owl#PublicInterestStatus> ;
  dc:created "2024-08-27"^^xsd:date ;
  ns1:term_status "accepted"@en ;
  skos:definition "Status where the public interest activity is ongoing"@en ;
  skos:prefLabel "Public Interest Ongoing"@en ;
  owl:sameAs <https://w3id.org/dpv#PublicInterestOngoing>, <https://w3id.org/dpv/dpv-owl#PublicInterestOngoing> .

<https://eu-upcast.github.io/vocabulary/index-en.html#hasCreationTime>
  a owl:DatatypeProperty ;
  rdfs:subPropertyOf owl:topDataProperty ;
  rdfs:domain odrl:Asset ;
  rdfs:range xsd:dateTime ;
  rdfs:comment "Used to restrict a collection of assets based on when they were created." ;
  rdfs:label "has creation time" .

<https://w3id.org/dpv/owl#hasNoticeIcon>
  a owl:ObjectProperty ;
  ns2:rangeIncludes <https://w3id.org/dpv/owl#NoticeIcon> ;
  dc:created "2024-08-17"^^xsd:date ;
  ns3:example <https://w3id.org/dpv/examples/owl#E0072> ;
  ns1:term_status "accepted"@en ;
  skos:definition "Indicates the concept can be represented graphically using the specified icon"@en ;
  skos:prefLabel "has notice icon"@en ;
  ns0:rangeIncludes <https://w3id.org/dpv/owl#NoticeIcon> ;
  owl:sameAs <https://w3id.org/dpv#hasNoticeIcon>, <https://w3id.org/dpv/dpv-owl#hasNoticeIcon> .

<https://w3id.org/dpv/owl#Monitor>
  a owl:Class, owl:NamedIndividual, <https://w3id.org/dpv/owl#Processing> ;
  rdfs:subClassOf <https://w3id.org/dpv/owl#Consult> ;
  dc:contributor _:genid4, _:genid1 ;
  dc:created "2022-06-15"^^xsd:date ;
  ns1:term_status "accepted"@en ;
  skos:definition "to monitor data for some criteria"@en ;
  skos:prefLabel "Monitor Data"@en ;
  owl:sameAs <https://w3id.org/dpv#Monitor>, <https://w3id.org/dpv/dpv-owl#Monitor> .

<https://w3id.org/dpv/owl#DataBreachNotification>
  a owl:Class, owl:NamedIndividual, <https://w3id.org/dpv/owl#OrganisationalMeasure> ;
  rdfs:subClassOf <https://w3id.org/dpv/owl#SecurityIncidentNotification> ;
  dc:contributor _:genid1 ;
  dc:created "2024-04-14"^^xsd:date ;
  dc:source " DGA 21.5 GDPR 33"@en, " GDPR 34"@en, "DGA 12.k"@en ;
  ns1:term_status "accepted"@en ;
  skos:definition "Notification of information about data breach(es) i.e. unauthorised transfer, access, use, or modification of data"@en ;
  skos:prefLabel "Data Breach Notification"@en ;
  owl:sameAs <https://w3id.org/dpv#DataBreachNotification>, <https://w3id.org/dpv/dpv-owl#DataBreachNotification> .

<https://w3id.org/dpv/owl#ContractualClausePartiallyFulfiled>
  a owl:Class, owl:NamedIndividual, <https://w3id.org/dpv/owl#ContractualClauseFulfilmentStatus> ;
  rdfs:subClassOf <https://w3id.org/dpv/owl#ContractualClauseFulfilmentStatus> ;
  dc:created "2024-08-27"^^xsd:date ;
  ns1:term_status "accepted"@en ;
  skos:definition "Status indicating some of the terms of the contractual clause have been fulfiled, and others have not yet been fulfiled in a manner that does not constitute a violation i.e. there is still an opportunity to complete them"@en ;
  skos:prefLabel "Contractual Clause Partially Fulfiled"@en ;
  owl:sameAs <https://w3id.org/dpv#ContractualClausePartiallyFulfiled>, <https://w3id.org/dpv/dpv-owl#ContractualClausePartiallyFulfiled> .

odrl:present
  a owl:NamedIndividual, skos:Concept, odrl:Action ;
  odrl:includedIn odrl:use ;
  rdfs:isDefinedBy odrl: ;
  rdfs:label "Present"@en ;
  skos:definition "To publicly perform the Asset."@en ;
  skos:note "The asset can be performed (or communicated) in public." ;
  skos:scopeNote "Non-Normative"@en .

<https://w3id.org/dpv/owl#hasData>
  a owl:ObjectProperty ;
  ns2:rangeIncludes <https://w3id.org/dpv/owl#Data> ;
  dc:contributor _:genid1 ;
  dc:created "2022-08-18"^^xsd:date ;
  ns1:term_status "accepted"@en ;
  skos:definition "Indicates associated with Data (may or may not be personal)"@en ;
  skos:prefLabel "has data"@en ;
  ns0:rangeIncludes <https://w3id.org/dpv/owl#Data> ;
  owl:sameAs <https://w3id.org/dpv#hasData>, <https://w3id.org/dpv/dpv-owl#hasData> .

<https://w3id.org/dpv/owl#LocalEnvironmentScale>
  a owl:Class, owl:NamedIndividual, <https://w3id.org/dpv/owl#GeographicCoverage> ;
  rdfs:subClassOf <https://w3id.org/dpv/owl#GeographicCoverage> ;
  dc:contributor _:genid1 ;
  dc:created "2022-06-15"^^xsd:date ;
  ns1:term_status "accepted"@en ;
  skos:definition "Geographic coverage spanning a specific environment within the locality"@en ;
  skos:prefLabel "Local Environment Scale"@en ;
  skos:scopeNote "For example, geographic scale of an event take place in a specific building or room"@en ;
  owl:sameAs <https://w3id.org/dpv#LocalEnvironmentScale>, <https://w3id.org/dpv/dpv-owl#LocalEnvironmentScale> .

<https://w3id.org/dpv/owl#FeeRequired>
  a owl:Class ;
  rdfs:subClassOf <https://w3id.org/dpv/owl#FeeRequirement> ;
  dc:created "2024-08-27"^^xsd:date ;
  ns1:term_status "accepted"@en ;
  skos:definition "Concept indicating a fee is required. The value of the fee should be specified using rdf:value or an another relevant means"@en ;
  skos:prefLabel "Fee Required"@en ;
  owl:sameAs <https://w3id.org/dpv#FeeRequired>, <https://w3id.org/dpv/dpv-owl#FeeRequired> .

<https://w3id.org/dpv/owl#VendorManagement>
  a owl:Class, owl:NamedIndividual, <https://w3id.org/dpv/owl#Purpose> ;
  rdfs:subClassOf <https://w3id.org/dpv/owl#Purpose> ;
  dc:contributor _:genid4, _:genid1, _:genid6, _:genid21 ;
  dc:created "2021-09-01"^^xsd:date ;
  dc:source [
    a ns0:WebPage ;
    ns0:name "Belgian DPA ROPA Template" ;
    ns0:url "https://www.privacycommission.be/nl/model-voor-een-register-van-de-verwerkingsactiviteiten"
  ] ;
  ns1:term_status "accepted"@en ;
  skos:definition "Purposes associated with manage orders, payment, evaluation, and prospecting related to vendors"@en ;
  skos:prefLabel "Vendor Management"@en ;
  owl:sameAs <https://w3id.org/dpv#VendorManagement>, <https://w3id.org/dpv/dpv-owl#VendorManagement> .

<https://w3id.org/dpv/owl#EconomicUnion>
  a owl:Class ;
  rdfs:subClassOf <https://w3id.org/dpv/owl#Location> ;
  dc:contributor _:genid1 ;
  dc:created "2022-01-19"^^xsd:date ;
  ns1:term_status "accepted"@en ;
  skos:definition "A political union of two or more countries based on economic or trade agreements"@en ;
  skos:prefLabel "Economic Union"@en ;
  owl:sameAs <https://w3id.org/dpv#EconomicUnion>, <https://w3id.org/dpv/dpv-owl#EconomicUnion> .

odrl:#assetConcepts
  a owl:NamedIndividual, skos:Collection ;
  skos:member odrl:Asset, odrl:AssetCollection ;
  skos:prefLabel "Asset"@en ;
  skos:scopeNote "ODRL Core Vocabulary Terms"@en .

<https://w3id.org/dpv/owl#hasResponsibleEntity>
  a owl:ObjectProperty ;
  rdfs:subPropertyOf <https://w3id.org/dpv/owl#hasEntity> ;
  ns2:rangeIncludes <https://w3id.org/dpv/owl#Entity> ;
  dc:contributor _:genid1 ;
  dc:created "2022-03-02"^^xsd:date ;
  ns1:term_status "accepted"@en ;
  skos:definition "Specifies the indicated entity is responsible within some context"@en ;
  skos:prefLabel "has responsible entity"@en ;
  ns0:rangeIncludes <https://w3id.org/dpv/owl#Entity> ;
  owl:sameAs <https://w3id.org/dpv#hasResponsibleEntity>, <https://w3id.org/dpv/dpv-owl#hasResponsibleEntity> .

<https://w3id.org/dpv/owl#VitalInterestStatus>
  a owl:Class ;
  rdfs:subClassOf <https://w3id.org/dpv/owl#Status> ;
  dc:created "2024-08-27"^^xsd:date ;
  ns3:example <https://w3id.org/dpv/examples/owl#E0083> ;
  ns1:term_status "accepted"@en ;
  skos:definition "Status associated with use of Vital Interest as a legal basis"@en ;
  skos:prefLabel "Vital Interest Status"@en ;
  owl:sameAs <https://w3id.org/dpv#VitalInterestStatus>, <https://w3id.org/dpv/dpv-owl#VitalInterestStatus> .

<https://w3id.org/dpv/owl#CounterMoneyLaundering>
  a owl:Class, owl:NamedIndividual, <https://w3id.org/dpv/owl#Purpose> ;
  rdfs:subClassOf <https://w3id.org/dpv/owl#FraudPreventionAndDetection> ;
  dc:contributor _:genid1 ;
  dc:created "2022-04-20"^^xsd:date ;
  ns1:term_status "accepted"@en ;
  skos:definition "Purposes associated with detection, prevention, and mitigation of mitigate money laundering"@en ;
  skos:prefLabel "Counter Money Laundering"@en ;
  owl:sameAs <https://w3id.org/dpv#CounterMoneyLaundering>, <https://w3id.org/dpv/dpv-owl#CounterMoneyLaundering> .

<https://w3id.org/dpv/owl#LegitimateInterestStatus>
  a owl:Class ;
  rdfs:subClassOf <https://w3id.org/dpv/owl#Status> ;
  dc:created "2024-08-27"^^xsd:date ;
  ns3:example <https://w3id.org/dpv/examples/owl#E0080> ;
  ns1:term_status "accepted"@en ;
  skos:definition "Status associated with use of Legitimate Interest as a legal basis"@en ;
  skos:prefLabel "Legitimate InterestStatus"@en ;
  owl:sameAs <https://w3id.org/dpv#LegitimateInterestStatus>, <https://w3id.org/dpv/dpv-owl#LegitimateInterestStatus> .

<https://w3id.org/dpv/owl#RecruitmentApplicantCriminalBackgroundCheck>
  a owl:Class, owl:NamedIndividual, <https://w3id.org/dpv/owl#Purpose> ;
  rdfs:subClassOf <https://w3id.org/dpv/owl#RecruitmentManagement> ;
  dc:created "2024-12-01"^^xsd:date ;
  ns1:term_status "accepted"@en ;
  skos:definition "Purposes associated with conducting criminal background assessment for prospective and current job applicants for recruitment"@en ;
  skos:prefLabel "Recruitment Applicant Criminal Background Check"@en ;
  owl:sameAs <https://w3id.org/dpv#RecruitmentApplicantCriminalBackgroundCheck>, <https://w3id.org/dpv/dpv-owl#RecruitmentApplicantCriminalBackgroundCheck> .

<https://w3id.org/dpv/owl#hasPurpose>
  a owl:ObjectProperty ;
  ns2:rangeIncludes <https://w3id.org/dpv/owl#Purpose> ;
  dc:contributor _:genid13, _:genid9, _:genid31, _:genid1, _:genid11 ;
  dc:created "2019-04-04"^^xsd:date ;
  dc:modified "2020-11-04"^^xsd:date ;
  dc:source [
    a ns0:WebPage ;
    ns0:name "SPECIAL Project" ;
    ns0:url "https://specialprivacy.ercim.eu/"
  ] ;
  ns1:term_status "accepted"@en ;
  skos:definition "Indicates association with Purpose"@en ;
  skos:prefLabel "has purpose"@en ;
  ns0:rangeIncludes <https://w3id.org/dpv/owl#Purpose> ;
  owl:sameAs <https://w3id.org/dpv#hasPurpose>, <https://w3id.org/dpv/dpv-owl#hasPurpose> .

odrl:virtualLocation
  a owl:NamedIndividual, skos:Concept, odrl:LeftOperand ;
  rdfs:isDefinedBy odrl: ;
  rdfs:label "Virtual IT Communication Location"@en ;
  skos:definition "An identified location of the IT communication space which is relevant for exercising the action of the Rule."@en ;
  skos:note "Example: an Internet domain or IP address range."@en ;
  skos:scopeNote "Non-Normative"@en .

<https://w3id.org/dpv/owl#Data>
  a owl:Class ;
  rdfs:subClassOf odrl:Asset ;
  dc:contributor _:genid1 ;
  dc:created "2022-01-19"^^xsd:date ;
  ns1:term_status "accepted"@en ;
  skos:definition "A broad concept representing  'data' or 'information'"@en ;
  skos:prefLabel "Data"@en ;
  owl:sameAs <https://w3id.org/dpv#Data>, <https://w3id.org/dpv/dpv-owl#Data> .

odrl:absoluteTemporalPosition
  a owl:NamedIndividual, skos:Concept, odrl:LeftOperand ;
  rdfs:isDefinedBy odrl: ;
  rdfs:label "Absolute Temporal Asset Position"@en ;
  skos:broaderTransitive odrl:absolutePosition ;
  skos:definition "The absolute temporal positions in a media stream the target Asset has to fit."@en ;
  skos:note "Use with Actions including the target Asset in a larger media stream. The fragment part of a Media Fragment URI (https://www.w3.org/TR/media-frags/) may be used for the right operand. See the Left Operand realativeTemporalPosition. <br />Example: The MP3 music file must be positioned between second 192 and 250 of the temporal length of a stream."@en ;
  skos:scopeNote "Non-Normative"@en .

<https://w3id.org/dpv/owl#SupraNationalAuthority>
  a owl:Class ;
  rdfs:subClassOf <https://w3id.org/dpv/owl#Authority> ;
  dc:contributor _:genid1 ;
  dc:created "2022-02-02"^^xsd:date ;
  dc:source [
    a ns0:WebPage ;
    ns0:name "ADMS controlled vocabulary" ;
    ns0:url "http://purl.org/adms"
  ] ;
  ns1:term_status "accepted"@en ;
  skos:definition "An authority tasked with overseeing legal compliance for a supra-national union e.g. EU"@en ;
  skos:prefLabel "Supranational Authority"@en ;
  owl:sameAs <https://w3id.org/dpv#SupraNationalAuthority>, <https://w3id.org/dpv/dpv-owl#SupraNationalAuthority> .

<https://w3id.org/dpv/owl#DashboardNotice>
  a owl:Class, owl:NamedIndividual, <https://w3id.org/dpv/owl#OrganisationalMeasure> ;
  rdfs:subClassOf <https://w3id.org/dpv/owl#Notice> ;
  dc:created "2024-08-17"^^xsd:date ;
  dc:source [
    a ns0:WebPage ;
    ns0:name "ICO - What methods can we use to provide privacy information?" ;
    ns0:url "https://ico.org.uk/for-organisations/uk-gdpr-guidance-and-resources/individual-rights/the-right-to-be-informed/what-methods-can-we-use-to-provide-privacy-information/"
  ] ;
  ns1:term_status "accepted"@en ;
  skos:definition "A notice that is provided within a dashboard also used for other purposes"@en ;
  skos:prefLabel "Dashboard Notice"@en ;
  owl:sameAs <https://w3id.org/dpv#DashboardNotice>, <https://w3id.org/dpv/dpv-owl#DashboardNotice> .

<https://w3id.org/dpv/owl#ContractPerformance>
  a owl:Class, owl:NamedIndividual, <https://w3id.org/dpv/owl#LegalBasis> ;
  rdfs:subClassOf <https://w3id.org/dpv/owl#Contract> ;
  dc:contributor _:genid4, _:genid1, _:genid6 ;
  dc:created "2021-04-07"^^xsd:date ;
  ns1:term_status "accepted"@en ;
  skos:definition "Fulfilment or performance of a contract involving specified processing of data or technologies"@en ;
  skos:prefLabel "Contract Performance"@en ;
  owl:sameAs <https://w3id.org/dpv#ContractPerformance>, <https://w3id.org/dpv/dpv-owl#ContractPerformance> .

<https://w3id.org/dpv/owl#ComplianceIndeterminate>
  a owl:Class, owl:NamedIndividual, <https://w3id.org/dpv/owl#ComplianceStatus> ;
  rdfs:subClassOf <https://w3id.org/dpv/owl#ComplianceStatus> ;
  dc:contributor _:genid1 ;
  dc:created "2022-09-07"^^xsd:date ;
  ns1:term_status "accepted"@en ;
  skos:definition "State where the status of compliance has not been fully assessed, evaluated, or determined"@en ;
  skos:prefLabel "Compliance Indeterminate"@en ;
  owl:sameAs <https://w3id.org/dpv#ComplianceIndeterminate>, <https://w3id.org/dpv/dpv-owl#ComplianceIndeterminate> .

<https://w3id.org/dpv/owl#hasConformanceStatus>
  a owl:ObjectProperty ;
  ns2:rangeIncludes <https://w3id.org/dpv/owl#ConformanceStatus> ;
  dc:contributor _:genid1 ;
  dc:created "2024-06-10"^^xsd:date ;
  ns1:term_status "accepted"@en ;
  skos:definition "Indicates the status of being conformant or non-conformant"@en ;
  skos:prefLabel "has conformance status"@en ;
  ns0:rangeIncludes <https://w3id.org/dpv/owl#ConformanceStatus> ;
  owl:sameAs <https://w3id.org/dpv#hasConformanceStatus>, <https://w3id.org/dpv/dpv-owl#hasConformanceStatus> .

<https://w3id.org/dpv/owl#PersonalDataAudit>
  a owl:Class, owl:NamedIndividual, <https://w3id.org/dpv/owl#OrganisationalMeasure> ;
  rdfs:subClassOf <https://w3id.org/dpv/owl#InformationAudit> ;
  dc:contributor _:genid1, _:genid6 ;
  dc:created "2024-12-17"^^xsd:date ;
  ns1:term_status "accepted"@en ;
  skos:definition "An audit that systematically examines the existence and use of personal data along with its associated resources (e.g. where it is stored) and flows (e.g. where it originates and with whom it is being shared)"@en ;
  skos:prefLabel "Personal Data Audit"@en ;
  skos:scopeNote "This concept is the same as \"Data Mapping\" and \"Data Flow Mapping Exercise\" used by the Information Comissioner's Office as \"to document the data that flows in, around, and out of information processing systems or services\""@en ;
  owl:sameAs <https://w3id.org/dpv#PersonalDataAudit>, <https://w3id.org/dpv/dpv-owl#PersonalDataAudit> .

odrl:profile
  a owl:AnnotationProperty, owl:NamedIndividual, skos:Concept ;
  rdfs:domain odrl:Policy ;
  rdfs:isDefinedBy odrl: ;
  rdfs:label "Profile"@en ;
  skos:definition "The identifier(s) of an ODRL Profile that the Policy conforms to."@en ;
  skos:note "The profile property is mandatory if the Policy is using an ODRL Profile."@en .

<https://w3id.org/dpv/owl#TechnicalOrganisationalMeasure>
  a owl:Class ;
  dc:contributor _:genid31 ;
  dc:created "2019-04-05"^^xsd:date ;
  dc:modified "2023-12-10"^^xsd:date ;
  ns1:term_status "accepted"@en ;
  skos:definition "Technical and Organisational measures used to safeguard and ensure good practices in connection with data and technologies"@en ;
  skos:prefLabel "Technical and Organisational Measure"@en ;
  owl:sameAs <https://w3id.org/dpv#TechnicalOrganisationalMeasure>, <https://w3id.org/dpv/dpv-owl#TechnicalOrganisationalMeasure> .

<https://w3id.org/dpv/owl#NDA>
  a owl:Class, owl:NamedIndividual, <https://w3id.org/dpv/owl#LegalMeasure> ;
  rdfs:subClassOf <https://w3id.org/dpv/owl#LegalAgreement> ;
  dc:contributor _:genid9, _:genid10, _:genid1, _:genid11 ;
  dc:created "2019-04-05"^^xsd:date ;
  dc:modified "2024-08-27"^^xsd:date ;
  ns1:term_status "accepted"@en ;
  skos:definition "Non-disclosure Agreements e.g. preserving confidentiality of information"@en ;
  skos:prefLabel "Non-Disclosure Agreement (NDA)"@en ;
  owl:sameAs <https://w3id.org/dpv#NDA>, <https://w3id.org/dpv/dpv-owl#NDA> .

odrl:AssetScope a owl:Class, owl:NamedIndividual, skos:Concept .
<https://w3id.org/dpv/owl#Tourist>
  a owl:Class, owl:NamedIndividual, <https://w3id.org/dpv/owl#HumanSubject> ;
  rdfs:subClassOf <https://w3id.org/dpv/owl#HumanSubject> ;
  dc:contributor _:genid4, _:genid5, _:genid1, _:genid17, _:genid6 ;
  dc:created "2022-04-06"^^xsd:date ;
  dc:modified "2024-12-17"^^xsd:date ;
  ns1:term_status "modified"@en ;
  skos:definition "Humans that are tourists i.e. not citizens and not immigrants"@en ;
  skos:prefLabel "Tourist"@en ;
  owl:sameAs <https://w3id.org/dpv#Tourist>, <https://w3id.org/dpv/dpv-owl#Tourist> .

<https://w3id.org/dpv/owl#hasPassiveEntity>
  a owl:ObjectProperty ;
  rdfs:subPropertyOf <https://w3id.org/dpv/owl#hasEntity> ;
  ns2:rangeIncludes <https://w3id.org/dpv/owl#Entity> ;
  dc:created "2024-05-11"^^xsd:date ;
  ns1:term_status "accepted"@en ;
  skos:definition "indicates the entity is passively involved in specified context"@en ;
  skos:prefLabel "has passive entity"@en ;
  ns0:rangeIncludes <https://w3id.org/dpv/owl#Entity> ;
  owl:sameAs <https://w3id.org/dpv#hasPassiveEntity>, <https://w3id.org/dpv/dpv-owl#hasPassiveEntity> .

<https://w3id.org/dpv/owl#TechnicalMeasure>
  a owl:Class ;
  rdfs:subClassOf <https://w3id.org/dpv/owl#TechnicalOrganisationalMeasure> ;
  dc:contributor _:genid9, _:genid10, _:genid1, _:genid11 ;
  dc:created "2019-04-05"^^xsd:date ;
  dc:modified "2023-12-10"^^xsd:date ;
  ns3:example <https://w3id.org/dpv/examples/owl#E0020>, <https://w3id.org/dpv/examples/owl#E0064> ;
  ns1:term_status "accepted"@en ;
  skos:definition "Technical measures used to safeguard and ensure good practices in connection with data and technologies"@en ;
  skos:prefLabel "Technical Measure"@en ;
  owl:sameAs <https://w3id.org/dpv#TechnicalMeasure>, <https://w3id.org/dpv/dpv-owl#TechnicalMeasure> .

<https://w3id.org/dpv/owl#SecurityIncidentNotice>
  a owl:Class, owl:NamedIndividual, <https://w3id.org/dpv/owl#OrganisationalMeasure> ;
  rdfs:subClassOf <https://w3id.org/dpv/owl#Notice> ;
  dc:contributor _:genid1 ;
  dc:created "2024-04-14"^^xsd:date ;
  ns1:term_status "accepted"@en ;
  skos:definition "A notice providing information about security incident(s)"@en ;
  skos:prefLabel "Security Incident Notice"@en ;
  owl:sameAs <https://w3id.org/dpv#SecurityIncidentNotice>, <https://w3id.org/dpv/dpv-owl#SecurityIncidentNotice> .

<https://w3id.org/dpv/owl#isExercisedAt>
  a owl:ObjectProperty ;
  ns2:domainIncludes <https://w3id.org/dpv/owl#ActiveRight> ;
  ns2:rangeIncludes <https://w3id.org/dpv/owl#RightExerciseNotice> ;
  dc:contributor _:genid1 ;
  dc:created "2022-10-22"^^xsd:date ;
  ns1:term_status "accepted"@en ;
  skos:definition "Indicates context or information about exercising a right"@en ;
  skos:prefLabel "is exercised at"@en ;
  ns0:domainIncludes <https://w3id.org/dpv/owl#ActiveRight> ;
  ns0:rangeIncludes <https://w3id.org/dpv/owl#RightExerciseNotice> ;
  owl:sameAs <https://w3id.org/dpv#isExercisedAt>, <https://w3id.org/dpv/dpv-owl#isExercisedAt> .

<https://w3id.org/dpv/owl#DisputeManagement>
  a owl:Class, owl:NamedIndividual, <https://w3id.org/dpv/owl#Purpose> ;
  rdfs:subClassOf <https://w3id.org/dpv/owl#OrganisationGovernance> ;
  dc:contributor _:genid4, _:genid5, _:genid1 ;
  dc:created "2021-09-08"^^xsd:date ;
  dc:source [
    a ns0:WebPage ;
    ns0:name "Belgian DPA ROPA Template" ;
    ns0:url "https://www.privacycommission.be/nl/model-voor-een-register-van-de-verwerkingsactiviteiten"
  ] ;
  ns1:term_status "accepted"@en ;
  skos:definition "Purposes associated with activities that manage disputes by natural persons, private bodies, or public authorities relevant to organisation"@en ;
  skos:prefLabel "Dispute Management"@en ;
  owl:sameAs <https://w3id.org/dpv#DisputeManagement>, <https://w3id.org/dpv/dpv-owl#DisputeManagement> .

<https://w3id.org/dpv/owl#StorageDuration>
  a owl:Class ;
  rdfs:subClassOf <https://w3id.org/dpv/owl#ProcessingDuration>, <https://w3id.org/dpv/owl#StorageCondition> ;
  dc:contributor _:genid9, _:genid10, _:genid1, _:genid11 ;
  dc:created "2019-04-05"^^xsd:date ;
  ns3:example <https://w3id.org/dpv/examples/owl#E0048> ;
  ns1:term_status "accepted"@en ;
  skos:definition "Duration or temporal limitation on storage of data"@en ;
  skos:prefLabel "Storage Duration"@en ;
  owl:sameAs <https://w3id.org/dpv#StorageDuration>, <https://w3id.org/dpv/dpv-owl#StorageDuration> .

odrl:spatialCoordinates
  a owl:NamedIndividual, skos:Concept, odrl:LeftOperand ;
  rdfs:isDefinedBy odrl: ;
  rdfs:label "Geospatial Coordinates"@en ;
  skos:broaderTransitive odrl:spatial ;
  skos:definition "A set of coordinates setting the borders of a geospatial area used for exercising the action of the Rule. The coordinates MUST include longitude and latitude, they MAY include altitude and the geodetic datum."@en ;
  skos:note "The default values are the altitude of earth's surface at this location and the WGS 84 datum."@en ;
  skos:scopeNote "Non-Normative"@en .

<https://w3id.org/dpv/owl#BackgroundChecks>
  a owl:Class, owl:NamedIndividual, <https://w3id.org/dpv/owl#OrganisationalMeasure> ;
  rdfs:subClassOf <https://w3id.org/dpv/owl#SecurityProcedure> ;
  dc:contributor _:genid1 ;
  dc:created "2022-08-17"^^xsd:date ;
  dc:source [
    a ns0:WebPage ;
    ns0:name "ENISA 5G Cybersecurity Standards" ;
    ns0:url "https://www.enisa.europa.eu/publications/5g-cybersecurity-standards"
  ] ;
  ns1:term_status "accepted"@en ;
  skos:definition "Procedure where the background of an entity is assessed to identity vulnerabilities and threats due to their current or intended role"@en ;
  skos:prefLabel "Background Checks"@en ;
  owl:sameAs <https://w3id.org/dpv#BackgroundChecks>, <https://w3id.org/dpv/dpv-owl#BackgroundChecks> .

<https://w3id.org/dpv/owl#hasNoticeStatus>
  a owl:ObjectProperty ;
  ns2:domainIncludes <https://w3id.org/dpv/owl#Notice> ;
  ns2:rangeIncludes <https://w3id.org/dpv/owl#NoticeStatus> ;
  dc:contributor _:genid4, _:genid1 ;
  dc:created "2024-12-01"^^xsd:date ;
  ns3:example <https://w3id.org/dpv/examples/owl#E0073> ;
  ns1:term_status "accepted"@en ;
  skos:definition "Indicates the status of the associated notice"@en ;
  skos:prefLabel "has notice status"@en ;
  ns0:domainIncludes <https://w3id.org/dpv/owl#Notice> ;
  ns0:rangeIncludes <https://w3id.org/dpv/owl#NoticeStatus> ;
  owl:sameAs <https://w3id.org/dpv#hasNoticeStatus>, <https://w3id.org/dpv/dpv-owl#hasNoticeStatus> .

<https://w3id.org/dpv/owl#DocumentRandomisedPseudonymisation>
  a owl:Class, owl:NamedIndividual, <https://w3id.org/dpv/owl#TechnicalMeasure> ;
  rdfs:subClassOf <https://w3id.org/dpv/owl#Pseudonymisation> ;
  dc:contributor _:genid1 ;
  dc:created "2022-08-17"^^xsd:date ;
  dc:source [
    a ns0:WebPage ;
    ns0:name "ENISA Data Pseudonymisation: Advanced Techniques and Use Cases" ;
    ns0:url "https://www.enisa.europa.eu/publications/data-pseudonymisation-advanced-techniques-and-use-cases"
  ] ;
  ns1:term_status "accepted"@en ;
  skos:definition "Use of randomised pseudonymisation where the same elements are assigned different values in the same document or database"@en ;
  skos:prefLabel "Document Randomised Pseudonymisation"@en ;
  owl:sameAs <https://w3id.org/dpv#DocumentRandomisedPseudonymisation>, <https://w3id.org/dpv/dpv-owl#DocumentRandomisedPseudonymisation> .

<https://w3id.org/dpv/owl#hasContractualClause>
  a owl:ObjectProperty ;
  ns2:domainIncludes <https://w3id.org/dpv/owl#Contract>, <https://w3id.org/dpv/owl#ContractualClause> ;
  ns2:rangeIncludes <https://w3id.org/dpv/owl#ContractualClause> ;
  dc:created "2024-12-17"^^xsd:date ;
  ns3:example <https://w3id.org/dpv/examples/owl#E0078> ;
  ns1:term_status "accepted"@en ;
  skos:definition "Indicates the association or involvement of specified contractual clause"@en ;
  skos:prefLabel "has contractual clause"@en ;
  ns0:domainIncludes <https://w3id.org/dpv/owl#Contract>, <https://w3id.org/dpv/owl#ContractualClause> ;
  ns0:rangeIncludes <https://w3id.org/dpv/owl#ContractualClause> ;
  owl:sameAs <https://w3id.org/dpv#hasContractualClause>, <https://w3id.org/dpv/dpv-owl#hasContractualClause> .

vcard:Agent a owl:Class .
<https://w3id.org/dpv/owl#SyntheticData>
  a owl:Class ;
  rdfs:subClassOf <https://w3id.org/dpv/owl#GeneratedData> ;
  dc:contributor _:genid1 ;
  dc:created "2022-08-18"^^xsd:date ;
  dc:modified "2023-12-10"^^xsd:date ;
  dc:source [
    a ns0:WebPage ;
    ns0:name "ENISA Data Protection Engineering" ;
    ns0:url "https://www.enisa.europa.eu/publications/data-protection-engineering"
  ] ;
  ns1:term_status "accepted"@en ;
  skos:definition "Synthetic data refers to artificially created data such that it is intended to resemble real data (personal or non-personal), but does not refer to any specific identified or identifiable individual, or to the real measure of an observable parameter in the case of non-personal data"@en ;
  skos:prefLabel "Synthetic Data"@en ;
  owl:sameAs <https://w3id.org/dpv#SyntheticData>, <https://w3id.org/dpv/dpv-owl#SyntheticData> .

<https://w3id.org/dpv/owl#MessageAuthenticationCodes>
  a owl:Class, owl:NamedIndividual, <https://w3id.org/dpv/owl#TechnicalMeasure> ;
  rdfs:subClassOf <https://w3id.org/dpv/owl#CryptographicAuthentication> ;
  dc:contributor _:genid1 ;
  dc:created "2022-08-17"^^xsd:date ;
  dc:source [
    a ns0:WebPage ;
    ns0:name "ENISA Reference Incident Classification Taxonomy 2018" ;
    ns0:url "https://www.enisa.europa.eu/publications/reference-incident-classification-taxonomy/"
  ] ;
  ns1:term_status "accepted"@en ;
  skos:definition "Use of cryptographic methods to authenticate messages"@en ;
  skos:prefLabel "Message Authentication Codes (MAC)"@en ;
  owl:sameAs <https://w3id.org/dpv#MessageAuthenticationCodes>, <https://w3id.org/dpv/dpv-owl#MessageAuthenticationCodes> .

<https://w3id.org/dpv/owl#ElderlyDataSubject>
  a owl:Class, owl:NamedIndividual, <https://w3id.org/dpv/owl#HumanSubject> ;
  rdfs:subClassOf <https://w3id.org/dpv/owl#VulnerableDataSubject> ;
  dc:contributor _:genid4 ;
  dc:created "2022-06-15"^^xsd:date ;
  dc:modified "2024-12-17"^^xsd:date ;
  ns1:term_status "modified"@en ;
  skos:definition "Data subjects that are considered elderly (i.e. based on age)"@en ;
  skos:prefLabel "Elderly Data Subject"@en ;
  owl:sameAs <https://w3id.org/dpv#ElderlyDataSubject>, <https://w3id.org/dpv/dpv-owl#ElderlyDataSubject> .

vcard:Organization a owl:Class .
<https://w3id.org/dpv/owl#ConsentStatus>
  a owl:Class ;
  rdfs:subClassOf <https://w3id.org/dpv/owl#Status> ;
  dc:contributor _:genid4, _:genid1, _:genid17, _:genid6 ;
  dc:created "2022-06-22"^^xsd:date ;
  dc:source [
    a ns0:WebPage ;
    ns0:name "GConsent" ;
    ns0:url "https://w3id.org/GConsent"
  ] ;
  ns1:term_status "accepted"@en ;
  skos:definition "The state or status of 'consent' that provides information reflecting its operational status and validity for processing data"@en ;
  skos:prefLabel "Consent Status"@en ;
  skos:scopeNote "States are useful as information artefacts to implement them in controlling processing, and to reflect the process and flow of obtaining and maintaining consent. For example, a database table that stores consent states for specific processing and can be queried to obtain them in an efficient manner. States are also useful in investigations to determine the use and validity of consenting practices"@en ;
  owl:sameAs <https://w3id.org/dpv#ConsentStatus>, <https://w3id.org/dpv/dpv-owl#ConsentStatus> .

<https://w3id.org/dpv/owl#SmallDataVolume>
  a owl:Class, owl:NamedIndividual, <https://w3id.org/dpv/owl#DataVolume> ;
  rdfs:subClassOf <https://w3id.org/dpv/owl#DataVolume> ;
  dc:contributor _:genid1 ;
  dc:created "2022-06-15"^^xsd:date ;
  ns1:term_status "accepted"@en ;
  skos:definition "Data volume that is considered small or limited within the context"@en ;
  skos:prefLabel "Small Data Volume"@en ;
  owl:sameAs <https://w3id.org/dpv#SmallDataVolume>, <https://w3id.org/dpv/dpv-owl#SmallDataVolume> .

<https://w3id.org/dpv/owl#hasOrganisationalMeasure>
  a owl:ObjectProperty ;
  rdfs:subPropertyOf <https://w3id.org/dpv/owl#hasTechnicalOrganisationalMeasure> ;
  ns2:rangeIncludes <https://w3id.org/dpv/owl#OrganisationalMeasure> ;
  dc:contributor _:genid1 ;
  dc:created "2022-02-09"^^xsd:date ;
  ns1:term_status "accepted"@en ;
  skos:definition "Indicates use or applicability of Organisational measure"@en ;
  skos:prefLabel "has organisational measure"@en ;
  ns0:rangeIncludes <https://w3id.org/dpv/owl#OrganisationalMeasure> ;
  owl:sameAs <https://w3id.org/dpv#hasOrganisationalMeasure>, <https://w3id.org/dpv/dpv-owl#hasOrganisationalMeasure> .

odrl:and
  a owl:ObjectProperty, owl:NamedIndividual, skos:Concept ;
  rdfs:subPropertyOf odrl:operand ;
  rdfs:isDefinedBy odrl: ;
  rdfs:label "And"@en ;
  skos:definition "The relation is satisfied when all of the Constraints are satisfied."@en ;
  skos:note "This property MUST only be used for Logical Constraints, and the list of operand values MUST be Constraint instances."@en .

<https://w3id.org/dpv/owl#CannotChallengeProcess>
  a owl:Class, owl:NamedIndividual, <https://w3id.org/dpv/owl#EntityNonPermissiveInvolvement> ;
  rdfs:subClassOf <https://w3id.org/dpv/owl#EntityNonPermissiveInvolvement> ;
  dc:contributor _:genid1, _:genid25, _:genid19 ;
  dc:created "2024-05-11"^^xsd:date ;
  ns1:term_status "accepted"@en ;
  skos:definition "Involvement where entity cannot challenge the process of specified context"@en ;
  skos:prefLabel "Cannot Challenge Process"@en ;
  skos:scopeNote "Challenge refers to raising questions about validity, necessity, correctness, or other similar 'trustworthiness' attributes regarding the process or plan or implementation"@en ;
  owl:sameAs <https://w3id.org/dpv#CannotChallengeProcess>, <https://w3id.org/dpv/dpv-owl#CannotChallengeProcess> .

odrl:informedParty
  a owl:ObjectProperty, owl:NamedIndividual, skos:Concept ;
  rdfs:subPropertyOf odrl:function ;
  rdfs:isDefinedBy odrl: ;
  rdfs:label "Informed Party"@en ;
  skos:definition "The Party to be informed of all uses."@en ;
  skos:note "Maybe specified as part of the inform action."@en ;
  skos:scopeNote "Non-Normative"@en .

odrl:print
  a owl:NamedIndividual, skos:Concept, odrl:Action ;
  odrl:includedIn odrl:use ;
  rdfs:isDefinedBy odrl: ;
  rdfs:label "Print"@en ;
  skos:definition "To create a tangible and permanent rendition of an Asset."@en ;
  skos:note "For example, creating a permanent, fixed (static), and directly perceivable representation of the Asset, such as printing onto paper."@en ;
  skos:scopeNote "Non-Normative"@en .

<https://w3id.org/dpv/owl#hasService>
  a owl:ObjectProperty ;
  ns2:rangeIncludes <https://w3id.org/dpv/owl#Service> ;
  dc:contributor _:genid1 ;
  dc:created "2024-04-20"^^xsd:date ;
  ns1:term_status "accepted"@en ;
  skos:definition "Indicates associated with the specified service"@en ;
  skos:prefLabel "has service"@en ;
  ns0:rangeIncludes <https://w3id.org/dpv/owl#Service> ;
  owl:sameAs <https://w3id.org/dpv#hasService>, <https://w3id.org/dpv/dpv-owl#hasService> .

<https://w3id.org/dpv/owl#ProcessingDuration>
  a owl:Class ;
  rdfs:subClassOf <https://w3id.org/dpv/owl#Duration>, <https://w3id.org/dpv/owl#ProcessingCondition> ;
  dc:created "2023-12-10"^^xsd:date ;
  dc:modified "2024-05-11"^^xsd:date ;
  ns3:example <https://w3id.org/dpv/examples/owl#E0047> ;
  ns1:term_status "accepted"@en ;
  skos:definition "Conditions regarding duration or temporal limitation for processing"@en ;
  skos:prefLabel "Processing Duration"@en ;
  owl:sameAs <https://w3id.org/dpv#ProcessingDuration>, <https://w3id.org/dpv/dpv-owl#ProcessingDuration> .

<https://w3id.org/dpv/owl#AutomatedScoringOfIndividuals>
  a owl:Class, owl:NamedIndividual, <https://w3id.org/dpv/owl#ScoringOfIndividuals> ;
  rdfs:subClassOf <https://w3id.org/dpv/owl#ScoringOfIndividuals> ;
  dc:contributor _:genid1 ;
  dc:created "2024-04-14"^^xsd:date ;
  ns1:term_status "accepted"@en ;
  skos:definition "Processing that involves automated scoring of individuals"@en ;
  skos:prefLabel "Automated Scoring of Individuals"@en ;
  skos:scopeNote "Scoring can lead to the action being considered Decision Making if the scoring is itself a decision - see 2023-MAR-16 opinion of Advocate General on Case C 634/21. Therefore, the assessment of whether scoring was automated or not is important given the legal obligations surrounding automated decision making e.g. in GDPR"@en ;
  owl:sameAs <https://w3id.org/dpv#AutomatedScoringOfIndividuals>, <https://w3id.org/dpv/dpv-owl#AutomatedScoringOfIndividuals> .

<https://w3id.org/dpv/owl#BiometricAuthentication>
  a owl:Class, owl:NamedIndividual, <https://w3id.org/dpv/owl#TechnicalMeasure> ;
  rdfs:subClassOf <https://w3id.org/dpv/owl#AuthenticationProtocols> ;
  dc:contributor _:genid1 ;
  dc:created "2022-08-17"^^xsd:date ;
  dc:source [
    a ns0:WebPage ;
    ns0:name "ENISA Reference Incident Classification Taxonomy 2018" ;
    ns0:url "https://www.enisa.europa.eu/publications/reference-incident-classification-taxonomy/"
  ] ;
  ns1:term_status "accepted"@en ;
  skos:definition "Use of biometric data for authentication"@en ;
  skos:prefLabel "Biometric Authentication"@en ;
  owl:sameAs <https://w3id.org/dpv#BiometricAuthentication>, <https://w3id.org/dpv/dpv-owl#BiometricAuthentication> .

dc:format
  a owl:AnnotationProperty, owl:ObjectProperty ;
  skos:prefLabel "dct:format"@en ;
  skos:scopeNote "Also used for specifying the format of provided information, for example a CSV dataset"@en .

odrl:Request
  a owl:Class, owl:NamedIndividual, skos:Concept ;
  rdfs:subClassOf odrl:Policy ;
  owl:disjointWith odrl:Set, odrl:Ticket ;
  rdfs:isDefinedBy odrl: ;
  rdfs:label "Request"@en ;
  skos:definition "A Policy that proposes a Rule over an Asset from an assignee."@en ;
  skos:note "A Request Policy  MUST contain a target Asset, a Party with Assignee function, and at least one of a Permission or Prohibition rule. The Request MAY also contain the Party with Assigner function if this is known. No privileges are granted to any Party."@en ;
  skos:scopeNote "Non-Normative"@en .

cc:Distribution
  a owl:NamedIndividual, skos:Concept, odrl:Action ;
  odrl:includedIn odrl:use ;
  rdfs:isDefinedBy odrl: ;
  rdfs:label "Distribution"@en ;
  skos:definition "Distribution, public display, and publicly performance."@en ;
  skos:note "This term is defined by Creative Commons."@en ;
  skos:scopeNote "Non-Normative"@en .

<https://w3id.org/dpv/owl#HealthcareOrganisation>
  a owl:Class ;
  rdfs:subClassOf <https://w3id.org/dpv/owl#Organisation> ;
  dc:contributor _:genid25 ;
  dc:created "2024-12-01"^^xsd:date ;
  ns1:term_status "accepted"@en ;
  skos:definition "An organisation that delivers medical services, promotes health, and provides care for individuals and communities"@en ;
  skos:prefLabel "Healthcare Organisation"@en ;
  owl:sameAs <https://w3id.org/dpv#HealthcareOrganisation>, <https://w3id.org/dpv/dpv-owl#HealthcareOrganisation> .

<https://w3id.org/dpv/owl#City>
  a owl:Class ;
  rdfs:subClassOf <https://w3id.org/dpv/owl#Region> ;
  dc:contributor _:genid1 ;
  dc:created "2022-10-22"^^xsd:date ;
  ns1:term_status "accepted"@en ;
  skos:definition "A region consisting of urban population and commerce"@en ;
  skos:prefLabel "City"@en ;
  owl:sameAs <https://w3id.org/dpv#City>, <https://w3id.org/dpv/dpv-owl#City> .

cc:ShareAlike
  a owl:NamedIndividual, skos:Concept, odrl:Action ;
  odrl:includedIn odrl:use ;
  rdfs:isDefinedBy odrl: ;
  rdfs:label "Share Alike"@en ;
  skos:definition "Derivative works be licensed under the same terms or compatible terms as the original work."@en ;
  skos:note "This term is defined by Creative Commons."@en ;
  skos:scopeNote "Non-Normative"@en .

skos:note a owl:AnnotationProperty .
<https://w3id.org/dpv/owl#ConsequenceAsSideEffect>
  a owl:Class ;
  rdfs:subClassOf <https://w3id.org/dpv/owl#Consequence> ;
  dc:contributor _:genid1 ;
  dc:created "2022-03-30"^^xsd:date ;
  ns1:term_status "accepted"@en ;
  skos:definition "The consequence(s) possible or arising as a side-effect of specified context"@en ;
  skos:prefLabel "Consequence as Side-Effect"@en ;
  owl:sameAs <https://w3id.org/dpv#ConsequenceAsSideEffect>, <https://w3id.org/dpv/dpv-owl#ConsequenceAsSideEffect> .

<https://w3id.org/dpv/owl#SingularFrequency>
  a owl:Class, owl:NamedIndividual, <https://w3id.org/dpv/owl#Frequency> ;
  rdfs:subClassOf <https://w3id.org/dpv/owl#Frequency> ;
  dc:contributor _:genid1 ;
  dc:created "2022-06-15"^^xsd:date ;
  dc:modified "2020-10-05"^^xsd:date ;
  ns1:term_status "accepted"@en ;
  skos:definition "Frequency where occurrences are singular i.e. they take place only once"@en ;
  skos:prefLabel "Singular Frequency"@en ;
  owl:sameAs <https://w3id.org/dpv#SingularFrequency>, <https://w3id.org/dpv/dpv-owl#SingularFrequency> .

odrl:RightOperand
  a owl:Class, owl:NamedIndividual, skos:Concept ;
  rdfs:isDefinedBy odrl: ;
  rdfs:label "Right Operand"@en ;
  skos:definition "Right operand for constraint expression."@en ;
  skos:note "Instances of the RightOperand class are used as the rightOperand of a Constraint."@en .

<https://w3id.org/dpv/owl#CannotReverseProcessEffects>
  a owl:Class, owl:NamedIndividual, <https://w3id.org/dpv/owl#EntityNonPermissiveInvolvement> ;
  rdfs:subClassOf <https://w3id.org/dpv/owl#EntityNonPermissiveInvolvement> ;
  dc:contributor _:genid1, _:genid25, _:genid19 ;
  dc:created "2024-05-11"^^xsd:date ;
  ns1:term_status "accepted"@en ;
  skos:definition "Involvement where entity cannot reverse effects of specified context"@en ;
  skos:prefLabel "Cannot Reverse Process Effects"@en ;
  skos:scopeNote "Effects refer to consequences and impacts arising from the process or from the outputs of a process"@en ;
  owl:sameAs <https://w3id.org/dpv#CannotReverseProcessEffects>, <https://w3id.org/dpv/dpv-owl#CannotReverseProcessEffects> .

<https://w3id.org/dpv/owl#ActivityHalted>
  a owl:Class, owl:NamedIndividual, <https://w3id.org/dpv/owl#ActivityStatus> ;
  rdfs:subClassOf <https://w3id.org/dpv/owl#ActivityStatus> ;
  dc:contributor _:genid1 ;
  dc:created "2022-05-18"^^xsd:date ;
  ns1:term_status "accepted"@en ;
  skos:definition "State of an activity that was occuring in the past, and has been halted or paused or stopped"@en ;
  skos:prefLabel "Activity Halted"@en ;
  owl:sameAs <https://w3id.org/dpv#ActivityHalted>, <https://w3id.org/dpv/dpv-owl#ActivityHalted> .

<https://w3id.org/dpv/owl#PartialAutomation>
  a owl:Class, owl:NamedIndividual, <https://w3id.org/dpv/owl#AutomationLevel> ;
  rdfs:subClassOf <https://w3id.org/dpv/owl#AutomationLevel> ;
  dc:contributor _:genid1, _:genid25 ;
  dc:created "2023-12-10"^^xsd:date ;
  dc:modified "2024-04-20"^^xsd:date ;
  dc:source [
    a ns0:WebPage ;
    ns0:name "ISO/IEC 22989:2022 Artificial intelligence concepts and terminology" ;
    ns0:url "https://www.iso.org/standard/74296.html"
  ] ;
  ns1:term_status "accepted"@en ;
  skos:definition "Level of automation corresponding to Level 2 in ISO/IEC 22989:2022 where the automation is present in multiple parts of the system or in a manner that does not require the human to control/use these parts while still retaining control over the system"@en ;
  skos:prefLabel "Partial Automation"@en ;
  skos:scopeNote "Human Involvement is implied here, specifically the ability to Control operations, but also possibly for intervention, oversight, and verification"@en ;
  owl:sameAs <https://w3id.org/dpv#PartialAutomation>, <https://w3id.org/dpv/dpv-owl#PartialAutomation> .

<https://w3id.org/dpv/owl#GeneratedData>
  a owl:Class ;
  rdfs:subClassOf <https://w3id.org/dpv/owl#Data> ;
  dc:created "2023-12-10"^^xsd:date ;
  ns1:term_status "accepted"@en ;
  skos:definition "Data that is generated or brought into existence without relation to existing data i.e. it is not derived or inferred from other data"@en ;
  skos:prefLabel "Generated Data"@en ;
  owl:sameAs <https://w3id.org/dpv#GeneratedData>, <https://w3id.org/dpv/dpv-owl#GeneratedData> .

<https://w3id.org/dpv/owl#RiskLevel>
  a owl:Class ;
  dc:contributor _:genid1 ;
  dc:created "2022-07-20"^^xsd:date ;
  ns3:example <https://w3id.org/dpv/examples/owl#E0068>, <https://w3id.org/dpv/examples/owl#E0071> ;
  ns1:term_status "accepted"@en ;
  skos:definition "The magnitude of a risk expressed as an indication to aid in its management"@en ;
  skos:prefLabel "Risk Level"@en ;
  skos:scopeNote "Risk Levels can be defined as a combination of different characteristics. For example, ISO 31073:2022 defines it as a combination of consequences and their likelihood. Another example would be the Risk Matrix where Risk Level is defined as a combination of Likelihood and Severity associated with the Risk."@en ;
  owl:sameAs <https://w3id.org/dpv#RiskLevel>, <https://w3id.org/dpv/dpv-owl#RiskLevel> .

<https://w3id.org/dpv/owl#EntityActiveInvolvement>
  a owl:Class ;
  rdfs:subClassOf <https://w3id.org/dpv/owl#EntityInvolvement> ;
  dc:contributor _:genid25 ;
  dc:created "2024-05-11"^^xsd:date ;
  ns1:term_status "accepted"@en ;
  skos:definition "Involvement where entity is 'actively' involved"@en ;
  skos:prefLabel "Entity Active Involvement"@en ;
  owl:sameAs <https://w3id.org/dpv#EntityActiveInvolvement>, <https://w3id.org/dpv/dpv-owl#EntityActiveInvolvement> .

<https://w3id.org/dpv/owl#Counterterrorism>
  a owl:Class, owl:NamedIndividual, <https://w3id.org/dpv/owl#Purpose> ;
  rdfs:subClassOf <https://w3id.org/dpv/owl#PublicBenefit> ;
  dc:contributor _:genid1 ;
  dc:created "2022-04-20"^^xsd:date ;
  dc:modified "2024-04-14"^^xsd:date ;
  ns1:term_status "accepted"@en ;
  skos:definition "Purposes associated with activities that detect, prevent, mitigate, or otherwise perform activities to combat or eliminate terrorism (also referred to as anti-terrorism)"@en ;
  skos:prefLabel "Counterterrorism"@en ;
  owl:sameAs <https://w3id.org/dpv#Counterterrorism>, <https://w3id.org/dpv/dpv-owl#Counterterrorism> .

<https://w3id.org/dpv/owl#Law>
  a owl:Class ;
  rdfs:subClassOf rdfs:Class ;
  dc:contributor _:genid1 ;
  dc:created "2022-01-19"^^xsd:date ;
  ns1:term_status "accepted"@en ;
  skos:definition "A law is a set of rules created by government or authorities"@en ;
  skos:prefLabel "Law"@en ;
  owl:sameAs <https://w3id.org/dpv#Law>, <https://w3id.org/dpv/dpv-owl#Law> .

odrl:concurrentUse
  a owl:NamedIndividual, skos:Concept, odrl:Action ;
  odrl:includedIn odrl:use ;
  rdfs:isDefinedBy odrl: ;
  rdfs:label "Concurrent Use"@en ;
  skos:definition "To create multiple copies of the Asset that are being concurrently used."@en ;
  skos:scopeNote "Non-Normative"@en .

odrl:trackingParty
  a owl:ObjectProperty, owl:NamedIndividual, skos:Concept ;
  rdfs:subPropertyOf odrl:function ;
  rdfs:isDefinedBy odrl: ;
  rdfs:label "Tracking Party"@en ;
  skos:definition "The Party who is tracking usage."@en ;
  skos:note "May be specified as part of the acceptTracking action."@en ;
  skos:scopeNote "Non-Normative"@en .

<https://w3id.org/dpv/owl#serialisation-jsonld>
  a owl:NamedIndividual, ns4:ResourceDescriptor ;
  dc:format <https://www.iana.org/assignments/media-types/application/ld+json> ;
  dc:conformsTo <https://www.w3.org/TR/json-ld11/> ;
  dc:title "Data Privacy Vocabulary (DPV) - JSON-LD serialiation" ;
  ns4:hasArtifact <https://w3id.org/dpv/dpv/dpv-owl.jsonld> ;
  ns4:hasRole <http://www.w3.org/ns/dx/prof/role/vocabulary> ;
  owl:sameAs <https://w3id.org/dpv#serialisation-jsonld>, <https://w3id.org/dpv/dpv-owl#serialisation-jsonld> .

<https://w3id.org/dpv/owl#PersonnelManagement>
  a owl:Class, owl:NamedIndividual, <https://w3id.org/dpv/owl#Purpose> ;
  rdfs:subClassOf <https://w3id.org/dpv/owl#HumanResourceManagement> ;
  dc:contributor _:genid1, _:genid6 ;
  dc:created "2022-03-30"^^xsd:date ;
  dc:source [
    a ns0:WebPage ;
    ns0:name "Belgian DPA ROPA Template" ;
    ns0:url "https://www.privacycommission.be/nl/model-voor-een-register-van-de-verwerkingsactiviteiten"
  ] ;
  ns1:term_status "accepted"@en ;
  skos:definition "Purposes associated with management of personnel associated with the organisation e.g. evaluation and management of employees and intermediaries"@en ;
  skos:prefLabel "Personnel Management"@en ;
  owl:sameAs <https://w3id.org/dpv#PersonnelManagement>, <https://w3id.org/dpv/dpv-owl#PersonnelManagement> .

odrl:inheritAllowed a owl:DatatypeProperty, owl:NamedIndividual, skos:Concept .
<https://w3id.org/dpv/owl#PhysicalInterceptionProtection>
  a owl:Class, owl:NamedIndividual, <https://w3id.org/dpv/owl#PhysicalMeasure> ;
  rdfs:subClassOf <https://w3id.org/dpv/owl#PhysicalMeasure> ;
  dc:contributor _:genid1 ;
  dc:created "2024-04-14"^^xsd:date ;
  dc:source "NIST SP 800-20"@en ;
  ns1:term_status "accepted"@en ;
  skos:definition "Physical protection against interception e.g. by posting a guard"@en ;
  skos:prefLabel "Physical Interception Protection"@en ;
  owl:sameAs <https://w3id.org/dpv#PhysicalInterceptionProtection>, <https://w3id.org/dpv/dpv-owl#PhysicalInterceptionProtection> .

<https://w3id.org/dpv/owl#DataBreachImpactAssessment>
  a owl:Class, owl:NamedIndividual, <https://w3id.org/dpv/owl#OrganisationalMeasure> ;
  rdfs:subClassOf <https://w3id.org/dpv/owl#RightsImpactAssessment> ;
  dc:contributor _:genid1 ;
  dc:created "2024-04-15"^^xsd:date ;
  ns1:term_status "accepted"@en ;
  skos:definition "Impact Assessment concerning the consequences and impacts of a data breach"@en ;
  skos:prefLabel "Data Breach Impact Assessment (DBIA)"@en ;
  skos:scopeNote "Data Breach assessments can require additional non-security related assessments such as GDPR Art.34 Rights Impact Assessment"@en ;
  owl:sameAs <https://w3id.org/dpv#DataBreachImpactAssessment>, <https://w3id.org/dpv/dpv-owl#DataBreachImpactAssessment> .

<https://w3id.org/dpv/owl#NoticeStatus>
  a owl:Class ;
  rdfs:subClassOf <https://w3id.org/dpv/owl#Status> ;
  dc:contributor _:genid4, _:genid1 ;
  dc:created "2024-12-01"^^xsd:date ;
  ns3:example <https://w3id.org/dpv/examples/owl#E0073> ;
  ns1:term_status "accepted"@en ;
  skos:definition "Status associated with notice provision, use, and management"@en ;
  skos:prefLabel "Notice Status"@en ;
  owl:sameAs <https://w3id.org/dpv#NoticeStatus>, <https://w3id.org/dpv/dpv-owl#NoticeStatus> .

odrl:#permissions
  a owl:NamedIndividual, skos:Collection ;
  skos:member odrl:Permission, odrl:permission ;
  skos:prefLabel "Permission"@en ;
  skos:scopeNote "ODRL Core Vocabulary Terms"@en .

foaf:logo a owl:AnnotationProperty .
<https://w3id.org/dpv/owl#CollectedData>
  a owl:Class ;
  rdfs:subClassOf <https://w3id.org/dpv/owl#Data> ;
  dc:created "2023-12-10"^^xsd:date ;
  ns1:term_status "accepted"@en ;
  skos:definition "Data that has been obtained by collecting it from a source"@en ;
  skos:prefLabel "Collected Data"@en ;
  owl:sameAs <https://w3id.org/dpv#CollectedData>, <https://w3id.org/dpv/dpv-owl#CollectedData> .

<https://w3id.org/dpv/owl#Format>
  a owl:Class, owl:NamedIndividual, <https://w3id.org/dpv/owl#Processing> ;
  rdfs:subClassOf <https://w3id.org/dpv/owl#Structure> ;
  dc:contributor _:genid5 ;
  dc:created "2024-04-14"^^xsd:date ;
  dc:source "DGA 12.d"@en ;
  ns1:term_status "accepted"@en ;
  skos:definition "to arrange or structure data in a specific form"@en ;
  skos:prefLabel "Format Data"@en ;
  owl:sameAs <https://w3id.org/dpv#Format>, <https://w3id.org/dpv/dpv-owl#Format> .

<https://eu-upcast.github.io/vocabulary/index-en.html#isMonitoredBy>
  a owl:ObjectProperty ;
  rdfs:domain odrl:purpose ;
  rdfs:comment "Defines the party or system in charge of monitoring compliance to the purpose."@en ;
  rdfs:label "is monitored by"@en .

odrl:Policy
  a owl:Class, owl:NamedIndividual, skos:Concept ;
  rdfs:isDefinedBy odrl: ;
  rdfs:label "Policy"@en ;
  skos:definition "A non-empty group of Permissions and/or Prohibitions."@en ;
  skos:note "A Policy may contain multiple Rules."@en .

<https://w3id.org/dpv/owl#C2BContract>
  a owl:Class, owl:NamedIndividual, <https://w3id.org/dpv/owl#LegalBasis> ;
  rdfs:subClassOf <https://w3id.org/dpv/owl#ContractByEntityType> ;
  dc:created "2024-08-27"^^xsd:date ;
  ns1:term_status "accepted"@en ;
  skos:definition "A contract between a consumer and a business where the business purchases goods or services from the consumer"@en ;
  skos:prefLabel "Consumer-to-Business Contract"@en ;
  owl:sameAs <https://w3id.org/dpv#C2BContract>, <https://w3id.org/dpv/dpv-owl#C2BContract> .

<https://w3id.org/dpv/owl#AmbulanceProvider>
  a owl:Class ;
  rdfs:subClassOf <https://w3id.org/dpv/owl#EmergencyServiceProvider> ;
  dc:contributor _:genid25 ;
  dc:created "2024-12-01"^^xsd:date ;
  ns1:term_status "accepted"@en ;
  skos:definition "An organisation that that offers transportation and medical care to patients requiring urgent medical attention"@en ;
  skos:prefLabel "Ambulance Provider"@en ;
  owl:sameAs <https://w3id.org/dpv#AmbulanceProvider>, <https://w3id.org/dpv/dpv-owl#AmbulanceProvider> .

<https://w3id.org/dpv/owl#Unintended>
  a owl:Class, owl:NamedIndividual, <https://w3id.org/dpv/owl#IntentionStatus> ;
  rdfs:subClassOf <https://w3id.org/dpv/owl#IntentionStatus> ;
  dc:contributor _:genid4, _:genid1, _:genid25, _:genid6 ;
  dc:created "2024-05-10"^^xsd:date ;
  ns1:term_status "accepted"@en ;
  skos:definition "Status indicating the specified context was unintended i.e. not intended"@en ;
  skos:prefLabel "Unintended"@en ;
  owl:sameAs <https://w3id.org/dpv#Unintended>, <https://w3id.org/dpv/dpv-owl#Unintended> .

ns0:version a owl:AnnotationProperty .
<https://w3id.org/dpv/owl#ParentOfDataSubject>
  a owl:Class, owl:NamedIndividual, <https://w3id.org/dpv/owl#HumanSubject> ;
  rdfs:subClassOf <https://w3id.org/dpv/owl#ParentOfHuman> ;
  dc:contributor _:genid4 ;
  dc:created "2022-08-03"^^xsd:date ;
  dc:modified "2024-12-17"^^xsd:date ;
  ns1:term_status "modified"@en ;
  skos:definition "Parent(s) of data subjects such as children"@en ;
  skos:prefLabel "Parent(s) of Data Subject"@en ;
  owl:sameAs <https://w3id.org/dpv#ParentOfDataSubject>, <https://w3id.org/dpv/dpv-owl#ParentOfDataSubject> .

odrl:attribute
  a owl:NamedIndividual, skos:Concept, odrl:Action ;
  odrl:includedIn odrl:use ;
  rdfs:isDefinedBy odrl: ;
  rdfs:label "Attribute"@en ;
  skos:definition "To attribute the use of the Asset."@en ;
  skos:note "May link to an Asset with the attribution information. May link to a Party with the  role “attributedParty” function."@en ;
  skos:scopeNote "Non-Normative"@en .

<https://w3id.org/dpv/owl#ExplicitlyExpressedConsent>
  a owl:Class, owl:NamedIndividual, <https://w3id.org/dpv/owl#LegalBasis> ;
  rdfs:subClassOf <https://w3id.org/dpv/owl#ExpressedConsent> ;
  dc:contributor _:genid4, _:genid1, _:genid17, _:genid6 ;
  dc:created "2022-06-21"^^xsd:date ;
  ns3:example <https://w3id.org/dpv/examples/owl#E0018> ;
  ns1:term_status "accepted"@en ;
  skos:definition "Consent that is expressed through an explicit action solely conveying a consenting decision"@en ;
  skos:prefLabel "Explicitly Expressed Consent"@en ;
  skos:scopeNote "Explicitly expressed consent is a more specific form of Expressed consent where the action taken must 'explicitly' relate to only the consent decision. Expressed consent where the consenting is part of other matters therefore cannot satisfy the requirements of explicitly expressed consent. An example of explicit action expressing the consenting decision is a button on a web form where the form only relates to consent, or it is accompanied with suitable text that reiterates what the consenting decision is about"@en ;
  owl:sameAs <https://w3id.org/dpv#ExplicitlyExpressedConsent>, <https://w3id.org/dpv/dpv-owl#ExplicitlyExpressedConsent> .

<https://w3id.org/dpv/owl#DataInteroperabilityManagement>
  a owl:Class, owl:NamedIndividual, <https://w3id.org/dpv/owl#OrganisationalMeasure> ;
  rdfs:subClassOf <https://w3id.org/dpv/owl#DataGovernance> ;
  dc:contributor _:genid1 ;
  dc:created "2024-04-14"^^xsd:date ;
  ns1:term_status "accepted"@en ;
  skos:definition "Measures associated with management of data interoperability"@en ;
  skos:prefLabel "Data Interoperability Management"@en ;
  owl:sameAs <https://w3id.org/dpv#DataInteroperabilityManagement>, <https://w3id.org/dpv/dpv-owl#DataInteroperabilityManagement> .

odrl:conflict
  a owl:ObjectProperty, owl:NamedIndividual, skos:Concept ;
  rdfs:domain odrl:Policy ;
  rdfs:range odrl:ConflictTerm ;
  rdfs:isDefinedBy odrl: ;
  rdfs:label "Handle Policy Conflicts"@en ;
  skos:definition "The conflict-resolution strategy for a Policy."@en ;
  skos:note "If no strategy is specified, the default is invalid."@en .

odrl:digitize
  a owl:NamedIndividual, skos:Concept, odrl:Action ;
  odrl:includedIn odrl:use ;
  rdfs:isDefinedBy odrl: ;
  rdfs:label "Digitize"@en ;
  skos:definition "To produce a digital copy of (or otherwise digitize) the Asset from its analogue form."@en ;
  skos:scopeNote "Non-Normative"@en .

<https://w3id.org/dpv/owl#hasRecipientDataController>
  a owl:ObjectProperty ;
  rdfs:subPropertyOf <https://w3id.org/dpv/owl#hasRecipient> ;
  ns2:rangeIncludes <https://w3id.org/dpv/owl#DataController> ;
  dc:contributor _:genid4, _:genid1, _:genid6 ;
  dc:created "2022-02-09"^^xsd:date ;
  ns1:term_status "accepted"@en ;
  skos:definition "Indiciates inclusion or applicability of a Data Controller as a Recipient of persona data"@en ;
  skos:prefLabel "has recipient data controller"@en ;
  ns0:rangeIncludes <https://w3id.org/dpv/owl#DataController> ;
  owl:sameAs <https://w3id.org/dpv#hasRecipientDataController>, <https://w3id.org/dpv/dpv-owl#hasRecipientDataController> .

<https://w3id.org/dpv/owl#ObservedPersonalData>
  a owl:Class ;
  rdfs:subClassOf <https://w3id.org/dpv/owl#CollectedPersonalData>, <https://w3id.org/dpv/owl#ObservedData> ;
  dc:contributor _:genid4 ;
  dc:created "2022-08-24"^^xsd:date ;
  dc:modified "2023-12-10"^^xsd:date ;
  ns1:term_status "accepted"@en ;
  skos:definition "Personal Data that has been collected through observation of the Data Subject(s)"@en ;
  skos:prefLabel "Observed Personal Data"@en ;
  owl:sameAs <https://w3id.org/dpv#ObservedPersonalData>, <https://w3id.org/dpv/dpv-owl#ObservedPersonalData> .

odrl:rightOperandReference
  a owl:AnnotationProperty, owl:NamedIndividual, skos:Concept ;
  rdfs:domain odrl:Constraint ;
  rdfs:isDefinedBy odrl: ;
  rdfs:label "Has Right Operand Reference"@en ;
  skos:definition "A reference to a web resource providing the value for the right operand of a Constraint."@en ;
  skos:note "An IRI that MUST be dereferenced to obtain the actual right operand value. When used with set-based operators, a list of IRIs may be used"@en .

<https://w3id.org/dpv/owl#ThirdPartySecurityProcedures>
  a owl:Class, owl:NamedIndividual, <https://w3id.org/dpv/owl#OrganisationalMeasure> ;
  rdfs:subClassOf <https://w3id.org/dpv/owl#SecurityProcedure> ;
  dc:contributor _:genid1 ;
  dc:created "2022-08-17"^^xsd:date ;
  dc:source [
    a ns0:WebPage ;
    ns0:name "ENISA 5G Cybersecurity Standards" ;
    ns0:url "https://www.enisa.europa.eu/publications/5g-cybersecurity-standards"
  ] ;
  ns1:term_status "accepted"@en ;
  skos:definition "Procedures related to security associated with Third Parties"@en ;
  skos:prefLabel "Third Party Security Procedures"@en ;
  owl:sameAs <https://w3id.org/dpv#ThirdPartySecurityProcedures>, <https://w3id.org/dpv/dpv-owl#ThirdPartySecurityProcedures> .

<https://w3id.org/dpv/owl#hasLegalMeasure>
  a owl:ObjectProperty ;
  rdfs:subPropertyOf <https://w3id.org/dpv/owl#hasOrganisationalMeasure> ;
  ns2:rangeIncludes <https://w3id.org/dpv/owl#LegalMeasure> ;
  dc:created "2023-12-10"^^xsd:date ;
  ns1:term_status "accepted"@en ;
  skos:definition "Indicates use or applicability of Legal measure"@en ;
  skos:prefLabel "has legal measure"@en ;
  ns0:rangeIncludes <https://w3id.org/dpv/owl#LegalMeasure> ;
  owl:sameAs <https://w3id.org/dpv#hasLegalMeasure>, <https://w3id.org/dpv/dpv-owl#hasLegalMeasure> .

odrl:percentage
  a owl:NamedIndividual, skos:Concept, odrl:LeftOperand ;
  rdfs:isDefinedBy odrl: ;
  rdfs:label "Asset Percentage"@en ;
  skos:definition "A percentage amount of the target Asset relevant for exercising the action of the Rule. Right operand value MUST be an xsd:decimal from 0 to 100."@en ;
  skos:note "Example: Extract less than or equal to 50%."@en ;
  skos:scopeNote "Non-Normative"@en .

<https://w3id.org/dpv/owl#ConditionalAutomation>
  a owl:Class, owl:NamedIndividual, <https://w3id.org/dpv/owl#AutomationLevel> ;
  rdfs:subClassOf <https://w3id.org/dpv/owl#AutomationLevel> ;
  dc:contributor _:genid1, _:genid25 ;
  dc:created "2023-12-10"^^xsd:date ;
  dc:modified "2024-04-20"^^xsd:date ;
  dc:source [
    a ns0:WebPage ;
    ns0:name "ISO/IEC 22989:2022 Artificial intelligence concepts and terminology" ;
    ns0:url "https://www.iso.org/standard/74296.html"
  ] ;
  ns1:term_status "accepted"@en ;
  skos:definition "Level of automation corresponding to Level 3 in ISO/IEC 22989:2022 where the automation is sufficient to perform most tasks of the system with the human present to take over where necessary"@en ;
  skos:prefLabel "Conditional Automation"@en ;
  skos:scopeNote "Human Involvement is implied here, e.g. for intervention, input, decisions"@en ;
  owl:sameAs <https://w3id.org/dpv#ConditionalAutomation>, <https://w3id.org/dpv/dpv-owl#ConditionalAutomation> .

<https://w3id.org/dpv/owl#TrustedComputing>
  a owl:Class, owl:NamedIndividual, <https://w3id.org/dpv/owl#TechnicalMeasure> ;
  rdfs:subClassOf <https://w3id.org/dpv/owl#CryptographicMethods> ;
  dc:contributor _:genid1 ;
  dc:created "2022-08-17"^^xsd:date ;
  dc:source [
    a ns0:WebPage ;
    ns0:name "ENISA Reference Incident Classification Taxonomy 2018" ;
    ns0:url "https://www.enisa.europa.eu/publications/reference-incident-classification-taxonomy/"
  ] ;
  ns1:term_status "accepted"@en ;
  skos:definition "Use of cryptographic methods to restrict access and execution to trusted parties and code"@en ;
  skos:prefLabel "Trusted Computing"@en ;
  owl:sameAs <https://w3id.org/dpv#TrustedComputing>, <https://w3id.org/dpv/dpv-owl#TrustedComputing> .

<https://w3id.org/dpv/guides>
  a owl:NamedIndividual, ns4:ResourceDescriptor ;
  dc:format <https://www.iana.org/assignments/media-types/text/html> ;
  dc:conformsTo <https://www.w3.org/TR/html/> ;
  dc:title "Guides for Data Privacy Vocabulary" ;
  ns4:hasArtifact <https://w3id.org/dpv/guides> ;
  ns4:hasRole <http://www.w3.org/ns/dx/prof/role/guidance> .

odrl:reproduce
  a owl:NamedIndividual, skos:Concept, odrl:Action ;
  odrl:includedIn odrl:use ;
  rdfs:isDefinedBy odrl: ;
  rdfs:label "Reproduce"@en ;
  skos:definition "To make duplicate copies the Asset in any material form."@en ;
  skos:scopeNote "Non-Normative"@en .

<https://w3id.org/dpv/owl#SecurityRoleProcedures>
  a owl:Class, owl:NamedIndividual, <https://w3id.org/dpv/owl#OrganisationalMeasure> ;
  rdfs:subClassOf <https://w3id.org/dpv/owl#SecurityProcedure> ;
  dc:contributor _:genid1 ;
  dc:created "2022-08-17"^^xsd:date ;
  dc:source [
    a ns0:WebPage ;
    ns0:name "ENISA 5G Cybersecurity Standards" ;
    ns0:url "https://www.enisa.europa.eu/publications/5g-cybersecurity-standards"
  ] ;
  ns1:term_status "accepted"@en ;
  skos:definition "Procedures related to security roles"@en ;
  skos:prefLabel "Security Role Procedures"@en ;
  owl:sameAs <https://w3id.org/dpv#SecurityRoleProcedures>, <https://w3id.org/dpv/dpv-owl#SecurityRoleProcedures> .

odrl:#actions
  a owl:NamedIndividual, skos:Collection ;
  skos:member odrl:transfer, odrl:use ;
  skos:prefLabel "Actions for Rules"@en ;
  skos:scopeNote "ODRL Core Vocabulary Terms"@en .

odrl:PartyScope a owl:Class, owl:NamedIndividual, skos:Concept .
odrl:failure
  a owl:ObjectProperty, owl:NamedIndividual, skos:Concept ;
  rdfs:domain odrl:Rule ;
  rdfs:range odrl:Rule ;
  rdfs:isDefinedBy odrl: ;
  rdfs:label "Failure"@en ;
  skos:definition "Failure is an abstract property that defines the violation (or unmet) relationship between Rules."@en ;
  skos:note "The parent property to sub-properties that express explicit failure contexts."@en .

<https://eu-upcast.github.io/vocabulary/index-en.html#hasFormat>
  a owl:ObjectProperty ;
  rdfs:subPropertyOf owl:topObjectProperty ;
  rdfs:domain odrl:Asset ;
  rdfs:label "has format" .

<https://w3id.org/dpv/owl#Adapt>
  a owl:Class, owl:NamedIndividual, <https://w3id.org/dpv/owl#Processing> ;
  rdfs:subClassOf <https://w3id.org/dpv/owl#Transform> ;
  dc:created "2019-05-07"^^xsd:date ;
  dc:source [
    a ns0:WebPage ;
    ns0:name "GDPR Art.4-2" ;
    ns0:url "https://eur-lex.europa.eu/eli/reg/2016/679/art_4/par_2/oj"
  ] ;
  ns1:term_status "accepted"@en ;
  skos:definition "to modify the data, often rewritten into a new form for a new use"@en ;
  skos:prefLabel "Adapt Data"@en ;
  owl:sameAs <https://w3id.org/dpv#Adapt>, <https://w3id.org/dpv/dpv-owl#Adapt> .

<https://w3id.org/dpv/owl#hasTechnicalOrganisationalMeasure>
  a owl:ObjectProperty ;
  ns2:rangeIncludes <https://w3id.org/dpv/owl#TechnicalOrganisationalMeasure> ;
  dc:contributor _:genid13, _:genid9, _:genid31, _:genid1, _:genid11 ;
  dc:created "2019-04-04"^^xsd:date ;
  dc:modified "2020-11-04"^^xsd:date ;
  ns1:term_status "accepted"@en ;
  skos:definition "Indicates use or applicability of Technical or Organisational measure"@en ;
  skos:prefLabel "has technical and organisational measure"@en ;
  ns0:rangeIncludes <https://w3id.org/dpv/owl#TechnicalOrganisationalMeasure> ;
  owl:sameAs <https://w3id.org/dpv#hasTechnicalOrganisationalMeasure>, <https://w3id.org/dpv/dpv-owl#hasTechnicalOrganisationalMeasure> .

odrl:timedCount
  a owl:DatatypeProperty, owl:NamedIndividual, skos:Concept ;
  rdfs:range rdfs:Literal .

odrl:Ticket
  a owl:Class, owl:NamedIndividual, skos:Concept ;
  rdfs:subClassOf odrl:Policy ;
  rdfs:isDefinedBy odrl: ;
  rdfs:label "Ticket"@en ;
  skos:definition "A Policy that grants the holder a Rule over an Asset from an assigner."@en ;
  skos:note "A Ticket Policy MUST contain a target Asset and at least one of a Permission or Prohibition rule.  The Ticket MAY contain the Party with Assigner function and MUST NOT contain an Assignee. The Ticket Policy will grant the terms of the Policy to the holder of that Ticket. The holder of the Ticket MAY remain unknown or MAY have to be identified at some later stage."@en ;
  skos:scopeNote "Non-Normative"@en .

<https://w3id.org/dpv/owl#PasswordAuthentication>
  a owl:Class, owl:NamedIndividual, <https://w3id.org/dpv/owl#TechnicalMeasure> ;
  rdfs:subClassOf <https://w3id.org/dpv/owl#AuthenticationProtocols> ;
  dc:contributor _:genid1 ;
  dc:created "2022-08-17"^^xsd:date ;
  dc:source [
    a ns0:WebPage ;
    ns0:name "ENISA Reference Incident Classification Taxonomy 2018" ;
    ns0:url "https://www.enisa.europa.eu/publications/reference-incident-classification-taxonomy/"
  ] ;
  ns1:term_status "accepted"@en ;
  skos:definition "Use of passwords to perform authentication"@en ;
  skos:prefLabel "Password Authentication"@en ;
  owl:sameAs <https://w3id.org/dpv#PasswordAuthentication>, <https://w3id.org/dpv/dpv-owl#PasswordAuthentication> .

<https://w3id.org/dpv/owl#EmergencyHealthcareProvider>
  a owl:Class ;
  rdfs:subClassOf <https://w3id.org/dpv/owl#EmergencyServiceProvider> ;
  dc:contributor _:genid25 ;
  dc:created "2024-12-01"^^xsd:date ;
  ns1:term_status "accepted"@en ;
  skos:definition "An organisation that is an emergency service provider focused on delivering immediate medical care to patients in critical or life-threatening situations"@en ;
  skos:prefLabel "Emergency Healthcare Provider"@en ;
  owl:sameAs <https://w3id.org/dpv#EmergencyHealthcareProvider>, <https://w3id.org/dpv/dpv-owl#EmergencyHealthcareProvider> .

cc:Notice
  a owl:NamedIndividual, skos:Concept, odrl:Action ;
  odrl:includedIn odrl:use ;
  rdfs:isDefinedBy odrl: ;
  rdfs:label "Notice"@en ;
  skos:definition "Copyright and license notices be kept intact."@en ;
  skos:note "This term is defined by Creative Commons."@en ;
  skos:scopeNote "Non-Normative"@en .

odrl:derive
  a owl:NamedIndividual, skos:Concept, odrl:Action ;
  odrl:includedIn odrl:use ;
  rdfs:isDefinedBy odrl: ;
  rdfs:label "Derive"@en ;
  skos:definition "To create a new derivative Asset from this Asset and to edit or modify the derivative."@en ;
  skos:note "A new asset is created and may have significant overlaps with the original Asset. (Note that the notion of whether or not the change is significant enough to qualify as a new asset is subjective). To the derived Asset a next policy may be applied."@en ;
  skos:scopeNote "Non-Normative"@en .

<https://w3id.org/dpv/owl#InnovativeUseOfExistingTechnology>
  a owl:Class, owl:NamedIndividual, <https://w3id.org/dpv/owl#InnovativeUseOfTechnology> ;
  rdfs:subClassOf <https://w3id.org/dpv/owl#InnovativeUseOfTechnology> ;
  dc:created "2023-12-10"^^xsd:date ;
  ns1:term_status "accepted"@en ;
  skos:definition "Involvement of existing technologies used in an innovative manner"@en ;
  skos:prefLabel "Innovative Use of Existing Technologies"@en ;
  owl:sameAs <https://w3id.org/dpv#InnovativeUseOfExistingTechnology>, <https://w3id.org/dpv/dpv-owl#InnovativeUseOfExistingTechnology> .

<https://w3id.org/dpv/owl#RequestStatus>
  a owl:Class ;
  rdfs:subClassOf <https://w3id.org/dpv/owl#Status> ;
  dc:contributor _:genid1 ;
  dc:created "2022-11-30"^^xsd:date ;
  ns1:term_status "accepted"@en ;
  skos:definition "Status associated with requests"@en ;
  skos:prefLabel "Request Status"@en ;
  owl:sameAs <https://w3id.org/dpv#RequestStatus>, <https://w3id.org/dpv/dpv-owl#RequestStatus> .

odrl:media
  a owl:NamedIndividual, skos:Concept, odrl:LeftOperand ;
  rdfs:isDefinedBy odrl: ;
  rdfs:label "Media Context"@en ;
  skos:definition "Category of a media asset setting a context for exercising the action of the Rule."@en ;
  skos:note "Example media types: electronic, print, advertising, marketing. Note: The used type should not be an IANA MediaType as they are focused on technical characteristics. "@en ;
  skos:scopeNote "Non-Normative"@en .

<https://w3id.org/dpv/owl#Necessity>
  a owl:Class ;
  rdfs:subClassOf <https://w3id.org/dpv/owl#Context> ;
  dc:contributor _:genid4, _:genid5, _:genid1, _:genid17, _:genid6 ;
  dc:created "2022-02-12"^^xsd:date ;
  ns3:example <https://w3id.org/dpv/examples/owl#E0026>, <https://w3id.org/dpv/examples/owl#E0052> ;
  ns1:term_status "accepted"@en ;
  skos:definition "An indication of 'necessity' within a context"@en ;
  skos:prefLabel "Necessity"@en ;
  skos:scopeNote "Necessity can be used to express need, essentiality, requirement, or compulsion."@en ;
  owl:sameAs <https://w3id.org/dpv#Necessity>, <https://w3id.org/dpv/dpv-owl#Necessity> .

<https://w3id.org/dpv/owl#ContractTerminationStatus>
  a owl:Class ;
  rdfs:subClassOf <https://w3id.org/dpv/owl#ContractStatus> ;
  dc:contributor _:genid4, _:genid1, _:genid17 ;
  dc:created "2025-01-09"^^xsd:date ;
  ns1:term_status "accepted"@en ;
  skos:definition "Status associated with termination of a contract"@en ;
  skos:prefLabel "Contract Termination Status"@en ;
  owl:sameAs <https://w3id.org/dpv#ContractTerminationStatus>, <https://w3id.org/dpv/dpv-owl#ContractTerminationStatus> .

<https://w3id.org/dpv/owl#LegitimateInterestNotObjected>
  a owl:Class, owl:NamedIndividual, <https://w3id.org/dpv/owl#LegitimateInterestStatus> ;
  rdfs:subClassOf <https://w3id.org/dpv/owl#LegitimateInterestStatus> ;
  dc:created "2024-08-27"^^xsd:date ;
  ns1:term_status "accepted"@en ;
  skos:definition "Status where the use of Legitimate Interest was not objected to"@en ;
  skos:prefLabel "Legitimate InterestNotObjected"@en ;
  owl:sameAs <https://w3id.org/dpv#LegitimateInterestNotObjected>, <https://w3id.org/dpv/dpv-owl#LegitimateInterestNotObjected> .

<https://w3id.org/dpv/owl#SmallScaleProcessing>
  a owl:Class, owl:NamedIndividual, <https://w3id.org/dpv/owl#ProcessingScale> ;
  rdfs:subClassOf <https://w3id.org/dpv/owl#ProcessingScale> ;
  dc:contributor _:genid1 ;
  dc:created "2022-09-07"^^xsd:date ;
  ns1:term_status "accepted"@en ;
  skos:definition "Processing that takes place at small scales (as specified by some criteria)"@en ;
  skos:prefLabel "Small Scale Processing"@en ;
  owl:sameAs <https://w3id.org/dpv#SmallScaleProcessing>, <https://w3id.org/dpv/dpv-owl#SmallScaleProcessing> .

<https://w3id.org/dpv/owl#ContractByNegotiationType>
  a owl:Class, owl:NamedIndividual, <https://w3id.org/dpv/owl#LegalBasis> ;
  rdfs:subClassOf <https://w3id.org/dpv/owl#Contract> ;
  dc:created "2024-12-17"^^xsd:date ;
  ns1:term_status "accepted"@en ;
  skos:definition "A generic concept representing contracts categorised based on their use or absence of negotiation in the contract forming process"@en ;
  skos:prefLabel "Contract by Negotiation Type"@en ;
  owl:sameAs <https://w3id.org/dpv#ContractByNegotiationType>, <https://w3id.org/dpv/dpv-owl#ContractByNegotiationType> .

<https://w3id.org/dpv/owl#hasFee>
  a owl:ObjectProperty ;
  ns2:rangeIncludes <https://w3id.org/dpv/owl#FeeRequirement> ;
  dc:created "2024-08-27"^^xsd:date ;
  ns1:term_status "accepted"@en ;
  skos:definition "Indicates whether a fee is required for the specified context"@en ;
  skos:prefLabel "has fee"@en ;
  ns0:rangeIncludes <https://w3id.org/dpv/owl#FeeRequirement> ;
  owl:sameAs <https://w3id.org/dpv#hasFee>, <https://w3id.org/dpv/dpv-owl#hasFee> .

dc:contributor a owl:AnnotationProperty .
<https://w3id.org/dpv/owl#EndToEndEncryption>
  a owl:Class, owl:NamedIndividual, <https://w3id.org/dpv/owl#TechnicalMeasure> ;
  rdfs:subClassOf <https://w3id.org/dpv/owl#Encryption> ;
  dc:contributor _:genid1 ;
  dc:created "2022-08-17"^^xsd:date ;
  dc:source [
    a ns0:WebPage ;
    ns0:name "ENISA Data Protection Engineering" ;
    ns0:url "https://www.enisa.europa.eu/publications/data-protection-engineering"
  ] ;
  ns1:term_status "accepted"@en ;
  skos:definition "Encrypted communications where data is encrypted by the sender and decrypted by the intended receiver to prevent access to any third party"@en ;
  skos:prefLabel "End-to-End Encryption (E2EE)"@en ;
  owl:sameAs <https://w3id.org/dpv#EndToEndEncryption>, <https://w3id.org/dpv/dpv-owl#EndToEndEncryption> .

<https://w3id.org/dpv/owl#HumanInvolvementForOversight>
  a owl:Class, owl:NamedIndividual, <https://w3id.org/dpv/owl#HumanInvolvement> ;
  rdfs:subClassOf <https://w3id.org/dpv/owl#HumanInvolvement> ;
  dc:contributor _:genid1 ;
  dc:created "2022-09-07"^^xsd:date ;
  dc:modified "2023-12-10"^^xsd:date ;
  ns1:term_status "accepted"@en ;
  skos:definition "Human involvement for the purposes of having oversight over the specified context regarding its operations, inputs, or outputs"@en ;
  skos:prefLabel "Human Involvement for Oversight"@en ;
  skos:scopeNote "Oversight by itself does not indicate the ability to intervene or control the operations."@en ;
  owl:sameAs <https://w3id.org/dpv#HumanInvolvementForOversight>, <https://w3id.org/dpv/dpv-owl#HumanInvolvementForOversight> .

<https://w3id.org/dpv/owl#AuthorisationProtocols>
  a owl:Class, owl:NamedIndividual, <https://w3id.org/dpv/owl#TechnicalMeasure> ;
  rdfs:subClassOf <https://w3id.org/dpv/owl#TechnicalMeasure> ;
  dc:contributor _:genid1 ;
  dc:created "2022-08-17"^^xsd:date ;
  dc:source [
    a ns0:WebPage ;
    ns0:name "ENISA Reference Incident Classification Taxonomy 2018" ;
    ns0:url "https://www.enisa.europa.eu/publications/reference-incident-classification-taxonomy/"
  ] ;
  ns1:term_status "accepted"@en ;
  skos:definition "Protocols involving authorisation of roles or profiles to determine permission, rights, or privileges"@en ;
  skos:prefLabel "Authorisation Protocols"@en ;
  owl:sameAs <https://w3id.org/dpv#AuthorisationProtocols>, <https://w3id.org/dpv/dpv-owl#AuthorisationProtocols> .

<https://w3id.org/dpv/owl#StatisticallyConfidentialData>
  a owl:Class ;
  rdfs:subClassOf <https://w3id.org/dpv/owl#ConfidentialData> ;
  dc:created "2024-02-14"^^xsd:date ;
  dc:source "DGA 2(20)"@en ;
  ns1:term_status "accepted"@en ;
  skos:definition "Data protected through Statistical Confidentiality regulations and agreements"@en ;
  skos:prefLabel "Statistically Confidential Data"@en ;
  owl:sameAs <https://w3id.org/dpv#StatisticallyConfidentialData>, <https://w3id.org/dpv/dpv-owl#StatisticallyConfidentialData> .

odrl:#logicalConstraints
  a owl:NamedIndividual, skos:Collection ;
  skos:member odrl:LogicalConstraint, odrl:operand ;
  skos:prefLabel "Logical Constraint"@en ;
  skos:scopeNote "ODRL Core Vocabulary Terms"@en .

cc:DerivativeWorks
  a owl:NamedIndividual, skos:Concept, odrl:Action ;
  odrl:includedIn odrl:use ;
  rdfs:isDefinedBy odrl: ;
  rdfs:label "Derivative Works"@en ;
  skos:definition "Distribution of derivative works."@en ;
  skos:note "This term is defined by Creative Commons."@en ;
  skos:scopeNote "Non-Normative"@en .

odrl:Rule
  a owl:Class, owl:NamedIndividual, skos:Concept ;
  rdfs:isDefinedBy odrl: ;
  rdfs:label "Rule"@en ;
  skos:definition "An abstract concept that represents the common characteristics of Permissions, Prohibitions, and Duties."@en ;
  skos:note "Rule is an abstract concept."@en .

<https://w3id.org/dpv/owl#G2BContract>
  a owl:Class, owl:NamedIndividual, <https://w3id.org/dpv/owl#LegalBasis> ;
  rdfs:subClassOf <https://w3id.org/dpv/owl#ContractByEntityType> ;
  dc:created "2024-08-27"^^xsd:date ;
  ns1:term_status "accepted"@en ;
  skos:definition "A contract between a government and a business"@en ;
  skos:prefLabel "Government-to-Business Contract"@en ;
  owl:sameAs <https://w3id.org/dpv#G2BContract>, <https://w3id.org/dpv/dpv-owl#G2BContract> .

dc:modified a owl:AnnotationProperty .
skos:ConceptScheme a owl:Class .
odrl:undefined
  a owl:ObjectProperty, owl:NamedIndividual, skos:Concept ;
  rdfs:range odrl:UndefinedTerm .

<https://w3id.org/dpv/owl#hasContractStatus>
  a owl:ObjectProperty ;
  rdfs:subPropertyOf <https://w3id.org/dpv/owl#hasStatus> ;
  ns2:domainIncludes <https://w3id.org/dpv/owl#Contract> ;
  ns2:rangeIncludes <https://w3id.org/dpv/owl#ContractStatus> ;
  dc:created "2024-08-27"^^xsd:date ;
  ns3:example <https://w3id.org/dpv/examples/owl#E0077> ;
  ns1:term_status "accepted"@en ;
  skos:definition "Indicates the status of the contract"@en ;
  skos:prefLabel "has contract status"@en ;
  ns0:domainIncludes <https://w3id.org/dpv/owl#Contract> ;
  ns0:rangeIncludes <https://w3id.org/dpv/owl#ContractStatus> ;
  owl:sameAs <https://w3id.org/dpv#hasContractStatus>, <https://w3id.org/dpv/dpv-owl#hasContractStatus> .

<https://w3id.org/dpv/owl#Export>
  a owl:Class, owl:NamedIndividual, <https://w3id.org/dpv/owl#Processing> ;
  rdfs:subClassOf <https://w3id.org/dpv/owl#Disclose> ;
  dc:contributor _:genid5 ;
  dc:created "2024-04-14"^^xsd:date ;
  dc:source "DGA 2.20"@en ;
  ns1:term_status "accepted"@en ;
  skos:definition "to provide a copy of data from one system to another"@en ;
  skos:prefLabel "Export Data"@en ;
  owl:sameAs <https://w3id.org/dpv#Export>, <https://w3id.org/dpv/dpv-owl#Export> .

foaf:page
  a owl:ObjectProperty ;
  ns2:domainIncludes <https://w3id.org/dpv/owl#RightExerciseActivity> ;
  skos:prefLabel "foaf:page"@en ;
  skos:scopeNote "Also used to indicate a web page or document providing information or functionality associated with a Right Exercise"@en ;
  ns0:domainIncludes <https://w3id.org/dpv/owl#RightExerciseActivity> .

<https://w3id.org/dpv/owl#AsymmetricCryptography>
  a owl:Class, owl:NamedIndividual, <https://w3id.org/dpv/owl#TechnicalMeasure> ;
  rdfs:subClassOf <https://w3id.org/dpv/owl#CryptographicMethods> ;
  dc:contributor _:genid1 ;
  dc:created "2022-08-17"^^xsd:date ;
  dc:source [
    a ns0:WebPage ;
    ns0:name "ENISA Reference Incident Classification Taxonomy 2018" ;
    ns0:url "https://www.enisa.europa.eu/publications/reference-incident-classification-taxonomy/"
  ] ;
  ns1:term_status "accepted"@en ;
  skos:definition "Use of public-key cryptography or asymmetric cryptography involving a public and private pair of keys"@en ;
  skos:prefLabel "Asymmetric Cryptography"@en ;
  owl:sameAs <https://w3id.org/dpv#AsymmetricCryptography>, <https://w3id.org/dpv/dpv-owl#AsymmetricCryptography> .

<https://w3id.org/dpv/owl#RightsFulfillment>
  a owl:Class, owl:NamedIndividual, <https://w3id.org/dpv/owl#Purpose> ;
  rdfs:subClassOf <https://w3id.org/dpv/owl#LegalObligation> ;
  dc:contributor _:genid4, _:genid5, _:genid1 ;
  dc:created "2024-02-14"^^xsd:date ;
  ns1:term_status "accepted"@en ;
  skos:definition "Purposes associated with the fulfillment of rights specified in law"@en ;
  skos:prefLabel "Rights Fulfillment"@en ;
  skos:scopeNote "Where Rights Fulfillment includes activities that are not legal obligations, for example conducting Identity Verification, the documentation should indicate this by expressing them as separate purposes within the same activity"@en ;
  owl:sameAs <https://w3id.org/dpv#RightsFulfillment>, <https://w3id.org/dpv/dpv-owl#RightsFulfillment> .

<https://w3id.org/dpv/owl#PaymentManagement>
  a owl:Class, owl:NamedIndividual, <https://w3id.org/dpv/owl#Purpose> ;
  rdfs:subClassOf <https://w3id.org/dpv/owl#ServiceProvision> ;
  dc:contributor _:genid4, _:genid5, _:genid1 ;
  dc:created "2020-11-04"^^xsd:date ;
  ns1:term_status "accepted"@en ;
  skos:definition "Purposes associated with processing and managing payment in relation to service, including invoicing and records"@en ;
  skos:prefLabel "Payment Management"@en ;
  owl:sameAs <https://w3id.org/dpv#PaymentManagement>, <https://w3id.org/dpv/dpv-owl#PaymentManagement> .

<https://w3id.org/dpv/owl#CannotOptOutFromProcess>
  a owl:Class, owl:NamedIndividual, <https://w3id.org/dpv/owl#EntityNonPermissiveInvolvement> ;
  rdfs:subClassOf <https://w3id.org/dpv/owl#EntityNonPermissiveInvolvement> ;
  dc:contributor _:genid1, _:genid25, _:genid19 ;
  dc:created "2024-05-11"^^xsd:date ;
  ns1:term_status "accepted"@en ;
  skos:definition "Involvement where entity cannot opt-out from specified context"@en ;
  skos:prefLabel "Cannot Opt-out from Process"@en ;
  owl:sameAs <https://w3id.org/dpv#CannotOptOutFromProcess>, <https://w3id.org/dpv/dpv-owl#CannotOptOutFromProcess> .

odrl:gt
  a owl:NamedIndividual, skos:Concept, odrl:Operator ;
  rdfs:isDefinedBy odrl: ;
  rdfs:label "Greater than"@en ;
  skos:definition "Indicating that a given value is greater than the right operand of the Constraint."@en .

<https://w3id.org/dpv/owl#HumanInvolvementForControl>
  a owl:Class, owl:NamedIndividual, <https://w3id.org/dpv/owl#HumanInvolvement> ;
  rdfs:subClassOf <https://w3id.org/dpv/owl#HumanInvolvement> ;
  dc:created "2022-09-04"^^xsd:date ;
  dc:modified "2023-12-10"^^xsd:date ;
  ns1:term_status "accepted"@en ;
  skos:definition "Human involvement for the purposes of exercising control over the specified operations in context"@en ;
  skos:prefLabel "Human Involvement for control"@en ;
  skos:scopeNote "Control is a broad term that can be applied to various stages and operations. It maps to None, Assistive, and Partial automation models."@en ;
  owl:sameAs <https://w3id.org/dpv#HumanInvolvementForControl>, <https://w3id.org/dpv/dpv-owl#HumanInvolvementForControl> .

<https://w3id.org/dpv/owl#ContractPartiallyFulfiled>
  a owl:Class, owl:NamedIndividual, <https://w3id.org/dpv/owl#ContractFulfilmentStatus> ;
  rdfs:subClassOf <https://w3id.org/dpv/owl#ContractFulfilmentStatus> ;
  dc:contributor _:genid4, _:genid1, _:genid17 ;
  dc:created "2025-01-09"^^xsd:date ;
  ns1:term_status "accepted"@en ;
  skos:definition "Status representing contract where some of its terms have been fulfiled, and others are yet to be fulfiled in a manner that does not constitute a violation or breach of the contract i.e. there is still time and opportunity to complete the terms"@en ;
  skos:prefLabel "Contract Partially Fulfiled"@en ;
  owl:sameAs <https://w3id.org/dpv#ContractPartiallyFulfiled>, <https://w3id.org/dpv/dpv-owl#ContractPartiallyFulfiled> .

<https://w3id.org/dpv/owl#IdentityManagementMethod>
  a owl:Class, owl:NamedIndividual, <https://w3id.org/dpv/owl#OrganisationalMeasure> ;
  rdfs:subClassOf <https://w3id.org/dpv/owl#AuthorisationProcedure> ;
  dc:contributor _:genid1 ;
  dc:created "2022-08-17"^^xsd:date ;
  dc:source [
    a ns0:WebPage ;
    ns0:name "ENISA Reference Incident Classification Taxonomy 2018" ;
    ns0:url "https://www.enisa.europa.eu/publications/reference-incident-classification-taxonomy/"
  ] ;
  ns1:term_status "accepted"@en ;
  skos:definition "Management of identity and identity-based processes"@en ;
  skos:prefLabel "Identity Management Method"@en ;
  owl:sameAs <https://w3id.org/dpv#IdentityManagementMethod>, <https://w3id.org/dpv/dpv-owl#IdentityManagementMethod> .

<https://w3id.org/dpv/owl#hasSubsidiary>
  a owl:ObjectProperty ;
  rdfs:subPropertyOf <https://w3id.org/dpv/owl#hasEntity> ;
  ns2:domainIncludes <https://w3id.org/dpv/owl#Organisation> ;
  ns2:rangeIncludes <https://w3id.org/dpv/owl#Organisation> ;
  dc:contributor _:genid4, _:genid1 ;
  dc:created "2024-04-14"^^xsd:date ;
  ns3:example <https://w3id.org/dpv/examples/owl#E0038> ;
  ns1:term_status "accepted"@en ;
  skos:definition "Indicates this entity has the specified entity as its subsidiary"@en ;
  skos:prefLabel "has subsidiary"@en ;
  ns0:domainIncludes <https://w3id.org/dpv/owl#Organisation> ;
  ns0:rangeIncludes <https://w3id.org/dpv/owl#Organisation> ;
  owl:sameAs <https://w3id.org/dpv#hasSubsidiary>, <https://w3id.org/dpv/dpv-owl#hasSubsidiary> .

<https://w3id.org/dpv/owl#Clinic>
  a owl:Class ;
  rdfs:subClassOf <https://w3id.org/dpv/owl#Organisation> ;
  dc:contributor _:genid25 ;
  dc:created "2024-12-01"^^xsd:date ;
  ns1:term_status "accepted"@en ;
  skos:definition "An organisation that is a smaller healthcare facility offering outpatient medical services for diagnosis and treatment"@en ;
  skos:prefLabel "Clinic"@en ;
  owl:sameAs <https://w3id.org/dpv#Clinic>, <https://w3id.org/dpv/dpv-owl#Clinic> .

<https://w3id.org/dpv/owl#G2GContract>
  a owl:Class, owl:NamedIndividual, <https://w3id.org/dpv/owl#LegalBasis> ;
  rdfs:subClassOf <https://w3id.org/dpv/owl#ContractByEntityType> ;
  dc:created "2024-08-27"^^xsd:date ;
  ns1:term_status "accepted"@en ;
  skos:definition "A contract between two governments or government departments or units"@en ;
  skos:prefLabel "Government-to-Government Contract"@en ;
  owl:sameAs <https://w3id.org/dpv#G2GContract>, <https://w3id.org/dpv/dpv-owl#G2GContract> .

dc:license a owl:AnnotationProperty .
<https://w3id.org/dpv/owl#EntityPassiveInvolvement>
  a owl:Class ;
  rdfs:subClassOf <https://w3id.org/dpv/owl#EntityInvolvement> ;
  dc:contributor _:genid25 ;
  dc:created "2024-05-11"^^xsd:date ;
  ns1:term_status "accepted"@en ;
  skos:definition "Involvement where entity is 'passively' or 'not actively' involved"@en ;
  skos:prefLabel "Entity Passive Involvement"@en ;
  owl:sameAs <https://w3id.org/dpv#EntityPassiveInvolvement>, <https://w3id.org/dpv/dpv-owl#EntityPassiveInvolvement> .

<https://w3id.org/dpv/owl#LegalEntity>
  a owl:Class ;
  rdfs:subClassOf <https://w3id.org/dpv/owl#Entity> ;
  dc:contributor _:genid1 ;
  dc:created "2019-04-05"^^xsd:date ;
  ns1:term_status "accepted"@en ;
  skos:definition "A human or non-human 'thing' that constitutes as an entity and which is recognised and defined in law"@en ;
  skos:prefLabel "Legal Entity"@en ;
  owl:sameAs <https://w3id.org/dpv#LegalEntity>, <https://w3id.org/dpv/dpv-owl#LegalEntity> .

ns3:example a owl:AnnotationProperty .
odrl:UndefinedTerm a owl:Class, owl:NamedIndividual, skos:Concept .
<https://www.iana.org/assignments/media-types/application/ld+json> a owl:NamedIndividual .
<https://w3id.org/dpv/owl#hasScale>
  a owl:ObjectProperty ;
  ns2:rangeIncludes <https://w3id.org/dpv/owl#Scale> ;
  dc:contributor _:genid1 ;
  dc:created "2022-06-15"^^xsd:date ;
  ns1:term_status "accepted"@en ;
  skos:definition "Indicates the scale of specified concept"@en ;
  skos:prefLabel "has scale"@en ;
  ns0:rangeIncludes <https://w3id.org/dpv/owl#Scale> ;
  owl:sameAs <https://w3id.org/dpv#hasScale>, <https://w3id.org/dpv/dpv-owl#hasScale> .

<https://www.iana.org/assignments/media-types/text/html> a owl:NamedIndividual .
dc:bibliographicCitation a owl:AnnotationProperty .
<https://w3id.org/dpv/owl#hasContractControl>
  a owl:ObjectProperty ;
  ns2:domainIncludes <https://w3id.org/dpv/owl#Contract> ;
  ns2:rangeIncludes <https://w3id.org/dpv/owl#ContractControl> ;
  dc:created "2024-08-27"^^xsd:date ;
  ns1:term_status "accepted"@en ;
  skos:definition "Indicates the contract to be used with a contract"@en ;
  skos:prefLabel "has contract control"@en ;
  ns0:domainIncludes <https://w3id.org/dpv/owl#Contract> ;
  ns0:rangeIncludes <https://w3id.org/dpv/owl#ContractControl> ;
  owl:sameAs <https://w3id.org/dpv#hasContractControl>, <https://w3id.org/dpv/dpv-owl#hasContractControl> .

vcard:Individual a owl:Class .
<https://w3id.org/dpv/owl#hasPolicy>
  a owl:ObjectProperty ;
  rdfs:subPropertyOf <https://w3id.org/dpv/owl#hasTechnicalOrganisationalMeasure> ;
  ns2:rangeIncludes <https://w3id.org/dpv/owl#Policy> ;
  dc:contributor _:genid1 ;
  dc:created "2022-01-26"^^xsd:date ;
  ns1:term_status "accepted"@en ;
  skos:definition "Indicates policy applicable or used"@en ;
  skos:prefLabel "has policy"@en ;
  ns0:rangeIncludes <https://w3id.org/dpv/owl#Policy> ;
  owl:sameAs <https://w3id.org/dpv#hasPolicy>, <https://w3id.org/dpv/dpv-owl#hasPolicy> .

skos:exactMatch a owl:AnnotationProperty .
<https://w3id.org/dpv/owl#RequestRejected>
  a owl:Class, owl:NamedIndividual, <https://w3id.org/dpv/owl#RequestStatus> ;
  rdfs:subClassOf <https://w3id.org/dpv/owl#RequestStatus> ;
  dc:contributor _:genid1 ;
  dc:created "2022-11-30"^^xsd:date ;
  ns1:term_status "accepted"@en ;
  skos:definition "State of a request being rejected towards non-fulfilment"@en ;
  skos:prefLabel "Request Rejected"@en ;
  owl:sameAs <https://w3id.org/dpv#RequestRejected>, <https://w3id.org/dpv/dpv-owl#RequestRejected> .

<https://w3id.org/dpv/owl#RepairImpairments>
  a owl:Class, owl:NamedIndividual, <https://w3id.org/dpv/owl#Purpose> ;
  rdfs:subClassOf <https://w3id.org/dpv/owl#ServiceProvision> ;
  dc:contributor _:genid1 ;
  dc:created "2022-08-24"^^xsd:date ;
  ns1:term_status "accepted"@en ;
  skos:definition "Purposes associated with identifying, rectifying, or otherwise undertaking activities intended to fix or repair impairments to existing functionalities"@en ;
  skos:prefLabel "Repair Impairments"@en ;
  skos:scopeNote "An example of identifying and rectifying impairments is the process of finding and fixing errors in products, commonly referred to as debugging"@en ;
  owl:sameAs <https://w3id.org/dpv#RepairImpairments>, <https://w3id.org/dpv/dpv-owl#RepairImpairments> .

<https://w3id.org/dpv/owl#Frequency>
  a owl:Class ;
  rdfs:subClassOf <https://w3id.org/dpv/owl#Context> ;
  dc:contributor _:genid1 ;
  dc:created "2022-02-16"^^xsd:date ;
  ns3:example <https://w3id.org/dpv/examples/owl#E0051> ;
  ns1:term_status "accepted"@en ;
  skos:definition "The frequency or information about periods and repetitions in terms of recurrence."@en ;
  skos:prefLabel "Frequency"@en ;
  owl:sameAs <https://w3id.org/dpv#Frequency>, <https://w3id.org/dpv/dpv-owl#Frequency> .

<https://w3id.org/dpv/owl#DataProcessor>
  a owl:Class ;
  rdfs:subClassOf <https://w3id.org/dpv/owl#Recipient> ;
  dc:contributor _:genid1 ;
  dc:created "2019-06-04"^^xsd:date ;
  dc:source [
    a ns0:WebPage ;
    ns0:name "GDPR Art.4-8" ;
    ns0:url "https://eur-lex.europa.eu/eli/reg/2016/679/art_4/par_8/oj"
  ] ;
  ns3:example <https://w3id.org/dpv/examples/owl#E0033> ;
  ns1:term_status "accepted"@en ;
  skos:definition "A ‘processor’ means a natural or legal person, public authority, agency or other body which processes data on behalf of the controller."@en ;
  skos:prefLabel "Data Processor"@en ;
  owl:sameAs <https://w3id.org/dpv#DataProcessor>, <https://w3id.org/dpv/dpv-owl#DataProcessor> .

<https://w3id.org/dpv/owl#CryptographicAuthentication>
  a owl:Class, owl:NamedIndividual, <https://w3id.org/dpv/owl#TechnicalMeasure> ;
  rdfs:subClassOf <https://w3id.org/dpv/owl#AuthenticationProtocols>, <https://w3id.org/dpv/owl#CryptographicMethods> ;
  dc:contributor _:genid1 ;
  dc:created "2022-08-17"^^xsd:date ;
  dc:source [
    a ns0:WebPage ;
    ns0:name "ENISA Reference Incident Classification Taxonomy 2018" ;
    ns0:url "https://www.enisa.europa.eu/publications/reference-incident-classification-taxonomy/"
  ] ;
  ns1:term_status "accepted"@en ;
  skos:definition "Use of cryptography for authentication"@en ;
  skos:prefLabel "Cryptographic Authentication"@en ;
  owl:sameAs <https://w3id.org/dpv#CryptographicAuthentication>, <https://w3id.org/dpv/dpv-owl#CryptographicAuthentication> .

<https://w3id.org/dpv/owl#NoticeLayer>
  a owl:Class ;
  dc:created "2024-08-17"^^xsd:date ;
  dc:source [
    a ns0:WebPage ;
    ns0:name "ICO - What methods can we use to provide privacy information?" ;
    ns0:url "https://ico.org.uk/for-organisations/uk-gdpr-guidance-and-resources/individual-rights/the-right-to-be-informed/what-methods-can-we-use-to-provide-privacy-information/"
  ] ;
  ns3:example <https://w3id.org/dpv/examples/owl#E0072> ;
  ns1:term_status "accepted"@en ;
  skos:definition "A layer within a layered notice where the layer can be used for providing specific information or controls"@en ;
  skos:prefLabel "Notice Layer"@en ;
  owl:sameAs <https://w3id.org/dpv#NoticeLayer>, <https://w3id.org/dpv/dpv-owl#NoticeLayer> .

<https://w3id.org/dpv/owl#Consequence>
  a owl:Class ;
  rdfs:subClassOf <https://w3id.org/dpv/owl#RiskConcept> ;
  dc:contributor _:genid1 ;
  dc:created "2022-01-26"^^xsd:date ;
  dc:modified "2024-08-16"^^xsd:date ;
  ns3:example <https://w3id.org/dpv/examples/owl#E0027>, <https://w3id.org/dpv/examples/owl#E0068>, <https://w3id.org/dpv/examples/owl#E0071> ;
  ns1:term_status "accepted"@en ;
  skos:definition "The consequence(s) possible or arising from specified context"@en ;
  skos:prefLabel "Consequence"@en ;
  owl:sameAs <https://w3id.org/dpv#Consequence>, <https://w3id.org/dpv/dpv-owl#Consequence> .

<https://w3id.org/dpv/owl#EmploymentContract>
  a owl:Class, owl:NamedIndividual, <https://w3id.org/dpv/owl#LegalBasis> ;
  rdfs:subClassOf <https://w3id.org/dpv/owl#ContractByDomain> ;
  dc:created "2024-08-27"^^xsd:date ;
  ns1:term_status "accepted"@en ;
  skos:definition "A contract regarding employment between an employer and an employee"@en ;
  skos:prefLabel "Employment Contract"@en ;
  owl:sameAs <https://w3id.org/dpv#EmploymentContract>, <https://w3id.org/dpv/dpv-owl#EmploymentContract> .

odrl:eq
  a owl:NamedIndividual, skos:Concept, odrl:Operator ;
  rdfs:isDefinedBy odrl: ;
  rdfs:label "Equal to"@en ;
  skos:definition "Indicating that a given value equals the right operand of the Constraint."@en .

dc:accessRights
  a owl:ObjectProperty ;
  skos:prefLabel "dct:accessRights"@en ;
  skos:scopeNote "Also used for specifying constraints on access associated with Rights Exercising (e.g. User must log in) or access to provided data (e.g. access via link)"@en .

<https://w3id.org/dpv/owl#EntityInvolvementStatus>
  a owl:Class ;
  rdfs:subClassOf <https://w3id.org/dpv/owl#EntityInvolvement>, <https://w3id.org/dpv/owl#Status> ;
  dc:contributor _:genid25 ;
  dc:created "2024-12-01"^^xsd:date ;
  ns1:term_status "accepted"@en ;
  skos:definition "Status indicating whether an entity is involved"@en ;
  skos:prefLabel "Entity Involvement Status"@en ;
  owl:sameAs <https://w3id.org/dpv#EntityInvolvementStatus>, <https://w3id.org/dpv/dpv-owl#EntityInvolvementStatus> .

dc:Agent a owl:Class .
<https://w3id.org/dpv/owl#ContractConfidentialityClause>
  a owl:Class, owl:NamedIndividual, <https://w3id.org/dpv/owl#ContractualClause> ;
  rdfs:subClassOf <https://w3id.org/dpv/owl#ContractualClause> ;
  dc:created "2024-08-27"^^xsd:date ;
  ns1:term_status "accepted"@en ;
  skos:definition "A provision requiring parties to keep certain information confidential and not disclose it to third parties"@en ;
  skos:prefLabel "Contract Confidentiality Clause"@en ;
  owl:sameAs <https://w3id.org/dpv#ContractConfidentialityClause>, <https://w3id.org/dpv/dpv-owl#ContractConfidentialityClause> .

<https://w3id.org/dpv/owl#Severity>
  a owl:Class ;
  dc:contributor _:genid1 ;
  dc:created "2022-07-21"^^xsd:date ;
  ns3:example <https://w3id.org/dpv/examples/owl#E0068> ;
  ns1:term_status "accepted"@en ;
  skos:definition "The magnitude of being unwanted or having negative effects such as harmful impacts"@en ;
  skos:prefLabel "Severity"@en ;
  skos:scopeNote "Severity can be associated with Risk, or its Consequences and Impacts"@en ;
  owl:sameAs <https://w3id.org/dpv#Severity>, <https://w3id.org/dpv/dpv-owl#Severity> .

rdfs:Label a owl:AnnotationProperty .
rdfs:Class a owl:Class .
<https://w3id.org/dpv/owl#hasPhysicalMeasure>
  a owl:ObjectProperty ;
  rdfs:subPropertyOf <https://w3id.org/dpv/owl#hasTechnicalOrganisationalMeasure> ;
  ns2:rangeIncludes <https://w3id.org/dpv/owl#PhysicalMeasure> ;
  dc:created "2023-12-10"^^xsd:date ;
  ns1:term_status "accepted"@en ;
  skos:definition "Indicates use or applicability of Physical measure"@en ;
  skos:prefLabel "has physical measure"@en ;
  ns0:rangeIncludes <https://w3id.org/dpv/owl#PhysicalMeasure> ;
  owl:sameAs <https://w3id.org/dpv#hasPhysicalMeasure>, <https://w3id.org/dpv/dpv-owl#hasPhysicalMeasure> .

xsd:anyURI a owl:Class .
skos:broader a owl:AnnotationProperty .
odrl:scope a owl:ObjectProperty, owl:NamedIndividual, skos:Concept .
ns1:term_status a owl:AnnotationProperty .
ns0:domainIncludes a owl:AnnotationProperty .
ns0:rangeIncludes a owl:AnnotationProperty .
<https://w3id.org/dpv/owl#EntityControl> owl:sameAs <https://w3id.org/dpv#EntityControl>, <https://w3id.org/dpv/dpv-owl#EntityControl> .
ns2:rangeIncludes a owl:AnnotationProperty .
<https://www.iana.org/assignments/media-types/text/turtle> a owl:NamedIndividual .
dc:creator a owl:AnnotationProperty .
dc:publisher a owl:AnnotationProperty .
ns4:hasResource a owl:AnnotationProperty .
odrl:#assetRelationsCommon
  a owl:NamedIndividual, skos:Collection ;
  skos:member odrl:output ;
  skos:prefLabel "Asset Relations"@en ;
  skos:scopeNote "ODRL Common Vocabulary Terms"@en .

dc:subject a owl:AnnotationProperty .
dc:title a owl:AnnotationProperty .
dc:identifier a owl:AnnotationProperty .
ns0:WebPage a owl:Class .
schema:Organization a owl:Class .
odrl:#prohibitions
  a owl:NamedIndividual, skos:Collection ;
  skos:member odrl:Prohibition, odrl:prohibition ;
  skos:prefLabel "Prohibition"@en ;
  skos:scopeNote "ODRL Core Vocabulary Terms"@en .

dc:source a owl:AnnotationProperty .
dc:created a owl:AnnotationProperty .
dc:valid
  a owl:ObjectProperty ;
  skos:prefLabel "dct:valid"@en ;
  skos:scopeNote "Also used for specifying the temporal validity of an activity associated with Right Exercise. For example, limits on duration for providing or accessing provided information"@en .

dc:description a owl:AnnotationProperty .
ns0:name a owl:AnnotationProperty .
schema:Action a owl:Class .
xsd:date a rdfs:Datatype .
dc:conformsTo a owl:AnnotationProperty .
ns2:domainIncludes a owl:AnnotationProperty .
foaf:Person a owl:Class .
ns3:preferredNamespacePrefix a owl:AnnotationProperty .
skos:prefLabel a owl:AnnotationProperty .
ns4:isProfileOf a owl:AnnotationProperty .
skos:definition a owl:AnnotationProperty .
ns4:hasArtifact a owl:AnnotationProperty .
dc:isVersionOf a owl:AnnotationProperty .
dc:issued a owl:AnnotationProperty .
ns3:preferredNamespaceUri a owl:AnnotationProperty .
skos:broaderTransitive a owl:AnnotationProperty .
foaf:name a owl:AnnotationProperty .
bibo:status a owl:AnnotationProperty .
rdfs:Datatype a owl:Class .
<https://www.iana.org/assignments/media-types/text/n3> a owl:NamedIndividual .
skos:Collection a owl:Class .
schema:Person a owl:Class .
_:genid19
  a dc:Agent, foaf:Person ;
  org:memberOf [
    a foaf:Organization ;
    foaf:name "Epistimis LLC"
  ] ;
  foaf:name "Steve Hickman" .

_:genid56
  a dc:Agent, foaf:Person ;
  org:memberOf [
    a foaf:Organization ;
    foaf:name "JLINC Labs"
  ] ;
  foaf:name "Iain Henderson" .

_:genid6
  a dc:Agent, foaf:Person ;
  ns5:hasORCID "0000-0003-0770-2737" ;
  org:memberOf [
    a foaf:Organization ;
    foaf:name "Uniphar PLC"
  ] ;
  foaf:name "Paul Ryan" .

_:genid21
  a dc:Agent, foaf:Person ;
  org:memberOf [
    a foaf:Organization ;
    foaf:name "Dublin City University"
  ] ;
  foaf:name "David Hickey" .

_:genid15
  a dc:Agent, foaf:Person ;
  org:memberOf [
    a foaf:Organization ;
    foaf:name "Vienna University of Technology"
  ] ;
  foaf:name "Fajar Ekaputra" .

_:genid147
  a foaf:Organization ;
  foaf:name "Unabhängige Landeszentrum für Datenschutz Schleswig-Holstein" .

_:genid156
  a foaf:Organization ;
  foaf:name "ADAPT Centre, Trinity College Dublin" .

_:genid13
  a dc:Agent, foaf:Person ;
  org:memberOf [
    a foaf:Organization ;
    foaf:name "Vienna University of Economics and Business"
  ] ;
  foaf:name "Javier Fernández" .

_:genid66
  a dc:Agent, foaf:Person ;
  org:memberOf [
    a foaf:Organization ;
    foaf:name "Proximus"
  ] ;
  foaf:name "Rudy Jacob" .

_:genid4
  a dc:Agent, foaf:Person ;
  org:memberOf [
    a foaf:Organization ;
    foaf:name "Signatu AS"
  ] ;
  foaf:homepage "https://www.linkedin.com/in/georg-philip-krog-a2a278104/" ;
  foaf:name "Georg P. Krog" .

_:genid1
  a dc:Agent, foaf:Person ;
  ns5:hasORCID "0000-0002-5068-3714" ;
  org:memberOf [
    a foaf:Organization ;
    foaf:name "ADAPT Centre, Dublin City University"
  ] ;
  foaf:homepage "https://harshp.com/" ;
  foaf:name "Harshvardhan J. Pandit" .

_:genid9
  a dc:Agent, foaf:Person ;
  org:memberOf [
    a foaf:Organization ;
    foaf:name "OpenConsent/Kantara Initiative"
  ] ;
  foaf:name "Mark Lizar" .

_:genid225
  a foaf:Organization ;
  foaf:name "No affiliation provided" .

_:genid17
  a dc:Agent, foaf:Person ;
  ns5:hasORCID "0009-0006-4623-1463" ;
  org:memberOf [
    a foaf:Organization ;
    foaf:name "University of Koblenz"
  ] ;
  foaf:name "Julian Flake" .

_:genid244
  a foaf:Organization ;
  foaf:name "Danish Agency for Digitisation" .

_:genid5
  a dc:Agent, foaf:Person ;
  ns5:hasORCID "0000-0003-0259-7560" ;
  org:memberOf [
    a foaf:Organization ;
    foaf:name "IDLab, IMEC, Ghent University"
  ] ;
  foaf:name "Beatriz Esteves" .

_:genid261
  a foaf:Organization ;
  foaf:name "Siemens" .

_:genid10
  a dc:Agent, foaf:Person ;
  org:memberOf [
    a foaf:Organization ;
    foaf:name "University College Dublin"
  ] ;
  foaf:name "Rob Brennan" .

_:genid11
  a dc:Agent, foaf:Person ;
  org:memberOf [
    a foaf:Organization ;
    foaf:name "Vienna University of Economics and Business"
  ] ;
  foaf:name "Axel Polleres" .

_:genid267
  a foaf:Organization ;
  foaf:name "Universidad Politécnica de Madrid" .

_:genid67
  a dc:Agent, foaf:Person ;
  org:memberOf [
    a foaf:Organization ;
    foaf:name "ADAPT Centre, Trinity College Dublin"
  ] ;
  foaf:name "Arthit Suriyawongkul" .

_:genid25
  a dc:Agent, foaf:Person ;
  ns5:hasORCID "0000-0002-1208-186X" ;
  org:memberOf _:genid156 ;
  foaf:name "Delaram Golpayegani" .

_:genid64
  a dc:Agent, foaf:Person ;
  org:memberOf _:genid225 ;
  foaf:name "Damien Desfontaines" .

_:genid14
  a dc:Agent, foaf:Person ;
  org:memberOf _:genid261 ;
  foaf:name "Simon Steyskal" .

_:genid65
  a dc:Agent, foaf:Person ;
  org:memberOf _:genid267 ;
  foaf:name "Rana Saniei" .

_:genid2
  a dc:Agent, foaf:Person ;
  org:memberOf [
    a foaf:Organization ;
    foaf:name "Università di Napoli Federico II"
  ] ;
  foaf:name "Piero Bonatti" .

_:genid68
  a dc:Agent, foaf:Person ;
  org:memberOf _:genid244 ;
  foaf:name "Maya Borges" .

_:genid31
  a dc:Agent, foaf:Person ;
  org:memberOf _:genid147 ;
  foaf:name "Bud Bruegger" .

_:genid16
  a dc:Agent, foaf:Person ;
  org:memberOf [
    a foaf:Organization ;
    foaf:name "Vienna University of Technology"
  ] ;
  foaf:name "Elmar Kiesling" .